Prefix: dul: <http://www.ontologydesignpatterns.org/ont/dul/d0.owl#>
Prefix: iptc: <http://cv.iptc.org/newscodes/mediatopic/>
Prefix: nao: <http://purl.org/news/angles/>
Prefix: nco: <http://data.open.ac.uk/ontology/newsclassification#>
Prefix: owl: <http://www.w3.org/2002/07/owl#>
Prefix: rdf: <http://www.w3.org/1999/02/22-rdf-syntax-ns#>
Prefix: rdfs: <http://www.w3.org/2000/01/rdf-schema#>
Prefix: skos: <http://www.w3.org/2004/02/skos/core#>
Prefix: swrl: <http://www.w3.org/2003/11/swrl#>
Prefix: swrla: <http://swrl.stanford.edu/ontologies/3.3/swrla.owl#>
Prefix: swrlb: <http://www.w3.org/2003/11/swrlb#>
Prefix: terms: <http://purl.org/dc/terms/>
Prefix: time: <http://www.w3.org/2006/time#>
Prefix: xml: <http://www.w3.org/XML/1998/namespace>
Prefix: xsd: <http://www.w3.org/2001/XMLSchema#>
Prefix: : <http://data.open.ac.uk/ontology/newsclassification>



Ontology: <http://data.open.ac.uk/ontology/newsclassification>
<http://data.open.ac.uk/ontology/newsclassification/1.4.2>
Import: <http://www.w3.org/2004/02/skos/core>
Import: <http://www.w3.org/2006/time#2016>

Annotations: 
    terms:title "News Classification Ontology (NCO)"@en,
    rdfs:comment "The News Classification Ontology (NCO) v1.4.2. It defines the concepts needed to discuss news coverage.  These concepts include Entities, Events, Situations, Categorical Topics, Claims and Viewpoints.

Preferred prefix is `nco: <http://data.open.ac.uk/ontology/newsclassification#>`."@en,
    rdfs:comment "We import SKOS, TimeOntology"@en,
    rdfs:label "News Classification Ontology (NCO)"@en

AnnotationProperty: rdfs:comment

    
AnnotationProperty: rdfs:label

    
AnnotationProperty: rdfs:seeAlso

    
AnnotationProperty: swrla:isRuleEnabled

    
AnnotationProperty: terms:contributor

    
AnnotationProperty: terms:created

    
AnnotationProperty: terms:creator

    
AnnotationProperty: terms:description

    
AnnotationProperty: terms:isVersionOf

    
AnnotationProperty: terms:license

    
AnnotationProperty: terms:modified

    
AnnotationProperty: terms:rights

    
AnnotationProperty: terms:title

    
AnnotationProperty: xsd:pattern

    
Datatype: rdf:PlainLiteral

    
Datatype: xsd:date

    
Datatype: xsd:duration

    
Datatype: xsd:gDay

    
Datatype: xsd:gMonth

    
Datatype: xsd:gYear

    
Datatype: xsd:gYearMonth

    
ObjectProperty: nco:characterisedBy

    Annotations: 
        rdfs:label "characterised by"@en
    
    InverseOf: 
        nco:characterises
    
    
ObjectProperty: nco:characterises

    Annotations: 
        rdfs:comment "This is the main relation linking descriptions to situations. A description provides an interpretation of a situation."@en,
        rdfs:label "characterises"@en
    
    Domain: 
        nco:Description
    
    Range: 
        nco:Situation
    
    InverseOf: 
        nco:characterisedBy
    
    
ObjectProperty: nco:claimInNewsItem

    SubPropertyOf: 
        nco:inNewsItem
    
    Domain: 
        nco:Claim
    
    Range: 
        nco:NewsItem
    
    InverseOf: 
        nco:hasClaim
    
    
ObjectProperty: nco:concernsTopic

    Annotations: 
        rdfs:comment "A claim is something that concerns a topic.  The property concernsTopic is used to express this relation",
        rdfs:label "concerns topic"@en
    
    Domain: 
        nco:Claim
    
    Range: 
        nco:Topic
    
    
ObjectProperty: nco:dependsOn

    Annotations: 
        rdfs:label "depends on"@en
    
    Characteristics: 
        Transitive
    
    Domain: 
        nco:EventOrSituation
    
    Range: 
        nco:EventOrSituation
    
    InverseOf: 
        nco:preconditionFor
    
    
ObjectProperty: nco:eventDependsOn

    Annotations: 
        rdfs:comment "range is {Event OR Situation}"@en,
        rdfs:label "event depends on"@en
    
    SubPropertyOf: 
        nco:dependsOn
    
    Domain: 
        nco:Event
    
    Range: 
        nco:EventOrSituation
    
    InverseOf: 
        nco:preconditionForEvent
    
    
ObjectProperty: nco:hasAgent

    Annotations: 
        rdfs:label "has agent"@en
    
    Domain: 
        nco:AgentComponent or nco:Claim
    
    Range: 
        nco:Agent
    
    
ObjectProperty: nco:hasAgentComponent

    Annotations: 
        rdfs:label "has agent component"@en
    
    Domain: 
        nco:Event
    
    Range: 
        nco:AgentComponent
    
    
ObjectProperty: nco:hasAgentRole

    Annotations: 
        rdfs:label "has actor role"@en
    
    Domain: 
        nco:AgentComponent
    
    Range: 
        nco:Agent
    
    
ObjectProperty: nco:hasAspect

    Annotations: 
        rdfs:comment "Connects an entity to its aspects - e.g., the financial status of an individual"@en,
        rdfs:label "has aspect"@en
    
    Domain: 
        nco:Entity
    
    Range: 
        nco:Aspect
    
    InverseOf: 
        nco:isAspectOf
    
    
ObjectProperty: nco:hasClaim

    Annotations: 
        rdfs:comment "Captures the relation between a news item and a claim expressed by an agent, which is reported in the news item in question"@en,
        rdfs:label "has claim"@en
    
    Domain: 
        nco:NewsItem
    
    Range: 
        nco:Claim
    
    InverseOf: 
        nco:claimInNewsItem
    
    
ObjectProperty: nco:hasElement

    Annotations: 
        rdfs:label "has element"@en
    
    SubPropertyChain: 
        nco:hasUnifyingFactor o nco:ufSatisfiedBy
    
    Domain: 
        nco:Collection
    
    Range: 
        owl:Thing
    
    InverseOf: 
        nco:isElementOf
    
    
ObjectProperty: nco:hasJustification

    Annotations: 
        rdfs:label "has justification"@en
    
    Domain: 
        nco:Claim
    
    Range: 
        nco:Justification
    
    InverseOf: 
        nco:isJustificationOf
    
    
ObjectProperty: nco:hasLocation

    Annotations: 
        rdfs:label "has location"@en
    
    Domain: 
        nco:Event
    
    Range: 
        nco:Location
    
    
ObjectProperty: nco:hasOmittedEvent

    Annotations: 
        rdfs:comment "captures the relation between an OmissionEvent and the event that has not been carried out - e.g., a soldier's failure to carry out an order"@en,
        rdfs:label "has omitted event"@en
    
    Domain: 
        nco:OmissionEvent
    
    Range: 
        nco:Event
    
    InverseOf: 
        nco:isOmittedEventOf
    
    
ObjectProperty: nco:hasPrediction

    Annotations: 
        rdfs:comment "captures the relation between a PredictionEvent and the event that has been predicted - forecasting an eruption"@en
    
    Domain: 
        nco:PredictionEvent
    
    Range: 
        nco:EventOrSituation
    
    
ObjectProperty: nco:hasSubEvent

    Annotations: 
        rdfs:label "has subevent"@en
    
    SubPropertyOf: 
        nco:preconditionForEvent
    
    Characteristics: 
        Transitive
    
    Domain: 
        nco:Event
    
    Range: 
        nco:Event
    
    InverseOf: 
        nco:subEventOf
    
    
ObjectProperty: nco:hasSubTopic

    Annotations: 
        rdfs:comment "This property captures hierarchical relations between topics – e.g., as expressed in the IPTC NewsCodes taxonomy"@en,
        rdfs:label "has subtopic"@en
    
    SubPropertyOf: 
        skos:narrowerTransitive
    
    Characteristics: 
        Transitive
    
    Domain: 
        nco:Topic
    
    Range: 
        nco:Topic
    
    InverseOf: 
        nco:subTopicOf
    
    
ObjectProperty: nco:hasTime

    Annotations: 
        rdfs:label "has time"@en
    
    SubPropertyOf: 
        time:hasTime
    
    SubPropertyChain: 
        nco:isOmittedEventOf o nco:hasTime
    
    Domain: 
        nco:EventOrSituation
    
    Range: 
        time:TemporalEntity
    
    InverseOf: 
        nco:isTimeOf
    
    
ObjectProperty: nco:hasTopic

    Annotations: 
        rdfs:comment "captures the relation between a news item and a topic, which is the focus of the news item in question"@en
    
    SubPropertyChain: 
        nco:hasTopic o nco:subTopicOf
    
    SubPropertyChain: 
        nco:hasTopic o nco:topicRoleOf o nco:isAspectOf o nco:topicRole
    
    SubPropertyChain: 
        nco:hasTopic o nco:topicRoleOf o nco:isClaimOf o nco:topicRole
    
    SubPropertyChain: 
        nco:hasTopic o nco:topicRoleOf o nco:object o nco:topicRole
    
    SubPropertyChain: 
        nco:hasTopic o nco:topicRoleOf o nco:predicate o nco:topicRole
    
    SubPropertyChain: 
        nco:hasTopic o nco:topicRoleOf o nco:subject o nco:topicRole
    
    Domain: 
        nco:NewsItem
    
    Range: 
        nco:Topic
    
    InverseOf: 
        nco:topicInNewsItem
    
    
ObjectProperty: nco:hasUnifyingFactor

    Annotations: 
        rdfs:comment "Relates a collection to the associated unifying factor"@en,
        rdfs:label "has unifying factor"@en
    
    Domain: 
        nco:Collection
    
    Range: 
        nco:UnifyingFactor
    
    InverseOf: 
        nco:isUnifyingFactorOf
    
    
ObjectProperty: nco:hasViewpoint

    Annotations: 
        rdfs:comment "Relates a news item to a viewpoint, say ?v, expressed in the news item in question. Normally this relation is not asserted but inferred on the basis of a claim, say ?c, appearing in the news item, where ?c is an element of ?v"@en
    
    SubPropertyChain: 
        nco:hasClaim o nco:isClaimOf
    
    Domain: 
        nco:NewsItem
    
    Range: 
        nco:Viewpoint
    
    InverseOf: 
        nco:viewpointInNewsItem
    
    
ObjectProperty: nco:inNewsItem

    Annotations: 
        rdfs:label "in news item"@en
    
    
ObjectProperty: nco:includesClaim

    Annotations: 
        rdfs:comment "A specialization of hasElement that is used to relate a claim to the viewpoint that includes it"@en
    
    SubPropertyOf: 
        nco:hasElement
    
    Domain: 
        nco:Viewpoint
    
    Range: 
        nco:Claim
    
    InverseOf: 
        nco:isClaimOf
    
    
ObjectProperty: nco:isAspectOf

    Annotations: 
        rdfs:label "is aspect of"@en
    
    Domain: 
        nco:Aspect
    
    Range: 
        owl:Thing
    
    InverseOf: 
        nco:hasAspect
    
    
ObjectProperty: nco:isClaimOf

    Annotations: 
        rdfs:label "is claim of"@en
    
    SubPropertyOf: 
        nco:isElementOf
    
    InverseOf: 
        nco:includesClaim
    
    
ObjectProperty: nco:isElementOf

    Annotations: 
        rdfs:label "is element of"@en
    
    Domain: 
        owl:Thing
    
    Range: 
        nco:Collection
    
    InverseOf: 
        nco:hasElement
    
    
ObjectProperty: nco:isJustificationOf

    InverseOf: 
        nco:hasJustification
    
    
ObjectProperty: nco:isOmittedEventOf

    InverseOf: 
        nco:hasOmittedEvent
    
    
ObjectProperty: nco:isTimeOf

    InverseOf: 
        nco:hasTime
    
    
ObjectProperty: nco:isUnifyingFactorOf

    Annotations: 
        rdfs:label "is unifying factor of"@en
    
    InverseOf: 
        nco:hasUnifyingFactor
    
    
ObjectProperty: nco:object

    Domain: 
        nco:Statement
    
    Range: 
        owl:Thing
    
    
ObjectProperty: nco:preconditionFor

    Annotations: 
        rdfs:label "precondition for"@en
    
    Characteristics: 
        Transitive
    
    Domain: 
        nco:EventOrSituation
    
    Range: 
        nco:EventOrSituation
    
    InverseOf: 
        nco:dependsOn
    
    
ObjectProperty: nco:preconditionForEvent

    Annotations: 
        rdfs:label "precondition for event"@en
    
    SubPropertyOf: 
        nco:preconditionFor
    
    Domain: 
        nco:EventOrSituation
    
    Range: 
        nco:Event
    
    InverseOf: 
        nco:eventDependsOn
    
    
ObjectProperty: nco:predicate

    Domain: 
        nco:Statement
    
    Range: 
        nco:Predicate
    
    
ObjectProperty: nco:satisfiesUf

    Annotations: 
        rdfs:comment "An element can be part of a collection if and only if it satisfies the relevant unifying factor. This relation captures the relation between the element in a collection and the relevant unifying factor.  In general, we expect instances of class Collection to specify this relation in domain-dependent ways"@en,
        rdfs:label "satisfies"@en
    
    SubPropertyChain: 
        nco:isElementOf o nco:hasUnifyingFactor
    
    Domain: 
        nco:isElementOf some nco:Collection
    
    Range: 
        nco:UnifyingFactor
    
    InverseOf: 
        nco:ufSatisfiedBy
    
    
ObjectProperty: nco:subEventOf

    Annotations: 
        rdfs:comment "Captures hierarchical relations between events - e.g., the event \"verdict\" in a trial is a subEventOf of a broader \"trial\" event"@en,
        rdfs:label "is subevent of"@en
    
    SubPropertyOf: 
        nco:eventDependsOn
    
    Domain: 
        nco:Event
    
    Range: 
        nco:Event
    
    InverseOf: 
        nco:hasSubEvent
    
    
ObjectProperty: nco:subTopicOf

    Annotations: 
        rdfs:label "subtopic of"@en
    
    SubPropertyOf: 
        skos:broaderTransitive
    
    Characteristics: 
        Transitive
    
    Domain: 
        nco:Topic
    
    Range: 
        nco:Topic
    
    InverseOf: 
        nco:hasSubTopic
    
    
ObjectProperty: nco:subject

    Domain: 
        nco:Statement
    
    Range: 
        owl:Thing
    
    
ObjectProperty: nco:topicInNewsItem

    SubPropertyOf: 
        nco:inNewsItem
    
    Domain: 
        nco:Topic
    
    Range: 
        nco:NewsItem
    
    InverseOf: 
        nco:hasTopic
    
    
ObjectProperty: nco:topicRole

    Annotations: 
        rdfs:comment "It is essential to distinguish an entity, e.g., the individual J.F. Kennedy, from the associated topic, e.g., T_J.F. Kennedy.  These are two different ontological objects with very different properties. For instance, while the time span of  J.F. Kennedy the person was 1917-1963,  the time span of the associated topic continued after his death.  More in general, this relation is needed every time an individual in our knowledge base, which is not ontologically a topic (e.g., a person, an event, a statement, etc.) plays the role of a topic in the model."@en
    
    Characteristics: 
        Functional,
        InverseFunctional
    
    Domain: 
        owl:Thing
    
    Range: 
        nco:Topic
    
    InverseOf: 
        nco:topicRoleOf
    
    
ObjectProperty: nco:topicRoleOf

    Annotations: 
        rdfs:comment "A given topic role is played by one and only thing."@en,
        rdfs:label "is topic role of"@en
    
    Characteristics: 
        Functional,
        InverseFunctional
    
    Domain: 
        nco:Topic
    
    Range: 
        owl:Thing
    
    InverseOf: 
        nco:topicRole
    
    
ObjectProperty: nco:ufSatisfiedBy

    Annotations: 
        rdfs:label "satisfied by"@en
    
    InverseOf: 
        nco:satisfiesUf
    
    
ObjectProperty: nco:viewpointInNewsItem

    SubPropertyOf: 
        nco:inNewsItem
    
    Domain: 
        nco:Viewpoint
    
    Range: 
        nco:NewsItem
    
    InverseOf: 
        nco:hasViewpoint
    
    
ObjectProperty: owl:annotatedProperty

    
ObjectProperty: owl:annotatedSource

    
ObjectProperty: owl:annotatedTarget

    
ObjectProperty: skos:broaderTransitive

    
ObjectProperty: skos:narrowerTransitive

    
ObjectProperty: time:hasTime

    
ObjectProperty: time:intervalBefore

    SubPropertyChain: 
        nco:isTimeOf o nco:hasPrediction o nco:hasTime
    
    
Class: nco:Agent

    Annotations: 
        rdfs:label "Agent"@en
    
    SubClassOf: 
        nco:Entity
    
    
Class: nco:AgentComponent

    Annotations: 
        rdfs:label "Agent component"@en,
        rdfs:seeAlso "nao:AgentComponent"
    
    SubClassOf: 
        nco:hasAgent only nco:Agent,
        nco:hasAgentRole only nco:AgentRole,
        nco:hasAgentRole max 1 nco:AgentRole
    
    
Class: nco:AgentRole

    Annotations: 
        rdfs:label "Agent role"@en
    
    
Class: nco:Aspect

    Annotations: 
        rdfs:comment "The notion of entity aspect discussed here is related to the second level of agenda setting theory, which deals with the salience of the attributes of the entities that are the focus of attention in the media (McCombs et al., 2014)"@en
    
    
Class: nco:CategoricalTopic

    Annotations: 
        rdfs:comment "A Categorical Topic is a broad topic for discussion and journalistic analysis that tends to be generally relevant and newsworthy. Such topics include social, economic and political issues, such as crime, poverty, taxation, finances, economic, foreign and defence policies, immigration, party politics, and many others. Broad taxonomies for journalism, such as the IPTC Media Topic NewsCodes, tend to focus on categorical topics"@en
    
    SubClassOf: 
        nco:Topic
    
    
Class: nco:Claim

    Annotations: 
        rdfs:comment "A claim is characterised in this ontology as a reified statement"@en,
        rdfs:label "Claim"@en
    
    SubClassOf: 
        nco:Statement,
        nco:claimInNewsItem some nco:NewsItem,
        nco:concernsTopic some nco:Topic,
        nco:hasAgent some nco:Agent,
        nco:claimInNewsItem only nco:NewsItem,
        nco:concernsTopic only nco:Topic,
        nco:hasAgent only nco:Agent,
        nco:hasJustification only nco:Justification
    
    
Class: nco:Collection

    Annotations: 
        rdfs:comment "Membership of a Collection is predicated on meeting the conditions associated with the associated unifying factor (Carriero et al., 2021)."@en,
        rdfs:label "Collection"@en,
        rdfs:seeAlso "Class Collection in Dolce D0, dul:Collection"@en
    
    SubClassOf: 
        nco:hasUnifyingFactor only nco:UnifyingFactor,
        nco:hasUnifyingFactor max 1 nco:UnifyingFactor
    
    DisjointUnionOf: 
        nco:CollectionOfEvents, nco:Description, nco:Situation, nco:Viewpoint
    
    
Class: nco:CollectionOfEvents

    Annotations: 
        rdfs:label "Collection of events"@en
    
    SubClassOf: 
        nco:Collection,
        nco:hasElement only nco:Event
    
    
Class: nco:Description

    Annotations: 
        rdfs:comment "Like a Situation, a Description is also characterised as a Collection of Statements"@en,
        rdfs:label "Description"@en
    
    SubClassOf: 
        nco:Collection,
        nco:characterises only nco:Situation,
        nco:hasElement only nco:Statement,
        nco:characterises min 1 nco:Situation,
        nco:hasElement min 1 nco:Statement
    
    
Class: nco:Entity

    
Class: nco:Event

    Annotations: 
        rdfs:comment "The notion of Event in NCO is based on the one used by the News Angle Ontology (Motta et al., 2020), which is in turn based on the Simple Event Model (van Hage et al., 2011).  An event in this model is characterised in terms of time, location and the actors involved in the event.  The relation between events and actors is mediated by actor components, which specify the role played by the actor in question in the event."@en,
        rdfs:label "Event"@en,
        rdfs:seeAlso "nao:Event"
    
    SubClassOf: 
        nco:EventOrSituation,
        nco:hasAgent only nco:AgentComponent,
        nco:hasLocation only nco:Location
    
    
Class: nco:EventOrSituation

    Annotations: 
        rdfs:comment "A pragmatic class to avoid having to refer to the union of Event and Situation in several expressions"@en
    
    EquivalentTo: 
        nco:Event or nco:Situation
    
    
Class: nco:Justification

    Annotations: 
        rdfs:comment "Class Justification refers to the justification for a claim.  Because this ontology focuses on news classification rather than argumentation, the definition here is simply a placeholder and is not further elaborated"@en
    
    SubClassOf: 
        owl:Thing
    
    
Class: nco:Location

    Annotations: 
        rdfs:label "Location"@en,
        rdfs:seeAlso "dul:Location"
    
    
Class: nco:NegativeEvent

    Annotations: 
        rdfs:label "Negative event"@en
    
    SubClassOf: 
        nco:Event
    
    
Class: nco:NewsItem

    Annotations: 
        rdfs:label "News item"@en
    
    SubClassOf: 
        owl:Thing
    
    
Class: nco:OmissionEvent

    Annotations: 
        rdfs:comment "An OmissionEvent is an event capturing an expression of agency realised by not carrying out an event that was expected of the agent in question – see Payton, J.D. (2018).  How to identify negative actions with positive events.  Australasian Journal of Philosophy, 96(1), pp. 87-101.

Following Payton, we impose the constraint that the time of the omitted event is the same as the one associated with the omission event. That is, 
OmissionEvent(?ev1) ^ :hasOmittedEvent(?ev1, ?ev2) ^ :hasTime(?ev1, ?t1) -> :hasTime(?ev2, ?t1)
This is expressed by  means of a property chain specialising property :hasTime"@en,
        rdfs:label "Omission event"@en
    
    SubClassOf: 
        nco:NegativeEvent
         and (nco:hasOmittedEvent only nco:Event)
         and (nco:hasOmittedEvent exactly 1 nco:Event)
    
    
Class: nco:Predicate

    Annotations: 
        rdfs:comment "This is a metaclass whose instances play the role of a predicate in reified triples.  It is needed because OWL does not allow object properties to be used directly as values in triples unless an individual with the same name has been defined"@en
    
    
Class: nco:PredictionEvent

    Annotations: 
        rdfs:comment "We impose the constraint that the time of the predicted event has to be after that associated with the prediction event. That is:

PredictionEvent(?ev1) & hasPrediction (?ev1 ?ev_or_sit) & :hasTime (?ev1 ?t1) & :hasTime (?ev_or_sit ?t2) --> time:intervalBefore (?t1 ?t2)

This constraint is expressed through a property chain specialising time:intervalBefore"@en,
        rdfs:label "Predicted event"@en
    
    SubClassOf: 
        nco:Event,
        nco:hasPrediction only nco:EventOrSituation,
        nco:hasPrediction exactly 1 nco:EventOrSituation
    
    
Class: nco:Situation

    Annotations: 
        rdfs:comment "A Situation is a collection of statements",
        rdfs:label "Situation"@en,
        rdfs:seeAlso "dul:Situation"@en
    
    SubClassOf: 
        nco:Collection,
        nco:EventOrSituation,
        nco:characterisedBy only nco:Description,
        nco:hasElement only nco:Statement,
        nco:hasElement min 1 nco:Statement
    
    
Class: nco:Statement

    Annotations: 
        rdfs:comment "A member of this class is an individual that reifies a triple."@en,
        rdfs:label "Statement"@en
    
    
Class: nco:Topic

    Annotations: 
        rdfs:comment "A Topic provides the main focus of a news item. A Topic can be an Entity, an Event (or a Collection of Events), a Viewpoint, a Situation or a Categorical Topic"@en,
        rdfs:label "Topic"@en
    
    SubClassOf: 
        skos:Concept,
        nco:topicRoleOf some owl:Thing,
        nco:topicRoleOf exactly 1 owl:Thing
    
    
Class: nco:UnifyingFactor

    Annotations: 
        rdfs:label "Unifying factor"@en
    
    
Class: nco:Viewpoint

    Annotations: 
        rdfs:comment "As pointed out in (Baden and Springer, 2017), when analysing the news discourse, we are interested in identifying viewpoints that “open up different perspectives” and “construct different meaning”. Hence, here we define a Viewpoint as a collection of claims that subscribe to the same perspective"@en,
        rdfs:label "Viewpoint"@en
    
    SubClassOf: 
        nco:Collection,
        (nco:hasElement only nco:Claim)
         and (nco:hasElement min 1 nco:Claim)
    
    
Class: owl:Annotation

    
Class: owl:Thing

    
Class: rdf:List

    
Class: skos:Concept

    
Class: time:TemporalEntity

    
Individual: <http://www.opengis.net/def/uom/ISO-8601/0/Gregorian>

    
Individual: nco:hasTopic

    Annotations: 
        rdfs:comment "captures the relation between a news item and a topic, which is the focus of the news item in question"@en
    
    Types: 
        nco:Predicate
    
    
Individual: time:Friday

    
Individual: time:Monday

    
Individual: time:Saturday

    
Individual: time:Sunday

    
Individual: time:Thursday

    
Individual: time:Tuesday

    
Individual: time:Wednesday

    
Individual: time:unitDay

    
Individual: time:unitHour

    
Individual: time:unitMinute

    
Individual: time:unitMonth

    
Individual: time:unitSecond

    
Individual: time:unitWeek

    
Individual: time:unitYear

    
DisjointClasses: 
    nco:Agent,nco:Collection,nco:Event,nco:NewsItem,nco:Statement,nco:UnifyingFactor

