
@prefix rdf: <http://www.w3.org/1999/02/22-rdf-syntax-ns#> .
@prefix dct: <http://purl.org/dc/terms/> .
@prefix xsd: <http://www.w3.org/2001/XMLSchema#> .

@prefix altidrole:  <http://cv.iptc.org/newscodes/altidrole/> .
@prefix aoprop:  <http://cv.iptc.org/newscodes/aoproperty/> .
@prefix app:  <http://cv.iptc.org/newscodes/application/> .
@prefix aspfacet:  <http://cv.iptc.org/newscodes/asportfacet/> .
@prefix aspfacetvalue:  <http://cv.iptc.org/newscodes/asportfacetvalue/> .
@prefix acdc:  <http://cv.iptc.org/newscodes/audiocodec/> .
@prefix catinat:  <http://cv.iptc.org/newscodes/catinature/> .
@prefix chprop:  <http://cv.iptc.org/newscodes/characteristicsproperty/> .
@prefix cinat:  <http://cv.iptc.org/newscodes/cinature/> .
@prefix colsp:  <http://cv.iptc.org/newscodes/colorspace/> .
@prefix colin:  <http://cv.iptc.org/newscodes/colourindicator/> .
@prefix ctech:  <http://cv.iptc.org/newscodes/commtech/> .
@prefix cptdefrole:  <http://cv.iptc.org/newscodes/conceptdefinitionrole/> .
@prefix cptnoterole:  <http://cv.iptc.org/newscodes/conceptnoterole/> .
@prefix cpprole: <http://cv.iptc.org/newscodes/contentprodpartyrole/> .
@prefix crel:  <http://cv.iptc.org/newscodes/conceptrelation/> .
@prefix conf:  <http://cv.iptc.org/newscodes/confidence/> .
@prefix ciprol:  <http://cv.iptc.org/newscodes/contactinfopartrole/> .
@prefix cwarn:  <http://cv.iptc.org/newscodes/contentwarning/> .
@prefix ctrol:  <http://cv.iptc.org/newscodes/contributorrole/> .
@prefix cpnat:  <http://cv.iptc.org/newscodes/cpnature/> .
@prefix drol:  <http://cv.iptc.org/newscodes/descriptionrole/> .
@prefix digsrctype:  <http://cv.iptc.org/newscodes/digitalsourcetype/> .
@prefix dimensionunit:  <http://cv.iptc.org/newscodes/dimensionunit/> .
@prefix ednoterole:  <http://cv.iptc.org/newscodes/ednoterole/> .
@prefix dummy:  <http://cv.iptc.org/newscodes/dummy/> .
@prefix erol:  <http://cv.iptc.org/newscodes/edrole/> .
@prefix encd:  <http://cv.iptc.org/newscodes/encoding/> .
@prefix entityprop:  <http://cv.iptc.org/newscodes/entityproperty/> .
@prefix ecirol:  <http://cv.iptc.org/newscodes/eventcontactinforole/> .
@prefix edconf:  <http://cv.iptc.org/newscodes/eventdateconfirm/> .
@prefix eocstat:  <http://cv.iptc.org/newscodes/eventoccurstatus/> .
@prefix eorol:  <http://cv.iptc.org/newscodes/eventorganiserrole/> .
@prefix eprol:  <http://cv.iptc.org/newscodes/eventparticipantrole/> .
@prefix eregrol:  <http://cv.iptc.org/newscodes/eventregrole/> .
@prefix fisymtype:  <http://cv.iptc.org/newscodes/financialinstrumentsymboltype/> .
@prefix frmt:  <http://cv.iptc.org/newscodes/format/> .
@prefix gen:  <http://cv.iptc.org/newscodes/generic/> .
@prefix genre:  <http://cv.iptc.org/newscodes/genre/> .
@prefix hashscope:  <http://cv.iptc.org/newscodes/hashscope/> .
@prefix hashtype:  <http://cv.iptc.org/newscodes/hashtype/> .
@prefix hopaction:  <http://cv.iptc.org/newscodes/hopaction/> .
@prefix hatarget:  <http://cv.iptc.org/newscodes/hopactiontarget/> .
@prefix howextr:  <http://cv.iptc.org/newscodes/howextracted/> .
@prefix howpr:  <http://cv.iptc.org/newscodes/howpresent/> .
@prefix ikos:  <http://cv.iptc.org/newscodes/ikos/> .
@prefix impt:  <http://cv.iptc.org/newscodes/importance/> .
@prefix isrol:  <http://cv.iptc.org/newscodes/infosourcerole/> .
@prefix irel:  <http://cv.iptc.org/newscodes/itemrelation/> .
@prefix irep:  <http://cv.iptc.org/newscodes/itemrepresentation/> .
@prefix lbtyp:  <http://cv.iptc.org/newscodes/labeltype/> .
@prefix lrol:  <http://cv.iptc.org/newscodes/languagerole/> .
@prefix loutorient:  <http://cv.iptc.org/newscodes/layoutorientation/> .
@prefix loctyp:  <http://cv.iptc.org/newscodes/location/> .
@prefix medtop:  <http://cv.iptc.org/newscodes/mediatopic/> .
@prefix mtyp:  <http://cv.iptc.org/newscodes/mediatype/> .
@prefix medtype:  <http://cv.iptc.org/newscodes/mediatype1/> .
@prefix nprt:  <http://cv.iptc.org/newscodes/namepart/> .
@prefix nrol:  <http://cv.iptc.org/newscodes/namerole/> .
@prefix ncostat:  <http://cv.iptc.org/newscodes/newscoveragestatus/> .
@prefix nityp:  <http://cv.iptc.org/newscodes/newsitemtype/> .
@prefix nmsig:  <http://cv.iptc.org/newscodes/newsmsgsignal/> .
@prefix nprod:  <http://cv.iptc.org/newscodes/newsproduct/> .
@prefix nprov:  <http://cv.iptc.org/newscodes/newsprovider/> .
@prefix ninat:  <http://cv.iptc.org/newscodes/ninature/> .
@prefix not:  <http://cv.iptc.org/newscodes/notation/> .
@prefix oito:  <http://cv.iptc.org/newscodes/ofinterestto/> .
@prefix pgrmod:  <http://cv.iptc.org/newscodes/pkggroupmode/> .
@prefix plinat:  <http://cv.iptc.org/newscodes/plinature/> .
@prefix prio:  <http://cv.iptc.org/newscodes/priority/> .
@prefix prodgenre:  <http://cv.iptc.org/newscodes/productgenre/> .
@prefix prop:  <http://cv.iptc.org/newscodes/property/> .
@prefix prov:  <http://cv.iptc.org/newscodes/provider/> .
@prefix stat:  <http://cv.iptc.org/newscodes/pubstatusg2/> .
@prefix rtype:  <http://cv.iptc.org/newscodes/ratertype/> .
@prefix rcalctype:  <http://cv.iptc.org/newscodes/rcalctype/> .
@prefix rel:  <http://cv.iptc.org/newscodes/relevance/> .
@prefix rnd:  <http://cv.iptc.org/newscodes/rendition/> .
@prefix riaspect:  <http://cv.iptc.org/newscodes/riaspect/> .
@prefix rightsprop:  <http://cv.iptc.org/newscodes/rightsproperty/> .
@prefix riscope:  <http://cv.iptc.org/newscodes/riscope/> .
@prefix role1:  <http://cv.iptc.org/newscodes/role1/> .
@prefix rscaleunit:  <http://cv.iptc.org/newscodes/rscaleunit/> .
@prefix scn:  <http://cv.iptc.org/newscodes/scene/> .
@prefix sev:  <http://cv.iptc.org/newscodes/severity/> .
@prefix sig:  <http://cv.iptc.org/newscodes/signal/> .
@prefix pst1:  <http://cv.iptc.org/newscodes/status1/> .
@prefix subj:  <http://cv.iptc.org/newscodes/subjectcode/> .
@prefix squ:  <http://cv.iptc.org/newscodes/subjectqualifier/> .
@prefix timeunit:  <http://cv.iptc.org/newscodes/timeunit/> .
@prefix tone:  <http://cv.iptc.org/newscodes/tone/> .
@prefix tpctyp:  <http://cv.iptc.org/newscodes/topictype/> .
@prefix trustindicator:  <http://cv.iptc.org/newscodes/trustindicator/> .
@prefix urgy:  <http://cv.iptc.org/newscodes/urgency/> .
@prefix useracttype:  <http://cv.iptc.org/newscodes/useractiontype/> .
@prefix valfmt:  <http://cv.iptc.org/newscodes/valueformat/> .
@prefix vcdc:  <http://cv.iptc.org/newscodes/videocodec/> .
@prefix videodef:  <http://cv.iptc.org/newscodes/videodefinition/> .
@prefix ivqu:  <http://cv.iptc.org/newscodes/videoqualifier/> .
@prefix sov:  <http://cv.iptc.org/newscodes/videoscaling/> .
@prefix why:  <http://cv.iptc.org/newscodes/whypresent/> .
@prefix wldreg:  <http://cv.iptc.org/newscodes/worldregion/> .
@prefix a1312cat:  <http://cvx.iptc.org/anpa1312-category/> .
@prefix a1312prio:  <http://cvx.iptc.org/anpa1312-priority/> .
@prefix a1312svc:  <http://cvx.iptc.org/anpa1312-servicelevel/> .
@prefix a1312vers:  <http://cvx.iptc.org/anpa1312-version/> .
@prefix bcp47:  <http://cvx.iptc.org/bcp47/> .
@prefix cusip:  <http://cvx.iptc.org/cusip/> .
@prefix gics:  <http://cvx.iptc.org/gics/> .
@prefix isin:  <http://cvx.iptc.org/isin/> .
@prefix mic:  <http://cvx.iptc.org/iso10383-mic/> .
@prefix iso3166-1a2:  <http://cvx.iptc.org/iso3166-1a2/> .
@prefix iso3166-1a3:  <http://cvx.iptc.org/iso3166-1a3/> .
@prefix iso4217a:  <http://cvx.iptc.org/iso4217a/> .
@prefix iso4217n:  <http://cvx.iptc.org/iso4217n/> .
@prefix secst:  <http://cvx.iptc.org/secst/> .
@prefix sedol:  <http://cvx.iptc.org/sedol/> .
@prefix tidm:  <http://cvx.iptc.org/tidm/> .
@prefix dbpedia:  <http://dbpedia.org/resource/> .
@prefix mb-artist:  <http://musicbrainz.org/artist/> .
@prefix mb-label:  <http://musicbrainz.org/label/> .
@prefix mb-recording:  <http://musicbrainz.org/recording/> .
@prefix mb-release:  <http://musicbrainz.org/release/> .
@prefix mb-releasegroup:  <http://musicbrainz.org/release-group/> .
@prefix mb-work:  <http://musicbrainz.org/work/> .
@prefix geonames:  <http://sws.geonames.org/> .
@prefix freebase:  <http://www.freebase.com> .
@prefix skos:  <http://www.w3.org/2004/02/skos/core#> .
@prefix wikidata:  <http://www.wikidata.org/entity/> .


<http://cv.iptc.org/newscodes/mediatopic/> 
	rdf:type skos:ConceptScheme ; 
  ikos:prefSchemeAlias "medtop" ;
  ikos:authority "http://www.iptc.org" ;
  dct:rightsHolder "IPTC, International Press Telecommunications Council - https://iptc.org" ;
  ikos:licenceLink "http://creativecommons.org/licenses/by/4.0/" ;
  ikos:dateReleased "2023-10-02T12:00:00+00:00"^^xsd:dateTime ;
  dct:dateSubmitted "2023-10-02T12:00:00+00:00"^^xsd:dateTime ;
  skos:prefLabel "Media Topic"@en-GB ;
  skos:definition "Indicates a subject of an item."@en-GB ;
  skos:note "The Media Topic NewsCodes has been IPTC's primary subject taxonomy since 2010, with a focus on classification of text. The development started with our previous Subject Codes taxonomy and extended the tree to 5 levels and reused the same 17 top level terms. The terms below the top level have been revised and rearranged. Most Media Topic concepts provide a mapping back to one of the Subject Codes, and many provide a mapping to Wikidata."@en-GB ;
	skos:hasTopConcept		medtop:01000000 ;
	skos:hasTopConcept		medtop:02000000 ;
	skos:hasTopConcept		medtop:03000000 ;
	skos:hasTopConcept		medtop:04000000 ;
	skos:hasTopConcept		medtop:05000000 ;
	skos:hasTopConcept		medtop:06000000 ;
	skos:hasTopConcept		medtop:07000000 ;
	skos:hasTopConcept		medtop:08000000 ;
	skos:hasTopConcept		medtop:09000000 ;
	skos:hasTopConcept		medtop:10000000 ;
	skos:hasTopConcept		medtop:11000000 ;
	skos:hasTopConcept		medtop:12000000 ;
	skos:hasTopConcept		medtop:13000000 ;
	skos:hasTopConcept		medtop:14000000 ;
	skos:hasTopConcept		medtop:15000000 ;
	skos:hasTopConcept		medtop:16000000 ;
	skos:hasTopConcept		medtop:17000000 .

medtop:01000000
	rdf:type skos:Concept ;
	skos:prefLabel	"arts, culture, entertainment and media"@en-GB ;
	skos:definition	"All forms of arts, entertainment, cultural heritage and media"@en-GB ;
	skos:inScheme <http://cv.iptc.org/newscodes/mediatopic/>  ;
	ikos:created "2009-10-22T02:00:00+00:00"^^xsd:dateTime ;
	dct:created "2009-10-22T02:00:00+00:00"^^xsd:dateTime ;
	ikos:modified "2021-02-18T12:00:00+00:00"^^xsd:dateTime ;
	dct:modified "2021-02-18T12:00:00+00:00"^^xsd:dateTime  ;
	skos:exactMatch subj:01000000 ;
	skos:narrower	medtop:20000002 ;
	skos:narrower	medtop:20000038 ;
	skos:narrower	medtop:20000045 .

medtop:02000000
	rdf:type skos:Concept ;
	skos:prefLabel	"crime, law and justice"@en-GB ;
	skos:definition	"The establishment and/or statement of the rules of behaviour in society, the enforcement of these rules, breaches of the rules, the punishment of offenders and the organisations and bodies involved in these activities"@en-GB ;
	skos:inScheme <http://cv.iptc.org/newscodes/mediatopic/>  ;
	ikos:created "2009-10-22T02:00:00+00:00"^^xsd:dateTime ;
	dct:created "2009-10-22T02:00:00+00:00"^^xsd:dateTime ;
	ikos:modified "2021-05-05T12:00:00+00:00"^^xsd:dateTime ;
	dct:modified "2021-05-05T12:00:00+00:00"^^xsd:dateTime  ;
	skos:exactMatch subj:02000000 ;
	skos:exactMatch <https://www.wikidata.org/entity/Q146491> ;
	skos:narrower	medtop:20000082 ;
	skos:narrower	medtop:20000106 ;
	skos:narrower	medtop:20000119 ;
	skos:narrower	medtop:20000121 ;
	skos:narrower	medtop:20000129 .

medtop:03000000
	rdf:type skos:Concept ;
	skos:prefLabel	"disaster, accident and emergency incident"@en-GB ;
	skos:definition	"Man made or natural event resulting in loss of life or injury to living creatures and/or damage to inanimate objects or property"@en-GB ;
	skos:inScheme <http://cv.iptc.org/newscodes/mediatopic/>  ;
	ikos:created "2009-10-22T02:00:00+00:00"^^xsd:dateTime ;
	dct:created "2009-10-22T02:00:00+00:00"^^xsd:dateTime ;
	ikos:modified "2021-05-05T12:00:00+00:00"^^xsd:dateTime ;
	dct:modified "2021-05-05T12:00:00+00:00"^^xsd:dateTime  ;
	skos:exactMatch subj:03000000 ;
	skos:exactMatch <https://www.wikidata.org/entity/Q18669875> ;
	skos:narrower	medtop:20000139 ;
	skos:narrower	medtop:20000148 ;
	skos:narrower	medtop:20000160 ;
	skos:narrower	medtop:20000167 ;
	skos:narrower	medtop:20000168 .

medtop:04000000
	rdf:type skos:Concept ;
	skos:prefLabel	"economy, business and finance"@en-GB ;
	skos:definition	"All matters concerning the planning, production and exchange of wealth."@en-GB ;
	skos:inScheme <http://cv.iptc.org/newscodes/mediatopic/>  ;
	ikos:created "2009-10-22T02:00:00+00:00"^^xsd:dateTime ;
	dct:created "2009-10-22T02:00:00+00:00"^^xsd:dateTime ;
	ikos:modified "2021-07-12T12:00:00+00:00"^^xsd:dateTime ;
	dct:modified "2021-07-12T12:00:00+00:00"^^xsd:dateTime  ;
	skos:exactMatch subj:04000000 ;
	skos:narrower	medtop:20000170 ;
	skos:narrower	medtop:20000209 ;
	skos:narrower	medtop:20000344 ;
	skos:narrower	medtop:20000385 .

medtop:05000000
	rdf:type skos:Concept ;
	skos:prefLabel	"education"@en-GB ;
	skos:definition	"All aspects of furthering knowledge, formally or informally"@en-GB ;
	skos:inScheme <http://cv.iptc.org/newscodes/mediatopic/>  ;
	ikos:created "2009-10-22T02:00:00+00:00"^^xsd:dateTime ;
	dct:created "2009-10-22T02:00:00+00:00"^^xsd:dateTime ;
	ikos:modified "2021-09-30T12:00:00+00:00"^^xsd:dateTime ;
	dct:modified "2021-09-30T12:00:00+00:00"^^xsd:dateTime  ;
	skos:exactMatch <https://www.wikidata.org/entity/Q8434> ;
	skos:exactMatch subj:05000000 ;
	skos:narrower	medtop:20000398 ;
	skos:narrower	medtop:20000399 ;
	skos:narrower	medtop:20000400 ;
	skos:narrower	medtop:20000410 ;
	skos:narrower	medtop:20000411 ;
	skos:narrower	medtop:20000412 ;
	skos:narrower	medtop:20000413 ;
	skos:narrower	medtop:20000414 ;
	skos:narrower	medtop:20000415 ;
	skos:narrower	medtop:20000416 ;
	skos:narrower	medtop:20001216 ;
	skos:narrower	medtop:20001217 ;
	skos:narrower	medtop:20001337 .

medtop:06000000
	rdf:type skos:Concept ;
	skos:prefLabel	"environment"@en-GB ;
	skos:definition	"All aspects of protection, damage, and condition of the ecosystem of the planet earth and its surroundings."@en-GB ;
	skos:inScheme <http://cv.iptc.org/newscodes/mediatopic/>  ;
	ikos:created "2009-10-22T02:00:00+00:00"^^xsd:dateTime ;
	dct:created "2009-10-22T02:00:00+00:00"^^xsd:dateTime ;
	ikos:modified "2021-02-18T12:00:00+00:00"^^xsd:dateTime ;
	dct:modified "2021-02-18T12:00:00+00:00"^^xsd:dateTime  ;
	skos:exactMatch subj:06000000 ;
	skos:exactMatch <https://www.wikidata.org/entity/Q43619> ;
	skos:narrower	medtop:20000418 ;
	skos:narrower	medtop:20000420 ;
	skos:narrower	medtop:20000424 ;
	skos:narrower	medtop:20000430 ;
	skos:narrower	medtop:20000441 ;
	skos:narrower	medtop:20001374 .

medtop:07000000
	rdf:type skos:Concept ;
	skos:prefLabel	"health"@en-GB ;
	skos:definition	"All aspects of physical and mental well-being"@en-GB ;
	skos:inScheme <http://cv.iptc.org/newscodes/mediatopic/>  ;
	ikos:created "2009-10-22T02:00:00+00:00"^^xsd:dateTime ;
	dct:created "2009-10-22T02:00:00+00:00"^^xsd:dateTime ;
	ikos:modified "2022-06-14T12:00:00+00:00"^^xsd:dateTime ;
	dct:modified "2022-06-14T12:00:00+00:00"^^xsd:dateTime  ;
	skos:exactMatch subj:07000000 ;
	skos:exactMatch <https://www.wikidata.org/entity/Q12147> ;
	skos:narrower	medtop:20000446 ;
	skos:narrower	medtop:20000461 ;
	skos:narrower	medtop:20000463 ;
	skos:narrower	medtop:20000464 ;
	skos:narrower	medtop:20000480 ;
	skos:narrower	medtop:20000483 ;
	skos:narrower	medtop:20000484 ;
	skos:narrower	medtop:20000485 ;
	skos:narrower	medtop:20000493 ;
	skos:narrower	medtop:20001358 .

medtop:08000000
	rdf:type skos:Concept ;
	skos:prefLabel	"human interest"@en-GB ;
	skos:definition	"Item that discusses individuals, groups, animals, plants or other objects in an emotional way"@en-GB ;
	skos:inScheme <http://cv.iptc.org/newscodes/mediatopic/>  ;
	ikos:created "2009-10-22T02:00:00+00:00"^^xsd:dateTime ;
	dct:created "2009-10-22T02:00:00+00:00"^^xsd:dateTime ;
	ikos:modified "2021-05-05T12:00:00+00:00"^^xsd:dateTime ;
	dct:modified "2021-05-05T12:00:00+00:00"^^xsd:dateTime  ;
	skos:exactMatch <https://www.wikidata.org/entity/Q361306> ;
	skos:closeMatch subj:08000000 ;
	skos:narrower	medtop:20000497 ;
	skos:narrower	medtop:20000498 ;
	skos:narrower	medtop:20000499 ;
	skos:narrower	medtop:20000501 ;
	skos:narrower	medtop:20000502 ;
	skos:narrower	medtop:20000503 ;
	skos:narrower	medtop:20000504 ;
	skos:narrower	medtop:20000505 ;
	skos:narrower	medtop:20001237 ;
	skos:narrower	medtop:20001238 .

medtop:09000000
	rdf:type skos:Concept ;
	skos:prefLabel	"labour"@en-GB ;
	skos:definition	"Social aspects, organisations, rules and conditions affecting the employment of human effort for the generation of wealth or provision of services and the economic support of the unemployed."@en-GB ;
	skos:inScheme <http://cv.iptc.org/newscodes/mediatopic/>  ;
	ikos:created "2009-10-22T02:00:00+00:00"^^xsd:dateTime ;
	dct:created "2009-10-22T02:00:00+00:00"^^xsd:dateTime ;
	ikos:modified "2021-02-18T12:00:00+00:00"^^xsd:dateTime ;
	dct:modified "2021-02-18T12:00:00+00:00"^^xsd:dateTime  ;
	skos:exactMatch subj:09000000 ;
	skos:exactMatch <https://www.wikidata.org/entity/Q268378> ;
	skos:narrower	medtop:20000509 ;
	skos:narrower	medtop:20000521 ;
	skos:narrower	medtop:20000523 ;
	skos:narrower	medtop:20000524 ;
	skos:narrower	medtop:20000531 ;
	skos:narrower	medtop:20000533 ;
	skos:narrower	medtop:20000536 .

medtop:10000000
	rdf:type skos:Concept ;
	skos:prefLabel	"lifestyle and leisure"@en-GB ;
	skos:definition	"Activities undertaken for pleasure, relaxation or recreation outside paid employment, including eating and travel."@en-GB ;
	skos:inScheme <http://cv.iptc.org/newscodes/mediatopic/>  ;
	ikos:created "2009-10-22T02:00:00+00:00"^^xsd:dateTime ;
	dct:created "2009-10-22T02:00:00+00:00"^^xsd:dateTime ;
	ikos:modified "2021-05-05T12:00:00+00:00"^^xsd:dateTime ;
	dct:modified "2021-05-05T12:00:00+00:00"^^xsd:dateTime  ;
	skos:exactMatch subj:10000000 ;
	skos:exactMatch <https://www.wikidata.org/entity/Q1267055> ;
	skos:narrower	medtop:20000538 ;
	skos:narrower	medtop:20000565 ;
	skos:narrower	medtop:20001339 .

medtop:11000000
	rdf:type skos:Concept ;
	skos:prefLabel	"politics"@en-GB ;
	skos:definition	"Local, regional, national and international exercise of power, or struggle for power, and the relationships between governing bodies and states."@en-GB ;
	skos:inScheme <http://cv.iptc.org/newscodes/mediatopic/>  ;
	ikos:created "2009-10-22T02:00:00+00:00"^^xsd:dateTime ;
	dct:created "2009-10-22T02:00:00+00:00"^^xsd:dateTime ;
	ikos:modified "2021-02-18T12:00:00+00:00"^^xsd:dateTime ;
	dct:modified "2021-02-18T12:00:00+00:00"^^xsd:dateTime  ;
	skos:exactMatch <https://www.wikidata.org/entity/Q7163> ;
	skos:exactMatch subj:11000000 ;
	skos:narrower	medtop:20000574 ;
	skos:narrower	medtop:20000587 ;
	skos:narrower	medtop:20000593 ;
	skos:narrower	medtop:20000621 ;
	skos:narrower	medtop:20000638 ;
	skos:narrower	medtop:20000646 ;
	skos:narrower	medtop:20000647 ;
	skos:narrower	medtop:20000648 ;
	skos:narrower	medtop:20000649 .

medtop:12000000
	rdf:type skos:Concept ;
	skos:prefLabel	"religion"@en-GB ;
	skos:definition	"Belief systems, institutions and people who provide moral guidance to followers"@en-GB ;
	skos:inScheme <http://cv.iptc.org/newscodes/mediatopic/>  ;
	ikos:created "2009-10-22T02:00:00+00:00"^^xsd:dateTime ;
	dct:created "2009-10-22T02:00:00+00:00"^^xsd:dateTime ;
	ikos:modified "2021-12-21T12:00:00+00:00"^^xsd:dateTime ;
	dct:modified "2021-12-21T12:00:00+00:00"^^xsd:dateTime  ;
	skos:exactMatch subj:12000000 ;
	skos:narrower	medtop:20000657 ;
	skos:narrower	medtop:20000687 ;
	skos:narrower	medtop:20000688 ;
	skos:narrower	medtop:20000689 ;
	skos:narrower	medtop:20000690 ;
	skos:narrower	medtop:20000696 ;
	skos:narrower	medtop:20000697 ;
	skos:narrower	medtop:20000702 ;
	skos:narrower	medtop:20000703 ;
	skos:narrower	medtop:20000705 .

medtop:13000000
	rdf:type skos:Concept ;
	skos:prefLabel	"science and technology"@en-GB ;
	skos:definition	"All aspects pertaining to human understanding of, as well as methodical study and research of natural, formal and social sciences, such as astronomy, linguistics or economics"@en-GB ;
	skos:inScheme <http://cv.iptc.org/newscodes/mediatopic/>  ;
	ikos:created "2009-10-22T02:00:00+00:00"^^xsd:dateTime ;
	dct:created "2009-10-22T02:00:00+00:00"^^xsd:dateTime ;
	ikos:modified "2021-02-18T12:00:00+00:00"^^xsd:dateTime ;
	dct:modified "2021-02-18T12:00:00+00:00"^^xsd:dateTime  ;
	skos:exactMatch subj:13000000 ;
	skos:exactMatch <https://www.wikidata.org/entity/Q34104> ;
	skos:narrower	medtop:20000710 ;
	skos:narrower	medtop:20000715 ;
	skos:narrower	medtop:20000717 ;
	skos:narrower	medtop:20000735 ;
	skos:narrower	medtop:20000741 ;
	skos:narrower	medtop:20000742 ;
	skos:narrower	medtop:20000755 ;
	skos:narrower	medtop:20000756 .

medtop:14000000
	rdf:type skos:Concept ;
	skos:prefLabel	"society"@en-GB ;
	skos:definition	"The concerns, issues, affairs and institutions relevant to human social interactions, problems and welfare, such as poverty, human rights and family planning"@en-GB ;
	skos:inScheme <http://cv.iptc.org/newscodes/mediatopic/>  ;
	ikos:created "2009-10-22T02:00:00+00:00"^^xsd:dateTime ;
	dct:created "2009-10-22T02:00:00+00:00"^^xsd:dateTime ;
	ikos:modified "2021-02-18T12:00:00+00:00"^^xsd:dateTime ;
	dct:modified "2021-02-18T12:00:00+00:00"^^xsd:dateTime  ;
	skos:exactMatch <https://www.wikidata.org/entity/Q8425> ;
	skos:exactMatch subj:14025000 ;
	skos:narrower	medtop:20000768 ;
	skos:narrower	medtop:20000770 ;
	skos:narrower	medtop:20000771 ;
	skos:narrower	medtop:20000772 ;
	skos:narrower	medtop:20000775 ;
	skos:narrower	medtop:20000780 ;
	skos:narrower	medtop:20000788 ;
	skos:narrower	medtop:20000799 ;
	skos:narrower	medtop:20000802 ;
	skos:narrower	medtop:20000808 ;
	skos:narrower	medtop:20000817 ;
	skos:narrower	medtop:20001373 .

medtop:15000000
	rdf:type skos:Concept ;
	skos:prefLabel	"sport"@en-GB ;
	skos:definition	"Competitive activity or skill that involves physical and/or mental effort and organisations and bodies involved in these activities"@en-GB ;
	skos:changeNote	"Changes: 2018-04-19 definition changed to make it fit better for chess and eSports."@en-GB ;
	skos:inScheme <http://cv.iptc.org/newscodes/mediatopic/>  ;
	ikos:created "2009-10-22T02:00:00+00:00"^^xsd:dateTime ;
	dct:created "2009-10-22T02:00:00+00:00"^^xsd:dateTime ;
	ikos:modified "2021-02-18T12:00:00+00:00"^^xsd:dateTime ;
	dct:modified "2021-02-18T12:00:00+00:00"^^xsd:dateTime  ;
	skos:exactMatch <https://www.wikidata.org/entity/Q349> ;
	skos:exactMatch subj:15000000 ;
	skos:narrower	medtop:20000822 ;
	skos:narrower	medtop:20001103 ;
	skos:narrower	medtop:20001104 ;
	skos:narrower	medtop:20001108 ;
	skos:narrower	medtop:20001124 ;
	skos:narrower	medtop:20001125 ;
	skos:narrower	medtop:20001126 ;
	skos:narrower	medtop:20001148 ;
	skos:narrower	medtop:20001301 ;
	skos:narrower	medtop:20001323 ;
	skos:narrower	medtop:20001324 ;
	skos:narrower	medtop:20001325 .

medtop:16000000
	rdf:type skos:Concept ;
	skos:prefLabel	"conflict, war and peace"@en-GB ;
	skos:definition	"Acts of socially or politically motivated protest or violence, military activities, geopolitical conflicts, as well as resolution efforts"@en-GB ;
	skos:inScheme <http://cv.iptc.org/newscodes/mediatopic/>  ;
	ikos:created "2009-10-22T02:00:00+00:00"^^xsd:dateTime ;
	dct:created "2009-10-22T02:00:00+00:00"^^xsd:dateTime ;
	ikos:modified "2021-02-18T12:00:00+00:00"^^xsd:dateTime ;
	dct:modified "2021-02-18T12:00:00+00:00"^^xsd:dateTime  ;
	skos:broadMatch subj:16000000 ;
	skos:narrower	medtop:20000053 ;
	skos:narrower	medtop:20000056 ;
	skos:narrower	medtop:20000065 ;
	skos:narrower	medtop:20000070 ;
	skos:narrower	medtop:20000071 ;
	skos:narrower	medtop:20000073 ;
	skos:narrower	medtop:20000077 ;
	skos:narrower	medtop:20000080 ;
	skos:narrower	medtop:20001361 .

medtop:17000000
	rdf:type skos:Concept ;
	skos:prefLabel	"weather"@en-GB ;
	skos:definition	"The study, prediction and reporting of meteorological phenomena"@en-GB ;
	skos:inScheme <http://cv.iptc.org/newscodes/mediatopic/>  ;
	ikos:created "2009-10-22T02:00:00+00:00"^^xsd:dateTime ;
	dct:created "2009-10-22T02:00:00+00:00"^^xsd:dateTime ;
	ikos:modified "2021-02-18T12:00:00+00:00"^^xsd:dateTime ;
	dct:modified "2021-02-18T12:00:00+00:00"^^xsd:dateTime  ;
	skos:exactMatch subj:17000000 ;
	skos:exactMatch <https://www.wikidata.org/entity/Q11663> ;
	skos:narrower	medtop:20001128 ;
	skos:narrower	medtop:20001129 ;
	skos:narrower	medtop:20001130 ;
	skos:narrower	medtop:20001131 .

medtop:20000002
	rdf:type skos:Concept ;
	skos:prefLabel	"arts and entertainment"@en-GB ;
	skos:definition	"All forms of arts and entertainment"@en-GB ;
	skos:inScheme <http://cv.iptc.org/newscodes/mediatopic/>  ;
	ikos:created "2009-10-22T02:00:00+00:00"^^xsd:dateTime ;
	dct:created "2009-10-22T02:00:00+00:00"^^xsd:dateTime ;
	ikos:modified "2021-02-18T12:00:00+00:00"^^xsd:dateTime ;
	dct:modified "2021-02-18T12:00:00+00:00"^^xsd:dateTime  ;
	skos:exactMatch <https://www.wikidata.org/entity/Q2018526> ;
	skos:broadMatch subj:01000000 ;
	skos:broader	medtop:01000000 ;
	skos:narrower	medtop:20000003 ;
	skos:narrower	medtop:20000004 ;
	skos:narrower	medtop:20000005 ;
	skos:narrower	medtop:20000007 ;
	skos:narrower	medtop:20000011 ;
	skos:narrower	medtop:20000013 ;
	skos:narrower	medtop:20000018 ;
	skos:narrower	medtop:20000029 ;
	skos:narrower	medtop:20000031 ;
	skos:narrower	medtop:20001179 ;
	skos:narrower	medtop:20001181 .

medtop:20000003
	rdf:type skos:Concept ;
	skos:prefLabel	"animation"@en-GB ;
	skos:definition	"Stories told through animated drawings in either full-length or short format"@en-GB ;
	skos:inScheme <http://cv.iptc.org/newscodes/mediatopic/>  ;
	ikos:created "2009-10-22T02:00:00+00:00"^^xsd:dateTime ;
	dct:created "2009-10-22T02:00:00+00:00"^^xsd:dateTime ;
	ikos:modified "2021-03-15T12:00:00+00:00"^^xsd:dateTime ;
	dct:modified "2021-03-15T12:00:00+00:00"^^xsd:dateTime  ;
	skos:exactMatch subj:01025000 ;
	skos:exactMatch <https://www.wikidata.org/entity/Q11425> ;
	skos:broader	medtop:20000002 .

medtop:20000004
	rdf:type skos:Concept ;
	skos:prefLabel	"cartoon"@en-GB ;
	skos:definition	"Drawings, such as editorial cartoons and comic strips, often using humour or satire"@en-GB ;
	skos:inScheme <http://cv.iptc.org/newscodes/mediatopic/>  ;
	ikos:created "2009-10-22T02:00:00+00:00"^^xsd:dateTime ;
	dct:created "2009-10-22T02:00:00+00:00"^^xsd:dateTime ;
	ikos:modified "2021-02-18T12:00:00+00:00"^^xsd:dateTime ;
	dct:modified "2021-02-18T12:00:00+00:00"^^xsd:dateTime  ;
	skos:exactMatch subj:01024000 ;
	skos:exactMatch <https://www.wikidata.org/entity/Q627603> ;
	skos:broader	medtop:20000002 .

medtop:20000005
	rdf:type skos:Concept ;
	skos:prefLabel	"cinema"@en-GB ;
	skos:definition	"Stories told through motion pictures, such as full-length or short format documentary or fictional features"@en-GB ;
	skos:inScheme <http://cv.iptc.org/newscodes/mediatopic/>  ;
	ikos:created "2009-10-22T02:00:00+00:00"^^xsd:dateTime ;
	dct:created "2009-10-22T02:00:00+00:00"^^xsd:dateTime ;
	ikos:modified "2021-02-18T12:00:00+00:00"^^xsd:dateTime ;
	dct:modified "2021-02-18T12:00:00+00:00"^^xsd:dateTime  ;
	skos:exactMatch subj:01005000 ;
	skos:exactMatch <https://www.wikidata.org/entity/Q16144339> ;
	skos:broader	medtop:20000002 .

medtop:20000006
	rdf:type skos:Concept ;
	skos:prefLabel	"film festival"@en-GB ;
	skos:definition	"All forms of national and international film festivals"@en-GB ;
	skos:changeNote	"Changes: 2018-04-09 other Broader Term"@en-GB ;
	skos:inScheme <http://cv.iptc.org/newscodes/mediatopic/>  ;
	ikos:created "2009-10-22T02:00:00+00:00"^^xsd:dateTime ;
	dct:created "2009-10-22T02:00:00+00:00"^^xsd:dateTime ;
	ikos:modified "2021-02-18T12:00:00+00:00"^^xsd:dateTime ;
	dct:modified "2021-02-18T12:00:00+00:00"^^xsd:dateTime  ;
	skos:exactMatch subj:01005001 ;
	skos:exactMatch <https://www.wikidata.org/entity/Q220505> ;
	skos:broader	medtop:20001181 .

medtop:20000007
	rdf:type skos:Concept ;
	skos:prefLabel	"dance"@en-GB ;
	skos:definition	"A form of performing art consisting of purposefully selected sequences of human movement"@en-GB ;
	skos:inScheme <http://cv.iptc.org/newscodes/mediatopic/>  ;
	ikos:created "2009-10-22T02:00:00+00:00"^^xsd:dateTime ;
	dct:created "2009-10-22T02:00:00+00:00"^^xsd:dateTime ;
	ikos:modified "2021-02-18T12:00:00+00:00"^^xsd:dateTime ;
	dct:modified "2021-02-18T12:00:00+00:00"^^xsd:dateTime  ;
	skos:exactMatch subj:01006000 ;
	skos:exactMatch <https://www.wikidata.org/entity/Q11639> ;
	skos:broader	medtop:20000002 ;
	skos:narrower	medtop:20000008 ;
	skos:narrower	medtop:20000009 ;
	skos:narrower	medtop:20000010 .

medtop:20000008
	rdf:type skos:Concept ;
	skos:prefLabel	"ballet"@en-GB ;
	skos:definition	"A classical dance form based on formal gestures, steps and postures"@en-GB ;
	skos:inScheme <http://cv.iptc.org/newscodes/mediatopic/>  ;
	ikos:created "2009-10-22T02:00:00+00:00"^^xsd:dateTime ;
	dct:created "2009-10-22T02:00:00+00:00"^^xsd:dateTime ;
	ikos:modified "2021-02-18T12:00:00+00:00"^^xsd:dateTime ;
	dct:modified "2021-02-18T12:00:00+00:00"^^xsd:dateTime  ;
	skos:broadMatch subj:01006000 ;
	skos:exactMatch <https://www.wikidata.org/entity/Q41425> ;
	skos:broader	medtop:20000007 .

medtop:20000009
	rdf:type skos:Concept ;
	skos:prefLabel	"modern dance"@en-GB ;
	skos:definition	"A theatrical dance style based on free-style expression rather than formal gestures"@en-GB ;
	skos:inScheme <http://cv.iptc.org/newscodes/mediatopic/>  ;
	ikos:created "2009-10-22T02:00:00+00:00"^^xsd:dateTime ;
	dct:created "2009-10-22T02:00:00+00:00"^^xsd:dateTime ;
	ikos:modified "2021-02-18T12:00:00+00:00"^^xsd:dateTime ;
	dct:modified "2021-02-18T12:00:00+00:00"^^xsd:dateTime  ;
	skos:broadMatch subj:01006000 ;
	skos:exactMatch <https://www.wikidata.org/entity/Q850130> ;
	skos:broader	medtop:20000007 .

medtop:20000010
	rdf:type skos:Concept ;
	skos:prefLabel	"traditional dance"@en-GB ;
	skos:definition	"Dance style that reflects the life and culture of a specific group of people or region, such as folk and ceremonial dance"@en-GB ;
	skos:inScheme <http://cv.iptc.org/newscodes/mediatopic/>  ;
	ikos:created "2009-10-22T02:00:00+00:00"^^xsd:dateTime ;
	dct:created "2009-10-22T02:00:00+00:00"^^xsd:dateTime ;
	ikos:modified "2021-02-18T12:00:00+00:00"^^xsd:dateTime ;
	dct:modified "2021-02-18T12:00:00+00:00"^^xsd:dateTime  ;
	skos:broadMatch subj:01006000 ;
	skos:exactMatch <https://www.wikidata.org/entity/Q201022> ;
	skos:broader	medtop:20000007 .

medtop:20000011
	rdf:type skos:Concept ;
	skos:prefLabel	"fashion"@en-GB ;
	skos:definition	"Styles and trends in clothing, footwear, accessories, including the design, presentation and wearing of these styles and trends"@en-GB ;
	skos:inScheme <http://cv.iptc.org/newscodes/mediatopic/>  ;
	ikos:created "2009-10-22T02:00:00+00:00"^^xsd:dateTime ;
	dct:created "2009-10-22T02:00:00+00:00"^^xsd:dateTime ;
	ikos:modified "2021-02-18T12:00:00+00:00"^^xsd:dateTime ;
	dct:modified "2021-02-18T12:00:00+00:00"^^xsd:dateTime  ;
	skos:exactMatch subj:01007000 ;
	skos:exactMatch <https://www.wikidata.org/entity/Q12684> ;
	skos:broader	medtop:20000002 ;
	skos:narrower	medtop:20000012 ;
	skos:narrower	medtop:20001248 ;
	skos:narrower	medtop:20001249 .

medtop:20000012
	rdf:type skos:Concept ;
	skos:prefLabel	"jewellery"@en-GB ;
	skos:definition	"Decorative items worn for personal expression and adornment, such as rings, necklaces, earrings"@en-GB ;
	skos:inScheme <http://cv.iptc.org/newscodes/mediatopic/>  ;
	ikos:created "2009-10-22T02:00:00+00:00"^^xsd:dateTime ;
	dct:created "2009-10-22T02:00:00+00:00"^^xsd:dateTime ;
	ikos:modified "2021-02-18T12:00:00+00:00"^^xsd:dateTime ;
	dct:modified "2021-02-18T12:00:00+00:00"^^xsd:dateTime  ;
	skos:exactMatch subj:01007001 ;
	skos:exactMatch <https://www.wikidata.org/entity/Q161439> ;
	skos:broader	medtop:20000011 .

medtop:20000013
	rdf:type skos:Concept ;
	skos:prefLabel	"literature"@en-GB ;
	skos:definition	"The telling of a story through written language"@en-GB ;
	skos:inScheme <http://cv.iptc.org/newscodes/mediatopic/>  ;
	ikos:created "2009-10-22T02:00:00+00:00"^^xsd:dateTime ;
	dct:created "2009-10-22T02:00:00+00:00"^^xsd:dateTime ;
	ikos:modified "2021-02-18T12:00:00+00:00"^^xsd:dateTime ;
	dct:modified "2021-02-18T12:00:00+00:00"^^xsd:dateTime  ;
	skos:exactMatch subj:01010000 ;
	skos:exactMatch <https://www.wikidata.org/entity/Q8242> ;
	skos:broader	medtop:20000002 ;
	skos:narrower	medtop:20000014 ;
	skos:narrower	medtop:20000015 ;
	skos:narrower	medtop:20000016 ;
	skos:narrower	medtop:20000017 .

medtop:20000014
	rdf:type skos:Concept ;
	skos:prefLabel	"drama (literature)"@en-GB ;
	skos:definition	"Work written to be performed on the stage"@en-GB ;
	skos:inScheme <http://cv.iptc.org/newscodes/mediatopic/>  ;
	ikos:created "2009-10-22T02:00:00+00:00"^^xsd:dateTime ;
	dct:created "2009-10-22T02:00:00+00:00"^^xsd:dateTime ;
	ikos:modified "2021-02-18T12:00:00+00:00"^^xsd:dateTime ;
	dct:modified "2021-02-18T12:00:00+00:00"^^xsd:dateTime  ;
	skos:broadMatch subj:01010000 ;
	skos:exactMatch <https://www.wikidata.org/entity/Q25372> ;
	skos:broader	medtop:20000013 .

medtop:20000015
	rdf:type skos:Concept ;
	skos:prefLabel	"fiction"@en-GB ;
	skos:definition	"Written works that are not based on fact, but are the creation of the author's imagination"@en-GB ;
	skos:inScheme <http://cv.iptc.org/newscodes/mediatopic/>  ;
	ikos:created "2009-10-22T02:00:00+00:00"^^xsd:dateTime ;
	dct:created "2009-10-22T02:00:00+00:00"^^xsd:dateTime ;
	ikos:modified "2021-02-18T12:00:00+00:00"^^xsd:dateTime ;
	dct:modified "2021-02-18T12:00:00+00:00"^^xsd:dateTime  ;
	skos:exactMatch subj:01010001 ;
	skos:exactMatch <https://www.wikidata.org/entity/Q38072107> ;
	skos:broader	medtop:20000013 .

medtop:20000016
	rdf:type skos:Concept ;
	skos:prefLabel	"non-fiction"@en-GB ;
	skos:definition	"Written works that are based on fact"@en-GB ;
	skos:inScheme <http://cv.iptc.org/newscodes/mediatopic/>  ;
	ikos:created "2009-10-22T02:00:00+00:00"^^xsd:dateTime ;
	dct:created "2009-10-22T02:00:00+00:00"^^xsd:dateTime ;
	ikos:modified "2021-02-18T12:00:00+00:00"^^xsd:dateTime ;
	dct:modified "2021-02-18T12:00:00+00:00"^^xsd:dateTime  ;
	skos:broadMatch subj:01010000 ;
	skos:exactMatch <https://www.wikidata.org/entity/Q213051> ;
	skos:broader	medtop:20000013 .

medtop:20000017
	rdf:type skos:Concept ;
	skos:prefLabel	"poetry"@en-GB ;
	skos:definition	"Written works that use the aesthetic and rhythmic qualities of language to express a message or emotion"@en-GB ;
	skos:inScheme <http://cv.iptc.org/newscodes/mediatopic/>  ;
	ikos:created "2009-10-22T02:00:00+00:00"^^xsd:dateTime ;
	dct:created "2009-10-22T02:00:00+00:00"^^xsd:dateTime ;
	ikos:modified "2021-02-18T12:00:00+00:00"^^xsd:dateTime ;
	dct:modified "2021-02-18T12:00:00+00:00"^^xsd:dateTime  ;
	skos:exactMatch subj:01010002 ;
	skos:exactMatch <https://www.wikidata.org/entity/Q482> ;
	skos:broader	medtop:20000013 .

medtop:20000018
	rdf:type skos:Concept ;
	skos:prefLabel	"music"@en-GB ;
	skos:definition	"A form of performing art using instruments or voice to create different sounds, tones and harmonies"@en-GB ;
	skos:inScheme <http://cv.iptc.org/newscodes/mediatopic/>  ;
	ikos:created "2009-10-22T02:00:00+00:00"^^xsd:dateTime ;
	dct:created "2009-10-22T02:00:00+00:00"^^xsd:dateTime ;
	ikos:modified "2021-02-18T12:00:00+00:00"^^xsd:dateTime ;
	dct:modified "2021-02-18T12:00:00+00:00"^^xsd:dateTime  ;
	skos:exactMatch subj:01011000 ;
	skos:exactMatch <https://www.wikidata.org/entity/Q638> ;
	skos:broader	medtop:20000002 ;
	skos:narrower	medtop:20000019 ;
	skos:narrower	medtop:20000020 ;
	skos:narrower	medtop:20000021 .

medtop:20000019
	rdf:type skos:Concept ;
	skos:prefLabel	"musical instrument"@en-GB ;
	skos:definition	"Objects used to play music on"@en-GB ;
	skos:inScheme <http://cv.iptc.org/newscodes/mediatopic/>  ;
	ikos:created "2009-10-22T02:00:00+00:00"^^xsd:dateTime ;
	dct:created "2009-10-22T02:00:00+00:00"^^xsd:dateTime ;
	ikos:modified "2021-02-18T12:00:00+00:00"^^xsd:dateTime ;
	dct:modified "2021-02-18T12:00:00+00:00"^^xsd:dateTime  ;
	skos:broadMatch subj:01011000 ;
	skos:exactMatch <https://www.wikidata.org/entity/Q34379> ;
	skos:broader	medtop:20000018 .

medtop:20000020
	rdf:type skos:Concept ;
	skos:prefLabel	"musical performance"@en-GB ;
	skos:definition	"Musicians performing for an audience for the purpose of entertainment"@en-GB ;
	skos:inScheme <http://cv.iptc.org/newscodes/mediatopic/>  ;
	ikos:created "2009-10-22T02:00:00+00:00"^^xsd:dateTime ;
	dct:created "2009-10-22T02:00:00+00:00"^^xsd:dateTime ;
	ikos:modified "2021-02-18T12:00:00+00:00"^^xsd:dateTime ;
	dct:modified "2021-02-18T12:00:00+00:00"^^xsd:dateTime  ;
	skos:broadMatch subj:01011000 ;
	skos:exactMatch <https://www.wikidata.org/entity/Q6942562> ;
	skos:broader	medtop:20000018 .

medtop:20000021
	rdf:type skos:Concept ;
	skos:prefLabel	"musical genre"@en-GB ;
	skos:definition	"A distinguishable type of music"@en-GB ;
	skos:inScheme <http://cv.iptc.org/newscodes/mediatopic/>  ;
	ikos:created "2009-10-22T02:00:00+00:00"^^xsd:dateTime ;
	dct:created "2009-10-22T02:00:00+00:00"^^xsd:dateTime ;
	ikos:modified "2021-02-18T12:00:00+00:00"^^xsd:dateTime ;
	dct:modified "2021-02-18T12:00:00+00:00"^^xsd:dateTime  ;
	skos:broadMatch subj:01011000 ;
	skos:exactMatch <https://www.wikidata.org/entity/Q188451> ;
	skos:broader	medtop:20000018 ;
	skos:narrower	medtop:20000022 ;
	skos:narrower	medtop:20000023 ;
	skos:narrower	medtop:20000024 ;
	skos:narrower	medtop:20000025 ;
	skos:narrower	medtop:20000026 ;
	skos:narrower	medtop:20000027 ;
	skos:narrower	medtop:20001184 ;
	skos:narrower	medtop:20001185 ;
	skos:narrower	medtop:20001186 ;
	skos:narrower	medtop:20001187 ;
	skos:narrower	medtop:20001188 ;
	skos:narrower	medtop:20001189 .

medtop:20000022
	rdf:type skos:Concept ;
	skos:prefLabel	"classical music"@en-GB ;
	skos:definition	"A genre of music rooted in the traditions of Western music, including both religious and secular music, such as symphony, concerto and sonata."@en-GB ;
	skos:inScheme <http://cv.iptc.org/newscodes/mediatopic/>  ;
	ikos:created "2009-10-22T02:00:00+00:00"^^xsd:dateTime ;
	dct:created "2009-10-22T02:00:00+00:00"^^xsd:dateTime ;
	ikos:modified "2021-02-18T12:00:00+00:00"^^xsd:dateTime ;
	dct:modified "2021-02-18T12:00:00+00:00"^^xsd:dateTime  ;
	skos:exactMatch subj:01011001 ;
	skos:exactMatch <https://www.wikidata.org/entity/Q9730> ;
	skos:broader	medtop:20000021 .

medtop:20000023
	rdf:type skos:Concept ;
	skos:prefLabel	"country music"@en-GB ;
	skos:definition	"A genre of music that originated in the southern United States, often consisting of ballads or dance tunes and featuring string instruments such as banjos, fiddles and guitars"@en-GB ;
	skos:inScheme <http://cv.iptc.org/newscodes/mediatopic/>  ;
	ikos:created "2009-10-22T02:00:00+00:00"^^xsd:dateTime ;
	dct:created "2009-10-22T02:00:00+00:00"^^xsd:dateTime ;
	ikos:modified "2021-02-18T12:00:00+00:00"^^xsd:dateTime ;
	dct:modified "2021-02-18T12:00:00+00:00"^^xsd:dateTime  ;
	skos:exactMatch subj:01011005 ;
	skos:exactMatch <https://www.wikidata.org/entity/Q83440> ;
	skos:broader	medtop:20000021 .

medtop:20000024
	rdf:type skos:Concept ;
	skos:prefLabel	"folk music"@en-GB ;
	skos:definition	"A genre of music that developed from traditional popular cultures, often based on story telling"@en-GB ;
	skos:inScheme <http://cv.iptc.org/newscodes/mediatopic/>  ;
	ikos:created "2009-10-22T02:00:00+00:00"^^xsd:dateTime ;
	dct:created "2009-10-22T02:00:00+00:00"^^xsd:dateTime ;
	ikos:modified "2021-02-18T12:00:00+00:00"^^xsd:dateTime ;
	dct:modified "2021-02-18T12:00:00+00:00"^^xsd:dateTime  ;
	skos:exactMatch subj:01011002 ;
	skos:exactMatch <https://www.wikidata.org/entity/Q235858> ;
	skos:broader	medtop:20000021 .

medtop:20000025
	rdf:type skos:Concept ;
	skos:prefLabel	"jazz music"@en-GB ;
	skos:definition	"A genre of music with roots in blues and ragtime that originated in African American communities of New Orleans in the United States in the late 19th and early 20th centuries"@en-GB ;
	skos:inScheme <http://cv.iptc.org/newscodes/mediatopic/>  ;
	ikos:created "2009-10-22T02:00:00+00:00"^^xsd:dateTime ;
	dct:created "2009-10-22T02:00:00+00:00"^^xsd:dateTime ;
	ikos:modified "2021-02-18T12:00:00+00:00"^^xsd:dateTime ;
	dct:modified "2021-02-18T12:00:00+00:00"^^xsd:dateTime  ;
	skos:exactMatch subj:01011003 ;
	skos:exactMatch <https://www.wikidata.org/entity/Q8341> ;
	skos:broader	medtop:20000021 .

medtop:20000026
	rdf:type skos:Concept ;
	skos:prefLabel	"popular music"@en-GB ;
	skos:definition	"A genre of music that is widely accessible and designed to appeal to all"@en-GB ;
	skos:inScheme <http://cv.iptc.org/newscodes/mediatopic/>  ;
	ikos:created "2009-10-22T02:00:00+00:00"^^xsd:dateTime ;
	dct:created "2009-10-22T02:00:00+00:00"^^xsd:dateTime ;
	ikos:modified "2021-02-18T12:00:00+00:00"^^xsd:dateTime ;
	dct:modified "2021-02-18T12:00:00+00:00"^^xsd:dateTime  ;
	skos:exactMatch subj:01011004 ;
	skos:exactMatch <https://www.wikidata.org/entity/Q373342> ;
	skos:broader	medtop:20000021 .

medtop:20000027
	rdf:type skos:Concept ;
	skos:prefLabel	"rock and roll music"@en-GB ;
	skos:definition	"A genre of music that originated in the United States during the late 1940s and early 1950s, evolving from African American musical styles such as gospel, jump blues, jazz, boogie woogie, and rhythm and blues."@en-GB ;
	skos:inScheme <http://cv.iptc.org/newscodes/mediatopic/>  ;
	ikos:created "2009-10-22T02:00:00+00:00"^^xsd:dateTime ;
	dct:created "2009-10-22T02:00:00+00:00"^^xsd:dateTime ;
	ikos:modified "2021-02-18T12:00:00+00:00"^^xsd:dateTime ;
	dct:modified "2021-02-18T12:00:00+00:00"^^xsd:dateTime  ;
	skos:exactMatch subj:01011006 ;
	skos:exactMatch <https://www.wikidata.org/entity/Q11399> ;
	skos:broader	medtop:20000021 .

medtop:20000028
	rdf:type skos:Concept ;
	skos:prefLabel	"opera"@en-GB ;
	skos:definition	"A form of performing art where classically trained musicians and singers perform a musical and dramatic work"@en-GB ;
	skos:changeNote	"Changes: 2018-04-09 other Broader Term"@en-GB ;
	skos:inScheme <http://cv.iptc.org/newscodes/mediatopic/>  ;
	ikos:created "2009-10-22T02:00:00+00:00"^^xsd:dateTime ;
	dct:created "2009-10-22T02:00:00+00:00"^^xsd:dateTime ;
	ikos:modified "2021-09-30T12:00:00+00:00"^^xsd:dateTime ;
	dct:modified "2021-09-30T12:00:00+00:00"^^xsd:dateTime  ;
	skos:broadMatch subj:01017001 ;
	skos:exactMatch <https://www.wikidata.org/entity/Q1344> ;
	skos:broader	medtop:20000029 .

medtop:20000029
	rdf:type skos:Concept ;
	skos:prefLabel	"theatre"@en-GB ;
	skos:definition	"A form of performing art where live performers portray a narrative to an audience through dialogue and action"@en-GB ;
	skos:inScheme <http://cv.iptc.org/newscodes/mediatopic/>  ;
	ikos:created "2009-10-22T02:00:00+00:00"^^xsd:dateTime ;
	dct:created "2009-10-22T02:00:00+00:00"^^xsd:dateTime ;
	ikos:modified "2021-02-18T12:00:00+00:00"^^xsd:dateTime ;
	dct:modified "2021-02-18T12:00:00+00:00"^^xsd:dateTime  ;
	skos:exactMatch subj:01017000 ;
	skos:exactMatch <https://www.wikidata.org/entity/Q11635> ;
	skos:broader	medtop:20000002 ;
	skos:narrower	medtop:20000028 ;
	skos:narrower	medtop:20000030 ;
	skos:narrower	medtop:20001133 ;
	skos:narrower	medtop:20001134 ;
	skos:narrower	medtop:20001180 ;
	skos:narrower	medtop:20001190 ;
	skos:narrower	medtop:20001191 .

medtop:20000030
	rdf:type skos:Concept ;
	skos:prefLabel	"music theatre"@en-GB ;
	skos:definition	"A form of performing art where live performers portray a narrative to an audience through song, dialogue and action, such as musicals and operettas"@en-GB ;
	skos:changeNote	"Retired on 2021-09-30. Child terms moved up to be children of medtop:20000029 theatre."@en-GB ;
	skos:inScheme <http://cv.iptc.org/newscodes/mediatopic/>  ;
	ikos:created "2009-10-22T02:00:00+00:00"^^xsd:dateTime ;
	dct:created "2009-10-22T02:00:00+00:00"^^xsd:dateTime ;
	ikos:modified "2021-09-30T12:00:00+00:00"^^xsd:dateTime ;
	dct:modified "2021-09-30T12:00:00+00:00"^^xsd:dateTime  ; 
	ikos:retired "2021-09-30T12:00:00+00:00"^^xsd:dateTime ;
	skos:exactMatch subj:01017001 ;
	skos:broader	medtop:20000029 .

medtop:20000031
	rdf:type skos:Concept ;
	skos:prefLabel	"visual arts"@en-GB ;
	skos:definition	"A form of art which appeals primarily to the visual senses, such as ceramics, drawing, painting, sculpture, printmaking, design, crafts, photography, video, filmmaking, and architecture."@en-GB ;
	skos:inScheme <http://cv.iptc.org/newscodes/mediatopic/>  ;
	ikos:created "2009-10-22T02:00:00+00:00"^^xsd:dateTime ;
	dct:created "2009-10-22T02:00:00+00:00"^^xsd:dateTime ;
	ikos:modified "2021-02-18T12:00:00+00:00"^^xsd:dateTime ;
	dct:modified "2021-02-18T12:00:00+00:00"^^xsd:dateTime  ;
	skos:broadMatch subj:01000000 ;
	skos:exactMatch <https://www.wikidata.org/entity/Q36649> ;
	skos:broader	medtop:20000002 ;
	skos:narrower	medtop:20000032 ;
	skos:narrower	medtop:20000033 ;
	skos:narrower	medtop:20000034 ;
	skos:narrower	medtop:20000035 ;
	skos:narrower	medtop:20000036 ;
	skos:narrower	medtop:20000037 ;
	skos:narrower	medtop:20001203 ;
	skos:narrower	medtop:20001204 ;
	skos:narrower	medtop:20001205 .

medtop:20000032
	rdf:type skos:Concept ;
	skos:prefLabel	"architecture"@en-GB ;
	skos:definition	"The design of buildings, monuments and the spaces around them"@en-GB ;
	skos:inScheme <http://cv.iptc.org/newscodes/mediatopic/>  ;
	ikos:created "2009-10-22T02:00:00+00:00"^^xsd:dateTime ;
	dct:created "2009-10-22T02:00:00+00:00"^^xsd:dateTime ;
	ikos:modified "2021-02-18T12:00:00+00:00"^^xsd:dateTime ;
	dct:modified "2021-02-18T12:00:00+00:00"^^xsd:dateTime  ;
	skos:exactMatch subj:01002000 ;
	skos:exactMatch <https://www.wikidata.org/entity/Q12271> ;
	skos:broader	medtop:20000031 .

medtop:20000033
	rdf:type skos:Concept ;
	skos:prefLabel	"design (visual arts)"@en-GB ;
	skos:definition	"An artistic discipline which focuses on visual communication and presentation, the final product of which can range from jewellery to interior design"@en-GB ;
	skos:inScheme <http://cv.iptc.org/newscodes/mediatopic/>  ;
	ikos:created "2009-10-22T02:00:00+00:00"^^xsd:dateTime ;
	dct:created "2009-10-22T02:00:00+00:00"^^xsd:dateTime ;
	ikos:modified "2021-02-18T12:00:00+00:00"^^xsd:dateTime ;
	dct:modified "2021-02-18T12:00:00+00:00"^^xsd:dateTime  ;
	skos:broadMatch subj:01000000 ;
	skos:exactMatch <https://www.wikidata.org/entity/Q82604> ;
	skos:broader	medtop:20000031 .

medtop:20000034
	rdf:type skos:Concept ;
	skos:prefLabel	"drawing"@en-GB ;
	skos:definition	"A form of visual arts using mediums such as pencils, markers, pen and ink, charcoal"@en-GB ;
	skos:inScheme <http://cv.iptc.org/newscodes/mediatopic/>  ;
	ikos:created "2009-10-22T02:00:00+00:00"^^xsd:dateTime ;
	dct:created "2009-10-22T02:00:00+00:00"^^xsd:dateTime ;
	ikos:modified "2021-02-18T12:00:00+00:00"^^xsd:dateTime ;
	dct:modified "2021-02-18T12:00:00+00:00"^^xsd:dateTime  ;
	skos:broadMatch subj:01000000 ;
	skos:exactMatch <https://www.wikidata.org/entity/Q2921001> ;
	skos:broader	medtop:20000031 .

medtop:20000035
	rdf:type skos:Concept ;
	skos:prefLabel	"painting"@en-GB ;
	skos:definition	"A form of visual arts using mediums such as oil paint, watercolour, pastel, crayon"@en-GB ;
	skos:inScheme <http://cv.iptc.org/newscodes/mediatopic/>  ;
	ikos:created "2009-10-22T02:00:00+00:00"^^xsd:dateTime ;
	dct:created "2009-10-22T02:00:00+00:00"^^xsd:dateTime ;
	ikos:modified "2021-02-18T12:00:00+00:00"^^xsd:dateTime ;
	dct:modified "2021-02-18T12:00:00+00:00"^^xsd:dateTime  ;
	skos:exactMatch subj:01012000 ;
	skos:exactMatch <https://www.wikidata.org/entity/Q11629> ;
	skos:broader	medtop:20000031 .

medtop:20000036
	rdf:type skos:Concept ;
	skos:prefLabel	"photography"@en-GB ;
	skos:definition	"A form of visual arts using photographic images"@en-GB ;
	skos:inScheme <http://cv.iptc.org/newscodes/mediatopic/>  ;
	ikos:created "2009-10-22T02:00:00+00:00"^^xsd:dateTime ;
	dct:created "2009-10-22T02:00:00+00:00"^^xsd:dateTime ;
	ikos:modified "2021-02-18T12:00:00+00:00"^^xsd:dateTime ;
	dct:modified "2021-02-18T12:00:00+00:00"^^xsd:dateTime  ;
	skos:exactMatch subj:01013000 ;
	skos:exactMatch <https://www.wikidata.org/entity/Q11633> ;
	skos:broader	medtop:20000031 .

medtop:20000037
	rdf:type skos:Concept ;
	skos:prefLabel	"sculpture"@en-GB ;
	skos:definition	"A form of visual arts using mediums such as clay, stone, wood and metal to create three-dimensional works"@en-GB ;
	skos:inScheme <http://cv.iptc.org/newscodes/mediatopic/>  ;
	ikos:created "2009-10-22T02:00:00+00:00"^^xsd:dateTime ;
	dct:created "2009-10-22T02:00:00+00:00"^^xsd:dateTime ;
	ikos:modified "2021-05-05T12:00:00+00:00"^^xsd:dateTime ;
	dct:modified "2021-05-05T12:00:00+00:00"^^xsd:dateTime  ;
	skos:exactMatch subj:01015000 ;
	skos:exactMatch <https://www.wikidata.org/entity/Q11634> ;
	skos:broader	medtop:20000031 .

medtop:20000038
	rdf:type skos:Concept ;
	skos:prefLabel	"culture"@en-GB ;
	skos:definition	"The ideas, customs, arts, traditions of a particular group of persons"@en-GB ;
	skos:inScheme <http://cv.iptc.org/newscodes/mediatopic/>  ;
	ikos:created "2009-10-22T02:00:00+00:00"^^xsd:dateTime ;
	dct:created "2009-10-22T02:00:00+00:00"^^xsd:dateTime ;
	ikos:modified "2021-02-18T12:00:00+00:00"^^xsd:dateTime ;
	dct:modified "2021-02-18T12:00:00+00:00"^^xsd:dateTime  ;
	skos:exactMatch <https://www.wikidata.org/entity/Q11042> ;
	skos:exactMatch subj:01022000 ;
	skos:broader	medtop:01000000 ;
	skos:narrower	medtop:20000039 ;
	skos:narrower	medtop:20000040 ;
	skos:narrower	medtop:20000041 ;
	skos:narrower	medtop:20000042 ;
	skos:narrower	medtop:20000043 ;
	skos:narrower	medtop:20000044 ;
	skos:narrower	medtop:20001135 .

medtop:20000039
	rdf:type skos:Concept ;
	skos:prefLabel	"cultural development"@en-GB ;
	skos:definition	"The history of the development of art and culture such as the rise of cave paintings, linguistic variations over time, the evolution of values"@en-GB ;
	skos:inScheme <http://cv.iptc.org/newscodes/mediatopic/>  ;
	ikos:created "2009-10-22T02:00:00+00:00"^^xsd:dateTime ;
	dct:created "2009-10-22T02:00:00+00:00"^^xsd:dateTime ;
	ikos:modified "2021-02-18T12:00:00+00:00"^^xsd:dateTime ;
	dct:modified "2021-02-18T12:00:00+00:00"^^xsd:dateTime  ;
	skos:exactMatch subj:01022001 ;
	skos:broader	medtop:20000038 .

medtop:20000040
	rdf:type skos:Concept ;
	skos:prefLabel	"customs and tradition"@en-GB ;
	skos:definition	"A particular way of behaving, or observances that have developed over time by a group of people"@en-GB ;
	skos:inScheme <http://cv.iptc.org/newscodes/mediatopic/>  ;
	ikos:created "2009-10-22T02:00:00+00:00"^^xsd:dateTime ;
	dct:created "2009-10-22T02:00:00+00:00"^^xsd:dateTime ;
	ikos:modified "2021-02-18T12:00:00+00:00"^^xsd:dateTime ;
	dct:modified "2021-02-18T12:00:00+00:00"^^xsd:dateTime  ;
	skos:exactMatch subj:01019000 ;
	skos:exactMatch <https://www.wikidata.org/entity/Q82821> ;
	skos:exactMatch <https://www.wikidata.org/entity/Q11042> ;
	skos:broader	medtop:20000038 .

medtop:20000041
	rdf:type skos:Concept ;
	skos:prefLabel	"festive event (culture)"@en-GB ;
	skos:definition	"An event ordinarily celebrated by a community and centring on some characteristic aspect of that community and its religion or traditions"@en-GB ;
	skos:inScheme <http://cv.iptc.org/newscodes/mediatopic/>  ;
	ikos:created "2009-10-22T02:00:00+00:00"^^xsd:dateTime ;
	dct:created "2009-10-22T02:00:00+00:00"^^xsd:dateTime ;
	ikos:modified "2021-02-18T12:00:00+00:00"^^xsd:dateTime ;
	dct:modified "2021-02-18T12:00:00+00:00"^^xsd:dateTime  ;
	skos:exactMatch subj:01004000 ;
	skos:exactMatch <https://www.wikidata.org/entity/Q132241> ;
	skos:broader	medtop:20000038 .

medtop:20000042
	rdf:type skos:Concept ;
	skos:prefLabel	"language"@en-GB ;
	skos:definition	"The method of human communication, either spoken or written, consisting of words that are used in a structured and conventional way"@en-GB ;
	skos:inScheme <http://cv.iptc.org/newscodes/mediatopic/>  ;
	ikos:created "2009-10-22T02:00:00+00:00"^^xsd:dateTime ;
	dct:created "2009-10-22T02:00:00+00:00"^^xsd:dateTime ;
	ikos:modified "2021-02-18T12:00:00+00:00"^^xsd:dateTime ;
	dct:modified "2021-02-18T12:00:00+00:00"^^xsd:dateTime  ;
	skos:exactMatch subj:01008000 ;
	skos:exactMatch <https://www.wikidata.org/entity/Q315> ;
	skos:broader	medtop:20000038 .

medtop:20000043
	rdf:type skos:Concept ;
	skos:prefLabel	"library and museum"@en-GB ;
	skos:definition	"Institutions that house collections of books, music, art, or objects from the past and present optionally for public use and display"@en-GB ;
	skos:inScheme <http://cv.iptc.org/newscodes/mediatopic/>  ;
	ikos:created "2009-10-22T02:00:00+00:00"^^xsd:dateTime ;
	dct:created "2009-10-22T02:00:00+00:00"^^xsd:dateTime ;
	ikos:modified "2021-05-05T12:00:00+00:00"^^xsd:dateTime ;
	dct:modified "2021-05-05T12:00:00+00:00"^^xsd:dateTime  ;
	skos:exactMatch subj:01009000 ;
	skos:exactMatch <https://www.wikidata.org/entity/Q5193377> ;
	skos:broader	medtop:20000038 .

medtop:20000044
	rdf:type skos:Concept ;
	skos:prefLabel	"monument and heritage site"@en-GB ;
	skos:definition	"Commemorations of historical people, events, or the areas containing them, in the form of structures such as sculptures, statues or buildings"@en-GB ;
	skos:inScheme <http://cv.iptc.org/newscodes/mediatopic/>  ;
	ikos:created "2009-10-22T02:00:00+00:00"^^xsd:dateTime ;
	dct:created "2009-10-22T02:00:00+00:00"^^xsd:dateTime ;
	ikos:modified "2021-05-05T12:00:00+00:00"^^xsd:dateTime ;
	dct:modified "2021-05-05T12:00:00+00:00"^^xsd:dateTime  ;
	skos:exactMatch subj:01018000 ;
	skos:exactMatch <https://www.wikidata.org/entity/Q914856> ;
	skos:broader	medtop:20000038 ;
	skos:narrower	medtop:20000242 .

medtop:20000045
	rdf:type skos:Concept ;
	skos:prefLabel	"mass media"@en-GB ;
	skos:definition	"Media addressing a large audience"@en-GB ;
	skos:inScheme <http://cv.iptc.org/newscodes/mediatopic/>  ;
	ikos:created "2009-10-22T02:00:00+00:00"^^xsd:dateTime ;
	dct:created "2009-10-22T02:00:00+00:00"^^xsd:dateTime ;
	ikos:modified "2021-02-18T12:00:00+00:00"^^xsd:dateTime ;
	dct:modified "2021-02-18T12:00:00+00:00"^^xsd:dateTime  ;
	skos:exactMatch <https://www.wikidata.org/entity/Q11033> ;
	skos:exactMatch subj:01026000 ;
	skos:broader	medtop:01000000 ;
	skos:narrower	medtop:20000046 ;
	skos:narrower	medtop:20000047 ;
	skos:narrower	medtop:20000048 ;
	skos:narrower	medtop:20000049 ;
	skos:narrower	medtop:20000050 ;
	skos:narrower	medtop:20000051 ;
	skos:narrower	medtop:20001182 ;
	skos:narrower	medtop:20001319 .

medtop:20000046
	rdf:type skos:Concept ;
	skos:prefLabel	"news media"@en-GB ;
	skos:definition	"The presentation of news to the public through different platforms, such as TV, radio, newspapers, magazines, web pages and blogs"@en-GB ;
	skos:inScheme <http://cv.iptc.org/newscodes/mediatopic/>  ;
	ikos:created "2009-10-22T02:00:00+00:00"^^xsd:dateTime ;
	dct:created "2009-10-22T02:00:00+00:00"^^xsd:dateTime ;
	ikos:modified "2021-02-18T12:00:00+00:00"^^xsd:dateTime ;
	dct:modified "2021-02-18T12:00:00+00:00"^^xsd:dateTime  ;
	skos:exactMatch subj:01026002 ;
	skos:exactMatch <https://www.wikidata.org/entity/Q1193236> ;
	skos:broader	medtop:20000045 .

medtop:20000047
	rdf:type skos:Concept ;
	skos:prefLabel	"newspaper"@en-GB ;
	skos:definition	"Daily or weekly publication that presents the news, locally, regionally or globally, as well as features, opinion columns, comics and other content"@en-GB ;
	skos:inScheme <http://cv.iptc.org/newscodes/mediatopic/>  ;
	ikos:created "2009-10-22T02:00:00+00:00"^^xsd:dateTime ;
	dct:created "2009-10-22T02:00:00+00:00"^^xsd:dateTime ;
	ikos:modified "2021-02-18T12:00:00+00:00"^^xsd:dateTime ;
	dct:modified "2021-02-18T12:00:00+00:00"^^xsd:dateTime  ;
	skos:exactMatch subj:01026003 ;
	skos:exactMatch <https://www.wikidata.org/entity/Q11032> ;
	skos:broader	medtop:20000045 .

medtop:20000048
	rdf:type skos:Concept ;
	skos:prefLabel	"online media outlet"@en-GB ;
	skos:definition	"Publication distributing content, such as articles, blogs, photos, video and music, only over the internet"@en-GB ;
	skos:inScheme <http://cv.iptc.org/newscodes/mediatopic/>  ;
	ikos:created "2009-10-22T02:00:00+00:00"^^xsd:dateTime ;
	dct:created "2009-10-22T02:00:00+00:00"^^xsd:dateTime ;
	ikos:modified "2021-05-05T12:00:00+00:00"^^xsd:dateTime ;
	dct:modified "2021-05-05T12:00:00+00:00"^^xsd:dateTime  ;
	skos:broadMatch subj:01026000 ;
	skos:exactMatch <https://www.wikidata.org/entity/Q1153191> ;
	skos:broader	medtop:20000045 .

medtop:20000049
	rdf:type skos:Concept ;
	skos:prefLabel	"periodical"@en-GB ;
	skos:definition	"Publication that is usually published weekly, bi-weekly, monthly or annually, such as magazines, journals or newsletters"@en-GB ;
	skos:inScheme <http://cv.iptc.org/newscodes/mediatopic/>  ;
	ikos:created "2009-10-22T02:00:00+00:00"^^xsd:dateTime ;
	dct:created "2009-10-22T02:00:00+00:00"^^xsd:dateTime ;
	ikos:modified "2021-02-18T12:00:00+00:00"^^xsd:dateTime ;
	dct:modified "2021-02-18T12:00:00+00:00"^^xsd:dateTime  ;
	skos:exactMatch subj:01026001 ;
	skos:exactMatch <https://www.wikidata.org/entity/Q1002697> ;
	skos:broader	medtop:20000045 .

medtop:20000050
	rdf:type skos:Concept ;
	skos:prefLabel	"radio"@en-GB ;
	skos:definition	"Audio content, such as news, entertainment or information, distributed via broadcast or internet"@en-GB ;
	skos:inScheme <http://cv.iptc.org/newscodes/mediatopic/>  ;
	ikos:created "2009-10-22T02:00:00+00:00"^^xsd:dateTime ;
	dct:created "2009-10-22T02:00:00+00:00"^^xsd:dateTime ;
	ikos:modified "2021-02-18T12:00:00+00:00"^^xsd:dateTime ;
	dct:modified "2021-02-18T12:00:00+00:00"^^xsd:dateTime  ;
	skos:exactMatch subj:01014000 ;
	skos:exactMatch <https://www.wikidata.org/entity/Q273623> ;
	skos:broader	medtop:20000045 .

medtop:20000051
	rdf:type skos:Concept ;
	skos:prefLabel	"television"@en-GB ;
	skos:definition	"Video content, such as news, entertainment or information, distributed via broadcast or internet"@en-GB ;
	skos:inScheme <http://cv.iptc.org/newscodes/mediatopic/>  ;
	ikos:created "2009-10-22T02:00:00+00:00"^^xsd:dateTime ;
	dct:created "2009-10-22T02:00:00+00:00"^^xsd:dateTime ;
	ikos:modified "2021-02-18T12:00:00+00:00"^^xsd:dateTime ;
	dct:modified "2021-02-18T12:00:00+00:00"^^xsd:dateTime  ;
	skos:exactMatch subj:01016000 ;
	skos:exactMatch <https://www.wikidata.org/entity/Q289> ;
	skos:broader	medtop:20000045 .

medtop:20000053
	rdf:type skos:Concept ;
	skos:prefLabel	"act of terror"@en-GB ;
	skos:definition	"Act of violence, often resulting in casualties, designed to raise fear and anxiety in a population"@en-GB ;
	skos:inScheme <http://cv.iptc.org/newscodes/mediatopic/>  ;
	ikos:created "2009-10-22T02:00:00+00:00"^^xsd:dateTime ;
	dct:created "2009-10-22T02:00:00+00:00"^^xsd:dateTime ;
	ikos:modified "2021-02-18T12:00:00+00:00"^^xsd:dateTime ;
	dct:modified "2021-02-18T12:00:00+00:00"^^xsd:dateTime  ;
	skos:exactMatch subj:16001000 ;
	skos:exactMatch <https://www.wikidata.org/entity/Q5710433> ;
	skos:broader	medtop:16000000 ;
	skos:narrower	medtop:20000054 ;
	skos:narrower	medtop:20000055 .

medtop:20000054
	rdf:type skos:Concept ;
	skos:prefLabel	"act of bioterrorism"@en-GB ;
	skos:definition	"Attacks using biological agents intended to raise the level of fear within a population"@en-GB ;
	skos:inScheme <http://cv.iptc.org/newscodes/mediatopic/>  ;
	ikos:created "2009-10-22T02:00:00+00:00"^^xsd:dateTime ;
	dct:created "2009-10-22T02:00:00+00:00"^^xsd:dateTime ;
	ikos:modified "2021-02-18T12:00:00+00:00"^^xsd:dateTime ;
	dct:modified "2021-02-18T12:00:00+00:00"^^xsd:dateTime  ;
	skos:exactMatch subj:16005001 ;
	skos:exactMatch <https://www.wikidata.org/entity/Q854975> ;
	skos:broader	medtop:20000053 .

medtop:20000055
	rdf:type skos:Concept ;
	skos:prefLabel	"terrorist bombings"@en-GB ;
	skos:definition	"Intentional use of explosive devices on people, buildings or other structures"@en-GB ;
	skos:inScheme <http://cv.iptc.org/newscodes/mediatopic/>  ;
	ikos:created "2009-10-22T02:00:00+00:00"^^xsd:dateTime ;
	dct:created "2009-10-22T02:00:00+00:00"^^xsd:dateTime ;
	ikos:modified "2023-03-31T12:00:00+00:00"^^xsd:dateTime ;
	dct:modified "2023-03-31T12:00:00+00:00"^^xsd:dateTime  ;
	skos:exactMatch subj:16005002 ;
	skos:exactMatch <https://www.wikidata.org/entity/Q891854> ;
	skos:broader	medtop:20000053 .

medtop:20000056
	rdf:type skos:Concept ;
	skos:prefLabel	"armed conflict"@en-GB ;
	skos:definition	"Disputes between opposing groups involving the use of weapons, but not necessarily formally declared wars"@en-GB ;
	skos:inScheme <http://cv.iptc.org/newscodes/mediatopic/>  ;
	ikos:created "2009-10-22T02:00:00+00:00"^^xsd:dateTime ;
	dct:created "2009-10-22T02:00:00+00:00"^^xsd:dateTime ;
	ikos:modified "2021-02-18T12:00:00+00:00"^^xsd:dateTime ;
	dct:modified "2021-02-18T12:00:00+00:00"^^xsd:dateTime  ;
	skos:exactMatch subj:16002000 ;
	skos:exactMatch <https://www.wikidata.org/entity/Q350604> ;
	skos:broader	medtop:16000000 ;
	skos:narrower	medtop:20000057 ;
	skos:narrower	medtop:20000058 ;
	skos:narrower	medtop:20000060 ;
	skos:narrower	medtop:20000061 ;
	skos:narrower	medtop:20000062 .

medtop:20000057
	rdf:type skos:Concept ;
	skos:prefLabel	"guerrilla activity"@en-GB ;
	skos:definition	"Anti-government or wartime actions by clandestine or non-state combatant groups, often using tactics such as ambush, sabotage, raids and kidnapping"@en-GB ;
	skos:inScheme <http://cv.iptc.org/newscodes/mediatopic/>  ;
	ikos:created "2009-10-22T02:00:00+00:00"^^xsd:dateTime ;
	dct:created "2009-10-22T02:00:00+00:00"^^xsd:dateTime ;
	ikos:modified "2021-02-18T12:00:00+00:00"^^xsd:dateTime ;
	dct:modified "2021-02-18T12:00:00+00:00"^^xsd:dateTime  ;
	skos:exactMatch subj:16005000 ;
	skos:exactMatch <https://www.wikidata.org/entity/Q80895> ;
	skos:broader	medtop:20000056 .

medtop:20000058
	rdf:type skos:Concept ;
	skos:prefLabel	"international military intervention"@en-GB ;
	skos:definition	"The temporary use of international forces in a country or region that requires outside help with resolving a crisis"@en-GB ;
	skos:inScheme <http://cv.iptc.org/newscodes/mediatopic/>  ;
	ikos:created "2009-10-22T02:00:00+00:00"^^xsd:dateTime ;
	dct:created "2009-10-22T02:00:00+00:00"^^xsd:dateTime ;
	ikos:modified "2021-02-18T12:00:00+00:00"^^xsd:dateTime ;
	dct:modified "2021-02-18T12:00:00+00:00"^^xsd:dateTime  ;
	skos:exactMatch subj:16009002 ;
	skos:exactMatch <https://www.wikidata.org/entity/Q1168287> ;
	skos:broader	medtop:20000056 ;
	skos:narrower	medtop:20000059 .

medtop:20000059
	rdf:type skos:Concept ;
	skos:prefLabel	"peacekeeping force"@en-GB ;
	skos:definition	"The military forces of a nation, or of several nations working together, whose mission is to maintain peace in areas of conflict"@en-GB ;
	skos:inScheme <http://cv.iptc.org/newscodes/mediatopic/>  ;
	ikos:created "2009-10-22T02:00:00+00:00"^^xsd:dateTime ;
	dct:created "2009-10-22T02:00:00+00:00"^^xsd:dateTime ;
	ikos:modified "2021-02-18T12:00:00+00:00"^^xsd:dateTime ;
	dct:modified "2021-02-18T12:00:00+00:00"^^xsd:dateTime  ;
	skos:exactMatch subj:16010001 ;
	skos:exactMatch <https://www.wikidata.org/entity/Q1456930> ;
	skos:broader	medtop:20000058 .

medtop:20000060
	rdf:type skos:Concept ;
	skos:prefLabel	"military occupation"@en-GB ;
	skos:definition	"The temporary forceful taking over of a country or region by invading military forces"@en-GB ;
	skos:inScheme <http://cv.iptc.org/newscodes/mediatopic/>  ;
	ikos:created "2009-10-22T02:00:00+00:00"^^xsd:dateTime ;
	dct:created "2009-10-22T02:00:00+00:00"^^xsd:dateTime ;
	ikos:modified "2021-02-18T12:00:00+00:00"^^xsd:dateTime ;
	dct:modified "2021-02-18T12:00:00+00:00"^^xsd:dateTime  ;
	skos:broadMatch subj:16000000 ;
	skos:exactMatch <https://www.wikidata.org/entity/Q188686> ;
	skos:broader	medtop:20000056 .

medtop:20000061
	rdf:type skos:Concept ;
	skos:prefLabel	"missing in action"@en-GB ;
	skos:definition	"Civilians or military personnel who have gone missing during or after hostilities, conflicts or war"@en-GB ;
	skos:inScheme <http://cv.iptc.org/newscodes/mediatopic/>  ;
	ikos:created "2009-10-22T02:00:00+00:00"^^xsd:dateTime ;
	dct:created "2009-10-22T02:00:00+00:00"^^xsd:dateTime ;
	ikos:modified "2021-02-18T12:00:00+00:00"^^xsd:dateTime ;
	dct:modified "2021-02-18T12:00:00+00:00"^^xsd:dateTime  ;
	skos:exactMatch subj:14017001 ;
	skos:exactMatch <https://www.wikidata.org/entity/Q2344557> ;
	skos:broader	medtop:20000056 .

medtop:20000062
	rdf:type skos:Concept ;
	skos:prefLabel	"war"@en-GB ;
	skos:definition	"Armed hostilities by one group or geopolitical entity against another"@en-GB ;
	skos:inScheme <http://cv.iptc.org/newscodes/mediatopic/>  ;
	ikos:created "2009-10-22T02:00:00+00:00"^^xsd:dateTime ;
	dct:created "2009-10-22T02:00:00+00:00"^^xsd:dateTime ;
	ikos:modified "2021-02-18T12:00:00+00:00"^^xsd:dateTime ;
	dct:modified "2021-02-18T12:00:00+00:00"^^xsd:dateTime  ;
	skos:exactMatch subj:16009000 ;
	skos:exactMatch <https://www.wikidata.org/entity/Q198> ;
	skos:broader	medtop:20000056 ;
	skos:narrower	medtop:20000063 ;
	skos:narrower	medtop:20000064 .

medtop:20000063
	rdf:type skos:Concept ;
	skos:prefLabel	"civil war"@en-GB ;
	skos:definition	"Armed conflict between members of the same country, in some cases with the goal of dividing the country"@en-GB ;
	skos:inScheme <http://cv.iptc.org/newscodes/mediatopic/>  ;
	ikos:created "2009-10-22T02:00:00+00:00"^^xsd:dateTime ;
	dct:created "2009-10-22T02:00:00+00:00"^^xsd:dateTime ;
	ikos:modified "2021-02-18T12:00:00+00:00"^^xsd:dateTime ;
	dct:modified "2021-02-18T12:00:00+00:00"^^xsd:dateTime  ;
	skos:exactMatch subj:16009001 ;
	skos:exactMatch <https://www.wikidata.org/entity/Q8465> ;
	skos:broader	medtop:20000062 .

medtop:20000064
	rdf:type skos:Concept ;
	skos:prefLabel	"war crime action"@en-GB ;
	skos:definition	"Actions alleged as crimes committed during a war or armed conflict, usually against civilians or POWs"@en-GB ;
	skos:changeNote	"2016-04-05: As two concepts with very similar definitions exist this concept (medtop:20000064) was retired and it is recommended to use war crime (medtop:20000105)"@en-GB ;
	skos:inScheme <http://cv.iptc.org/newscodes/mediatopic/>  ;
	ikos:created "2009-10-22T02:00:00+00:00"^^xsd:dateTime ;
	dct:created "2009-10-22T02:00:00+00:00"^^xsd:dateTime ;
	ikos:modified "2021-05-05T12:00:00+00:00"^^xsd:dateTime ;
	dct:modified "2021-05-05T12:00:00+00:00"^^xsd:dateTime  ; 
	ikos:retired "2016-04-05T12:00:00+00:00"^^xsd:dateTime ;
	skos:exactMatch subj:16009000 ;
	skos:exactMatch <https://www.wikidata.org/entity/Q135010> ;
	skos:broader	medtop:20000062 .

medtop:20000065
	rdf:type skos:Concept ;
	skos:prefLabel	"civil unrest"@en-GB ;
	skos:definition	"Rallies, strikes, demonstrations, riots or other disturbances by a population, often in protest to a government or other organization's policies or actions"@en-GB ;
	skos:inScheme <http://cv.iptc.org/newscodes/mediatopic/>  ;
	ikos:created "2009-10-22T02:00:00+00:00"^^xsd:dateTime ;
	dct:created "2009-10-22T02:00:00+00:00"^^xsd:dateTime ;
	ikos:modified "2021-02-18T12:00:00+00:00"^^xsd:dateTime ;
	dct:modified "2021-02-18T12:00:00+00:00"^^xsd:dateTime  ;
	skos:exactMatch subj:16003000 ;
	skos:exactMatch <https://www.wikidata.org/entity/Q686984> ;
	skos:broader	medtop:16000000 ;
	skos:narrower	medtop:20000066 ;
	skos:narrower	medtop:20000067 ;
	skos:narrower	medtop:20000068 ;
	skos:narrower	medtop:20000069 .

medtop:20000066
	rdf:type skos:Concept ;
	skos:prefLabel	"demonstration"@en-GB ;
	skos:definition	"A non-violent public show of support for or opposition to a cause, idea or policy, in the form of a mass meeting or march"@en-GB ;
	skos:inScheme <http://cv.iptc.org/newscodes/mediatopic/>  ;
	ikos:created "2009-10-22T02:00:00+00:00"^^xsd:dateTime ;
	dct:created "2009-10-22T02:00:00+00:00"^^xsd:dateTime ;
	ikos:modified "2021-02-18T12:00:00+00:00"^^xsd:dateTime ;
	dct:modified "2021-02-18T12:00:00+00:00"^^xsd:dateTime  ;
	skos:exactMatch subj:16008000 ;
	skos:exactMatch <https://www.wikidata.org/entity/Q175331> ;
	skos:broader	medtop:20000065 .

medtop:20000067
	rdf:type skos:Concept ;
	skos:prefLabel	"rebellion"@en-GB ;
	skos:definition	"Organized actions of opposition to a government or ruling party by a country's residents, often violent and with the aim of overthrowing the government"@en-GB ;
	skos:inScheme <http://cv.iptc.org/newscodes/mediatopic/>  ;
	ikos:created "2009-10-22T02:00:00+00:00"^^xsd:dateTime ;
	dct:created "2009-10-22T02:00:00+00:00"^^xsd:dateTime ;
	ikos:modified "2021-02-18T12:00:00+00:00"^^xsd:dateTime ;
	dct:modified "2021-02-18T12:00:00+00:00"^^xsd:dateTime  ;
	skos:exactMatch subj:16003002 ;
	skos:exactMatch <https://www.wikidata.org/entity/Q124734> ;
	skos:broader	medtop:20000065 .

medtop:20000068
	rdf:type skos:Concept ;
	skos:prefLabel	"revolution"@en-GB ;
	skos:definition	"A forcible and often violent change to, or overthrow of, a country's political system or social order by internal forces, in favour of a new system"@en-GB ;
	skos:inScheme <http://cv.iptc.org/newscodes/mediatopic/>  ;
	ikos:created "2009-10-22T02:00:00+00:00"^^xsd:dateTime ;
	dct:created "2009-10-22T02:00:00+00:00"^^xsd:dateTime ;
	ikos:modified "2021-02-18T12:00:00+00:00"^^xsd:dateTime ;
	dct:modified "2021-02-18T12:00:00+00:00"^^xsd:dateTime  ;
	skos:exactMatch subj:16003001 ;
	skos:exactMatch <https://www.wikidata.org/entity/Q10931> ;
	skos:broader	medtop:20000065 .

medtop:20000069
	rdf:type skos:Concept ;
	skos:prefLabel	"riot"@en-GB ;
	skos:definition	"Violent, destructive events of civil disorder by groups of people, usually in response to a grievance or as acts of opposition, often involving injury to individuals and destruction of property"@en-GB ;
	skos:inScheme <http://cv.iptc.org/newscodes/mediatopic/>  ;
	ikos:created "2009-10-22T02:00:00+00:00"^^xsd:dateTime ;
	dct:created "2009-10-22T02:00:00+00:00"^^xsd:dateTime ;
	ikos:modified "2021-02-18T12:00:00+00:00"^^xsd:dateTime ;
	dct:modified "2021-02-18T12:00:00+00:00"^^xsd:dateTime  ;
	skos:exactMatch subj:16007000 ;
	skos:exactMatch <https://www.wikidata.org/entity/Q124757> ;
	skos:broader	medtop:20000065 .

medtop:20000070
	rdf:type skos:Concept ;
	skos:prefLabel	"coup d'etat"@en-GB ;
	skos:definition	"The overthrow of an established government by an organised military or political group"@en-GB ;
	skos:inScheme <http://cv.iptc.org/newscodes/mediatopic/>  ;
	ikos:created "2009-10-22T02:00:00+00:00"^^xsd:dateTime ;
	dct:created "2009-10-22T02:00:00+00:00"^^xsd:dateTime ;
	ikos:modified "2021-02-18T12:00:00+00:00"^^xsd:dateTime ;
	dct:modified "2021-02-18T12:00:00+00:00"^^xsd:dateTime  ;
	skos:exactMatch <https://www.wikidata.org/entity/Q45382> ;
	skos:exactMatch subj:16004000 ;
	skos:broader	medtop:16000000 .

medtop:20000071
	rdf:type skos:Concept ;
	skos:prefLabel	"massacre"@en-GB ;
	skos:definition	"The mass killing of people, usually civilians, during wartime hostilities"@en-GB ;
	skos:inScheme <http://cv.iptc.org/newscodes/mediatopic/>  ;
	ikos:created "2009-10-22T02:00:00+00:00"^^xsd:dateTime ;
	dct:created "2009-10-22T02:00:00+00:00"^^xsd:dateTime ;
	ikos:modified "2021-02-18T12:00:00+00:00"^^xsd:dateTime ;
	dct:modified "2021-02-18T12:00:00+00:00"^^xsd:dateTime  ;
	skos:exactMatch subj:16006000 ;
	skos:exactMatch <https://www.wikidata.org/entity/Q3199915> ;
	skos:broader	medtop:16000000 ;
	skos:narrower	medtop:20000072 .

medtop:20000072
	rdf:type skos:Concept ;
	skos:prefLabel	"genocide"@en-GB ;
	skos:definition	"The systematic killing of one clan, tribe, or religious or ethnic group by another"@en-GB ;
	skos:inScheme <http://cv.iptc.org/newscodes/mediatopic/>  ;
	ikos:created "2009-10-22T02:00:00+00:00"^^xsd:dateTime ;
	dct:created "2009-10-22T02:00:00+00:00"^^xsd:dateTime ;
	ikos:modified "2021-02-18T12:00:00+00:00"^^xsd:dateTime ;
	dct:modified "2021-02-18T12:00:00+00:00"^^xsd:dateTime  ;
	skos:exactMatch subj:16006001 ;
	skos:exactMatch <https://www.wikidata.org/entity/Q41397> ;
	skos:broader	medtop:20000071 .

medtop:20000073
	rdf:type skos:Concept ;
	skos:prefLabel	"peace process"@en-GB ;
	skos:definition	"Organized actions to end a war or conflict, usually involving peace negotiations and agreements"@en-GB ;
	skos:inScheme <http://cv.iptc.org/newscodes/mediatopic/>  ;
	ikos:created "2009-10-22T02:00:00+00:00"^^xsd:dateTime ;
	dct:created "2009-10-22T02:00:00+00:00"^^xsd:dateTime ;
	ikos:modified "2021-02-18T12:00:00+00:00"^^xsd:dateTime ;
	dct:modified "2021-02-18T12:00:00+00:00"^^xsd:dateTime  ;
	skos:broadMatch subj:11002003 ;
	skos:exactMatch <https://www.wikidata.org/entity/Q2632158> ;
	skos:broader	medtop:16000000 ;
	skos:narrower	medtop:20000074 ;
	skos:narrower	medtop:20000075 ;
	skos:narrower	medtop:20000076 .

medtop:20000074
	rdf:type skos:Concept ;
	skos:prefLabel	"peace envoy"@en-GB ;
	skos:definition	"Person or organisation initiating and carrying out a peace process"@en-GB ;
	skos:inScheme <http://cv.iptc.org/newscodes/mediatopic/>  ;
	ikos:created "2009-10-22T02:00:00+00:00"^^xsd:dateTime ;
	dct:created "2009-10-22T02:00:00+00:00"^^xsd:dateTime ;
	ikos:modified "2021-07-12T12:00:00+00:00"^^xsd:dateTime ;
	dct:modified "2021-07-12T12:00:00+00:00"^^xsd:dateTime  ;
	skos:broadMatch subj:11002003 ;
	skos:broader	medtop:20000073 .

medtop:20000075
	rdf:type skos:Concept ;
	skos:prefLabel	"peace plan"@en-GB ;
	skos:definition	"A strategy for achieving peace in a warring nation or area of conflict"@en-GB ;
	skos:inScheme <http://cv.iptc.org/newscodes/mediatopic/>  ;
	ikos:created "2009-10-22T02:00:00+00:00"^^xsd:dateTime ;
	dct:created "2009-10-22T02:00:00+00:00"^^xsd:dateTime ;
	ikos:modified "2021-02-18T12:00:00+00:00"^^xsd:dateTime ;
	dct:modified "2021-02-18T12:00:00+00:00"^^xsd:dateTime  ;
	skos:broadMatch subj:11002003 ;
	skos:broader	medtop:20000073 .

medtop:20000076
	rdf:type skos:Concept ;
	skos:prefLabel	"peace talks"@en-GB ;
	skos:definition	"Discussions between countries, world regions or geopolitical entities in conflict or at war, often with a mediator, with the goal of arriving at a solution for peace"@en-GB ;
	skos:inScheme <http://cv.iptc.org/newscodes/mediatopic/>  ;
	ikos:created "2009-10-22T02:00:00+00:00"^^xsd:dateTime ;
	dct:created "2009-10-22T02:00:00+00:00"^^xsd:dateTime ;
	ikos:modified "2021-05-05T12:00:00+00:00"^^xsd:dateTime ;
	dct:modified "2021-05-05T12:00:00+00:00"^^xsd:dateTime  ;
	skos:broadMatch subj:11002003 ;
	skos:exactMatch <https://www.wikidata.org/entity/Q98077935> ;
	skos:broader	medtop:20000073 .

medtop:20000077
	rdf:type skos:Concept ;
	skos:prefLabel	"post-war reconstruction"@en-GB ;
	skos:definition	"Actions to rebuild a society, economy or political system in an area affected by war"@en-GB ;
	skos:inScheme <http://cv.iptc.org/newscodes/mediatopic/>  ;
	ikos:created "2009-10-22T02:00:00+00:00"^^xsd:dateTime ;
	dct:created "2009-10-22T02:00:00+00:00"^^xsd:dateTime ;
	ikos:modified "2021-02-18T12:00:00+00:00"^^xsd:dateTime ;
	dct:modified "2021-02-18T12:00:00+00:00"^^xsd:dateTime  ;
	skos:broadMatch subj:11002000 ;
	skos:exactMatch <https://www.wikidata.org/entity/Q3422086> ;
	skos:broader	medtop:16000000 ;
	skos:narrower	medtop:20000078 ;
	skos:narrower	medtop:20000079 .

medtop:20000078
	rdf:type skos:Concept ;
	skos:prefLabel	"disarmament"@en-GB ;
	skos:definition	"The abolishment or reduction of a country's military weapons cache"@en-GB ;
	skos:inScheme <http://cv.iptc.org/newscodes/mediatopic/>  ;
	ikos:created "2009-10-22T02:00:00+00:00"^^xsd:dateTime ;
	dct:created "2009-10-22T02:00:00+00:00"^^xsd:dateTime ;
	ikos:modified "2021-02-18T12:00:00+00:00"^^xsd:dateTime ;
	dct:modified "2021-02-18T12:00:00+00:00"^^xsd:dateTime  ;
	skos:broadMatch subj:11002000 ;
	skos:exactMatch <https://www.wikidata.org/entity/Q331662> ;
	skos:broader	medtop:20000077 .

medtop:20000079
	rdf:type skos:Concept ;
	skos:prefLabel	"ordnance clearance"@en-GB ;
	skos:definition	"The removal or neutralisation of ordnance such as landmines or cluster bombs that may remain after a war or armed conflict on public ground"@en-GB ;
	skos:inScheme <http://cv.iptc.org/newscodes/mediatopic/>  ;
	ikos:created "2009-10-22T02:00:00+00:00"^^xsd:dateTime ;
	dct:created "2009-10-22T02:00:00+00:00"^^xsd:dateTime ;
	ikos:modified "2021-02-18T12:00:00+00:00"^^xsd:dateTime ;
	dct:modified "2021-02-18T12:00:00+00:00"^^xsd:dateTime  ;
	skos:exactMatch subj:14026000 ;
	skos:broader	medtop:20000077 .

medtop:20000080
	rdf:type skos:Concept ;
	skos:prefLabel	"prisoners of war"@en-GB ;
	skos:definition	"Individuals captured, imprisoned or detained by enemy factions during military conflicts or war"@en-GB ;
	skos:inScheme <http://cv.iptc.org/newscodes/mediatopic/>  ;
	ikos:created "2009-10-22T02:00:00+00:00"^^xsd:dateTime ;
	dct:created "2009-10-22T02:00:00+00:00"^^xsd:dateTime ;
	ikos:modified "2021-05-05T12:00:00+00:00"^^xsd:dateTime ;
	dct:modified "2021-05-05T12:00:00+00:00"^^xsd:dateTime  ;
	skos:exactMatch subj:16009003 ;
	skos:exactMatch <https://www.wikidata.org/entity/Q179637> ;
	skos:broader	medtop:16000000 .

medtop:20000082
	rdf:type skos:Concept ;
	skos:prefLabel	"crime"@en-GB ;
	skos:definition	"Violations of laws by individuals, companies or organisations"@en-GB ;
	skos:inScheme <http://cv.iptc.org/newscodes/mediatopic/>  ;
	ikos:created "2009-10-22T02:00:00+00:00"^^xsd:dateTime ;
	dct:created "2009-10-22T02:00:00+00:00"^^xsd:dateTime ;
	ikos:modified "2021-02-18T12:00:00+00:00"^^xsd:dateTime ;
	dct:modified "2021-02-18T12:00:00+00:00"^^xsd:dateTime  ;
	skos:exactMatch subj:02001000 ;
	skos:exactMatch <https://www.wikidata.org/entity/Q83267> ;
	skos:broader	medtop:02000000 ;
	skos:narrower	medtop:20000083 ;
	skos:narrower	medtop:20000084 ;
	skos:narrower	medtop:20000086 ;
	skos:narrower	medtop:20000087 ;
	skos:narrower	medtop:20000093 ;
	skos:narrower	medtop:20000095 ;
	skos:narrower	medtop:20000097 ;
	skos:narrower	medtop:20000098 ;
	skos:narrower	medtop:20000099 ;
	skos:narrower	medtop:20000100 ;
	skos:narrower	medtop:20000101 ;
	skos:narrower	medtop:20000103 ;
	skos:narrower	medtop:20000104 ;
	skos:narrower	medtop:20000105 ;
	skos:narrower	medtop:20001196 ;
	skos:narrower	medtop:20001283 ;
	skos:narrower	medtop:20001285 ;
	skos:narrower	medtop:20001313 ;
	skos:narrower	medtop:20001314 ;
	skos:narrower	medtop:20001320 .

medtop:20000083
	rdf:type skos:Concept ;
	skos:prefLabel	"arson"@en-GB ;
	skos:definition	"The intentional setting of fires with criminal intent"@en-GB ;
	skos:inScheme <http://cv.iptc.org/newscodes/mediatopic/>  ;
	ikos:created "2009-10-22T02:00:00+00:00"^^xsd:dateTime ;
	dct:created "2009-10-22T02:00:00+00:00"^^xsd:dateTime ;
	ikos:modified "2021-02-18T12:00:00+00:00"^^xsd:dateTime ;
	dct:modified "2021-02-18T12:00:00+00:00"^^xsd:dateTime  ;
	skos:exactMatch subj:02001008 ;
	skos:exactMatch <https://www.wikidata.org/entity/Q327541> ;
	skos:broader	medtop:20000082 .

medtop:20000084
	rdf:type skos:Concept ;
	skos:prefLabel	"assault"@en-GB ;
	skos:definition	"Physical crime against a person, including battery, brawls and threat of bodily harm"@en-GB ;
	skos:inScheme <http://cv.iptc.org/newscodes/mediatopic/>  ;
	ikos:created "2009-10-22T02:00:00+00:00"^^xsd:dateTime ;
	dct:created "2009-10-22T02:00:00+00:00"^^xsd:dateTime ;
	ikos:modified "2021-02-18T12:00:00+00:00"^^xsd:dateTime ;
	dct:modified "2021-02-18T12:00:00+00:00"^^xsd:dateTime  ;
	skos:exactMatch subj:02001006 ;
	skos:exactMatch <https://www.wikidata.org/entity/Q365680> ;
	skos:broader	medtop:20000082 ;
	skos:narrower	medtop:20000085 .

medtop:20000085
	rdf:type skos:Concept ;
	skos:prefLabel	"sex crime"@en-GB ;
	skos:definition	"Sexual crimes against a person, such as rape, harassment, molestation or groping"@en-GB ;
	skos:inScheme <http://cv.iptc.org/newscodes/mediatopic/>  ;
	ikos:created "2009-10-22T02:00:00+00:00"^^xsd:dateTime ;
	dct:created "2009-10-22T02:00:00+00:00"^^xsd:dateTime ;
	ikos:modified "2021-02-18T12:00:00+00:00"^^xsd:dateTime ;
	dct:modified "2021-02-18T12:00:00+00:00"^^xsd:dateTime  ;
	skos:exactMatch subj:02001005 ;
	skos:exactMatch <https://www.wikidata.org/entity/Q673281> ;
	skos:broader	medtop:20000084 .

medtop:20000086
	rdf:type skos:Concept ;
	skos:prefLabel	"cyber crime"@en-GB ;
	skos:definition	"Criminal activities carried out by means of computers or the internet, such as hacking, phishing scams and identity theft"@en-GB ;
	skos:inScheme <http://cv.iptc.org/newscodes/mediatopic/>  ;
	ikos:created "2009-10-22T02:00:00+00:00"^^xsd:dateTime ;
	dct:created "2009-10-22T02:00:00+00:00"^^xsd:dateTime ;
	ikos:modified "2023-03-31T12:00:00+00:00"^^xsd:dateTime ;
	dct:modified "2023-03-31T12:00:00+00:00"^^xsd:dateTime  ;
	skos:exactMatch subj:02001002 ;
	skos:exactMatch <https://www.wikidata.org/entity/Q29137> ;
	skos:broader	medtop:20000082 .

medtop:20000087
	rdf:type skos:Concept ;
	skos:prefLabel	"corporate crime"@en-GB ;
	skos:definition	"Crimes committed by a corporation or by individuals acting on behalf of a corporation"@en-GB ;
	skos:inScheme <http://cv.iptc.org/newscodes/mediatopic/>  ;
	ikos:created "2009-10-22T02:00:00+00:00"^^xsd:dateTime ;
	dct:created "2009-10-22T02:00:00+00:00"^^xsd:dateTime ;
	ikos:modified "2021-02-18T12:00:00+00:00"^^xsd:dateTime ;
	dct:modified "2021-02-18T12:00:00+00:00"^^xsd:dateTime  ;
	skos:exactMatch subj:02012000 ;
	skos:exactMatch <https://www.wikidata.org/entity/Q5172452> ;
	skos:broader	medtop:20000082 ;
	skos:narrower	medtop:20000088 ;
	skos:narrower	medtop:20000089 ;
	skos:narrower	medtop:20000090 ;
	skos:narrower	medtop:20000091 ;
	skos:narrower	medtop:20000092 ;
	skos:narrower	medtop:20001194 .

medtop:20000088
	rdf:type skos:Concept ;
	skos:prefLabel	"anti-trust crime"@en-GB ;
	skos:definition	"Violations of laws aimed at corporations to promote fair competition for the benefit of consumers"@en-GB ;
	skos:inScheme <http://cv.iptc.org/newscodes/mediatopic/>  ;
	ikos:created "2009-10-22T02:00:00+00:00"^^xsd:dateTime ;
	dct:created "2009-10-22T02:00:00+00:00"^^xsd:dateTime ;
	ikos:modified "2021-05-05T12:00:00+00:00"^^xsd:dateTime ;
	dct:modified "2021-05-05T12:00:00+00:00"^^xsd:dateTime  ;
	skos:exactMatch subj:02012005 ;
	skos:exactMatch <https://www.wikidata.org/entity/Q326498> ;
	skos:broader	medtop:20000087 .

medtop:20000089
	rdf:type skos:Concept ;
	skos:prefLabel	"breach of contract"@en-GB ;
	skos:definition	"The breaking of terms set in a contractual agreement"@en-GB ;
	skos:inScheme <http://cv.iptc.org/newscodes/mediatopic/>  ;
	ikos:created "2009-10-22T02:00:00+00:00"^^xsd:dateTime ;
	dct:created "2009-10-22T02:00:00+00:00"^^xsd:dateTime ;
	ikos:modified "2021-02-18T12:00:00+00:00"^^xsd:dateTime ;
	dct:modified "2021-02-18T12:00:00+00:00"^^xsd:dateTime  ;
	skos:exactMatch subj:02012004 ;
	skos:exactMatch <https://www.wikidata.org/entity/Q562566> ;
	skos:broader	medtop:20000087 .

medtop:20000090
	rdf:type skos:Concept ;
	skos:prefLabel	"embezzlement"@en-GB ;
	skos:definition	"The intentional theft or misuse of money left in one's care or belonging to one's employer"@en-GB ;
	skos:inScheme <http://cv.iptc.org/newscodes/mediatopic/>  ;
	ikos:created "2009-10-22T02:00:00+00:00"^^xsd:dateTime ;
	dct:created "2009-10-22T02:00:00+00:00"^^xsd:dateTime ;
	ikos:modified "2021-02-18T12:00:00+00:00"^^xsd:dateTime ;
	dct:modified "2021-02-18T12:00:00+00:00"^^xsd:dateTime  ;
	skos:exactMatch subj:02012002 ;
	skos:exactMatch <https://www.wikidata.org/entity/Q157833> ;
	skos:broader	medtop:20000087 .

medtop:20000091
	rdf:type skos:Concept ;
	skos:prefLabel	"insider trading"@en-GB ;
	skos:definition	"Trading of stocks by persons having access to internal information not made public at the time"@en-GB ;
	skos:inScheme <http://cv.iptc.org/newscodes/mediatopic/>  ;
	ikos:created "2009-10-22T02:00:00+00:00"^^xsd:dateTime ;
	dct:created "2009-10-22T02:00:00+00:00"^^xsd:dateTime ;
	ikos:modified "2021-02-18T12:00:00+00:00"^^xsd:dateTime ;
	dct:modified "2021-02-18T12:00:00+00:00"^^xsd:dateTime  ;
	skos:exactMatch subj:04016022 ;
	skos:exactMatch <https://www.wikidata.org/entity/Q854623> ;
	skos:broader	medtop:20000087 .

medtop:20000092
	rdf:type skos:Concept ;
	skos:prefLabel	"restraint of trade"@en-GB ;
	skos:definition	"Interference in free competition in business and trade"@en-GB ;
	skos:inScheme <http://cv.iptc.org/newscodes/mediatopic/>  ;
	ikos:created "2009-10-22T02:00:00+00:00"^^xsd:dateTime ;
	dct:created "2009-10-22T02:00:00+00:00"^^xsd:dateTime ;
	ikos:modified "2021-02-18T12:00:00+00:00"^^xsd:dateTime ;
	dct:modified "2021-02-18T12:00:00+00:00"^^xsd:dateTime  ;
	skos:exactMatch subj:02012003 ;
	skos:exactMatch <https://www.wikidata.org/entity/Q7316269> ;
	skos:broader	medtop:20000087 .

medtop:20000093
	rdf:type skos:Concept ;
	skos:prefLabel	"corruption"@en-GB ;
	skos:definition	"Dishonest actions by a person in power in return for pecuniary or personal gain"@en-GB ;
	skos:inScheme <http://cv.iptc.org/newscodes/mediatopic/>  ;
	ikos:created "2009-10-22T02:00:00+00:00"^^xsd:dateTime ;
	dct:created "2009-10-22T02:00:00+00:00"^^xsd:dateTime ;
	ikos:modified "2021-02-18T12:00:00+00:00"^^xsd:dateTime ;
	dct:modified "2021-02-18T12:00:00+00:00"^^xsd:dateTime  ;
	skos:exactMatch subj:02012006 ;
	skos:exactMatch <https://www.wikidata.org/entity/Q366> ;
	skos:broader	medtop:20000082 ;
	skos:narrower	medtop:20000094 .

medtop:20000094
	rdf:type skos:Concept ;
	skos:prefLabel	"bribery"@en-GB ;
	skos:definition	"The giving of money or favours in order to influence the judgment or conduct of a person in a position of power"@en-GB ;
	skos:inScheme <http://cv.iptc.org/newscodes/mediatopic/>  ;
	ikos:created "2009-10-22T02:00:00+00:00"^^xsd:dateTime ;
	dct:created "2009-10-22T02:00:00+00:00"^^xsd:dateTime ;
	ikos:modified "2021-02-18T12:00:00+00:00"^^xsd:dateTime ;
	dct:modified "2021-02-18T12:00:00+00:00"^^xsd:dateTime  ;
	skos:exactMatch subj:02012007 ;
	skos:exactMatch <https://www.wikidata.org/entity/Q187436> ;
	skos:broader	medtop:20000093 .

medtop:20000095
	rdf:type skos:Concept ;
	skos:prefLabel	"drug related crimes"@en-GB ;
	skos:definition	"Illegal activities involving illicit substances, including buying, distribution, selling and smuggling"@en-GB ;
	skos:inScheme <http://cv.iptc.org/newscodes/mediatopic/>  ;
	ikos:created "2009-10-22T02:00:00+00:00"^^xsd:dateTime ;
	dct:created "2009-10-22T02:00:00+00:00"^^xsd:dateTime ;
	ikos:modified "2021-02-18T12:00:00+00:00"^^xsd:dateTime ;
	dct:modified "2021-02-18T12:00:00+00:00"^^xsd:dateTime  ;
	skos:broadMatch subj:02001000 ;
	skos:exactMatch <https://www.wikidata.org/entity/Q1259975> ;
	skos:broader	medtop:20000082 ;
	skos:narrower	medtop:20000096 .

medtop:20000096
	rdf:type skos:Concept ;
	skos:prefLabel	"drug trafficking"@en-GB ;
	skos:definition	"Dealing in illicit often harmful substances"@en-GB ;
	skos:inScheme <http://cv.iptc.org/newscodes/mediatopic/>  ;
	ikos:created "2009-10-22T02:00:00+00:00"^^xsd:dateTime ;
	dct:created "2009-10-22T02:00:00+00:00"^^xsd:dateTime ;
	ikos:modified "2021-02-18T12:00:00+00:00"^^xsd:dateTime ;
	dct:modified "2021-02-18T12:00:00+00:00"^^xsd:dateTime  ;
	skos:exactMatch subj:02001004 ;
	skos:exactMatch <https://www.wikidata.org/entity/Q844924> ;
	skos:broader	medtop:20000095 .

medtop:20000097
	rdf:type skos:Concept ;
	skos:prefLabel	"fraud"@en-GB ;
	skos:definition	"Intentional deception for personal or financial gain"@en-GB ;
	skos:inScheme <http://cv.iptc.org/newscodes/mediatopic/>  ;
	ikos:created "2009-10-22T02:00:00+00:00"^^xsd:dateTime ;
	dct:created "2009-10-22T02:00:00+00:00"^^xsd:dateTime ;
	ikos:modified "2021-02-18T12:00:00+00:00"^^xsd:dateTime ;
	dct:modified "2021-02-18T12:00:00+00:00"^^xsd:dateTime  ;
	skos:exactMatch subj:02012001 ;
	skos:exactMatch <https://www.wikidata.org/entity/Q28813> ;
	skos:broader	medtop:20000082 ;
	skos:narrower	medtop:20001195 .

medtop:20000098
	rdf:type skos:Concept ;
	skos:prefLabel	"hijacking"@en-GB ;
	skos:definition	"Taking over a transportation vehicle by force"@en-GB ;
	skos:inScheme <http://cv.iptc.org/newscodes/mediatopic/>  ;
	ikos:created "2009-10-22T02:00:00+00:00"^^xsd:dateTime ;
	dct:created "2009-10-22T02:00:00+00:00"^^xsd:dateTime ;
	ikos:modified "2021-02-18T12:00:00+00:00"^^xsd:dateTime ;
	dct:modified "2021-02-18T12:00:00+00:00"^^xsd:dateTime  ;
	skos:broadMatch subj:02001000 ;
	skos:exactMatch <https://www.wikidata.org/entity/Q1933595> ;
	skos:broader	medtop:20000082 .

medtop:20000099
	rdf:type skos:Concept ;
	skos:prefLabel	"homicide"@en-GB ;
	skos:definition	"The killing of one person by another, including murder and manslaughter"@en-GB ;
	skos:inScheme <http://cv.iptc.org/newscodes/mediatopic/>  ;
	ikos:created "2009-10-22T02:00:00+00:00"^^xsd:dateTime ;
	dct:created "2009-10-22T02:00:00+00:00"^^xsd:dateTime ;
	ikos:modified "2021-03-31T12:00:00+00:00"^^xsd:dateTime ;
	dct:modified "2021-03-31T12:00:00+00:00"^^xsd:dateTime  ;
	skos:exactMatch subj:02001001 ;
	skos:exactMatch <https://www.wikidata.org/entity/Q149086> ;
	skos:broader	medtop:20000082 .

medtop:20000100
	rdf:type skos:Concept ;
	skos:prefLabel	"kidnapping"@en-GB ;
	skos:definition	"To seize and detain a person against that person's will by unlawful threat, force or fraud"@en-GB ;
	skos:inScheme <http://cv.iptc.org/newscodes/mediatopic/>  ;
	ikos:created "2009-10-22T02:00:00+00:00"^^xsd:dateTime ;
	dct:created "2009-10-22T02:00:00+00:00"^^xsd:dateTime ;
	ikos:modified "2021-02-18T12:00:00+00:00"^^xsd:dateTime ;
	dct:modified "2021-02-18T12:00:00+00:00"^^xsd:dateTime  ;
	skos:exactMatch subj:02001007 ;
	skos:exactMatch <https://www.wikidata.org/entity/Q318296> ;
	skos:broader	medtop:20000082 .

medtop:20000101
	rdf:type skos:Concept ;
	skos:prefLabel	"organised crime"@en-GB ;
	skos:definition	"Crimes committed by gangs or criminal organizations, such as the mafia"@en-GB ;
	skos:inScheme <http://cv.iptc.org/newscodes/mediatopic/>  ;
	ikos:created "2009-10-22T02:00:00+00:00"^^xsd:dateTime ;
	dct:created "2009-10-22T02:00:00+00:00"^^xsd:dateTime ;
	ikos:modified "2021-02-18T12:00:00+00:00"^^xsd:dateTime ;
	dct:modified "2021-02-18T12:00:00+00:00"^^xsd:dateTime  ;
	skos:exactMatch subj:02010000 ;
	skos:exactMatch <https://www.wikidata.org/entity/Q46952> ;
	skos:broader	medtop:20000082 ;
	skos:narrower	medtop:20000102 .

medtop:20000102
	rdf:type skos:Concept ;
	skos:prefLabel	"gang activity"@en-GB ;
	skos:definition	"Criminal activities by groups of individuals, who are allied by common territories, languages or ethnic backgrounds and identify by a common group identity by using a shared name, tattoo, hand sign, clothing style or graffiti symbol"@en-GB ;
	skos:inScheme <http://cv.iptc.org/newscodes/mediatopic/>  ;
	ikos:created "2009-10-22T02:00:00+00:00"^^xsd:dateTime ;
	dct:created "2009-10-22T02:00:00+00:00"^^xsd:dateTime ;
	ikos:modified "2021-05-05T12:00:00+00:00"^^xsd:dateTime ;
	dct:modified "2021-05-05T12:00:00+00:00"^^xsd:dateTime  ;
	skos:exactMatch subj:02001009 ;
	skos:exactMatch <https://www.wikidata.org/entity/Q5185620> ;
	skos:broader	medtop:20000101 .

medtop:20000103
	rdf:type skos:Concept ;
	skos:prefLabel	"terrorism"@en-GB ;
	skos:definition	"Violence against people to create fear in order to achieve political or ideological objectives"@en-GB ;
	skos:inScheme <http://cv.iptc.org/newscodes/mediatopic/>  ;
	ikos:created "2009-10-22T02:00:00+00:00"^^xsd:dateTime ;
	dct:created "2009-10-22T02:00:00+00:00"^^xsd:dateTime ;
	ikos:modified "2021-02-18T12:00:00+00:00"^^xsd:dateTime ;
	dct:modified "2021-02-18T12:00:00+00:00"^^xsd:dateTime  ;
	skos:exactMatch subj:02001010 ;
	skos:exactMatch <https://www.wikidata.org/entity/Q7283> ;
	skos:broader	medtop:20000082 .

medtop:20000104
	rdf:type skos:Concept ;
	skos:prefLabel	"robbery and theft"@en-GB ;
	skos:definition	"The taking of another person's property without their consent, sometimes by force"@en-GB ;
	skos:inScheme <http://cv.iptc.org/newscodes/mediatopic/>  ;
	ikos:created "2009-10-22T02:00:00+00:00"^^xsd:dateTime ;
	dct:created "2009-10-22T02:00:00+00:00"^^xsd:dateTime ;
	ikos:modified "2021-05-05T12:00:00+00:00"^^xsd:dateTime ;
	dct:modified "2021-05-05T12:00:00+00:00"^^xsd:dateTime  ;
	skos:exactMatch subj:02001003 ;
	skos:exactMatch <https://www.wikidata.org/entity/Q2727213> ;
	skos:broader	medtop:20000082 .

medtop:20000105
	rdf:type skos:Concept ;
	skos:prefLabel	"war crime"@en-GB ;
	skos:definition	"Crimes committed during a war or armed conflict, usually against civilians or POWs, including the prosecution of such crimes"@en-GB ;
	skos:inScheme <http://cv.iptc.org/newscodes/mediatopic/>  ;
	ikos:created "2009-10-22T02:00:00+00:00"^^xsd:dateTime ;
	dct:created "2009-10-22T02:00:00+00:00"^^xsd:dateTime ;
	ikos:modified "2023-03-31T12:00:00+00:00"^^xsd:dateTime ;
	dct:modified "2023-03-31T12:00:00+00:00"^^xsd:dateTime  ;
	skos:exactMatch subj:02013000 ;
	skos:exactMatch <https://www.wikidata.org/entity/Q135010> ;
	skos:broader	medtop:20000082 .

medtop:20000106
	rdf:type skos:Concept ;
	skos:prefLabel	"judiciary"@en-GB ;
	skos:definition	"The system of courts of law"@en-GB ;
	skos:inScheme <http://cv.iptc.org/newscodes/mediatopic/>  ;
	ikos:created "2009-10-22T02:00:00+00:00"^^xsd:dateTime ;
	dct:created "2009-10-22T02:00:00+00:00"^^xsd:dateTime ;
	ikos:modified "2021-02-18T12:00:00+00:00"^^xsd:dateTime ;
	dct:modified "2021-02-18T12:00:00+00:00"^^xsd:dateTime  ;
	skos:exactMatch <https://www.wikidata.org/entity/Q105985> ;
	skos:exactMatch subj:02002000 ;
	skos:broader	medtop:02000000 ;
	skos:narrower	medtop:20000107 ;
	skos:narrower	medtop:20000116 ;
	skos:narrower	medtop:20000118 .

medtop:20000107
	rdf:type skos:Concept ;
	skos:prefLabel	"court"@en-GB ;
	skos:definition	"Place where legal cases are heard and decided"@en-GB ;
	skos:inScheme <http://cv.iptc.org/newscodes/mediatopic/>  ;
	ikos:created "2009-10-22T02:00:00+00:00"^^xsd:dateTime ;
	dct:created "2009-10-22T02:00:00+00:00"^^xsd:dateTime ;
	ikos:modified "2021-02-18T12:00:00+00:00"^^xsd:dateTime ;
	dct:modified "2021-02-18T12:00:00+00:00"^^xsd:dateTime  ;
	skos:broadMatch subj:02007000 ;
	skos:exactMatch <https://www.wikidata.org/entity/Q41487> ;
	skos:broader	medtop:20000106 ;
	skos:narrower	medtop:20000108 ;
	skos:narrower	medtop:20000109 ;
	skos:narrower	medtop:20000110 ;
	skos:narrower	medtop:20000111 ;
	skos:narrower	medtop:20001287 .

medtop:20000108
	rdf:type skos:Concept ;
	skos:prefLabel	"appeal (court)"@en-GB ;
	skos:definition	"Process in which parties request a formal change to an official decision"@en-GB ;
	skos:inScheme <http://cv.iptc.org/newscodes/mediatopic/>  ;
	ikos:created "2009-10-22T02:00:00+00:00"^^xsd:dateTime ;
	dct:created "2009-10-22T02:00:00+00:00"^^xsd:dateTime ;
	ikos:modified "2021-02-18T12:00:00+00:00"^^xsd:dateTime ;
	dct:modified "2021-02-18T12:00:00+00:00"^^xsd:dateTime  ;
	skos:broadMatch subj:02000000 ;
	skos:exactMatch <https://www.wikidata.org/entity/Q329777> ;
	skos:broader	medtop:20000107 .

medtop:20000109
	rdf:type skos:Concept ;
	skos:prefLabel	"court administration"@en-GB ;
	skos:definition	"Court clerks, bailiffs, stenographers etc."@en-GB ;
	skos:inScheme <http://cv.iptc.org/newscodes/mediatopic/>  ;
	ikos:created "2009-10-22T02:00:00+00:00"^^xsd:dateTime ;
	dct:created "2009-10-22T02:00:00+00:00"^^xsd:dateTime ;
	ikos:modified "2021-05-05T12:00:00+00:00"^^xsd:dateTime ;
	dct:modified "2021-05-05T12:00:00+00:00"^^xsd:dateTime  ; 
	ikos:retired "2019-10-07T12:00:00+00:00"^^xsd:dateTime ;
	skos:exactMatch subj:02002003 ;
	skos:exactMatch <https://www.wikidata.org/entity/Q12666235> ;
	skos:broader	medtop:20000107 .

medtop:20000110
	rdf:type skos:Concept ;
	skos:prefLabel	"judge"@en-GB ;
	skos:definition	"Official who decides cases in a court of law and passes sentences on those found guilty"@en-GB ;
	skos:inScheme <http://cv.iptc.org/newscodes/mediatopic/>  ;
	ikos:created "2009-10-22T02:00:00+00:00"^^xsd:dateTime ;
	dct:created "2009-10-22T02:00:00+00:00"^^xsd:dateTime ;
	ikos:modified "2021-02-18T12:00:00+00:00"^^xsd:dateTime ;
	dct:modified "2021-02-18T12:00:00+00:00"^^xsd:dateTime  ;
	skos:exactMatch subj:02002002 ;
	skos:exactMatch <https://www.wikidata.org/entity/Q16533> ;
	skos:broader	medtop:20000107 .

medtop:20000111
	rdf:type skos:Concept ;
	skos:prefLabel	"trial (court)"@en-GB ;
	skos:definition	"The process by which evidence is presented and guilt, innocence or culpability is determined"@en-GB ;
	skos:inScheme <http://cv.iptc.org/newscodes/mediatopic/>  ;
	ikos:created "2009-10-22T02:00:00+00:00"^^xsd:dateTime ;
	dct:created "2009-10-22T02:00:00+00:00"^^xsd:dateTime ;
	ikos:modified "2021-02-18T12:00:00+00:00"^^xsd:dateTime ;
	dct:modified "2021-02-18T12:00:00+00:00"^^xsd:dateTime  ;
	skos:exactMatch subj:02008000 ;
	skos:exactMatch <https://www.wikidata.org/entity/Q8016240> ;
	skos:broader	medtop:20000107 ;
	skos:narrower	medtop:20000112 ;
	skos:narrower	medtop:20000113 ;
	skos:narrower	medtop:20000114 ;
	skos:narrower	medtop:20000115 ;
	skos:narrower	medtop:20000134 .

medtop:20000112
	rdf:type skos:Concept ;
	skos:prefLabel	"pre-trial"@en-GB ;
	skos:definition	"Actions that happen before the start of a trial, such as pleas, bail motions, discovery and depositions"@en-GB ;
	skos:inScheme <http://cv.iptc.org/newscodes/mediatopic/>  ;
	ikos:created "2009-10-22T02:00:00+00:00"^^xsd:dateTime ;
	dct:created "2009-10-22T02:00:00+00:00"^^xsd:dateTime ;
	ikos:modified "2021-05-05T12:00:00+00:00"^^xsd:dateTime ;
	dct:modified "2021-05-05T12:00:00+00:00"^^xsd:dateTime  ;
	skos:exactMatch subj:02008003 ;
	skos:exactMatch <https://www.wikidata.org/entity/Q4354932> ;
	skos:broader	medtop:20000111 .

medtop:20000113
	rdf:type skos:Concept ;
	skos:prefLabel	"defendant"@en-GB ;
	skos:definition	"The person on trial"@en-GB ;
	skos:inScheme <http://cv.iptc.org/newscodes/mediatopic/>  ;
	ikos:created "2009-10-22T02:00:00+00:00"^^xsd:dateTime ;
	dct:created "2009-10-22T02:00:00+00:00"^^xsd:dateTime ;
	ikos:modified "2021-02-18T12:00:00+00:00"^^xsd:dateTime ;
	dct:modified "2021-02-18T12:00:00+00:00"^^xsd:dateTime  ; 
	ikos:retired "2019-10-07T12:00:00+00:00"^^xsd:dateTime ;
	skos:exactMatch subj:02009001 ;
	skos:exactMatch <https://www.wikidata.org/entity/Q159394> ;
	skos:broader	medtop:20000111 .

medtop:20000114
	rdf:type skos:Concept ;
	skos:prefLabel	"litigation"@en-GB ;
	skos:definition	"Taking disputed issues to court for settlement by judge and/or jury"@en-GB ;
	skos:inScheme <http://cv.iptc.org/newscodes/mediatopic/>  ;
	ikos:created "2009-10-22T02:00:00+00:00"^^xsd:dateTime ;
	dct:created "2009-10-22T02:00:00+00:00"^^xsd:dateTime ;
	ikos:modified "2021-05-05T12:00:00+00:00"^^xsd:dateTime ;
	dct:modified "2021-05-05T12:00:00+00:00"^^xsd:dateTime  ;
	skos:exactMatch subj:02008001 ;
	skos:exactMatch <https://www.wikidata.org/entity/Q697327> ;
	skos:broader	medtop:20000111 .

medtop:20000115
	rdf:type skos:Concept ;
	skos:prefLabel	"witness"@en-GB ;
	skos:definition	"A person who testifies"@en-GB ;
	skos:inScheme <http://cv.iptc.org/newscodes/mediatopic/>  ;
	ikos:created "2009-10-22T02:00:00+00:00"^^xsd:dateTime ;
	dct:created "2009-10-22T02:00:00+00:00"^^xsd:dateTime ;
	ikos:modified "2021-02-18T12:00:00+00:00"^^xsd:dateTime ;
	dct:modified "2021-02-18T12:00:00+00:00"^^xsd:dateTime  ; 
	ikos:retired "2019-10-07T12:00:00+00:00"^^xsd:dateTime ;
	skos:exactMatch subj:02009002 ;
	skos:exactMatch <https://www.wikidata.org/entity/Q196939> ;
	skos:broader	medtop:20000111 .

medtop:20000116
	rdf:type skos:Concept ;
	skos:prefLabel	"out of court procedures"@en-GB ;
	skos:definition	"Legal issues which are settled outside of court"@en-GB ;
	skos:inScheme <http://cv.iptc.org/newscodes/mediatopic/>  ;
	ikos:created "2009-10-22T02:00:00+00:00"^^xsd:dateTime ;
	dct:created "2009-10-22T02:00:00+00:00"^^xsd:dateTime ;
	ikos:modified "2021-05-05T12:00:00+00:00"^^xsd:dateTime ;
	dct:modified "2021-05-05T12:00:00+00:00"^^xsd:dateTime  ;
	skos:broadMatch subj:02000000 ;
	skos:exactMatch <https://www.wikidata.org/entity/Q167412> ;
	skos:broader	medtop:20000106 ;
	skos:narrower	medtop:20000117 .

medtop:20000117
	rdf:type skos:Concept ;
	skos:prefLabel	"arbitration and mediation"@en-GB ;
	skos:definition	"Resolution of disputed issues by a neutral panel, including conciliation, negotiation and tribunals"@en-GB ;
	skos:inScheme <http://cv.iptc.org/newscodes/mediatopic/>  ;
	ikos:created "2009-10-22T02:00:00+00:00"^^xsd:dateTime ;
	dct:created "2009-10-22T02:00:00+00:00"^^xsd:dateTime ;
	ikos:modified "2021-12-21T12:00:00+00:00"^^xsd:dateTime ;
	dct:modified "2021-12-21T12:00:00+00:00"^^xsd:dateTime  ;
	skos:exactMatch subj:02008002 ;
	skos:exactMatch <https://www.wikidata.org/entity/Q207946> ;
	skos:broader	medtop:20000116 .

medtop:20000118
	rdf:type skos:Concept ;
	skos:prefLabel	"prosecution and prosecutors"@en-GB ;
	skos:definition	"The process of holding a trial against a person who is accused of a crime to determine guilt and the lawyers and legal team who argue that the accused is guilty"@en-GB ;
	skos:inScheme <http://cv.iptc.org/newscodes/mediatopic/>  ;
	ikos:created "2009-10-22T02:00:00+00:00"^^xsd:dateTime ;
	dct:created "2009-10-22T02:00:00+00:00"^^xsd:dateTime ;
	ikos:modified "2021-03-31T12:00:00+00:00"^^xsd:dateTime ;
	dct:modified "2021-03-31T12:00:00+00:00"^^xsd:dateTime  ;
	skos:exactMatch subj:02009000 ;
	skos:exactMatch <https://www.wikidata.org/entity/Q6559173> ;
	skos:broader	medtop:20000106 .

medtop:20000119
	rdf:type skos:Concept ;
	skos:prefLabel	"justice"@en-GB ;
	skos:definition	"The equitable administration of laws and regulations"@en-GB ;
	skos:changeNote	"Retired. Use a more specific term instead."@en-GB ;
	skos:inScheme <http://cv.iptc.org/newscodes/mediatopic/>  ;
	ikos:created "2009-10-22T02:00:00+00:00"^^xsd:dateTime ;
	dct:created "2009-10-22T02:00:00+00:00"^^xsd:dateTime ;
	ikos:modified "2023-10-02T12:00:00+00:00"^^xsd:dateTime ;
	dct:modified "2023-10-02T12:00:00+00:00"^^xsd:dateTime  ; 
	ikos:retired "2023-10-02T12:00:00+00:00"^^xsd:dateTime ;
	skos:exactMatch subj:02007000 ;
	skos:exactMatch <https://www.wikidata.org/entity/Q5167661> ;
	skos:broader	medtop:02000000 .

medtop:20000120
	rdf:type skos:Concept ;
	skos:prefLabel	"civil rights"@en-GB ;
	skos:definition	"Rights of individuals under civil law"@en-GB ;
	skos:inScheme <http://cv.iptc.org/newscodes/mediatopic/>  ;
	ikos:created "2009-10-22T02:00:00+00:00"^^xsd:dateTime ;
	dct:created "2009-10-22T02:00:00+00:00"^^xsd:dateTime ;
	ikos:modified "2021-02-18T12:00:00+00:00"^^xsd:dateTime ;
	dct:modified "2021-02-18T12:00:00+00:00"^^xsd:dateTime  ;
	skos:exactMatch subj:02007001 ;
	skos:exactMatch <https://www.wikidata.org/entity/Q191600> ;
	skos:broader	medtop:20000587 .

medtop:20000121
	rdf:type skos:Concept ;
	skos:prefLabel	"law"@en-GB ;
	skos:definition	"The codification of rules of behaviour"@en-GB ;
	skos:inScheme <http://cv.iptc.org/newscodes/mediatopic/>  ;
	ikos:created "2009-10-22T02:00:00+00:00"^^xsd:dateTime ;
	dct:created "2009-10-22T02:00:00+00:00"^^xsd:dateTime ;
	ikos:modified "2021-02-18T12:00:00+00:00"^^xsd:dateTime ;
	dct:modified "2021-02-18T12:00:00+00:00"^^xsd:dateTime  ;
	skos:exactMatch <https://www.wikidata.org/entity/Q7748> ;
	skos:exactMatch subj:02006000 ;
	skos:broader	medtop:02000000 ;
	skos:narrower	medtop:20000122 ;
	skos:narrower	medtop:20000125 ;
	skos:narrower	medtop:20000126 ;
	skos:narrower	medtop:20001197 .

medtop:20000122
	rdf:type skos:Concept ;
	skos:prefLabel	"civil law"@en-GB ;
	skos:definition	"The system of law focused on private rights and disputes between individuals in such areas as contracts, torts, property, and family law"@en-GB ;
	skos:inScheme <http://cv.iptc.org/newscodes/mediatopic/>  ;
	ikos:created "2009-10-22T02:00:00+00:00"^^xsd:dateTime ;
	dct:created "2009-10-22T02:00:00+00:00"^^xsd:dateTime ;
	ikos:modified "2021-03-31T12:00:00+00:00"^^xsd:dateTime ;
	dct:modified "2021-03-31T12:00:00+00:00"^^xsd:dateTime  ;
	skos:exactMatch subj:02006002 ;
	skos:exactMatch <https://www.wikidata.org/entity/Q222249> ;
	skos:broader	medtop:20000121 ;
	skos:narrower	medtop:20000124 .

medtop:20000123
	rdf:type skos:Concept ;
	skos:prefLabel	"antitrust regulations"@en-GB ;
	skos:definition	"laws to promote competition between companies for the benefit of consumers"@en-GB ;
	skos:inScheme <http://cv.iptc.org/newscodes/mediatopic/>  ;
	ikos:created "2009-10-22T02:00:00+00:00"^^xsd:dateTime ;
	dct:created "2009-10-22T02:00:00+00:00"^^xsd:dateTime ;
	ikos:modified "2021-02-18T12:00:00+00:00"^^xsd:dateTime ;
	dct:modified "2021-02-18T12:00:00+00:00"^^xsd:dateTime  ;
	skos:exactMatch subj:04016004 ;
	skos:exactMatch <https://www.wikidata.org/entity/Q326498> ;
	skos:broader	medtop:20000124 .

medtop:20000124
	rdf:type skos:Concept ;
	skos:prefLabel	"regulations"@en-GB ;
	skos:definition	"laws that guide the conduct and organization of business corporations"@en-GB ;
	skos:inScheme <http://cv.iptc.org/newscodes/mediatopic/>  ;
	ikos:created "2009-10-22T02:00:00+00:00"^^xsd:dateTime ;
	dct:created "2009-10-22T02:00:00+00:00"^^xsd:dateTime ;
	ikos:modified "2021-03-31T12:00:00+00:00"^^xsd:dateTime ;
	dct:modified "2021-03-31T12:00:00+00:00"^^xsd:dateTime  ;
	skos:broadMatch subj:02006002 ;
	skos:exactMatch <https://www.wikidata.org/entity/Q428148> ;
	skos:broader	medtop:20000122 ;
	skos:narrower	medtop:20000123 .

medtop:20000125
	rdf:type skos:Concept ;
	skos:prefLabel	"criminal law"@en-GB ;
	skos:definition	"The system of law concerned with the punishment of those who commit crimes"@en-GB ;
	skos:inScheme <http://cv.iptc.org/newscodes/mediatopic/>  ;
	ikos:created "2009-10-22T02:00:00+00:00"^^xsd:dateTime ;
	dct:created "2009-10-22T02:00:00+00:00"^^xsd:dateTime ;
	ikos:modified "2021-02-18T12:00:00+00:00"^^xsd:dateTime ;
	dct:modified "2021-02-18T12:00:00+00:00"^^xsd:dateTime  ;
	skos:exactMatch subj:02006001 ;
	skos:exactMatch <https://www.wikidata.org/entity/Q146491> ;
	skos:broader	medtop:20000121 .

medtop:20000126
	rdf:type skos:Concept ;
	skos:prefLabel	"international law"@en-GB ;
	skos:definition	"The system of laws embraced by all nations, such as the Geneva Convention and the International Law of the Seas"@en-GB ;
	skos:inScheme <http://cv.iptc.org/newscodes/mediatopic/>  ;
	ikos:created "2009-10-22T02:00:00+00:00"^^xsd:dateTime ;
	dct:created "2009-10-22T02:00:00+00:00"^^xsd:dateTime ;
	ikos:modified "2021-02-18T12:00:00+00:00"^^xsd:dateTime ;
	dct:modified "2021-02-18T12:00:00+00:00"^^xsd:dateTime  ;
	skos:exactMatch subj:02011000 ;
	skos:exactMatch <https://www.wikidata.org/entity/Q4394526> ;
	skos:broader	medtop:20000121 ;
	skos:narrower	medtop:20000127 ;
	skos:narrower	medtop:20000128 .

medtop:20000127
	rdf:type skos:Concept ;
	skos:prefLabel	"extradition"@en-GB ;
	skos:definition	"Legal transfer of criminals or suspects between countries"@en-GB ;
	skos:inScheme <http://cv.iptc.org/newscodes/mediatopic/>  ;
	ikos:created "2009-10-22T02:00:00+00:00"^^xsd:dateTime ;
	dct:created "2009-10-22T02:00:00+00:00"^^xsd:dateTime ;
	ikos:modified "2021-02-18T12:00:00+00:00"^^xsd:dateTime ;
	dct:modified "2021-02-18T12:00:00+00:00"^^xsd:dateTime  ;
	skos:exactMatch subj:02011002 ;
	skos:exactMatch <https://www.wikidata.org/entity/Q210603> ;
	skos:broader	medtop:20000126 .

medtop:20000128
	rdf:type skos:Concept ;
	skos:prefLabel	"international court and tribunal"@en-GB ;
	skos:definition	"The activities of courts under the authority of international organizations or formed by treaties between nations, such as the European Court for Human Rights and International Court of Justice"@en-GB ;
	skos:inScheme <http://cv.iptc.org/newscodes/mediatopic/>  ;
	ikos:created "2009-10-22T02:00:00+00:00"^^xsd:dateTime ;
	dct:created "2009-10-22T02:00:00+00:00"^^xsd:dateTime ;
	ikos:modified "2021-12-17T12:00:00+00:00"^^xsd:dateTime ;
	dct:modified "2021-12-17T12:00:00+00:00"^^xsd:dateTime  ;
	skos:exactMatch subj:02011001 ;
	skos:exactMatch <https://www.wikidata.org/entity/Q1262438> ;
	skos:broader	medtop:20000126 .

medtop:20000129
	rdf:type skos:Concept ;
	skos:prefLabel	"law enforcement"@en-GB ;
	skos:definition	"Agencies that attempt to prevent disobedience to established laws or bring to justice those who disobey those laws"@en-GB ;
	skos:inScheme <http://cv.iptc.org/newscodes/mediatopic/>  ;
	ikos:created "2009-10-22T02:00:00+00:00"^^xsd:dateTime ;
	dct:created "2009-10-22T02:00:00+00:00"^^xsd:dateTime ;
	ikos:modified "2021-02-18T12:00:00+00:00"^^xsd:dateTime ;
	dct:modified "2021-02-18T12:00:00+00:00"^^xsd:dateTime  ;
	skos:exactMatch subj:02003001 ;
	skos:exactMatch <https://www.wikidata.org/entity/Q44554> ;
	skos:broader	medtop:02000000 ;
	skos:narrower	medtop:20000130 ;
	skos:narrower	medtop:20000131 ;
	skos:narrower	medtop:20000133 ;
	skos:narrower	medtop:20001299 .

medtop:20000130
	rdf:type skos:Concept ;
	skos:prefLabel	"arrest"@en-GB ;
	skos:definition	"The detention of a suspect of a crime"@en-GB ;
	skos:inScheme <http://cv.iptc.org/newscodes/mediatopic/>  ;
	ikos:created "2009-10-22T02:00:00+00:00"^^xsd:dateTime ;
	dct:created "2009-10-22T02:00:00+00:00"^^xsd:dateTime ;
	ikos:modified "2021-02-18T12:00:00+00:00"^^xsd:dateTime ;
	dct:modified "2021-02-18T12:00:00+00:00"^^xsd:dateTime  ;
	skos:exactMatch subj:02003003 ;
	skos:exactMatch <https://www.wikidata.org/entity/Q1403016> ;
	skos:broader	medtop:20000129 .

medtop:20000131
	rdf:type skos:Concept ;
	skos:prefLabel	"investigation (criminal)"@en-GB ;
	skos:definition	"Inquiry into an alleged crime, including searching, interviews, interrogations and evidence collection"@en-GB ;
	skos:inScheme <http://cv.iptc.org/newscodes/mediatopic/>  ;
	ikos:created "2009-10-22T02:00:00+00:00"^^xsd:dateTime ;
	dct:created "2009-10-22T02:00:00+00:00"^^xsd:dateTime ;
	ikos:modified "2021-02-18T12:00:00+00:00"^^xsd:dateTime ;
	dct:modified "2021-02-18T12:00:00+00:00"^^xsd:dateTime  ;
	skos:exactMatch subj:02003002 ;
	skos:exactMatch <https://www.wikidata.org/entity/Q1964968> ;
	skos:broader	medtop:20000129 ;
	skos:narrower	medtop:20000132 ;
	skos:narrower	medtop:20001200 .

medtop:20000132
	rdf:type skos:Concept ;
	skos:prefLabel	"missing person"@en-GB ;
	skos:definition	"An adult whose disappearance is possibly not voluntary, or a child whose whereabouts are unknown to the child's legal guardian"@en-GB ;
	skos:inScheme <http://cv.iptc.org/newscodes/mediatopic/>  ;
	ikos:created "2009-10-22T02:00:00+00:00"^^xsd:dateTime ;
	dct:created "2009-10-22T02:00:00+00:00"^^xsd:dateTime ;
	ikos:modified "2021-02-18T12:00:00+00:00"^^xsd:dateTime ;
	dct:modified "2021-02-18T12:00:00+00:00"^^xsd:dateTime  ;
	skos:exactMatch subj:14017000 ;
	skos:exactMatch <https://www.wikidata.org/entity/Q388505> ;
	skos:broader	medtop:20000131 .

medtop:20000133
	rdf:type skos:Concept ;
	skos:prefLabel	"police"@en-GB ;
	skos:definition	"Civil force of a national, regional or local government that is responsible for the prevention and detection of crime and the maintenance of public order"@en-GB ;
	skos:inScheme <http://cv.iptc.org/newscodes/mediatopic/>  ;
	ikos:created "2009-10-22T02:00:00+00:00"^^xsd:dateTime ;
	dct:created "2009-10-22T02:00:00+00:00"^^xsd:dateTime ;
	ikos:modified "2021-03-31T12:00:00+00:00"^^xsd:dateTime ;
	dct:modified "2021-03-31T12:00:00+00:00"^^xsd:dateTime  ;
	skos:exactMatch subj:02003000 ;
	skos:exactMatch <https://www.wikidata.org/entity/Q35535> ;
	skos:broader	medtop:20000129 .

medtop:20000134
	rdf:type skos:Concept ;
	skos:prefLabel	"sentencing (criminal)"@en-GB ;
	skos:definition	"The retribution handed out to those who break laws"@en-GB ;
	skos:inScheme <http://cv.iptc.org/newscodes/mediatopic/>  ;
	ikos:created "2009-10-22T02:00:00+00:00"^^xsd:dateTime ;
	dct:created "2009-10-22T02:00:00+00:00"^^xsd:dateTime ;
	ikos:modified "2021-02-18T12:00:00+00:00"^^xsd:dateTime ;
	dct:modified "2021-02-18T12:00:00+00:00"^^xsd:dateTime  ;
	skos:exactMatch subj:02004000 ;
	skos:exactMatch <https://www.wikidata.org/entity/Q186361> ;
	skos:broader	medtop:20000111 ;
	skos:narrower	medtop:20000135 ;
	skos:narrower	medtop:20000136 ;
	skos:narrower	medtop:20000137 ;
	skos:narrower	medtop:20001198 ;
	skos:narrower	medtop:20001199 .

medtop:20000135
	rdf:type skos:Concept ;
	skos:prefLabel	"capital punishment"@en-GB ;
	skos:definition	"The legally authorised execution of someone as punishment for a crime"@en-GB ;
	skos:inScheme <http://cv.iptc.org/newscodes/mediatopic/>  ;
	ikos:created "2009-10-22T02:00:00+00:00"^^xsd:dateTime ;
	dct:created "2009-10-22T02:00:00+00:00"^^xsd:dateTime ;
	ikos:modified "2021-02-18T12:00:00+00:00"^^xsd:dateTime ;
	dct:modified "2021-02-18T12:00:00+00:00"^^xsd:dateTime  ;
	skos:broadMatch subj:14025005 ;
	skos:exactMatch <https://www.wikidata.org/entity/Q8454> ;
	skos:broader	medtop:20000134 .

medtop:20000136
	rdf:type skos:Concept ;
	skos:prefLabel	"fine (penalty)"@en-GB ;
	skos:definition	"Money that a court of law or other authority decides has to be paid as punishment for a crime or other offence"@en-GB ;
	skos:inScheme <http://cv.iptc.org/newscodes/mediatopic/>  ;
	ikos:created "2009-10-22T02:00:00+00:00"^^xsd:dateTime ;
	dct:created "2009-10-22T02:00:00+00:00"^^xsd:dateTime ;
	ikos:modified "2021-02-18T12:00:00+00:00"^^xsd:dateTime ;
	dct:modified "2021-02-18T12:00:00+00:00"^^xsd:dateTime  ;
	skos:exactMatch subj:02004001 ;
	skos:exactMatch <https://www.wikidata.org/entity/Q2842797> ;
	skos:broader	medtop:20000134 .

medtop:20000137
	rdf:type skos:Concept ;
	skos:prefLabel	"prison"@en-GB ;
	skos:definition	"Facility where people are held as a punishment for a crime they have committed or while awaiting trial"@en-GB ;
	skos:inScheme <http://cv.iptc.org/newscodes/mediatopic/>  ;
	ikos:created "2009-10-22T02:00:00+00:00"^^xsd:dateTime ;
	dct:created "2009-10-22T02:00:00+00:00"^^xsd:dateTime ;
	ikos:modified "2021-03-31T12:00:00+00:00"^^xsd:dateTime ;
	dct:modified "2021-03-31T12:00:00+00:00"^^xsd:dateTime  ;
	skos:exactMatch subj:02005000 ;
	skos:exactMatch <https://www.wikidata.org/entity/Q40357> ;
	skos:broader	medtop:20000134 .

medtop:20000139
	rdf:type skos:Concept ;
	skos:prefLabel	"accident and emergency incident"@en-GB ;
	skos:definition	"A sudden, unexpected event that causes unwanted consequences or requires immediate action"@en-GB ;
	skos:changeNote	"Change Note 2015-08-27: Concept medtop:20000160 was merged into this one as their semantics were not sufficiently different"@en-GB ;
	skos:inScheme <http://cv.iptc.org/newscodes/mediatopic/>  ;
	ikos:created "2009-10-22T02:00:00+00:00"^^xsd:dateTime ;
	dct:created "2009-10-22T02:00:00+00:00"^^xsd:dateTime ;
	ikos:modified "2021-02-18T12:00:00+00:00"^^xsd:dateTime ;
	dct:modified "2021-02-18T12:00:00+00:00"^^xsd:dateTime  ;
	skos:exactMatch <https://www.wikidata.org/entity/Q171558> ;
	skos:exactMatch subj:03013000 ;
	skos:broader	medtop:03000000 ;
	skos:narrower	medtop:20000140 ;
	skos:narrower	medtop:20000141 ;
	skos:narrower	medtop:20000143 ;
	skos:narrower	medtop:20000161 ;
	skos:narrower	medtop:20001321 .

medtop:20000140
	rdf:type skos:Concept ;
	skos:prefLabel	"explosion accident and incident"@en-GB ;
	skos:definition	"Explosions caused by an accidental, non-combat, or non-terrorism source. Also use when the source of the explosion is non-specified or unknown"@en-GB ;
	skos:changeNote	"Change Note 2015-08-27: English name changed"@en-GB ;
	skos:inScheme <http://cv.iptc.org/newscodes/mediatopic/>  ;
	ikos:created "2009-10-22T02:00:00+00:00"^^xsd:dateTime ;
	dct:created "2009-10-22T02:00:00+00:00"^^xsd:dateTime ;
	ikos:modified "2021-05-05T12:00:00+00:00"^^xsd:dateTime ;
	dct:modified "2021-05-05T12:00:00+00:00"^^xsd:dateTime  ;
	skos:exactMatch subj:03014001 ;
	skos:exactMatch <https://www.wikidata.org/entity/Q179057> ;
	skos:broader	medtop:20000139 .

medtop:20000141
	rdf:type skos:Concept ;
	skos:prefLabel	"industrial accident and incident"@en-GB ;
	skos:definition	"Any unplanned event or mishap in an industrial setting that result in injuries to people and damage to property or the environment"@en-GB ;
	skos:changeNote	"Change Note 2015-08-27: English name changed"@en-GB ;
	skos:inScheme <http://cv.iptc.org/newscodes/mediatopic/>  ;
	ikos:created "2009-10-22T02:00:00+00:00"^^xsd:dateTime ;
	dct:created "2009-10-22T02:00:00+00:00"^^xsd:dateTime ;
	ikos:modified "2021-05-05T12:00:00+00:00"^^xsd:dateTime ;
	dct:modified "2021-05-05T12:00:00+00:00"^^xsd:dateTime  ;
	skos:exactMatch subj:03006000 ;
	skos:exactMatch <https://www.wikidata.org/entity/Q629257> ;
	skos:broader	medtop:20000139 ;
	skos:narrower	medtop:20000142 .

medtop:20000142
	rdf:type skos:Concept ;
	skos:prefLabel	"nuclear accident and incident"@en-GB ;
	skos:definition	"Any unplanned event that causes unwanted consequences involving radioactive materials"@en-GB ;
	skos:changeNote	"Change Note 2015-08-27: English name changed"@en-GB ;
	skos:inScheme <http://cv.iptc.org/newscodes/mediatopic/>  ;
	ikos:created "2009-10-22T02:00:00+00:00"^^xsd:dateTime ;
	dct:created "2009-10-22T02:00:00+00:00"^^xsd:dateTime ;
	ikos:modified "2021-02-18T12:00:00+00:00"^^xsd:dateTime ;
	dct:modified "2021-02-18T12:00:00+00:00"^^xsd:dateTime  ;
	skos:exactMatch subj:03008000 ;
	skos:exactMatch <https://www.wikidata.org/entity/Q1620824> ;
	skos:broader	medtop:20000141 .

medtop:20000143
	rdf:type skos:Concept ;
	skos:prefLabel	"transportation accident and incident"@en-GB ;
	skos:definition	"An accident or incident involving one or more vehicles"@en-GB ;
	skos:changeNote	"Change Note 2015-08-27: Concept medtop:20000162 was merged into this one as their semantics were not sufficiently different"@en-GB ;
	skos:inScheme <http://cv.iptc.org/newscodes/mediatopic/>  ;
	ikos:created "2009-10-22T02:00:00+00:00"^^xsd:dateTime ;
	dct:created "2009-10-22T02:00:00+00:00"^^xsd:dateTime ;
	ikos:modified "2021-05-05T12:00:00+00:00"^^xsd:dateTime ;
	dct:modified "2021-05-05T12:00:00+00:00"^^xsd:dateTime  ;
	skos:exactMatch subj:03010000 ;
	skos:exactMatch <https://www.wikidata.org/entity/Q11822042> ;
	skos:broader	medtop:20000139 ;
	skos:narrower	medtop:20000144 ;
	skos:narrower	medtop:20000145 ;
	skos:narrower	medtop:20000146 ;
	skos:narrower	medtop:20000147 .

medtop:20000144
	rdf:type skos:Concept ;
	skos:prefLabel	"air and space accident and incident"@en-GB ;
	skos:definition	"An accident or incident involving aircrafts or spacecrafts"@en-GB ;
	skos:changeNote	"Change Note 2015-08-27: Concept medtop:20000163 was merged into this one as their semantics were not sufficiently different"@en-GB ;
	skos:inScheme <http://cv.iptc.org/newscodes/mediatopic/>  ;
	ikos:created "2009-10-22T02:00:00+00:00"^^xsd:dateTime ;
	dct:created "2009-10-22T02:00:00+00:00"^^xsd:dateTime ;
	ikos:modified "2021-02-18T12:00:00+00:00"^^xsd:dateTime ;
	dct:modified "2021-02-18T12:00:00+00:00"^^xsd:dateTime  ;
	skos:exactMatch subj:03010003 ;
	skos:exactMatch <https://www.wikidata.org/entity/Q744913> ;
	skos:broader	medtop:20000143 .

medtop:20000145
	rdf:type skos:Concept ;
	skos:prefLabel	"maritime accident and incident"@en-GB ;
	skos:definition	"An accident or incident involving marine vessels."@en-GB ;
	skos:changeNote	"Change Note 2015-08-27: Concept medtop:20000164 was merged into this one as their semantics were not sufficiently different"@en-GB ;
	skos:inScheme <http://cv.iptc.org/newscodes/mediatopic/>  ;
	ikos:created "2009-10-22T02:00:00+00:00"^^xsd:dateTime ;
	dct:created "2009-10-22T02:00:00+00:00"^^xsd:dateTime ;
	ikos:modified "2021-02-18T12:00:00+00:00"^^xsd:dateTime ;
	dct:modified "2021-02-18T12:00:00+00:00"^^xsd:dateTime  ;
	skos:exactMatch subj:03010004 ;
	skos:exactMatch <https://www.wikidata.org/entity/Q2235325> ;
	skos:broader	medtop:20000143 .

medtop:20000146
	rdf:type skos:Concept ;
	skos:prefLabel	"railway accident and incident"@en-GB ;
	skos:definition	"An accident or incident involving trains."@en-GB ;
	skos:changeNote	"Change Note 2015-08-27: Concept medtop:20000165 was merged into this one as their semantics were not sufficiently different. Note 2016-08-24: typo in name fixed"@en-GB ;
	skos:inScheme <http://cv.iptc.org/newscodes/mediatopic/>  ;
	ikos:created "2009-10-22T02:00:00+00:00"^^xsd:dateTime ;
	dct:created "2009-10-22T02:00:00+00:00"^^xsd:dateTime ;
	ikos:modified "2021-02-18T12:00:00+00:00"^^xsd:dateTime ;
	dct:modified "2021-02-18T12:00:00+00:00"^^xsd:dateTime  ;
	skos:exactMatch subj:03010002 ;
	skos:exactMatch <https://www.wikidata.org/entity/Q19403959> ;
	skos:broader	medtop:20000143 .

medtop:20000147
	rdf:type skos:Concept ;
	skos:prefLabel	"road accident and incident"@en-GB ;
	skos:definition	"An accident or incident involving road vehicles."@en-GB ;
	skos:changeNote	"Change Note 2015-08-27: Concept medtop:20000166 was merged into this one as their semantics were not sufficiently different"@en-GB ;
	skos:inScheme <http://cv.iptc.org/newscodes/mediatopic/>  ;
	ikos:created "2009-10-22T02:00:00+00:00"^^xsd:dateTime ;
	dct:created "2009-10-22T02:00:00+00:00"^^xsd:dateTime ;
	ikos:modified "2021-02-18T12:00:00+00:00"^^xsd:dateTime ;
	dct:modified "2021-02-18T12:00:00+00:00"^^xsd:dateTime  ;
	skos:exactMatch subj:03010001 ;
	skos:exactMatch <https://www.wikidata.org/entity/Q9687> ;
	skos:broader	medtop:20000143 ;
	skos:narrower	medtop:20001201 .

medtop:20000148
	rdf:type skos:Concept ;
	skos:prefLabel	"disaster"@en-GB ;
	skos:definition	"A sudden, unplanned event that causes great damage or loss of life, such as an accident or a natural catastrophe"@en-GB ;
	skos:inScheme <http://cv.iptc.org/newscodes/mediatopic/>  ;
	ikos:created "2009-10-22T02:00:00+00:00"^^xsd:dateTime ;
	dct:created "2009-10-22T02:00:00+00:00"^^xsd:dateTime ;
	ikos:modified "2021-02-18T12:00:00+00:00"^^xsd:dateTime ;
	dct:modified "2021-02-18T12:00:00+00:00"^^xsd:dateTime  ;
	skos:exactMatch <https://www.wikidata.org/entity/Q3839081> ;
	skos:exactMatch subj:03015000 ;
	skos:broader	medtop:03000000 ;
	skos:narrower	medtop:20000149 ;
	skos:narrower	medtop:20000150 ;
	skos:narrower	medtop:20000151 .

medtop:20000149
	rdf:type skos:Concept ;
	skos:prefLabel	"famine"@en-GB ;
	skos:definition	"Severe lack of food for a large population"@en-GB ;
	skos:inScheme <http://cv.iptc.org/newscodes/mediatopic/>  ;
	ikos:created "2009-10-22T02:00:00+00:00"^^xsd:dateTime ;
	dct:created "2009-10-22T02:00:00+00:00"^^xsd:dateTime ;
	ikos:modified "2021-02-18T12:00:00+00:00"^^xsd:dateTime ;
	dct:modified "2021-02-18T12:00:00+00:00"^^xsd:dateTime  ;
	skos:exactMatch subj:03003000 ;
	skos:exactMatch <https://www.wikidata.org/entity/Q168247> ;
	skos:broader	medtop:20000148 .

medtop:20000150
	rdf:type skos:Concept ;
	skos:prefLabel	"fire"@en-GB ;
	skos:definition	"Fires started by an accidental or unknown source. For wildfires, use wildfire. For fires started with a criminal intent, use arson."@en-GB ;
	skos:inScheme <http://cv.iptc.org/newscodes/mediatopic/>  ;
	ikos:created "2009-10-22T02:00:00+00:00"^^xsd:dateTime ;
	dct:created "2009-10-22T02:00:00+00:00"^^xsd:dateTime ;
	ikos:modified "2021-02-18T12:00:00+00:00"^^xsd:dateTime ;
	dct:modified "2021-02-18T12:00:00+00:00"^^xsd:dateTime  ;
	skos:exactMatch subj:03004000 ;
	skos:exactMatch <https://www.wikidata.org/entity/Q3196> ;
	skos:broader	medtop:20000148 ;
	skos:narrower	medtop:20001202 .

medtop:20000151
	rdf:type skos:Concept ;
	skos:prefLabel	"natural disaster"@en-GB ;
	skos:definition	"Destructive incidents caused by nature, such as earthquakes and floods"@en-GB ;
	skos:inScheme <http://cv.iptc.org/newscodes/mediatopic/>  ;
	ikos:created "2009-10-22T02:00:00+00:00"^^xsd:dateTime ;
	dct:created "2009-10-22T02:00:00+00:00"^^xsd:dateTime ;
	ikos:modified "2021-02-18T12:00:00+00:00"^^xsd:dateTime ;
	dct:modified "2021-02-18T12:00:00+00:00"^^xsd:dateTime  ;
	skos:exactMatch subj:03015001 ;
	skos:exactMatch <https://www.wikidata.org/entity/Q8065> ;
	skos:broader	medtop:20000148 ;
	skos:narrower	medtop:20000152 ;
	skos:narrower	medtop:20000153 ;
	skos:narrower	medtop:20000154 ;
	skos:narrower	medtop:20000155 ;
	skos:narrower	medtop:20000157 ;
	skos:narrower	medtop:20000159 ;
	skos:narrower	medtop:20001353 .

medtop:20000152
	rdf:type skos:Concept ;
	skos:prefLabel	"drought"@en-GB ;
	skos:definition	"A severe lack of water over a period of time"@en-GB ;
	skos:inScheme <http://cv.iptc.org/newscodes/mediatopic/>  ;
	ikos:created "2009-10-22T02:00:00+00:00"^^xsd:dateTime ;
	dct:created "2009-10-22T02:00:00+00:00"^^xsd:dateTime ;
	ikos:modified "2021-02-18T12:00:00+00:00"^^xsd:dateTime ;
	dct:modified "2021-02-18T12:00:00+00:00"^^xsd:dateTime  ;
	skos:exactMatch subj:03001000 ;
	skos:exactMatch <https://www.wikidata.org/entity/Q43059> ;
	skos:broader	medtop:20000151 .

medtop:20000153
	rdf:type skos:Concept ;
	skos:prefLabel	"earthquake"@en-GB ;
	skos:definition	"The shifting of the tectonic plates of the Earth, creating in some cases damage to structures"@en-GB ;
	skos:inScheme <http://cv.iptc.org/newscodes/mediatopic/>  ;
	ikos:created "2009-10-22T02:00:00+00:00"^^xsd:dateTime ;
	dct:created "2009-10-22T02:00:00+00:00"^^xsd:dateTime ;
	ikos:modified "2021-02-18T12:00:00+00:00"^^xsd:dateTime ;
	dct:modified "2021-02-18T12:00:00+00:00"^^xsd:dateTime  ;
	skos:exactMatch subj:03002000 ;
	skos:exactMatch <https://www.wikidata.org/entity/Q7944> ;
	skos:broader	medtop:20000151 .

medtop:20000154
	rdf:type skos:Concept ;
	skos:prefLabel	"flood"@en-GB ;
	skos:definition	"Surfeit of water, caused by heavy rains or melting snow, usually in places where it's not wanted"@en-GB ;
	skos:inScheme <http://cv.iptc.org/newscodes/mediatopic/>  ;
	ikos:created "2009-10-22T02:00:00+00:00"^^xsd:dateTime ;
	dct:created "2009-10-22T02:00:00+00:00"^^xsd:dateTime ;
	ikos:modified "2021-02-18T12:00:00+00:00"^^xsd:dateTime ;
	dct:modified "2021-02-18T12:00:00+00:00"^^xsd:dateTime  ;
	skos:exactMatch subj:03005000 ;
	skos:exactMatch <https://www.wikidata.org/entity/Q8068> ;
	skos:broader	medtop:20000151 .

medtop:20000155
	rdf:type skos:Concept ;
	skos:prefLabel	"landslide"@en-GB ;
	skos:definition	"Sudden dislodging of massive amounts of snow or soil"@en-GB ;
	skos:inScheme <http://cv.iptc.org/newscodes/mediatopic/>  ;
	ikos:created "2009-10-22T02:00:00+00:00"^^xsd:dateTime ;
	dct:created "2009-10-22T02:00:00+00:00"^^xsd:dateTime ;
	ikos:modified "2021-02-18T12:00:00+00:00"^^xsd:dateTime ;
	dct:modified "2021-02-18T12:00:00+00:00"^^xsd:dateTime  ;
	skos:broadMatch subj:03015002 ;
	skos:exactMatch <https://www.wikidata.org/entity/Q167903> ;
	skos:broader	medtop:20000151 ;
	skos:narrower	medtop:20000156 .

medtop:20000156
	rdf:type skos:Concept ;
	skos:prefLabel	"avalanche"@en-GB ;
	skos:definition	"A sudden fall of snow, ice, rock, or mud down the side of a mountain"@en-GB ;
	skos:inScheme <http://cv.iptc.org/newscodes/mediatopic/>  ;
	ikos:created "2009-10-22T02:00:00+00:00"^^xsd:dateTime ;
	dct:created "2009-10-22T02:00:00+00:00"^^xsd:dateTime ;
	ikos:modified "2021-02-18T12:00:00+00:00"^^xsd:dateTime ;
	dct:modified "2021-02-18T12:00:00+00:00"^^xsd:dateTime  ;
	skos:broadMatch subj:03015002 ;
	skos:exactMatch <https://www.wikidata.org/entity/Q7935> ;
	skos:broader	medtop:20000155 .

medtop:20000157
	rdf:type skos:Concept ;
	skos:prefLabel	"meteorological disaster"@en-GB ;
	skos:definition	"A weather-related disaster"@en-GB ;
	skos:inScheme <http://cv.iptc.org/newscodes/mediatopic/>  ;
	ikos:created "2009-10-22T02:00:00+00:00"^^xsd:dateTime ;
	dct:created "2009-10-22T02:00:00+00:00"^^xsd:dateTime ;
	ikos:modified "2021-02-18T12:00:00+00:00"^^xsd:dateTime ;
	dct:modified "2021-02-18T12:00:00+00:00"^^xsd:dateTime  ;
	skos:exactMatch subj:03007000 ;
	skos:exactMatch <https://www.wikidata.org/entity/Q6823473> ;
	skos:broader	medtop:20000151 ;
	skos:narrower	medtop:20000158 ;
	skos:narrower	medtop:20001280 .

medtop:20000158
	rdf:type skos:Concept ;
	skos:prefLabel	"windstorms"@en-GB ;
	skos:definition	"A storm with very strong wind but little or no rain or snow"@en-GB ;
	skos:inScheme <http://cv.iptc.org/newscodes/mediatopic/>  ;
	ikos:created "2009-10-22T02:00:00+00:00"^^xsd:dateTime ;
	dct:created "2009-10-22T02:00:00+00:00"^^xsd:dateTime ;
	ikos:modified "2021-05-05T12:00:00+00:00"^^xsd:dateTime ;
	dct:modified "2021-05-05T12:00:00+00:00"^^xsd:dateTime  ;
	skos:exactMatch subj:03007001 ;
	skos:exactMatch <https://www.wikidata.org/entity/Q148942> ;
	skos:broader	medtop:20000157 .

medtop:20000159
	rdf:type skos:Concept ;
	skos:prefLabel	"volcanic eruption"@en-GB ;
	skos:definition	"A rupture in the crust of the Earth allowing molten material to escape to the surface"@en-GB ;
	skos:inScheme <http://cv.iptc.org/newscodes/mediatopic/>  ;
	ikos:created "2009-10-22T02:00:00+00:00"^^xsd:dateTime ;
	dct:created "2009-10-22T02:00:00+00:00"^^xsd:dateTime ;
	ikos:modified "2021-07-12T12:00:00+00:00"^^xsd:dateTime ;
	dct:modified "2021-07-12T12:00:00+00:00"^^xsd:dateTime  ;
	skos:exactMatch subj:03011000 ;
	skos:exactMatch <https://www.wikidata.org/entity/Q7692360> ;
	skos:broader	medtop:20000151 .

medtop:20000160
	rdf:type skos:Concept ;
	skos:prefLabel	"emergency incident"@en-GB ;
	skos:definition	"A sudden, unexpected event that requires immediate action to prevent serious consequences"@en-GB ;
	skos:changeNote	"Change Note 2015-08-27: This concept was merged into concept medtop:20000139 as their semantics were not sufficiently different"@en-GB ;
	skos:inScheme <http://cv.iptc.org/newscodes/mediatopic/>  ;
	ikos:created "2009-10-22T02:00:00+00:00"^^xsd:dateTime ;
	dct:created "2009-10-22T02:00:00+00:00"^^xsd:dateTime ;
	ikos:modified "2021-12-21T12:00:00+00:00"^^xsd:dateTime ;
	dct:modified "2021-12-21T12:00:00+00:00"^^xsd:dateTime  ; 
	ikos:retired "2015-08-27T12:00:00+00:00"^^xsd:dateTime ;
	skos:exactMatch subj:03014000 ;
	skos:exactMatch <https://www.wikidata.org/entity/Q5070802> ;
	skos:broader	medtop:03000000 ;
	skos:narrower	medtop:20000162 .

medtop:20000161
	rdf:type skos:Concept ;
	skos:prefLabel	"structural failure"@en-GB ;
	skos:definition	"The unexpected collapse of a building, bridge or other structure"@en-GB ;
	skos:changeNote	"Change Note 2015-08-27: broader term changed"@en-GB ;
	skos:inScheme <http://cv.iptc.org/newscodes/mediatopic/>  ;
	ikos:created "2009-10-22T02:00:00+00:00"^^xsd:dateTime ;
	dct:created "2009-10-22T02:00:00+00:00"^^xsd:dateTime ;
	ikos:modified "2021-02-18T12:00:00+00:00"^^xsd:dateTime ;
	dct:modified "2021-02-18T12:00:00+00:00"^^xsd:dateTime  ;
	skos:exactMatch subj:03006001 ;
	skos:exactMatch <https://www.wikidata.org/entity/Q1309431> ;
	skos:broader	medtop:20000139 .

medtop:20000162
	rdf:type skos:Concept ;
	skos:prefLabel	"transport incident"@en-GB ;
	skos:definition	"An incident involving one or more vehicles"@en-GB ;
	skos:changeNote	"Change Note 2015-08-27: This concept was merged into concept medtop:20000143 as their semantics were not sufficiently different"@en-GB ;
	skos:inScheme <http://cv.iptc.org/newscodes/mediatopic/>  ;
	ikos:created "2009-10-22T02:00:00+00:00"^^xsd:dateTime ;
	dct:created "2009-10-22T02:00:00+00:00"^^xsd:dateTime ;
	ikos:modified "2021-12-21T12:00:00+00:00"^^xsd:dateTime ;
	dct:modified "2021-12-21T12:00:00+00:00"^^xsd:dateTime  ; 
	ikos:retired "2015-08-27T12:00:00+00:00"^^xsd:dateTime ;
	skos:broadMatch subj:03010000 ;
	skos:exactMatch <https://www.wikidata.org/entity/Q11822042> ;
	skos:broader	medtop:20000160 ;
	skos:narrower	medtop:20000163 ;
	skos:narrower	medtop:20000164 ;
	skos:narrower	medtop:20000165 ;
	skos:narrower	medtop:20000166 .

medtop:20000163
	rdf:type skos:Concept ;
	skos:prefLabel	"air and space incident"@en-GB ;
	skos:definition	"Incident involving craft in air or space."@en-GB ;
	skos:changeNote	"Change Note 2015-08-27: This concept was merged into concept medtop:20000144 as their semantics were not sufficiently different"@en-GB ;
	skos:inScheme <http://cv.iptc.org/newscodes/mediatopic/>  ;
	ikos:created "2009-10-22T02:00:00+00:00"^^xsd:dateTime ;
	dct:created "2009-10-22T02:00:00+00:00"^^xsd:dateTime ;
	ikos:modified "2021-12-21T12:00:00+00:00"^^xsd:dateTime ;
	dct:modified "2021-12-21T12:00:00+00:00"^^xsd:dateTime  ; 
	ikos:retired "2015-08-27T12:00:00+00:00"^^xsd:dateTime ;
	skos:broadMatch subj:03010003 ;
	skos:broader	medtop:20000162 .

medtop:20000164
	rdf:type skos:Concept ;
	skos:prefLabel	"maritime incident"@en-GB ;
	skos:definition	"Incident involving marine vessels."@en-GB ;
	skos:changeNote	"Change Note 2015-08-27: This concept was merged into concept medtop:20000145 as their semantics were not sufficiently different"@en-GB ;
	skos:inScheme <http://cv.iptc.org/newscodes/mediatopic/>  ;
	ikos:created "2009-10-22T02:00:00+00:00"^^xsd:dateTime ;
	dct:created "2009-10-22T02:00:00+00:00"^^xsd:dateTime ;
	ikos:modified "2021-12-21T12:00:00+00:00"^^xsd:dateTime ;
	dct:modified "2021-12-21T12:00:00+00:00"^^xsd:dateTime  ; 
	ikos:retired "2015-08-27T12:00:00+00:00"^^xsd:dateTime ;
	skos:broadMatch subj:03010004 ;
	skos:broader	medtop:20000162 .

medtop:20000165
	rdf:type skos:Concept ;
	skos:prefLabel	"railway incident"@en-GB ;
	skos:definition	"Incident involving trains."@en-GB ;
	skos:changeNote	"Change Note 2015-08-27: This concept was merged into concept medtop:20000146 as their semantics were not sufficiently different"@en-GB ;
	skos:inScheme <http://cv.iptc.org/newscodes/mediatopic/>  ;
	ikos:created "2009-10-22T02:00:00+00:00"^^xsd:dateTime ;
	dct:created "2009-10-22T02:00:00+00:00"^^xsd:dateTime ;
	ikos:modified "2021-12-21T12:00:00+00:00"^^xsd:dateTime ;
	dct:modified "2021-12-21T12:00:00+00:00"^^xsd:dateTime  ; 
	ikos:retired "2015-08-27T12:00:00+00:00"^^xsd:dateTime ;
	skos:broadMatch subj:03010002 ;
	skos:exactMatch <https://www.wikidata.org/entity/Q4202290> ;
	skos:broader	medtop:20000162 .

medtop:20000166
	rdf:type skos:Concept ;
	skos:prefLabel	"road incident"@en-GB ;
	skos:definition	"Incident involving road vehicles."@en-GB ;
	skos:changeNote	"Change Note 2015-08-27: This concept was merged into concept medtop:20000147 as their semantics were not sufficiently different"@en-GB ;
	skos:inScheme <http://cv.iptc.org/newscodes/mediatopic/>  ;
	ikos:created "2009-10-22T02:00:00+00:00"^^xsd:dateTime ;
	dct:created "2009-10-22T02:00:00+00:00"^^xsd:dateTime ;
	ikos:modified "2021-12-21T12:00:00+00:00"^^xsd:dateTime ;
	dct:modified "2021-12-21T12:00:00+00:00"^^xsd:dateTime  ; 
	ikos:retired "2015-08-27T12:00:00+00:00"^^xsd:dateTime ;
	skos:broadMatch subj:03010001 ;
	skos:exactMatch <https://www.wikidata.org/entity/Q9687> ;
	skos:broader	medtop:20000162 .

medtop:20000167
	rdf:type skos:Concept ;
	skos:prefLabel	"emergency planning"@en-GB ;
	skos:definition	"Planning for actions to deal with sudden, unplanned events"@en-GB ;
	skos:changeNote	"2019-12-11: Retired. Use medtop:20000168 emergency response instead"@en-GB ;
	skos:inScheme <http://cv.iptc.org/newscodes/mediatopic/>  ;
	ikos:created "2009-10-22T02:00:00+00:00"^^xsd:dateTime ;
	dct:created "2009-10-22T02:00:00+00:00"^^xsd:dateTime ;
	ikos:modified "2021-02-18T12:00:00+00:00"^^xsd:dateTime ;
	dct:modified "2021-02-18T12:00:00+00:00"^^xsd:dateTime  ; 
	ikos:retired "2019-12-11T12:00:00+00:00"^^xsd:dateTime ;
	skos:exactMatch subj:03016000 ;
	skos:exactMatch <https://www.wikidata.org/entity/Q1460420> ;
	skos:broader	medtop:03000000 .

medtop:20000168
	rdf:type skos:Concept ;
	skos:prefLabel	"emergency response"@en-GB ;
	skos:definition	"The planning and efforts made by people and organizations to help victims of a sudden, unplanned event, natural disaster or crisis"@en-GB ;
	skos:inScheme <http://cv.iptc.org/newscodes/mediatopic/>  ;
	ikos:created "2009-10-22T02:00:00+00:00"^^xsd:dateTime ;
	dct:created "2009-10-22T02:00:00+00:00"^^xsd:dateTime ;
	ikos:modified "2021-02-18T12:00:00+00:00"^^xsd:dateTime ;
	dct:modified "2021-02-18T12:00:00+00:00"^^xsd:dateTime  ;
	skos:broadMatch subj:03012000 ;
	skos:exactMatch <https://www.wikidata.org/entity/Q55692637> ;
	skos:broader	medtop:03000000 .

medtop:20000170
	rdf:type skos:Concept ;
	skos:prefLabel	"business information"@en-GB ;
	skos:definition	"Information about individual business entities, including companies, corporations, charities"@en-GB ;
	skos:inScheme <http://cv.iptc.org/newscodes/mediatopic/>  ;
	ikos:created "2009-10-22T02:00:00+00:00"^^xsd:dateTime ;
	dct:created "2009-10-22T02:00:00+00:00"^^xsd:dateTime ;
	ikos:modified "2021-05-05T12:00:00+00:00"^^xsd:dateTime ;
	dct:modified "2021-05-05T12:00:00+00:00"^^xsd:dateTime  ;
	skos:exactMatch subj:04016000 ;
	skos:exactMatch <https://www.wikidata.org/entity/Q1391314> ;
	skos:broader	medtop:04000000 ;
	skos:narrower	medtop:20000171 ;
	skos:narrower	medtop:20000183 ;
	skos:narrower	medtop:20000188 ;
	skos:narrower	medtop:20000192 ;
	skos:narrower	medtop:20000199 ;
	skos:narrower	medtop:20001365 ;
	skos:narrower	medtop:20001366 .

medtop:20000171
	rdf:type skos:Concept ;
	skos:prefLabel	"business finance"@en-GB ;
	skos:definition	"A business entity's finances"@en-GB ;
	skos:inScheme <http://cv.iptc.org/newscodes/mediatopic/>  ;
	ikos:created "2009-10-22T02:00:00+00:00"^^xsd:dateTime ;
	dct:created "2009-10-22T02:00:00+00:00"^^xsd:dateTime ;
	ikos:modified "2023-03-31T12:00:00+00:00"^^xsd:dateTime ;
	dct:modified "2023-03-31T12:00:00+00:00"^^xsd:dateTime  ; 
	ikos:retired "2023-03-31T12:00:00+00:00"^^xsd:dateTime ;
	skos:broadMatch subj:04000000 ;
	skos:broader	medtop:20000170 ;
	skos:narrower	medtop:20000173 .

medtop:20000172
	rdf:type skos:Concept ;
	skos:prefLabel	"accounting and audit"@en-GB ;
	skos:definition	"Changes regarding applicable accounting rules and the audit of accounting"@en-GB ;
	skos:changeNote	"Retired. Use medtop:20001365 business reporting and performance or medtop:20000272 accountancy and auditing instead."@en-GB ;
	skos:inScheme <http://cv.iptc.org/newscodes/mediatopic/>  ;
	ikos:created "2009-10-22T02:00:00+00:00"^^xsd:dateTime ;
	dct:created "2009-10-22T02:00:00+00:00"^^xsd:dateTime ;
	ikos:modified "2023-03-31T12:00:00+00:00"^^xsd:dateTime ;
	dct:modified "2023-03-31T12:00:00+00:00"^^xsd:dateTime  ; 
	ikos:retired "2023-03-31T12:00:00+00:00"^^xsd:dateTime ;
	skos:exactMatch subj:04016001 ;
	skos:broader	medtop:20001365 .

medtop:20000173
	rdf:type skos:Concept ;
	skos:prefLabel	"analysts comment"@en-GB ;
	skos:definition	"Stock analyst comments, analysis and recommendations."@en-GB ;
	skos:changeNote	"Retired. Use medtop:20000396 stocks and securities and/or genre:Analysis instead."@en-GB ;
	skos:inScheme <http://cv.iptc.org/newscodes/mediatopic/>  ;
	ikos:created "2009-10-22T02:00:00+00:00"^^xsd:dateTime ;
	dct:created "2009-10-22T02:00:00+00:00"^^xsd:dateTime ;
	ikos:modified "2023-03-31T12:00:00+00:00"^^xsd:dateTime ;
	dct:modified "2023-03-31T12:00:00+00:00"^^xsd:dateTime  ; 
	ikos:retired "2023-03-31T12:00:00+00:00"^^xsd:dateTime ;
	skos:exactMatch subj:04016006 ;
	skos:broader	medtop:20000171 .

medtop:20000174
	rdf:type skos:Concept ;
	skos:prefLabel	"bankruptcy"@en-GB ;
	skos:definition	"Organisations that cannot pay their debts and file for special treatment by governments and financial systems"@en-GB ;
	skos:inScheme <http://cv.iptc.org/newscodes/mediatopic/>  ;
	ikos:created "2009-10-22T02:00:00+00:00"^^xsd:dateTime ;
	dct:created "2009-10-22T02:00:00+00:00"^^xsd:dateTime ;
	ikos:modified "2023-03-31T12:00:00+00:00"^^xsd:dateTime ;
	dct:modified "2023-03-31T12:00:00+00:00"^^xsd:dateTime  ;
	skos:exactMatch subj:04016007 ;
	skos:exactMatch <https://www.wikidata.org/entity/Q152074> ;
	skos:broader	medtop:20000183 .

medtop:20000175
	rdf:type skos:Concept ;
	skos:prefLabel	"stock buyback"@en-GB ;
	skos:definition	"Corporate actions in which companies buy back their own shares"@en-GB ;
	skos:inScheme <http://cv.iptc.org/newscodes/mediatopic/>  ;
	ikos:created "2009-10-22T02:00:00+00:00"^^xsd:dateTime ;
	dct:created "2009-10-22T02:00:00+00:00"^^xsd:dateTime ;
	ikos:modified "2023-03-31T12:00:00+00:00"^^xsd:dateTime ;
	dct:modified "2023-03-31T12:00:00+00:00"^^xsd:dateTime  ;
	skos:exactMatch subj:04016009 ;
	skos:exactMatch <https://www.wikidata.org/entity/Q939290> ;
	skos:broader	medtop:20000396 .

medtop:20000176
	rdf:type skos:Concept ;
	skos:prefLabel	"credit rating"@en-GB ;
	skos:definition	"Formal statements by certain rating agencies on the investment risk of a company or enterprise"@en-GB ;
	skos:inScheme <http://cv.iptc.org/newscodes/mediatopic/>  ;
	ikos:created "2009-10-22T02:00:00+00:00"^^xsd:dateTime ;
	dct:created "2009-10-22T02:00:00+00:00"^^xsd:dateTime ;
	ikos:modified "2023-03-31T12:00:00+00:00"^^xsd:dateTime ;
	dct:modified "2023-03-31T12:00:00+00:00"^^xsd:dateTime  ;
	skos:exactMatch subj:04016050 ;
	skos:exactMatch <https://www.wikidata.org/entity/Q372765> ;
	skos:broader	medtop:20001365 .

medtop:20000177
	rdf:type skos:Concept ;
	skos:prefLabel	"corporate dividends"@en-GB ;
	skos:definition	"Distribution of company profits to shareholders via dividend payments"@en-GB ;
	skos:inScheme <http://cv.iptc.org/newscodes/mediatopic/>  ;
	ikos:created "2009-10-22T02:00:00+00:00"^^xsd:dateTime ;
	dct:created "2009-10-22T02:00:00+00:00"^^xsd:dateTime ;
	ikos:modified "2023-03-31T12:00:00+00:00"^^xsd:dateTime ;
	dct:modified "2023-03-31T12:00:00+00:00"^^xsd:dateTime  ;
	skos:exactMatch subj:04016015 ;
	skos:exactMatch <https://www.wikidata.org/entity/Q181201> ;
	skos:broader	medtop:20000396 .

medtop:20000178
	rdf:type skos:Concept ;
	skos:prefLabel	"corporate earnings"@en-GB ;
	skos:definition	"Announcements and discussions of corporate earnings"@en-GB ;
	skos:inScheme <http://cv.iptc.org/newscodes/mediatopic/>  ;
	ikos:created "2009-10-22T02:00:00+00:00"^^xsd:dateTime ;
	dct:created "2009-10-22T02:00:00+00:00"^^xsd:dateTime ;
	ikos:modified "2023-03-31T12:00:00+00:00"^^xsd:dateTime ;
	dct:modified "2023-03-31T12:00:00+00:00"^^xsd:dateTime  ;
	skos:exactMatch subj:04016018 ;
	skos:exactMatch <https://www.wikidata.org/entity/Q5326940> ;
	skos:broader	medtop:20001365 .

medtop:20000179
	rdf:type skos:Concept ;
	skos:prefLabel	"earnings forecast"@en-GB ;
	skos:definition	"Analyst prediction of company earnings."@en-GB ;
	skos:changeNote	"Retired. Use medtop:20000178 corporate earnings instead."@en-GB ;
	skos:inScheme <http://cv.iptc.org/newscodes/mediatopic/>  ;
	ikos:created "2009-10-22T02:00:00+00:00"^^xsd:dateTime ;
	dct:created "2009-10-22T02:00:00+00:00"^^xsd:dateTime ;
	ikos:modified "2023-03-31T12:00:00+00:00"^^xsd:dateTime ;
	dct:modified "2023-03-31T12:00:00+00:00"^^xsd:dateTime  ; 
	ikos:retired "2023-03-31T12:00:00+00:00"^^xsd:dateTime ;
	skos:exactMatch subj:04016016 ;
	skos:exactMatch <https://www.wikidata.org/entity/Q5449712> ;
	skos:broader	medtop:20001365 .

medtop:20000180
	rdf:type skos:Concept ;
	skos:prefLabel	"financial statement"@en-GB ;
	skos:definition	"Formal statements about the company financials typically delivered annually or quarterly"@en-GB ;
	skos:inScheme <http://cv.iptc.org/newscodes/mediatopic/>  ;
	ikos:created "2009-10-22T02:00:00+00:00"^^xsd:dateTime ;
	dct:created "2009-10-22T02:00:00+00:00"^^xsd:dateTime ;
	ikos:modified "2023-03-31T12:00:00+00:00"^^xsd:dateTime ;
	dct:modified "2023-03-31T12:00:00+00:00"^^xsd:dateTime  ;
	skos:exactMatch subj:04016038 ;
	skos:exactMatch <https://www.wikidata.org/entity/Q192907> ;
	skos:broader	medtop:20001365 .

medtop:20000181
	rdf:type skos:Concept ;
	skos:prefLabel	"proxy filing"@en-GB ;
	skos:definition	"Filings with regulatory agencies of proxy statements for upcoming shareholder votes."@en-GB ;
	skos:inScheme <http://cv.iptc.org/newscodes/mediatopic/>  ;
	ikos:created "2009-10-22T02:00:00+00:00"^^xsd:dateTime ;
	dct:created "2009-10-22T02:00:00+00:00"^^xsd:dateTime ;
	ikos:modified "2023-03-31T12:00:00+00:00"^^xsd:dateTime ;
	dct:modified "2023-03-31T12:00:00+00:00"^^xsd:dateTime  ;
	skos:exactMatch subj:04016035 ;
	skos:broader	medtop:20000199 .

medtop:20000182
	rdf:type skos:Concept ;
	skos:prefLabel	"financially distressed company"@en-GB ;
	skos:definition	"Indications that a company is financially distressed but not having filed for bankruptcy yet"@en-GB ;
	skos:inScheme <http://cv.iptc.org/newscodes/mediatopic/>  ;
	ikos:created "2009-10-22T02:00:00+00:00"^^xsd:dateTime ;
	dct:created "2009-10-22T02:00:00+00:00"^^xsd:dateTime ;
	ikos:modified "2023-03-31T12:00:00+00:00"^^xsd:dateTime ;
	dct:modified "2023-03-31T12:00:00+00:00"^^xsd:dateTime  ;
	skos:exactMatch subj:04016017 ;
	skos:exactMatch <https://www.wikidata.org/entity/Q1785212> ;
	skos:broader	medtop:20000183 .

medtop:20000183
	rdf:type skos:Concept ;
	skos:prefLabel	"business financing"@en-GB ;
	skos:definition	"The financing, capital structuring, and investment decisions of a business"@en-GB ;
	skos:inScheme <http://cv.iptc.org/newscodes/mediatopic/>  ;
	ikos:created "2009-10-22T02:00:00+00:00"^^xsd:dateTime ;
	dct:created "2009-10-22T02:00:00+00:00"^^xsd:dateTime ;
	ikos:modified "2023-03-31T12:00:00+00:00"^^xsd:dateTime ;
	dct:modified "2023-03-31T12:00:00+00:00"^^xsd:dateTime  ;
	skos:exactMatch subj:04016019 ;
	skos:exactMatch <https://www.wikidata.org/entity/Q1134763> ;
	skos:broader	medtop:20000170 ;
	skos:narrower	medtop:20000174 ;
	skos:narrower	medtop:20000182 ;
	skos:narrower	medtop:20000184 ;
	skos:narrower	medtop:20000394 ;
	skos:narrower	medtop:20000396 ;
	skos:narrower	medtop:20001294 .

medtop:20000184
	rdf:type skos:Concept ;
	skos:prefLabel	"restructuring and recapitalisation"@en-GB ;
	skos:definition	"The sale of company units, splits of existing companies into units under a holding company, etc."@en-GB ;
	skos:changeNote	"Use medtop:20001366 business restructuring instead."@en-GB ;
	skos:inScheme <http://cv.iptc.org/newscodes/mediatopic/>  ;
	ikos:created "2009-10-22T02:00:00+00:00"^^xsd:dateTime ;
	dct:created "2009-10-22T02:00:00+00:00"^^xsd:dateTime ;
	ikos:modified "2023-10-02T12:00:00+00:00"^^xsd:dateTime ;
	dct:modified "2023-10-02T12:00:00+00:00"^^xsd:dateTime  ; 
	ikos:retired "2023-10-02T12:00:00+00:00"^^xsd:dateTime ;
	skos:exactMatch subj:04016039 ;
	skos:exactMatch <https://www.wikidata.org/entity/Q1376796> ;
	skos:broader	medtop:20000183 .

medtop:20000185
	rdf:type skos:Concept ;
	skos:prefLabel	"shareholder activity"@en-GB ;
	skos:definition	"Actions taken by owners of one or more shares of a company, including shareholder activism"@en-GB ;
	skos:inScheme <http://cv.iptc.org/newscodes/mediatopic/>  ;
	ikos:created "2009-10-22T02:00:00+00:00"^^xsd:dateTime ;
	dct:created "2009-10-22T02:00:00+00:00"^^xsd:dateTime ;
	ikos:modified "2023-03-31T12:00:00+00:00"^^xsd:dateTime ;
	dct:modified "2023-03-31T12:00:00+00:00"^^xsd:dateTime  ;
	skos:exactMatch subj:04016047 ;
	skos:exactMatch <https://www.wikidata.org/entity/Q381136> ;
	skos:broader	medtop:20000199 .

medtop:20000186
	rdf:type skos:Concept ;
	skos:prefLabel	"stock activity"@en-GB ;
	skos:definition	"Announcements of major stock events: splits, block trades, new highs or lows, etc."@en-GB ;
	skos:inScheme <http://cv.iptc.org/newscodes/mediatopic/>  ;
	ikos:created "2009-10-22T02:00:00+00:00"^^xsd:dateTime ;
	dct:created "2009-10-22T02:00:00+00:00"^^xsd:dateTime ;
	ikos:modified "2023-03-31T12:00:00+00:00"^^xsd:dateTime ;
	dct:modified "2023-03-31T12:00:00+00:00"^^xsd:dateTime  ;
	skos:exactMatch subj:04016041 ;
	skos:broader	medtop:20000396 .

medtop:20000187
	rdf:type skos:Concept ;
	skos:prefLabel	"stock flotation"@en-GB ;
	skos:definition	"The issuing of stock shares to the public for the first time, also called an Initial Public Offering (IPO)"@en-GB ;
	skos:inScheme <http://cv.iptc.org/newscodes/mediatopic/>  ;
	ikos:created "2009-10-22T02:00:00+00:00"^^xsd:dateTime ;
	dct:created "2009-10-22T02:00:00+00:00"^^xsd:dateTime ;
	ikos:modified "2021-02-18T12:00:00+00:00"^^xsd:dateTime ;
	dct:modified "2021-02-18T12:00:00+00:00"^^xsd:dateTime  ;
	skos:broadMatch subj:04016019 ;
	skos:exactMatch <https://www.wikidata.org/entity/Q185142> ;
	skos:broader	medtop:20000396 .

medtop:20000188
	rdf:type skos:Concept ;
	skos:prefLabel	"human resources"@en-GB ;
	skos:definition	"People working for a business and how they are managed"@en-GB ;
	skos:inScheme <http://cv.iptc.org/newscodes/mediatopic/>  ;
	ikos:created "2009-10-22T02:00:00+00:00"^^xsd:dateTime ;
	dct:created "2009-10-22T02:00:00+00:00"^^xsd:dateTime ;
	ikos:modified "2021-02-18T12:00:00+00:00"^^xsd:dateTime ;
	dct:modified "2021-02-18T12:00:00+00:00"^^xsd:dateTime  ;
	skos:broadMatch subj:09000000 ;
	skos:exactMatch <https://www.wikidata.org/entity/Q1920785> ;
	skos:broader	medtop:20000170 ;
	skos:narrower	medtop:20000189 ;
	skos:narrower	medtop:20000190 .

medtop:20000189
	rdf:type skos:Concept ;
	skos:prefLabel	"layoffs and downsizing"@en-GB ;
	skos:definition	"Planned or actual reductions in the labour force."@en-GB ;
	skos:inScheme <http://cv.iptc.org/newscodes/mediatopic/>  ;
	ikos:created "2009-10-22T02:00:00+00:00"^^xsd:dateTime ;
	dct:created "2009-10-22T02:00:00+00:00"^^xsd:dateTime ;
	ikos:modified "2021-05-05T12:00:00+00:00"^^xsd:dateTime ;
	dct:modified "2021-05-05T12:00:00+00:00"^^xsd:dateTime  ;
	skos:exactMatch subj:04016025 ;
	skos:exactMatch <https://www.wikidata.org/entity/Q13634065> ;
	skos:broader	medtop:20000188 .

medtop:20000190
	rdf:type skos:Concept ;
	skos:prefLabel	"executive officer"@en-GB ;
	skos:definition	"Company executive officers including appointments and changes"@en-GB ;
	skos:inScheme <http://cv.iptc.org/newscodes/mediatopic/>  ;
	ikos:created "2009-10-22T02:00:00+00:00"^^xsd:dateTime ;
	dct:created "2009-10-22T02:00:00+00:00"^^xsd:dateTime ;
	ikos:modified "2023-03-31T12:00:00+00:00"^^xsd:dateTime ;
	dct:modified "2023-03-31T12:00:00+00:00"^^xsd:dateTime  ;
	skos:broadMatch subj:04016028 ;
	skos:exactMatch <https://www.wikidata.org/entity/Q2462658> ;
	skos:broader	medtop:20000188 .

medtop:20000191
	rdf:type skos:Concept ;
	skos:prefLabel	"stock option"@en-GB ;
	skos:definition	"An agreement to either buy or sell a stock when it meets a certain price, sometimes used as an incentive for employees and officers of a company"@en-GB ;
	skos:changeNote	"Retired. Use derivatives medtop:20000395 instead."@en-GB ;
	skos:inScheme <http://cv.iptc.org/newscodes/mediatopic/>  ;
	ikos:created "2009-10-22T02:00:00+00:00"^^xsd:dateTime ;
	dct:created "2009-10-22T02:00:00+00:00"^^xsd:dateTime ;
	ikos:modified "2023-03-31T12:00:00+00:00"^^xsd:dateTime ;
	dct:modified "2023-03-31T12:00:00+00:00"^^xsd:dateTime  ; 
	ikos:retired "2023-03-31T12:00:00+00:00"^^xsd:dateTime ;
	skos:exactMatch subj:04016052 ;
	skos:exactMatch <https://www.wikidata.org/entity/Q187860> ;
	skos:broader	medtop:20000394 .

medtop:20000192
	rdf:type skos:Concept ;
	skos:prefLabel	"business strategy and marketing"@en-GB ;
	skos:definition	"Planning the direction of a company and selling its products and services to achieve the strategy"@en-GB ;
	skos:inScheme <http://cv.iptc.org/newscodes/mediatopic/>  ;
	ikos:created "2009-10-22T02:00:00+00:00"^^xsd:dateTime ;
	dct:created "2009-10-22T02:00:00+00:00"^^xsd:dateTime ;
	ikos:modified "2023-03-31T12:00:00+00:00"^^xsd:dateTime ;
	dct:modified "2023-03-31T12:00:00+00:00"^^xsd:dateTime  ;
	skos:broadMatch subj:04016029 ;
	skos:exactMatch <https://www.wikidata.org/entity/Q39809> ;
	skos:broader	medtop:20000170 ;
	skos:narrower	medtop:20000196 ;
	skos:narrower	medtop:20000198 ;
	skos:narrower	medtop:20000202 ;
	skos:narrower	medtop:20000205 ;
	skos:narrower	medtop:20000206 ;
	skos:narrower	medtop:20000207 ;
	skos:narrower	medtop:20000208 ;
	skos:narrower	medtop:20000283 ;
	skos:narrower	medtop:20000284 ;
	skos:narrower	medtop:20001159 ;
	skos:narrower	medtop:20001163 ;
	skos:narrower	medtop:20001295 .

medtop:20000193
	rdf:type skos:Concept ;
	skos:prefLabel	"annual and special corporate meeting"@en-GB ;
	skos:definition	"News surrounding company reports and annual or special corporate meetings"@en-GB ;
	skos:inScheme <http://cv.iptc.org/newscodes/mediatopic/>  ;
	ikos:created "2009-10-22T02:00:00+00:00"^^xsd:dateTime ;
	dct:created "2009-10-22T02:00:00+00:00"^^xsd:dateTime ;
	ikos:modified "2023-03-31T12:00:00+00:00"^^xsd:dateTime ;
	dct:modified "2023-03-31T12:00:00+00:00"^^xsd:dateTime  ;
	skos:exactMatch subj:04016002 ;
	skos:exactMatch <https://www.wikidata.org/entity/Q1077012> ;
	skos:broader	medtop:20000199 .

medtop:20000194
	rdf:type skos:Concept ;
	skos:prefLabel	"annual report"@en-GB ;
	skos:definition	"Availability or contents of annual company reports."@en-GB ;
	skos:inScheme <http://cv.iptc.org/newscodes/mediatopic/>  ;
	ikos:created "2009-10-22T02:00:00+00:00"^^xsd:dateTime ;
	dct:created "2009-10-22T02:00:00+00:00"^^xsd:dateTime ;
	ikos:modified "2023-03-31T12:00:00+00:00"^^xsd:dateTime ;
	dct:modified "2023-03-31T12:00:00+00:00"^^xsd:dateTime  ;
	skos:exactMatch subj:04016003 ;
	skos:exactMatch <https://www.wikidata.org/entity/Q699735> ;
	skos:broader	medtop:20000199 .

medtop:20000195
	rdf:type skos:Concept ;
	skos:prefLabel	"board of directors"@en-GB ;
	skos:definition	"Appointments to or changes in the board of directors for a company."@en-GB ;
	skos:inScheme <http://cv.iptc.org/newscodes/mediatopic/>  ;
	ikos:created "2009-10-22T02:00:00+00:00"^^xsd:dateTime ;
	dct:created "2009-10-22T02:00:00+00:00"^^xsd:dateTime ;
	ikos:modified "2023-03-31T12:00:00+00:00"^^xsd:dateTime ;
	dct:modified "2023-03-31T12:00:00+00:00"^^xsd:dateTime  ;
	skos:exactMatch subj:04016008 ;
	skos:exactMatch <https://www.wikidata.org/entity/Q188628> ;
	skos:broader	medtop:20000199 .

medtop:20000196
	rdf:type skos:Concept ;
	skos:prefLabel	"commercial contract"@en-GB ;
	skos:definition	"Contracts regarding commercial activities"@en-GB ;
	skos:inScheme <http://cv.iptc.org/newscodes/mediatopic/>  ;
	ikos:created "2009-10-22T02:00:00+00:00"^^xsd:dateTime ;
	dct:created "2009-10-22T02:00:00+00:00"^^xsd:dateTime ;
	ikos:modified "2021-02-18T12:00:00+00:00"^^xsd:dateTime ;
	dct:modified "2021-02-18T12:00:00+00:00"^^xsd:dateTime  ;
	skos:exactMatch subj:04016013 ;
	skos:broader	medtop:20000192 .

medtop:20000197
	rdf:type skos:Concept ;
	skos:prefLabel	"company spin-off"@en-GB ;
	skos:definition	"The creation of new companies being spun off from existing companies"@en-GB ;
	skos:inScheme <http://cv.iptc.org/newscodes/mediatopic/>  ;
	ikos:created "2009-10-22T02:00:00+00:00"^^xsd:dateTime ;
	dct:created "2009-10-22T02:00:00+00:00"^^xsd:dateTime ;
	ikos:modified "2023-03-31T12:00:00+00:00"^^xsd:dateTime ;
	dct:modified "2023-03-31T12:00:00+00:00"^^xsd:dateTime  ;
	skos:exactMatch subj:04016040 ;
	skos:exactMatch <https://www.wikidata.org/entity/Q1186164> ;
	skos:broader	medtop:20001366 .

medtop:20000198
	rdf:type skos:Concept ;
	skos:prefLabel	"economic globalisation"@en-GB ;
	skos:definition	"Doing business around the world"@en-GB ;
	skos:inScheme <http://cv.iptc.org/newscodes/mediatopic/>  ;
	ikos:created "2009-10-22T02:00:00+00:00"^^xsd:dateTime ;
	dct:created "2009-10-22T02:00:00+00:00"^^xsd:dateTime ;
	ikos:modified "2021-02-18T12:00:00+00:00"^^xsd:dateTime ;
	dct:modified "2021-02-18T12:00:00+00:00"^^xsd:dateTime  ;
	skos:exactMatch subj:04016054 ;
	skos:exactMatch <https://www.wikidata.org/entity/Q2339766> ;
	skos:broader	medtop:20000192 .

medtop:20000199
	rdf:type skos:Concept ;
	skos:prefLabel	"business governance"@en-GB ;
	skos:definition	"The rules, practices, and processes used to oversee and manage a company"@en-GB ;
	skos:inScheme <http://cv.iptc.org/newscodes/mediatopic/>  ;
	ikos:created "2009-10-22T02:00:00+00:00"^^xsd:dateTime ;
	dct:created "2009-10-22T02:00:00+00:00"^^xsd:dateTime ;
	ikos:modified "2023-03-31T12:00:00+00:00"^^xsd:dateTime ;
	dct:modified "2023-03-31T12:00:00+00:00"^^xsd:dateTime  ;
	skos:broadMatch subj:04016027 ;
	skos:exactMatch <https://www.wikidata.org/entity/Q2920921> ;
	skos:broader	medtop:20000170 ;
	skos:narrower	medtop:20000181 ;
	skos:narrower	medtop:20000185 ;
	skos:narrower	medtop:20000193 ;
	skos:narrower	medtop:20000194 ;
	skos:narrower	medtop:20000195 ;
	skos:narrower	medtop:20001230 .

medtop:20000200
	rdf:type skos:Concept ;
	skos:prefLabel	"joint venture"@en-GB ;
	skos:definition	"Two or more companies agreeing on a venture."@en-GB ;
	skos:inScheme <http://cv.iptc.org/newscodes/mediatopic/>  ;
	ikos:created "2009-10-22T02:00:00+00:00"^^xsd:dateTime ;
	dct:created "2009-10-22T02:00:00+00:00"^^xsd:dateTime ;
	ikos:modified "2023-03-31T12:00:00+00:00"^^xsd:dateTime ;
	dct:modified "2023-03-31T12:00:00+00:00"^^xsd:dateTime  ;
	skos:exactMatch subj:04016023 ;
	skos:exactMatch <https://www.wikidata.org/entity/Q489209> ;
	skos:broader	medtop:20001366 .

medtop:20000201
	rdf:type skos:Concept ;
	skos:prefLabel	"leveraged buyout"@en-GB ;
	skos:definition	"Acquiring control over a company by buying its shares with borrowed money."@en-GB ;
	skos:inScheme <http://cv.iptc.org/newscodes/mediatopic/>  ;
	ikos:created "2009-10-22T02:00:00+00:00"^^xsd:dateTime ;
	dct:created "2009-10-22T02:00:00+00:00"^^xsd:dateTime ;
	ikos:modified "2023-03-31T12:00:00+00:00"^^xsd:dateTime ;
	dct:modified "2023-03-31T12:00:00+00:00"^^xsd:dateTime  ;
	skos:exactMatch subj:04016024 ;
	skos:exactMatch <https://www.wikidata.org/entity/Q1058381> ;
	skos:broader	medtop:20001366 .

medtop:20000202
	rdf:type skos:Concept ;
	skos:prefLabel	"licensing agreement"@en-GB ;
	skos:definition	"The document defining the terms for licensing intellectual property"@en-GB ;
	skos:changeNote	"Retired. Use medtop:20000196 commercial contract instead."@en-GB ;
	skos:inScheme <http://cv.iptc.org/newscodes/mediatopic/>  ;
	ikos:created "2009-10-22T02:00:00+00:00"^^xsd:dateTime ;
	dct:created "2009-10-22T02:00:00+00:00"^^xsd:dateTime ;
	ikos:modified "2023-03-31T12:00:00+00:00"^^xsd:dateTime ;
	dct:modified "2023-03-31T12:00:00+00:00"^^xsd:dateTime  ; 
	ikos:retired "2023-03-31T12:00:00+00:00"^^xsd:dateTime ;
	skos:exactMatch subj:04016026 ;
	skos:exactMatch <https://www.wikidata.org/entity/Q79719> ;
	skos:broader	medtop:20000192 .

medtop:20000203
	rdf:type skos:Concept ;
	skos:prefLabel	"management buyout"@en-GB ;
	skos:definition	"Acquiring control over a company by the management buying its shares."@en-GB ;
	skos:inScheme <http://cv.iptc.org/newscodes/mediatopic/>  ;
	ikos:created "2009-10-22T02:00:00+00:00"^^xsd:dateTime ;
	dct:created "2009-10-22T02:00:00+00:00"^^xsd:dateTime ;
	ikos:modified "2023-03-31T12:00:00+00:00"^^xsd:dateTime ;
	dct:modified "2023-03-31T12:00:00+00:00"^^xsd:dateTime  ;
	skos:broadMatch subj:04000000 ;
	skos:exactMatch <https://www.wikidata.org/entity/Q1501578> ;
	skos:broader	medtop:20001366 .

medtop:20000204
	rdf:type skos:Concept ;
	skos:prefLabel	"merger or acquisition"@en-GB ;
	skos:definition	"Two or more companies forming a new company mergers, takeovers or acquisitions."@en-GB ;
	skos:inScheme <http://cv.iptc.org/newscodes/mediatopic/>  ;
	ikos:created "2009-10-22T02:00:00+00:00"^^xsd:dateTime ;
	dct:created "2009-10-22T02:00:00+00:00"^^xsd:dateTime ;
	ikos:modified "2023-03-31T12:00:00+00:00"^^xsd:dateTime ;
	dct:modified "2023-03-31T12:00:00+00:00"^^xsd:dateTime  ;
	skos:exactMatch subj:04016005 ;
	skos:exactMatch <https://www.wikidata.org/entity/Q731112> ;
	skos:broader	medtop:20001366 .

medtop:20000205
	rdf:type skos:Concept ;
	skos:prefLabel	"new product or service"@en-GB ;
	skos:definition	"The introduction of products or services to the market"@en-GB ;
	skos:inScheme <http://cv.iptc.org/newscodes/mediatopic/>  ;
	ikos:created "2009-10-22T02:00:00+00:00"^^xsd:dateTime ;
	dct:created "2009-10-22T02:00:00+00:00"^^xsd:dateTime ;
	ikos:modified "2023-03-31T12:00:00+00:00"^^xsd:dateTime ;
	dct:modified "2023-03-31T12:00:00+00:00"^^xsd:dateTime  ;
	skos:broadMatch subj:04016030 ;
	skos:exactMatch <https://www.wikidata.org/entity/Q1395034> ;
	skos:broader	medtop:20000192 .

medtop:20000206
	rdf:type skos:Concept ;
	skos:prefLabel	"patent, copyright and trademark"@en-GB ;
	skos:definition	"Intellectual properties such as patents, copyright and trademarks"@en-GB ;
	skos:inScheme <http://cv.iptc.org/newscodes/mediatopic/>  ;
	ikos:created "2009-10-22T02:00:00+00:00"^^xsd:dateTime ;
	dct:created "2009-10-22T02:00:00+00:00"^^xsd:dateTime ;
	ikos:modified "2023-03-31T12:00:00+00:00"^^xsd:dateTime ;
	dct:modified "2023-03-31T12:00:00+00:00"^^xsd:dateTime  ;
	skos:exactMatch subj:04016031 ;
	skos:exactMatch <https://www.wikidata.org/entity/Q131257> ;
	skos:broader	medtop:20000192 .

medtop:20000207
	rdf:type skos:Concept ;
	skos:prefLabel	"product recall"@en-GB ;
	skos:definition	"A decision by a company to take back or repair a defective product"@en-GB ;
	skos:inScheme <http://cv.iptc.org/newscodes/mediatopic/>  ;
	ikos:created "2009-10-22T02:00:00+00:00"^^xsd:dateTime ;
	dct:created "2009-10-22T02:00:00+00:00"^^xsd:dateTime ;
	ikos:modified "2021-02-18T12:00:00+00:00"^^xsd:dateTime ;
	dct:modified "2021-02-18T12:00:00+00:00"^^xsd:dateTime  ;
	skos:exactMatch subj:04016053 ;
	skos:exactMatch <https://www.wikidata.org/entity/Q359495> ;
	skos:broader	medtop:20000192 .

medtop:20000208
	rdf:type skos:Concept ;
	skos:prefLabel	"research and development"@en-GB ;
	skos:definition	"Research and expenditure on new product or service development"@en-GB ;
	skos:inScheme <http://cv.iptc.org/newscodes/mediatopic/>  ;
	ikos:created "2009-10-22T02:00:00+00:00"^^xsd:dateTime ;
	dct:created "2009-10-22T02:00:00+00:00"^^xsd:dateTime ;
	ikos:modified "2021-02-18T12:00:00+00:00"^^xsd:dateTime ;
	dct:modified "2021-02-18T12:00:00+00:00"^^xsd:dateTime  ;
	skos:exactMatch subj:04016037 ;
	skos:exactMatch <https://www.wikidata.org/entity/Q276099> ;
	skos:broader	medtop:20000192 .

medtop:20000209
	rdf:type skos:Concept ;
	skos:prefLabel	"products and services"@en-GB ;
	skos:definition	"Products and services consumed by companies and individuals and the companies that manufacture or manage them"@en-GB ;
	skos:inScheme <http://cv.iptc.org/newscodes/mediatopic/>  ;
	ikos:created "2009-10-22T02:00:00+00:00"^^xsd:dateTime ;
	dct:created "2009-10-22T02:00:00+00:00"^^xsd:dateTime ;
	ikos:modified "2023-03-31T12:00:00+00:00"^^xsd:dateTime ;
	dct:modified "2023-03-31T12:00:00+00:00"^^xsd:dateTime  ;
	skos:broadMatch subj:04000000 ;
	skos:exactMatch <https://www.wikidata.org/entity/Q3958441> ;
	skos:broader	medtop:04000000 ;
	skos:narrower	medtop:20000210 ;
	skos:narrower	medtop:20000213 ;
	skos:narrower	medtop:20000214 ;
	skos:narrower	medtop:20000217 ;
	skos:narrower	medtop:20000224 ;
	skos:narrower	medtop:20000225 ;
	skos:narrower	medtop:20000235 ;
	skos:narrower	medtop:20000243 ;
	skos:narrower	medtop:20000256 ;
	skos:narrower	medtop:20000271 ;
	skos:narrower	medtop:20000294 ;
	skos:narrower	medtop:20000304 ;
	skos:narrower	medtop:20000316 ;
	skos:narrower	medtop:20000322 ;
	skos:narrower	medtop:20000331 ;
	skos:narrower	medtop:20000337 ;
	skos:narrower	medtop:20001244 ;
	skos:narrower	medtop:20001289 ;
	skos:narrower	medtop:20001354 ;
	skos:narrower	medtop:20001370 ;
	skos:narrower	medtop:20001371 .

medtop:20000210
	rdf:type skos:Concept ;
	skos:prefLabel	"agriculture"@en-GB ;
	skos:definition	"The growing and raising of plants and animals for consumption and the processing, cleaning, packing or storage of these products"@en-GB ;
	skos:inScheme <http://cv.iptc.org/newscodes/mediatopic/>  ;
	ikos:created "2009-10-22T02:00:00+00:00"^^xsd:dateTime ;
	dct:created "2009-10-22T02:00:00+00:00"^^xsd:dateTime ;
	ikos:modified "2023-03-31T12:00:00+00:00"^^xsd:dateTime ;
	dct:modified "2023-03-31T12:00:00+00:00"^^xsd:dateTime  ;
	skos:exactMatch subj:04001000 ;
	skos:exactMatch <https://www.wikidata.org/entity/Q11451> ;
	skos:broader	medtop:20000209 ;
	skos:narrower	medtop:20000211 ;
	skos:narrower	medtop:20000212 ;
	skos:narrower	medtop:20000215 ;
	skos:narrower	medtop:20000216 .

medtop:20000211
	rdf:type skos:Concept ;
	skos:prefLabel	"aquaculture"@en-GB ;
	skos:definition	"Growing plants or animals in water for human consumption"@en-GB ;
	skos:changeNote	"Retired. Use medtop:20000210 agriculture instead."@en-GB ;
	skos:inScheme <http://cv.iptc.org/newscodes/mediatopic/>  ;
	ikos:created "2009-10-22T02:00:00+00:00"^^xsd:dateTime ;
	dct:created "2009-10-22T02:00:00+00:00"^^xsd:dateTime ;
	ikos:modified "2023-03-31T12:00:00+00:00"^^xsd:dateTime ;
	dct:modified "2023-03-31T12:00:00+00:00"^^xsd:dateTime  ; 
	ikos:retired "2023-03-31T12:00:00+00:00"^^xsd:dateTime ;
	skos:exactMatch subj:04001006 ;
	skos:exactMatch <https://www.wikidata.org/entity/Q188989> ;
	skos:broader	medtop:20000210 .

medtop:20000212
	rdf:type skos:Concept ;
	skos:prefLabel	"arable farming"@en-GB ;
	skos:definition	"The growing of plants on a large scale commercially, especially a cereal, fruit, grain or vegetable"@en-GB ;
	skos:changeNote	"Retired. Use medtop:20000210 agriculture instead."@en-GB ;
	skos:inScheme <http://cv.iptc.org/newscodes/mediatopic/>  ;
	ikos:created "2009-10-22T02:00:00+00:00"^^xsd:dateTime ;
	dct:created "2009-10-22T02:00:00+00:00"^^xsd:dateTime ;
	ikos:modified "2023-03-31T12:00:00+00:00"^^xsd:dateTime ;
	dct:modified "2023-03-31T12:00:00+00:00"^^xsd:dateTime  ; 
	ikos:retired "2023-03-31T12:00:00+00:00"^^xsd:dateTime ;
	skos:exactMatch subj:04001001 ;
	skos:exactMatch <https://www.wikidata.org/entity/Q51075346> ;
	skos:broader	medtop:20000210 .

medtop:20000213
	rdf:type skos:Concept ;
	skos:prefLabel	"commercial fishing"@en-GB ;
	skos:definition	"Fish farming and commercial activity around the catching of fish and seafood for consumption"@en-GB ;
	skos:inScheme <http://cv.iptc.org/newscodes/mediatopic/>  ;
	ikos:created "2009-10-22T02:00:00+00:00"^^xsd:dateTime ;
	dct:created "2009-10-22T02:00:00+00:00"^^xsd:dateTime ;
	ikos:modified "2023-03-31T12:00:00+00:00"^^xsd:dateTime ;
	dct:modified "2023-03-31T12:00:00+00:00"^^xsd:dateTime  ;
	skos:exactMatch subj:04001002 ;
	skos:exactMatch <https://www.wikidata.org/entity/Q635139> ;
	skos:broader	medtop:20000209 .

medtop:20000214
	rdf:type skos:Concept ;
	skos:prefLabel	"forestry and timber"@en-GB ;
	skos:definition	"The production, collection and preparation of wood products"@en-GB ;
	skos:inScheme <http://cv.iptc.org/newscodes/mediatopic/>  ;
	ikos:created "2009-10-22T02:00:00+00:00"^^xsd:dateTime ;
	dct:created "2009-10-22T02:00:00+00:00"^^xsd:dateTime ;
	ikos:modified "2023-03-31T12:00:00+00:00"^^xsd:dateTime ;
	dct:modified "2023-03-31T12:00:00+00:00"^^xsd:dateTime  ;
	skos:exactMatch subj:04001003 ;
	skos:exactMatch <https://www.wikidata.org/entity/Q38112> ;
	skos:broader	medtop:20000209 .

medtop:20000215
	rdf:type skos:Concept ;
	skos:prefLabel	"livestock farming"@en-GB ;
	skos:definition	"Raising of animals for their by-products, such as meat, eggs, milk, fur and wool"@en-GB ;
	skos:changeNote	"Retired. Use medtop:20000210 agriculture instead."@en-GB ;
	skos:inScheme <http://cv.iptc.org/newscodes/mediatopic/>  ;
	ikos:created "2009-10-22T02:00:00+00:00"^^xsd:dateTime ;
	dct:created "2009-10-22T02:00:00+00:00"^^xsd:dateTime ;
	ikos:modified "2023-03-31T12:00:00+00:00"^^xsd:dateTime ;
	dct:modified "2023-03-31T12:00:00+00:00"^^xsd:dateTime  ; 
	ikos:retired "2023-03-31T12:00:00+00:00"^^xsd:dateTime ;
	skos:exactMatch subj:04001004 ;
	skos:exactMatch <https://www.wikidata.org/entity/Q7143051> ;
	skos:broader	medtop:20000210 .

medtop:20000216
	rdf:type skos:Concept ;
	skos:prefLabel	"viniculture"@en-GB ;
	skos:definition	"Production of wines from the vines to the finished products"@en-GB ;
	skos:changeNote	"Retired. Use medtop:20000324 beverage and grocery instead."@en-GB ;
	skos:inScheme <http://cv.iptc.org/newscodes/mediatopic/>  ;
	ikos:created "2009-10-22T02:00:00+00:00"^^xsd:dateTime ;
	dct:created "2009-10-22T02:00:00+00:00"^^xsd:dateTime ;
	ikos:modified "2023-03-31T12:00:00+00:00"^^xsd:dateTime ;
	dct:modified "2023-03-31T12:00:00+00:00"^^xsd:dateTime  ; 
	ikos:retired "2023-03-31T12:00:00+00:00"^^xsd:dateTime ;
	skos:exactMatch subj:04001005 ;
	skos:exactMatch <https://www.wikidata.org/entity/Q3560277> ;
	skos:broader	medtop:20000210 .

medtop:20000217
	rdf:type skos:Concept ;
	skos:prefLabel	"chemicals"@en-GB ;
	skos:definition	"Natural or manmade materials used to produce other materials"@en-GB ;
	skos:inScheme <http://cv.iptc.org/newscodes/mediatopic/>  ;
	ikos:created "2009-10-22T02:00:00+00:00"^^xsd:dateTime ;
	dct:created "2009-10-22T02:00:00+00:00"^^xsd:dateTime ;
	ikos:modified "2021-02-18T12:00:00+00:00"^^xsd:dateTime ;
	dct:modified "2021-02-18T12:00:00+00:00"^^xsd:dateTime  ;
	skos:exactMatch subj:04002000 ;
	skos:exactMatch <https://www.wikidata.org/entity/Q79529> ;
	skos:broader	medtop:20000209 ;
	skos:narrower	medtop:20000219 ;
	skos:narrower	medtop:20000220 ;
	skos:narrower	medtop:20000221 ;
	skos:narrower	medtop:20000222 .

medtop:20000218
	rdf:type skos:Concept ;
	skos:prefLabel	"biotechnology business"@en-GB ;
	skos:definition	"The business of using engineering technology to study and solve problems of living organisms"@en-GB ;
	skos:inScheme <http://cv.iptc.org/newscodes/mediatopic/>  ;
	ikos:created "2009-10-22T02:00:00+00:00"^^xsd:dateTime ;
	dct:created "2009-10-22T02:00:00+00:00"^^xsd:dateTime ;
	ikos:modified "2022-06-14T12:00:00+00:00"^^xsd:dateTime ;
	dct:modified "2022-06-14T12:00:00+00:00"^^xsd:dateTime  ;
	skos:exactMatch subj:04002001 ;
	skos:exactMatch <https://www.wikidata.org/entity/Q90298876> ;
	skos:broader	medtop:20001354 .

medtop:20000219
	rdf:type skos:Concept ;
	skos:prefLabel	"fertiliser"@en-GB ;
	skos:definition	"Natural or manmade materials used to encourage the growth of plants"@en-GB ;
	skos:changeNote	"Retired. Use medtop:20000217 chemicals instead."@en-GB ;
	skos:inScheme <http://cv.iptc.org/newscodes/mediatopic/>  ;
	ikos:created "2009-10-22T02:00:00+00:00"^^xsd:dateTime ;
	dct:created "2009-10-22T02:00:00+00:00"^^xsd:dateTime ;
	ikos:modified "2023-03-31T12:00:00+00:00"^^xsd:dateTime ;
	dct:modified "2023-03-31T12:00:00+00:00"^^xsd:dateTime  ; 
	ikos:retired "2023-03-31T12:00:00+00:00"^^xsd:dateTime ;
	skos:exactMatch subj:04002002 ;
	skos:exactMatch <https://www.wikidata.org/entity/Q83323> ;
	skos:broader	medtop:20000217 .

medtop:20000220
	rdf:type skos:Concept ;
	skos:prefLabel	"health and beauty product"@en-GB ;
	skos:definition	"Compilation of chemicals and other substances for use in enhancing ones looks or smell"@en-GB ;
	skos:changeNote	"Retired. Use medtop:20001248 cosmetics instead."@en-GB ;
	skos:inScheme <http://cv.iptc.org/newscodes/mediatopic/>  ;
	ikos:created "2009-10-22T02:00:00+00:00"^^xsd:dateTime ;
	dct:created "2009-10-22T02:00:00+00:00"^^xsd:dateTime ;
	ikos:modified "2023-03-31T12:00:00+00:00"^^xsd:dateTime ;
	dct:modified "2023-03-31T12:00:00+00:00"^^xsd:dateTime  ; 
	ikos:retired "2023-03-31T12:00:00+00:00"^^xsd:dateTime ;
	skos:exactMatch subj:04002003 ;
	skos:exactMatch <https://www.wikidata.org/entity/Q131207> ;
	skos:broader	medtop:20000217 .

medtop:20000221
	rdf:type skos:Concept ;
	skos:prefLabel	"inorganic chemical"@en-GB ;
	skos:definition	"The branch of chemistry dealing with minerals and metals"@en-GB ;
	skos:changeNote	"Retired. Use medtop:20000217 chemicals instead."@en-GB ;
	skos:inScheme <http://cv.iptc.org/newscodes/mediatopic/>  ;
	ikos:created "2009-10-22T02:00:00+00:00"^^xsd:dateTime ;
	dct:created "2009-10-22T02:00:00+00:00"^^xsd:dateTime ;
	ikos:modified "2023-03-31T12:00:00+00:00"^^xsd:dateTime ;
	dct:modified "2023-03-31T12:00:00+00:00"^^xsd:dateTime  ; 
	ikos:retired "2023-03-31T12:00:00+00:00"^^xsd:dateTime ;
	skos:exactMatch subj:04002004 ;
	skos:exactMatch <https://www.wikidata.org/entity/Q11165> ;
	skos:broader	medtop:20000217 .

medtop:20000222
	rdf:type skos:Concept ;
	skos:prefLabel	"organic chemical"@en-GB ;
	skos:definition	"The branch of chemistry dealing with human, animal or carbon-based substances"@en-GB ;
	skos:changeNote	"Retired. Use medtop:20000217 chemicals instead."@en-GB ;
	skos:inScheme <http://cv.iptc.org/newscodes/mediatopic/>  ;
	ikos:created "2009-10-22T02:00:00+00:00"^^xsd:dateTime ;
	dct:created "2009-10-22T02:00:00+00:00"^^xsd:dateTime ;
	ikos:modified "2023-03-31T12:00:00+00:00"^^xsd:dateTime ;
	dct:modified "2023-03-31T12:00:00+00:00"^^xsd:dateTime  ; 
	ikos:retired "2023-03-31T12:00:00+00:00"^^xsd:dateTime ;
	skos:exactMatch subj:04002005 ;
	skos:exactMatch <https://www.wikidata.org/entity/Q11351> ;
	skos:broader	medtop:20000217 .

medtop:20000223
	rdf:type skos:Concept ;
	skos:prefLabel	"pharmaceutical"@en-GB ;
	skos:definition	"The production of medicines from various chemicals and natural substances and the research and discovery around new medications"@en-GB ;
	skos:inScheme <http://cv.iptc.org/newscodes/mediatopic/>  ;
	ikos:created "2009-10-22T02:00:00+00:00"^^xsd:dateTime ;
	dct:created "2009-10-22T02:00:00+00:00"^^xsd:dateTime ;
	ikos:modified "2023-03-31T12:00:00+00:00"^^xsd:dateTime ;
	dct:modified "2023-03-31T12:00:00+00:00"^^xsd:dateTime  ;
	skos:exactMatch subj:04002006 ;
	skos:exactMatch <https://www.wikidata.org/entity/Q507443> ;
	skos:broader	medtop:20001354 .

medtop:20000224
	rdf:type skos:Concept ;
	skos:prefLabel	"plastic"@en-GB ;
	skos:definition	"The production of plastics and issues around plastic consumption, including bans, recycling, using less plastics and plastic alternatives"@en-GB ;
	skos:inScheme <http://cv.iptc.org/newscodes/mediatopic/>  ;
	ikos:created "2009-10-22T02:00:00+00:00"^^xsd:dateTime ;
	dct:created "2009-10-22T02:00:00+00:00"^^xsd:dateTime ;
	ikos:modified "2023-03-31T12:00:00+00:00"^^xsd:dateTime ;
	dct:modified "2023-03-31T12:00:00+00:00"^^xsd:dateTime  ;
	skos:exactMatch subj:04002007 ;
	skos:broader	medtop:20000209 .

medtop:20000225
	rdf:type skos:Concept ;
	skos:prefLabel	"computing and information technology"@en-GB ;
	skos:definition	"Computers and the transmission of information"@en-GB ;
	skos:inScheme <http://cv.iptc.org/newscodes/mediatopic/>  ;
	ikos:created "2009-10-22T02:00:00+00:00"^^xsd:dateTime ;
	dct:created "2009-10-22T02:00:00+00:00"^^xsd:dateTime ;
	ikos:modified "2023-03-31T12:00:00+00:00"^^xsd:dateTime ;
	dct:modified "2023-03-31T12:00:00+00:00"^^xsd:dateTime  ;
	skos:exactMatch subj:04003000 ;
	skos:exactMatch <https://www.wikidata.org/entity/Q179310> ;
	skos:broader	medtop:20000209 ;
	skos:narrower	medtop:20000226 ;
	skos:narrower	medtop:20000227 ;
	skos:narrower	medtop:20000228 ;
	skos:narrower	medtop:20000229 ;
	skos:narrower	medtop:20000230 ;
	skos:narrower	medtop:20000231 ;
	skos:narrower	medtop:20000232 ;
	skos:narrower	medtop:20000233 ;
	skos:narrower	medtop:20000234 ;
	skos:narrower	medtop:20001161 .

medtop:20000226
	rdf:type skos:Concept ;
	skos:prefLabel	"computer and telecommunications hardware"@en-GB ;
	skos:definition	"Physical devices used to provide computer and telecommunication service, such as modems, keyboards, hard drives, telephones, routers and monitors"@en-GB ;
	skos:inScheme <http://cv.iptc.org/newscodes/mediatopic/>  ;
	ikos:created "2009-10-22T02:00:00+00:00"^^xsd:dateTime ;
	dct:created "2009-10-22T02:00:00+00:00"^^xsd:dateTime ;
	ikos:modified "2023-03-31T12:00:00+00:00"^^xsd:dateTime ;
	dct:modified "2023-03-31T12:00:00+00:00"^^xsd:dateTime  ;
	skos:exactMatch subj:04003001 ;
	skos:exactMatch <https://www.wikidata.org/entity/Q3966> ;
	skos:broader	medtop:20000225 .

medtop:20000227
	rdf:type skos:Concept ;
	skos:prefLabel	"computer networking"@en-GB ;
	skos:definition	"The interconnectivity between hardware that provides the medium for the transmission of data."@en-GB ;
	skos:inScheme <http://cv.iptc.org/newscodes/mediatopic/>  ;
	ikos:created "2009-10-22T02:00:00+00:00"^^xsd:dateTime ;
	dct:created "2009-10-22T02:00:00+00:00"^^xsd:dateTime ;
	ikos:modified "2023-03-31T12:00:00+00:00"^^xsd:dateTime ;
	dct:modified "2023-03-31T12:00:00+00:00"^^xsd:dateTime  ; 
	ikos:retired "2023-03-31T12:00:00+00:00"^^xsd:dateTime ;
	skos:exactMatch subj:04003002 ;
	skos:exactMatch <https://www.wikidata.org/entity/Q10336440> ;
	skos:broader	medtop:20000225 .

medtop:20000228
	rdf:type skos:Concept ;
	skos:prefLabel	"satellite technology"@en-GB ;
	skos:definition	"Hardware and software that enables ground-based devices to send signals to each other via an orbiting satellite."@en-GB ;
	skos:inScheme <http://cv.iptc.org/newscodes/mediatopic/>  ;
	ikos:created "2009-10-22T02:00:00+00:00"^^xsd:dateTime ;
	dct:created "2009-10-22T02:00:00+00:00"^^xsd:dateTime ;
	ikos:modified "2021-05-05T12:00:00+00:00"^^xsd:dateTime ;
	dct:modified "2021-05-05T12:00:00+00:00"^^xsd:dateTime  ;
	skos:exactMatch subj:04003003 ;
	skos:broader	medtop:20000225 .

medtop:20000229
	rdf:type skos:Concept ;
	skos:prefLabel	"computer security"@en-GB ;
	skos:definition	"To encompass technical developments in hardware and software, basic research and related areas such as cyber security"@en-GB ;
	skos:changeNote	"Retired. Use medtop:20000086 cyber crime or medtop:20001361 cyber warfare instead."@en-GB ;
	skos:inScheme <http://cv.iptc.org/newscodes/mediatopic/>  ;
	ikos:created "2009-10-22T02:00:00+00:00"^^xsd:dateTime ;
	dct:created "2009-10-22T02:00:00+00:00"^^xsd:dateTime ;
	ikos:modified "2023-03-31T12:00:00+00:00"^^xsd:dateTime ;
	dct:modified "2023-03-31T12:00:00+00:00"^^xsd:dateTime  ; 
	ikos:retired "2023-03-31T12:00:00+00:00"^^xsd:dateTime ;
	skos:exactMatch subj:04003008 ;
	skos:exactMatch <https://www.wikidata.org/entity/Q3510521> ;
	skos:broader	medtop:20000225 .

medtop:20000230
	rdf:type skos:Concept ;
	skos:prefLabel	"semiconductor and electronic component"@en-GB ;
	skos:definition	"The basic components that together create working electronic devices such as computer chips, transistors, diodes and integrated circuits"@en-GB ;
	skos:inScheme <http://cv.iptc.org/newscodes/mediatopic/>  ;
	ikos:created "2009-10-22T02:00:00+00:00"^^xsd:dateTime ;
	dct:created "2009-10-22T02:00:00+00:00"^^xsd:dateTime ;
	ikos:modified "2023-03-31T12:00:00+00:00"^^xsd:dateTime ;
	dct:modified "2023-03-31T12:00:00+00:00"^^xsd:dateTime  ;
	skos:exactMatch subj:04003004 ;
	skos:exactMatch <https://www.wikidata.org/entity/Q11456> ;
	skos:broader	medtop:20000225 .

medtop:20000231
	rdf:type skos:Concept ;
	skos:prefLabel	"software and applications"@en-GB ;
	skos:definition	"Computer programs including mobile or web apps and operating systems"@en-GB ;
	skos:inScheme <http://cv.iptc.org/newscodes/mediatopic/>  ;
	ikos:created "2009-10-22T02:00:00+00:00"^^xsd:dateTime ;
	dct:created "2009-10-22T02:00:00+00:00"^^xsd:dateTime ;
	ikos:modified "2023-03-31T12:00:00+00:00"^^xsd:dateTime ;
	dct:modified "2023-03-31T12:00:00+00:00"^^xsd:dateTime  ;
	skos:exactMatch subj:04003005 ;
	skos:exactMatch <https://www.wikidata.org/entity/Q7397> ;
	skos:broader	medtop:20000225 .

medtop:20000232
	rdf:type skos:Concept ;
	skos:prefLabel	"telecommunication equipment"@en-GB ;
	skos:definition	"Devices such as telephone sets, voice/data switches, modems etc that facilitate point-to-point voice/data transmissions"@en-GB ;
	skos:changeNote	"Retired. Use medtop:20000226 computer and telecommuncations hardware instead."@en-GB ;
	skos:inScheme <http://cv.iptc.org/newscodes/mediatopic/>  ;
	ikos:created "2009-10-22T02:00:00+00:00"^^xsd:dateTime ;
	dct:created "2009-10-22T02:00:00+00:00"^^xsd:dateTime ;
	ikos:modified "2023-03-31T12:00:00+00:00"^^xsd:dateTime ;
	dct:modified "2023-03-31T12:00:00+00:00"^^xsd:dateTime  ; 
	ikos:retired "2023-03-31T12:00:00+00:00"^^xsd:dateTime ;
	skos:exactMatch subj:04003006 ;
	skos:broader	medtop:20000225 .

medtop:20000233
	rdf:type skos:Concept ;
	skos:prefLabel	"telecommunication service"@en-GB ;
	skos:definition	"Services provided by commercial companies that facilitate connections between telephones and computers"@en-GB ;
	skos:inScheme <http://cv.iptc.org/newscodes/mediatopic/>  ;
	ikos:created "2009-10-22T02:00:00+00:00"^^xsd:dateTime ;
	dct:created "2009-10-22T02:00:00+00:00"^^xsd:dateTime ;
	ikos:modified "2023-03-31T12:00:00+00:00"^^xsd:dateTime ;
	dct:modified "2023-03-31T12:00:00+00:00"^^xsd:dateTime  ;
	skos:exactMatch subj:04003007 ;
	skos:exactMatch <https://www.wikidata.org/entity/Q25245117> ;
	skos:broader	medtop:20000225 .

medtop:20000234
	rdf:type skos:Concept ;
	skos:prefLabel	"wireless technology"@en-GB ;
	skos:definition	"Technology and services that permit the transfer of information between separated points without physical connection, including bluetooth and wifi networks"@en-GB ;
	skos:inScheme <http://cv.iptc.org/newscodes/mediatopic/>  ;
	ikos:created "2009-10-22T02:00:00+00:00"^^xsd:dateTime ;
	dct:created "2009-10-22T02:00:00+00:00"^^xsd:dateTime ;
	ikos:modified "2023-03-31T12:00:00+00:00"^^xsd:dateTime ;
	dct:modified "2023-03-31T12:00:00+00:00"^^xsd:dateTime  ;
	skos:exactMatch subj:04003009 ;
	skos:exactMatch <https://www.wikidata.org/entity/Q249> ;
	skos:broader	medtop:20000225 .

medtop:20000235
	rdf:type skos:Concept ;
	skos:prefLabel	"construction and property"@en-GB ;
	skos:definition	"All items pertaining to the construction and sale of property"@en-GB ;
	skos:inScheme <http://cv.iptc.org/newscodes/mediatopic/>  ;
	ikos:created "2009-10-22T02:00:00+00:00"^^xsd:dateTime ;
	dct:created "2009-10-22T02:00:00+00:00"^^xsd:dateTime ;
	ikos:modified "2021-02-18T12:00:00+00:00"^^xsd:dateTime ;
	dct:modified "2021-02-18T12:00:00+00:00"^^xsd:dateTime  ;
	skos:exactMatch subj:04004000 ;
	skos:broader	medtop:20000209 ;
	skos:narrower	medtop:20000236 ;
	skos:narrower	medtop:20000237 ;
	skos:narrower	medtop:20000238 ;
	skos:narrower	medtop:20000239 ;
	skos:narrower	medtop:20000240 ;
	skos:narrower	medtop:20000241 ;
	skos:narrower	medtop:20000317 ;
	skos:narrower	medtop:20001245 ;
	skos:narrower	medtop:20001246 ;
	skos:narrower	medtop:20001367 ;
	skos:narrower	medtop:20001368 .

medtop:20000236
	rdf:type skos:Concept ;
	skos:prefLabel	"design and engineering"@en-GB ;
	skos:definition	"Design and planning by engineers, architects etc. of roads, offices, factories, dams , offshore structures."@en-GB ;
	skos:changeNote	"Retired. Use medtop:20001245 infrastructure projects instead."@en-GB ;
	skos:inScheme <http://cv.iptc.org/newscodes/mediatopic/>  ;
	ikos:created "2009-10-22T02:00:00+00:00"^^xsd:dateTime ;
	dct:created "2009-10-22T02:00:00+00:00"^^xsd:dateTime ;
	ikos:modified "2023-03-31T12:00:00+00:00"^^xsd:dateTime ;
	dct:modified "2023-03-31T12:00:00+00:00"^^xsd:dateTime  ; 
	ikos:retired "2023-03-31T12:00:00+00:00"^^xsd:dateTime ;
	skos:exactMatch subj:04004007 ;
	skos:exactMatch <https://www.wikidata.org/entity/Q11023> ;
	skos:broader	medtop:20000235 .

medtop:20000237
	rdf:type skos:Concept ;
	skos:prefLabel	"farms"@en-GB ;
	skos:definition	"Agricultural areas for the production of foodstuffs, including dairy products, fruits and livestock, such as cattle and fish"@en-GB ;
	skos:changeNote	"Retired. Use medtop:20000210 agriculture instead."@en-GB ;
	skos:inScheme <http://cv.iptc.org/newscodes/mediatopic/>  ;
	ikos:created "2009-10-22T02:00:00+00:00"^^xsd:dateTime ;
	dct:created "2009-10-22T02:00:00+00:00"^^xsd:dateTime ;
	ikos:modified "2023-03-31T12:00:00+00:00"^^xsd:dateTime ;
	dct:modified "2023-03-31T12:00:00+00:00"^^xsd:dateTime  ; 
	ikos:retired "2019-10-07T12:00:00+00:00"^^xsd:dateTime ;
	skos:exactMatch subj:04004004 ;
	skos:exactMatch <https://www.wikidata.org/entity/Q131596> ;
	skos:broader	medtop:20000235 .

medtop:20000238
	rdf:type skos:Concept ;
	skos:prefLabel	"heavy construction"@en-GB ;
	skos:definition	"Large scale construction projects, construction of roads, dams, office/factory buildings, offshore and onshore structures, large sport stadiums"@en-GB ;
	skos:changeNote	"Retired. Use medtop:20000235 construction and property instead."@en-GB ;
	skos:inScheme <http://cv.iptc.org/newscodes/mediatopic/>  ;
	ikos:created "2009-10-22T02:00:00+00:00"^^xsd:dateTime ;
	dct:created "2009-10-22T02:00:00+00:00"^^xsd:dateTime ;
	ikos:modified "2023-03-31T12:00:00+00:00"^^xsd:dateTime ;
	dct:modified "2023-03-31T12:00:00+00:00"^^xsd:dateTime  ; 
	ikos:retired "2019-07-25T12:00:00+00:00"^^xsd:dateTime ;
	skos:exactMatch subj:04004001 ;
	skos:broader	medtop:20000235 .

medtop:20000239
	rdf:type skos:Concept ;
	skos:prefLabel	"house building"@en-GB ;
	skos:definition	"Construction of residences, for private use"@en-GB ;
	skos:changeNote	"Retired. Use medtop:20001368 residential real estate instead."@en-GB ;
	skos:inScheme <http://cv.iptc.org/newscodes/mediatopic/>  ;
	ikos:created "2009-10-22T02:00:00+00:00"^^xsd:dateTime ;
	dct:created "2009-10-22T02:00:00+00:00"^^xsd:dateTime ;
	ikos:modified "2023-03-31T12:00:00+00:00"^^xsd:dateTime ;
	dct:modified "2023-03-31T12:00:00+00:00"^^xsd:dateTime  ; 
	ikos:retired "2023-03-31T12:00:00+00:00"^^xsd:dateTime ;
	skos:exactMatch subj:04004002 ;
	skos:exactMatch <https://www.wikidata.org/entity/Q1799415> ;
	skos:broader	medtop:20000235 .

medtop:20000240
	rdf:type skos:Concept ;
	skos:prefLabel	"land price"@en-GB ;
	skos:definition	"The price of land in specific zoned areas such as commercial, residential or arable as provided by a responsible body"@en-GB ;
	skos:changeNote	"Retired. Use medtop:20001368 residential real estate instead."@en-GB ;
	skos:inScheme <http://cv.iptc.org/newscodes/mediatopic/>  ;
	ikos:created "2009-10-22T02:00:00+00:00"^^xsd:dateTime ;
	dct:created "2009-10-22T02:00:00+00:00"^^xsd:dateTime ;
	ikos:modified "2023-03-31T12:00:00+00:00"^^xsd:dateTime ;
	dct:modified "2023-03-31T12:00:00+00:00"^^xsd:dateTime  ; 
	ikos:retired "2023-03-31T12:00:00+00:00"^^xsd:dateTime ;
	skos:exactMatch subj:04004005 ;
	skos:broader	medtop:20000235 .

medtop:20000241
	rdf:type skos:Concept ;
	skos:prefLabel	"real estate"@en-GB ;
	skos:definition	"The buying, selling, renting and leasing of properties of all types"@en-GB ;
	skos:changeNote	"Retired. Use medtop:20001368 residential real estate or medtop:20001367 commercial real estate instead."@en-GB ;
	skos:inScheme <http://cv.iptc.org/newscodes/mediatopic/>  ;
	ikos:created "2009-10-22T02:00:00+00:00"^^xsd:dateTime ;
	dct:created "2009-10-22T02:00:00+00:00"^^xsd:dateTime ;
	ikos:modified "2023-03-31T12:00:00+00:00"^^xsd:dateTime ;
	dct:modified "2023-03-31T12:00:00+00:00"^^xsd:dateTime  ; 
	ikos:retired "2023-03-31T12:00:00+00:00"^^xsd:dateTime ;
	skos:exactMatch subj:04004003 ;
	skos:exactMatch <https://www.wikidata.org/entity/Q10494269> ;
	skos:broader	medtop:20000235 .

medtop:20000242
	rdf:type skos:Concept ;
	skos:prefLabel	"restoration"@en-GB ;
	skos:definition	"Restoring historic or important properties or structures to a former better state by cleaning, repairing or rebuilding"@en-GB ;
	skos:inScheme <http://cv.iptc.org/newscodes/mediatopic/>  ;
	ikos:created "2009-10-22T02:00:00+00:00"^^xsd:dateTime ;
	dct:created "2009-10-22T02:00:00+00:00"^^xsd:dateTime ;
	ikos:modified "2023-03-31T12:00:00+00:00"^^xsd:dateTime ;
	dct:modified "2023-03-31T12:00:00+00:00"^^xsd:dateTime  ;
	skos:exactMatch subj:04004006 ;
	skos:exactMatch <https://www.wikidata.org/entity/Q2144402> ;
	skos:broader	medtop:20000044 .

medtop:20000243
	rdf:type skos:Concept ;
	skos:prefLabel	"consumer goods"@en-GB ;
	skos:definition	"Items produced for and sold to individuals"@en-GB ;
	skos:inScheme <http://cv.iptc.org/newscodes/mediatopic/>  ;
	ikos:created "2009-10-22T02:00:00+00:00"^^xsd:dateTime ;
	dct:created "2009-10-22T02:00:00+00:00"^^xsd:dateTime ;
	ikos:modified "2021-02-18T12:00:00+00:00"^^xsd:dateTime ;
	dct:modified "2021-02-18T12:00:00+00:00"^^xsd:dateTime  ;
	skos:exactMatch subj:04007000 ;
	skos:exactMatch <https://www.wikidata.org/entity/Q868404> ;
	skos:broader	medtop:20000209 ;
	skos:narrower	medtop:20000244 ;
	skos:narrower	medtop:20000245 ;
	skos:narrower	medtop:20000248 ;
	skos:narrower	medtop:20000249 ;
	skos:narrower	medtop:20000251 ;
	skos:narrower	medtop:20000254 ;
	skos:narrower	medtop:20000324 ;
	skos:narrower	medtop:20000325 ;
	skos:narrower	medtop:20000330 ;
	skos:narrower	medtop:20001160 ;
	skos:narrower	medtop:20001168 ;
	skos:narrower	medtop:20001258 .

medtop:20000244
	rdf:type skos:Concept ;
	skos:prefLabel	"beverage"@en-GB ;
	skos:definition	"Liquid consumables, both alcoholic and non-alcoholic"@en-GB ;
	skos:changeNote	"Retired. Use medtop:20000324 beverage and grocery instead."@en-GB ;
	skos:inScheme <http://cv.iptc.org/newscodes/mediatopic/>  ;
	ikos:created "2009-10-22T02:00:00+00:00"^^xsd:dateTime ;
	dct:created "2009-10-22T02:00:00+00:00"^^xsd:dateTime ;
	ikos:modified "2023-03-31T12:00:00+00:00"^^xsd:dateTime ;
	dct:modified "2023-03-31T12:00:00+00:00"^^xsd:dateTime  ; 
	ikos:retired "2023-03-31T12:00:00+00:00"^^xsd:dateTime ;
	skos:exactMatch subj:04007008 ;
	skos:exactMatch <https://www.wikidata.org/entity/Q40050> ;
	skos:broader	medtop:20000243 .

medtop:20000245
	rdf:type skos:Concept ;
	skos:prefLabel	"clothing"@en-GB ;
	skos:definition	"The manufacturing and purchasing of apparel"@en-GB ;
	skos:inScheme <http://cv.iptc.org/newscodes/mediatopic/>  ;
	ikos:created "2009-10-22T02:00:00+00:00"^^xsd:dateTime ;
	dct:created "2009-10-22T02:00:00+00:00"^^xsd:dateTime ;
	ikos:modified "2023-03-31T12:00:00+00:00"^^xsd:dateTime ;
	dct:modified "2023-03-31T12:00:00+00:00"^^xsd:dateTime  ;
	skos:exactMatch subj:04007001 ;
	skos:exactMatch <https://www.wikidata.org/entity/Q11460> ;
	skos:broader	medtop:20000243 .

medtop:20000246
	rdf:type skos:Concept ;
	skos:prefLabel	"department store"@en-GB ;
	skos:definition	"Store selling a variety of goods, such as clothing, housewares, jewellery and cosmetics"@en-GB ;
	skos:inScheme <http://cv.iptc.org/newscodes/mediatopic/>  ;
	ikos:created "2009-10-22T02:00:00+00:00"^^xsd:dateTime ;
	dct:created "2009-10-22T02:00:00+00:00"^^xsd:dateTime ;
	ikos:modified "2021-02-18T12:00:00+00:00"^^xsd:dateTime ;
	dct:modified "2021-02-18T12:00:00+00:00"^^xsd:dateTime  ;
	skos:exactMatch subj:04007002 ;
	skos:exactMatch <https://www.wikidata.org/entity/Q216107> ;
	skos:broader	medtop:20000252 .

medtop:20000247
	rdf:type skos:Concept ;
	skos:prefLabel	"online shopping"@en-GB ;
	skos:definition	"Buying and selling items through the internet"@en-GB ;
	skos:inScheme <http://cv.iptc.org/newscodes/mediatopic/>  ;
	ikos:created "2009-10-22T02:00:00+00:00"^^xsd:dateTime ;
	dct:created "2009-10-22T02:00:00+00:00"^^xsd:dateTime ;
	ikos:modified "2023-03-31T12:00:00+00:00"^^xsd:dateTime ;
	dct:modified "2023-03-31T12:00:00+00:00"^^xsd:dateTime  ;
	skos:exactMatch subj:04007009 ;
	skos:exactMatch <https://www.wikidata.org/entity/Q484847> ;
	skos:broader	medtop:20000252 .

medtop:20000248
	rdf:type skos:Concept ;
	skos:prefLabel	"grocery"@en-GB ;
	skos:definition	"The selling of edible goods for human consumption to the end customers"@en-GB ;
	skos:changeNote	"Retired. Use medtop:20000324 beverage and grocery instead."@en-GB ;
	skos:inScheme <http://cv.iptc.org/newscodes/mediatopic/>  ;
	ikos:created "2009-10-22T02:00:00+00:00"^^xsd:dateTime ;
	dct:created "2009-10-22T02:00:00+00:00"^^xsd:dateTime ;
	ikos:modified "2023-03-31T12:00:00+00:00"^^xsd:dateTime ;
	dct:modified "2023-03-31T12:00:00+00:00"^^xsd:dateTime  ; 
	ikos:retired "2023-03-31T12:00:00+00:00"^^xsd:dateTime ;
	skos:exactMatch subj:04007003 ;
	skos:exactMatch <https://www.wikidata.org/entity/Q2095> ;
	skos:broader	medtop:20000243 .

medtop:20000249
	rdf:type skos:Concept ;
	skos:prefLabel	"luxury good"@en-GB ;
	skos:definition	"Non-essential high-end goods, such as leather bags, jewellery or supercars"@en-GB ;
	skos:inScheme <http://cv.iptc.org/newscodes/mediatopic/>  ;
	ikos:created "2009-10-22T02:00:00+00:00"^^xsd:dateTime ;
	dct:created "2009-10-22T02:00:00+00:00"^^xsd:dateTime ;
	ikos:modified "2023-03-31T12:00:00+00:00"^^xsd:dateTime ;
	dct:modified "2023-03-31T12:00:00+00:00"^^xsd:dateTime  ;
	skos:exactMatch subj:04007010 ;
	skos:exactMatch <https://www.wikidata.org/entity/Q949715> ;
	skos:broader	medtop:20000243 .

medtop:20000250
	rdf:type skos:Concept ;
	skos:prefLabel	"mail order"@en-GB ;
	skos:definition	"Items sold through and delivered by mail"@en-GB ;
	skos:changeNote	"Retired. Use medtop:20000247 online shopping instead."@en-GB ;
	skos:inScheme <http://cv.iptc.org/newscodes/mediatopic/>  ;
	ikos:created "2009-10-22T02:00:00+00:00"^^xsd:dateTime ;
	dct:created "2009-10-22T02:00:00+00:00"^^xsd:dateTime ;
	ikos:modified "2023-03-31T12:00:00+00:00"^^xsd:dateTime ;
	dct:modified "2023-03-31T12:00:00+00:00"^^xsd:dateTime  ; 
	ikos:retired "2023-03-31T12:00:00+00:00"^^xsd:dateTime ;
	skos:exactMatch subj:04007004 ;
	skos:exactMatch <https://www.wikidata.org/entity/Q425779> ;
	skos:broader	medtop:20000252 .

medtop:20000251
	rdf:type skos:Concept ;
	skos:prefLabel	"non-durable good"@en-GB ;
	skos:definition	"Products meant to only be used for a short period of time"@en-GB ;
	skos:changeNote	"Retired. Use medtop:20000243 consumer goods instead."@en-GB ;
	skos:inScheme <http://cv.iptc.org/newscodes/mediatopic/>  ;
	ikos:created "2009-10-22T02:00:00+00:00"^^xsd:dateTime ;
	dct:created "2009-10-22T02:00:00+00:00"^^xsd:dateTime ;
	ikos:modified "2023-03-31T12:00:00+00:00"^^xsd:dateTime ;
	dct:modified "2023-03-31T12:00:00+00:00"^^xsd:dateTime  ; 
	ikos:retired "2023-03-31T12:00:00+00:00"^^xsd:dateTime ;
	skos:exactMatch subj:04007011 ;
	skos:exactMatch <https://www.wikidata.org/entity/Q1681365> ;
	skos:broader	medtop:20000243 .

medtop:20000252
	rdf:type skos:Concept ;
	skos:prefLabel	"retail"@en-GB ;
	skos:definition	"The selling of goods directly to consumers"@en-GB ;
	skos:inScheme <http://cv.iptc.org/newscodes/mediatopic/>  ;
	ikos:created "2009-10-22T02:00:00+00:00"^^xsd:dateTime ;
	dct:created "2009-10-22T02:00:00+00:00"^^xsd:dateTime ;
	ikos:modified "2023-03-31T12:00:00+00:00"^^xsd:dateTime ;
	dct:modified "2023-03-31T12:00:00+00:00"^^xsd:dateTime  ;
	skos:exactMatch subj:04007005 ;
	skos:exactMatch <https://www.wikidata.org/entity/Q126793> ;
	skos:broader	medtop:20001289 ;
	skos:narrower	medtop:20000246 ;
	skos:narrower	medtop:20000247 ;
	skos:narrower	medtop:20000250 ;
	skos:narrower	medtop:20000253 ;
	skos:narrower	medtop:20001296 ;
	skos:narrower	medtop:20001297 .

medtop:20000253
	rdf:type skos:Concept ;
	skos:prefLabel	"specialty store"@en-GB ;
	skos:definition	"Retail outlets that specialise in categories such as shoes, coats, power tools, etc"@en-GB ;
	skos:inScheme <http://cv.iptc.org/newscodes/mediatopic/>  ;
	ikos:created "2009-10-22T02:00:00+00:00"^^xsd:dateTime ;
	dct:created "2009-10-22T02:00:00+00:00"^^xsd:dateTime ;
	ikos:modified "2021-05-05T12:00:00+00:00"^^xsd:dateTime ;
	dct:modified "2021-05-05T12:00:00+00:00"^^xsd:dateTime  ;
	skos:exactMatch subj:04007006 ;
	skos:exactMatch <https://www.wikidata.org/entity/Q57335508> ;
	skos:broader	medtop:20000252 .

medtop:20000254
	rdf:type skos:Concept ;
	skos:prefLabel	"toy and game"@en-GB ;
	skos:definition	"Children's playthings or collectible items for adults, such as dolls, action figures and miniatures"@en-GB ;
	skos:inScheme <http://cv.iptc.org/newscodes/mediatopic/>  ;
	ikos:created "2009-10-22T02:00:00+00:00"^^xsd:dateTime ;
	dct:created "2009-10-22T02:00:00+00:00"^^xsd:dateTime ;
	ikos:modified "2023-03-31T12:00:00+00:00"^^xsd:dateTime ;
	dct:modified "2023-03-31T12:00:00+00:00"^^xsd:dateTime  ;
	skos:exactMatch subj:04007012 ;
	skos:exactMatch <https://www.wikidata.org/entity/Q11422> ;
	skos:broader	medtop:20000243 .

medtop:20000255
	rdf:type skos:Concept ;
	skos:prefLabel	"wholesale"@en-GB ;
	skos:definition	"The first link in the sales chain after production"@en-GB ;
	skos:inScheme <http://cv.iptc.org/newscodes/mediatopic/>  ;
	ikos:created "2009-10-22T02:00:00+00:00"^^xsd:dateTime ;
	dct:created "2009-10-22T02:00:00+00:00"^^xsd:dateTime ;
	ikos:modified "2023-03-31T12:00:00+00:00"^^xsd:dateTime ;
	dct:modified "2023-03-31T12:00:00+00:00"^^xsd:dateTime  ;
	skos:exactMatch subj:04007007 ;
	skos:exactMatch <https://www.wikidata.org/entity/Q220695> ;
	skos:broader	medtop:20001289 .

medtop:20000256
	rdf:type skos:Concept ;
	skos:prefLabel	"energy and resource"@en-GB ;
	skos:definition	"The use of natural resources to generate energy"@en-GB ;
	skos:inScheme <http://cv.iptc.org/newscodes/mediatopic/>  ;
	ikos:created "2009-10-22T02:00:00+00:00"^^xsd:dateTime ;
	dct:created "2009-10-22T02:00:00+00:00"^^xsd:dateTime ;
	ikos:modified "2023-03-31T12:00:00+00:00"^^xsd:dateTime ;
	dct:modified "2023-03-31T12:00:00+00:00"^^xsd:dateTime  ;
	skos:exactMatch subj:04005000 ;
	skos:exactMatch <https://www.wikidata.org/entity/Q2151621> ;
	skos:broader	medtop:20000209 ;
	skos:narrower	medtop:20000257 ;
	skos:narrower	medtop:20000258 ;
	skos:narrower	medtop:20000261 ;
	skos:narrower	medtop:20000265 ;
	skos:narrower	medtop:20000266 ;
	skos:narrower	medtop:20000267 ;
	skos:narrower	medtop:20001207 ;
	skos:narrower	medtop:20001243 .

medtop:20000257
	rdf:type skos:Concept ;
	skos:prefLabel	"renewable energy"@en-GB ;
	skos:definition	"Energy derived from sustainable sources"@en-GB ;
	skos:inScheme <http://cv.iptc.org/newscodes/mediatopic/>  ;
	ikos:created "2009-10-22T02:00:00+00:00"^^xsd:dateTime ;
	dct:created "2009-10-22T02:00:00+00:00"^^xsd:dateTime ;
	ikos:modified "2023-03-31T12:00:00+00:00"^^xsd:dateTime ;
	dct:modified "2023-03-31T12:00:00+00:00"^^xsd:dateTime  ;
	skos:exactMatch subj:04005001 ;
	skos:exactMatch <https://www.wikidata.org/entity/Q4202245> ;
	skos:broader	medtop:20000256 ;
	skos:narrower	medtop:20001208 ;
	skos:narrower	medtop:20001209 ;
	skos:narrower	medtop:20001210 ;
	skos:narrower	medtop:20001211 .

medtop:20000258
	rdf:type skos:Concept ;
	skos:prefLabel	"coal"@en-GB ;
	skos:definition	"Production and mining of anthracite and bituminous products for use in power production"@en-GB ;
	skos:inScheme <http://cv.iptc.org/newscodes/mediatopic/>  ;
	ikos:created "2009-10-22T02:00:00+00:00"^^xsd:dateTime ;
	dct:created "2009-10-22T02:00:00+00:00"^^xsd:dateTime ;
	ikos:modified "2021-02-18T12:00:00+00:00"^^xsd:dateTime ;
	dct:modified "2021-02-18T12:00:00+00:00"^^xsd:dateTime  ;
	skos:exactMatch subj:04005002 ;
	skos:exactMatch <https://www.wikidata.org/entity/Q1778629> ;
	skos:broader	medtop:20000256 .

medtop:20000259
	rdf:type skos:Concept ;
	skos:prefLabel	"diesel fuel"@en-GB ;
	skos:definition	"A distilled petroleum product heavier than gasoline used for trucks, marine engines, certain cars and in some forms for home heating"@en-GB ;
	skos:inScheme <http://cv.iptc.org/newscodes/mediatopic/>  ;
	ikos:created "2009-10-22T02:00:00+00:00"^^xsd:dateTime ;
	dct:created "2009-10-22T02:00:00+00:00"^^xsd:dateTime ;
	ikos:modified "2023-03-31T12:00:00+00:00"^^xsd:dateTime ;
	dct:modified "2023-03-31T12:00:00+00:00"^^xsd:dateTime  ;
	skos:exactMatch subj:04005013 ;
	skos:exactMatch <https://www.wikidata.org/entity/Q38423> ;
	skos:broader	medtop:20001243 .

medtop:20000260
	rdf:type skos:Concept ;
	skos:prefLabel	"electricity"@en-GB ;
	skos:definition	"The power line distribution system and the sale of electrical power at wholesale and retail levels"@en-GB ;
	skos:inScheme <http://cv.iptc.org/newscodes/mediatopic/>  ;
	ikos:created "2009-10-22T02:00:00+00:00"^^xsd:dateTime ;
	dct:created "2009-10-22T02:00:00+00:00"^^xsd:dateTime ;
	ikos:modified "2023-03-31T12:00:00+00:00"^^xsd:dateTime ;
	dct:modified "2023-03-31T12:00:00+00:00"^^xsd:dateTime  ;
	skos:exactMatch subj:04005006 ;
	skos:exactMatch <https://www.wikidata.org/entity/Q2316331> ;
	skos:broader	medtop:20001244 .

medtop:20000261
	rdf:type skos:Concept ;
	skos:prefLabel	"energy industry"@en-GB ;
	skos:definition	"The energy industry, not focused on any specific sector"@en-GB ;
	skos:inScheme <http://cv.iptc.org/newscodes/mediatopic/>  ;
	ikos:created "2009-10-22T02:00:00+00:00"^^xsd:dateTime ;
	dct:created "2009-10-22T02:00:00+00:00"^^xsd:dateTime ;
	ikos:modified "2021-07-12T12:00:00+00:00"^^xsd:dateTime ;
	dct:modified "2021-07-12T12:00:00+00:00"^^xsd:dateTime  ; 
	ikos:retired "2019-07-25T12:00:00+00:00"^^xsd:dateTime ;
	skos:closeMatch subj:04005000 ;
	skos:exactMatch <https://www.wikidata.org/entity/Q2151621> ;
	skos:broader	medtop:20000256 .

medtop:20000262
	rdf:type skos:Concept ;
	skos:prefLabel	"kerosene/paraffin"@en-GB ;
	skos:definition	"A light petroleum distillate used for cooking fuel, aircraft jet engines, lamps, heating and cleaning"@en-GB ;
	skos:changeNote	"Retired. Use medtop:20001243 oil and gas instead."@en-GB ;
	skos:inScheme <http://cv.iptc.org/newscodes/mediatopic/>  ;
	ikos:created "2009-10-22T02:00:00+00:00"^^xsd:dateTime ;
	dct:created "2009-10-22T02:00:00+00:00"^^xsd:dateTime ;
	ikos:modified "2023-03-31T12:00:00+00:00"^^xsd:dateTime ;
	dct:modified "2023-03-31T12:00:00+00:00"^^xsd:dateTime  ; 
	ikos:retired "2023-03-31T12:00:00+00:00"^^xsd:dateTime ;
	skos:exactMatch subj:04005014 ;
	skos:exactMatch <https://www.wikidata.org/entity/Q76904> ;
	skos:broader	medtop:20001243 .

medtop:20000263
	rdf:type skos:Concept ;
	skos:prefLabel	"natural gas"@en-GB ;
	skos:definition	"A natural resource, mainly methane in a flammable gaseous state extracted from the ground"@en-GB ;
	skos:inScheme <http://cv.iptc.org/newscodes/mediatopic/>  ;
	ikos:created "2009-10-22T02:00:00+00:00"^^xsd:dateTime ;
	dct:created "2009-10-22T02:00:00+00:00"^^xsd:dateTime ;
	ikos:modified "2023-03-31T12:00:00+00:00"^^xsd:dateTime ;
	dct:modified "2023-03-31T12:00:00+00:00"^^xsd:dateTime  ;
	skos:exactMatch subj:04005011 ;
	skos:exactMatch <https://www.wikidata.org/entity/Q40858> ;
	skos:broader	medtop:20001243 .

medtop:20000265
	rdf:type skos:Concept ;
	skos:prefLabel	"nuclear power"@en-GB ;
	skos:definition	"Use of radioactive materials for power production"@en-GB ;
	skos:inScheme <http://cv.iptc.org/newscodes/mediatopic/>  ;
	ikos:created "2009-10-22T02:00:00+00:00"^^xsd:dateTime ;
	dct:created "2009-10-22T02:00:00+00:00"^^xsd:dateTime ;
	ikos:modified "2021-07-12T12:00:00+00:00"^^xsd:dateTime ;
	dct:modified "2021-07-12T12:00:00+00:00"^^xsd:dateTime  ;
	skos:exactMatch subj:04005005 ;
	skos:exactMatch <https://www.wikidata.org/entity/Q12739> ;
	skos:broader	medtop:20000256 .

medtop:20000266
	rdf:type skos:Concept ;
	skos:prefLabel	"oil and gas - downstream activities"@en-GB ;
	skos:definition	"All matters concerning oil and gas, typically refining and distribution activities"@en-GB ;
	skos:inScheme <http://cv.iptc.org/newscodes/mediatopic/>  ;
	ikos:created "2009-10-22T02:00:00+00:00"^^xsd:dateTime ;
	dct:created "2009-10-22T02:00:00+00:00"^^xsd:dateTime ;
	ikos:modified "2021-05-05T12:00:00+00:00"^^xsd:dateTime ;
	dct:modified "2021-05-05T12:00:00+00:00"^^xsd:dateTime  ; 
	ikos:retired "2019-07-25T12:00:00+00:00"^^xsd:dateTime ;
	skos:exactMatch subj:04005003 ;
	skos:exactMatch <https://www.wikidata.org/entity/Q3444730> ;
	skos:broader	medtop:20000256 .

medtop:20000267
	rdf:type skos:Concept ;
	skos:prefLabel	"oil and gas - upstream activities"@en-GB ;
	skos:definition	"All matters concerning oil and gas, typically supply chain activities from the reservoir to the refinery gate"@en-GB ;
	skos:inScheme <http://cv.iptc.org/newscodes/mediatopic/>  ;
	ikos:created "2009-10-22T02:00:00+00:00"^^xsd:dateTime ;
	dct:created "2009-10-22T02:00:00+00:00"^^xsd:dateTime ;
	ikos:modified "2021-05-05T12:00:00+00:00"^^xsd:dateTime ;
	dct:modified "2021-05-05T12:00:00+00:00"^^xsd:dateTime  ; 
	ikos:retired "2019-07-25T12:00:00+00:00"^^xsd:dateTime ;
	skos:exactMatch subj:04005004 ;
	skos:exactMatch <https://www.wikidata.org/entity/Q2542096> ;
	skos:broader	medtop:20000256 .

medtop:20000268
	rdf:type skos:Concept ;
	skos:prefLabel	"petrol"@en-GB ;
	skos:definition	"Distilled petroleum product used for automotive fuel, with or without additives"@en-GB ;
	skos:inScheme <http://cv.iptc.org/newscodes/mediatopic/>  ;
	ikos:created "2009-10-22T02:00:00+00:00"^^xsd:dateTime ;
	dct:created "2009-10-22T02:00:00+00:00"^^xsd:dateTime ;
	ikos:modified "2021-02-18T12:00:00+00:00"^^xsd:dateTime ;
	dct:modified "2021-02-18T12:00:00+00:00"^^xsd:dateTime  ;
	skos:exactMatch subj:04005012 ;
	skos:exactMatch <https://www.wikidata.org/entity/Q39558> ;
	skos:broader	medtop:20001243 .

medtop:20000269
	rdf:type skos:Concept ;
	skos:prefLabel	"waste management"@en-GB ;
	skos:definition	"The collecting, disposing or recycling of household and business waste"@en-GB ;
	skos:inScheme <http://cv.iptc.org/newscodes/mediatopic/>  ;
	ikos:created "2009-10-22T02:00:00+00:00"^^xsd:dateTime ;
	dct:created "2009-10-22T02:00:00+00:00"^^xsd:dateTime ;
	ikos:modified "2023-03-31T12:00:00+00:00"^^xsd:dateTime ;
	dct:modified "2023-03-31T12:00:00+00:00"^^xsd:dateTime  ;
	skos:exactMatch subj:04005007 ;
	skos:exactMatch <https://www.wikidata.org/entity/Q180388> ;
	skos:broader	medtop:20001244 .

medtop:20000270
	rdf:type skos:Concept ;
	skos:prefLabel	"water supply"@en-GB ;
	skos:definition	"The business of providing water for household and commercial use"@en-GB ;
	skos:inScheme <http://cv.iptc.org/newscodes/mediatopic/>  ;
	ikos:created "2009-10-22T02:00:00+00:00"^^xsd:dateTime ;
	dct:created "2009-10-22T02:00:00+00:00"^^xsd:dateTime ;
	ikos:modified "2023-03-31T12:00:00+00:00"^^xsd:dateTime ;
	dct:modified "2023-03-31T12:00:00+00:00"^^xsd:dateTime  ;
	skos:exactMatch subj:04005008 ;
	skos:exactMatch <https://www.wikidata.org/entity/Q1061108> ;
	skos:broader	medtop:20001244 .

medtop:20000271
	rdf:type skos:Concept ;
	skos:prefLabel	"financial and business service"@en-GB ;
	skos:definition	"Services that transmit, safeguard, keep track of money or provide backup to commercial enterprises"@en-GB ;
	skos:changeNote	"Retired. Use medtop:20001370 financial service or medtop:20001371 business service instead."@en-GB ;
	skos:inScheme <http://cv.iptc.org/newscodes/mediatopic/>  ;
	ikos:created "2009-10-22T02:00:00+00:00"^^xsd:dateTime ;
	dct:created "2009-10-22T02:00:00+00:00"^^xsd:dateTime ;
	ikos:modified "2023-03-31T12:00:00+00:00"^^xsd:dateTime ;
	dct:modified "2023-03-31T12:00:00+00:00"^^xsd:dateTime  ; 
	ikos:retired "2023-03-31T12:00:00+00:00"^^xsd:dateTime ;
	skos:exactMatch subj:04006000 ;
	skos:exactMatch <https://www.wikidata.org/entity/Q837171> ;
	skos:broader	medtop:20000209 ;
	skos:narrower	medtop:20000277 ;
	skos:narrower	medtop:20000285 ;
	skos:narrower	medtop:20000286 ;
	skos:narrower	medtop:20000289 .

medtop:20000272
	rdf:type skos:Concept ;
	skos:prefLabel	"accountancy and auditing"@en-GB ;
	skos:definition	"Companies that provide balance sheet preparation and budget reconciliation services and examine accuracy of financial statements"@en-GB ;
	skos:inScheme <http://cv.iptc.org/newscodes/mediatopic/>  ;
	ikos:created "2009-10-22T02:00:00+00:00"^^xsd:dateTime ;
	dct:created "2009-10-22T02:00:00+00:00"^^xsd:dateTime ;
	ikos:modified "2023-03-31T12:00:00+00:00"^^xsd:dateTime ;
	dct:modified "2023-03-31T12:00:00+00:00"^^xsd:dateTime  ;
	skos:exactMatch subj:04006001 ;
	skos:exactMatch <https://www.wikidata.org/entity/Q4116214> ;
	skos:broader	medtop:20001370 .

medtop:20000273
	rdf:type skos:Concept ;
	skos:prefLabel	"auction"@en-GB ;
	skos:definition	"Auction houses and all types of auctions, such as police auctions and silent auctions"@en-GB ;
	skos:inScheme <http://cv.iptc.org/newscodes/mediatopic/>  ;
	ikos:created "2009-10-22T02:00:00+00:00"^^xsd:dateTime ;
	dct:created "2009-10-22T02:00:00+00:00"^^xsd:dateTime ;
	ikos:modified "2023-03-31T12:00:00+00:00"^^xsd:dateTime ;
	dct:modified "2023-03-31T12:00:00+00:00"^^xsd:dateTime  ;
	skos:exactMatch subj:04006020 ;
	skos:exactMatch <https://www.wikidata.org/entity/Q177923> ;
	skos:broader	medtop:20001289 .

medtop:20000274
	rdf:type skos:Concept ;
	skos:prefLabel	"banking"@en-GB ;
	skos:definition	"Financial institutions and services for storing, transmitting, receiving and delivering money"@en-GB ;
	skos:inScheme <http://cv.iptc.org/newscodes/mediatopic/>  ;
	ikos:created "2009-10-22T02:00:00+00:00"^^xsd:dateTime ;
	dct:created "2009-10-22T02:00:00+00:00"^^xsd:dateTime ;
	ikos:modified "2023-03-31T12:00:00+00:00"^^xsd:dateTime ;
	dct:modified "2023-03-31T12:00:00+00:00"^^xsd:dateTime  ;
	skos:exactMatch subj:04006002 ;
	skos:exactMatch <https://www.wikidata.org/entity/Q3435731> ;
	skos:broader	medtop:20001370 .

medtop:20000275
	rdf:type skos:Concept ;
	skos:prefLabel	"consultancy"@en-GB ;
	skos:definition	"Providers of expert knowledge in a wide range of fields usually on a temporary, contract basis"@en-GB ;
	skos:inScheme <http://cv.iptc.org/newscodes/mediatopic/>  ;
	ikos:created "2009-10-22T02:00:00+00:00"^^xsd:dateTime ;
	dct:created "2009-10-22T02:00:00+00:00"^^xsd:dateTime ;
	ikos:modified "2023-03-31T12:00:00+00:00"^^xsd:dateTime ;
	dct:modified "2023-03-31T12:00:00+00:00"^^xsd:dateTime  ;
	skos:exactMatch subj:04006003 ;
	skos:exactMatch <https://www.wikidata.org/entity/Q268626> ;
	skos:broader	medtop:20001371 .

medtop:20000276
	rdf:type skos:Concept ;
	skos:prefLabel	"employment agency"@en-GB ;
	skos:definition	"A service helping people find jobs, and companies to find workers"@en-GB ;
	skos:inScheme <http://cv.iptc.org/newscodes/mediatopic/>  ;
	ikos:created "2009-10-22T02:00:00+00:00"^^xsd:dateTime ;
	dct:created "2009-10-22T02:00:00+00:00"^^xsd:dateTime ;
	ikos:modified "2023-03-31T12:00:00+00:00"^^xsd:dateTime ;
	dct:modified "2023-03-31T12:00:00+00:00"^^xsd:dateTime  ;
	skos:exactMatch subj:04006004 ;
	skos:exactMatch <https://www.wikidata.org/entity/Q261362> ;
	skos:broader	medtop:20001371 .

medtop:20000277
	rdf:type skos:Concept ;
	skos:prefLabel	"funeral parlour and crematorium"@en-GB ;
	skos:definition	"Companies that provide services for disposal of the dead"@en-GB ;
	skos:changeNote	"Retired. Use medtop:20001235 funeral and memorial service instead."@en-GB ;
	skos:inScheme <http://cv.iptc.org/newscodes/mediatopic/>  ;
	ikos:created "2009-10-22T02:00:00+00:00"^^xsd:dateTime ;
	dct:created "2009-10-22T02:00:00+00:00"^^xsd:dateTime ;
	ikos:modified "2023-03-31T12:00:00+00:00"^^xsd:dateTime ;
	dct:modified "2023-03-31T12:00:00+00:00"^^xsd:dateTime  ; 
	ikos:retired "2023-03-31T12:00:00+00:00"^^xsd:dateTime ;
	skos:exactMatch subj:04006015 ;
	skos:broader	medtop:20000271 .

medtop:20000278
	rdf:type skos:Concept ;
	skos:prefLabel	"health care provider"@en-GB ;
	skos:definition	"Organisations and individuals that provide medical services at all levels"@en-GB ;
	skos:inScheme <http://cv.iptc.org/newscodes/mediatopic/>  ;
	ikos:created "2009-10-22T02:00:00+00:00"^^xsd:dateTime ;
	dct:created "2009-10-22T02:00:00+00:00"^^xsd:dateTime ;
	ikos:modified "2022-06-14T12:00:00+00:00"^^xsd:dateTime ;
	dct:modified "2022-06-14T12:00:00+00:00"^^xsd:dateTime  ;
	skos:exactMatch subj:04006005 ;
	skos:exactMatch <https://www.wikidata.org/entity/Q55645123> ;
	skos:broader	medtop:20001354 .

medtop:20000279
	rdf:type skos:Concept ;
	skos:prefLabel	"insurance"@en-GB ;
	skos:definition	"A risk-taking venture that allows individuals to pay small amounts periodically to guard financially against unexpected events"@en-GB ;
	skos:inScheme <http://cv.iptc.org/newscodes/mediatopic/>  ;
	ikos:created "2009-10-22T02:00:00+00:00"^^xsd:dateTime ;
	dct:created "2009-10-22T02:00:00+00:00"^^xsd:dateTime ;
	ikos:modified "2023-03-31T12:00:00+00:00"^^xsd:dateTime ;
	dct:modified "2023-03-31T12:00:00+00:00"^^xsd:dateTime  ;
	skos:exactMatch subj:04006006 ;
	skos:exactMatch <https://www.wikidata.org/entity/Q43183> ;
	skos:broader	medtop:20001370 .

medtop:20000280
	rdf:type skos:Concept ;
	skos:prefLabel	"financial advisory service"@en-GB ;
	skos:definition	"Financial advisers, as opposed to stock dealers or consultants"@en-GB ;
	skos:inScheme <http://cv.iptc.org/newscodes/mediatopic/>  ;
	ikos:created "2009-10-22T02:00:00+00:00"^^xsd:dateTime ;
	dct:created "2009-10-22T02:00:00+00:00"^^xsd:dateTime ;
	ikos:modified "2023-03-31T12:00:00+00:00"^^xsd:dateTime ;
	dct:modified "2023-03-31T12:00:00+00:00"^^xsd:dateTime  ;
	skos:exactMatch subj:04006022 ;
	skos:exactMatch <https://www.wikidata.org/entity/Q557705> ;
	skos:broader	medtop:20001370 .

medtop:20000281
	rdf:type skos:Concept ;
	skos:prefLabel	"janitorial service"@en-GB ;
	skos:definition	"Companies that provide cleaning and similar services for homes and businesses."@en-GB ;
	skos:changeNote	"Retired."@en-GB ;
	skos:inScheme <http://cv.iptc.org/newscodes/mediatopic/>  ;
	ikos:created "2009-10-22T02:00:00+00:00"^^xsd:dateTime ;
	dct:created "2009-10-22T02:00:00+00:00"^^xsd:dateTime ;
	ikos:modified "2023-03-31T12:00:00+00:00"^^xsd:dateTime ;
	dct:modified "2023-03-31T12:00:00+00:00"^^xsd:dateTime  ; 
	ikos:retired "2023-03-31T12:00:00+00:00"^^xsd:dateTime ;
	skos:exactMatch subj:04006014 ;
	skos:exactMatch <https://www.wikidata.org/entity/Q6735317> ;
	skos:broader	medtop:20001371 .

medtop:20000282
	rdf:type skos:Concept ;
	skos:prefLabel	"legal service"@en-GB ;
	skos:definition	"Lawyers, notaries and others who help companies and individuals deal with state, federal and local laws"@en-GB ;
	skos:changeNote	"2016-04-04: definition slightly modified."@en-GB ;
	skos:inScheme <http://cv.iptc.org/newscodes/mediatopic/>  ;
	ikos:created "2009-10-22T02:00:00+00:00"^^xsd:dateTime ;
	dct:created "2009-10-22T02:00:00+00:00"^^xsd:dateTime ;
	ikos:modified "2023-03-31T12:00:00+00:00"^^xsd:dateTime ;
	dct:modified "2023-03-31T12:00:00+00:00"^^xsd:dateTime  ;
	skos:exactMatch subj:04006007 ;
	skos:exactMatch <https://www.wikidata.org/entity/Q1494322> ;
	skos:broader	medtop:20001371 .

medtop:20000283
	rdf:type skos:Concept ;
	skos:prefLabel	"market research"@en-GB ;
	skos:definition	"Gathering information about the needs and wants of consumers"@en-GB ;
	skos:inScheme <http://cv.iptc.org/newscodes/mediatopic/>  ;
	ikos:created "2009-10-22T02:00:00+00:00"^^xsd:dateTime ;
	dct:created "2009-10-22T02:00:00+00:00"^^xsd:dateTime ;
	ikos:modified "2023-03-31T12:00:00+00:00"^^xsd:dateTime ;
	dct:modified "2023-03-31T12:00:00+00:00"^^xsd:dateTime  ;
	skos:exactMatch subj:04006008 ;
	skos:exactMatch <https://www.wikidata.org/entity/Q913709> ;
	skos:broader	medtop:20000192 .

medtop:20000284
	rdf:type skos:Concept ;
	skos:prefLabel	"market trend"@en-GB ;
	skos:definition	"Statistically significant consumer behaviour."@en-GB ;
	skos:inScheme <http://cv.iptc.org/newscodes/mediatopic/>  ;
	ikos:created "2009-10-22T02:00:00+00:00"^^xsd:dateTime ;
	dct:created "2009-10-22T02:00:00+00:00"^^xsd:dateTime ;
	ikos:modified "2023-03-31T12:00:00+00:00"^^xsd:dateTime ;
	dct:modified "2023-03-31T12:00:00+00:00"^^xsd:dateTime  ;
	skos:exactMatch subj:04006011 ;
	skos:exactMatch <https://www.wikidata.org/entity/Q1004322> ;
	skos:broader	medtop:20000192 .

medtop:20000285
	rdf:type skos:Concept ;
	skos:prefLabel	"personal finance"@en-GB ;
	skos:definition	"An individual's income and expenses"@en-GB ;
	skos:inScheme <http://cv.iptc.org/newscodes/mediatopic/>  ;
	ikos:created "2009-10-22T02:00:00+00:00"^^xsd:dateTime ;
	dct:created "2009-10-22T02:00:00+00:00"^^xsd:dateTime ;
	ikos:modified "2023-03-31T12:00:00+00:00"^^xsd:dateTime ;
	dct:modified "2023-03-31T12:00:00+00:00"^^xsd:dateTime  ; 
	ikos:retired "2023-03-31T12:00:00+00:00"^^xsd:dateTime ;
	skos:exactMatch subj:04006018 ;
	skos:exactMatch <https://www.wikidata.org/entity/Q253613> ;
	skos:broader	medtop:20000271 .

medtop:20000286
	rdf:type skos:Concept ;
	skos:prefLabel	"personal income"@en-GB ;
	skos:definition	"Money that a person earns and is his/hers to keep or spend"@en-GB ;
	skos:inScheme <http://cv.iptc.org/newscodes/mediatopic/>  ;
	ikos:created "2009-10-22T02:00:00+00:00"^^xsd:dateTime ;
	dct:created "2009-10-22T02:00:00+00:00"^^xsd:dateTime ;
	ikos:modified "2023-03-31T12:00:00+00:00"^^xsd:dateTime ;
	dct:modified "2023-03-31T12:00:00+00:00"^^xsd:dateTime  ; 
	ikos:retired "2023-03-31T12:00:00+00:00"^^xsd:dateTime ;
	skos:exactMatch subj:04006019 ;
	skos:exactMatch <https://www.wikidata.org/entity/Q7170591> ;
	skos:broader	medtop:20000271 .

medtop:20000287
	rdf:type skos:Concept ;
	skos:prefLabel	"personal finance and investment"@en-GB ;
	skos:definition	"Investing an individual's savings in the hope of future gains"@en-GB ;
	skos:inScheme <http://cv.iptc.org/newscodes/mediatopic/>  ;
	ikos:created "2009-10-22T02:00:00+00:00"^^xsd:dateTime ;
	dct:created "2009-10-22T02:00:00+00:00"^^xsd:dateTime ;
	ikos:modified "2023-03-31T12:00:00+00:00"^^xsd:dateTime ;
	dct:modified "2023-03-31T12:00:00+00:00"^^xsd:dateTime  ;
	skos:exactMatch subj:04006010 ;
	skos:exactMatch <https://www.wikidata.org/entity/Q253613> ;
	skos:broader	medtop:20001370 .

medtop:20000288
	rdf:type skos:Concept ;
	skos:prefLabel	"personal service"@en-GB ;
	skos:definition	"Consumer service that is intangible e.g. beauty care such as hairdressing"@en-GB ;
	skos:changeNote	"Retired. Use medtop:20001249 hairstyles or medtop:20000220 cosmetics instead."@en-GB ;
	skos:inScheme <http://cv.iptc.org/newscodes/mediatopic/>  ;
	ikos:created "2009-10-22T02:00:00+00:00"^^xsd:dateTime ;
	dct:created "2009-10-22T02:00:00+00:00"^^xsd:dateTime ;
	ikos:modified "2023-03-31T12:00:00+00:00"^^xsd:dateTime ;
	dct:modified "2023-03-31T12:00:00+00:00"^^xsd:dateTime  ; 
	ikos:retired "2023-03-31T12:00:00+00:00"^^xsd:dateTime ;
	skos:exactMatch subj:04006013 ;
	skos:broader	medtop:20001371 .

medtop:20000289
	rdf:type skos:Concept ;
	skos:prefLabel	"printing service"@en-GB ;
	skos:definition	"The production of printed matter such as flyers, ads, signs, etc."@en-GB ;
	skos:inScheme <http://cv.iptc.org/newscodes/mediatopic/>  ;
	ikos:created "2009-10-22T02:00:00+00:00"^^xsd:dateTime ;
	dct:created "2009-10-22T02:00:00+00:00"^^xsd:dateTime ;
	ikos:modified "2023-03-31T12:00:00+00:00"^^xsd:dateTime ;
	dct:modified "2023-03-31T12:00:00+00:00"^^xsd:dateTime  ; 
	ikos:retired "2023-03-31T12:00:00+00:00"^^xsd:dateTime ;
	skos:exactMatch subj:04006021 ;
	skos:exactMatch <https://www.wikidata.org/entity/Q47003909> ;
	skos:broader	medtop:20000271 .

medtop:20000290
	rdf:type skos:Concept ;
	skos:prefLabel	"rental service"@en-GB ;
	skos:definition	"Companies that provide items on a short-term rental basis, including motor vehicles, clothing, tools, heavy equipment and other supplies"@en-GB ;
	skos:inScheme <http://cv.iptc.org/newscodes/mediatopic/>  ;
	ikos:created "2009-10-22T02:00:00+00:00"^^xsd:dateTime ;
	dct:created "2009-10-22T02:00:00+00:00"^^xsd:dateTime ;
	ikos:modified "2023-03-31T12:00:00+00:00"^^xsd:dateTime ;
	dct:modified "2023-03-31T12:00:00+00:00"^^xsd:dateTime  ;
	skos:exactMatch subj:04006016 ;
	skos:broader	medtop:20001371 .

medtop:20000291
	rdf:type skos:Concept ;
	skos:prefLabel	"shipping and postal service"@en-GB ;
	skos:definition	"Organisations that prepare and transport packages and documents for individuals or companies by any means, including postal services"@en-GB ;
	skos:inScheme <http://cv.iptc.org/newscodes/mediatopic/>  ;
	ikos:created "2009-10-22T02:00:00+00:00"^^xsd:dateTime ;
	dct:created "2009-10-22T02:00:00+00:00"^^xsd:dateTime ;
	ikos:modified "2023-03-31T12:00:00+00:00"^^xsd:dateTime ;
	dct:modified "2023-03-31T12:00:00+00:00"^^xsd:dateTime  ;
	skos:exactMatch subj:04006012 ;
	skos:exactMatch <https://www.wikidata.org/entity/Q1447463> ;
	skos:broader	medtop:20001371 .

medtop:20000292
	rdf:type skos:Concept ;
	skos:prefLabel	"stock broking"@en-GB ;
	skos:definition	"The buying and selling of company shares on behalf of individuals or other entities"@en-GB ;
	skos:inScheme <http://cv.iptc.org/newscodes/mediatopic/>  ;
	ikos:created "2009-10-22T02:00:00+00:00"^^xsd:dateTime ;
	dct:created "2009-10-22T02:00:00+00:00"^^xsd:dateTime ;
	ikos:modified "2023-03-31T12:00:00+00:00"^^xsd:dateTime ;
	dct:modified "2023-03-31T12:00:00+00:00"^^xsd:dateTime  ;
	skos:exactMatch subj:04006009 ;
	skos:exactMatch <https://www.wikidata.org/entity/Q2073644> ;
	skos:broader	medtop:20001370 .

medtop:20000293
	rdf:type skos:Concept ;
	skos:prefLabel	"wedding service"@en-GB ;
	skos:definition	"Services and products related to the wedding industry"@en-GB ;
	skos:changeNote	"Retired. Use medtop:20001236 wedding instead."@en-GB ;
	skos:inScheme <http://cv.iptc.org/newscodes/mediatopic/>  ;
	ikos:created "2009-10-22T02:00:00+00:00"^^xsd:dateTime ;
	dct:created "2009-10-22T02:00:00+00:00"^^xsd:dateTime ;
	ikos:modified "2023-03-31T12:00:00+00:00"^^xsd:dateTime ;
	dct:modified "2023-03-31T12:00:00+00:00"^^xsd:dateTime  ; 
	ikos:retired "2023-03-31T12:00:00+00:00"^^xsd:dateTime ;
	skos:exactMatch subj:04006017 ;
	skos:exactMatch <https://www.wikidata.org/entity/Q25421835> ;
	skos:broader	medtop:20001371 .

medtop:20000294
	rdf:type skos:Concept ;
	skos:prefLabel	"manufacturing and engineering"@en-GB ;
	skos:definition	"Manufacturers of electrical, electronic and mechanical equipment but does not cover civil engineering."@en-GB ;
	skos:inScheme <http://cv.iptc.org/newscodes/mediatopic/>  ;
	ikos:created "2009-10-22T02:00:00+00:00"^^xsd:dateTime ;
	dct:created "2009-10-22T02:00:00+00:00"^^xsd:dateTime ;
	ikos:modified "2021-02-18T12:00:00+00:00"^^xsd:dateTime ;
	dct:modified "2021-02-18T12:00:00+00:00"^^xsd:dateTime  ;
	skos:exactMatch subj:04011000 ;
	skos:exactMatch <https://www.wikidata.org/entity/Q187939> ;
	skos:broader	medtop:20000209 ;
	skos:narrower	medtop:20000295 ;
	skos:narrower	medtop:20000296 ;
	skos:narrower	medtop:20000297 ;
	skos:narrower	medtop:20000298 ;
	skos:narrower	medtop:20000299 ;
	skos:narrower	medtop:20000300 ;
	skos:narrower	medtop:20000301 ;
	skos:narrower	medtop:20000302 ;
	skos:narrower	medtop:20000303 ;
	skos:narrower	medtop:20001165 ;
	skos:narrower	medtop:20001166 .

medtop:20000295
	rdf:type skos:Concept ;
	skos:prefLabel	"aerospace"@en-GB ;
	skos:definition	"Companies that assemble or manufacture components for airplanes and space ships."@en-GB ;
	skos:inScheme <http://cv.iptc.org/newscodes/mediatopic/>  ;
	ikos:created "2009-10-22T02:00:00+00:00"^^xsd:dateTime ;
	dct:created "2009-10-22T02:00:00+00:00"^^xsd:dateTime ;
	ikos:modified "2021-02-18T12:00:00+00:00"^^xsd:dateTime ;
	dct:modified "2021-02-18T12:00:00+00:00"^^xsd:dateTime  ;
	skos:exactMatch subj:04011001 ;
	skos:exactMatch <https://www.wikidata.org/entity/Q3477363> ;
	skos:broader	medtop:20000294 .

medtop:20000296
	rdf:type skos:Concept ;
	skos:prefLabel	"automotive"@en-GB ;
	skos:definition	"Companies that manufacture automotive components and assemble automobiles"@en-GB ;
	skos:inScheme <http://cv.iptc.org/newscodes/mediatopic/>  ;
	ikos:created "2009-10-22T02:00:00+00:00"^^xsd:dateTime ;
	dct:created "2009-10-22T02:00:00+00:00"^^xsd:dateTime ;
	ikos:modified "2021-02-18T12:00:00+00:00"^^xsd:dateTime ;
	dct:modified "2021-02-18T12:00:00+00:00"^^xsd:dateTime  ;
	skos:exactMatch subj:04011002 ;
	skos:exactMatch <https://www.wikidata.org/entity/Q190117> ;
	skos:broader	medtop:20000294 .

medtop:20000297
	rdf:type skos:Concept ;
	skos:prefLabel	"defence equipment"@en-GB ;
	skos:definition	"Manufacturers of guns, tanks, ships or other equipment for military and non-military protection services"@en-GB ;
	skos:inScheme <http://cv.iptc.org/newscodes/mediatopic/>  ;
	ikos:created "2009-10-22T02:00:00+00:00"^^xsd:dateTime ;
	dct:created "2009-10-22T02:00:00+00:00"^^xsd:dateTime ;
	ikos:modified "2023-03-31T12:00:00+00:00"^^xsd:dateTime ;
	dct:modified "2023-03-31T12:00:00+00:00"^^xsd:dateTime  ;
	skos:exactMatch subj:04011003 ;
	skos:exactMatch <https://www.wikidata.org/entity/Q392933> ;
	skos:broader	medtop:20000294 .

medtop:20000298
	rdf:type skos:Concept ;
	skos:prefLabel	"electrical appliance"@en-GB ;
	skos:definition	"Makers of large and small electrical goods for use in homes or business"@en-GB ;
	skos:inScheme <http://cv.iptc.org/newscodes/mediatopic/>  ;
	ikos:created "2009-10-22T02:00:00+00:00"^^xsd:dateTime ;
	dct:created "2009-10-22T02:00:00+00:00"^^xsd:dateTime ;
	ikos:modified "2021-02-18T12:00:00+00:00"^^xsd:dateTime ;
	dct:modified "2021-02-18T12:00:00+00:00"^^xsd:dateTime  ;
	skos:exactMatch subj:04011004 ;
	skos:exactMatch <https://www.wikidata.org/entity/Q56604188> ;
	skos:broader	medtop:20000294 .

medtop:20000299
	rdf:type skos:Concept ;
	skos:prefLabel	"heavy engineering"@en-GB ;
	skos:definition	"Manufacturers of engineering equipment, such as cranes and bulldozers, for use in major construction projects"@en-GB ;
	skos:inScheme <http://cv.iptc.org/newscodes/mediatopic/>  ;
	ikos:created "2009-10-22T02:00:00+00:00"^^xsd:dateTime ;
	dct:created "2009-10-22T02:00:00+00:00"^^xsd:dateTime ;
	ikos:modified "2023-03-31T12:00:00+00:00"^^xsd:dateTime ;
	dct:modified "2023-03-31T12:00:00+00:00"^^xsd:dateTime  ;
	skos:exactMatch subj:04011005 ;
	skos:exactMatch <https://www.wikidata.org/entity/Q874311> ;
	skos:broader	medtop:20000294 .

medtop:20000300
	rdf:type skos:Concept ;
	skos:prefLabel	"industrial component"@en-GB ;
	skos:definition	"Manufacturers of mechanical, electrical, electronic items needed in the manufacture of other items"@en-GB ;
	skos:inScheme <http://cv.iptc.org/newscodes/mediatopic/>  ;
	ikos:created "2009-10-22T02:00:00+00:00"^^xsd:dateTime ;
	dct:created "2009-10-22T02:00:00+00:00"^^xsd:dateTime ;
	ikos:modified "2023-03-31T12:00:00+00:00"^^xsd:dateTime ;
	dct:modified "2023-03-31T12:00:00+00:00"^^xsd:dateTime  ; 
	ikos:retired "2023-03-31T12:00:00+00:00"^^xsd:dateTime ;
	skos:exactMatch subj:04011006 ;
	skos:broader	medtop:20000294 .

medtop:20000301
	rdf:type skos:Concept ;
	skos:prefLabel	"instrument engineering"@en-GB ;
	skos:definition	"Manufacturers of instruments for calibration, measurement of things like speed, pressure, distance"@en-GB ;
	skos:inScheme <http://cv.iptc.org/newscodes/mediatopic/>  ;
	ikos:created "2009-10-22T02:00:00+00:00"^^xsd:dateTime ;
	dct:created "2009-10-22T02:00:00+00:00"^^xsd:dateTime ;
	ikos:modified "2023-03-31T12:00:00+00:00"^^xsd:dateTime ;
	dct:modified "2023-03-31T12:00:00+00:00"^^xsd:dateTime  ; 
	ikos:retired "2023-03-31T12:00:00+00:00"^^xsd:dateTime ;
	skos:exactMatch subj:04011007 ;
	skos:exactMatch <https://www.wikidata.org/entity/Q56604289> ;
	skos:broader	medtop:20000294 .

medtop:20000302
	rdf:type skos:Concept ;
	skos:prefLabel	"machine manufacturing"@en-GB ;
	skos:definition	"Manufacturers of turbines, engines, fans, pumps, motors and other components for powered equipment"@en-GB ;
	skos:inScheme <http://cv.iptc.org/newscodes/mediatopic/>  ;
	ikos:created "2009-10-22T02:00:00+00:00"^^xsd:dateTime ;
	dct:created "2009-10-22T02:00:00+00:00"^^xsd:dateTime ;
	ikos:modified "2023-03-31T12:00:00+00:00"^^xsd:dateTime ;
	dct:modified "2023-03-31T12:00:00+00:00"^^xsd:dateTime  ;
	skos:exactMatch subj:04011009 ;
	skos:broader	medtop:20000294 .

medtop:20000303
	rdf:type skos:Concept ;
	skos:prefLabel	"shipbuilding"@en-GB ;
	skos:definition	"Manufacturers of ships and submersibles and suppliers for the maintenance and repair of these vessels"@en-GB ;
	skos:inScheme <http://cv.iptc.org/newscodes/mediatopic/>  ;
	ikos:created "2009-10-22T02:00:00+00:00"^^xsd:dateTime ;
	dct:created "2009-10-22T02:00:00+00:00"^^xsd:dateTime ;
	ikos:modified "2023-03-31T12:00:00+00:00"^^xsd:dateTime ;
	dct:modified "2023-03-31T12:00:00+00:00"^^xsd:dateTime  ;
	skos:exactMatch subj:04011008 ;
	skos:exactMatch <https://www.wikidata.org/entity/Q474200> ;
	skos:broader	medtop:20000294 .

medtop:20000304
	rdf:type skos:Concept ;
	skos:prefLabel	"media and entertainment industry"@en-GB ;
	skos:definition	"The various means of disseminating news, information and entertainment to the public"@en-GB ;
	skos:inScheme <http://cv.iptc.org/newscodes/mediatopic/>  ;
	ikos:created "2009-10-22T02:00:00+00:00"^^xsd:dateTime ;
	dct:created "2009-10-22T02:00:00+00:00"^^xsd:dateTime ;
	ikos:modified "2023-03-31T12:00:00+00:00"^^xsd:dateTime ;
	dct:modified "2023-03-31T12:00:00+00:00"^^xsd:dateTime  ;
	skos:exactMatch subj:04010000 ;
	skos:exactMatch <https://www.wikidata.org/entity/Q56611639> ;
	skos:broader	medtop:20000209 ;
	skos:narrower	medtop:20000305 ;
	skos:narrower	medtop:20000306 ;
	skos:narrower	medtop:20000307 ;
	skos:narrower	medtop:20000308 ;
	skos:narrower	medtop:20000309 ;
	skos:narrower	medtop:20000310 ;
	skos:narrower	medtop:20000311 ;
	skos:narrower	medtop:20000312 ;
	skos:narrower	medtop:20000313 ;
	skos:narrower	medtop:20000314 ;
	skos:narrower	medtop:20000315 ;
	skos:narrower	medtop:20001293 ;
	skos:narrower	medtop:20001369 ;
	skos:narrower	medtop:20001372 .

medtop:20000305
	rdf:type skos:Concept ;
	skos:prefLabel	"advertising"@en-GB ;
	skos:definition	"Methods of promoting goods and services to consumers"@en-GB ;
	skos:inScheme <http://cv.iptc.org/newscodes/mediatopic/>  ;
	ikos:created "2009-10-22T02:00:00+00:00"^^xsd:dateTime ;
	dct:created "2009-10-22T02:00:00+00:00"^^xsd:dateTime ;
	ikos:modified "2023-03-31T12:00:00+00:00"^^xsd:dateTime ;
	dct:modified "2023-03-31T12:00:00+00:00"^^xsd:dateTime  ;
	skos:exactMatch subj:04010001 ;
	skos:exactMatch <https://www.wikidata.org/entity/Q23700481> ;
	skos:broader	medtop:20000304 .

medtop:20000306
	rdf:type skos:Concept ;
	skos:prefLabel	"books and publishing"@en-GB ;
	skos:definition	"The business of producing and selling books, including e-books and audiobooks"@en-GB ;
	skos:inScheme <http://cv.iptc.org/newscodes/mediatopic/>  ;
	ikos:created "2009-10-22T02:00:00+00:00"^^xsd:dateTime ;
	dct:created "2009-10-22T02:00:00+00:00"^^xsd:dateTime ;
	ikos:modified "2023-03-31T12:00:00+00:00"^^xsd:dateTime ;
	dct:modified "2023-03-31T12:00:00+00:00"^^xsd:dateTime  ;
	skos:exactMatch subj:04010002 ;
	skos:exactMatch <https://www.wikidata.org/entity/Q56560668> ;
	skos:broader	medtop:20000304 .

medtop:20000307
	rdf:type skos:Concept ;
	skos:prefLabel	"film industry"@en-GB ;
	skos:definition	"The business of making, selling and distributing films"@en-GB ;
	skos:inScheme <http://cv.iptc.org/newscodes/mediatopic/>  ;
	ikos:created "2009-10-22T02:00:00+00:00"^^xsd:dateTime ;
	dct:created "2009-10-22T02:00:00+00:00"^^xsd:dateTime ;
	ikos:modified "2023-03-31T12:00:00+00:00"^^xsd:dateTime ;
	dct:modified "2023-03-31T12:00:00+00:00"^^xsd:dateTime  ;
	skos:exactMatch subj:04010003 ;
	skos:exactMatch <https://www.wikidata.org/entity/Q1415395> ;
	skos:broader	medtop:20000304 .

medtop:20000308
	rdf:type skos:Concept ;
	skos:prefLabel	"music industry"@en-GB ;
	skos:definition	"Recording, production and marketing of music"@en-GB ;
	skos:inScheme <http://cv.iptc.org/newscodes/mediatopic/>  ;
	ikos:created "2009-10-22T02:00:00+00:00"^^xsd:dateTime ;
	dct:created "2009-10-22T02:00:00+00:00"^^xsd:dateTime ;
	ikos:modified "2023-03-31T12:00:00+00:00"^^xsd:dateTime ;
	dct:modified "2023-03-31T12:00:00+00:00"^^xsd:dateTime  ;
	skos:exactMatch subj:04010011 ;
	skos:exactMatch <https://www.wikidata.org/entity/Q746359> ;
	skos:broader	medtop:20000304 .

medtop:20000309
	rdf:type skos:Concept ;
	skos:prefLabel	"news agency"@en-GB ;
	skos:definition	"Commercial agencies for production and distribution of newsworthy events through print, broadcast, video or electronic media"@en-GB ;
	skos:changeNote	"Retired. Use medtop:20001372 news industry instead."@en-GB ;
	skos:inScheme <http://cv.iptc.org/newscodes/mediatopic/>  ;
	ikos:created "2009-10-22T02:00:00+00:00"^^xsd:dateTime ;
	dct:created "2009-10-22T02:00:00+00:00"^^xsd:dateTime ;
	ikos:modified "2023-03-31T12:00:00+00:00"^^xsd:dateTime ;
	dct:modified "2023-03-31T12:00:00+00:00"^^xsd:dateTime  ; 
	ikos:retired "2023-03-31T12:00:00+00:00"^^xsd:dateTime ;
	skos:exactMatch subj:04010004 ;
	skos:exactMatch <https://www.wikidata.org/entity/Q192283> ;
	skos:broader	medtop:20000304 .

medtop:20000310
	rdf:type skos:Concept ;
	skos:prefLabel	"newspaper and magazine"@en-GB ;
	skos:definition	"The business of producing bound and unbound printed paper products for periodic distribution of news items"@en-GB ;
	skos:changeNote	"Retired. Use medtop:20001372 news industry instead."@en-GB ;
	skos:inScheme <http://cv.iptc.org/newscodes/mediatopic/>  ;
	ikos:created "2009-10-22T02:00:00+00:00"^^xsd:dateTime ;
	dct:created "2009-10-22T02:00:00+00:00"^^xsd:dateTime ;
	ikos:modified "2023-03-31T12:00:00+00:00"^^xsd:dateTime ;
	dct:modified "2023-03-31T12:00:00+00:00"^^xsd:dateTime  ; 
	ikos:retired "2023-03-31T12:00:00+00:00"^^xsd:dateTime ;
	skos:exactMatch subj:04010005 ;
	skos:exactMatch <https://www.wikidata.org/entity/Q3579160> ;
	skos:broader	medtop:20000304 .

medtop:20000311
	rdf:type skos:Concept ;
	skos:prefLabel	"online media industry"@en-GB ;
	skos:definition	"The business of distributing news and information through computer networks for public consumption"@en-GB ;
	skos:changeNote	"Retired. Use medtop:20001372 news industry instead."@en-GB ;
	skos:inScheme <http://cv.iptc.org/newscodes/mediatopic/>  ;
	ikos:created "2009-10-22T02:00:00+00:00"^^xsd:dateTime ;
	dct:created "2009-10-22T02:00:00+00:00"^^xsd:dateTime ;
	ikos:modified "2023-03-31T12:00:00+00:00"^^xsd:dateTime ;
	dct:modified "2023-03-31T12:00:00+00:00"^^xsd:dateTime  ; 
	ikos:retired "2023-03-31T12:00:00+00:00"^^xsd:dateTime ;
	skos:exactMatch subj:04010006 ;
	skos:exactMatch <https://www.wikidata.org/entity/Q1076968> ;
	skos:broader	medtop:20000304 .

medtop:20000312
	rdf:type skos:Concept ;
	skos:prefLabel	"public relations"@en-GB ;
	skos:definition	"The business of managing and disseminating information from an individual or an organization to the public in order to influence their perception"@en-GB ;
	skos:inScheme <http://cv.iptc.org/newscodes/mediatopic/>  ;
	ikos:created "2009-10-22T02:00:00+00:00"^^xsd:dateTime ;
	dct:created "2009-10-22T02:00:00+00:00"^^xsd:dateTime ;
	ikos:modified "2023-03-31T12:00:00+00:00"^^xsd:dateTime ;
	dct:modified "2023-03-31T12:00:00+00:00"^^xsd:dateTime  ;
	skos:exactMatch subj:04010007 ;
	skos:exactMatch <https://www.wikidata.org/entity/Q133080> ;
	skos:broader	medtop:20000304 .

medtop:20000313
	rdf:type skos:Concept ;
	skos:prefLabel	"radio industry"@en-GB ;
	skos:definition	"Companies and organisations involved in the broadcast of radio stations and their content to the public"@en-GB ;
	skos:inScheme <http://cv.iptc.org/newscodes/mediatopic/>  ;
	ikos:created "2009-10-22T02:00:00+00:00"^^xsd:dateTime ;
	dct:created "2009-10-22T02:00:00+00:00"^^xsd:dateTime ;
	ikos:modified "2023-03-31T12:00:00+00:00"^^xsd:dateTime ;
	dct:modified "2023-03-31T12:00:00+00:00"^^xsd:dateTime  ;
	skos:exactMatch subj:04010008 ;
	skos:exactMatch <https://www.wikidata.org/entity/Q7281175> ;
	skos:broader	medtop:20000304 .

medtop:20000314
	rdf:type skos:Concept ;
	skos:prefLabel	"satellite and cable service"@en-GB ;
	skos:definition	"The business of transmitting news, entertainment and information via satellite or cable television services"@en-GB ;
	skos:inScheme <http://cv.iptc.org/newscodes/mediatopic/>  ;
	ikos:created "2009-10-22T02:00:00+00:00"^^xsd:dateTime ;
	dct:created "2009-10-22T02:00:00+00:00"^^xsd:dateTime ;
	ikos:modified "2021-05-05T12:00:00+00:00"^^xsd:dateTime ;
	dct:modified "2021-05-05T12:00:00+00:00"^^xsd:dateTime  ;
	skos:exactMatch subj:04010009 ;
	skos:exactMatch <https://www.wikidata.org/entity/Q11058702> ;
	skos:broader	medtop:20000304 .

medtop:20000315
	rdf:type skos:Concept ;
	skos:prefLabel	"television industry"@en-GB ;
	skos:definition	"The production and broadcasting of television content"@en-GB ;
	skos:inScheme <http://cv.iptc.org/newscodes/mediatopic/>  ;
	ikos:created "2009-10-22T02:00:00+00:00"^^xsd:dateTime ;
	dct:created "2009-10-22T02:00:00+00:00"^^xsd:dateTime ;
	ikos:modified "2023-03-31T12:00:00+00:00"^^xsd:dateTime ;
	dct:modified "2023-03-31T12:00:00+00:00"^^xsd:dateTime  ;
	skos:exactMatch subj:04010010 ;
	skos:exactMatch <https://www.wikidata.org/entity/Q209588> ;
	skos:broader	medtop:20000304 .

medtop:20000316
	rdf:type skos:Concept ;
	skos:prefLabel	"metal and mineral mining and refining"@en-GB ;
	skos:definition	"The extractive businesses that remove raw materials, including coal, gold iron and copper, from the earth by drilling and pumping, quarrying or mining"@en-GB ;
	skos:inScheme <http://cv.iptc.org/newscodes/mediatopic/>  ;
	ikos:created "2009-10-22T02:00:00+00:00"^^xsd:dateTime ;
	dct:created "2009-10-22T02:00:00+00:00"^^xsd:dateTime ;
	ikos:modified "2023-03-31T12:00:00+00:00"^^xsd:dateTime ;
	dct:modified "2023-03-31T12:00:00+00:00"^^xsd:dateTime  ;
	skos:exactMatch subj:04012000 ;
	skos:exactMatch <https://www.wikidata.org/entity/Q11467> ;
	skos:broader	medtop:20000209 ;
	skos:narrower	medtop:20000318 ;
	skos:narrower	medtop:20000319 ;
	skos:narrower	medtop:20000320 ;
	skos:narrower	medtop:20000321 .

medtop:20000317
	rdf:type skos:Concept ;
	skos:prefLabel	"building material"@en-GB ;
	skos:definition	"Manufacturing of the materials used in construction, such as wallboard, lumber and wire"@en-GB ;
	skos:inScheme <http://cv.iptc.org/newscodes/mediatopic/>  ;
	ikos:created "2009-10-22T02:00:00+00:00"^^xsd:dateTime ;
	dct:created "2009-10-22T02:00:00+00:00"^^xsd:dateTime ;
	ikos:modified "2023-03-31T12:00:00+00:00"^^xsd:dateTime ;
	dct:modified "2023-03-31T12:00:00+00:00"^^xsd:dateTime  ;
	skos:exactMatch subj:04012001 ;
	skos:exactMatch <https://www.wikidata.org/entity/Q56887369> ;
	skos:broader	medtop:20000235 .

medtop:20000318
	rdf:type skos:Concept ;
	skos:prefLabel	"precious material"@en-GB ;
	skos:definition	"The mining, refining and sale of materials such as gold, silver, precious metals, diamonds and rare earths"@en-GB ;
	skos:inScheme <http://cv.iptc.org/newscodes/mediatopic/>  ;
	ikos:created "2009-10-22T02:00:00+00:00"^^xsd:dateTime ;
	dct:created "2009-10-22T02:00:00+00:00"^^xsd:dateTime ;
	ikos:modified "2023-03-31T12:00:00+00:00"^^xsd:dateTime ;
	dct:modified "2023-03-31T12:00:00+00:00"^^xsd:dateTime  ;
	skos:exactMatch subj:04012002 ;
	skos:exactMatch <https://www.wikidata.org/entity/Q56573752> ;
	skos:broader	medtop:20000316 .

medtop:20000319
	rdf:type skos:Concept ;
	skos:prefLabel	"iron and steel"@en-GB ;
	skos:definition	"Mining, refining and sales of iron-based metals"@en-GB ;
	skos:changeNote	"Retired. Use medtop:20000316 metal and mineral mining and refining instead."@en-GB ;
	skos:inScheme <http://cv.iptc.org/newscodes/mediatopic/>  ;
	ikos:created "2009-10-22T02:00:00+00:00"^^xsd:dateTime ;
	dct:created "2009-10-22T02:00:00+00:00"^^xsd:dateTime ;
	ikos:modified "2023-03-31T12:00:00+00:00"^^xsd:dateTime ;
	dct:modified "2023-03-31T12:00:00+00:00"^^xsd:dateTime  ; 
	ikos:retired "2023-03-31T12:00:00+00:00"^^xsd:dateTime ;
	skos:exactMatch subj:04012003 ;
	skos:exactMatch <https://www.wikidata.org/entity/Q11649792> ;
	skos:broader	medtop:20000316 .

medtop:20000320
	rdf:type skos:Concept ;
	skos:prefLabel	"mining"@en-GB ;
	skos:definition	"The industry of digging for metals, minerals, raw materials, such as coal, or precious gems, such as diamonds"@en-GB ;
	skos:changeNote	"Retired. Use medtop:20000316 metal and mineral mining and refining instead."@en-GB ;
	skos:inScheme <http://cv.iptc.org/newscodes/mediatopic/>  ;
	ikos:created "2009-10-22T02:00:00+00:00"^^xsd:dateTime ;
	dct:created "2009-10-22T02:00:00+00:00"^^xsd:dateTime ;
	ikos:modified "2023-03-31T12:00:00+00:00"^^xsd:dateTime ;
	dct:modified "2023-03-31T12:00:00+00:00"^^xsd:dateTime  ; 
	ikos:retired "2023-03-31T12:00:00+00:00"^^xsd:dateTime ;
	skos:exactMatch subj:04012005 ;
	skos:exactMatch <https://www.wikidata.org/entity/Q44497> ;
	skos:broader	medtop:20000316 .

medtop:20000321
	rdf:type skos:Concept ;
	skos:prefLabel	"non-ferrous metal"@en-GB ;
	skos:definition	"Mining, refining and sales of copper, zinc, aluminium, and other metals not based on iron"@en-GB ;
	skos:changeNote	"Retired. Use medtop:20000316 metal and mineral mining and refining instead."@en-GB ;
	skos:inScheme <http://cv.iptc.org/newscodes/mediatopic/>  ;
	ikos:created "2009-10-22T02:00:00+00:00"^^xsd:dateTime ;
	dct:created "2009-10-22T02:00:00+00:00"^^xsd:dateTime ;
	ikos:modified "2023-03-31T12:00:00+00:00"^^xsd:dateTime ;
	dct:modified "2023-03-31T12:00:00+00:00"^^xsd:dateTime  ; 
	ikos:retired "2023-03-31T12:00:00+00:00"^^xsd:dateTime ;
	skos:exactMatch subj:04012004 ;
	skos:exactMatch <https://www.wikidata.org/entity/Q56574140> ;
	skos:broader	medtop:20000316 .

medtop:20000322
	rdf:type skos:Concept ;
	skos:prefLabel	"process industry"@en-GB ;
	skos:definition	"The business of turning raw materials into useable products"@en-GB ;
	skos:changeNote	"Retired. Use more specific terms instead."@en-GB ;
	skos:inScheme <http://cv.iptc.org/newscodes/mediatopic/>  ;
	ikos:created "2009-10-22T02:00:00+00:00"^^xsd:dateTime ;
	dct:created "2009-10-22T02:00:00+00:00"^^xsd:dateTime ;
	ikos:modified "2023-03-31T12:00:00+00:00"^^xsd:dateTime ;
	dct:modified "2023-03-31T12:00:00+00:00"^^xsd:dateTime  ; 
	ikos:retired "2023-03-31T12:00:00+00:00"^^xsd:dateTime ;
	skos:exactMatch subj:04013000 ;
	skos:exactMatch <https://www.wikidata.org/entity/Q15991203> ;
	skos:broader	medtop:20000209 ;
	skos:narrower	medtop:20000323 ;
	skos:narrower	medtop:20000326 ;
	skos:narrower	medtop:20000327 ;
	skos:narrower	medtop:20000328 ;
	skos:narrower	medtop:20000329 ;
	skos:narrower	medtop:20001169 .

medtop:20000323
	rdf:type skos:Concept ;
	skos:prefLabel	"distiller and brewer"@en-GB ;
	skos:definition	"Manufacture of alcoholic beverages"@en-GB ;
	skos:changeNote	"Retired. Use medtop:20000324 beverage and grocery instead."@en-GB ;
	skos:inScheme <http://cv.iptc.org/newscodes/mediatopic/>  ;
	ikos:created "2009-10-22T02:00:00+00:00"^^xsd:dateTime ;
	dct:created "2009-10-22T02:00:00+00:00"^^xsd:dateTime ;
	ikos:modified "2023-03-31T12:00:00+00:00"^^xsd:dateTime ;
	dct:modified "2023-03-31T12:00:00+00:00"^^xsd:dateTime  ; 
	ikos:retired "2023-03-31T12:00:00+00:00"^^xsd:dateTime ;
	skos:exactMatch subj:04013001 ;
	skos:exactMatch <https://www.wikidata.org/entity/Q3150593> ;
	skos:broader	medtop:20000322 .

medtop:20000324
	rdf:type skos:Concept ;
	skos:prefLabel	"beverage and grocery"@en-GB ;
	skos:definition	"The production and sale of foodstuffs"@en-GB ;
	skos:inScheme <http://cv.iptc.org/newscodes/mediatopic/>  ;
	ikos:created "2009-10-22T02:00:00+00:00"^^xsd:dateTime ;
	dct:created "2009-10-22T02:00:00+00:00"^^xsd:dateTime ;
	ikos:modified "2023-03-31T12:00:00+00:00"^^xsd:dateTime ;
	dct:modified "2023-03-31T12:00:00+00:00"^^xsd:dateTime  ;
	skos:exactMatch subj:04013002 ;
	skos:exactMatch <https://www.wikidata.org/entity/Q540912> ;
	skos:broader	medtop:20000243 .

medtop:20000325
	rdf:type skos:Concept ;
	skos:prefLabel	"furnishings and furniture"@en-GB ;
	skos:definition	"Manufacture of furniture, wallpaper, paints and fabrics for interior decoration"@en-GB ;
	skos:inScheme <http://cv.iptc.org/newscodes/mediatopic/>  ;
	ikos:created "2009-10-22T02:00:00+00:00"^^xsd:dateTime ;
	dct:created "2009-10-22T02:00:00+00:00"^^xsd:dateTime ;
	ikos:modified "2023-03-31T12:00:00+00:00"^^xsd:dateTime ;
	dct:modified "2023-03-31T12:00:00+00:00"^^xsd:dateTime  ;
	skos:exactMatch subj:04013003 ;
	skos:exactMatch <https://www.wikidata.org/entity/Q12122106> ;
	skos:broader	medtop:20000243 .

medtop:20000326
	rdf:type skos:Concept ;
	skos:prefLabel	"paper and packaging product"@en-GB ;
	skos:definition	"Production of paper material for writing, wrapping, printing, or packaging"@en-GB ;
	skos:inScheme <http://cv.iptc.org/newscodes/mediatopic/>  ;
	ikos:created "2009-10-22T02:00:00+00:00"^^xsd:dateTime ;
	dct:created "2009-10-22T02:00:00+00:00"^^xsd:dateTime ;
	ikos:modified "2023-03-31T12:00:00+00:00"^^xsd:dateTime ;
	dct:modified "2023-03-31T12:00:00+00:00"^^xsd:dateTime  ; 
	ikos:retired "2023-03-31T12:00:00+00:00"^^xsd:dateTime ;
	skos:exactMatch subj:04013004 ;
	skos:exactMatch <https://www.wikidata.org/entity/Q2283886> ;
	skos:broader	medtop:20000322 .

medtop:20000327
	rdf:type skos:Concept ;
	skos:prefLabel	"rubber product"@en-GB ;
	skos:definition	"Production of rubber-based materials for gloves, protective coatings, hoses and the like"@en-GB ;
	skos:inScheme <http://cv.iptc.org/newscodes/mediatopic/>  ;
	ikos:created "2009-10-22T02:00:00+00:00"^^xsd:dateTime ;
	dct:created "2009-10-22T02:00:00+00:00"^^xsd:dateTime ;
	ikos:modified "2023-03-31T12:00:00+00:00"^^xsd:dateTime ;
	dct:modified "2023-03-31T12:00:00+00:00"^^xsd:dateTime  ; 
	ikos:retired "2023-03-31T12:00:00+00:00"^^xsd:dateTime ;
	skos:exactMatch subj:04013005 ;
	skos:exactMatch <https://www.wikidata.org/entity/Q56604620> ;
	skos:broader	medtop:20000322 .

medtop:20000328
	rdf:type skos:Concept ;
	skos:prefLabel	"soft drinks"@en-GB ;
	skos:definition	"Production of non-alcoholic drinks"@en-GB ;
	skos:changeNote	"Retired. Use medtop:20000324 beverage and grocery instead."@en-GB ;
	skos:inScheme <http://cv.iptc.org/newscodes/mediatopic/>  ;
	ikos:created "2009-10-22T02:00:00+00:00"^^xsd:dateTime ;
	dct:created "2009-10-22T02:00:00+00:00"^^xsd:dateTime ;
	ikos:modified "2023-03-31T12:00:00+00:00"^^xsd:dateTime ;
	dct:modified "2023-03-31T12:00:00+00:00"^^xsd:dateTime  ; 
	ikos:retired "2023-03-31T12:00:00+00:00"^^xsd:dateTime ;
	skos:exactMatch subj:04013006 ;
	skos:exactMatch <https://www.wikidata.org/entity/Q56882638> ;
	skos:broader	medtop:20000322 .

medtop:20000329
	rdf:type skos:Concept ;
	skos:prefLabel	"textile and clothing"@en-GB ;
	skos:definition	"Production of fabrics for furnishings and fixtures, and for clothing of various types"@en-GB ;
	skos:changeNote	"Retired. Use medtop:20000245 clothing instead."@en-GB ;
	skos:inScheme <http://cv.iptc.org/newscodes/mediatopic/>  ;
	ikos:created "2009-10-22T02:00:00+00:00"^^xsd:dateTime ;
	dct:created "2009-10-22T02:00:00+00:00"^^xsd:dateTime ;
	ikos:modified "2023-03-31T12:00:00+00:00"^^xsd:dateTime ;
	dct:modified "2023-03-31T12:00:00+00:00"^^xsd:dateTime  ; 
	ikos:retired "2023-03-31T12:00:00+00:00"^^xsd:dateTime ;
	skos:exactMatch subj:04013007 ;
	skos:exactMatch <https://www.wikidata.org/entity/Q607081> ;
	skos:broader	medtop:20000322 .

medtop:20000330
	rdf:type skos:Concept ;
	skos:prefLabel	"tobacco and nicotine"@en-GB ;
	skos:definition	"The sale and maufacturing of tobacco products for consumers, including cigarettes, e-cigarettes and vaping cartridges"@en-GB ;
	skos:inScheme <http://cv.iptc.org/newscodes/mediatopic/>  ;
	ikos:created "2009-10-22T02:00:00+00:00"^^xsd:dateTime ;
	dct:created "2009-10-22T02:00:00+00:00"^^xsd:dateTime ;
	ikos:modified "2023-03-31T12:00:00+00:00"^^xsd:dateTime ;
	dct:modified "2023-03-31T12:00:00+00:00"^^xsd:dateTime  ;
	skos:exactMatch subj:04013008 ;
	skos:exactMatch <https://www.wikidata.org/wiki/Q907703> ;
	skos:broader	medtop:20000243 .

medtop:20000331
	rdf:type skos:Concept ;
	skos:prefLabel	"tourism and leisure industry"@en-GB ;
	skos:definition	"Commercial organisations and operations dealing with travel and the pursuit of recreational activities"@en-GB ;
	skos:inScheme <http://cv.iptc.org/newscodes/mediatopic/>  ;
	ikos:created "2009-10-22T02:00:00+00:00"^^xsd:dateTime ;
	dct:created "2009-10-22T02:00:00+00:00"^^xsd:dateTime ;
	ikos:modified "2023-03-31T12:00:00+00:00"^^xsd:dateTime ;
	dct:modified "2023-03-31T12:00:00+00:00"^^xsd:dateTime  ;
	skos:exactMatch subj:04014000 ;
	skos:exactMatch <https://www.wikidata.org/entity/Q11630521> ;
	skos:broader	medtop:20000209 ;
	skos:narrower	medtop:20000332 ;
	skos:narrower	medtop:20000333 ;
	skos:narrower	medtop:20000334 ;
	skos:narrower	medtop:20000335 ;
	skos:narrower	medtop:20000336 .

medtop:20000332
	rdf:type skos:Concept ;
	skos:prefLabel	"casinos and gambling"@en-GB ;
	skos:definition	"Organisations providing outlets for betting money on games of chance or animal races"@en-GB ;
	skos:inScheme <http://cv.iptc.org/newscodes/mediatopic/>  ;
	ikos:created "2009-10-22T02:00:00+00:00"^^xsd:dateTime ;
	dct:created "2009-10-22T02:00:00+00:00"^^xsd:dateTime ;
	ikos:modified "2023-03-31T12:00:00+00:00"^^xsd:dateTime ;
	dct:modified "2023-03-31T12:00:00+00:00"^^xsd:dateTime  ;
	skos:exactMatch subj:04014001 ;
	skos:exactMatch <https://www.wikidata.org/entity/Q61054412> ;
	skos:broader	medtop:20000331 .

medtop:20000333
	rdf:type skos:Concept ;
	skos:prefLabel	"hotel and accommodation"@en-GB ;
	skos:definition	"The business of providing lodging to travellers"@en-GB ;
	skos:inScheme <http://cv.iptc.org/newscodes/mediatopic/>  ;
	ikos:created "2009-10-22T02:00:00+00:00"^^xsd:dateTime ;
	dct:created "2009-10-22T02:00:00+00:00"^^xsd:dateTime ;
	ikos:modified "2023-03-31T12:00:00+00:00"^^xsd:dateTime ;
	dct:modified "2023-03-31T12:00:00+00:00"^^xsd:dateTime  ;
	skos:exactMatch subj:04014002 ;
	skos:exactMatch <https://www.wikidata.org/entity/Q1495452> ;
	skos:broader	medtop:20000331 .

medtop:20000334
	rdf:type skos:Concept ;
	skos:prefLabel	"recreational and sporting goods"@en-GB ;
	skos:definition	"Manufacture of goods for leisure activities"@en-GB ;
	skos:inScheme <http://cv.iptc.org/newscodes/mediatopic/>  ;
	ikos:created "2009-10-22T02:00:00+00:00"^^xsd:dateTime ;
	dct:created "2009-10-22T02:00:00+00:00"^^xsd:dateTime ;
	ikos:modified "2021-02-18T12:00:00+00:00"^^xsd:dateTime ;
	dct:modified "2021-02-18T12:00:00+00:00"^^xsd:dateTime  ;
	skos:exactMatch subj:04014003 ;
	skos:exactMatch <https://www.wikidata.org/entity/Q57264543> ;
	skos:broader	medtop:20000331 .

medtop:20000335
	rdf:type skos:Concept ;
	skos:prefLabel	"restaurant and catering"@en-GB ;
	skos:definition	"The business of providing prepared food for customers"@en-GB ;
	skos:inScheme <http://cv.iptc.org/newscodes/mediatopic/>  ;
	ikos:created "2009-10-22T02:00:00+00:00"^^xsd:dateTime ;
	dct:created "2009-10-22T02:00:00+00:00"^^xsd:dateTime ;
	ikos:modified "2023-03-31T12:00:00+00:00"^^xsd:dateTime ;
	dct:modified "2023-03-31T12:00:00+00:00"^^xsd:dateTime  ;
	skos:exactMatch subj:04014004 ;
	skos:exactMatch <https://www.wikidata.org/entity/Q41958> ;
	skos:broader	medtop:20000331 .

medtop:20000336
	rdf:type skos:Concept ;
	skos:prefLabel	"tour operator"@en-GB ;
	skos:definition	"Operators of trips either locally or internationally"@en-GB ;
	skos:inScheme <http://cv.iptc.org/newscodes/mediatopic/>  ;
	ikos:created "2009-10-22T02:00:00+00:00"^^xsd:dateTime ;
	dct:created "2009-10-22T02:00:00+00:00"^^xsd:dateTime ;
	ikos:modified "2023-03-31T12:00:00+00:00"^^xsd:dateTime ;
	dct:modified "2023-03-31T12:00:00+00:00"^^xsd:dateTime  ;
	skos:exactMatch subj:04014005 ;
	skos:exactMatch <https://www.wikidata.org/entity/Q133744> ;
	skos:broader	medtop:20000331 .

medtop:20000337
	rdf:type skos:Concept ;
	skos:prefLabel	"transport"@en-GB ;
	skos:definition	"The means of getting people or goods from one place to another"@en-GB ;
	skos:changeNote	"2016-04-05: definition slightly changed"@en-GB ;
	skos:inScheme <http://cv.iptc.org/newscodes/mediatopic/>  ;
	ikos:created "2009-10-22T02:00:00+00:00"^^xsd:dateTime ;
	dct:created "2009-10-22T02:00:00+00:00"^^xsd:dateTime ;
	ikos:modified "2023-03-31T12:00:00+00:00"^^xsd:dateTime ;
	dct:modified "2023-03-31T12:00:00+00:00"^^xsd:dateTime  ;
	skos:exactMatch subj:04015000 ;
	skos:exactMatch <https://www.wikidata.org/entity/Q7590> ;
	skos:broader	medtop:20000209 ;
	skos:narrower	medtop:20000338 ;
	skos:narrower	medtop:20000340 ;
	skos:narrower	medtop:20000341 ;
	skos:narrower	medtop:20000342 ;
	skos:narrower	medtop:20000343 ;
	skos:narrower	medtop:20001170 ;
	skos:narrower	medtop:20001362 ;
	skos:narrower	medtop:20001363 ;
	skos:narrower	medtop:20001364 .

medtop:20000338
	rdf:type skos:Concept ;
	skos:prefLabel	"air transport"@en-GB ;
	skos:definition	"The movement of passengers and freight by air"@en-GB ;
	skos:inScheme <http://cv.iptc.org/newscodes/mediatopic/>  ;
	ikos:created "2009-10-22T02:00:00+00:00"^^xsd:dateTime ;
	dct:created "2009-10-22T02:00:00+00:00"^^xsd:dateTime ;
	ikos:modified "2023-03-31T12:00:00+00:00"^^xsd:dateTime ;
	dct:modified "2023-03-31T12:00:00+00:00"^^xsd:dateTime  ;
	skos:exactMatch subj:04015001 ;
	skos:exactMatch <https://www.wikidata.org/entity/Q1757562> ;
	skos:broader	medtop:20000337 .

medtop:20000339
	rdf:type skos:Concept ;
	skos:prefLabel	"commuting"@en-GB ;
	skos:definition	"The process of getting to and from work, including transport options, travel networks, car pooling."@en-GB ;
	skos:inScheme <http://cv.iptc.org/newscodes/mediatopic/>  ;
	ikos:created "2009-10-22T02:00:00+00:00"^^xsd:dateTime ;
	dct:created "2009-10-22T02:00:00+00:00"^^xsd:dateTime ;
	ikos:modified "2021-02-18T12:00:00+00:00"^^xsd:dateTime ;
	dct:modified "2021-02-18T12:00:00+00:00"^^xsd:dateTime  ;
	skos:broadMatch subj:10007000 ;
	skos:exactMatch <https://www.wikidata.org/entity/Q48442> ;
	skos:broader	medtop:20000509 .

medtop:20000340
	rdf:type skos:Concept ;
	skos:prefLabel	"railway transport"@en-GB ;
	skos:definition	"The movement of passengers and freight by rail"@en-GB ;
	skos:inScheme <http://cv.iptc.org/newscodes/mediatopic/>  ;
	ikos:created "2009-10-22T02:00:00+00:00"^^xsd:dateTime ;
	dct:created "2009-10-22T02:00:00+00:00"^^xsd:dateTime ;
	ikos:modified "2023-03-31T12:00:00+00:00"^^xsd:dateTime ;
	dct:modified "2023-03-31T12:00:00+00:00"^^xsd:dateTime  ;
	skos:exactMatch subj:04015002 ;
	skos:exactMatch <https://www.wikidata.org/entity/Q3565868> ;
	skos:broader	medtop:20000337 .

medtop:20000341
	rdf:type skos:Concept ;
	skos:prefLabel	"road transport"@en-GB ;
	skos:definition	"The movement of passengers and freight by road"@en-GB ;
	skos:inScheme <http://cv.iptc.org/newscodes/mediatopic/>  ;
	ikos:created "2009-10-22T02:00:00+00:00"^^xsd:dateTime ;
	dct:created "2009-10-22T02:00:00+00:00"^^xsd:dateTime ;
	ikos:modified "2023-03-31T12:00:00+00:00"^^xsd:dateTime ;
	dct:modified "2023-03-31T12:00:00+00:00"^^xsd:dateTime  ;
	skos:exactMatch subj:04015003 ;
	skos:exactMatch <https://www.wikidata.org/entity/Q516739> ;
	skos:broader	medtop:20000337 .

medtop:20000342
	rdf:type skos:Concept ;
	skos:prefLabel	"traffic"@en-GB ;
	skos:definition	"Traffic reports and/or warnings"@en-GB ;
	skos:inScheme <http://cv.iptc.org/newscodes/mediatopic/>  ;
	ikos:created "2009-10-22T02:00:00+00:00"^^xsd:dateTime ;
	dct:created "2009-10-22T02:00:00+00:00"^^xsd:dateTime ;
	ikos:modified "2023-03-31T12:00:00+00:00"^^xsd:dateTime ;
	dct:modified "2023-03-31T12:00:00+00:00"^^xsd:dateTime  ; 
	ikos:retired "2023-03-31T12:00:00+00:00"^^xsd:dateTime ;
	skos:exactMatch subj:10007001 ;
	skos:exactMatch <https://www.wikidata.org/entity/Q4323994> ;
	skos:broader	medtop:20000337 .

medtop:20000343
	rdf:type skos:Concept ;
	skos:prefLabel	"waterway and maritime transport"@en-GB ;
	skos:definition	"Commercial movement of people or goods via boats, ships and water"@en-GB ;
	skos:inScheme <http://cv.iptc.org/newscodes/mediatopic/>  ;
	ikos:created "2009-10-22T02:00:00+00:00"^^xsd:dateTime ;
	dct:created "2009-10-22T02:00:00+00:00"^^xsd:dateTime ;
	ikos:modified "2021-02-18T12:00:00+00:00"^^xsd:dateTime ;
	dct:modified "2021-02-18T12:00:00+00:00"^^xsd:dateTime  ;
	skos:exactMatch subj:04015004 ;
	skos:exactMatch <https://www.wikidata.org/entity/Q155930> ;
	skos:broader	medtop:20000337 .

medtop:20000344
	rdf:type skos:Concept ;
	skos:prefLabel	"economy"@en-GB ;
	skos:definition	"Content of a general nature about trade and the economy"@en-GB ;
	skos:inScheme <http://cv.iptc.org/newscodes/mediatopic/>  ;
	ikos:created "2009-10-22T02:00:00+00:00"^^xsd:dateTime ;
	dct:created "2009-10-22T02:00:00+00:00"^^xsd:dateTime ;
	ikos:modified "2021-07-12T12:00:00+00:00"^^xsd:dateTime ;
	dct:modified "2021-07-12T12:00:00+00:00"^^xsd:dateTime  ;
	skos:exactMatch <https://www.wikidata.org/entity/Q159810> ;
	skos:exactMatch subj:04017000 ;
	skos:broader	medtop:04000000 ;
	skos:narrower	medtop:20000346 ;
	skos:narrower	medtop:20001171 .

medtop:20000345
	rdf:type skos:Concept ;
	skos:prefLabel	"economic policy"@en-GB ;
	skos:definition	"Government directed policy on production, taxes, tariffs and things that affect the direction and health of the economy"@en-GB ;
	skos:inScheme <http://cv.iptc.org/newscodes/mediatopic/>  ;
	ikos:created "2009-10-22T02:00:00+00:00"^^xsd:dateTime ;
	dct:created "2009-10-22T02:00:00+00:00"^^xsd:dateTime ;
	ikos:modified "2021-02-18T12:00:00+00:00"^^xsd:dateTime ;
	dct:modified "2021-02-18T12:00:00+00:00"^^xsd:dateTime  ;
	skos:exactMatch subj:04017001 ;
	skos:exactMatch <https://www.wikidata.org/entity/Q582577> ;
	skos:broader	medtop:20000621 ;
	skos:narrower	medtop:20000623 ;
	skos:narrower	medtop:20000624 ;
	skos:narrower	medtop:20000625 ;
	skos:narrower	medtop:20001292 .

medtop:20000346
	rdf:type skos:Concept ;
	skos:prefLabel	"macro economics"@en-GB ;
	skos:definition	"Broad scale economics at the world or national level"@en-GB ;
	skos:inScheme <http://cv.iptc.org/newscodes/mediatopic/>  ;
	ikos:created "2009-10-22T02:00:00+00:00"^^xsd:dateTime ;
	dct:created "2009-10-22T02:00:00+00:00"^^xsd:dateTime ;
	ikos:modified "2021-02-18T12:00:00+00:00"^^xsd:dateTime ;
	dct:modified "2021-02-18T12:00:00+00:00"^^xsd:dateTime  ;
	skos:exactMatch subj:04008000 ;
	skos:exactMatch <https://www.wikidata.org/entity/Q39680> ;
	skos:broader	medtop:20000344 ;
	skos:narrower	medtop:20000347 ;
	skos:narrower	medtop:20000348 ;
	skos:narrower	medtop:20000349 ;
	skos:narrower	medtop:20000350 ;
	skos:narrower	medtop:20000351 ;
	skos:narrower	medtop:20000354 ;
	skos:narrower	medtop:20000355 ;
	skos:narrower	medtop:20000356 ;
	skos:narrower	medtop:20000357 ;
	skos:narrower	medtop:20000358 ;
	skos:narrower	medtop:20000363 ;
	skos:narrower	medtop:20000364 ;
	skos:narrower	medtop:20000365 ;
	skos:narrower	medtop:20000366 ;
	skos:narrower	medtop:20000367 ;
	skos:narrower	medtop:20000368 ;
	skos:narrower	medtop:20000369 ;
	skos:narrower	medtop:20000370 ;
	skos:narrower	medtop:20000371 ;
	skos:narrower	medtop:20000372 ;
	skos:narrower	medtop:20000373 ;
	skos:narrower	medtop:20000378 ;
	skos:narrower	medtop:20000379 ;
	skos:narrower	medtop:20000380 ;
	skos:narrower	medtop:20000381 ;
	skos:narrower	medtop:20000382 ;
	skos:narrower	medtop:20000383 ;
	skos:narrower	medtop:20000384 .

medtop:20000347
	rdf:type skos:Concept ;
	skos:prefLabel	"bonds"@en-GB ;
	skos:definition	"Corporate or governmental paper representing the loan of money at a fixed rate and for a fixed time to that company or government"@en-GB ;
	skos:inScheme <http://cv.iptc.org/newscodes/mediatopic/>  ;
	ikos:created "2009-10-22T02:00:00+00:00"^^xsd:dateTime ;
	dct:created "2009-10-22T02:00:00+00:00"^^xsd:dateTime ;
	ikos:modified "2021-02-18T12:00:00+00:00"^^xsd:dateTime ;
	dct:modified "2021-02-18T12:00:00+00:00"^^xsd:dateTime  ;
	skos:exactMatch subj:04008027 ;
	skos:exactMatch <https://www.wikidata.org/entity/Q11693> ;
	skos:broader	medtop:20000346 .

medtop:20000348
	rdf:type skos:Concept ;
	skos:prefLabel	"budgets and budgeting"@en-GB ;
	skos:definition	"A method of balancing revenues against expenses"@en-GB ;
	skos:inScheme <http://cv.iptc.org/newscodes/mediatopic/>  ;
	ikos:created "2009-10-22T02:00:00+00:00"^^xsd:dateTime ;
	dct:created "2009-10-22T02:00:00+00:00"^^xsd:dateTime ;
	ikos:modified "2021-02-18T12:00:00+00:00"^^xsd:dateTime ;
	dct:modified "2021-02-18T12:00:00+00:00"^^xsd:dateTime  ;
	skos:exactMatch subj:04008019 ;
	skos:exactMatch <https://www.wikidata.org/entity/Q41263> ;
	skos:broader	medtop:20000346 .

medtop:20000349
	rdf:type skos:Concept ;
	skos:prefLabel	"business enterprise"@en-GB ;
	skos:definition	"Organisations set up usually for profit-making purposes by creating and selling a product or service"@en-GB ;
	skos:inScheme <http://cv.iptc.org/newscodes/mediatopic/>  ;
	ikos:created "2009-10-22T02:00:00+00:00"^^xsd:dateTime ;
	dct:created "2009-10-22T02:00:00+00:00"^^xsd:dateTime ;
	ikos:modified "2021-02-18T12:00:00+00:00"^^xsd:dateTime ;
	dct:modified "2021-02-18T12:00:00+00:00"^^xsd:dateTime  ;
	skos:exactMatch subj:04008034 ;
	skos:exactMatch <https://www.wikidata.org/entity/Q4830453> ;
	skos:broader	medtop:20000346 ;
	skos:narrower	medtop:20001158 ;
	skos:narrower	medtop:20001172 ;
	skos:narrower	medtop:20001278 .

medtop:20000350
	rdf:type skos:Concept ;
	skos:prefLabel	"central bank"@en-GB ;
	skos:definition	"A country's major bank that sets interest rates, and provides transfer of funds between commercial banks"@en-GB ;
	skos:inScheme <http://cv.iptc.org/newscodes/mediatopic/>  ;
	ikos:created "2009-10-22T02:00:00+00:00"^^xsd:dateTime ;
	dct:created "2009-10-22T02:00:00+00:00"^^xsd:dateTime ;
	ikos:modified "2021-02-18T12:00:00+00:00"^^xsd:dateTime ;
	dct:modified "2021-02-18T12:00:00+00:00"^^xsd:dateTime  ;
	skos:exactMatch subj:04008001 ;
	skos:exactMatch <https://www.wikidata.org/entity/Q66344> ;
	skos:broader	medtop:20000346 .

medtop:20000351
	rdf:type skos:Concept ;
	skos:prefLabel	"consumers"@en-GB ;
	skos:definition	"Buyers of goods and services"@en-GB ;
	skos:inScheme <http://cv.iptc.org/newscodes/mediatopic/>  ;
	ikos:created "2009-10-22T02:00:00+00:00"^^xsd:dateTime ;
	dct:created "2009-10-22T02:00:00+00:00"^^xsd:dateTime ;
	ikos:modified "2021-02-18T12:00:00+00:00"^^xsd:dateTime ;
	dct:modified "2021-02-18T12:00:00+00:00"^^xsd:dateTime  ;
	skos:exactMatch subj:04016055 ;
	skos:exactMatch <https://www.wikidata.org/entity/Q22855> ;
	skos:broader	medtop:20000346 ;
	skos:narrower	medtop:20000352 ;
	skos:narrower	medtop:20000353 .

medtop:20000352
	rdf:type skos:Concept ;
	skos:prefLabel	"consumer confidence"@en-GB ;
	skos:definition	"The confidence of consumers in the economy."@en-GB ;
	skos:inScheme <http://cv.iptc.org/newscodes/mediatopic/>  ;
	ikos:created "2009-10-22T02:00:00+00:00"^^xsd:dateTime ;
	dct:created "2009-10-22T02:00:00+00:00"^^xsd:dateTime ;
	ikos:modified "2021-02-18T12:00:00+00:00"^^xsd:dateTime ;
	dct:modified "2021-02-18T12:00:00+00:00"^^xsd:dateTime  ;
	skos:exactMatch subj:04008014 ;
	skos:exactMatch <https://www.wikidata.org/entity/Q4925768> ;
	skos:broader	medtop:20000351 .

medtop:20000353
	rdf:type skos:Concept ;
	skos:prefLabel	"consumer issue"@en-GB ;
	skos:definition	"Issues, such as prices, inflation/deflation, quality of goods, at the retail sales level"@en-GB ;
	skos:inScheme <http://cv.iptc.org/newscodes/mediatopic/>  ;
	ikos:created "2009-10-22T02:00:00+00:00"^^xsd:dateTime ;
	dct:created "2009-10-22T02:00:00+00:00"^^xsd:dateTime ;
	ikos:modified "2021-02-18T12:00:00+00:00"^^xsd:dateTime ;
	dct:modified "2021-02-18T12:00:00+00:00"^^xsd:dateTime  ;
	skos:exactMatch subj:04008002 ;
	skos:exactMatch <https://www.wikidata.org/entity/Q664183> ;
	skos:broader	medtop:20000351 .

medtop:20000354
	rdf:type skos:Concept ;
	skos:prefLabel	"credit and debt"@en-GB ;
	skos:definition	"Credit: the amount of money available to you, often by loan. Debt: the amount you owe."@en-GB ;
	skos:inScheme <http://cv.iptc.org/newscodes/mediatopic/>  ;
	ikos:created "2009-10-22T02:00:00+00:00"^^xsd:dateTime ;
	dct:created "2009-10-22T02:00:00+00:00"^^xsd:dateTime ;
	ikos:modified "2021-02-18T12:00:00+00:00"^^xsd:dateTime ;
	dct:modified "2021-02-18T12:00:00+00:00"^^xsd:dateTime  ;
	skos:exactMatch subj:04008020 ;
	skos:exactMatch <https://www.wikidata.org/entity/Q3196867> ;
	skos:broader	medtop:20000346 .

medtop:20000355
	rdf:type skos:Concept ;
	skos:prefLabel	"currency"@en-GB ;
	skos:definition	"the system of money used by a country, including the value of one currency as measured against another"@en-GB ;
	skos:inScheme <http://cv.iptc.org/newscodes/mediatopic/>  ;
	ikos:created "2009-10-22T02:00:00+00:00"^^xsd:dateTime ;
	dct:created "2009-10-22T02:00:00+00:00"^^xsd:dateTime ;
	ikos:modified "2021-02-18T12:00:00+00:00"^^xsd:dateTime ;
	dct:modified "2021-02-18T12:00:00+00:00"^^xsd:dateTime  ;
	skos:exactMatch subj:04008018 ;
	skos:exactMatch <https://www.wikidata.org/entity/Q66100> ;
	skos:broader	medtop:20000346 ;
	skos:narrower	medtop:20001279 .

medtop:20000356
	rdf:type skos:Concept ;
	skos:prefLabel	"deflation"@en-GB ;
	skos:definition	"A fall in prices"@en-GB ;
	skos:inScheme <http://cv.iptc.org/newscodes/mediatopic/>  ;
	ikos:created "2009-10-22T02:00:00+00:00"^^xsd:dateTime ;
	dct:created "2009-10-22T02:00:00+00:00"^^xsd:dateTime ;
	ikos:modified "2021-02-18T12:00:00+00:00"^^xsd:dateTime ;
	dct:modified "2021-02-18T12:00:00+00:00"^^xsd:dateTime  ;
	skos:broadMatch subj:04008016 ;
	skos:exactMatch <https://www.wikidata.org/entity/Q161081> ;
	skos:broader	medtop:20000346 .

medtop:20000357
	rdf:type skos:Concept ;
	skos:prefLabel	"economic growth"@en-GB ;
	skos:definition	"An increase of the GDP"@en-GB ;
	skos:inScheme <http://cv.iptc.org/newscodes/mediatopic/>  ;
	ikos:created "2009-10-22T02:00:00+00:00"^^xsd:dateTime ;
	dct:created "2009-10-22T02:00:00+00:00"^^xsd:dateTime ;
	ikos:modified "2021-02-18T12:00:00+00:00"^^xsd:dateTime ;
	dct:modified "2021-02-18T12:00:00+00:00"^^xsd:dateTime  ;
	skos:broadMatch subj:04000000 ;
	skos:exactMatch <https://www.wikidata.org/entity/Q189833> ;
	skos:broader	medtop:20000346 .

medtop:20000358
	rdf:type skos:Concept ;
	skos:prefLabel	"economic indicator"@en-GB ;
	skos:definition	"Certain indexes, such as company inventories, the movement of prices that show whether the economy is improving or declining"@en-GB ;
	skos:inScheme <http://cv.iptc.org/newscodes/mediatopic/>  ;
	ikos:created "2009-10-22T02:00:00+00:00"^^xsd:dateTime ;
	dct:created "2009-10-22T02:00:00+00:00"^^xsd:dateTime ;
	ikos:modified "2021-02-18T12:00:00+00:00"^^xsd:dateTime ;
	dct:modified "2021-02-18T12:00:00+00:00"^^xsd:dateTime  ;
	skos:exactMatch subj:04008004 ;
	skos:exactMatch <https://www.wikidata.org/entity/Q1167393> ;
	skos:broader	medtop:20000346 ;
	skos:narrower	medtop:20000359 ;
	skos:narrower	medtop:20000360 ;
	skos:narrower	medtop:20000361 ;
	skos:narrower	medtop:20000362 .

medtop:20000359
	rdf:type skos:Concept ;
	skos:prefLabel	"gross domestic product"@en-GB ;
	skos:definition	"A measure of a region's economic performance, commonly abbreviated as GDP"@en-GB ;
	skos:inScheme <http://cv.iptc.org/newscodes/mediatopic/>  ;
	ikos:created "2009-10-22T02:00:00+00:00"^^xsd:dateTime ;
	dct:created "2009-10-22T02:00:00+00:00"^^xsd:dateTime ;
	ikos:modified "2021-02-18T12:00:00+00:00"^^xsd:dateTime ;
	dct:modified "2021-02-18T12:00:00+00:00"^^xsd:dateTime  ;
	skos:broadMatch subj:04000000 ;
	skos:exactMatch <https://www.wikidata.org/entity/Q12638> ;
	skos:broader	medtop:20000358 .

medtop:20000360
	rdf:type skos:Concept ;
	skos:prefLabel	"industrial production"@en-GB ;
	skos:definition	"Manufacture of durable and non-durable goods"@en-GB ;
	skos:inScheme <http://cv.iptc.org/newscodes/mediatopic/>  ;
	ikos:created "2009-10-22T02:00:00+00:00"^^xsd:dateTime ;
	dct:created "2009-10-22T02:00:00+00:00"^^xsd:dateTime ;
	ikos:modified "2021-02-18T12:00:00+00:00"^^xsd:dateTime ;
	dct:modified "2021-02-18T12:00:00+00:00"^^xsd:dateTime  ;
	skos:exactMatch subj:04016042 ;
	skos:exactMatch <https://www.wikidata.org/entity/Q1419090> ;
	skos:broader	medtop:20000358 .

medtop:20000361
	rdf:type skos:Concept ;
	skos:prefLabel	"inventories"@en-GB ;
	skos:definition	"Goods not sold and held by the producer, wholesaler or retailer"@en-GB ;
	skos:inScheme <http://cv.iptc.org/newscodes/mediatopic/>  ;
	ikos:created "2009-10-22T02:00:00+00:00"^^xsd:dateTime ;
	dct:created "2009-10-22T02:00:00+00:00"^^xsd:dateTime ;
	ikos:modified "2021-02-18T12:00:00+00:00"^^xsd:dateTime ;
	dct:modified "2021-02-18T12:00:00+00:00"^^xsd:dateTime  ;
	skos:exactMatch subj:04016044 ;
	skos:exactMatch <https://www.wikidata.org/entity/Q815410> ;
	skos:broader	medtop:20000358 .

medtop:20000362
	rdf:type skos:Concept ;
	skos:prefLabel	"productivity"@en-GB ;
	skos:definition	"A measure of output from production or service"@en-GB ;
	skos:inScheme <http://cv.iptc.org/newscodes/mediatopic/>  ;
	ikos:created "2009-10-22T02:00:00+00:00"^^xsd:dateTime ;
	dct:created "2009-10-22T02:00:00+00:00"^^xsd:dateTime ;
	ikos:modified "2021-02-18T12:00:00+00:00"^^xsd:dateTime ;
	dct:modified "2021-02-18T12:00:00+00:00"^^xsd:dateTime  ;
	skos:exactMatch subj:04016043 ;
	skos:exactMatch <https://www.wikidata.org/entity/Q2111958> ;
	skos:broader	medtop:20000358 .

medtop:20000363
	rdf:type skos:Concept ;
	skos:prefLabel	"economic organisation"@en-GB ;
	skos:definition	"Business, industrial and trade associations, societies and other private-sector groups."@en-GB ;
	skos:inScheme <http://cv.iptc.org/newscodes/mediatopic/>  ;
	ikos:created "2009-10-22T02:00:00+00:00"^^xsd:dateTime ;
	dct:created "2009-10-22T02:00:00+00:00"^^xsd:dateTime ;
	ikos:modified "2021-02-18T12:00:00+00:00"^^xsd:dateTime ;
	dct:modified "2021-02-18T12:00:00+00:00"^^xsd:dateTime  ;
	skos:exactMatch subj:04008013 ;
	skos:broader	medtop:20000346 .

medtop:20000364
	rdf:type skos:Concept ;
	skos:prefLabel	"emerging market"@en-GB ;
	skos:definition	"Those markets that are struggling to enter the world economies and those requiring financial help from international lenders"@en-GB ;
	skos:inScheme <http://cv.iptc.org/newscodes/mediatopic/>  ;
	ikos:created "2009-10-22T02:00:00+00:00"^^xsd:dateTime ;
	dct:created "2009-10-22T02:00:00+00:00"^^xsd:dateTime ;
	ikos:modified "2021-02-18T12:00:00+00:00"^^xsd:dateTime ;
	dct:modified "2021-02-18T12:00:00+00:00"^^xsd:dateTime  ;
	skos:exactMatch subj:04008005 ;
	skos:exactMatch <https://www.wikidata.org/entity/Q546395> ;
	skos:broader	medtop:20000346 .

medtop:20000365
	rdf:type skos:Concept ;
	skos:prefLabel	"employment statistics"@en-GB ;
	skos:definition	"Statistics about employment"@en-GB ;
	skos:inScheme <http://cv.iptc.org/newscodes/mediatopic/>  ;
	ikos:created "2009-10-22T02:00:00+00:00"^^xsd:dateTime ;
	dct:created "2009-10-22T02:00:00+00:00"^^xsd:dateTime ;
	ikos:modified "2021-02-18T12:00:00+00:00"^^xsd:dateTime ;
	dct:modified "2021-02-18T12:00:00+00:00"^^xsd:dateTime  ;
	skos:broadMatch subj:04008000 ;
	skos:broader	medtop:20000346 .

medtop:20000366
	rdf:type skos:Concept ;
	skos:prefLabel	"exports"@en-GB ;
	skos:definition	"What is produced or manufactured in your country and sent and sold elsewhere"@en-GB ;
	skos:inScheme <http://cv.iptc.org/newscodes/mediatopic/>  ;
	ikos:created "2009-10-22T02:00:00+00:00"^^xsd:dateTime ;
	dct:created "2009-10-22T02:00:00+00:00"^^xsd:dateTime ;
	ikos:modified "2021-02-18T12:00:00+00:00"^^xsd:dateTime ;
	dct:modified "2021-02-18T12:00:00+00:00"^^xsd:dateTime  ;
	skos:exactMatch subj:04008031 ;
	skos:exactMatch <https://www.wikidata.org/entity/Q182722> ;
	skos:broader	medtop:20000346 .

medtop:20000367
	rdf:type skos:Concept ;
	skos:prefLabel	"government aid"@en-GB ;
	skos:definition	"Supply of financial and other help by one government, usually to another"@en-GB ;
	skos:inScheme <http://cv.iptc.org/newscodes/mediatopic/>  ;
	ikos:created "2009-10-22T02:00:00+00:00"^^xsd:dateTime ;
	dct:created "2009-10-22T02:00:00+00:00"^^xsd:dateTime ;
	ikos:modified "2021-02-18T12:00:00+00:00"^^xsd:dateTime ;
	dct:modified "2021-02-18T12:00:00+00:00"^^xsd:dateTime  ;
	skos:exactMatch subj:04008007 ;
	skos:exactMatch <https://www.wikidata.org/entity/Q12002754> ;
	skos:broader	medtop:20000346 .

medtop:20000368
	rdf:type skos:Concept ;
	skos:prefLabel	"government debt"@en-GB ;
	skos:definition	"The amount a government owes on bonds, services and for goods and services for which it has no ready cash"@en-GB ;
	skos:inScheme <http://cv.iptc.org/newscodes/mediatopic/>  ;
	ikos:created "2009-10-22T02:00:00+00:00"^^xsd:dateTime ;
	dct:created "2009-10-22T02:00:00+00:00"^^xsd:dateTime ;
	ikos:modified "2021-02-18T12:00:00+00:00"^^xsd:dateTime ;
	dct:modified "2021-02-18T12:00:00+00:00"^^xsd:dateTime  ;
	skos:exactMatch subj:04008008 ;
	skos:exactMatch <https://www.wikidata.org/entity/Q12695> ;
	skos:broader	medtop:20000346 .

medtop:20000369
	rdf:type skos:Concept ;
	skos:prefLabel	"imports"@en-GB ;
	skos:definition	"What is bought abroad and brought into a country for resale"@en-GB ;
	skos:inScheme <http://cv.iptc.org/newscodes/mediatopic/>  ;
	ikos:created "2009-10-22T02:00:00+00:00"^^xsd:dateTime ;
	dct:created "2009-10-22T02:00:00+00:00"^^xsd:dateTime ;
	ikos:modified "2021-02-18T12:00:00+00:00"^^xsd:dateTime ;
	dct:modified "2021-02-18T12:00:00+00:00"^^xsd:dateTime  ;
	skos:exactMatch subj:04008030 ;
	skos:exactMatch <https://www.wikidata.org/entity/Q62955> ;
	skos:broader	medtop:20000346 .

medtop:20000370
	rdf:type skos:Concept ;
	skos:prefLabel	"inflation"@en-GB ;
	skos:definition	"A rise in prices"@en-GB ;
	skos:inScheme <http://cv.iptc.org/newscodes/mediatopic/>  ;
	ikos:created "2009-10-22T02:00:00+00:00"^^xsd:dateTime ;
	dct:created "2009-10-22T02:00:00+00:00"^^xsd:dateTime ;
	ikos:modified "2021-02-18T12:00:00+00:00"^^xsd:dateTime ;
	dct:modified "2021-02-18T12:00:00+00:00"^^xsd:dateTime  ;
	skos:broadMatch subj:04008016 ;
	skos:exactMatch <https://www.wikidata.org/entity/Q35865> ;
	skos:broader	medtop:20000346 .

medtop:20000371
	rdf:type skos:Concept ;
	skos:prefLabel	"interest rate"@en-GB ;
	skos:definition	"The amount of money one must pay to borrow money"@en-GB ;
	skos:inScheme <http://cv.iptc.org/newscodes/mediatopic/>  ;
	ikos:created "2009-10-22T02:00:00+00:00"^^xsd:dateTime ;
	dct:created "2009-10-22T02:00:00+00:00"^^xsd:dateTime ;
	ikos:modified "2021-02-18T12:00:00+00:00"^^xsd:dateTime ;
	dct:modified "2021-02-18T12:00:00+00:00"^^xsd:dateTime  ;
	skos:exactMatch subj:04008009 ;
	skos:exactMatch <https://www.wikidata.org/entity/Q179179> ;
	skos:broader	medtop:20000346 .

medtop:20000372
	rdf:type skos:Concept ;
	skos:prefLabel	"international economic institution"@en-GB ;
	skos:definition	"Entities such as UNIDO, World Bank, World Trade Organization, the Import-Expert Bank etc that deals at a world level"@en-GB ;
	skos:inScheme <http://cv.iptc.org/newscodes/mediatopic/>  ;
	ikos:created "2009-10-22T02:00:00+00:00"^^xsd:dateTime ;
	dct:created "2009-10-22T02:00:00+00:00"^^xsd:dateTime ;
	ikos:modified "2021-05-05T12:00:00+00:00"^^xsd:dateTime ;
	dct:modified "2021-05-05T12:00:00+00:00"^^xsd:dateTime  ;
	skos:exactMatch subj:04008010 ;
	skos:exactMatch <https://www.wikidata.org/entity/Q1345691> ;
	skos:broader	medtop:20000346 .

medtop:20000373
	rdf:type skos:Concept ;
	skos:prefLabel	"international trade"@en-GB ;
	skos:definition	"Trade of goods and services between nations"@en-GB ;
	skos:inScheme <http://cv.iptc.org/newscodes/mediatopic/>  ;
	ikos:created "2009-10-22T02:00:00+00:00"^^xsd:dateTime ;
	dct:created "2009-10-22T02:00:00+00:00"^^xsd:dateTime ;
	ikos:modified "2021-02-18T12:00:00+00:00"^^xsd:dateTime ;
	dct:modified "2021-02-18T12:00:00+00:00"^^xsd:dateTime  ;
	skos:exactMatch subj:04008011 ;
	skos:exactMatch <https://www.wikidata.org/entity/Q178803> ;
	skos:broader	medtop:20000346 ;
	skos:narrower	medtop:20000374 ;
	skos:narrower	medtop:20000375 ;
	skos:narrower	medtop:20000376 ;
	skos:narrower	medtop:20000377 .

medtop:20000374
	rdf:type skos:Concept ;
	skos:prefLabel	"trade agreements"@en-GB ;
	skos:definition	"Government level agreements between countries for the sale and purchase of goods and services"@en-GB ;
	skos:inScheme <http://cv.iptc.org/newscodes/mediatopic/>  ;
	ikos:created "2009-10-22T02:00:00+00:00"^^xsd:dateTime ;
	dct:created "2009-10-22T02:00:00+00:00"^^xsd:dateTime ;
	ikos:modified "2021-02-18T12:00:00+00:00"^^xsd:dateTime ;
	dct:modified "2021-02-18T12:00:00+00:00"^^xsd:dateTime  ;
	skos:exactMatch subj:04008032 ;
	skos:exactMatch <https://www.wikidata.org/entity/Q252550> ;
	skos:broader	medtop:20000373 .

medtop:20000375
	rdf:type skos:Concept ;
	skos:prefLabel	"trade balance"@en-GB ;
	skos:definition	"The difference between the financial value of imports and exports"@en-GB ;
	skos:inScheme <http://cv.iptc.org/newscodes/mediatopic/>  ;
	ikos:created "2009-10-22T02:00:00+00:00"^^xsd:dateTime ;
	dct:created "2009-10-22T02:00:00+00:00"^^xsd:dateTime ;
	ikos:modified "2021-02-18T12:00:00+00:00"^^xsd:dateTime ;
	dct:modified "2021-02-18T12:00:00+00:00"^^xsd:dateTime  ;
	skos:exactMatch subj:04008036 ;
	skos:exactMatch <https://www.wikidata.org/entity/Q192796> ;
	skos:broader	medtop:20000373 .

medtop:20000376
	rdf:type skos:Concept ;
	skos:prefLabel	"trade dispute"@en-GB ;
	skos:definition	"International dispute over trade barriers, cartels, dumping etc."@en-GB ;
	skos:inScheme <http://cv.iptc.org/newscodes/mediatopic/>  ;
	ikos:created "2009-10-22T02:00:00+00:00"^^xsd:dateTime ;
	dct:created "2009-10-22T02:00:00+00:00"^^xsd:dateTime ;
	ikos:modified "2021-05-05T12:00:00+00:00"^^xsd:dateTime ;
	dct:modified "2021-05-05T12:00:00+00:00"^^xsd:dateTime  ;
	skos:exactMatch subj:04008015 ;
	skos:exactMatch <https://www.wikidata.org/entity/Q692412> ;
	skos:broader	medtop:20000373 .

medtop:20000377
	rdf:type skos:Concept ;
	skos:prefLabel	"trade policy"@en-GB ;
	skos:definition	"Governmental decisions on tariffs, shipping, embargoes, and the types or kinds of goods and services to be imported and exported"@en-GB ;
	skos:inScheme <http://cv.iptc.org/newscodes/mediatopic/>  ;
	ikos:created "2009-10-22T02:00:00+00:00"^^xsd:dateTime ;
	dct:created "2009-10-22T02:00:00+00:00"^^xsd:dateTime ;
	ikos:modified "2021-02-18T12:00:00+00:00"^^xsd:dateTime ;
	dct:modified "2021-02-18T12:00:00+00:00"^^xsd:dateTime  ;
	skos:exactMatch subj:04008033 ;
	skos:exactMatch <https://www.wikidata.org/entity/Q959108> ;
	skos:broader	medtop:20000373 .

medtop:20000378
	rdf:type skos:Concept ;
	skos:prefLabel	"investments"@en-GB ;
	skos:definition	"Speculative purchases of corporate instruments, of commodities, currencies, or parts thereof"@en-GB ;
	skos:inScheme <http://cv.iptc.org/newscodes/mediatopic/>  ;
	ikos:created "2009-10-22T02:00:00+00:00"^^xsd:dateTime ;
	dct:created "2009-10-22T02:00:00+00:00"^^xsd:dateTime ;
	ikos:modified "2021-02-18T12:00:00+00:00"^^xsd:dateTime ;
	dct:modified "2021-02-18T12:00:00+00:00"^^xsd:dateTime  ;
	skos:exactMatch subj:04008025 ;
	skos:exactMatch <https://www.wikidata.org/entity/Q4290> ;
	skos:broader	medtop:20000346 .

medtop:20000379
	rdf:type skos:Concept ;
	skos:prefLabel	"monetary policy"@en-GB ;
	skos:definition	"Government bank directed policy on the amount of money in circulation and the rate at which it can be loaned"@en-GB ;
	skos:inScheme <http://cv.iptc.org/newscodes/mediatopic/>  ;
	ikos:created "2009-10-22T02:00:00+00:00"^^xsd:dateTime ;
	dct:created "2009-10-22T02:00:00+00:00"^^xsd:dateTime ;
	ikos:modified "2021-02-18T12:00:00+00:00"^^xsd:dateTime ;
	dct:modified "2021-02-18T12:00:00+00:00"^^xsd:dateTime  ;
	skos:exactMatch subj:04019001 ;
	skos:exactMatch <https://www.wikidata.org/entity/Q178476> ;
	skos:broader	medtop:20000346 .

medtop:20000380
	rdf:type skos:Concept ;
	skos:prefLabel	"mortgage"@en-GB ;
	skos:definition	"The loan of money for the purpose of purchasing a property, whether land or building. Or, for homeowners to repair or maintain properties, often based on owner equity in a property"@en-GB ;
	skos:inScheme <http://cv.iptc.org/newscodes/mediatopic/>  ;
	ikos:created "2009-10-22T02:00:00+00:00"^^xsd:dateTime ;
	dct:created "2009-10-22T02:00:00+00:00"^^xsd:dateTime ;
	ikos:modified "2021-02-18T12:00:00+00:00"^^xsd:dateTime ;
	dct:modified "2021-02-18T12:00:00+00:00"^^xsd:dateTime  ;
	skos:exactMatch subj:04008022 ;
	skos:exactMatch <https://www.wikidata.org/entity/Q1210094> ;
	skos:broader	medtop:20000346 .

medtop:20000381
	rdf:type skos:Concept ;
	skos:prefLabel	"mutual funds"@en-GB ;
	skos:definition	"Pools of shares or bonds for sale often grouped by investment intention, such as growth, income or security"@en-GB ;
	skos:inScheme <http://cv.iptc.org/newscodes/mediatopic/>  ;
	ikos:created "2009-10-22T02:00:00+00:00"^^xsd:dateTime ;
	dct:created "2009-10-22T02:00:00+00:00"^^xsd:dateTime ;
	ikos:modified "2021-02-18T12:00:00+00:00"^^xsd:dateTime ;
	dct:modified "2021-02-18T12:00:00+00:00"^^xsd:dateTime  ;
	skos:exactMatch subj:04008028 ;
	skos:exactMatch <https://www.wikidata.org/entity/Q791974> ;
	skos:broader	medtop:20000346 .

medtop:20000382
	rdf:type skos:Concept ;
	skos:prefLabel	"prices"@en-GB ;
	skos:definition	"The monetary value of goods, services or stocks and bonds"@en-GB ;
	skos:inScheme <http://cv.iptc.org/newscodes/mediatopic/>  ;
	ikos:created "2009-10-22T02:00:00+00:00"^^xsd:dateTime ;
	dct:created "2009-10-22T02:00:00+00:00"^^xsd:dateTime ;
	ikos:modified "2021-02-18T12:00:00+00:00"^^xsd:dateTime ;
	dct:modified "2021-02-18T12:00:00+00:00"^^xsd:dateTime  ;
	skos:exactMatch subj:04008017 ;
	skos:exactMatch <https://www.wikidata.org/entity/Q160151> ;
	skos:broader	medtop:20000346 .

medtop:20000383
	rdf:type skos:Concept ;
	skos:prefLabel	"recession"@en-GB ;
	skos:definition	"A decrease in the GDP over a period of 2 quarters in a row."@en-GB ;
	skos:inScheme <http://cv.iptc.org/newscodes/mediatopic/>  ;
	ikos:created "2009-10-22T02:00:00+00:00"^^xsd:dateTime ;
	dct:created "2009-10-22T02:00:00+00:00"^^xsd:dateTime ;
	ikos:modified "2021-02-18T12:00:00+00:00"^^xsd:dateTime ;
	dct:modified "2021-02-18T12:00:00+00:00"^^xsd:dateTime  ;
	skos:broadMatch subj:04000000 ;
	skos:exactMatch <https://www.wikidata.org/entity/Q176494> ;
	skos:broader	medtop:20000346 .

medtop:20000384
	rdf:type skos:Concept ;
	skos:prefLabel	"tariff"@en-GB ;
	skos:definition	"Fees placed on goods imported or exported, often punitive"@en-GB ;
	skos:inScheme <http://cv.iptc.org/newscodes/mediatopic/>  ;
	ikos:created "2009-10-22T02:00:00+00:00"^^xsd:dateTime ;
	dct:created "2009-10-22T02:00:00+00:00"^^xsd:dateTime ;
	ikos:modified "2021-02-18T12:00:00+00:00"^^xsd:dateTime ;
	dct:modified "2021-02-18T12:00:00+00:00"^^xsd:dateTime  ;
	skos:exactMatch subj:04008035 ;
	skos:exactMatch <https://www.wikidata.org/entity/Q52389> ;
	skos:broader	medtop:20000346 .

medtop:20000385
	rdf:type skos:Concept ;
	skos:prefLabel	"market and exchange"@en-GB ;
	skos:definition	"Organised entities for buying and selling stocks, currencies, commodities and other goods"@en-GB ;
	skos:inScheme <http://cv.iptc.org/newscodes/mediatopic/>  ;
	ikos:created "2009-10-22T02:00:00+00:00"^^xsd:dateTime ;
	dct:created "2009-10-22T02:00:00+00:00"^^xsd:dateTime ;
	ikos:modified "2021-02-18T12:00:00+00:00"^^xsd:dateTime ;
	dct:modified "2021-02-18T12:00:00+00:00"^^xsd:dateTime  ;
	skos:exactMatch subj:04009000 ;
	skos:exactMatch <https://www.wikidata.org/entity/Q179076> ;
	skos:broader	medtop:04000000 ;
	skos:narrower	medtop:20000386 ;
	skos:narrower	medtop:20000390 ;
	skos:narrower	medtop:20000391 ;
	skos:narrower	medtop:20000392 .

medtop:20000386
	rdf:type skos:Concept ;
	skos:prefLabel	"commodity market"@en-GB ;
	skos:definition	"The bartering or trading of goods such as cotton, oil, coal, metals, etc"@en-GB ;
	skos:inScheme <http://cv.iptc.org/newscodes/mediatopic/>  ;
	ikos:created "2009-10-22T02:00:00+00:00"^^xsd:dateTime ;
	dct:created "2009-10-22T02:00:00+00:00"^^xsd:dateTime ;
	ikos:modified "2021-02-18T12:00:00+00:00"^^xsd:dateTime ;
	dct:modified "2021-02-18T12:00:00+00:00"^^xsd:dateTime  ;
	skos:exactMatch subj:04008024 ;
	skos:exactMatch <https://www.wikidata.org/entity/Q2922469> ;
	skos:broader	medtop:20000385 ;
	skos:narrower	medtop:20000387 ;
	skos:narrower	medtop:20000388 ;
	skos:narrower	medtop:20000389 .

medtop:20000387
	rdf:type skos:Concept ;
	skos:prefLabel	"energy market"@en-GB ;
	skos:definition	"Energy trading and markets"@en-GB ;
	skos:inScheme <http://cv.iptc.org/newscodes/mediatopic/>  ;
	ikos:created "2009-10-22T02:00:00+00:00"^^xsd:dateTime ;
	dct:created "2009-10-22T02:00:00+00:00"^^xsd:dateTime ;
	ikos:modified "2021-02-18T12:00:00+00:00"^^xsd:dateTime ;
	dct:modified "2021-02-18T12:00:00+00:00"^^xsd:dateTime  ;
	skos:exactMatch subj:04009001 ;
	skos:exactMatch <https://www.wikidata.org/entity/Q1239166> ;
	skos:broader	medtop:20000386 .

medtop:20000388
	rdf:type skos:Concept ;
	skos:prefLabel	"metal"@en-GB ;
	skos:definition	"Markets for trading base metals such as copper, aluminium, steel, zinc etc"@en-GB ;
	skos:inScheme <http://cv.iptc.org/newscodes/mediatopic/>  ;
	ikos:created "2009-10-22T02:00:00+00:00"^^xsd:dateTime ;
	dct:created "2009-10-22T02:00:00+00:00"^^xsd:dateTime ;
	ikos:modified "2021-02-18T12:00:00+00:00"^^xsd:dateTime ;
	dct:modified "2021-02-18T12:00:00+00:00"^^xsd:dateTime  ;
	skos:exactMatch subj:04009002 ;
	skos:exactMatch <https://www.wikidata.org/entity/Q56557589> ;
	skos:broader	medtop:20000386 .

medtop:20000389
	rdf:type skos:Concept ;
	skos:prefLabel	"soft commodity"@en-GB ;
	skos:definition	"Trading in commodities such as cotton, sugar, sorghum, soybeans etc."@en-GB ;
	skos:changeNote	"Retired. Use medtop:20000386 commodity market instead."@en-GB ;
	skos:inScheme <http://cv.iptc.org/newscodes/mediatopic/>  ;
	ikos:created "2009-10-22T02:00:00+00:00"^^xsd:dateTime ;
	dct:created "2009-10-22T02:00:00+00:00"^^xsd:dateTime ;
	ikos:modified "2023-10-02T12:00:00+00:00"^^xsd:dateTime ;
	dct:modified "2023-10-02T12:00:00+00:00"^^xsd:dateTime  ; 
	ikos:retired "2023-10-02T12:00:00+00:00"^^xsd:dateTime ;
	skos:exactMatch subj:04009004 ;
	skos:exactMatch <https://www.wikidata.org/entity/Q396212> ;
	skos:broader	medtop:20000386 .

medtop:20000390
	rdf:type skos:Concept ;
	skos:prefLabel	"debt market"@en-GB ;
	skos:definition	"Market for trading debt instruments such as bonds, CDs, banker's acceptances, T-bills, notes, IOUs etc"@en-GB ;
	skos:inScheme <http://cv.iptc.org/newscodes/mediatopic/>  ;
	ikos:created "2009-10-22T02:00:00+00:00"^^xsd:dateTime ;
	dct:created "2009-10-22T02:00:00+00:00"^^xsd:dateTime ;
	ikos:modified "2021-05-05T12:00:00+00:00"^^xsd:dateTime ;
	dct:modified "2021-05-05T12:00:00+00:00"^^xsd:dateTime  ;
	skos:exactMatch subj:04008003 ;
	skos:exactMatch <https://www.wikidata.org/entity/Q540626> ;
	skos:broader	medtop:20000385 .

medtop:20000391
	rdf:type skos:Concept ;
	skos:prefLabel	"foreign exchange market"@en-GB ;
	skos:definition	"The trading of shekels, dinars, euros, dollars etc around the world through regulated markets"@en-GB ;
	skos:inScheme <http://cv.iptc.org/newscodes/mediatopic/>  ;
	ikos:created "2009-10-22T02:00:00+00:00"^^xsd:dateTime ;
	dct:created "2009-10-22T02:00:00+00:00"^^xsd:dateTime ;
	ikos:modified "2021-02-18T12:00:00+00:00"^^xsd:dateTime ;
	dct:modified "2021-02-18T12:00:00+00:00"^^xsd:dateTime  ;
	skos:exactMatch subj:04008006 ;
	skos:exactMatch <https://www.wikidata.org/entity/Q66076> ;
	skos:broader	medtop:20000385 .

medtop:20000392
	rdf:type skos:Concept ;
	skos:prefLabel	"loan market"@en-GB ;
	skos:definition	"The market where money is available to borrow, at certain rates of interest"@en-GB ;
	skos:inScheme <http://cv.iptc.org/newscodes/mediatopic/>  ;
	ikos:created "2009-10-22T02:00:00+00:00"^^xsd:dateTime ;
	dct:created "2009-10-22T02:00:00+00:00"^^xsd:dateTime ;
	ikos:modified "2021-02-18T12:00:00+00:00"^^xsd:dateTime ;
	dct:modified "2021-02-18T12:00:00+00:00"^^xsd:dateTime  ;
	skos:exactMatch subj:04008012 ;
	skos:exactMatch <https://www.wikidata.org/entity/Q627543> ;
	skos:broader	medtop:20000385 ;
	skos:narrower	medtop:20000393 .

medtop:20000393
	rdf:type skos:Concept ;
	skos:prefLabel	"loans"@en-GB ;
	skos:definition	"An agreement by one individual or institution to temporarily disperse money to another, with an agreed rate and time for its return"@en-GB ;
	skos:inScheme <http://cv.iptc.org/newscodes/mediatopic/>  ;
	ikos:created "2009-10-22T02:00:00+00:00"^^xsd:dateTime ;
	dct:created "2009-10-22T02:00:00+00:00"^^xsd:dateTime ;
	ikos:modified "2021-02-18T12:00:00+00:00"^^xsd:dateTime ;
	dct:modified "2021-02-18T12:00:00+00:00"^^xsd:dateTime  ;
	skos:exactMatch subj:04008021 ;
	skos:exactMatch <https://www.wikidata.org/entity/Q189539> ;
	skos:broader	medtop:20000392 .

medtop:20000394
	rdf:type skos:Concept ;
	skos:prefLabel	"securities"@en-GB ;
	skos:definition	"Markets for trading types of company paper such as stocks and bonds"@en-GB ;
	skos:changeNote	"Retired. Use medtop:20000396 stocks and securities"@en-GB ;
	skos:inScheme <http://cv.iptc.org/newscodes/mediatopic/>  ;
	ikos:created "2009-10-22T02:00:00+00:00"^^xsd:dateTime ;
	dct:created "2009-10-22T02:00:00+00:00"^^xsd:dateTime ;
	ikos:modified "2023-03-31T12:00:00+00:00"^^xsd:dateTime ;
	dct:modified "2023-03-31T12:00:00+00:00"^^xsd:dateTime  ; 
	ikos:retired "2023-03-31T12:00:00+00:00"^^xsd:dateTime ;
	skos:exactMatch subj:04009003 ;
	skos:exactMatch <https://www.wikidata.org/entity/Q169489> ;
	skos:broader	medtop:20000183 ;
	skos:narrower	medtop:20000191 .

medtop:20000395
	rdf:type skos:Concept ;
	skos:prefLabel	"derivatives"@en-GB ;
	skos:definition	"Financial instruments such as futures, swaps and options that depend on an underlying instrument such as a commodity, bond, equity or currency"@en-GB ;
	skos:inScheme <http://cv.iptc.org/newscodes/mediatopic/>  ;
	ikos:created "2009-10-22T02:00:00+00:00"^^xsd:dateTime ;
	dct:created "2009-10-22T02:00:00+00:00"^^xsd:dateTime ;
	ikos:modified "2023-03-31T12:00:00+00:00"^^xsd:dateTime ;
	dct:modified "2023-03-31T12:00:00+00:00"^^xsd:dateTime  ;
	skos:exactMatch subj:04008029 ;
	skos:exactMatch <https://www.wikidata.org/entity/Q66295> ;
	skos:broader	medtop:20000396 .

medtop:20000396
	rdf:type skos:Concept ;
	skos:prefLabel	"stocks and securities"@en-GB ;
	skos:definition	"Financial insturments such as company shares and bonds"@en-GB ;
	skos:inScheme <http://cv.iptc.org/newscodes/mediatopic/>  ;
	ikos:created "2009-10-22T02:00:00+00:00"^^xsd:dateTime ;
	dct:created "2009-10-22T02:00:00+00:00"^^xsd:dateTime ;
	ikos:modified "2023-03-31T12:00:00+00:00"^^xsd:dateTime ;
	dct:modified "2023-03-31T12:00:00+00:00"^^xsd:dateTime  ;
	skos:exactMatch subj:04008026 ;
	skos:exactMatch <https://www.wikidata.org/entity/Q1196314> ;
	skos:broader	medtop:20000183 ;
	skos:narrower	medtop:20000175 ;
	skos:narrower	medtop:20000177 ;
	skos:narrower	medtop:20000186 ;
	skos:narrower	medtop:20000187 ;
	skos:narrower	medtop:20000395 ;
	skos:narrower	medtop:20001137 ;
	skos:narrower	medtop:20001141 .

medtop:20000398
	rdf:type skos:Concept ;
	skos:prefLabel	"parents group"@en-GB ;
	skos:definition	"Group of parents set up to support educational activities of their children"@en-GB ;
	skos:inScheme <http://cv.iptc.org/newscodes/mediatopic/>  ;
	ikos:created "2009-10-22T02:00:00+00:00"^^xsd:dateTime ;
	dct:created "2009-10-22T02:00:00+00:00"^^xsd:dateTime ;
	ikos:modified "2021-09-30T12:00:00+00:00"^^xsd:dateTime ;
	dct:modified "2021-09-30T12:00:00+00:00"^^xsd:dateTime  ;
	skos:closeMatch subj:05003000 ;
	skos:exactMatch <https://www.wikidata.org/entity/Q706242> ;
	skos:broader	medtop:05000000 .

medtop:20000399
	rdf:type skos:Concept ;
	skos:prefLabel	"religious education"@en-GB ;
	skos:definition	"Instruction by any faith about that faith's principles and beliefs, including Sunday school or preparation for a religious rite, such as a bar mitzvah"@en-GB ;
	skos:inScheme <http://cv.iptc.org/newscodes/mediatopic/>  ;
	ikos:created "2009-10-22T02:00:00+00:00"^^xsd:dateTime ;
	dct:created "2009-10-22T02:00:00+00:00"^^xsd:dateTime ;
	ikos:modified "2021-09-30T12:00:00+00:00"^^xsd:dateTime ;
	dct:modified "2021-09-30T12:00:00+00:00"^^xsd:dateTime  ;
	skos:exactMatch <https://www.wikidata.org/entity/Q1412471> ;
	skos:exactMatch subj:05011000 ;
	skos:broader	medtop:05000000 .

medtop:20000400
	rdf:type skos:Concept ;
	skos:prefLabel	"school"@en-GB ;
	skos:definition	"A building or institution in which education is provided"@en-GB ;
	skos:inScheme <http://cv.iptc.org/newscodes/mediatopic/>  ;
	ikos:created "2009-10-22T02:00:00+00:00"^^xsd:dateTime ;
	dct:created "2009-10-22T02:00:00+00:00"^^xsd:dateTime ;
	ikos:modified "2021-09-30T12:00:00+00:00"^^xsd:dateTime ;
	dct:modified "2021-09-30T12:00:00+00:00"^^xsd:dateTime  ;
	skos:exactMatch <https://www.wikidata.org/entity/Q3914> ;
	skos:exactMatch subj:05005000 ;
	skos:broader	medtop:05000000 ;
	skos:narrower	medtop:20000401 ;
	skos:narrower	medtop:20000402 ;
	skos:narrower	medtop:20000403 ;
	skos:narrower	medtop:20000404 ;
	skos:narrower	medtop:20000405 ;
	skos:narrower	medtop:20000408 ;
	skos:narrower	medtop:20000409 ;
	skos:narrower	medtop:20001212 ;
	skos:narrower	medtop:20001213 ;
	skos:narrower	medtop:20001214 ;
	skos:narrower	medtop:20001215 .

medtop:20000401
	rdf:type skos:Concept ;
	skos:prefLabel	"primary education"@en-GB ;
	skos:definition	"Education and schools designed to provide students with fundamental skills in reading, writing and mathematics and to establish a solid foundation for later learning"@en-GB ;
	skos:inScheme <http://cv.iptc.org/newscodes/mediatopic/>  ;
	ikos:created "2009-10-22T02:00:00+00:00"^^xsd:dateTime ;
	dct:created "2009-10-22T02:00:00+00:00"^^xsd:dateTime ;
	ikos:modified "2021-09-30T12:00:00+00:00"^^xsd:dateTime ;
	dct:modified "2021-09-30T12:00:00+00:00"^^xsd:dateTime  ;
	skos:exactMatch subj:05005001 ;
	skos:exactMatch <https://www.wikidata.org/entity/Q9842> ;
	skos:broader	medtop:20000400 .

medtop:20000402
	rdf:type skos:Concept ;
	skos:prefLabel	"further education"@en-GB ;
	skos:definition	"Any form of education beyond basic education of several levels"@en-GB ;
	skos:changeNote	"Retired on 2021-09-30T12:00:00+00:00. Use medtop:20000403 adult and continuing education or medtop:20001216 vocational education"@en-GB ;
	skos:inScheme <http://cv.iptc.org/newscodes/mediatopic/>  ;
	ikos:created "2009-10-22T02:00:00+00:00"^^xsd:dateTime ;
	dct:created "2009-10-22T02:00:00+00:00"^^xsd:dateTime ;
	ikos:modified "2021-09-30T12:00:00+00:00"^^xsd:dateTime ;
	dct:modified "2021-09-30T12:00:00+00:00"^^xsd:dateTime  ; 
	ikos:retired "2021-09-30T12:00:00+00:00"^^xsd:dateTime ;
	skos:exactMatch subj:05002000 ;
	skos:exactMatch <https://www.wikidata.org/entity/Q765192> ;
	skos:broader	medtop:20000400 .

medtop:20000403
	rdf:type skos:Concept ;
	skos:prefLabel	"adult and continuing education"@en-GB ;
	skos:definition	"Education for adults who have left the formal education system that offers new forms of knowledge or skills, including professional certificates and online courses provided by companies such as CodeAcademy or Udemy"@en-GB ;
	skos:inScheme <http://cv.iptc.org/newscodes/mediatopic/>  ;
	ikos:created "2009-10-22T02:00:00+00:00"^^xsd:dateTime ;
	dct:created "2009-10-22T02:00:00+00:00"^^xsd:dateTime ;
	ikos:modified "2021-09-30T12:00:00+00:00"^^xsd:dateTime ;
	dct:modified "2021-09-30T12:00:00+00:00"^^xsd:dateTime  ;
	skos:exactMatch subj:05001000 ;
	skos:exactMatch <https://www.wikidata.org/entity/Q1319035> ;
	skos:broader	medtop:20000400 .

medtop:20000404
	rdf:type skos:Concept ;
	skos:prefLabel	"upper secondary education"@en-GB ;
	skos:definition	"Education and schools preparing students for tertiary eduction or providing skills relevant to employment through a curriculum with an increased range of subject options and streams"@en-GB ;
	skos:inScheme <http://cv.iptc.org/newscodes/mediatopic/>  ;
	ikos:created "2009-10-22T02:00:00+00:00"^^xsd:dateTime ;
	dct:created "2009-10-22T02:00:00+00:00"^^xsd:dateTime ;
	ikos:modified "2021-09-30T12:00:00+00:00"^^xsd:dateTime ;
	dct:modified "2021-09-30T12:00:00+00:00"^^xsd:dateTime  ;
	skos:exactMatch subj:05005003 ;
	skos:exactMatch <https://www.wikidata.org/entity/Q9826> ;
	skos:broader	medtop:20000400 .

medtop:20000405
	rdf:type skos:Concept ;
	skos:prefLabel	"college and university"@en-GB ;
	skos:definition	"Institutions of higher learning that provide degrees in a course of study at the undergraduate, postgraduate or doctorate level"@en-GB ;
	skos:inScheme <http://cv.iptc.org/newscodes/mediatopic/>  ;
	ikos:created "2009-10-22T02:00:00+00:00"^^xsd:dateTime ;
	dct:created "2009-10-22T02:00:00+00:00"^^xsd:dateTime ;
	ikos:modified "2021-09-30T12:00:00+00:00"^^xsd:dateTime ;
	dct:modified "2021-09-30T12:00:00+00:00"^^xsd:dateTime  ;
	skos:broadMatch subj:05000000 ;
	skos:exactMatch <https://www.wikidata.org/entity/Q136822> ;
	skos:broader	medtop:20000400 ;
	skos:narrower	medtop:20000406 ;
	skos:narrower	medtop:20000407 .

medtop:20000406
	rdf:type skos:Concept ;
	skos:prefLabel	"college"@en-GB ;
	skos:definition	"Institution of higher learning, its specific scope is set differently in different countries"@en-GB ;
	skos:changeNote	"Retired. Use medtop:20000405 college and university"@en-GB ;
	skos:inScheme <http://cv.iptc.org/newscodes/mediatopic/>  ;
	ikos:created "2009-10-22T02:00:00+00:00"^^xsd:dateTime ;
	dct:created "2009-10-22T02:00:00+00:00"^^xsd:dateTime ;
	ikos:modified "2021-09-30T12:00:00+00:00"^^xsd:dateTime ;
	dct:modified "2021-09-30T12:00:00+00:00"^^xsd:dateTime  ; 
	ikos:retired "2021-09-30T12:00:00+00:00"^^xsd:dateTime ;
	skos:broadMatch subj:05000000 ;
	skos:exactMatch <https://www.wikidata.org/entity/Q189004> ;
	skos:broader	medtop:20000405 .

medtop:20000407
	rdf:type skos:Concept ;
	skos:prefLabel	"university"@en-GB ;
	skos:definition	"Institutions of higher learning capable of providing doctorate degrees"@en-GB ;
	skos:changeNote	"Retired. Use medtop:20000405 college and university"@en-GB ;
	skos:inScheme <http://cv.iptc.org/newscodes/mediatopic/>  ;
	ikos:created "2009-10-22T02:00:00+00:00"^^xsd:dateTime ;
	dct:created "2009-10-22T02:00:00+00:00"^^xsd:dateTime ;
	ikos:modified "2021-09-30T12:00:00+00:00"^^xsd:dateTime ;
	dct:modified "2021-09-30T12:00:00+00:00"^^xsd:dateTime  ; 
	ikos:retired "2021-09-30T12:00:00+00:00"^^xsd:dateTime ;
	skos:exactMatch subj:05007000 ;
	skos:exactMatch <https://www.wikidata.org/entity/Q3918> ;
	skos:broader	medtop:20000405 .

medtop:20000408
	rdf:type skos:Concept ;
	skos:prefLabel	"lower secondary education"@en-GB ;
	skos:definition	"Education and schools that build on primary education with a more subject-oriented curriculum. Schools may be called middle schools or junior highs in the United States."@en-GB ;
	skos:inScheme <http://cv.iptc.org/newscodes/mediatopic/>  ;
	ikos:created "2009-10-22T02:00:00+00:00"^^xsd:dateTime ;
	dct:created "2009-10-22T02:00:00+00:00"^^xsd:dateTime ;
	ikos:modified "2021-09-30T12:00:00+00:00"^^xsd:dateTime ;
	dct:modified "2021-09-30T12:00:00+00:00"^^xsd:dateTime  ;
	skos:exactMatch subj:05005002 ;
	skos:exactMatch <https://www.wikidata.org/entity/Q149566> ;
	skos:broader	medtop:20000400 .

medtop:20000409
	rdf:type skos:Concept ;
	skos:prefLabel	"early childhood education"@en-GB ;
	skos:definition	"Education for children under the national compulsory education age"@en-GB ;
	skos:inScheme <http://cv.iptc.org/newscodes/mediatopic/>  ;
	ikos:created "2009-10-22T02:00:00+00:00"^^xsd:dateTime ;
	dct:created "2009-10-22T02:00:00+00:00"^^xsd:dateTime ;
	ikos:modified "2021-09-30T12:00:00+00:00"^^xsd:dateTime ;
	dct:modified "2021-09-30T12:00:00+00:00"^^xsd:dateTime  ;
	skos:exactMatch subj:05004000 ;
	skos:exactMatch <https://www.wikidata.org/entity/Q1076052> ;
	skos:broader	medtop:20000400 .

medtop:20000410
	rdf:type skos:Concept ;
	skos:prefLabel	"social learning"@en-GB ;
	skos:definition	"The learning of social skills and behaviors through the imitation and observation of others. This can include formal and informal instruction around empathy, emotions and mental health."@en-GB ;
	skos:inScheme <http://cv.iptc.org/newscodes/mediatopic/>  ;
	ikos:created "2009-10-22T02:00:00+00:00"^^xsd:dateTime ;
	dct:created "2009-10-22T02:00:00+00:00"^^xsd:dateTime ;
	ikos:modified "2021-09-30T12:00:00+00:00"^^xsd:dateTime ;
	dct:modified "2021-09-30T12:00:00+00:00"^^xsd:dateTime  ;
	skos:broadMatch subj:05008000 ;
	skos:exactMatch <https://www.wikidata.org/entity/Q2305519> ;
	skos:broader	medtop:05000000 .

medtop:20000411
	rdf:type skos:Concept ;
	skos:prefLabel	"teaching and learning"@en-GB ;
	skos:definition	"Either end of the education equation"@en-GB ;
	skos:changeNote	"Retired. Use more specific terms instead."@en-GB ;
	skos:inScheme <http://cv.iptc.org/newscodes/mediatopic/>  ;
	ikos:created "2009-10-22T02:00:00+00:00"^^xsd:dateTime ;
	dct:created "2009-10-22T02:00:00+00:00"^^xsd:dateTime ;
	ikos:modified "2021-09-30T12:00:00+00:00"^^xsd:dateTime ;
	dct:modified "2021-09-30T12:00:00+00:00"^^xsd:dateTime  ; 
	ikos:retired "2021-09-30T12:00:00+00:00"^^xsd:dateTime ;
	skos:exactMatch subj:05010000 ;
	skos:exactMatch <https://www.wikidata.org/entity/Q8434> ;
	skos:broader	medtop:05000000 .

medtop:20000412
	rdf:type skos:Concept ;
	skos:prefLabel	"curriculum"@en-GB ;
	skos:definition	"The courses offered by a learning institution and the regulation of those courses"@en-GB ;
	skos:inScheme <http://cv.iptc.org/newscodes/mediatopic/>  ;
	ikos:created "2009-10-22T02:00:00+00:00"^^xsd:dateTime ;
	dct:created "2009-10-22T02:00:00+00:00"^^xsd:dateTime ;
	ikos:modified "2021-09-30T12:00:00+00:00"^^xsd:dateTime ;
	dct:modified "2021-09-30T12:00:00+00:00"^^xsd:dateTime  ;
	skos:exactMatch subj:05010003 ;
	skos:exactMatch <https://www.wikidata.org/entity/Q207137> ;
	skos:broader	medtop:05000000 .

medtop:20000413
	rdf:type skos:Concept ;
	skos:prefLabel	"educational testing and examinations"@en-GB ;
	skos:definition	"Polices and standards around the testing and assessment of students, including the merits of standardised testing, and testing methods"@en-GB ;
	skos:inScheme <http://cv.iptc.org/newscodes/mediatopic/>  ;
	ikos:created "2009-10-22T02:00:00+00:00"^^xsd:dateTime ;
	dct:created "2009-10-22T02:00:00+00:00"^^xsd:dateTime ;
	ikos:modified "2021-09-30T12:00:00+00:00"^^xsd:dateTime ;
	dct:modified "2021-09-30T12:00:00+00:00"^^xsd:dateTime  ;
	skos:broadMatch subj:05010004 ;
	skos:exactMatch <https://www.wikidata.org/entity/Q27318> ;
	skos:broader	medtop:05000000 .

medtop:20000414
	rdf:type skos:Concept ;
	skos:prefLabel	"entrance examination"@en-GB ;
	skos:definition	"Exams for entering colleges, universities and all other higher and lower education institutions"@en-GB ;
	skos:inScheme <http://cv.iptc.org/newscodes/mediatopic/>  ;
	ikos:created "2009-10-22T02:00:00+00:00"^^xsd:dateTime ;
	dct:created "2009-10-22T02:00:00+00:00"^^xsd:dateTime ;
	ikos:modified "2021-09-30T12:00:00+00:00"^^xsd:dateTime ;
	dct:modified "2021-09-30T12:00:00+00:00"^^xsd:dateTime  ;
	skos:exactMatch subj:05009000 ;
	skos:exactMatch <https://www.wikidata.org/entity/Q759860> ;
	skos:broader	medtop:05000000 .

medtop:20000415
	rdf:type skos:Concept ;
	skos:prefLabel	"students"@en-GB ;
	skos:definition	"Students as a demographic, including student protests and requests for change and trends among students"@en-GB ;
	skos:inScheme <http://cv.iptc.org/newscodes/mediatopic/>  ;
	ikos:created "2009-10-22T02:00:00+00:00"^^xsd:dateTime ;
	dct:created "2009-10-22T02:00:00+00:00"^^xsd:dateTime ;
	ikos:modified "2021-09-30T12:00:00+00:00"^^xsd:dateTime ;
	dct:modified "2021-09-30T12:00:00+00:00"^^xsd:dateTime  ;
	skos:exactMatch subj:05010001 ;
	skos:exactMatch <https://www.wikidata.org/entity/Q48282> ;
	skos:broader	medtop:05000000 .

medtop:20000416
	rdf:type skos:Concept ;
	skos:prefLabel	"teachers"@en-GB ;
	skos:definition	"Teachers as a demographic, including teacher unions, teacher education and training and the criteria for teachers in various locations"@en-GB ;
	skos:inScheme <http://cv.iptc.org/newscodes/mediatopic/>  ;
	ikos:created "2009-10-22T02:00:00+00:00"^^xsd:dateTime ;
	dct:created "2009-10-22T02:00:00+00:00"^^xsd:dateTime ;
	ikos:modified "2021-09-30T12:00:00+00:00"^^xsd:dateTime ;
	dct:modified "2021-09-30T12:00:00+00:00"^^xsd:dateTime  ;
	skos:exactMatch subj:05010002 ;
	skos:exactMatch <https://www.wikidata.org/entity/Q37226> ;
	skos:broader	medtop:05000000 .

medtop:20000418
	rdf:type skos:Concept ;
	skos:prefLabel	"climate change"@en-GB ;
	skos:definition	"Significant change in measures of climate (such as temperature, precipitation, or wind) lasting for an extended period"@en-GB ;
	skos:inScheme <http://cv.iptc.org/newscodes/mediatopic/>  ;
	ikos:created "2009-10-22T02:00:00+00:00"^^xsd:dateTime ;
	dct:created "2009-10-22T02:00:00+00:00"^^xsd:dateTime ;
	ikos:modified "2021-02-18T12:00:00+00:00"^^xsd:dateTime ;
	dct:modified "2021-02-18T12:00:00+00:00"^^xsd:dateTime  ;
	skos:exactMatch <https://www.wikidata.org/entity/Q125928> ;
	skos:exactMatch subj:17002000 ;
	skos:broader	medtop:06000000 ;
	skos:narrower	medtop:20000419 .

medtop:20000419
	rdf:type skos:Concept ;
	skos:prefLabel	"global warming"@en-GB ;
	skos:definition	"This category includes all issues relating to global warming including temperature research, remote sensing on temperature trends, debate on global warming, ways to reduce emissions and carbon trading."@en-GB ;
	skos:inScheme <http://cv.iptc.org/newscodes/mediatopic/>  ;
	ikos:created "2009-10-22T02:00:00+00:00"^^xsd:dateTime ;
	dct:created "2009-10-22T02:00:00+00:00"^^xsd:dateTime ;
	ikos:modified "2021-02-18T12:00:00+00:00"^^xsd:dateTime ;
	dct:modified "2021-02-18T12:00:00+00:00"^^xsd:dateTime  ;
	skos:exactMatch subj:06011000 ;
	skos:exactMatch <https://www.wikidata.org/entity/Q7942> ;
	skos:broader	medtop:20000418 .

medtop:20000420
	rdf:type skos:Concept ;
	skos:prefLabel	"conservation"@en-GB ;
	skos:definition	"Preservation of wilderness areas, flora and fauna, including species extinction"@en-GB ;
	skos:inScheme <http://cv.iptc.org/newscodes/mediatopic/>  ;
	ikos:created "2009-10-22T02:00:00+00:00"^^xsd:dateTime ;
	dct:created "2009-10-22T02:00:00+00:00"^^xsd:dateTime ;
	ikos:modified "2021-02-18T12:00:00+00:00"^^xsd:dateTime ;
	dct:modified "2021-02-18T12:00:00+00:00"^^xsd:dateTime  ;
	skos:exactMatch subj:06002000 ;
	skos:exactMatch <https://www.wikidata.org/entity/Q628403> ;
	skos:broader	medtop:06000000 ;
	skos:narrower	medtop:20000421 ;
	skos:narrower	medtop:20000422 .

medtop:20000421
	rdf:type skos:Concept ;
	skos:prefLabel	"energy saving"@en-GB ;
	skos:definition	"Conservation of electrical, and other power sources"@en-GB ;
	skos:inScheme <http://cv.iptc.org/newscodes/mediatopic/>  ;
	ikos:created "2009-10-22T02:00:00+00:00"^^xsd:dateTime ;
	dct:created "2009-10-22T02:00:00+00:00"^^xsd:dateTime ;
	ikos:modified "2021-07-12T12:00:00+00:00"^^xsd:dateTime ;
	dct:modified "2021-07-12T12:00:00+00:00"^^xsd:dateTime  ;
	skos:exactMatch subj:06003000 ;
	skos:exactMatch <https://www.wikidata.org/entity/Q380170> ;
	skos:broader	medtop:20000420 .

medtop:20000422
	rdf:type skos:Concept ;
	skos:prefLabel	"parks"@en-GB ;
	skos:definition	"Areas set aside for preservation"@en-GB ;
	skos:inScheme <http://cv.iptc.org/newscodes/mediatopic/>  ;
	ikos:created "2009-10-22T02:00:00+00:00"^^xsd:dateTime ;
	dct:created "2009-10-22T02:00:00+00:00"^^xsd:dateTime ;
	ikos:modified "2021-02-18T12:00:00+00:00"^^xsd:dateTime ;
	dct:modified "2021-02-18T12:00:00+00:00"^^xsd:dateTime  ;
	skos:closeMatch subj:06002000 ;
	skos:exactMatch <https://www.wikidata.org/entity/Q22698> ;
	skos:broader	medtop:20000420 .

medtop:20000423
	rdf:type skos:Concept ;
	skos:prefLabel	"environmental policy"@en-GB ;
	skos:definition	"Government programs and policies related to the environment and proposals to change or protests against those positions"@en-GB ;
	skos:inScheme <http://cv.iptc.org/newscodes/mediatopic/>  ;
	ikos:created "2009-10-22T02:00:00+00:00"^^xsd:dateTime ;
	dct:created "2009-10-22T02:00:00+00:00"^^xsd:dateTime ;
	ikos:modified "2021-12-21T12:00:00+00:00"^^xsd:dateTime ;
	dct:modified "2021-12-21T12:00:00+00:00"^^xsd:dateTime  ;
	skos:exactMatch subj:06004000 ;
	skos:exactMatch <https://www.wikidata.org/entity/Q5381346> ;
	skos:broader	medtop:20000621 .

medtop:20000424
	rdf:type skos:Concept ;
	skos:prefLabel	"environmental pollution"@en-GB ;
	skos:definition	"Corruption of air, water, land etc. by harmful substances"@en-GB ;
	skos:inScheme <http://cv.iptc.org/newscodes/mediatopic/>  ;
	ikos:created "2009-10-22T02:00:00+00:00"^^xsd:dateTime ;
	dct:created "2009-10-22T02:00:00+00:00"^^xsd:dateTime ;
	ikos:modified "2021-02-18T12:00:00+00:00"^^xsd:dateTime ;
	dct:modified "2021-02-18T12:00:00+00:00"^^xsd:dateTime  ;
	skos:exactMatch subj:06005000 ;
	skos:exactMatch <https://www.wikidata.org/entity/Q58734> ;
	skos:broader	medtop:06000000 ;
	skos:narrower	medtop:20000425 ;
	skos:narrower	medtop:20000426 ;
	skos:narrower	medtop:20000427 ;
	skos:narrower	medtop:20000428 ;
	skos:narrower	medtop:20000429 .

medtop:20000425
	rdf:type skos:Concept ;
	skos:prefLabel	"air pollution"@en-GB ;
	skos:definition	"Solid or gaseous matter affecting the quality of air that we breathe"@en-GB ;
	skos:inScheme <http://cv.iptc.org/newscodes/mediatopic/>  ;
	ikos:created "2009-10-22T02:00:00+00:00"^^xsd:dateTime ;
	dct:created "2009-10-22T02:00:00+00:00"^^xsd:dateTime ;
	ikos:modified "2021-02-18T12:00:00+00:00"^^xsd:dateTime ;
	dct:modified "2021-02-18T12:00:00+00:00"^^xsd:dateTime  ;
	skos:exactMatch subj:06005001 ;
	skos:exactMatch <https://www.wikidata.org/entity/Q131123> ;
	skos:broader	medtop:20000424 .

medtop:20000426
	rdf:type skos:Concept ;
	skos:prefLabel	"environmental clean-up"@en-GB ;
	skos:definition	"Processes whereby contaminated areas are cleaned of hazardous materials so they can be inhabited again by either people or animals."@en-GB ;
	skos:inScheme <http://cv.iptc.org/newscodes/mediatopic/>  ;
	ikos:created "2009-10-22T02:00:00+00:00"^^xsd:dateTime ;
	dct:created "2009-10-22T02:00:00+00:00"^^xsd:dateTime ;
	ikos:modified "2021-05-05T12:00:00+00:00"^^xsd:dateTime ;
	dct:modified "2021-05-05T12:00:00+00:00"^^xsd:dateTime  ;
	skos:exactMatch subj:06013000 ;
	skos:exactMatch <https://www.wikidata.org/entity/Q2019586> ;
	skos:broader	medtop:20000424 .

medtop:20000427
	rdf:type skos:Concept ;
	skos:prefLabel	"hazardous materials"@en-GB ;
	skos:definition	"Materials that are harmful to humans or animals if they are exposed to them. Includes radiation, poison gases, chemicals, heavy metals, PCBs, and certain plant products"@en-GB ;
	skos:inScheme <http://cv.iptc.org/newscodes/mediatopic/>  ;
	ikos:created "2009-10-22T02:00:00+00:00"^^xsd:dateTime ;
	dct:created "2009-10-22T02:00:00+00:00"^^xsd:dateTime ;
	ikos:modified "2021-02-18T12:00:00+00:00"^^xsd:dateTime ;
	dct:modified "2021-02-18T12:00:00+00:00"^^xsd:dateTime  ;
	skos:exactMatch subj:06012000 ;
	skos:exactMatch <https://www.wikidata.org/entity/Q757138> ;
	skos:broader	medtop:20000424 .

medtop:20000428
	rdf:type skos:Concept ;
	skos:prefLabel	"waste materials"@en-GB ;
	skos:definition	"The environmental impact of waste, including recycling efforts"@en-GB ;
	skos:inScheme <http://cv.iptc.org/newscodes/mediatopic/>  ;
	ikos:created "2009-10-22T02:00:00+00:00"^^xsd:dateTime ;
	dct:created "2009-10-22T02:00:00+00:00"^^xsd:dateTime ;
	ikos:modified "2021-02-18T12:00:00+00:00"^^xsd:dateTime ;
	dct:modified "2021-02-18T12:00:00+00:00"^^xsd:dateTime  ;
	skos:exactMatch subj:06009000 ;
	skos:exactMatch <https://www.wikidata.org/entity/Q45701> ;
	skos:broader	medtop:20000424 .

medtop:20000429
	rdf:type skos:Concept ;
	skos:prefLabel	"water pollution"@en-GB ;
	skos:definition	"Solids or liquids that corrupt the quality of water that could be used for drinking or irrigation"@en-GB ;
	skos:inScheme <http://cv.iptc.org/newscodes/mediatopic/>  ;
	ikos:created "2009-10-22T02:00:00+00:00"^^xsd:dateTime ;
	dct:created "2009-10-22T02:00:00+00:00"^^xsd:dateTime ;
	ikos:modified "2021-02-18T12:00:00+00:00"^^xsd:dateTime ;
	dct:modified "2021-02-18T12:00:00+00:00"^^xsd:dateTime  ;
	skos:exactMatch subj:06005002 ;
	skos:exactMatch <https://www.wikidata.org/entity/Q183129> ;
	skos:broader	medtop:20000424 .

medtop:20000430
	rdf:type skos:Concept ;
	skos:prefLabel	"natural resources"@en-GB ;
	skos:definition	"Environmental issues related to the exploitation of natural resources"@en-GB ;
	skos:inScheme <http://cv.iptc.org/newscodes/mediatopic/>  ;
	ikos:created "2009-10-22T02:00:00+00:00"^^xsd:dateTime ;
	dct:created "2009-10-22T02:00:00+00:00"^^xsd:dateTime ;
	ikos:modified "2021-02-18T12:00:00+00:00"^^xsd:dateTime ;
	dct:modified "2021-02-18T12:00:00+00:00"^^xsd:dateTime  ;
	skos:exactMatch subj:06006000 ;
	skos:exactMatch <https://www.wikidata.org/entity/Q188460> ;
	skos:broader	medtop:06000000 ;
	skos:narrower	medtop:20000431 ;
	skos:narrower	medtop:20000432 ;
	skos:narrower	medtop:20000435 ;
	skos:narrower	medtop:20000436 ;
	skos:narrower	medtop:20000437 .

medtop:20000431
	rdf:type skos:Concept ;
	skos:prefLabel	"energy resources"@en-GB ;
	skos:definition	"Such resources as coal, gas, wind, sunlight etc., used to generate heat, electricity and power"@en-GB ;
	skos:inScheme <http://cv.iptc.org/newscodes/mediatopic/>  ;
	ikos:created "2009-10-22T02:00:00+00:00"^^xsd:dateTime ;
	dct:created "2009-10-22T02:00:00+00:00"^^xsd:dateTime ;
	ikos:modified "2021-07-12T12:00:00+00:00"^^xsd:dateTime ;
	dct:modified "2021-07-12T12:00:00+00:00"^^xsd:dateTime  ;
	skos:exactMatch subj:06006009 ;
	skos:exactMatch <https://www.wikidata.org/entity/Q1522115> ;
	skos:broader	medtop:20000430 .

medtop:20000432
	rdf:type skos:Concept ;
	skos:prefLabel	"land resources"@en-GB ;
	skos:definition	"That portion of a nation or state that is above water and available for development either for profit or for the general good of the public"@en-GB ;
	skos:inScheme <http://cv.iptc.org/newscodes/mediatopic/>  ;
	ikos:created "2009-10-22T02:00:00+00:00"^^xsd:dateTime ;
	dct:created "2009-10-22T02:00:00+00:00"^^xsd:dateTime ;
	ikos:modified "2021-02-18T12:00:00+00:00"^^xsd:dateTime ;
	dct:modified "2021-02-18T12:00:00+00:00"^^xsd:dateTime  ;
	skos:exactMatch subj:06006001 ;
	skos:exactMatch <https://www.wikidata.org/entity/Q55725874> ;
	skos:broader	medtop:20000430 ;
	skos:narrower	medtop:20000433 ;
	skos:narrower	medtop:20000434 .

medtop:20000433
	rdf:type skos:Concept ;
	skos:prefLabel	"forests"@en-GB ;
	skos:definition	"Open areas of trees either available for public enjoyment, or for commercial purposes"@en-GB ;
	skos:inScheme <http://cv.iptc.org/newscodes/mediatopic/>  ;
	ikos:created "2009-10-22T02:00:00+00:00"^^xsd:dateTime ;
	dct:created "2009-10-22T02:00:00+00:00"^^xsd:dateTime ;
	ikos:modified "2021-02-18T12:00:00+00:00"^^xsd:dateTime ;
	dct:modified "2021-02-18T12:00:00+00:00"^^xsd:dateTime  ;
	skos:exactMatch subj:06006003 ;
	skos:exactMatch <https://www.wikidata.org/entity/Q4421> ;
	skos:broader	medtop:20000432 .

medtop:20000434
	rdf:type skos:Concept ;
	skos:prefLabel	"mountains"@en-GB ;
	skos:definition	"Elevated land masses formed over the ages either by erosion, volcanic eruption, or movement of massive geographical formations called plates"@en-GB ;
	skos:inScheme <http://cv.iptc.org/newscodes/mediatopic/>  ;
	ikos:created "2009-10-22T02:00:00+00:00"^^xsd:dateTime ;
	dct:created "2009-10-22T02:00:00+00:00"^^xsd:dateTime ;
	ikos:modified "2021-02-18T12:00:00+00:00"^^xsd:dateTime ;
	dct:modified "2021-02-18T12:00:00+00:00"^^xsd:dateTime  ;
	skos:exactMatch subj:06006005 ;
	skos:exactMatch <https://www.wikidata.org/entity/Q8502> ;
	skos:broader	medtop:20000432 .

medtop:20000435
	rdf:type skos:Concept ;
	skos:prefLabel	"population growth"@en-GB ;
	skos:definition	"People and their growth and development within a natural setting"@en-GB ;
	skos:inScheme <http://cv.iptc.org/newscodes/mediatopic/>  ;
	ikos:created "2009-10-22T02:00:00+00:00"^^xsd:dateTime ;
	dct:created "2009-10-22T02:00:00+00:00"^^xsd:dateTime ;
	ikos:modified "2021-02-18T12:00:00+00:00"^^xsd:dateTime ;
	dct:modified "2021-02-18T12:00:00+00:00"^^xsd:dateTime  ;
	skos:exactMatch subj:06008000 ;
	skos:exactMatch <https://www.wikidata.org/entity/Q386191> ;
	skos:broader	medtop:20000430 .

medtop:20000436
	rdf:type skos:Concept ;
	skos:prefLabel	"renewable energy"@en-GB ;
	skos:definition	"The environmental impact of renewable energy, including solar, wind, hydro, biomass and geothermal"@en-GB ;
	skos:changeNote	"Retired. Use medtop:20000431 energy resources for environmental impacts or medtop:20000257 renewable energy for the general concept."@en-GB ;
	skos:inScheme <http://cv.iptc.org/newscodes/mediatopic/>  ;
	ikos:created "2009-10-22T02:00:00+00:00"^^xsd:dateTime ;
	dct:created "2009-10-22T02:00:00+00:00"^^xsd:dateTime ;
	ikos:modified "2023-03-31T12:00:00+00:00"^^xsd:dateTime ;
	dct:modified "2023-03-31T12:00:00+00:00"^^xsd:dateTime  ; 
	ikos:retired "2023-03-31T12:00:00+00:00"^^xsd:dateTime ;
	skos:exactMatch subj:06001000 ;
	skos:exactMatch <https://www.wikidata.org/entity/Q12705> ;
	skos:broader	medtop:20000430 .

medtop:20000437
	rdf:type skos:Concept ;
	skos:prefLabel	"water"@en-GB ;
	skos:definition	"Environmental issues about bodies of water, including oceans, lakes, streams and reservoirs, as well as ice, glaciers and forms of precipitation"@en-GB ;
	skos:inScheme <http://cv.iptc.org/newscodes/mediatopic/>  ;
	ikos:created "2009-10-22T02:00:00+00:00"^^xsd:dateTime ;
	dct:created "2009-10-22T02:00:00+00:00"^^xsd:dateTime ;
	ikos:modified "2021-02-18T12:00:00+00:00"^^xsd:dateTime ;
	dct:modified "2021-02-18T12:00:00+00:00"^^xsd:dateTime  ;
	skos:exactMatch subj:06010000 ;
	skos:exactMatch <https://www.wikidata.org/entity/Q283> ;
	skos:broader	medtop:20000430 ;
	skos:narrower	medtop:20000438 ;
	skos:narrower	medtop:20000439 ;
	skos:narrower	medtop:20000440 .

medtop:20000438
	rdf:type skos:Concept ;
	skos:prefLabel	"oceans"@en-GB ;
	skos:definition	"Salt water masses separating continents or other major geographical masses. smaller forms are seas or lakes or ponds"@en-GB ;
	skos:inScheme <http://cv.iptc.org/newscodes/mediatopic/>  ;
	ikos:created "2009-10-22T02:00:00+00:00"^^xsd:dateTime ;
	dct:created "2009-10-22T02:00:00+00:00"^^xsd:dateTime ;
	ikos:modified "2021-02-18T12:00:00+00:00"^^xsd:dateTime ;
	dct:modified "2021-02-18T12:00:00+00:00"^^xsd:dateTime  ;
	skos:exactMatch subj:06006007 ;
	skos:exactMatch <https://www.wikidata.org/entity/Q9430> ;
	skos:broader	medtop:20000437 .

medtop:20000439
	rdf:type skos:Concept ;
	skos:prefLabel	"rivers"@en-GB ;
	skos:definition	"Moving water areas bounded by land that extend from earth sources and meander through land areas to join with other water areas. In smaller forms they are creeks, rivulets, streams etc"@en-GB ;
	skos:inScheme <http://cv.iptc.org/newscodes/mediatopic/>  ;
	ikos:created "2009-10-22T02:00:00+00:00"^^xsd:dateTime ;
	dct:created "2009-10-22T02:00:00+00:00"^^xsd:dateTime ;
	ikos:modified "2021-02-18T12:00:00+00:00"^^xsd:dateTime ;
	dct:modified "2021-02-18T12:00:00+00:00"^^xsd:dateTime  ;
	skos:exactMatch subj:06006006 ;
	skos:exactMatch <https://www.wikidata.org/entity/Q4022> ;
	skos:broader	medtop:20000437 .

medtop:20000440
	rdf:type skos:Concept ;
	skos:prefLabel	"wetlands"@en-GB ;
	skos:definition	"Areas generally marshy and not either under water or dry land. Often related to aquifers for water quality and/or wildlife"@en-GB ;
	skos:inScheme <http://cv.iptc.org/newscodes/mediatopic/>  ;
	ikos:created "2009-10-22T02:00:00+00:00"^^xsd:dateTime ;
	dct:created "2009-10-22T02:00:00+00:00"^^xsd:dateTime ;
	ikos:modified "2021-02-18T12:00:00+00:00"^^xsd:dateTime ;
	dct:modified "2021-02-18T12:00:00+00:00"^^xsd:dateTime  ;
	skos:exactMatch subj:06006004 ;
	skos:exactMatch <https://www.wikidata.org/entity/Q170321> ;
	skos:broader	medtop:20000437 .

medtop:20000441
	rdf:type skos:Concept ;
	skos:prefLabel	"nature"@en-GB ;
	skos:definition	"The natural world in its entirety"@en-GB ;
	skos:inScheme <http://cv.iptc.org/newscodes/mediatopic/>  ;
	ikos:created "2009-10-22T02:00:00+00:00"^^xsd:dateTime ;
	dct:created "2009-10-22T02:00:00+00:00"^^xsd:dateTime ;
	ikos:modified "2021-02-18T12:00:00+00:00"^^xsd:dateTime ;
	dct:modified "2021-02-18T12:00:00+00:00"^^xsd:dateTime  ;
	skos:exactMatch <https://www.wikidata.org/entity/Q7860> ;
	skos:closeMatch subj:06007000 ;
	skos:broader	medtop:06000000 ;
	skos:narrower	medtop:20000442 ;
	skos:narrower	medtop:20000443 ;
	skos:narrower	medtop:20000444 ;
	skos:narrower	medtop:20000500 ;
	skos:narrower	medtop:20000507 .

medtop:20000442
	rdf:type skos:Concept ;
	skos:prefLabel	"ecosystem"@en-GB ;
	skos:definition	"A system of plants, animals and bacteria interrelated in its physical/chemical environment"@en-GB ;
	skos:inScheme <http://cv.iptc.org/newscodes/mediatopic/>  ;
	ikos:created "2009-10-22T02:00:00+00:00"^^xsd:dateTime ;
	dct:created "2009-10-22T02:00:00+00:00"^^xsd:dateTime ;
	ikos:modified "2021-07-12T12:00:00+00:00"^^xsd:dateTime ;
	dct:modified "2021-07-12T12:00:00+00:00"^^xsd:dateTime  ;
	skos:exactMatch subj:06002002 ;
	skos:exactMatch <https://www.wikidata.org/entity/Q37813> ;
	skos:broader	medtop:20000441 .

medtop:20000443
	rdf:type skos:Concept ;
	skos:prefLabel	"endangered species"@en-GB ;
	skos:definition	"Those species in danger of disappearing, largely because of changes in environment, hunting, or weather"@en-GB ;
	skos:inScheme <http://cv.iptc.org/newscodes/mediatopic/>  ;
	ikos:created "2009-10-22T02:00:00+00:00"^^xsd:dateTime ;
	dct:created "2009-10-22T02:00:00+00:00"^^xsd:dateTime ;
	ikos:modified "2021-02-18T12:00:00+00:00"^^xsd:dateTime ;
	dct:modified "2021-02-18T12:00:00+00:00"^^xsd:dateTime  ;
	skos:exactMatch subj:06002001 ;
	skos:exactMatch <https://www.wikidata.org/entity/Q11394> ;
	skos:broader	medtop:20000441 .

medtop:20000444
	rdf:type skos:Concept ;
	skos:prefLabel	"invasive species"@en-GB ;
	skos:definition	"Non-native plants, animals and other organisms that tend to take over native species"@en-GB ;
	skos:inScheme <http://cv.iptc.org/newscodes/mediatopic/>  ;
	ikos:created "2009-10-22T02:00:00+00:00"^^xsd:dateTime ;
	dct:created "2009-10-22T02:00:00+00:00"^^xsd:dateTime ;
	ikos:modified "2021-02-18T12:00:00+00:00"^^xsd:dateTime ;
	dct:modified "2021-02-18T12:00:00+00:00"^^xsd:dateTime  ;
	skos:exactMatch subj:06007001 ;
	skos:exactMatch <https://www.wikidata.org/entity/Q183368> ;
	skos:broader	medtop:20000441 .

medtop:20000446
	rdf:type skos:Concept ;
	skos:prefLabel	"disease and condition"@en-GB ;
	skos:definition	"Any health conditions affecting humans"@en-GB ;
	skos:inScheme <http://cv.iptc.org/newscodes/mediatopic/>  ;
	ikos:created "2009-10-22T02:00:00+00:00"^^xsd:dateTime ;
	dct:created "2009-10-22T02:00:00+00:00"^^xsd:dateTime ;
	ikos:modified "2022-06-14T12:00:00+00:00"^^xsd:dateTime ;
	dct:modified "2022-06-14T12:00:00+00:00"^^xsd:dateTime  ;
	skos:broadMatch subj:07001000 ;
	skos:exactMatch <https://www.wikidata.org/entity/Q12136> ;
	skos:broader	medtop:07000000 ;
	skos:narrower	medtop:20000447 ;
	skos:narrower	medtop:20000448 ;
	skos:narrower	medtop:20000454 ;
	skos:narrower	medtop:20000455 ;
	skos:narrower	medtop:20000456 ;
	skos:narrower	medtop:20000457 ;
	skos:narrower	medtop:20000458 ;
	skos:narrower	medtop:20001322 ;
	skos:narrower	medtop:20001355 .

medtop:20000447
	rdf:type skos:Concept ;
	skos:prefLabel	"cancer"@en-GB ;
	skos:definition	"A serious and often fatal disease caused when normal cells mutate into tumours"@en-GB ;
	skos:inScheme <http://cv.iptc.org/newscodes/mediatopic/>  ;
	ikos:created "2009-10-22T02:00:00+00:00"^^xsd:dateTime ;
	dct:created "2009-10-22T02:00:00+00:00"^^xsd:dateTime ;
	ikos:modified "2021-02-18T12:00:00+00:00"^^xsd:dateTime ;
	dct:modified "2021-02-18T12:00:00+00:00"^^xsd:dateTime  ;
	skos:exactMatch subj:07001004 ;
	skos:exactMatch <https://www.wikidata.org/entity/Q12078> ;
	skos:broader	medtop:20000446 .

medtop:20000448
	rdf:type skos:Concept ;
	skos:prefLabel	"communicable disease"@en-GB ;
	skos:definition	"Diseases that can be transmitted from one person or animal to another"@en-GB ;
	skos:inScheme <http://cv.iptc.org/newscodes/mediatopic/>  ;
	ikos:created "2009-10-22T02:00:00+00:00"^^xsd:dateTime ;
	dct:created "2009-10-22T02:00:00+00:00"^^xsd:dateTime ;
	ikos:modified "2021-02-18T12:00:00+00:00"^^xsd:dateTime ;
	dct:modified "2021-02-18T12:00:00+00:00"^^xsd:dateTime  ;
	skos:exactMatch subj:07001001 ;
	skos:exactMatch <https://www.wikidata.org/entity/Q18123741> ;
	skos:broader	medtop:20000446 ;
	skos:narrower	medtop:20000449 ;
	skos:narrower	medtop:20000451 .

medtop:20000449
	rdf:type skos:Concept ;
	skos:prefLabel	"epidemic and pandemic"@en-GB ;
	skos:definition	"A disease that affects a large number of people within a community, population, region or that has spread to multiple countries or continents across the world"@en-GB ;
	skos:inScheme <http://cv.iptc.org/newscodes/mediatopic/>  ;
	ikos:created "2009-10-22T02:00:00+00:00"^^xsd:dateTime ;
	dct:created "2009-10-22T02:00:00+00:00"^^xsd:dateTime ;
	ikos:modified "2022-06-14T12:00:00+00:00"^^xsd:dateTime ;
	dct:modified "2022-06-14T12:00:00+00:00"^^xsd:dateTime  ;
	skos:broadMatch subj:07002000 ;
	skos:exactMatch <https://www.wikidata.org/entity/Q44512> ;
	skos:broader	medtop:20000448 ;
	skos:narrower	medtop:20000450 ;
	skos:narrower	medtop:20001218 .

medtop:20000450
	rdf:type skos:Concept ;
	skos:prefLabel	"plague (disease)"@en-GB ;
	skos:definition	"A highly infectious epidemic disease caused by the Yersinia pestis bacteria"@en-GB ;
	skos:changeNote	"Retired. Use medtop:20000449 epidemic and pandemic instead."@en-GB ;
	skos:inScheme <http://cv.iptc.org/newscodes/mediatopic/>  ;
	ikos:created "2009-10-22T02:00:00+00:00"^^xsd:dateTime ;
	dct:created "2009-10-22T02:00:00+00:00"^^xsd:dateTime ;
	ikos:modified "2022-06-14T12:00:00+00:00"^^xsd:dateTime ;
	dct:modified "2022-06-14T12:00:00+00:00"^^xsd:dateTime  ; 
	ikos:retired "2022-06-14T12:00:00+00:00"^^xsd:dateTime ;
	skos:broadMatch subj:07002000 ;
	skos:exactMatch <https://www.wikidata.org/entity/Q133780> ;
	skos:broader	medtop:20000449 .

medtop:20000451
	rdf:type skos:Concept ;
	skos:prefLabel	"viral disease"@en-GB ;
	skos:definition	"Diseases caused by an infection by viruses"@en-GB ;
	skos:inScheme <http://cv.iptc.org/newscodes/mediatopic/>  ;
	ikos:created "2009-10-22T02:00:00+00:00"^^xsd:dateTime ;
	dct:created "2009-10-22T02:00:00+00:00"^^xsd:dateTime ;
	ikos:modified "2022-06-14T12:00:00+00:00"^^xsd:dateTime ;
	dct:modified "2022-06-14T12:00:00+00:00"^^xsd:dateTime  ;
	skos:exactMatch subj:07001002 ;
	skos:exactMatch <https://www.wikidata.org/entity/Q1928978> ;
	skos:broader	medtop:20000448 ;
	skos:narrower	medtop:20000452 ;
	skos:narrower	medtop:20000453 .

medtop:20000452
	rdf:type skos:Concept ;
	skos:prefLabel	"HIV and AIDS"@en-GB ;
	skos:definition	"HIV, a virus that attacks the body's immune system, and AIDS the disease caused by HIV"@en-GB ;
	skos:inScheme <http://cv.iptc.org/newscodes/mediatopic/>  ;
	ikos:created "2009-10-22T02:00:00+00:00"^^xsd:dateTime ;
	dct:created "2009-10-22T02:00:00+00:00"^^xsd:dateTime ;
	ikos:modified "2022-06-14T12:00:00+00:00"^^xsd:dateTime ;
	dct:modified "2022-06-14T12:00:00+00:00"^^xsd:dateTime  ;
	skos:exactMatch subj:07001003 ;
	skos:exactMatch <https://www.wikidata.org/entity/Q12199> ;
	skos:broader	medtop:20000451 .

medtop:20000453
	rdf:type skos:Concept ;
	skos:prefLabel	"retrovirus"@en-GB ;
	skos:definition	"A family of RNA viruses such as those causing leukaemia and AIDS"@en-GB ;
	skos:changeNote	"Retired. Use a more specific term or medtop:20000446 disease and condition instead."@en-GB ;
	skos:inScheme <http://cv.iptc.org/newscodes/mediatopic/>  ;
	ikos:created "2009-10-22T02:00:00+00:00"^^xsd:dateTime ;
	dct:created "2009-10-22T02:00:00+00:00"^^xsd:dateTime ;
	ikos:modified "2022-06-14T12:00:00+00:00"^^xsd:dateTime ;
	dct:modified "2022-06-14T12:00:00+00:00"^^xsd:dateTime  ; 
	ikos:retired "2022-06-14T12:00:00+00:00"^^xsd:dateTime ;
	skos:exactMatch subj:07001009 ;
	skos:exactMatch <https://www.wikidata.org/entity/Q189308> ;
	skos:broader	medtop:20000451 .

medtop:20000454
	rdf:type skos:Concept ;
	skos:prefLabel	"heart disease"@en-GB ;
	skos:definition	"Diseases and conditions affecting the heart such as heart attacks, the narrowing of arteries, arrhythmia or cardiomyopathy"@en-GB ;
	skos:inScheme <http://cv.iptc.org/newscodes/mediatopic/>  ;
	ikos:created "2009-10-22T02:00:00+00:00"^^xsd:dateTime ;
	dct:created "2009-10-22T02:00:00+00:00"^^xsd:dateTime ;
	ikos:modified "2022-06-14T12:00:00+00:00"^^xsd:dateTime ;
	dct:modified "2022-06-14T12:00:00+00:00"^^xsd:dateTime  ;
	skos:exactMatch subj:07001005 ;
	skos:exactMatch <https://www.wikidata.org/entity/Q190805> ;
	skos:broader	medtop:20000446 .

medtop:20000455
	rdf:type skos:Concept ;
	skos:prefLabel	"illness"@en-GB ;
	skos:definition	"Non-specific maladies such as stomach aches, headaches, flat feet, lumbago"@en-GB ;
	skos:changeNote	"Retired. Use a more specific term or medtop:20000446 disease and condition instead."@en-GB ;
	skos:inScheme <http://cv.iptc.org/newscodes/mediatopic/>  ;
	ikos:created "2009-10-22T02:00:00+00:00"^^xsd:dateTime ;
	dct:created "2009-10-22T02:00:00+00:00"^^xsd:dateTime ;
	ikos:modified "2022-06-14T12:00:00+00:00"^^xsd:dateTime ;
	dct:modified "2022-06-14T12:00:00+00:00"^^xsd:dateTime  ; 
	ikos:retired "2022-06-14T12:00:00+00:00"^^xsd:dateTime ;
	skos:exactMatch subj:07017000 ;
	skos:exactMatch <https://www.wikidata.org/entity/Q814207> ;
	skos:broader	medtop:20000446 .

medtop:20000456
	rdf:type skos:Concept ;
	skos:prefLabel	"injury"@en-GB ;
	skos:definition	"Harm caused to the human body by external forces such as falls, weapons or accidents"@en-GB ;
	skos:inScheme <http://cv.iptc.org/newscodes/mediatopic/>  ;
	ikos:created "2009-10-22T02:00:00+00:00"^^xsd:dateTime ;
	dct:created "2009-10-22T02:00:00+00:00"^^xsd:dateTime ;
	ikos:modified "2022-06-14T12:00:00+00:00"^^xsd:dateTime ;
	dct:modified "2022-06-14T12:00:00+00:00"^^xsd:dateTime  ;
	skos:exactMatch subj:07009000 ;
	skos:exactMatch <https://www.wikidata.org/entity/Q193078> ;
	skos:broader	medtop:20000446 .

medtop:20000457
	rdf:type skos:Concept ;
	skos:prefLabel	"medical condition"@en-GB ;
	skos:definition	"An abnormal condition that affects the structure and functioning of the body, such as chronic pain, high blood pressure or osteoperosis"@en-GB ;
	skos:inScheme <http://cv.iptc.org/newscodes/mediatopic/>  ;
	ikos:created "2009-10-22T02:00:00+00:00"^^xsd:dateTime ;
	dct:created "2009-10-22T02:00:00+00:00"^^xsd:dateTime ;
	ikos:modified "2022-06-14T12:00:00+00:00"^^xsd:dateTime ;
	dct:modified "2022-06-14T12:00:00+00:00"^^xsd:dateTime  ;
	skos:exactMatch subj:07018000 ;
	skos:exactMatch <https://www.wikidata.org/entity/Q12136> ;
	skos:broader	medtop:20000446 ;
	skos:narrower	medtop:20000460 .

medtop:20000458
	rdf:type skos:Concept ;
	skos:prefLabel	"mental health and disorder"@en-GB ;
	skos:definition	"The psychological well-being of an individual and the diseases and disorders that affect mood, thinking and behaviour as well as actions taken to bring improvement and awareness to these conditions"@en-GB ;
	skos:inScheme <http://cv.iptc.org/newscodes/mediatopic/>  ;
	ikos:created "2009-10-22T02:00:00+00:00"^^xsd:dateTime ;
	dct:created "2009-10-22T02:00:00+00:00"^^xsd:dateTime ;
	ikos:modified "2022-06-14T12:00:00+00:00"^^xsd:dateTime ;
	dct:modified "2022-06-14T12:00:00+00:00"^^xsd:dateTime  ;
	skos:broadMatch subj:07000000 ;
	skos:exactMatch <https://www.wikidata.org/entity/Q30085742> ;
	skos:broader	medtop:20000446 ;
	skos:narrower	medtop:20000459 ;
	skos:narrower	medtop:20001356 ;
	skos:narrower	medtop:20001357 .

medtop:20000459
	rdf:type skos:Concept ;
	skos:prefLabel	"eating disorder"@en-GB ;
	skos:definition	"Anorexia, bulimia, overeating and similar illnesses"@en-GB ;
	skos:inScheme <http://cv.iptc.org/newscodes/mediatopic/>  ;
	ikos:created "2009-10-22T02:00:00+00:00"^^xsd:dateTime ;
	dct:created "2009-10-22T02:00:00+00:00"^^xsd:dateTime ;
	ikos:modified "2021-02-18T12:00:00+00:00"^^xsd:dateTime ;
	dct:modified "2021-02-18T12:00:00+00:00"^^xsd:dateTime  ;
	skos:exactMatch subj:07017002 ;
	skos:exactMatch <https://www.wikidata.org/entity/Q373822> ;
	skos:broader	medtop:20000458 .

medtop:20000460
	rdf:type skos:Concept ;
	skos:prefLabel	"obesity"@en-GB ;
	skos:definition	"A condition of body weight generally considered 20 percent above the norm for gender, age, height and bone structure"@en-GB ;
	skos:inScheme <http://cv.iptc.org/newscodes/mediatopic/>  ;
	ikos:created "2009-10-22T02:00:00+00:00"^^xsd:dateTime ;
	dct:created "2009-10-22T02:00:00+00:00"^^xsd:dateTime ;
	ikos:modified "2022-06-14T12:00:00+00:00"^^xsd:dateTime ;
	dct:modified "2022-06-14T12:00:00+00:00"^^xsd:dateTime  ;
	skos:exactMatch subj:07017003 ;
	skos:exactMatch <https://www.wikidata.org/entity/Q12174> ;
	skos:broader	medtop:20000457 .

medtop:20000461
	rdf:type skos:Concept ;
	skos:prefLabel	"health facility"@en-GB ;
	skos:definition	"Facilities used for any kind of health care"@en-GB ;
	skos:inScheme <http://cv.iptc.org/newscodes/mediatopic/>  ;
	ikos:created "2009-10-22T02:00:00+00:00"^^xsd:dateTime ;
	dct:created "2009-10-22T02:00:00+00:00"^^xsd:dateTime ;
	ikos:modified "2022-06-14T12:00:00+00:00"^^xsd:dateTime ;
	dct:modified "2022-06-14T12:00:00+00:00"^^xsd:dateTime  ;
	skos:broadMatch subj:07010000 ;
	skos:exactMatch <https://www.wikidata.org/entity/Q4260475> ;
	skos:broader	medtop:07000000 ;
	skos:narrower	medtop:20000462 ;
	skos:narrower	medtop:20001229 .

medtop:20000462
	rdf:type skos:Concept ;
	skos:prefLabel	"hospital"@en-GB ;
	skos:definition	"Medical facilities for the treatment of illnesses and injury"@en-GB ;
	skos:inScheme <http://cv.iptc.org/newscodes/mediatopic/>  ;
	ikos:created "2009-10-22T02:00:00+00:00"^^xsd:dateTime ;
	dct:created "2009-10-22T02:00:00+00:00"^^xsd:dateTime ;
	ikos:modified "2021-05-05T12:00:00+00:00"^^xsd:dateTime ;
	dct:modified "2021-05-05T12:00:00+00:00"^^xsd:dateTime  ;
	skos:exactMatch subj:07010000 ;
	skos:exactMatch <https://www.wikidata.org/entity/Q16917> ;
	skos:broader	medtop:20000461 .

medtop:20000463
	rdf:type skos:Concept ;
	skos:prefLabel	"health organisation"@en-GB ;
	skos:definition	"Specific health organisations, including professional associations, non-profit and international groups"@en-GB ;
	skos:inScheme <http://cv.iptc.org/newscodes/mediatopic/>  ;
	ikos:created "2009-10-22T02:00:00+00:00"^^xsd:dateTime ;
	dct:created "2009-10-22T02:00:00+00:00"^^xsd:dateTime ;
	ikos:modified "2022-06-14T12:00:00+00:00"^^xsd:dateTime ;
	dct:modified "2022-06-14T12:00:00+00:00"^^xsd:dateTime  ;
	skos:exactMatch subj:07004000 ;
	skos:exactMatch <https://www.wikidata.org/entity/Q5691113> ;
	skos:broader	medtop:07000000 .

medtop:20000464
	rdf:type skos:Concept ;
	skos:prefLabel	"health treatment and procedure"@en-GB ;
	skos:definition	"Remedies, therapies, interventions, medications, testing and treatments to prevent, diagnose, manage or improve a health condition"@en-GB ;
	skos:inScheme <http://cv.iptc.org/newscodes/mediatopic/>  ;
	ikos:created "2009-10-22T02:00:00+00:00"^^xsd:dateTime ;
	dct:created "2009-10-22T02:00:00+00:00"^^xsd:dateTime ;
	ikos:modified "2022-06-14T12:00:00+00:00"^^xsd:dateTime ;
	dct:modified "2022-06-14T12:00:00+00:00"^^xsd:dateTime  ;
	skos:exactMatch subj:07003000 ;
	skos:exactMatch <https://www.wikidata.org/entity/Q65982936> ;
	skos:broader	medtop:07000000 ;
	skos:narrower	medtop:20000465 ;
	skos:narrower	medtop:20000467 ;
	skos:narrower	medtop:20000468 ;
	skos:narrower	medtop:20000469 ;
	skos:narrower	medtop:20000470 ;
	skos:narrower	medtop:20000475 ;
	skos:narrower	medtop:20000476 ;
	skos:narrower	medtop:20000477 ;
	skos:narrower	medtop:20000478 ;
	skos:narrower	medtop:20001219 ;
	skos:narrower	medtop:20001221 ;
	skos:narrower	medtop:20001228 .

medtop:20000465
	rdf:type skos:Concept ;
	skos:prefLabel	"diet"@en-GB ;
	skos:definition	"Ways of eating to benefit health or treat a condition, such as plant-based, low-salt, high-fibre or gluten-free"@en-GB ;
	skos:inScheme <http://cv.iptc.org/newscodes/mediatopic/>  ;
	ikos:created "2009-10-22T02:00:00+00:00"^^xsd:dateTime ;
	dct:created "2009-10-22T02:00:00+00:00"^^xsd:dateTime ;
	ikos:modified "2022-06-14T12:00:00+00:00"^^xsd:dateTime ;
	dct:modified "2022-06-14T12:00:00+00:00"^^xsd:dateTime  ;
	skos:exactMatch subj:07003003 ;
	skos:exactMatch <https://www.wikidata.org/entity/Q26869695> ;
	skos:broader	medtop:20000464 ;
	skos:narrower	medtop:20000466 .

medtop:20000466
	rdf:type skos:Concept ;
	skos:prefLabel	"dietary supplement"@en-GB ;
	skos:definition	"Nutrients taken in addition to food to bolster health"@en-GB ;
	skos:inScheme <http://cv.iptc.org/newscodes/mediatopic/>  ;
	ikos:created "2009-10-22T02:00:00+00:00"^^xsd:dateTime ;
	dct:created "2009-10-22T02:00:00+00:00"^^xsd:dateTime ;
	ikos:modified "2022-06-14T12:00:00+00:00"^^xsd:dateTime ;
	dct:modified "2022-06-14T12:00:00+00:00"^^xsd:dateTime  ;
	skos:exactMatch subj:07003002 ;
	skos:exactMatch <https://www.wikidata.org/entity/Q645858> ;
	skos:broader	medtop:20000465 .

medtop:20000467
	rdf:type skos:Concept ;
	skos:prefLabel	"non-prescription drug"@en-GB ;
	skos:definition	"Chemical substances used in the treatment or prevention of physical or mental condition or disease"@en-GB ;
	skos:inScheme <http://cv.iptc.org/newscodes/mediatopic/>  ;
	ikos:created "2009-10-22T02:00:00+00:00"^^xsd:dateTime ;
	dct:created "2009-10-22T02:00:00+00:00"^^xsd:dateTime ;
	ikos:modified "2022-06-14T12:00:00+00:00"^^xsd:dateTime ;
	dct:modified "2022-06-14T12:00:00+00:00"^^xsd:dateTime  ;
	skos:broadMatch subj:07000000 ;
	skos:exactMatch <https://www.wikidata.org/entity/Q12140> ;
	skos:broader	medtop:20000464 .

medtop:20000468
	rdf:type skos:Concept ;
	skos:prefLabel	"prescription drug"@en-GB ;
	skos:definition	"Drugs that can be obtained only with a doctor's authorisation"@en-GB ;
	skos:inScheme <http://cv.iptc.org/newscodes/mediatopic/>  ;
	ikos:created "2009-10-22T02:00:00+00:00"^^xsd:dateTime ;
	dct:created "2009-10-22T02:00:00+00:00"^^xsd:dateTime ;
	ikos:modified "2022-06-14T12:00:00+00:00"^^xsd:dateTime ;
	dct:modified "2022-06-14T12:00:00+00:00"^^xsd:dateTime  ;
	skos:exactMatch subj:07003001 ;
	skos:exactMatch <https://www.wikidata.org/entity/Q1643563> ;
	skos:broader	medtop:20000464 .

medtop:20000469
	rdf:type skos:Concept ;
	skos:prefLabel	"medical test"@en-GB ;
	skos:definition	"Diagnostic procedure, such as stress test, blood test, CAT scan or MRI"@en-GB ;
	skos:inScheme <http://cv.iptc.org/newscodes/mediatopic/>  ;
	ikos:created "2009-10-22T02:00:00+00:00"^^xsd:dateTime ;
	dct:created "2009-10-22T02:00:00+00:00"^^xsd:dateTime ;
	ikos:modified "2022-06-14T12:00:00+00:00"^^xsd:dateTime ;
	dct:modified "2022-06-14T12:00:00+00:00"^^xsd:dateTime  ;
	skos:exactMatch subj:07003004 ;
	skos:exactMatch <https://www.wikidata.org/entity/Q796194> ;
	skos:broader	medtop:20000464 .

medtop:20000470
	rdf:type skos:Concept ;
	skos:prefLabel	"health care approach"@en-GB ;
	skos:definition	"Different approaches to medical care that vary in the methods and substances used to treat symptoms"@en-GB ;
	skos:inScheme <http://cv.iptc.org/newscodes/mediatopic/>  ;
	ikos:created "2009-10-22T02:00:00+00:00"^^xsd:dateTime ;
	dct:created "2009-10-22T02:00:00+00:00"^^xsd:dateTime ;
	ikos:modified "2022-06-14T12:00:00+00:00"^^xsd:dateTime ;
	dct:modified "2022-06-14T12:00:00+00:00"^^xsd:dateTime  ;
	skos:exactMatch subj:07007000 ;
	skos:exactMatch <https://www.wikidata.org/entity/Q11190> ;
	skos:broader	medtop:20000464 ;
	skos:narrower	medtop:20000471 ;
	skos:narrower	medtop:20000472 ;
	skos:narrower	medtop:20000473 ;
	skos:narrower	medtop:20000474 .

medtop:20000471
	rdf:type skos:Concept ;
	skos:prefLabel	"herbal medicine"@en-GB ;
	skos:definition	"Treatment based on the use of herbs and other plants to cure or alleviate symptoms"@en-GB ;
	skos:inScheme <http://cv.iptc.org/newscodes/mediatopic/>  ;
	ikos:created "2009-10-22T02:00:00+00:00"^^xsd:dateTime ;
	dct:created "2009-10-22T02:00:00+00:00"^^xsd:dateTime ;
	ikos:modified "2022-06-14T12:00:00+00:00"^^xsd:dateTime ;
	dct:modified "2022-06-14T12:00:00+00:00"^^xsd:dateTime  ;
	skos:exactMatch subj:07007001 ;
	skos:exactMatch <https://www.wikidata.org/entity/Q861699> ;
	skos:broader	medtop:20000470 .

medtop:20000472
	rdf:type skos:Concept ;
	skos:prefLabel	"holistic medicine"@en-GB ;
	skos:definition	"Treatment of the whole person including mental and environmental factors in addition to treating symptoms"@en-GB ;
	skos:inScheme <http://cv.iptc.org/newscodes/mediatopic/>  ;
	ikos:created "2009-10-22T02:00:00+00:00"^^xsd:dateTime ;
	dct:created "2009-10-22T02:00:00+00:00"^^xsd:dateTime ;
	ikos:modified "2022-06-14T12:00:00+00:00"^^xsd:dateTime ;
	dct:modified "2022-06-14T12:00:00+00:00"^^xsd:dateTime  ;
	skos:exactMatch subj:07007002 ;
	skos:exactMatch <https://www.wikidata.org/entity/Q188504> ;
	skos:broader	medtop:20000470 .

medtop:20000473
	rdf:type skos:Concept ;
	skos:prefLabel	"traditional Chinese medicine"@en-GB ;
	skos:definition	"The practice of diagnosis, treatment and prevention of disease based on traditional methods developed in Eastern Asia"@en-GB ;
	skos:inScheme <http://cv.iptc.org/newscodes/mediatopic/>  ;
	ikos:created "2009-10-22T02:00:00+00:00"^^xsd:dateTime ;
	dct:created "2009-10-22T02:00:00+00:00"^^xsd:dateTime ;
	ikos:modified "2022-06-14T12:00:00+00:00"^^xsd:dateTime ;
	dct:modified "2022-06-14T12:00:00+00:00"^^xsd:dateTime  ;
	skos:exactMatch subj:07007004 ;
	skos:exactMatch <https://www.wikidata.org/entity/Q200253> ;
	skos:broader	medtop:20000470 .

medtop:20000474
	rdf:type skos:Concept ;
	skos:prefLabel	"conventional medicine"@en-GB ;
	skos:definition	"The practice of diagnosis, treatment and prevention of disease based on modern scientific research"@en-GB ;
	skos:inScheme <http://cv.iptc.org/newscodes/mediatopic/>  ;
	ikos:created "2009-10-22T02:00:00+00:00"^^xsd:dateTime ;
	dct:created "2009-10-22T02:00:00+00:00"^^xsd:dateTime ;
	ikos:modified "2022-06-14T12:00:00+00:00"^^xsd:dateTime ;
	dct:modified "2022-06-14T12:00:00+00:00"^^xsd:dateTime  ;
	skos:exactMatch subj:07007003 ;
	skos:exactMatch <https://www.wikidata.org/entity/Q691640> ;
	skos:broader	medtop:20000470 .

medtop:20000475
	rdf:type skos:Concept ;
	skos:prefLabel	"physical fitness"@en-GB ;
	skos:definition	"The measure of the body's ability to function efficiently and effectively during work and leisure activities."@en-GB ;
	skos:changeNote	"Retired. Use medtop:20001239 exercise and fitness instead."@en-GB ;
	skos:inScheme <http://cv.iptc.org/newscodes/mediatopic/>  ;
	ikos:created "2009-10-22T02:00:00+00:00"^^xsd:dateTime ;
	dct:created "2009-10-22T02:00:00+00:00"^^xsd:dateTime ;
	ikos:modified "2022-06-14T12:00:00+00:00"^^xsd:dateTime ;
	dct:modified "2022-06-14T12:00:00+00:00"^^xsd:dateTime  ; 
	ikos:retired "2022-06-14T12:00:00+00:00"^^xsd:dateTime ;
	skos:exactMatch subj:07016000 ;
	skos:exactMatch <https://www.wikidata.org/entity/Q309252> ;
	skos:broader	medtop:20000464 .

medtop:20000476
	rdf:type skos:Concept ;
	skos:prefLabel	"preventative medicine"@en-GB ;
	skos:definition	"Substances used to prevent diseases or illnesses"@en-GB ;
	skos:changeNote	"Retired."@en-GB ;
	skos:inScheme <http://cv.iptc.org/newscodes/mediatopic/>  ;
	ikos:created "2009-10-22T02:00:00+00:00"^^xsd:dateTime ;
	dct:created "2009-10-22T02:00:00+00:00"^^xsd:dateTime ;
	ikos:modified "2022-06-14T12:00:00+00:00"^^xsd:dateTime ;
	dct:modified "2022-06-14T12:00:00+00:00"^^xsd:dateTime  ; 
	ikos:retired "2022-06-14T12:00:00+00:00"^^xsd:dateTime ;
	skos:exactMatch subj:07008000 ;
	skos:exactMatch <https://www.wikidata.org/entity/Q1773974> ;
	skos:broader	medtop:20000464 .

medtop:20000477
	rdf:type skos:Concept ;
	skos:prefLabel	"vaccine"@en-GB ;
	skos:definition	"Medications designed to create immunity to diseases"@en-GB ;
	skos:inScheme <http://cv.iptc.org/newscodes/mediatopic/>  ;
	ikos:created "2009-10-22T02:00:00+00:00"^^xsd:dateTime ;
	dct:created "2009-10-22T02:00:00+00:00"^^xsd:dateTime ;
	ikos:modified "2022-06-14T12:00:00+00:00"^^xsd:dateTime ;
	dct:modified "2022-06-14T12:00:00+00:00"^^xsd:dateTime  ;
	skos:exactMatch subj:07008001 ;
	skos:exactMatch <https://www.wikidata.org/entity/Q134808> ;
	skos:broader	medtop:20000464 .

medtop:20000478
	rdf:type skos:Concept ;
	skos:prefLabel	"therapy"@en-GB ;
	skos:definition	"Treatment of physical, mental or medical conditions by non-surgical means"@en-GB ;
	skos:inScheme <http://cv.iptc.org/newscodes/mediatopic/>  ;
	ikos:created "2009-10-22T02:00:00+00:00"^^xsd:dateTime ;
	dct:created "2009-10-22T02:00:00+00:00"^^xsd:dateTime ;
	ikos:modified "2021-02-18T12:00:00+00:00"^^xsd:dateTime ;
	dct:modified "2021-02-18T12:00:00+00:00"^^xsd:dateTime  ;
	skos:exactMatch subj:07003005 ;
	skos:exactMatch <https://www.wikidata.org/entity/Q179661> ;
	skos:broader	medtop:20000464 .

medtop:20000479
	rdf:type skos:Concept ;
	skos:prefLabel	"healthcare policy"@en-GB ;
	skos:definition	"Health-related policy decisions including what different countries are doing regarding prescription drug policies, psychiatric care, health care funding, pandemic response and related topics"@en-GB ;
	skos:inScheme <http://cv.iptc.org/newscodes/mediatopic/>  ;
	ikos:created "2009-10-22T02:00:00+00:00"^^xsd:dateTime ;
	dct:created "2009-10-22T02:00:00+00:00"^^xsd:dateTime ;
	ikos:modified "2022-06-14T12:00:00+00:00"^^xsd:dateTime ;
	dct:modified "2022-06-14T12:00:00+00:00"^^xsd:dateTime  ;
	skos:exactMatch subj:07013000 ;
	skos:exactMatch <https://www.wikidata.org/entity/Q1519812> ;
	skos:broader	medtop:20000621 .

medtop:20000480
	rdf:type skos:Concept ;
	skos:prefLabel	"government health care"@en-GB ;
	skos:definition	"Health care provided by governments at any level"@en-GB ;
	skos:inScheme <http://cv.iptc.org/newscodes/mediatopic/>  ;
	ikos:created "2009-10-22T02:00:00+00:00"^^xsd:dateTime ;
	dct:created "2009-10-22T02:00:00+00:00"^^xsd:dateTime ;
	ikos:modified "2022-06-14T12:00:00+00:00"^^xsd:dateTime ;
	dct:modified "2022-06-14T12:00:00+00:00"^^xsd:dateTime  ;
	skos:exactMatch subj:07011000 ;
	skos:exactMatch <https://www.wikidata.org/entity/Q1519138> ;
	skos:broader	medtop:07000000 ;
	skos:narrower	medtop:20000481 ;
	skos:narrower	medtop:20000482 .

medtop:20000481
	rdf:type skos:Concept ;
	skos:prefLabel	"Medicaid"@en-GB ;
	skos:definition	"A program of the U.S. government to provide health care to needy citizens of all ages"@en-GB ;
	skos:changeNote	"This US-specific entity is not appropriate for Media Topics. The general concept of government-provided health care is covered by the parent."@en-GB ;
	skos:inScheme <http://cv.iptc.org/newscodes/mediatopic/>  ;
	ikos:created "2009-10-22T02:00:00+00:00"^^xsd:dateTime ;
	dct:created "2009-10-22T02:00:00+00:00"^^xsd:dateTime ;
	ikos:modified "2021-02-18T12:00:00+00:00"^^xsd:dateTime ;
	dct:modified "2021-02-18T12:00:00+00:00"^^xsd:dateTime  ; 
	ikos:retired "2014-06-02T12:00:00+00:00"^^xsd:dateTime ;
	skos:exactMatch subj:07011002 ;
	skos:exactMatch <https://www.wikidata.org/entity/Q1141363> ;
	skos:broader	medtop:20000480 .

medtop:20000482
	rdf:type skos:Concept ;
	skos:prefLabel	"Medicare"@en-GB ;
	skos:definition	"A program of the U.S. government to provide health care to senior citizens"@en-GB ;
	skos:changeNote	"This US-specific entity is not appropriate for Media Topics. The general concept of government-provided health care is covered by the parent."@en-GB ;
	skos:inScheme <http://cv.iptc.org/newscodes/mediatopic/>  ;
	ikos:created "2009-10-22T02:00:00+00:00"^^xsd:dateTime ;
	dct:created "2009-10-22T02:00:00+00:00"^^xsd:dateTime ;
	ikos:modified "2021-02-18T12:00:00+00:00"^^xsd:dateTime ;
	dct:modified "2021-02-18T12:00:00+00:00"^^xsd:dateTime  ; 
	ikos:retired "2014-06-02T12:00:00+00:00"^^xsd:dateTime ;
	skos:exactMatch subj:07011001 ;
	skos:exactMatch <https://www.wikidata.org/entity/Q559392> ;
	skos:broader	medtop:20000480 .

medtop:20000483
	rdf:type skos:Concept ;
	skos:prefLabel	"health insurance"@en-GB ;
	skos:definition	"Insurance covering medical costs"@en-GB ;
	skos:inScheme <http://cv.iptc.org/newscodes/mediatopic/>  ;
	ikos:created "2009-10-22T02:00:00+00:00"^^xsd:dateTime ;
	dct:created "2009-10-22T02:00:00+00:00"^^xsd:dateTime ;
	ikos:modified "2022-06-14T12:00:00+00:00"^^xsd:dateTime ;
	dct:modified "2022-06-14T12:00:00+00:00"^^xsd:dateTime  ;
	skos:exactMatch subj:14008000 ;
	skos:exactMatch <https://www.wikidata.org/entity/Q334911> ;
	skos:broader	medtop:07000000 .

medtop:20000484
	rdf:type skos:Concept ;
	skos:prefLabel	"private health care"@en-GB ;
	skos:definition	"Health care provided by private organisations"@en-GB ;
	skos:inScheme <http://cv.iptc.org/newscodes/mediatopic/>  ;
	ikos:created "2009-10-22T02:00:00+00:00"^^xsd:dateTime ;
	dct:created "2009-10-22T02:00:00+00:00"^^xsd:dateTime ;
	ikos:modified "2022-06-14T12:00:00+00:00"^^xsd:dateTime ;
	dct:modified "2022-06-14T12:00:00+00:00"^^xsd:dateTime  ;
	skos:exactMatch subj:07012000 ;
	skos:exactMatch <https://www.wikidata.org/entity/Q615678> ;
	skos:broader	medtop:07000000 .

medtop:20000485
	rdf:type skos:Concept ;
	skos:prefLabel	"medical profession"@en-GB ;
	skos:definition	"Profession requiring formal training in the study, diagnosis, treatment, care and prevention of disease, medical condition or injury"@en-GB ;
	skos:inScheme <http://cv.iptc.org/newscodes/mediatopic/>  ;
	ikos:created "2009-10-22T02:00:00+00:00"^^xsd:dateTime ;
	dct:created "2009-10-22T02:00:00+00:00"^^xsd:dateTime ;
	ikos:modified "2022-06-14T12:00:00+00:00"^^xsd:dateTime ;
	dct:modified "2022-06-14T12:00:00+00:00"^^xsd:dateTime  ;
	skos:broadMatch subj:07006000 ;
	skos:exactMatch <https://www.wikidata.org/entity/Q66811410> ;
	skos:broader	medtop:07000000 ;
	skos:narrower	medtop:20000486 ;
	skos:narrower	medtop:20000487 ;
	skos:narrower	medtop:20000492 .

medtop:20000486
	rdf:type skos:Concept ;
	skos:prefLabel	"medical service"@en-GB ;
	skos:definition	"Medical support for doctors, including blood tests and other medical tests on individuals, X-rays, CAT scans, MRIs, etc"@en-GB ;
	skos:inScheme <http://cv.iptc.org/newscodes/mediatopic/>  ;
	ikos:created "2009-10-22T02:00:00+00:00"^^xsd:dateTime ;
	dct:created "2009-10-22T02:00:00+00:00"^^xsd:dateTime ;
	ikos:modified "2022-06-14T12:00:00+00:00"^^xsd:dateTime ;
	dct:modified "2022-06-14T12:00:00+00:00"^^xsd:dateTime  ;
	skos:exactMatch subj:07015000 ;
	skos:exactMatch <https://www.wikidata.org/entity/Q55698119> ;
	skos:broader	medtop:20000485 .

medtop:20000487
	rdf:type skos:Concept ;
	skos:prefLabel	"medical specialisation"@en-GB ;
	skos:definition	"The different medical specialist areas"@en-GB ;
	skos:inScheme <http://cv.iptc.org/newscodes/mediatopic/>  ;
	ikos:created "2009-10-22T02:00:00+00:00"^^xsd:dateTime ;
	dct:created "2009-10-22T02:00:00+00:00"^^xsd:dateTime ;
	ikos:modified "2022-06-14T12:00:00+00:00"^^xsd:dateTime ;
	dct:modified "2022-06-14T12:00:00+00:00"^^xsd:dateTime  ;
	skos:exactMatch subj:07014000 ;
	skos:exactMatch <https://www.wikidata.org/entity/Q930752> ;
	skos:broader	medtop:20000485 ;
	skos:narrower	medtop:20000488 ;
	skos:narrower	medtop:20000489 ;
	skos:narrower	medtop:20000490 ;
	skos:narrower	medtop:20000491 ;
	skos:narrower	medtop:20000712 ;
	skos:narrower	medtop:20000713 ;
	skos:narrower	medtop:20000714 ;
	skos:narrower	medtop:20001220 ;
	skos:narrower	medtop:20001222 ;
	skos:narrower	medtop:20001223 ;
	skos:narrower	medtop:20001224 ;
	skos:narrower	medtop:20001225 ;
	skos:narrower	medtop:20001226 ;
	skos:narrower	medtop:20001227 .

medtop:20000488
	rdf:type skos:Concept ;
	skos:prefLabel	"geriatric medicine"@en-GB ;
	skos:definition	"Specialty focusing on ageing and age-related issues including age-related illnesses, medical research, and trends."@en-GB ;
	skos:changeNote	"Retired. Use medtop:20001232 elderly care instead."@en-GB ;
	skos:inScheme <http://cv.iptc.org/newscodes/mediatopic/>  ;
	ikos:created "2009-10-22T02:00:00+00:00"^^xsd:dateTime ;
	dct:created "2009-10-22T02:00:00+00:00"^^xsd:dateTime ;
	ikos:modified "2022-06-14T12:00:00+00:00"^^xsd:dateTime ;
	dct:modified "2022-06-14T12:00:00+00:00"^^xsd:dateTime  ; 
	ikos:retired "2022-06-14T12:00:00+00:00"^^xsd:dateTime ;
	skos:exactMatch subj:07014001 ;
	skos:exactMatch <https://www.wikidata.org/entity/Q10384> ;
	skos:broader	medtop:20000487 .

medtop:20000489
	rdf:type skos:Concept ;
	skos:prefLabel	"obstetrics/gynaecology"@en-GB ;
	skos:definition	"Specialty of female reproductive organs"@en-GB ;
	skos:changeNote	"Retired. Use medtop:20001359 pregnancy and childbirth instead."@en-GB ;
	skos:inScheme <http://cv.iptc.org/newscodes/mediatopic/>  ;
	ikos:created "2009-10-22T02:00:00+00:00"^^xsd:dateTime ;
	dct:created "2009-10-22T02:00:00+00:00"^^xsd:dateTime ;
	ikos:modified "2022-06-14T12:00:00+00:00"^^xsd:dateTime ;
	dct:modified "2022-06-14T12:00:00+00:00"^^xsd:dateTime  ; 
	ikos:retired "2022-06-14T12:00:00+00:00"^^xsd:dateTime ;
	skos:exactMatch subj:07014005 ;
	skos:exactMatch <https://www.wikidata.org/entity/Q80015> ;
	skos:broader	medtop:20000487 .

medtop:20000490
	rdf:type skos:Concept ;
	skos:prefLabel	"paediatrics"@en-GB ;
	skos:definition	"Medical specialisation that focuses on treating the young, including premature babies, infant care, childhood diseases and teenage health and behaviour problems"@en-GB ;
	skos:inScheme <http://cv.iptc.org/newscodes/mediatopic/>  ;
	ikos:created "2009-10-22T02:00:00+00:00"^^xsd:dateTime ;
	dct:created "2009-10-22T02:00:00+00:00"^^xsd:dateTime ;
	ikos:modified "2022-06-14T12:00:00+00:00"^^xsd:dateTime ;
	dct:modified "2022-06-14T12:00:00+00:00"^^xsd:dateTime  ;
	skos:exactMatch subj:07014002 ;
	skos:exactMatch <https://www.wikidata.org/entity/Q123028> ;
	skos:broader	medtop:20000487 .

medtop:20000491
	rdf:type skos:Concept ;
	skos:prefLabel	"reproductive medicine"@en-GB ;
	skos:definition	"Speciality of reproductive technologies like invitro fertilisation"@en-GB ;
	skos:changeNote	"Retired. Use medtop:20000784 family planning instead if relevant."@en-GB ;
	skos:inScheme <http://cv.iptc.org/newscodes/mediatopic/>  ;
	ikos:created "2009-10-22T02:00:00+00:00"^^xsd:dateTime ;
	dct:created "2009-10-22T02:00:00+00:00"^^xsd:dateTime ;
	ikos:modified "2022-06-14T12:00:00+00:00"^^xsd:dateTime ;
	dct:modified "2022-06-14T12:00:00+00:00"^^xsd:dateTime  ; 
	ikos:retired "2022-06-14T12:00:00+00:00"^^xsd:dateTime ;
	skos:broadMatch subj:07014003 ;
	skos:exactMatch <https://www.wikidata.org/entity/Q351870> ;
	skos:broader	medtop:20000487 .

medtop:20000492
	rdf:type skos:Concept ;
	skos:prefLabel	"medical staff"@en-GB ;
	skos:definition	"Doctors, nurses, interns and others in a medical facility"@en-GB ;
	skos:inScheme <http://cv.iptc.org/newscodes/mediatopic/>  ;
	ikos:created "2009-10-22T02:00:00+00:00"^^xsd:dateTime ;
	dct:created "2009-10-22T02:00:00+00:00"^^xsd:dateTime ;
	ikos:modified "2021-05-05T12:00:00+00:00"^^xsd:dateTime ;
	dct:modified "2021-05-05T12:00:00+00:00"^^xsd:dateTime  ;
	skos:exactMatch subj:07006000 ;
	skos:exactMatch <https://www.wikidata.org/entity/Q69948433> ;
	skos:broader	medtop:20000485 .

medtop:20000493
	rdf:type skos:Concept ;
	skos:prefLabel	"non-human diseases"@en-GB ;
	skos:definition	"Any harmful or destructive health condition affecting animals, plants or microorganisms."@en-GB ;
	skos:changeNote	"Retired. Use medtop:20000494 animal disease or medtop:20000495 plant disease instead."@en-GB ;
	skos:inScheme <http://cv.iptc.org/newscodes/mediatopic/>  ;
	ikos:created "2009-10-22T02:00:00+00:00"^^xsd:dateTime ;
	dct:created "2009-10-22T02:00:00+00:00"^^xsd:dateTime ;
	ikos:modified "2022-06-14T12:00:00+00:00"^^xsd:dateTime ;
	dct:modified "2022-06-14T12:00:00+00:00"^^xsd:dateTime  ; 
	ikos:retired "2022-06-14T12:00:00+00:00"^^xsd:dateTime ;
	skos:broadMatch subj:07001000 ;
	skos:broader	medtop:07000000 .

medtop:20000494
	rdf:type skos:Concept ;
	skos:prefLabel	"animal disease"@en-GB ;
	skos:definition	"Disease affecting animals"@en-GB ;
	skos:inScheme <http://cv.iptc.org/newscodes/mediatopic/>  ;
	ikos:created "2009-10-22T02:00:00+00:00"^^xsd:dateTime ;
	dct:created "2009-10-22T02:00:00+00:00"^^xsd:dateTime ;
	ikos:modified "2022-06-14T12:00:00+00:00"^^xsd:dateTime ;
	dct:modified "2022-06-14T12:00:00+00:00"^^xsd:dateTime  ;
	skos:exactMatch subj:07001007 ;
	skos:exactMatch <https://www.wikidata.org/entity/Q9190427> ;
	skos:broader	medtop:20000500 .

medtop:20000495
	rdf:type skos:Concept ;
	skos:prefLabel	"plant disease"@en-GB ;
	skos:definition	"Disorders affecting plants caused either by parasites or environmental factors"@en-GB ;
	skos:inScheme <http://cv.iptc.org/newscodes/mediatopic/>  ;
	ikos:created "2009-10-22T02:00:00+00:00"^^xsd:dateTime ;
	dct:created "2009-10-22T02:00:00+00:00"^^xsd:dateTime ;
	ikos:modified "2022-06-14T12:00:00+00:00"^^xsd:dateTime ;
	dct:modified "2022-06-14T12:00:00+00:00"^^xsd:dateTime  ;
	skos:exactMatch subj:07001008 ;
	skos:exactMatch <https://www.wikidata.org/entity/Q2662845> ;
	skos:broader	medtop:20000507 .

medtop:20000497
	rdf:type skos:Concept ;
	skos:prefLabel	"accomplishment"@en-GB ;
	skos:definition	"Achievements by individuals or groups, animals, plants or other objects, such as winning a competitive contest etc"@en-GB ;
	skos:changeNote	"2021-05-05: Retired. Use award and prize (20000498) or record and achievement (20000499) instead."@en-GB ;
	skos:inScheme <http://cv.iptc.org/newscodes/mediatopic/>  ;
	ikos:created "2009-10-22T02:00:00+00:00"^^xsd:dateTime ;
	dct:created "2009-10-22T02:00:00+00:00"^^xsd:dateTime ;
	ikos:modified "2021-05-05T12:00:00+00:00"^^xsd:dateTime ;
	dct:modified "2021-05-05T12:00:00+00:00"^^xsd:dateTime  ; 
	ikos:retired "2021-05-05T12:00:00+00:00"^^xsd:dateTime ;
	skos:closeMatch subj:08003003 ;
	skos:exactMatch <https://www.wikidata.org/entity/Q21013267> ;
	skos:broader	medtop:08000000 .

medtop:20000498
	rdf:type skos:Concept ;
	skos:prefLabel	"award and prize"@en-GB ;
	skos:definition	"The recognition of an achievement in a field in the form of a symbolic item, such as a plaque or trophy or in the form of a monetary gift, such as a cash prize or grant, given by a government or private institution"@en-GB ;
	skos:inScheme <http://cv.iptc.org/newscodes/mediatopic/>  ;
	ikos:created "2009-10-22T02:00:00+00:00"^^xsd:dateTime ;
	dct:created "2009-10-22T02:00:00+00:00"^^xsd:dateTime ;
	ikos:modified "2021-05-05T12:00:00+00:00"^^xsd:dateTime ;
	dct:modified "2021-05-05T12:00:00+00:00"^^xsd:dateTime  ;
	skos:exactMatch subj:08006000 ;
	skos:exactMatch <https://www.wikidata.org/entity/Q618779> ;
	skos:broader	medtop:08000000 .

medtop:20000499
	rdf:type skos:Concept ;
	skos:prefLabel	"record and achievement"@en-GB ;
	skos:definition	"Non-sport achievement by an individual or group that sets a new record, such as most books read or holding one's breath the longest"@en-GB ;
	skos:inScheme <http://cv.iptc.org/newscodes/mediatopic/>  ;
	ikos:created "2009-10-22T02:00:00+00:00"^^xsd:dateTime ;
	dct:created "2009-10-22T02:00:00+00:00"^^xsd:dateTime ;
	ikos:modified "2021-05-05T12:00:00+00:00"^^xsd:dateTime ;
	dct:modified "2021-05-05T12:00:00+00:00"^^xsd:dateTime  ;
	skos:exactMatch subj:08006001 ;
	skos:exactMatch <https://www.wikidata.org/entity/Q1241356> ;
	skos:broader	medtop:08000000 .

medtop:20000500
	rdf:type skos:Concept ;
	skos:prefLabel	"animal"@en-GB ;
	skos:definition	"Human interest and cultural stories related to animals, including pets"@en-GB ;
	skos:inScheme <http://cv.iptc.org/newscodes/mediatopic/>  ;
	ikos:created "2009-10-22T02:00:00+00:00"^^xsd:dateTime ;
	dct:created "2009-10-22T02:00:00+00:00"^^xsd:dateTime ;
	ikos:modified "2022-06-14T12:00:00+00:00"^^xsd:dateTime ;
	dct:modified "2022-06-14T12:00:00+00:00"^^xsd:dateTime  ;
	skos:exactMatch <https://www.wikidata.org/entity/Q729> ;
	skos:closeMatch subj:08001000 ;
	skos:broader	medtop:20000441 ;
	skos:narrower	medtop:20000494 ;
	skos:narrower	medtop:20001318 .

medtop:20000501
	rdf:type skos:Concept ;
	skos:prefLabel	"ceremony"@en-GB ;
	skos:definition	"Rituals, such as dedications, wreath laying or celebrating the launching of a ship"@en-GB ;
	skos:inScheme <http://cv.iptc.org/newscodes/mediatopic/>  ;
	ikos:created "2009-10-22T02:00:00+00:00"^^xsd:dateTime ;
	dct:created "2009-10-22T02:00:00+00:00"^^xsd:dateTime ;
	ikos:modified "2021-05-05T12:00:00+00:00"^^xsd:dateTime ;
	dct:modified "2021-05-05T12:00:00+00:00"^^xsd:dateTime  ;
	skos:exactMatch subj:08005001 ;
	skos:exactMatch <https://www.wikidata.org/entity/Q2627975> ;
	skos:broader	medtop:08000000 ;
	skos:narrower	medtop:20001233 ;
	skos:narrower	medtop:20001234 ;
	skos:narrower	medtop:20001235 ;
	skos:narrower	medtop:20001236 .

medtop:20000502
	rdf:type skos:Concept ;
	skos:prefLabel	"people"@en-GB ;
	skos:definition	"Individuals or groups with a focus on emotional facets"@en-GB ;
	skos:changeNote	"2021-05-05: Retired. Use more specific terms instead."@en-GB ;
	skos:inScheme <http://cv.iptc.org/newscodes/mediatopic/>  ;
	ikos:created "2009-10-22T02:00:00+00:00"^^xsd:dateTime ;
	dct:created "2009-10-22T02:00:00+00:00"^^xsd:dateTime ;
	ikos:modified "2021-02-18T12:00:00+00:00"^^xsd:dateTime ;
	dct:modified "2021-02-18T12:00:00+00:00"^^xsd:dateTime  ; 
	ikos:retired "2021-05-05T12:00:00+00:00"^^xsd:dateTime ;
	skos:closeMatch subj:08003000 ;
	skos:exactMatch <https://www.wikidata.org/entity/Q2472587> ;
	skos:broader	medtop:08000000 .

medtop:20000503
	rdf:type skos:Concept ;
	skos:prefLabel	"human mishap"@en-GB ;
	skos:definition	"Silly or stupid human errors"@en-GB ;
	skos:inScheme <http://cv.iptc.org/newscodes/mediatopic/>  ;
	ikos:created "2009-10-22T02:00:00+00:00"^^xsd:dateTime ;
	dct:created "2009-10-22T02:00:00+00:00"^^xsd:dateTime ;
	ikos:modified "2021-05-12T12:00:00+00:00"^^xsd:dateTime ;
	dct:modified "2021-05-12T12:00:00+00:00"^^xsd:dateTime  ;
	skos:closeMatch subj:08003004 ;
	skos:exactMatch <https://www.wikidata.org/entity/Q5937752> ;
	skos:broader	medtop:08000000 .

medtop:20000504
	rdf:type skos:Concept ;
	skos:prefLabel	"high society"@en-GB ;
	skos:definition	"Life and behaviour of the rich and socialites"@en-GB ;
	skos:inScheme <http://cv.iptc.org/newscodes/mediatopic/>  ;
	ikos:created "2009-10-22T02:00:00+00:00"^^xsd:dateTime ;
	dct:created "2009-10-22T02:00:00+00:00"^^xsd:dateTime ;
	ikos:modified "2021-05-05T12:00:00+00:00"^^xsd:dateTime ;
	dct:modified "2021-05-05T12:00:00+00:00"^^xsd:dateTime  ;
	skos:closeMatch subj:08005000 ;
	skos:exactMatch <https://www.wikidata.org/entity/Q17126676> ;
	skos:broader	medtop:08000000 ;
	skos:narrower	medtop:20000506 .

medtop:20000505
	rdf:type skos:Concept ;
	skos:prefLabel	"celebrity"@en-GB ;
	skos:definition	"Life and behaviour of famous people"@en-GB ;
	skos:inScheme <http://cv.iptc.org/newscodes/mediatopic/>  ;
	ikos:created "2009-10-22T02:00:00+00:00"^^xsd:dateTime ;
	dct:created "2009-10-22T02:00:00+00:00"^^xsd:dateTime ;
	ikos:modified "2021-05-05T12:00:00+00:00"^^xsd:dateTime ;
	dct:modified "2021-05-05T12:00:00+00:00"^^xsd:dateTime  ;
	skos:closeMatch subj:08003002 ;
	skos:exactMatch <https://www.wikidata.org/entity/Q211236> ;
	skos:broader	medtop:08000000 .

medtop:20000506
	rdf:type skos:Concept ;
	skos:prefLabel	"royalty"@en-GB ;
	skos:definition	"Imperial and royal family members in their societal rather than governmental roles"@en-GB ;
	skos:inScheme <http://cv.iptc.org/newscodes/mediatopic/>  ;
	ikos:created "2009-10-22T02:00:00+00:00"^^xsd:dateTime ;
	dct:created "2009-10-22T02:00:00+00:00"^^xsd:dateTime ;
	ikos:modified "2021-05-05T12:00:00+00:00"^^xsd:dateTime ;
	dct:modified "2021-05-05T12:00:00+00:00"^^xsd:dateTime  ;
	skos:exactMatch subj:08007000 ;
	skos:broader	medtop:20000504 .

medtop:20000507
	rdf:type skos:Concept ;
	skos:prefLabel	"flowers and plants"@en-GB ;
	skos:definition	"Human interest and cultural stories related to plants, flowers and trees"@en-GB ;
	skos:inScheme <http://cv.iptc.org/newscodes/mediatopic/>  ;
	ikos:created "2009-10-22T02:00:00+00:00"^^xsd:dateTime ;
	dct:created "2009-10-22T02:00:00+00:00"^^xsd:dateTime ;
	ikos:modified "2022-06-14T12:00:00+00:00"^^xsd:dateTime ;
	dct:modified "2022-06-14T12:00:00+00:00"^^xsd:dateTime  ;
	skos:exactMatch <https://www.wikidata.org/entity/Q756> ;
	skos:closeMatch subj:08008000 ;
	skos:broader	medtop:20000441 ;
	skos:narrower	medtop:20000495 .

medtop:20000509
	rdf:type skos:Concept ;
	skos:prefLabel	"employment"@en-GB ;
	skos:definition	"The state of having work, usually paid, for a company, organisation, or individual"@en-GB ;
	skos:inScheme <http://cv.iptc.org/newscodes/mediatopic/>  ;
	ikos:created "2009-10-22T02:00:00+00:00"^^xsd:dateTime ;
	dct:created "2009-10-22T02:00:00+00:00"^^xsd:dateTime ;
	ikos:modified "2021-02-18T12:00:00+00:00"^^xsd:dateTime ;
	dct:modified "2021-02-18T12:00:00+00:00"^^xsd:dateTime  ;
	skos:closeMatch subj:09003000 ;
	skos:exactMatch <https://www.wikidata.org/entity/Q656365> ;
	skos:broader	medtop:09000000 ;
	skos:narrower	medtop:20000339 ;
	skos:narrower	medtop:20000510 ;
	skos:narrower	medtop:20000511 ;
	skos:narrower	medtop:20000512 ;
	skos:narrower	medtop:20000513 ;
	skos:narrower	medtop:20000514 ;
	skos:narrower	medtop:20000517 ;
	skos:narrower	medtop:20000518 ;
	skos:narrower	medtop:20001206 ;
	skos:narrower	medtop:20001276 ;
	skos:narrower	medtop:20001277 .

medtop:20000510
	rdf:type skos:Concept ;
	skos:prefLabel	"apprenticeship"@en-GB ;
	skos:definition	"A period of work used to learn a skill or trade"@en-GB ;
	skos:inScheme <http://cv.iptc.org/newscodes/mediatopic/>  ;
	ikos:created "2009-10-22T02:00:00+00:00"^^xsd:dateTime ;
	dct:created "2009-10-22T02:00:00+00:00"^^xsd:dateTime ;
	ikos:modified "2021-02-18T12:00:00+00:00"^^xsd:dateTime ;
	dct:modified "2021-02-18T12:00:00+00:00"^^xsd:dateTime  ;
	skos:exactMatch subj:09001000 ;
	skos:exactMatch <https://www.wikidata.org/entity/Q253567> ;
	skos:broader	medtop:20000509 .

medtop:20000511
	rdf:type skos:Concept ;
	skos:prefLabel	"child labour"@en-GB ;
	skos:definition	"The employment of children"@en-GB ;
	skos:inScheme <http://cv.iptc.org/newscodes/mediatopic/>  ;
	ikos:created "2009-10-22T02:00:00+00:00"^^xsd:dateTime ;
	dct:created "2009-10-22T02:00:00+00:00"^^xsd:dateTime ;
	ikos:modified "2021-02-18T12:00:00+00:00"^^xsd:dateTime ;
	dct:modified "2021-02-18T12:00:00+00:00"^^xsd:dateTime  ;
	skos:exactMatch subj:09003003 ;
	skos:exactMatch <https://www.wikidata.org/entity/Q192571> ;
	skos:broader	medtop:20000509 .

medtop:20000512
	rdf:type skos:Concept ;
	skos:prefLabel	"employee"@en-GB ;
	skos:definition	"Those who are paid or otherwise compensated for providing services to employers"@en-GB ;
	skos:inScheme <http://cv.iptc.org/newscodes/mediatopic/>  ;
	ikos:created "2009-10-22T02:00:00+00:00"^^xsd:dateTime ;
	dct:created "2009-10-22T02:00:00+00:00"^^xsd:dateTime ;
	ikos:modified "2021-02-18T12:00:00+00:00"^^xsd:dateTime ;
	dct:modified "2021-02-18T12:00:00+00:00"^^xsd:dateTime  ;
	skos:exactMatch subj:09016000 ;
	skos:exactMatch <https://www.wikidata.org/entity/Q703534> ;
	skos:broader	medtop:20000509 .

medtop:20000513
	rdf:type skos:Concept ;
	skos:prefLabel	"employer"@en-GB ;
	skos:definition	"People and organisations that pay employees to provide services"@en-GB ;
	skos:inScheme <http://cv.iptc.org/newscodes/mediatopic/>  ;
	ikos:created "2009-10-22T02:00:00+00:00"^^xsd:dateTime ;
	dct:created "2009-10-22T02:00:00+00:00"^^xsd:dateTime ;
	ikos:modified "2021-02-18T12:00:00+00:00"^^xsd:dateTime ;
	dct:modified "2021-02-18T12:00:00+00:00"^^xsd:dateTime  ;
	skos:exactMatch subj:09015000 ;
	skos:exactMatch <https://www.wikidata.org/entity/Q3053337> ;
	skos:broader	medtop:20000509 .

medtop:20000514
	rdf:type skos:Concept ;
	skos:prefLabel	"employment training"@en-GB ;
	skos:definition	"Learning new skills as part of an existing job, such as developing specialisations, learning new techniques or retraining when an employee's skills are no longer relevant"@en-GB ;
	skos:inScheme <http://cv.iptc.org/newscodes/mediatopic/>  ;
	ikos:created "2009-10-22T02:00:00+00:00"^^xsd:dateTime ;
	dct:created "2009-10-22T02:00:00+00:00"^^xsd:dateTime ;
	ikos:modified "2021-02-18T12:00:00+00:00"^^xsd:dateTime ;
	dct:modified "2021-02-18T12:00:00+00:00"^^xsd:dateTime  ;
	skos:broadMatch subj:09003000 ;
	skos:exactMatch <https://www.wikidata.org/entity/Q828812> ;
	skos:broader	medtop:20000509 ;
	skos:narrower	medtop:20000515 ;
	skos:narrower	medtop:20000516 .

medtop:20000515
	rdf:type skos:Concept ;
	skos:prefLabel	"advanced training"@en-GB ;
	skos:definition	"Additional training to enhance current skills"@en-GB ;
	skos:inScheme <http://cv.iptc.org/newscodes/mediatopic/>  ;
	ikos:created "2009-10-22T02:00:00+00:00"^^xsd:dateTime ;
	dct:created "2009-10-22T02:00:00+00:00"^^xsd:dateTime ;
	ikos:modified "2021-05-05T12:00:00+00:00"^^xsd:dateTime ;
	dct:modified "2021-05-05T12:00:00+00:00"^^xsd:dateTime  ; 
	ikos:retired "2019-10-07T12:00:00+00:00"^^xsd:dateTime ;
	skos:exactMatch subj:09014000 ;
	skos:exactMatch <https://www.wikidata.org/entity/Q828748> ;
	skos:broader	medtop:20000514 .

medtop:20000516
	rdf:type skos:Concept ;
	skos:prefLabel	"retraining"@en-GB ;
	skos:definition	"Providing a worker training in new skills when his old skills are no longer applicable"@en-GB ;
	skos:inScheme <http://cv.iptc.org/newscodes/mediatopic/>  ;
	ikos:created "2009-10-22T02:00:00+00:00"^^xsd:dateTime ;
	dct:created "2009-10-22T02:00:00+00:00"^^xsd:dateTime ;
	ikos:modified "2021-02-18T12:00:00+00:00"^^xsd:dateTime ;
	dct:modified "2021-02-18T12:00:00+00:00"^^xsd:dateTime  ; 
	ikos:retired "2019-10-07T12:00:00+00:00"^^xsd:dateTime ;
	skos:exactMatch subj:09007000 ;
	skos:exactMatch <https://www.wikidata.org/entity/Q3505966> ;
	skos:broader	medtop:20000514 .

medtop:20000517
	rdf:type skos:Concept ;
	skos:prefLabel	"occupations"@en-GB ;
	skos:definition	"Generally one's trade, profession or business although professions are usually such things as lawyers and doctors, and occupations are such as clerks or truckers"@en-GB ;
	skos:inScheme <http://cv.iptc.org/newscodes/mediatopic/>  ;
	ikos:created "2009-10-22T02:00:00+00:00"^^xsd:dateTime ;
	dct:created "2009-10-22T02:00:00+00:00"^^xsd:dateTime ;
	ikos:modified "2021-02-18T12:00:00+00:00"^^xsd:dateTime ;
	dct:modified "2021-02-18T12:00:00+00:00"^^xsd:dateTime  ; 
	ikos:retired "2019-10-07T12:00:00+00:00"^^xsd:dateTime ;
	skos:exactMatch subj:09003004 ;
	skos:exactMatch <https://www.wikidata.org/entity/Q12737077> ;
	skos:broader	medtop:20000509 .

medtop:20000518
	rdf:type skos:Concept ;
	skos:prefLabel	"wages and benefits"@en-GB ;
	skos:definition	"Money, or other items of value such as pension contributions and health insurance, paid to employees as compensation for their work"@en-GB ;
	skos:inScheme <http://cv.iptc.org/newscodes/mediatopic/>  ;
	ikos:created "2009-10-22T02:00:00+00:00"^^xsd:dateTime ;
	dct:created "2009-10-22T02:00:00+00:00"^^xsd:dateTime ;
	ikos:modified "2021-02-18T12:00:00+00:00"^^xsd:dateTime ;
	dct:modified "2021-02-18T12:00:00+00:00"^^xsd:dateTime  ;
	skos:broadMatch subj:09011001 ;
	skos:exactMatch <https://www.wikidata.org/entity/Q6821213> ;
	skos:broader	medtop:20000509 ;
	skos:narrower	medtop:20000519 ;
	skos:narrower	medtop:20000520 ;
	skos:narrower	medtop:20001375 .

medtop:20000519
	rdf:type skos:Concept ;
	skos:prefLabel	"employee benefits"@en-GB ;
	skos:definition	"Benefits provided to an employee by a company, such as pension contributions, health insurance."@en-GB ;
	skos:inScheme <http://cv.iptc.org/newscodes/mediatopic/>  ;
	ikos:created "2009-10-22T02:00:00+00:00"^^xsd:dateTime ;
	dct:created "2009-10-22T02:00:00+00:00"^^xsd:dateTime ;
	ikos:modified "2021-02-18T12:00:00+00:00"^^xsd:dateTime ;
	dct:modified "2021-02-18T12:00:00+00:00"^^xsd:dateTime  ; 
	ikos:retired "2019-10-07T12:00:00+00:00"^^xsd:dateTime ;
	skos:closeMatch subj:09011001 ;
	skos:exactMatch <https://www.wikidata.org/entity/Q678774> ;
	skos:broader	medtop:20000518 .

medtop:20000520
	rdf:type skos:Concept ;
	skos:prefLabel	"social security"@en-GB ;
	skos:definition	"a government system that provides monetary assistance to people with inadequate or no incomes, such as retirees, disabled people or carers"@en-GB ;
	skos:inScheme <http://cv.iptc.org/newscodes/mediatopic/>  ;
	ikos:created "2009-10-22T02:00:00+00:00"^^xsd:dateTime ;
	dct:created "2009-10-22T02:00:00+00:00"^^xsd:dateTime ;
	ikos:modified "2021-02-18T12:00:00+00:00"^^xsd:dateTime ;
	dct:modified "2021-02-18T12:00:00+00:00"^^xsd:dateTime  ;
	skos:exactMatch subj:09011002 ;
	skos:exactMatch <https://www.wikidata.org/entity/Q2483208> ;
	skos:broader	medtop:20000518 .

medtop:20000521
	rdf:type skos:Concept ;
	skos:prefLabel	"employment legislation"@en-GB ;
	skos:definition	"Laws governing employment"@en-GB ;
	skos:inScheme <http://cv.iptc.org/newscodes/mediatopic/>  ;
	ikos:created "2009-10-22T02:00:00+00:00"^^xsd:dateTime ;
	dct:created "2009-10-22T02:00:00+00:00"^^xsd:dateTime ;
	ikos:modified "2021-02-18T12:00:00+00:00"^^xsd:dateTime ;
	dct:modified "2021-02-18T12:00:00+00:00"^^xsd:dateTime  ;
	skos:broadMatch subj:09005000 ;
	skos:exactMatch <https://www.wikidata.org/entity/Q7498399> ;
	skos:broader	medtop:09000000 ;
	skos:narrower	medtop:20000522 .

medtop:20000522
	rdf:type skos:Concept ;
	skos:prefLabel	"workplace health and safety"@en-GB ;
	skos:definition	"Laws protecting a safe and healthy work environment"@en-GB ;
	skos:inScheme <http://cv.iptc.org/newscodes/mediatopic/>  ;
	ikos:created "2009-10-22T02:00:00+00:00"^^xsd:dateTime ;
	dct:created "2009-10-22T02:00:00+00:00"^^xsd:dateTime ;
	ikos:modified "2021-02-18T12:00:00+00:00"^^xsd:dateTime ;
	dct:modified "2021-02-18T12:00:00+00:00"^^xsd:dateTime  ;
	skos:exactMatch subj:09013000 ;
	skos:exactMatch <https://www.wikidata.org/entity/Q629029> ;
	skos:broader	medtop:20000521 .

medtop:20000523
	rdf:type skos:Concept ;
	skos:prefLabel	"labour market"@en-GB ;
	skos:definition	"The supply and demand of labour in an economy"@en-GB ;
	skos:inScheme <http://cv.iptc.org/newscodes/mediatopic/>  ;
	ikos:created "2009-10-22T02:00:00+00:00"^^xsd:dateTime ;
	dct:created "2009-10-22T02:00:00+00:00"^^xsd:dateTime ;
	ikos:modified "2021-02-18T12:00:00+00:00"^^xsd:dateTime ;
	dct:modified "2021-02-18T12:00:00+00:00"^^xsd:dateTime  ;
	skos:exactMatch subj:09003001 ;
	skos:exactMatch <https://www.wikidata.org/entity/Q305186> ;
	skos:broader	medtop:09000000 ;
	skos:narrower	medtop:20001275 .

medtop:20000524
	rdf:type skos:Concept ;
	skos:prefLabel	"labour relations"@en-GB ;
	skos:definition	"The relationship between workers and employers"@en-GB ;
	skos:inScheme <http://cv.iptc.org/newscodes/mediatopic/>  ;
	ikos:created "2009-10-22T02:00:00+00:00"^^xsd:dateTime ;
	dct:created "2009-10-22T02:00:00+00:00"^^xsd:dateTime ;
	ikos:modified "2021-02-18T12:00:00+00:00"^^xsd:dateTime ;
	dct:modified "2021-02-18T12:00:00+00:00"^^xsd:dateTime  ;
	skos:exactMatch <https://www.wikidata.org/entity/Q608190> ;
	skos:broadMatch subj:09012000 ;
	skos:broader	medtop:09000000 ;
	skos:narrower	medtop:20000525 ;
	skos:narrower	medtop:20000529 .

medtop:20000525
	rdf:type skos:Concept ;
	skos:prefLabel	"collective agreements"@en-GB ;
	skos:definition	"Negotiated guidelines for relationships between groups of employees and employers, including issues such as working hours, wages, health care, pensions and other benefits"@en-GB ;
	skos:inScheme <http://cv.iptc.org/newscodes/mediatopic/>  ;
	ikos:created "2009-10-22T02:00:00+00:00"^^xsd:dateTime ;
	dct:created "2009-10-22T02:00:00+00:00"^^xsd:dateTime ;
	ikos:modified "2021-02-18T12:00:00+00:00"^^xsd:dateTime ;
	dct:modified "2021-02-18T12:00:00+00:00"^^xsd:dateTime  ;
	skos:exactMatch subj:09002000 ;
	skos:exactMatch <https://www.wikidata.org/entity/Q163887> ;
	skos:broader	medtop:20000524 ;
	skos:narrower	medtop:20000526 ;
	skos:narrower	medtop:20000527 ;
	skos:narrower	medtop:20000528 .

medtop:20000526
	rdf:type skos:Concept ;
	skos:prefLabel	"contract issue-healthcare"@en-GB ;
	skos:definition	"Element of contracts and contract discussions centring on health care issues"@en-GB ;
	skos:inScheme <http://cv.iptc.org/newscodes/mediatopic/>  ;
	ikos:created "2009-10-22T02:00:00+00:00"^^xsd:dateTime ;
	dct:created "2009-10-22T02:00:00+00:00"^^xsd:dateTime ;
	ikos:modified "2021-05-05T12:00:00+00:00"^^xsd:dateTime ;
	dct:modified "2021-05-05T12:00:00+00:00"^^xsd:dateTime  ; 
	ikos:retired "2019-10-07T12:00:00+00:00"^^xsd:dateTime ;
	skos:exactMatch subj:09002002 ;
	skos:exactMatch <https://www.wikidata.org/entity/Q629029> ;
	skos:broader	medtop:20000525 .

medtop:20000527
	rdf:type skos:Concept ;
	skos:prefLabel	"contract issue-wages"@en-GB ;
	skos:definition	"Element of contracts and contract discussions centring on remuneration"@en-GB ;
	skos:inScheme <http://cv.iptc.org/newscodes/mediatopic/>  ;
	ikos:created "2009-10-22T02:00:00+00:00"^^xsd:dateTime ;
	dct:created "2009-10-22T02:00:00+00:00"^^xsd:dateTime ;
	ikos:modified "2021-05-05T12:00:00+00:00"^^xsd:dateTime ;
	dct:modified "2021-05-05T12:00:00+00:00"^^xsd:dateTime  ; 
	ikos:retired "2019-10-07T12:00:00+00:00"^^xsd:dateTime ;
	skos:exactMatch subj:09002001 ;
	skos:exactMatch <https://www.wikidata.org/entity/Q6821213> ;
	skos:broader	medtop:20000525 .

medtop:20000528
	rdf:type skos:Concept ;
	skos:prefLabel	"contract issue-work rules"@en-GB ;
	skos:definition	"Element of contracts and contract discussions centring on rules affecting issues such as lunch and other breaks, work shifts, vacation scheduling, seniority, sick leave etc."@en-GB ;
	skos:inScheme <http://cv.iptc.org/newscodes/mediatopic/>  ;
	ikos:created "2009-10-22T02:00:00+00:00"^^xsd:dateTime ;
	dct:created "2009-10-22T02:00:00+00:00"^^xsd:dateTime ;
	ikos:modified "2021-02-18T12:00:00+00:00"^^xsd:dateTime ;
	dct:modified "2021-02-18T12:00:00+00:00"^^xsd:dateTime  ; 
	ikos:retired "2019-10-07T12:00:00+00:00"^^xsd:dateTime ;
	skos:exactMatch subj:09002003 ;
	skos:broader	medtop:20000525 .

medtop:20000529
	rdf:type skos:Concept ;
	skos:prefLabel	"labour dispute"@en-GB ;
	skos:definition	"Disagreements between employers and employees regarding work conditions, pay or other issues"@en-GB ;
	skos:inScheme <http://cv.iptc.org/newscodes/mediatopic/>  ;
	ikos:created "2009-10-22T02:00:00+00:00"^^xsd:dateTime ;
	dct:created "2009-10-22T02:00:00+00:00"^^xsd:dateTime ;
	ikos:modified "2021-02-18T12:00:00+00:00"^^xsd:dateTime ;
	dct:modified "2021-02-18T12:00:00+00:00"^^xsd:dateTime  ;
	skos:exactMatch subj:09004000 ;
	skos:exactMatch <https://www.wikidata.org/entity/Q2310419> ;
	skos:broader	medtop:20000524 ;
	skos:narrower	medtop:20000530 .

medtop:20000530
	rdf:type skos:Concept ;
	skos:prefLabel	"labour strike"@en-GB ;
	skos:definition	"Groups of employees agreeing to cease work activities with the aim of achieving better pay or work conditions"@en-GB ;
	skos:inScheme <http://cv.iptc.org/newscodes/mediatopic/>  ;
	ikos:created "2009-10-22T02:00:00+00:00"^^xsd:dateTime ;
	dct:created "2009-10-22T02:00:00+00:00"^^xsd:dateTime ;
	ikos:modified "2021-02-18T12:00:00+00:00"^^xsd:dateTime ;
	dct:modified "2021-02-18T12:00:00+00:00"^^xsd:dateTime  ;
	skos:exactMatch subj:09008000 ;
	skos:exactMatch <https://www.wikidata.org/entity/Q49776> ;
	skos:broader	medtop:20000529 .

medtop:20000531
	rdf:type skos:Concept ;
	skos:prefLabel	"retirement"@en-GB ;
	skos:definition	"The years after work"@en-GB ;
	skos:inScheme <http://cv.iptc.org/newscodes/mediatopic/>  ;
	ikos:created "2009-10-22T02:00:00+00:00"^^xsd:dateTime ;
	dct:created "2009-10-22T02:00:00+00:00"^^xsd:dateTime ;
	ikos:modified "2021-02-18T12:00:00+00:00"^^xsd:dateTime ;
	dct:modified "2021-02-18T12:00:00+00:00"^^xsd:dateTime  ;
	skos:exactMatch subj:09006000 ;
	skos:exactMatch <https://www.wikidata.org/entity/Q946865> ;
	skos:broader	medtop:09000000 ;
	skos:narrower	medtop:20000532 .

medtop:20000532
	rdf:type skos:Concept ;
	skos:prefLabel	"pension"@en-GB ;
	skos:definition	"Payments, either government or private, to retired people"@en-GB ;
	skos:inScheme <http://cv.iptc.org/newscodes/mediatopic/>  ;
	ikos:created "2009-10-22T02:00:00+00:00"^^xsd:dateTime ;
	dct:created "2009-10-22T02:00:00+00:00"^^xsd:dateTime ;
	ikos:modified "2021-02-18T12:00:00+00:00"^^xsd:dateTime ;
	dct:modified "2021-02-18T12:00:00+00:00"^^xsd:dateTime  ;
	skos:broadMatch subj:09006000 ;
	skos:exactMatch <https://www.wikidata.org/entity/Q156223> ;
	skos:broader	medtop:20000531 .

medtop:20000533
	rdf:type skos:Concept ;
	skos:prefLabel	"unemployment"@en-GB ;
	skos:definition	"The state of being available to work but not having a job"@en-GB ;
	skos:inScheme <http://cv.iptc.org/newscodes/mediatopic/>  ;
	ikos:created "2009-10-22T02:00:00+00:00"^^xsd:dateTime ;
	dct:created "2009-10-22T02:00:00+00:00"^^xsd:dateTime ;
	ikos:modified "2021-02-18T12:00:00+00:00"^^xsd:dateTime ;
	dct:modified "2021-02-18T12:00:00+00:00"^^xsd:dateTime  ;
	skos:closeMatch subj:09009000 ;
	skos:exactMatch <https://www.wikidata.org/entity/Q41171> ;
	skos:broader	medtop:09000000 ;
	skos:narrower	medtop:20000534 ;
	skos:narrower	medtop:20000535 .

medtop:20000534
	rdf:type skos:Concept ;
	skos:prefLabel	"job layoffs"@en-GB ;
	skos:definition	"The reduction of a company's work force through dismissal because of changing economic factors"@en-GB ;
	skos:inScheme <http://cv.iptc.org/newscodes/mediatopic/>  ;
	ikos:created "2009-10-22T02:00:00+00:00"^^xsd:dateTime ;
	dct:created "2009-10-22T02:00:00+00:00"^^xsd:dateTime ;
	ikos:modified "2021-02-18T12:00:00+00:00"^^xsd:dateTime ;
	dct:modified "2021-02-18T12:00:00+00:00"^^xsd:dateTime  ; 
	ikos:retired "2019-10-07T12:00:00+00:00"^^xsd:dateTime ;
	skos:exactMatch subj:09003002 ;
	skos:exactMatch <https://www.wikidata.org/entity/Q1462531> ;
	skos:broader	medtop:20000533 .

medtop:20000535
	rdf:type skos:Concept ;
	skos:prefLabel	"unemployment benefits"@en-GB ;
	skos:definition	"Monetary compensation paid to the jobless"@en-GB ;
	skos:inScheme <http://cv.iptc.org/newscodes/mediatopic/>  ;
	ikos:created "2009-10-22T02:00:00+00:00"^^xsd:dateTime ;
	dct:created "2009-10-22T02:00:00+00:00"^^xsd:dateTime ;
	ikos:modified "2021-02-18T12:00:00+00:00"^^xsd:dateTime ;
	dct:modified "2021-02-18T12:00:00+00:00"^^xsd:dateTime  ;
	skos:broadMatch subj:09009000 ;
	skos:exactMatch <https://www.wikidata.org/entity/Q311255> ;
	skos:broader	medtop:20000533 .

medtop:20000536
	rdf:type skos:Concept ;
	skos:prefLabel	"unions"@en-GB ;
	skos:definition	"Groups established to represent bodies of workers in order to obtain better workplace conditions through collective bargaining"@en-GB ;
	skos:inScheme <http://cv.iptc.org/newscodes/mediatopic/>  ;
	ikos:created "2009-10-22T02:00:00+00:00"^^xsd:dateTime ;
	dct:created "2009-10-22T02:00:00+00:00"^^xsd:dateTime ;
	ikos:modified "2021-02-18T12:00:00+00:00"^^xsd:dateTime ;
	dct:modified "2021-02-18T12:00:00+00:00"^^xsd:dateTime  ;
	skos:exactMatch subj:09010000 ;
	skos:exactMatch <https://www.wikidata.org/entity/Q178790> ;
	skos:broader	medtop:09000000 .

medtop:20000538
	rdf:type skos:Concept ;
	skos:prefLabel	"leisure"@en-GB ;
	skos:definition	"Activities carried out in ones' spare time and not in a competitive way."@en-GB ;
	skos:inScheme <http://cv.iptc.org/newscodes/mediatopic/>  ;
	ikos:created "2009-10-22T02:00:00+00:00"^^xsd:dateTime ;
	dct:created "2009-10-22T02:00:00+00:00"^^xsd:dateTime ;
	ikos:modified "2021-02-18T12:00:00+00:00"^^xsd:dateTime ;
	dct:modified "2021-02-18T12:00:00+00:00"^^xsd:dateTime  ;
	skos:broadMatch subj:10010000 ;
	skos:exactMatch <https://www.wikidata.org/entity/Q180910> ;
	skos:broader	medtop:10000000 ;
	skos:narrower	medtop:20000539 ;
	skos:narrower	medtop:20000540 ;
	skos:narrower	medtop:20000549 ;
	skos:narrower	medtop:20000550 ;
	skos:narrower	medtop:20000551 ;
	skos:narrower	medtop:20000553 ;
	skos:narrower	medtop:20000560 ;
	skos:narrower	medtop:20000563 .

medtop:20000539
	rdf:type skos:Concept ;
	skos:prefLabel	"club and association"@en-GB ;
	skos:definition	"Organisations joined by individuals because of similar interests"@en-GB ;
	skos:inScheme <http://cv.iptc.org/newscodes/mediatopic/>  ;
	ikos:created "2009-10-22T02:00:00+00:00"^^xsd:dateTime ;
	dct:created "2009-10-22T02:00:00+00:00"^^xsd:dateTime ;
	ikos:modified "2021-02-18T12:00:00+00:00"^^xsd:dateTime ;
	dct:modified "2021-02-18T12:00:00+00:00"^^xsd:dateTime  ;
	skos:exactMatch subj:10008000 ;
	skos:exactMatch <https://www.wikidata.org/entity/Q48204> ;
	skos:broader	medtop:20000538 .

medtop:20000540
	rdf:type skos:Concept ;
	skos:prefLabel	"game"@en-GB ;
	skos:definition	"Contests generally for one's amusement"@en-GB ;
	skos:inScheme <http://cv.iptc.org/newscodes/mediatopic/>  ;
	ikos:created "2009-10-22T02:00:00+00:00"^^xsd:dateTime ;
	dct:created "2009-10-22T02:00:00+00:00"^^xsd:dateTime ;
	ikos:modified "2021-02-18T12:00:00+00:00"^^xsd:dateTime ;
	dct:modified "2021-02-18T12:00:00+00:00"^^xsd:dateTime  ;
	skos:exactMatch subj:10001000 ;
	skos:exactMatch <https://www.wikidata.org/entity/Q11410> ;
	skos:broader	medtop:20000538 ;
	skos:narrower	medtop:20000541 ;
	skos:narrower	medtop:20000542 ;
	skos:narrower	medtop:20000543 ;
	skos:narrower	medtop:20000544 ;
	skos:narrower	medtop:20000545 ;
	skos:narrower	medtop:20000546 ;
	skos:narrower	medtop:20000547 ;
	skos:narrower	medtop:20000548 .

medtop:20000541
	rdf:type skos:Concept ;
	skos:prefLabel	"board game"@en-GB ;
	skos:definition	"A game played on a board"@en-GB ;
	skos:inScheme <http://cv.iptc.org/newscodes/mediatopic/>  ;
	ikos:created "2009-10-22T02:00:00+00:00"^^xsd:dateTime ;
	dct:created "2009-10-22T02:00:00+00:00"^^xsd:dateTime ;
	ikos:modified "2021-02-18T12:00:00+00:00"^^xsd:dateTime ;
	dct:modified "2021-02-18T12:00:00+00:00"^^xsd:dateTime  ;
	skos:broadMatch subj:10001000 ;
	skos:exactMatch <https://www.wikidata.org/entity/Q131436> ;
	skos:broader	medtop:20000540 .

medtop:20000542
	rdf:type skos:Concept ;
	skos:prefLabel	"card game"@en-GB ;
	skos:definition	"A game played with a pack of cards"@en-GB ;
	skos:inScheme <http://cv.iptc.org/newscodes/mediatopic/>  ;
	ikos:created "2009-10-22T02:00:00+00:00"^^xsd:dateTime ;
	dct:created "2009-10-22T02:00:00+00:00"^^xsd:dateTime ;
	ikos:modified "2021-02-18T12:00:00+00:00"^^xsd:dateTime ;
	dct:modified "2021-02-18T12:00:00+00:00"^^xsd:dateTime  ;
	skos:broadMatch subj:10001000 ;
	skos:exactMatch <https://www.wikidata.org/entity/Q142714> ;
	skos:broader	medtop:20000540 .

medtop:20000543
	rdf:type skos:Concept ;
	skos:prefLabel	"children's game"@en-GB ;
	skos:definition	"A game designed for and most often played by children"@en-GB ;
	skos:inScheme <http://cv.iptc.org/newscodes/mediatopic/>  ;
	ikos:created "2009-10-22T02:00:00+00:00"^^xsd:dateTime ;
	dct:created "2009-10-22T02:00:00+00:00"^^xsd:dateTime ;
	ikos:modified "2021-04-09T12:00:00+00:00"^^xsd:dateTime ;
	dct:modified "2021-04-09T12:00:00+00:00"^^xsd:dateTime  ;
	skos:broadMatch subj:10001000 ;
	skos:exactMatch <https://www.wikidata.org/entity/Q1509934> ;
	skos:broader	medtop:20000540 .

medtop:20000544
	rdf:type skos:Concept ;
	skos:prefLabel	"dice game"@en-GB ;
	skos:definition	"A game played using dice only"@en-GB ;
	skos:inScheme <http://cv.iptc.org/newscodes/mediatopic/>  ;
	ikos:created "2009-10-22T02:00:00+00:00"^^xsd:dateTime ;
	dct:created "2009-10-22T02:00:00+00:00"^^xsd:dateTime ;
	ikos:modified "2021-02-18T12:00:00+00:00"^^xsd:dateTime ;
	dct:modified "2021-02-18T12:00:00+00:00"^^xsd:dateTime  ;
	skos:broadMatch subj:10001000 ;
	skos:exactMatch <https://www.wikidata.org/entity/Q1515156> ;
	skos:broader	medtop:20000540 .

medtop:20000545
	rdf:type skos:Concept ;
	skos:prefLabel	"outdoor game"@en-GB ;
	skos:definition	"A game played in an open space"@en-GB ;
	skos:inScheme <http://cv.iptc.org/newscodes/mediatopic/>  ;
	ikos:created "2009-10-22T02:00:00+00:00"^^xsd:dateTime ;
	dct:created "2009-10-22T02:00:00+00:00"^^xsd:dateTime ;
	ikos:modified "2021-02-18T12:00:00+00:00"^^xsd:dateTime ;
	dct:modified "2021-02-18T12:00:00+00:00"^^xsd:dateTime  ;
	skos:broadMatch subj:10001000 ;
	skos:exactMatch <https://www.wikidata.org/entity/Q1499881> ;
	skos:broader	medtop:20000540 .

medtop:20000546
	rdf:type skos:Concept ;
	skos:prefLabel	"puzzle"@en-GB ;
	skos:definition	"A game played solving logic problems for entertainment"@en-GB ;
	skos:inScheme <http://cv.iptc.org/newscodes/mediatopic/>  ;
	ikos:created "2009-10-22T02:00:00+00:00"^^xsd:dateTime ;
	dct:created "2009-10-22T02:00:00+00:00"^^xsd:dateTime ;
	ikos:modified "2021-02-18T12:00:00+00:00"^^xsd:dateTime ;
	dct:modified "2021-02-18T12:00:00+00:00"^^xsd:dateTime  ;
	skos:broadMatch subj:10001000 ;
	skos:exactMatch <https://www.wikidata.org/entity/Q3177897> ;
	skos:broader	medtop:20000540 .

medtop:20000547
	rdf:type skos:Concept ;
	skos:prefLabel	"tile game"@en-GB ;
	skos:definition	"A game played using tiles"@en-GB ;
	skos:inScheme <http://cv.iptc.org/newscodes/mediatopic/>  ;
	ikos:created "2009-10-22T02:00:00+00:00"^^xsd:dateTime ;
	dct:created "2009-10-22T02:00:00+00:00"^^xsd:dateTime ;
	ikos:modified "2021-02-18T12:00:00+00:00"^^xsd:dateTime ;
	dct:modified "2021-02-18T12:00:00+00:00"^^xsd:dateTime  ;
	skos:broadMatch subj:10001000 ;
	skos:exactMatch <https://www.wikidata.org/entity/Q1272194> ;
	skos:broader	medtop:20000540 .

medtop:20000548
	rdf:type skos:Concept ;
	skos:prefLabel	"video game"@en-GB ;
	skos:definition	"A game played using a video display"@en-GB ;
	skos:inScheme <http://cv.iptc.org/newscodes/mediatopic/>  ;
	ikos:created "2009-10-22T02:00:00+00:00"^^xsd:dateTime ;
	dct:created "2009-10-22T02:00:00+00:00"^^xsd:dateTime ;
	ikos:modified "2021-02-18T12:00:00+00:00"^^xsd:dateTime ;
	dct:modified "2021-02-18T12:00:00+00:00"^^xsd:dateTime  ;
	skos:broadMatch subj:10001000 ;
	skos:exactMatch <https://www.wikidata.org/entity/Q7889> ;
	skos:broader	medtop:20000540 .

medtop:20000549
	rdf:type skos:Concept ;
	skos:prefLabel	"gaming and lottery"@en-GB ;
	skos:definition	"Gambling, often involving selection of sets of numbers one expects to come up"@en-GB ;
	skos:inScheme <http://cv.iptc.org/newscodes/mediatopic/>  ;
	ikos:created "2009-10-22T02:00:00+00:00"^^xsd:dateTime ;
	dct:created "2009-10-22T02:00:00+00:00"^^xsd:dateTime ;
	ikos:modified "2021-02-18T12:00:00+00:00"^^xsd:dateTime ;
	dct:modified "2021-02-18T12:00:00+00:00"^^xsd:dateTime  ;
	skos:exactMatch subj:10002000 ;
	skos:exactMatch <https://www.wikidata.org/entity/Q11416> ;
	skos:broader	medtop:20000538 .

medtop:20000550
	rdf:type skos:Concept ;
	skos:prefLabel	"hobby"@en-GB ;
	skos:definition	"Recreational pursuit"@en-GB ;
	skos:inScheme <http://cv.iptc.org/newscodes/mediatopic/>  ;
	ikos:created "2009-10-22T02:00:00+00:00"^^xsd:dateTime ;
	dct:created "2009-10-22T02:00:00+00:00"^^xsd:dateTime ;
	ikos:modified "2021-02-18T12:00:00+00:00"^^xsd:dateTime ;
	dct:modified "2021-02-18T12:00:00+00:00"^^xsd:dateTime  ;
	skos:exactMatch subj:10004000 ;
	skos:exactMatch <https://www.wikidata.org/entity/Q47728> ;
	skos:broader	medtop:20000538 ;
	skos:narrower	medtop:20000566 ;
	skos:narrower	medtop:20000567 ;
	skos:narrower	medtop:20000568 ;
	skos:narrower	medtop:20000571 ;
	skos:narrower	medtop:20001247 .

medtop:20000551
	rdf:type skos:Concept ;
	skos:prefLabel	"holiday"@en-GB ;
	skos:definition	"Time spent not at work for rest and relaxation"@en-GB ;
	skos:inScheme <http://cv.iptc.org/newscodes/mediatopic/>  ;
	ikos:created "2009-10-22T02:00:00+00:00"^^xsd:dateTime ;
	dct:created "2009-10-22T02:00:00+00:00"^^xsd:dateTime ;
	ikos:modified "2021-02-18T12:00:00+00:00"^^xsd:dateTime ;
	dct:modified "2021-02-18T12:00:00+00:00"^^xsd:dateTime  ;
	skos:broadMatch subj:10005000 ;
	skos:exactMatch <https://www.wikidata.org/entity/Q116213> ;
	skos:broader	medtop:20000538 ;
	skos:narrower	medtop:20000552 ;
	skos:narrower	medtop:20001270 .

medtop:20000552
	rdf:type skos:Concept ;
	skos:prefLabel	"public holiday"@en-GB ;
	skos:definition	"A day of celebration declared by a government"@en-GB ;
	skos:inScheme <http://cv.iptc.org/newscodes/mediatopic/>  ;
	ikos:created "2009-10-22T02:00:00+00:00"^^xsd:dateTime ;
	dct:created "2009-10-22T02:00:00+00:00"^^xsd:dateTime ;
	ikos:modified "2021-02-18T12:00:00+00:00"^^xsd:dateTime ;
	dct:modified "2021-02-18T12:00:00+00:00"^^xsd:dateTime  ;
	skos:closeMatch subj:10011000 ;
	skos:exactMatch <https://www.wikidata.org/entity/Q1197685> ;
	skos:broader	medtop:20000551 ;
	skos:narrower	medtop:20001267 ;
	skos:narrower	medtop:20001268 ;
	skos:narrower	medtop:20001269 .

medtop:20000553
	rdf:type skos:Concept ;
	skos:prefLabel	"leisure venue"@en-GB ;
	skos:definition	"A place where people go to be entertained or amused. For sporting events, use sport venue."@en-GB ;
	skos:inScheme <http://cv.iptc.org/newscodes/mediatopic/>  ;
	ikos:created "2009-10-22T02:00:00+00:00"^^xsd:dateTime ;
	dct:created "2009-10-22T02:00:00+00:00"^^xsd:dateTime ;
	ikos:modified "2021-05-05T12:00:00+00:00"^^xsd:dateTime ;
	dct:modified "2021-05-05T12:00:00+00:00"^^xsd:dateTime  ;
	skos:broadMatch subj:10000000 ;
	skos:exactMatch <https://www.wikidata.org/entity/Q18674739> ;
	skos:broader	medtop:20000538 ;
	skos:narrower	medtop:20000554 ;
	skos:narrower	medtop:20000555 ;
	skos:narrower	medtop:20000556 ;
	skos:narrower	medtop:20000557 ;
	skos:narrower	medtop:20000558 ;
	skos:narrower	medtop:20000559 ;
	skos:narrower	medtop:20001315 .

medtop:20000554
	rdf:type skos:Concept ;
	skos:prefLabel	"amusement park"@en-GB ;
	skos:definition	"A park providing various rides and entertainment attractions for both adults and children, including theme parks"@en-GB ;
	skos:inScheme <http://cv.iptc.org/newscodes/mediatopic/>  ;
	ikos:created "2009-10-22T02:00:00+00:00"^^xsd:dateTime ;
	dct:created "2009-10-22T02:00:00+00:00"^^xsd:dateTime ;
	ikos:modified "2021-02-18T12:00:00+00:00"^^xsd:dateTime ;
	dct:modified "2021-02-18T12:00:00+00:00"^^xsd:dateTime  ;
	skos:broadMatch subj:10000000 ;
	skos:exactMatch <https://www.wikidata.org/entity/Q194195> ;
	skos:broader	medtop:20000553 .

medtop:20000555
	rdf:type skos:Concept ;
	skos:prefLabel	"bar"@en-GB ;
	skos:definition	"A business where drinks are prepared and served to the public for consumption on the premises"@en-GB ;
	skos:inScheme <http://cv.iptc.org/newscodes/mediatopic/>  ;
	ikos:created "2009-10-22T02:00:00+00:00"^^xsd:dateTime ;
	dct:created "2009-10-22T02:00:00+00:00"^^xsd:dateTime ;
	ikos:modified "2021-02-18T12:00:00+00:00"^^xsd:dateTime ;
	dct:modified "2021-02-18T12:00:00+00:00"^^xsd:dateTime  ;
	skos:broadMatch subj:10000000 ;
	skos:exactMatch <https://www.wikidata.org/entity/Q187456> ;
	skos:broader	medtop:20000553 .

medtop:20000556
	rdf:type skos:Concept ;
	skos:prefLabel	"cafe"@en-GB ;
	skos:definition	"A small business where drinks and snacks are prepared and served - its specifics may depend on the local culture"@en-GB ;
	skos:inScheme <http://cv.iptc.org/newscodes/mediatopic/>  ;
	ikos:created "2009-10-22T02:00:00+00:00"^^xsd:dateTime ;
	dct:created "2009-10-22T02:00:00+00:00"^^xsd:dateTime ;
	ikos:modified "2021-02-18T12:00:00+00:00"^^xsd:dateTime ;
	dct:modified "2021-02-18T12:00:00+00:00"^^xsd:dateTime  ;
	skos:broadMatch subj:10000000 ;
	skos:exactMatch <https://www.wikidata.org/entity/Q30022> ;
	skos:broader	medtop:20000553 .

medtop:20000557
	rdf:type skos:Concept ;
	skos:prefLabel	"nightclub"@en-GB ;
	skos:definition	"A commercial establishment providing music, or other entertainment along with food and drink to selected clientele"@en-GB ;
	skos:inScheme <http://cv.iptc.org/newscodes/mediatopic/>  ;
	ikos:created "2009-10-22T02:00:00+00:00"^^xsd:dateTime ;
	dct:created "2009-10-22T02:00:00+00:00"^^xsd:dateTime ;
	ikos:modified "2021-02-18T12:00:00+00:00"^^xsd:dateTime ;
	dct:modified "2021-02-18T12:00:00+00:00"^^xsd:dateTime  ;
	skos:exactMatch subj:01023000 ;
	skos:exactMatch <https://www.wikidata.org/entity/Q622425> ;
	skos:broader	medtop:20000553 .

medtop:20000558
	rdf:type skos:Concept ;
	skos:prefLabel	"restaurant"@en-GB ;
	skos:definition	"A business where meals are prepared and served to the public"@en-GB ;
	skos:inScheme <http://cv.iptc.org/newscodes/mediatopic/>  ;
	ikos:created "2009-10-22T02:00:00+00:00"^^xsd:dateTime ;
	dct:created "2009-10-22T02:00:00+00:00"^^xsd:dateTime ;
	ikos:modified "2021-02-18T12:00:00+00:00"^^xsd:dateTime ;
	dct:modified "2021-02-18T12:00:00+00:00"^^xsd:dateTime  ;
	skos:broadMatch subj:10000000 ;
	skos:exactMatch <https://www.wikidata.org/entity/Q11707> ;
	skos:broader	medtop:20000553 .

medtop:20000559
	rdf:type skos:Concept ;
	skos:prefLabel	"sports facilities"@en-GB ;
	skos:definition	"Gymnasiums, stadiums or arenas where sports events take place"@en-GB ;
	skos:inScheme <http://cv.iptc.org/newscodes/mediatopic/>  ;
	ikos:created "2009-10-22T02:00:00+00:00"^^xsd:dateTime ;
	dct:created "2009-10-22T02:00:00+00:00"^^xsd:dateTime ;
	ikos:modified "2021-02-18T12:00:00+00:00"^^xsd:dateTime ;
	dct:modified "2021-02-18T12:00:00+00:00"^^xsd:dateTime  ; 
	ikos:retired "2021-02-18T12:00:00+00:00"^^xsd:dateTime ;
	skos:broadMatch subj:10000000 ;
	skos:exactMatch <https://www.wikidata.org/entity/Q1076486> ;
	skos:broader	medtop:20000553 .

medtop:20000560
	rdf:type skos:Concept ;
	skos:prefLabel	"outdoor recreational activities"@en-GB ;
	skos:definition	"Leisure activities engaged in the outdoors, most commonly in natural settings"@en-GB ;
	skos:inScheme <http://cv.iptc.org/newscodes/mediatopic/>  ;
	ikos:created "2009-10-22T02:00:00+00:00"^^xsd:dateTime ;
	dct:created "2009-10-22T02:00:00+00:00"^^xsd:dateTime ;
	ikos:modified "2021-02-18T12:00:00+00:00"^^xsd:dateTime ;
	dct:modified "2021-02-18T12:00:00+00:00"^^xsd:dateTime  ;
	skos:broadMatch subj:10000000 ;
	skos:exactMatch <https://www.wikidata.org/entity/Q184872> ;
	skos:broader	medtop:20000538 ;
	skos:narrower	medtop:20000561 ;
	skos:narrower	medtop:20000562 ;
	skos:narrower	medtop:20000917 ;
	skos:narrower	medtop:20001142 ;
	skos:narrower	medtop:20001241 .

medtop:20000561
	rdf:type skos:Concept ;
	skos:prefLabel	"fishing"@en-GB ;
	skos:definition	"A recreational activity involving the use of baits, lures, weapons and traps for the capture of aquatic species."@en-GB ;
	skos:inScheme <http://cv.iptc.org/newscodes/mediatopic/>  ;
	ikos:created "2009-10-22T02:00:00+00:00"^^xsd:dateTime ;
	dct:created "2009-10-22T02:00:00+00:00"^^xsd:dateTime ;
	ikos:modified "2021-02-18T12:00:00+00:00"^^xsd:dateTime ;
	dct:modified "2021-02-18T12:00:00+00:00"^^xsd:dateTime  ;
	skos:exactMatch subj:10013000 ;
	skos:exactMatch <https://www.wikidata.org/entity/Q14373> ;
	skos:broader	medtop:20000560 .

medtop:20000562
	rdf:type skos:Concept ;
	skos:prefLabel	"hunting"@en-GB ;
	skos:definition	"An activity involving the use of weapons or traps for the capturing of animals"@en-GB ;
	skos:inScheme <http://cv.iptc.org/newscodes/mediatopic/>  ;
	ikos:created "2009-10-22T02:00:00+00:00"^^xsd:dateTime ;
	dct:created "2009-10-22T02:00:00+00:00"^^xsd:dateTime ;
	ikos:modified "2021-02-18T12:00:00+00:00"^^xsd:dateTime ;
	dct:modified "2021-02-18T12:00:00+00:00"^^xsd:dateTime  ;
	skos:exactMatch subj:10012000 ;
	skos:exactMatch <https://www.wikidata.org/entity/Q36963> ;
	skos:broader	medtop:20000560 .

medtop:20000563
	rdf:type skos:Concept ;
	skos:prefLabel	"travel and tourism"@en-GB ;
	skos:definition	"Spending time away from home in pursuit of recreation, relaxation or pleasure"@en-GB ;
	skos:inScheme <http://cv.iptc.org/newscodes/mediatopic/>  ;
	ikos:created "2009-10-22T02:00:00+00:00"^^xsd:dateTime ;
	dct:created "2009-10-22T02:00:00+00:00"^^xsd:dateTime ;
	ikos:modified "2021-02-18T12:00:00+00:00"^^xsd:dateTime ;
	dct:modified "2021-02-18T12:00:00+00:00"^^xsd:dateTime  ;
	skos:broadMatch subj:10000000 ;
	skos:exactMatch <https://www.wikidata.org/entity/Q61509> ;
	skos:broader	medtop:20000538 ;
	skos:narrower	medtop:20000564 .

medtop:20000564
	rdf:type skos:Concept ;
	skos:prefLabel	"tourism"@en-GB ;
	skos:definition	"Leisure travel involving visits to a number of locations and/or countries over an extended period of time, often as part of an organised group"@en-GB ;
	skos:inScheme <http://cv.iptc.org/newscodes/mediatopic/>  ;
	ikos:created "2009-10-22T02:00:00+00:00"^^xsd:dateTime ;
	dct:created "2009-10-22T02:00:00+00:00"^^xsd:dateTime ;
	ikos:modified "2021-02-18T12:00:00+00:00"^^xsd:dateTime ;
	dct:modified "2021-02-18T12:00:00+00:00"^^xsd:dateTime  ; 
	ikos:retired "2019-07-22T12:00:00+00:00"^^xsd:dateTime ;
	skos:closeMatch subj:10006000 ;
	skos:exactMatch <https://www.wikidata.org/entity/Q49389> ;
	skos:broader	medtop:20000563 .

medtop:20000565
	rdf:type skos:Concept ;
	skos:prefLabel	"lifestyle"@en-GB ;
	skos:definition	"The way in which a person lives, including their style and possessions"@en-GB ;
	skos:inScheme <http://cv.iptc.org/newscodes/mediatopic/>  ;
	ikos:created "2009-10-22T02:00:00+00:00"^^xsd:dateTime ;
	dct:created "2009-10-22T02:00:00+00:00"^^xsd:dateTime ;
	ikos:modified "2021-02-18T12:00:00+00:00"^^xsd:dateTime ;
	dct:modified "2021-02-18T12:00:00+00:00"^^xsd:dateTime  ;
	skos:broadMatch subj:10000000 ;
	skos:exactMatch <https://www.wikidata.org/entity/Q32090> ;
	skos:broader	medtop:10000000 ;
	skos:narrower	medtop:20000569 ;
	skos:narrower	medtop:20000570 ;
	skos:narrower	medtop:20000572 ;
	skos:narrower	medtop:20001143 .

medtop:20000566
	rdf:type skos:Concept ;
	skos:prefLabel	"automobile enthusiasm"@en-GB ;
	skos:definition	"Interest in new and classic cars"@en-GB ;
	skos:inScheme <http://cv.iptc.org/newscodes/mediatopic/>  ;
	ikos:created "2009-10-22T02:00:00+00:00"^^xsd:dateTime ;
	dct:created "2009-10-22T02:00:00+00:00"^^xsd:dateTime ;
	ikos:modified "2021-02-18T12:00:00+00:00"^^xsd:dateTime ;
	dct:modified "2021-02-18T12:00:00+00:00"^^xsd:dateTime  ;
	skos:broadMatch subj:10000000 ;
	skos:broader	medtop:20000550 .

medtop:20000567
	rdf:type skos:Concept ;
	skos:prefLabel	"bicycle enthusiasm"@en-GB ;
	skos:definition	"Interest in new and classic manpowered cycles"@en-GB ;
	skos:inScheme <http://cv.iptc.org/newscodes/mediatopic/>  ;
	ikos:created "2009-10-22T02:00:00+00:00"^^xsd:dateTime ;
	dct:created "2009-10-22T02:00:00+00:00"^^xsd:dateTime ;
	ikos:modified "2021-02-18T12:00:00+00:00"^^xsd:dateTime ;
	dct:modified "2021-02-18T12:00:00+00:00"^^xsd:dateTime  ;
	skos:broadMatch subj:10000000 ;
	skos:broader	medtop:20000550 .

medtop:20000568
	rdf:type skos:Concept ;
	skos:prefLabel	"food and drink enthusiasm"@en-GB ;
	skos:definition	"Interest in eating and drinking"@en-GB ;
	skos:inScheme <http://cv.iptc.org/newscodes/mediatopic/>  ;
	ikos:created "2009-10-22T02:00:00+00:00"^^xsd:dateTime ;
	dct:created "2009-10-22T02:00:00+00:00"^^xsd:dateTime ;
	ikos:modified "2021-02-18T12:00:00+00:00"^^xsd:dateTime ;
	dct:modified "2021-02-18T12:00:00+00:00"^^xsd:dateTime  ;
	skos:broadMatch subj:10000000 ;
	skos:broader	medtop:20000550 ;
	skos:narrower	medtop:20001253 ;
	skos:narrower	medtop:20001254 .

medtop:20000569
	rdf:type skos:Concept ;
	skos:prefLabel	"organic food"@en-GB ;
	skos:definition	"Food which is grown using no artificial fertilisers or chemical compounds"@en-GB ;
	skos:inScheme <http://cv.iptc.org/newscodes/mediatopic/>  ;
	ikos:created "2009-10-22T02:00:00+00:00"^^xsd:dateTime ;
	dct:created "2009-10-22T02:00:00+00:00"^^xsd:dateTime ;
	ikos:modified "2021-02-18T12:00:00+00:00"^^xsd:dateTime ;
	dct:modified "2021-02-18T12:00:00+00:00"^^xsd:dateTime  ;
	skos:exactMatch subj:10003001 ;
	skos:exactMatch <https://www.wikidata.org/entity/Q380778> ;
	skos:broader	medtop:20000565 .

medtop:20000570
	rdf:type skos:Concept ;
	skos:prefLabel	"house and home"@en-GB ;
	skos:definition	"Interest in maintaining and decorating one's home"@en-GB ;
	skos:inScheme <http://cv.iptc.org/newscodes/mediatopic/>  ;
	ikos:created "2009-10-22T02:00:00+00:00"^^xsd:dateTime ;
	dct:created "2009-10-22T02:00:00+00:00"^^xsd:dateTime ;
	ikos:modified "2021-02-18T12:00:00+00:00"^^xsd:dateTime ;
	dct:modified "2021-02-18T12:00:00+00:00"^^xsd:dateTime  ;
	skos:broadMatch subj:10000000 ;
	skos:broader	medtop:20000565 ;
	skos:narrower	medtop:20001255 ;
	skos:narrower	medtop:20001256 ;
	skos:narrower	medtop:20001257 .

medtop:20000571
	rdf:type skos:Concept ;
	skos:prefLabel	"motorcycle enthusiasm"@en-GB ;
	skos:definition	"Interest in new and classic motor-powered cycles"@en-GB ;
	skos:inScheme <http://cv.iptc.org/newscodes/mediatopic/>  ;
	ikos:created "2009-10-22T02:00:00+00:00"^^xsd:dateTime ;
	dct:created "2009-10-22T02:00:00+00:00"^^xsd:dateTime ;
	ikos:modified "2021-05-05T12:00:00+00:00"^^xsd:dateTime ;
	dct:modified "2021-05-05T12:00:00+00:00"^^xsd:dateTime  ;
	skos:broadMatch subj:10000000 ;
	skos:broader	medtop:20000550 .

medtop:20000572
	rdf:type skos:Concept ;
	skos:prefLabel	"trend"@en-GB ;
	skos:definition	"Interest in what is considered hip or popular at a certain point in time"@en-GB ;
	skos:inScheme <http://cv.iptc.org/newscodes/mediatopic/>  ;
	ikos:created "2009-10-22T02:00:00+00:00"^^xsd:dateTime ;
	dct:created "2009-10-22T02:00:00+00:00"^^xsd:dateTime ;
	ikos:modified "2021-02-18T12:00:00+00:00"^^xsd:dateTime ;
	dct:modified "2021-02-18T12:00:00+00:00"^^xsd:dateTime  ;
	skos:broadMatch subj:10000000 ;
	skos:exactMatch <https://www.wikidata.org/entity/Q28972120> ;
	skos:broader	medtop:20000565 ;
	skos:narrower	medtop:20001250 .

medtop:20000574
	rdf:type skos:Concept ;
	skos:prefLabel	"election"@en-GB ;
	skos:definition	"The selection of representatives by the casting of votes"@en-GB ;
	skos:inScheme <http://cv.iptc.org/newscodes/mediatopic/>  ;
	ikos:created "2009-10-22T02:00:00+00:00"^^xsd:dateTime ;
	dct:created "2009-10-22T02:00:00+00:00"^^xsd:dateTime ;
	ikos:modified "2021-07-12T12:00:00+00:00"^^xsd:dateTime ;
	dct:modified "2021-07-12T12:00:00+00:00"^^xsd:dateTime  ;
	skos:exactMatch subj:11003000 ;
	skos:exactMatch <https://www.wikidata.org/entity/Q40231> ;
	skos:broader	medtop:11000000 ;
	skos:narrower	medtop:20000575 ;
	skos:narrower	medtop:20000576 ;
	skos:narrower	medtop:20000577 ;
	skos:narrower	medtop:20000578 ;
	skos:narrower	medtop:20000579 ;
	skos:narrower	medtop:20000580 ;
	skos:narrower	medtop:20000582 ;
	skos:narrower	medtop:20000583 ;
	skos:narrower	medtop:20000584 ;
	skos:narrower	medtop:20000585 ;
	skos:narrower	medtop:20000586 ;
	skos:narrower	medtop:20001263 ;
	skos:narrower	medtop:20001266 .

medtop:20000575
	rdf:type skos:Concept ;
	skos:prefLabel	"citizens' initiative and recall"@en-GB ;
	skos:definition	"Political suggestions by non-government officials for corrective action, or for changes in existing rules and regulations"@en-GB ;
	skos:inScheme <http://cv.iptc.org/newscodes/mediatopic/>  ;
	ikos:created "2009-10-22T02:00:00+00:00"^^xsd:dateTime ;
	dct:created "2009-10-22T02:00:00+00:00"^^xsd:dateTime ;
	ikos:modified "2021-05-12T12:00:00+00:00"^^xsd:dateTime ;
	dct:modified "2021-05-12T12:00:00+00:00"^^xsd:dateTime  ;
	skos:exactMatch subj:11018000 ;
	skos:broader	medtop:20000574 .

medtop:20000576
	rdf:type skos:Concept ;
	skos:prefLabel	"electoral system"@en-GB ;
	skos:definition	"Voting systems"@en-GB ;
	skos:inScheme <http://cv.iptc.org/newscodes/mediatopic/>  ;
	ikos:created "2009-10-22T02:00:00+00:00"^^xsd:dateTime ;
	dct:created "2009-10-22T02:00:00+00:00"^^xsd:dateTime ;
	ikos:modified "2021-02-18T12:00:00+00:00"^^xsd:dateTime ;
	dct:modified "2021-02-18T12:00:00+00:00"^^xsd:dateTime  ;
	skos:broadMatch subj:11000000 ;
	skos:exactMatch <https://www.wikidata.org/entity/Q182985> ;
	skos:broader	medtop:20000574 .

medtop:20000577
	rdf:type skos:Concept ;
	skos:prefLabel	"intergovernmental elections"@en-GB ;
	skos:definition	"Choosing individuals for the government of an international organization, such as the United Nations, European Union, NATO and World Bank"@en-GB ;
	skos:inScheme <http://cv.iptc.org/newscodes/mediatopic/>  ;
	ikos:created "2009-10-22T02:00:00+00:00"^^xsd:dateTime ;
	dct:created "2009-10-22T02:00:00+00:00"^^xsd:dateTime ;
	ikos:modified "2021-07-12T12:00:00+00:00"^^xsd:dateTime ;
	dct:modified "2021-07-12T12:00:00+00:00"^^xsd:dateTime  ;
	skos:broadMatch subj:11000000 ;
	skos:exactMatch <https://www.wikidata.org/entity/Q8550213> ;
	skos:broader	medtop:20000574 .

medtop:20000578
	rdf:type skos:Concept ;
	skos:prefLabel	"local elections"@en-GB ;
	skos:definition	"Choosing individuals for government at the basic level, whether city, village or county"@en-GB ;
	skos:inScheme <http://cv.iptc.org/newscodes/mediatopic/>  ;
	ikos:created "2009-10-22T02:00:00+00:00"^^xsd:dateTime ;
	dct:created "2009-10-22T02:00:00+00:00"^^xsd:dateTime ;
	ikos:modified "2021-07-12T12:00:00+00:00"^^xsd:dateTime ;
	dct:modified "2021-07-12T12:00:00+00:00"^^xsd:dateTime  ;
	skos:exactMatch subj:11003006 ;
	skos:exactMatch <https://www.wikidata.org/entity/Q15966540> ;
	skos:broader	medtop:20000574 .

medtop:20000579
	rdf:type skos:Concept ;
	skos:prefLabel	"national elections"@en-GB ;
	skos:definition	"Choosing individuals for government at a national level"@en-GB ;
	skos:inScheme <http://cv.iptc.org/newscodes/mediatopic/>  ;
	ikos:created "2009-10-22T02:00:00+00:00"^^xsd:dateTime ;
	dct:created "2009-10-22T02:00:00+00:00"^^xsd:dateTime ;
	ikos:modified "2021-07-12T12:00:00+00:00"^^xsd:dateTime ;
	dct:modified "2021-07-12T12:00:00+00:00"^^xsd:dateTime  ;
	skos:exactMatch subj:11003004 ;
	skos:exactMatch <https://www.wikidata.org/entity/Q1076105> ;
	skos:broader	medtop:20000574 .

medtop:20000580
	rdf:type skos:Concept ;
	skos:prefLabel	"political campaigns"@en-GB ;
	skos:definition	"Campaigns for public office"@en-GB ;
	skos:inScheme <http://cv.iptc.org/newscodes/mediatopic/>  ;
	ikos:created "2009-10-22T02:00:00+00:00"^^xsd:dateTime ;
	dct:created "2009-10-22T02:00:00+00:00"^^xsd:dateTime ;
	ikos:modified "2021-02-18T12:00:00+00:00"^^xsd:dateTime ;
	dct:modified "2021-02-18T12:00:00+00:00"^^xsd:dateTime  ;
	skos:exactMatch subj:11003002 ;
	skos:exactMatch <https://www.wikidata.org/entity/Q847301> ;
	skos:broader	medtop:20000574 ;
	skos:narrower	medtop:20000581 .

medtop:20000581
	rdf:type skos:Concept ;
	skos:prefLabel	"campaign finance"@en-GB ;
	skos:definition	"The money that makes campaigns for public office possible"@en-GB ;
	skos:inScheme <http://cv.iptc.org/newscodes/mediatopic/>  ;
	ikos:created "2009-10-22T02:00:00+00:00"^^xsd:dateTime ;
	dct:created "2009-10-22T02:00:00+00:00"^^xsd:dateTime ;
	ikos:modified "2021-02-18T12:00:00+00:00"^^xsd:dateTime ;
	dct:modified "2021-02-18T12:00:00+00:00"^^xsd:dateTime  ;
	skos:exactMatch subj:11003003 ;
	skos:exactMatch <https://www.wikidata.org/entity/Q1352232> ;
	skos:broader	medtop:20000580 .

medtop:20000582
	rdf:type skos:Concept ;
	skos:prefLabel	"political candidates"@en-GB ;
	skos:definition	"Individuals who are chosen to stand for office"@en-GB ;
	skos:inScheme <http://cv.iptc.org/newscodes/mediatopic/>  ;
	ikos:created "2009-10-22T02:00:00+00:00"^^xsd:dateTime ;
	dct:created "2009-10-22T02:00:00+00:00"^^xsd:dateTime ;
	ikos:modified "2021-02-18T12:00:00+00:00"^^xsd:dateTime ;
	dct:modified "2021-02-18T12:00:00+00:00"^^xsd:dateTime  ;
	skos:exactMatch subj:11003001 ;
	skos:exactMatch <https://www.wikidata.org/entity/Q19772737> ;
	skos:broader	medtop:20000574 .

medtop:20000583
	rdf:type skos:Concept ;
	skos:prefLabel	"primary elections"@en-GB ;
	skos:definition	"Preliminary elections on a local or regional basis leading up to a regional or national election"@en-GB ;
	skos:inScheme <http://cv.iptc.org/newscodes/mediatopic/>  ;
	ikos:created "2009-10-22T02:00:00+00:00"^^xsd:dateTime ;
	dct:created "2009-10-22T02:00:00+00:00"^^xsd:dateTime ;
	ikos:modified "2021-07-12T12:00:00+00:00"^^xsd:dateTime ;
	dct:modified "2021-07-12T12:00:00+00:00"^^xsd:dateTime  ;
	skos:exactMatch subj:11003010 ;
	skos:exactMatch <https://www.wikidata.org/entity/Q669262> ;
	skos:broader	medtop:20000574 .

medtop:20000584
	rdf:type skos:Concept ;
	skos:prefLabel	"referenda"@en-GB ;
	skos:definition	"Political proposals, laws and actions suggested by non-government officials to be voted on by the entire voting body"@en-GB ;
	skos:inScheme <http://cv.iptc.org/newscodes/mediatopic/>  ;
	ikos:created "2009-10-22T02:00:00+00:00"^^xsd:dateTime ;
	dct:created "2009-10-22T02:00:00+00:00"^^xsd:dateTime ;
	ikos:modified "2021-02-18T12:00:00+00:00"^^xsd:dateTime ;
	dct:modified "2021-02-18T12:00:00+00:00"^^xsd:dateTime  ;
	skos:exactMatch subj:11019000 ;
	skos:exactMatch <https://www.wikidata.org/entity/Q43109> ;
	skos:broader	medtop:20000574 .

medtop:20000585
	rdf:type skos:Concept ;
	skos:prefLabel	"regional elections"@en-GB ;
	skos:definition	"Choosing individuals for government at a regional level"@en-GB ;
	skos:inScheme <http://cv.iptc.org/newscodes/mediatopic/>  ;
	ikos:created "2009-10-22T02:00:00+00:00"^^xsd:dateTime ;
	dct:created "2009-10-22T02:00:00+00:00"^^xsd:dateTime ;
	ikos:modified "2021-07-12T12:00:00+00:00"^^xsd:dateTime ;
	dct:modified "2021-07-12T12:00:00+00:00"^^xsd:dateTime  ;
	skos:exactMatch subj:11003005 ;
	skos:exactMatch <https://www.wikidata.org/entity/Q15966540> ;
	skos:broader	medtop:20000574 .

medtop:20000586
	rdf:type skos:Concept ;
	skos:prefLabel	"voting"@en-GB ;
	skos:definition	"The act of selecting an individual you would like to represent your interests in government"@en-GB ;
	skos:inScheme <http://cv.iptc.org/newscodes/mediatopic/>  ;
	ikos:created "2009-10-22T02:00:00+00:00"^^xsd:dateTime ;
	dct:created "2009-10-22T02:00:00+00:00"^^xsd:dateTime ;
	ikos:modified "2021-02-18T12:00:00+00:00"^^xsd:dateTime ;
	dct:modified "2021-02-18T12:00:00+00:00"^^xsd:dateTime  ;
	skos:exactMatch subj:11003007 ;
	skos:exactMatch <https://www.wikidata.org/entity/Q189760> ;
	skos:broader	medtop:20000574 .

medtop:20000587
	rdf:type skos:Concept ;
	skos:prefLabel	"fundamental rights"@en-GB ;
	skos:definition	"The political, social and economic rights to which all creatures are entitled, usually upheld by law."@en-GB ;
	skos:inScheme <http://cv.iptc.org/newscodes/mediatopic/>  ;
	ikos:created "2009-10-22T02:00:00+00:00"^^xsd:dateTime ;
	dct:created "2009-10-22T02:00:00+00:00"^^xsd:dateTime ;
	ikos:modified "2021-02-18T12:00:00+00:00"^^xsd:dateTime ;
	dct:modified "2021-02-18T12:00:00+00:00"^^xsd:dateTime  ;
	skos:exactMatch <https://www.wikidata.org/entity/Q3237872> ;
	skos:broadMatch subj:02007000 ;
	skos:broader	medtop:11000000 ;
	skos:narrower	medtop:20000120 ;
	skos:narrower	medtop:20000588 ;
	skos:narrower	medtop:20000590 ;
	skos:narrower	medtop:20000591 ;
	skos:narrower	medtop:20000592 ;
	skos:narrower	medtop:20001300 ;
	skos:narrower	medtop:20001326 .

medtop:20000588
	rdf:type skos:Concept ;
	skos:prefLabel	"censorship and freedom of speech"@en-GB ;
	skos:definition	"Attempts by any group to control freedoms of speech, religion, and ideas distributed in print, graphics, cyberspace and other ways. Does not include official standards such as cinema ratings, advertising and broadcast standards."@en-GB ;
	skos:inScheme <http://cv.iptc.org/newscodes/mediatopic/>  ;
	ikos:created "2009-10-22T02:00:00+00:00"^^xsd:dateTime ;
	dct:created "2009-10-22T02:00:00+00:00"^^xsd:dateTime ;
	ikos:modified "2021-02-18T12:00:00+00:00"^^xsd:dateTime ;
	dct:modified "2021-02-18T12:00:00+00:00"^^xsd:dateTime  ;
	skos:exactMatch subj:11023000 ;
	skos:exactMatch <https://www.wikidata.org/entity/Q543> ;
	skos:broader	medtop:20000587 .

medtop:20000590
	rdf:type skos:Concept ;
	skos:prefLabel	"freedom of religion"@en-GB ;
	skos:definition	"Religious rights and freedoms, pressure and intimidation of believers, censorship in mass media, activities of government bodies, journalistic associations and/or organisations and other NGOs in regard to freedom of belief and practice"@en-GB ;
	skos:inScheme <http://cv.iptc.org/newscodes/mediatopic/>  ;
	ikos:created "2009-10-22T02:00:00+00:00"^^xsd:dateTime ;
	dct:created "2009-10-22T02:00:00+00:00"^^xsd:dateTime ;
	ikos:modified "2021-05-05T12:00:00+00:00"^^xsd:dateTime ;
	dct:modified "2021-05-05T12:00:00+00:00"^^xsd:dateTime  ;
	skos:exactMatch subj:11026000 ;
	skos:exactMatch <https://www.wikidata.org/entity/Q171899> ;
	skos:broader	medtop:20000587 .

medtop:20000591
	rdf:type skos:Concept ;
	skos:prefLabel	"freedom of the press"@en-GB ;
	skos:definition	"Mass media rights and freedoms, pressure and intimidation of the journalists, censorship in mass media, activities of government bodies, journalistic associations and/or organisations and other NGOs in regards to press freedom"@en-GB ;
	skos:inScheme <http://cv.iptc.org/newscodes/mediatopic/>  ;
	ikos:created "2009-10-22T02:00:00+00:00"^^xsd:dateTime ;
	dct:created "2009-10-22T02:00:00+00:00"^^xsd:dateTime ;
	ikos:modified "2021-02-18T12:00:00+00:00"^^xsd:dateTime ;
	dct:modified "2021-02-18T12:00:00+00:00"^^xsd:dateTime  ;
	skos:exactMatch subj:11025000 ;
	skos:exactMatch <https://www.wikidata.org/entity/Q22688> ;
	skos:broader	medtop:20000587 .

medtop:20000592
	rdf:type skos:Concept ;
	skos:prefLabel	"human rights"@en-GB ;
	skos:definition	"Rights entitled to be enjoyed by all citizens universally"@en-GB ;
	skos:inScheme <http://cv.iptc.org/newscodes/mediatopic/>  ;
	ikos:created "2009-10-22T02:00:00+00:00"^^xsd:dateTime ;
	dct:created "2009-10-22T02:00:00+00:00"^^xsd:dateTime ;
	ikos:modified "2021-02-18T12:00:00+00:00"^^xsd:dateTime ;
	dct:modified "2021-02-18T12:00:00+00:00"^^xsd:dateTime  ;
	skos:exactMatch subj:11007000 ;
	skos:exactMatch <https://www.wikidata.org/entity/Q8458> ;
	skos:broader	medtop:20000587 .

medtop:20000593
	rdf:type skos:Concept ;
	skos:prefLabel	"government"@en-GB ;
	skos:definition	"The system for ruling a country"@en-GB ;
	skos:inScheme <http://cv.iptc.org/newscodes/mediatopic/>  ;
	ikos:created "2009-10-22T02:00:00+00:00"^^xsd:dateTime ;
	dct:created "2009-10-22T02:00:00+00:00"^^xsd:dateTime ;
	ikos:modified "2021-02-18T12:00:00+00:00"^^xsd:dateTime ;
	dct:modified "2021-02-18T12:00:00+00:00"^^xsd:dateTime  ;
	skos:exactMatch subj:11006000 ;
	skos:exactMatch <https://www.wikidata.org/entity/Q7188> ;
	skos:broader	medtop:11000000 ;
	skos:narrower	medtop:20000594 ;
	skos:narrower	medtop:20000597 ;
	skos:narrower	medtop:20000598 ;
	skos:narrower	medtop:20000605 ;
	skos:narrower	medtop:20000606 ;
	skos:narrower	medtop:20000607 ;
	skos:narrower	medtop:20000609 ;
	skos:narrower	medtop:20000610 ;
	skos:narrower	medtop:20000611 ;
	skos:narrower	medtop:20000612 ;
	skos:narrower	medtop:20000613 ;
	skos:narrower	medtop:20000614 ;
	skos:narrower	medtop:20000615 ;
	skos:narrower	medtop:20000618 ;
	skos:narrower	medtop:20001173 ;
	skos:narrower	medtop:20001259 ;
	skos:narrower	medtop:20001260 ;
	skos:narrower	medtop:20001261 ;
	skos:narrower	medtop:20001262 .

medtop:20000594
	rdf:type skos:Concept ;
	skos:prefLabel	"civil and public service"@en-GB ;
	skos:definition	"The paid service by civilians for the government, and the often non-paid service of individuals for the benefit of others (public service)"@en-GB ;
	skos:inScheme <http://cv.iptc.org/newscodes/mediatopic/>  ;
	ikos:created "2009-10-22T02:00:00+00:00"^^xsd:dateTime ;
	dct:created "2009-10-22T02:00:00+00:00"^^xsd:dateTime ;
	ikos:modified "2021-05-05T12:00:00+00:00"^^xsd:dateTime ;
	dct:modified "2021-05-05T12:00:00+00:00"^^xsd:dateTime  ;
	skos:exactMatch subj:11006001 ;
	skos:exactMatch <https://www.wikidata.org/entity/Q11771944> ;
	skos:broader	medtop:20000593 ;
	skos:narrower	medtop:20000595 ;
	skos:narrower	medtop:20000596 ;
	skos:narrower	medtop:20001144 .

medtop:20000595
	rdf:type skos:Concept ;
	skos:prefLabel	"public employees"@en-GB ;
	skos:definition	"People employed by a government at all levels"@en-GB ;
	skos:inScheme <http://cv.iptc.org/newscodes/mediatopic/>  ;
	ikos:created "2009-10-22T02:00:00+00:00"^^xsd:dateTime ;
	dct:created "2009-10-22T02:00:00+00:00"^^xsd:dateTime ;
	ikos:modified "2021-02-18T12:00:00+00:00"^^xsd:dateTime ;
	dct:modified "2021-02-18T12:00:00+00:00"^^xsd:dateTime  ;
	skos:exactMatch subj:11006010 ;
	skos:exactMatch <https://www.wikidata.org/entity/Q212238> ;
	skos:broader	medtop:20000594 .

medtop:20000596
	rdf:type skos:Concept ;
	skos:prefLabel	"public officials"@en-GB ;
	skos:definition	"Individuals, usually elected, who are in public service or commonly in the public eye."@en-GB ;
	skos:inScheme <http://cv.iptc.org/newscodes/mediatopic/>  ;
	ikos:created "2009-10-22T02:00:00+00:00"^^xsd:dateTime ;
	dct:created "2009-10-22T02:00:00+00:00"^^xsd:dateTime ;
	ikos:modified "2021-02-18T12:00:00+00:00"^^xsd:dateTime ;
	dct:modified "2021-02-18T12:00:00+00:00"^^xsd:dateTime  ;
	skos:exactMatch subj:11006008 ;
	skos:exactMatch <https://www.wikidata.org/entity/Q599151> ;
	skos:broader	medtop:20000594 .

medtop:20000597
	rdf:type skos:Concept ;
	skos:prefLabel	"constitution (law)"@en-GB ;
	skos:definition	"Usually a written document setting forth the operations of a government and the rights of the citizens therein"@en-GB ;
	skos:inScheme <http://cv.iptc.org/newscodes/mediatopic/>  ;
	ikos:created "2009-10-22T02:00:00+00:00"^^xsd:dateTime ;
	dct:created "2009-10-22T02:00:00+00:00"^^xsd:dateTime ;
	ikos:modified "2021-02-18T12:00:00+00:00"^^xsd:dateTime ;
	dct:modified "2021-02-18T12:00:00+00:00"^^xsd:dateTime  ;
	skos:exactMatch subj:11015000 ;
	skos:exactMatch <https://www.wikidata.org/entity/Q7755> ;
	skos:broader	medtop:20000593 .

medtop:20000598
	rdf:type skos:Concept ;
	skos:prefLabel	"defence"@en-GB ;
	skos:definition	"Anything involving the protection of one's own country"@en-GB ;
	skos:inScheme <http://cv.iptc.org/newscodes/mediatopic/>  ;
	ikos:created "2009-10-22T02:00:00+00:00"^^xsd:dateTime ;
	dct:created "2009-10-22T02:00:00+00:00"^^xsd:dateTime ;
	ikos:modified "2021-02-18T12:00:00+00:00"^^xsd:dateTime ;
	dct:modified "2021-02-18T12:00:00+00:00"^^xsd:dateTime  ;
	skos:exactMatch subj:11001000 ;
	skos:exactMatch <https://www.wikidata.org/entity/Q17991228> ;
	skos:broader	medtop:20000593 ;
	skos:narrower	medtop:20000599 ;
	skos:narrower	medtop:20000601 ;
	skos:narrower	medtop:20000603 .

medtop:20000599
	rdf:type skos:Concept ;
	skos:prefLabel	"armed forces"@en-GB ;
	skos:definition	"Those employed by a government to conduct war, or to enforce the security of a nation"@en-GB ;
	skos:inScheme <http://cv.iptc.org/newscodes/mediatopic/>  ;
	ikos:created "2009-10-22T02:00:00+00:00"^^xsd:dateTime ;
	dct:created "2009-10-22T02:00:00+00:00"^^xsd:dateTime ;
	ikos:modified "2021-02-18T12:00:00+00:00"^^xsd:dateTime ;
	dct:modified "2021-02-18T12:00:00+00:00"^^xsd:dateTime  ;
	skos:exactMatch subj:11001004 ;
	skos:exactMatch <https://www.wikidata.org/entity/Q772547> ;
	skos:broader	medtop:20000598 ;
	skos:narrower	medtop:20000600 ;
	skos:narrower	medtop:20001145 .

medtop:20000600
	rdf:type skos:Concept ;
	skos:prefLabel	"veterans' affairs"@en-GB ;
	skos:definition	"Care and provision for those who served in the military"@en-GB ;
	skos:inScheme <http://cv.iptc.org/newscodes/mediatopic/>  ;
	ikos:created "2009-10-22T02:00:00+00:00"^^xsd:dateTime ;
	dct:created "2009-10-22T02:00:00+00:00"^^xsd:dateTime ;
	ikos:modified "2021-05-05T12:00:00+00:00"^^xsd:dateTime ;
	dct:modified "2021-05-05T12:00:00+00:00"^^xsd:dateTime  ;
	skos:exactMatch subj:11001001 ;
	skos:exactMatch <https://www.wikidata.org/entity/Q7923600> ;
	skos:broader	medtop:20000599 .

medtop:20000601
	rdf:type skos:Concept ;
	skos:prefLabel	"military equipment"@en-GB ;
	skos:definition	"Equipment issued to members of the armed forces"@en-GB ;
	skos:inScheme <http://cv.iptc.org/newscodes/mediatopic/>  ;
	ikos:created "2009-10-22T02:00:00+00:00"^^xsd:dateTime ;
	dct:created "2009-10-22T02:00:00+00:00"^^xsd:dateTime ;
	ikos:modified "2021-07-12T12:00:00+00:00"^^xsd:dateTime ;
	dct:modified "2021-07-12T12:00:00+00:00"^^xsd:dateTime  ;
	skos:exactMatch subj:11001005 ;
	skos:exactMatch <https://www.wikidata.org/entity/Q18643213> ;
	skos:broader	medtop:20000598 ;
	skos:narrower	medtop:20000602 .

medtop:20000602
	rdf:type skos:Concept ;
	skos:prefLabel	"military weaponry"@en-GB ;
	skos:definition	"A country's collection of armaments"@en-GB ;
	skos:inScheme <http://cv.iptc.org/newscodes/mediatopic/>  ;
	ikos:created "2009-10-22T02:00:00+00:00"^^xsd:dateTime ;
	dct:created "2009-10-22T02:00:00+00:00"^^xsd:dateTime ;
	ikos:modified "2021-02-18T12:00:00+00:00"^^xsd:dateTime ;
	dct:modified "2021-02-18T12:00:00+00:00"^^xsd:dateTime  ;
	skos:exactMatch subj:16012000 ;
	skos:broader	medtop:20000601 .

medtop:20000603
	rdf:type skos:Concept ;
	skos:prefLabel	"security measures (defence)"@en-GB ;
	skos:definition	"Means of making a nation, a state, a building or a person secure from harm and outside interference."@en-GB ;
	skos:inScheme <http://cv.iptc.org/newscodes/mediatopic/>  ;
	ikos:created "2009-10-22T02:00:00+00:00"^^xsd:dateTime ;
	dct:created "2009-10-22T02:00:00+00:00"^^xsd:dateTime ;
	ikos:modified "2021-02-18T12:00:00+00:00"^^xsd:dateTime ;
	dct:modified "2021-02-18T12:00:00+00:00"^^xsd:dateTime  ;
	skos:exactMatch subj:11001003 ;
	skos:exactMatch <https://www.wikidata.org/entity/Q852008> ;
	skos:broader	medtop:20000598 ;
	skos:narrower	medtop:20000604 .

medtop:20000604
	rdf:type skos:Concept ;
	skos:prefLabel	"national security"@en-GB ;
	skos:definition	"The philosophy of securing a nation and its borders, as well as the well-being of its citizens"@en-GB ;
	skos:inScheme <http://cv.iptc.org/newscodes/mediatopic/>  ;
	ikos:created "2009-10-22T02:00:00+00:00"^^xsd:dateTime ;
	dct:created "2009-10-22T02:00:00+00:00"^^xsd:dateTime ;
	ikos:modified "2021-05-05T12:00:00+00:00"^^xsd:dateTime ;
	dct:modified "2021-05-05T12:00:00+00:00"^^xsd:dateTime  ;
	skos:exactMatch subj:11001002 ;
	skos:exactMatch <https://www.wikidata.org/entity/Q258307> ;
	skos:broader	medtop:20000603 .

medtop:20000605
	rdf:type skos:Concept ;
	skos:prefLabel	"espionage and intelligence"@en-GB ;
	skos:definition	"Covert collection of information"@en-GB ;
	skos:inScheme <http://cv.iptc.org/newscodes/mediatopic/>  ;
	ikos:created "2009-10-22T02:00:00+00:00"^^xsd:dateTime ;
	dct:created "2009-10-22T02:00:00+00:00"^^xsd:dateTime ;
	ikos:modified "2021-02-18T12:00:00+00:00"^^xsd:dateTime ;
	dct:modified "2021-02-18T12:00:00+00:00"^^xsd:dateTime  ;
	skos:exactMatch subj:11004000 ;
	skos:exactMatch <https://www.wikidata.org/entity/Q165950> ;
	skos:broader	medtop:20000593 .

medtop:20000606
	rdf:type skos:Concept ;
	skos:prefLabel	"executive (government)"@en-GB ;
	skos:definition	"That portion of a ruling body involving the overall operation of government"@en-GB ;
	skos:inScheme <http://cv.iptc.org/newscodes/mediatopic/>  ;
	ikos:created "2009-10-22T02:00:00+00:00"^^xsd:dateTime ;
	dct:created "2009-10-22T02:00:00+00:00"^^xsd:dateTime ;
	ikos:modified "2021-02-18T12:00:00+00:00"^^xsd:dateTime ;
	dct:modified "2021-02-18T12:00:00+00:00"^^xsd:dateTime  ;
	skos:exactMatch subj:11006005 ;
	skos:exactMatch <https://www.wikidata.org/entity/Q35798> ;
	skos:broader	medtop:20000593 .

medtop:20000607
	rdf:type skos:Concept ;
	skos:prefLabel	"government budget"@en-GB ;
	skos:definition	"The expenses and revenues approved by the legislature."@en-GB ;
	skos:inScheme <http://cv.iptc.org/newscodes/mediatopic/>  ;
	ikos:created "2009-10-22T02:00:00+00:00"^^xsd:dateTime ;
	dct:created "2009-10-22T02:00:00+00:00"^^xsd:dateTime ;
	ikos:modified "2021-02-18T12:00:00+00:00"^^xsd:dateTime ;
	dct:modified "2021-02-18T12:00:00+00:00"^^xsd:dateTime  ;
	skos:broadMatch subj:11013000 ;
	skos:exactMatch <https://www.wikidata.org/entity/Q271855> ;
	skos:broader	medtop:20000593 ;
	skos:narrower	medtop:20000608 .

medtop:20000608
	rdf:type skos:Concept ;
	skos:prefLabel	"public finance"@en-GB ;
	skos:definition	"The money of government used for paying for public programmes and services and public debt"@en-GB ;
	skos:inScheme <http://cv.iptc.org/newscodes/mediatopic/>  ;
	ikos:created "2009-10-22T02:00:00+00:00"^^xsd:dateTime ;
	dct:created "2009-10-22T02:00:00+00:00"^^xsd:dateTime ;
	ikos:modified "2021-05-05T12:00:00+00:00"^^xsd:dateTime ;
	dct:modified "2021-05-05T12:00:00+00:00"^^xsd:dateTime  ;
	skos:exactMatch subj:11013001 ;
	skos:exactMatch <https://www.wikidata.org/wiki/Q1929688> ;
	skos:broader	medtop:20000607 .

medtop:20000609
	rdf:type skos:Concept ;
	skos:prefLabel	"government department"@en-GB ;
	skos:definition	"Divisions of a government that concentrate on specific areas such as health, welfare, economy or war"@en-GB ;
	skos:inScheme <http://cv.iptc.org/newscodes/mediatopic/>  ;
	ikos:created "2009-10-22T02:00:00+00:00"^^xsd:dateTime ;
	dct:created "2009-10-22T02:00:00+00:00"^^xsd:dateTime ;
	ikos:modified "2021-02-18T12:00:00+00:00"^^xsd:dateTime ;
	dct:modified "2021-02-18T12:00:00+00:00"^^xsd:dateTime  ;
	skos:exactMatch subj:11006007 ;
	skos:exactMatch <https://www.wikidata.org/entity/Q327333> ;
	skos:broader	medtop:20000593 .

medtop:20000610
	rdf:type skos:Concept ;
	skos:prefLabel	"heads of state"@en-GB ;
	skos:definition	"Symbolic or actual chief representative of a nation, such as royalty, or president or emir, for example"@en-GB ;
	skos:inScheme <http://cv.iptc.org/newscodes/mediatopic/>  ;
	ikos:created "2009-10-22T02:00:00+00:00"^^xsd:dateTime ;
	dct:created "2009-10-22T02:00:00+00:00"^^xsd:dateTime ;
	ikos:modified "2021-02-18T12:00:00+00:00"^^xsd:dateTime ;
	dct:modified "2021-02-18T12:00:00+00:00"^^xsd:dateTime  ;
	skos:exactMatch subj:11006006 ;
	skos:exactMatch <https://www.wikidata.org/entity/Q48352> ;
	skos:broader	medtop:20000593 .

medtop:20000611
	rdf:type skos:Concept ;
	skos:prefLabel	"impeachment"@en-GB ;
	skos:definition	"The process of bringing a public official before a tribunal to answer charges of wrongdoing"@en-GB ;
	skos:inScheme <http://cv.iptc.org/newscodes/mediatopic/>  ;
	ikos:created "2009-10-22T02:00:00+00:00"^^xsd:dateTime ;
	dct:created "2009-10-22T02:00:00+00:00"^^xsd:dateTime ;
	ikos:modified "2021-02-18T12:00:00+00:00"^^xsd:dateTime ;
	dct:modified "2021-02-18T12:00:00+00:00"^^xsd:dateTime  ;
	skos:exactMatch subj:11006013 ;
	skos:exactMatch <https://www.wikidata.org/entity/Q480498> ;
	skos:broader	medtop:20000593 .

medtop:20000612
	rdf:type skos:Concept ;
	skos:prefLabel	"local government and authority"@en-GB ;
	skos:definition	"Authorities at borough, city or county level"@en-GB ;
	skos:inScheme <http://cv.iptc.org/newscodes/mediatopic/>  ;
	ikos:created "2009-10-22T02:00:00+00:00"^^xsd:dateTime ;
	dct:created "2009-10-22T02:00:00+00:00"^^xsd:dateTime ;
	ikos:modified "2021-02-18T12:00:00+00:00"^^xsd:dateTime ;
	dct:modified "2021-02-18T12:00:00+00:00"^^xsd:dateTime  ;
	skos:exactMatch subj:11008000 ;
	skos:exactMatch <https://www.wikidata.org/entity/Q6501447> ;
	skos:broader	medtop:20000593 .

medtop:20000613
	rdf:type skos:Concept ;
	skos:prefLabel	"minister and secretary (government)"@en-GB ;
	skos:definition	"Senior government official, either elected or appointed, who heads a government department"@en-GB ;
	skos:inScheme <http://cv.iptc.org/newscodes/mediatopic/>  ;
	ikos:created "2009-10-22T02:00:00+00:00"^^xsd:dateTime ;
	dct:created "2009-10-22T02:00:00+00:00"^^xsd:dateTime ;
	ikos:modified "2021-05-05T12:00:00+00:00"^^xsd:dateTime ;
	dct:modified "2021-05-05T12:00:00+00:00"^^xsd:dateTime  ;
	skos:exactMatch subj:11006009 ;
	skos:exactMatch <https://www.wikidata.org/entity/Q165950> ;
	skos:broader	medtop:20000593 .

medtop:20000614
	rdf:type skos:Concept ;
	skos:prefLabel	"national government"@en-GB ;
	skos:definition	"The ruling body of a nation"@en-GB ;
	skos:inScheme <http://cv.iptc.org/newscodes/mediatopic/>  ;
	ikos:created "2009-10-22T02:00:00+00:00"^^xsd:dateTime ;
	dct:created "2009-10-22T02:00:00+00:00"^^xsd:dateTime ;
	ikos:modified "2021-02-18T12:00:00+00:00"^^xsd:dateTime ;
	dct:modified "2021-02-18T12:00:00+00:00"^^xsd:dateTime  ;
	skos:exactMatch subj:11006004 ;
	skos:exactMatch <https://www.wikidata.org/entity/Q1320217> ;
	skos:broader	medtop:20000593 .

medtop:20000615
	rdf:type skos:Concept ;
	skos:prefLabel	"legislative body"@en-GB ;
	skos:definition	"A legislature of elected officials representing the people that has the authority to make laws"@en-GB ;
	skos:inScheme <http://cv.iptc.org/newscodes/mediatopic/>  ;
	ikos:created "2009-10-22T02:00:00+00:00"^^xsd:dateTime ;
	dct:created "2009-10-22T02:00:00+00:00"^^xsd:dateTime ;
	ikos:modified "2021-03-31T12:00:00+00:00"^^xsd:dateTime ;
	dct:modified "2021-03-31T12:00:00+00:00"^^xsd:dateTime  ;
	skos:exactMatch subj:11009000 ;
	skos:exactMatch <https://www.wikidata.org/entity/Q35749> ;
	skos:broader	medtop:20000593 ;
	skos:narrower	medtop:20000616 ;
	skos:narrower	medtop:20000617 .

medtop:20000616
	rdf:type skos:Concept ;
	skos:prefLabel	"lower house (legislature)"@en-GB ;
	skos:definition	"Lower chamber of a legislative body, such as the US House of Representatives or UK House of Commons"@en-GB ;
	skos:editorialNote	"Note to translators: the examples in the English definition should be converted to relevant examples in countries which speak the target language."@en-GB ;
	skos:inScheme <http://cv.iptc.org/newscodes/mediatopic/>  ;
	ikos:created "2009-10-22T02:00:00+00:00"^^xsd:dateTime ;
	dct:created "2009-10-22T02:00:00+00:00"^^xsd:dateTime ;
	ikos:modified "2021-02-18T12:00:00+00:00"^^xsd:dateTime ;
	dct:modified "2021-02-18T12:00:00+00:00"^^xsd:dateTime  ;
	skos:exactMatch subj:11009002 ;
	skos:exactMatch <https://www.wikidata.org/entity/Q375928> ;
	skos:broader	medtop:20000615 .

medtop:20000617
	rdf:type skos:Concept ;
	skos:prefLabel	"upper house (legislature)"@en-GB ;
	skos:definition	"Senior chamber of a legislative body, such as the US Senate or UK House of Lords"@en-GB ;
	skos:editorialNote	"Note to translators: the examples in the English definition should be converted to relevant examples in countries which speak the target language."@en-GB ;
	skos:inScheme <http://cv.iptc.org/newscodes/mediatopic/>  ;
	ikos:created "2009-10-22T02:00:00+00:00"^^xsd:dateTime ;
	dct:created "2009-10-22T02:00:00+00:00"^^xsd:dateTime ;
	ikos:modified "2021-02-18T12:00:00+00:00"^^xsd:dateTime ;
	dct:modified "2021-02-18T12:00:00+00:00"^^xsd:dateTime  ;
	skos:exactMatch subj:11009001 ;
	skos:exactMatch <https://www.wikidata.org/entity/Q637846> ;
	skos:broader	medtop:20000615 .

medtop:20000618
	rdf:type skos:Concept ;
	skos:prefLabel	"regional government and authority"@en-GB ;
	skos:definition	"Authorities at a level above the local and below the national one. Could be named a state, province, department etc."@en-GB ;
	skos:inScheme <http://cv.iptc.org/newscodes/mediatopic/>  ;
	ikos:created "2009-10-22T02:00:00+00:00"^^xsd:dateTime ;
	dct:created "2009-10-22T02:00:00+00:00"^^xsd:dateTime ;
	ikos:modified "2021-02-18T12:00:00+00:00"^^xsd:dateTime ;
	dct:modified "2021-02-18T12:00:00+00:00"^^xsd:dateTime  ;
	skos:closeMatch subj:11012000 ;
	skos:exactMatch <https://www.wikidata.org/entity/Q1802419> ;
	skos:broader	medtop:20000593 .

medtop:20000619
	rdf:type skos:Concept ;
	skos:prefLabel	"safety of citizens"@en-GB ;
	skos:definition	"Government policies to protect the well-being of its citizens"@en-GB ;
	skos:inScheme <http://cv.iptc.org/newscodes/mediatopic/>  ;
	ikos:created "2009-10-22T02:00:00+00:00"^^xsd:dateTime ;
	dct:created "2009-10-22T02:00:00+00:00"^^xsd:dateTime ;
	ikos:modified "2021-05-05T12:00:00+00:00"^^xsd:dateTime ;
	dct:modified "2021-05-05T12:00:00+00:00"^^xsd:dateTime  ;
	skos:exactMatch subj:11006002 ;
	skos:exactMatch <https://www.wikidata.org/entity/Q294240> ;
	skos:broader	medtop:20000621 .

medtop:20000620
	rdf:type skos:Concept ;
	skos:prefLabel	"taxation"@en-GB ;
	skos:definition	"A levy to fund government expenditure"@en-GB ;
	skos:inScheme <http://cv.iptc.org/newscodes/mediatopic/>  ;
	ikos:created "2009-10-22T02:00:00+00:00"^^xsd:dateTime ;
	dct:created "2009-10-22T02:00:00+00:00"^^xsd:dateTime ;
	ikos:modified "2021-02-18T12:00:00+00:00"^^xsd:dateTime ;
	dct:modified "2021-02-18T12:00:00+00:00"^^xsd:dateTime  ;
	skos:broadMatch subj:11013000 ;
	skos:exactMatch <https://www.wikidata.org/entity/Q8161> ;
	skos:broader	medtop:20000621 .

medtop:20000621
	rdf:type skos:Concept ;
	skos:prefLabel	"government policy"@en-GB ;
	skos:definition	"An overall plan or course of action set out by a government intended to influence and guide decisions and actions towards a desired outcome."@en-GB ;
	skos:inScheme <http://cv.iptc.org/newscodes/mediatopic/>  ;
	ikos:created "2009-10-22T02:00:00+00:00"^^xsd:dateTime ;
	dct:created "2009-10-22T02:00:00+00:00"^^xsd:dateTime ;
	ikos:modified "2021-02-18T12:00:00+00:00"^^xsd:dateTime ;
	dct:modified "2021-02-18T12:00:00+00:00"^^xsd:dateTime  ;
	skos:broadMatch subj:11006000 ;
	skos:exactMatch <https://www.wikidata.org/entity/Q546113> ;
	skos:broader	medtop:11000000 ;
	skos:narrower	medtop:20000345 ;
	skos:narrower	medtop:20000423 ;
	skos:narrower	medtop:20000479 ;
	skos:narrower	medtop:20000619 ;
	skos:narrower	medtop:20000620 ;
	skos:narrower	medtop:20000626 ;
	skos:narrower	medtop:20000634 ;
	skos:narrower	medtop:20000635 ;
	skos:narrower	medtop:20000636 ;
	skos:narrower	medtop:20001132 ;
	skos:narrower	medtop:20001147 ;
	skos:narrower	medtop:20001265 ;
	skos:narrower	medtop:20001338 .

medtop:20000623
	rdf:type skos:Concept ;
	skos:prefLabel	"nationalisation"@en-GB ;
	skos:definition	"State takeover of private companies or properties"@en-GB ;
	skos:inScheme <http://cv.iptc.org/newscodes/mediatopic/>  ;
	ikos:created "2009-10-22T02:00:00+00:00"^^xsd:dateTime ;
	dct:created "2009-10-22T02:00:00+00:00"^^xsd:dateTime ;
	ikos:modified "2021-02-18T12:00:00+00:00"^^xsd:dateTime ;
	dct:modified "2021-02-18T12:00:00+00:00"^^xsd:dateTime  ;
	skos:exactMatch subj:11006012 ;
	skos:exactMatch <https://www.wikidata.org/entity/Q178564> ;
	skos:broader	medtop:20000345 .

medtop:20000624
	rdf:type skos:Concept ;
	skos:prefLabel	"privatisation"@en-GB ;
	skos:definition	"The transfer of state-owned companies or properties to private owners"@en-GB ;
	skos:inScheme <http://cv.iptc.org/newscodes/mediatopic/>  ;
	ikos:created "2009-10-22T02:00:00+00:00"^^xsd:dateTime ;
	dct:created "2009-10-22T02:00:00+00:00"^^xsd:dateTime ;
	ikos:modified "2021-02-18T12:00:00+00:00"^^xsd:dateTime ;
	dct:modified "2021-02-18T12:00:00+00:00"^^xsd:dateTime  ;
	skos:exactMatch subj:04016034 ;
	skos:exactMatch <https://www.wikidata.org/entity/Q161500> ;
	skos:broader	medtop:20000345 .

medtop:20000625
	rdf:type skos:Concept ;
	skos:prefLabel	"state-owned enterprise"@en-GB ;
	skos:definition	"The government as owner of companies, either complete or partial"@en-GB ;
	skos:inScheme <http://cv.iptc.org/newscodes/mediatopic/>  ;
	ikos:created "2009-10-22T02:00:00+00:00"^^xsd:dateTime ;
	dct:created "2009-10-22T02:00:00+00:00"^^xsd:dateTime ;
	ikos:modified "2021-02-18T12:00:00+00:00"^^xsd:dateTime ;
	dct:modified "2021-02-18T12:00:00+00:00"^^xsd:dateTime  ;
	skos:broadMatch subj:04017001 ;
	skos:exactMatch <https://www.wikidata.org/entity/Q270791> ;
	skos:broader	medtop:20000345 .

medtop:20000626
	rdf:type skos:Concept ;
	skos:prefLabel	"interior policy"@en-GB ;
	skos:definition	"Government policies affecting internal affairs"@en-GB ;
	skos:inScheme <http://cv.iptc.org/newscodes/mediatopic/>  ;
	ikos:created "2009-10-22T02:00:00+00:00"^^xsd:dateTime ;
	dct:created "2009-10-22T02:00:00+00:00"^^xsd:dateTime ;
	ikos:modified "2021-02-18T12:00:00+00:00"^^xsd:dateTime ;
	dct:modified "2021-02-18T12:00:00+00:00"^^xsd:dateTime  ;
	skos:closeMatch subj:11016000 ;
	skos:exactMatch <https://www.wikidata.org/entity/Q1573035> ;
	skos:broader	medtop:20000621 ;
	skos:narrower	medtop:20000627 ;
	skos:narrower	medtop:20000628 ;
	skos:narrower	medtop:20000629 ;
	skos:narrower	medtop:20000630 ;
	skos:narrower	medtop:20000631 ;
	skos:narrower	medtop:20000632 ;
	skos:narrower	medtop:20000633 ;
	skos:narrower	medtop:20001146 ;
	skos:narrower	medtop:20001174 ;
	skos:narrower	medtop:20001264 .

medtop:20000627
	rdf:type skos:Concept ;
	skos:prefLabel	"data protection policy"@en-GB ;
	skos:definition	"Efforts to protect personal information in either written, oral or electronic form"@en-GB ;
	skos:inScheme <http://cv.iptc.org/newscodes/mediatopic/>  ;
	ikos:created "2009-10-22T02:00:00+00:00"^^xsd:dateTime ;
	dct:created "2009-10-22T02:00:00+00:00"^^xsd:dateTime ;
	ikos:modified "2021-02-18T12:00:00+00:00"^^xsd:dateTime ;
	dct:modified "2021-02-18T12:00:00+00:00"^^xsd:dateTime  ;
	skos:exactMatch subj:11016001 ;
	skos:exactMatch <https://www.wikidata.org/entity/Q23647168> ;
	skos:broader	medtop:20000626 .

medtop:20000628
	rdf:type skos:Concept ;
	skos:prefLabel	"housing and urban planning policy"@en-GB ;
	skos:definition	"Systematic planning of urban and suburban areas and the housing within those areas"@en-GB ;
	skos:inScheme <http://cv.iptc.org/newscodes/mediatopic/>  ;
	ikos:created "2009-10-22T02:00:00+00:00"^^xsd:dateTime ;
	dct:created "2009-10-22T02:00:00+00:00"^^xsd:dateTime ;
	ikos:modified "2021-02-18T12:00:00+00:00"^^xsd:dateTime ;
	dct:modified "2021-02-18T12:00:00+00:00"^^xsd:dateTime  ;
	skos:exactMatch subj:11016002 ;
	skos:exactMatch <https://www.wikidata.org/entity/Q69883> ;
	skos:broader	medtop:20000626 .

medtop:20000629
	rdf:type skos:Concept ;
	skos:prefLabel	"policy towards indigenous people"@en-GB ;
	skos:definition	"Government policies toward indigenous peoples"@en-GB ;
	skos:inScheme <http://cv.iptc.org/newscodes/mediatopic/>  ;
	ikos:created "2009-10-22T02:00:00+00:00"^^xsd:dateTime ;
	dct:created "2009-10-22T02:00:00+00:00"^^xsd:dateTime ;
	ikos:modified "2021-02-18T12:00:00+00:00"^^xsd:dateTime ;
	dct:modified "2021-02-18T12:00:00+00:00"^^xsd:dateTime  ;
	skos:exactMatch subj:11016005 ;
	skos:broader	medtop:20000626 .

medtop:20000630
	rdf:type skos:Concept ;
	skos:prefLabel	"pension and welfare policy"@en-GB ;
	skos:definition	"Government policies affecting the well-being of its citizens through unemployment benefits, state pensions and other similar payments"@en-GB ;
	skos:inScheme <http://cv.iptc.org/newscodes/mediatopic/>  ;
	ikos:created "2009-10-22T02:00:00+00:00"^^xsd:dateTime ;
	dct:created "2009-10-22T02:00:00+00:00"^^xsd:dateTime ;
	ikos:modified "2021-05-05T12:00:00+00:00"^^xsd:dateTime ;
	dct:modified "2021-05-05T12:00:00+00:00"^^xsd:dateTime  ;
	skos:exactMatch subj:11016003 ;
	skos:exactMatch <https://www.wikidata.org/entity/Q828395> ;
	skos:broader	medtop:20000626 .

medtop:20000631
	rdf:type skos:Concept ;
	skos:prefLabel	"personal data collection policy"@en-GB ;
	skos:definition	"The collection, by government or other entities of information on individuals"@en-GB ;
	skos:inScheme <http://cv.iptc.org/newscodes/mediatopic/>  ;
	ikos:created "2009-10-22T02:00:00+00:00"^^xsd:dateTime ;
	dct:created "2009-10-22T02:00:00+00:00"^^xsd:dateTime ;
	ikos:modified "2021-05-05T12:00:00+00:00"^^xsd:dateTime ;
	dct:modified "2021-05-05T12:00:00+00:00"^^xsd:dateTime  ;
	skos:exactMatch subj:11016006 ;
	skos:exactMatch <https://www.wikidata.org/entity/Q1999831> ;
	skos:broader	medtop:20000626 .

medtop:20000632
	rdf:type skos:Concept ;
	skos:prefLabel	"personal weapon control policy"@en-GB ;
	skos:definition	"Government control of personal ownership of firearms and other offensive weapons, including control of weapons used for sports through licenses and other means"@en-GB ;
	skos:inScheme <http://cv.iptc.org/newscodes/mediatopic/>  ;
	ikos:created "2009-10-22T02:00:00+00:00"^^xsd:dateTime ;
	dct:created "2009-10-22T02:00:00+00:00"^^xsd:dateTime ;
	ikos:modified "2021-02-18T12:00:00+00:00"^^xsd:dateTime ;
	dct:modified "2021-02-18T12:00:00+00:00"^^xsd:dateTime  ;
	skos:exactMatch subj:11016004 ;
	skos:exactMatch <https://www.wikidata.org/entity/Q1328508> ;
	skos:broader	medtop:20000626 .

medtop:20000633
	rdf:type skos:Concept ;
	skos:prefLabel	"planning inquiries"@en-GB ;
	skos:definition	"Public hearings or planning inquiries on proposed constructions, e.g. Construction of water driven power station in a National Park."@en-GB ;
	skos:inScheme <http://cv.iptc.org/newscodes/mediatopic/>  ;
	ikos:created "2009-10-22T02:00:00+00:00"^^xsd:dateTime ;
	dct:created "2009-10-22T02:00:00+00:00"^^xsd:dateTime ;
	ikos:modified "2021-02-18T12:00:00+00:00"^^xsd:dateTime ;
	dct:modified "2021-02-18T12:00:00+00:00"^^xsd:dateTime  ;
	skos:exactMatch subj:11016007 ;
	skos:broader	medtop:20000626 .

medtop:20000634
	rdf:type skos:Concept ;
	skos:prefLabel	"migration policy"@en-GB ;
	skos:definition	"Movement of one body of persons from one place to another"@en-GB ;
	skos:inScheme <http://cv.iptc.org/newscodes/mediatopic/>  ;
	ikos:created "2009-10-22T02:00:00+00:00"^^xsd:dateTime ;
	dct:created "2009-10-22T02:00:00+00:00"^^xsd:dateTime ;
	ikos:modified "2021-02-18T12:00:00+00:00"^^xsd:dateTime ;
	dct:modified "2021-02-18T12:00:00+00:00"^^xsd:dateTime  ;
	skos:exactMatch subj:11017000 ;
	skos:exactMatch <https://www.wikidata.org/entity/Q15064326> ;
	skos:broader	medtop:20000621 .

medtop:20000635
	rdf:type skos:Concept ;
	skos:prefLabel	"nuclear policy"@en-GB ;
	skos:definition	"Government policies as regards to use of nuclear fuels for power production or weapons"@en-GB ;
	skos:inScheme <http://cv.iptc.org/newscodes/mediatopic/>  ;
	ikos:created "2009-10-22T02:00:00+00:00"^^xsd:dateTime ;
	dct:created "2009-10-22T02:00:00+00:00"^^xsd:dateTime ;
	ikos:modified "2021-02-18T12:00:00+00:00"^^xsd:dateTime ;
	dct:modified "2021-02-18T12:00:00+00:00"^^xsd:dateTime  ;
	skos:exactMatch subj:11020000 ;
	skos:exactMatch <https://www.wikidata.org/entity/Q757637> ;
	skos:broader	medtop:20000621 .

medtop:20000636
	rdf:type skos:Concept ;
	skos:prefLabel	"regulation of industry"@en-GB ;
	skos:definition	"The rules and bodies, both national and international, that govern conflict of interest and good practice regulations."@en-GB ;
	skos:inScheme <http://cv.iptc.org/newscodes/mediatopic/>  ;
	ikos:created "2009-10-22T02:00:00+00:00"^^xsd:dateTime ;
	dct:created "2009-10-22T02:00:00+00:00"^^xsd:dateTime ;
	ikos:modified "2021-02-18T12:00:00+00:00"^^xsd:dateTime ;
	dct:modified "2021-02-18T12:00:00+00:00"^^xsd:dateTime  ;
	skos:exactMatch subj:11022000 ;
	skos:broader	medtop:20000621 ;
	skos:narrower	medtop:20000637 .

medtop:20000637
	rdf:type skos:Concept ;
	skos:prefLabel	"food and drink regulations"@en-GB ;
	skos:definition	"Government policies relating to food and drink"@en-GB ;
	skos:inScheme <http://cv.iptc.org/newscodes/mediatopic/>  ;
	ikos:created "2009-10-22T02:00:00+00:00"^^xsd:dateTime ;
	dct:created "2009-10-22T02:00:00+00:00"^^xsd:dateTime ;
	ikos:modified "2021-02-18T12:00:00+00:00"^^xsd:dateTime ;
	dct:modified "2021-02-18T12:00:00+00:00"^^xsd:dateTime  ;
	skos:broadMatch subj:11022000 ;
	skos:broader	medtop:20000636 .

medtop:20000638
	rdf:type skos:Concept ;
	skos:prefLabel	"international relations"@en-GB ;
	skos:definition	"Non-violent relations between nations through negotiation, treaty, or personal meetings"@en-GB ;
	skos:inScheme <http://cv.iptc.org/newscodes/mediatopic/>  ;
	ikos:created "2009-10-22T02:00:00+00:00"^^xsd:dateTime ;
	dct:created "2009-10-22T02:00:00+00:00"^^xsd:dateTime ;
	ikos:modified "2021-02-18T12:00:00+00:00"^^xsd:dateTime ;
	dct:modified "2021-02-18T12:00:00+00:00"^^xsd:dateTime  ;
	skos:exactMatch <https://www.wikidata.org/entity/Q166542> ;
	skos:exactMatch subj:11002002 ;
	skos:broader	medtop:11000000 ;
	skos:narrower	medtop:20000639 ;
	skos:narrower	medtop:20000642 ;
	skos:narrower	medtop:20000643 ;
	skos:narrower	medtop:20000644 ;
	skos:narrower	medtop:20000645 ;
	skos:narrower	medtop:20001316 .

medtop:20000639
	rdf:type skos:Concept ;
	skos:prefLabel	"diplomacy"@en-GB ;
	skos:definition	"The use of verbal and written skills for persuading others to your point of view"@en-GB ;
	skos:inScheme <http://cv.iptc.org/newscodes/mediatopic/>  ;
	ikos:created "2009-10-22T02:00:00+00:00"^^xsd:dateTime ;
	dct:created "2009-10-22T02:00:00+00:00"^^xsd:dateTime ;
	ikos:modified "2021-02-18T12:00:00+00:00"^^xsd:dateTime ;
	dct:modified "2021-02-18T12:00:00+00:00"^^xsd:dateTime  ;
	skos:exactMatch subj:11002000 ;
	skos:exactMatch <https://www.wikidata.org/entity/Q1889> ;
	skos:broader	medtop:20000638 ;
	skos:narrower	medtop:20000640 ;
	skos:narrower	medtop:20000641 .

medtop:20000640
	rdf:type skos:Concept ;
	skos:prefLabel	"summit meetings"@en-GB ;
	skos:definition	"Includes meetings of leaders, foreign and finance ministers from the Group of Eight major nations and Group of Seven industrialized nations."@en-GB ;
	skos:inScheme <http://cv.iptc.org/newscodes/mediatopic/>  ;
	ikos:created "2009-10-22T02:00:00+00:00"^^xsd:dateTime ;
	dct:created "2009-10-22T02:00:00+00:00"^^xsd:dateTime ;
	ikos:modified "2021-02-18T12:00:00+00:00"^^xsd:dateTime ;
	dct:modified "2021-02-18T12:00:00+00:00"^^xsd:dateTime  ;
	skos:exactMatch subj:11002001 ;
	skos:exactMatch <https://www.wikidata.org/entity/Q1072326> ;
	skos:broader	medtop:20000639 .

medtop:20000641
	rdf:type skos:Concept ;
	skos:prefLabel	"treaty"@en-GB ;
	skos:definition	"A treaty (as defined by the Vienna Convention on the Law of Treaties) is a written agreement between international entities that is binding under international law."@en-GB ;
	skos:inScheme <http://cv.iptc.org/newscodes/mediatopic/>  ;
	ikos:created "2009-10-22T02:00:00+00:00"^^xsd:dateTime ;
	dct:created "2009-10-22T02:00:00+00:00"^^xsd:dateTime ;
	ikos:modified "2021-02-18T12:00:00+00:00"^^xsd:dateTime ;
	dct:modified "2021-02-18T12:00:00+00:00"^^xsd:dateTime  ;
	skos:exactMatch subj:11027000 ;
	skos:exactMatch <https://www.wikidata.org/entity/Q131569> ;
	skos:broader	medtop:20000639 .

medtop:20000642
	rdf:type skos:Concept ;
	skos:prefLabel	"economic sanction"@en-GB ;
	skos:definition	"Punitive actions taken by one country against another including trade restrictions, embargoes etc."@en-GB ;
	skos:inScheme <http://cv.iptc.org/newscodes/mediatopic/>  ;
	ikos:created "2009-10-22T02:00:00+00:00"^^xsd:dateTime ;
	dct:created "2009-10-22T02:00:00+00:00"^^xsd:dateTime ;
	ikos:modified "2021-02-18T12:00:00+00:00"^^xsd:dateTime ;
	dct:modified "2021-02-18T12:00:00+00:00"^^xsd:dateTime  ;
	skos:exactMatch subj:11005001 ;
	skos:exactMatch <https://www.wikidata.org/entity/Q1248258> ;
	skos:broader	medtop:20000638 .

medtop:20000643
	rdf:type skos:Concept ;
	skos:prefLabel	"foreign aid"@en-GB ;
	skos:definition	"Help provided by one nation to another"@en-GB ;
	skos:inScheme <http://cv.iptc.org/newscodes/mediatopic/>  ;
	ikos:created "2009-10-22T02:00:00+00:00"^^xsd:dateTime ;
	dct:created "2009-10-22T02:00:00+00:00"^^xsd:dateTime ;
	ikos:modified "2021-02-18T12:00:00+00:00"^^xsd:dateTime ;
	dct:modified "2021-02-18T12:00:00+00:00"^^xsd:dateTime  ;
	skos:exactMatch subj:11005000 ;
	skos:exactMatch <https://www.wikidata.org/entity/Q2827815> ;
	skos:broader	medtop:20000638 .

medtop:20000644
	rdf:type skos:Concept ;
	skos:prefLabel	"international organisation"@en-GB ;
	skos:definition	"Includes organisations with members and functions that cross international borders, and may include intergovernmental organisations of sovereign nations."@en-GB ;
	skos:inScheme <http://cv.iptc.org/newscodes/mediatopic/>  ;
	ikos:created "2009-10-22T02:00:00+00:00"^^xsd:dateTime ;
	dct:created "2009-10-22T02:00:00+00:00"^^xsd:dateTime ;
	ikos:modified "2021-02-18T12:00:00+00:00"^^xsd:dateTime ;
	dct:modified "2021-02-18T12:00:00+00:00"^^xsd:dateTime  ;
	skos:exactMatch subj:11028000 ;
	skos:exactMatch <https://www.wikidata.org/entity/Q484652> ;
	skos:broader	medtop:20000638 .

medtop:20000645
	rdf:type skos:Concept ;
	skos:prefLabel	"refugees and internally displaced people"@en-GB ;
	skos:definition	"A person seeking shelter in another country because of some fear of persecution in his own country"@en-GB ;
	skos:inScheme <http://cv.iptc.org/newscodes/mediatopic/>  ;
	ikos:created "2009-10-22T02:00:00+00:00"^^xsd:dateTime ;
	dct:created "2009-10-22T02:00:00+00:00"^^xsd:dateTime ;
	ikos:modified "2021-02-18T12:00:00+00:00"^^xsd:dateTime ;
	dct:modified "2021-02-18T12:00:00+00:00"^^xsd:dateTime  ;
	skos:exactMatch subj:11011000 ;
	skos:exactMatch <https://www.wikidata.org/entity/Q131572> ;
	skos:broader	medtop:20000638 .

medtop:20000646
	rdf:type skos:Concept ;
	skos:prefLabel	"non-governmental organisation"@en-GB ;
	skos:definition	"Groups officially outside of government that lobby, demonstrate or campaign on a wide range of issues such as economics, environment healthcare etc."@en-GB ;
	skos:inScheme <http://cv.iptc.org/newscodes/mediatopic/>  ;
	ikos:created "2009-10-22T02:00:00+00:00"^^xsd:dateTime ;
	dct:created "2009-10-22T02:00:00+00:00"^^xsd:dateTime ;
	ikos:modified "2021-02-18T12:00:00+00:00"^^xsd:dateTime ;
	dct:modified "2021-02-18T12:00:00+00:00"^^xsd:dateTime  ;
	skos:exactMatch <https://www.wikidata.org/entity/Q79913> ;
	skos:exactMatch subj:11010001 ;
	skos:broader	medtop:11000000 .

medtop:20000647
	rdf:type skos:Concept ;
	skos:prefLabel	"political crisis"@en-GB ;
	skos:definition	"Conflict that rises to a level where, depending on events, governments can fall etc"@en-GB ;
	skos:inScheme <http://cv.iptc.org/newscodes/mediatopic/>  ;
	ikos:created "2009-10-22T02:00:00+00:00"^^xsd:dateTime ;
	dct:created "2009-10-22T02:00:00+00:00"^^xsd:dateTime ;
	ikos:modified "2021-02-18T12:00:00+00:00"^^xsd:dateTime ;
	dct:modified "2021-02-18T12:00:00+00:00"^^xsd:dateTime  ;
	skos:broadMatch subj:16011000 ;
	skos:exactMatch <https://www.wikidata.org/entity/Q3002772> ;
	skos:broader	medtop:11000000 .

medtop:20000648
	rdf:type skos:Concept ;
	skos:prefLabel	"political dissent"@en-GB ;
	skos:definition	"Disagreement between political groups, usually organised and sometimes resulting in imprisonment of the dissenters"@en-GB ;
	skos:inScheme <http://cv.iptc.org/newscodes/mediatopic/>  ;
	ikos:created "2009-10-22T02:00:00+00:00"^^xsd:dateTime ;
	dct:created "2009-10-22T02:00:00+00:00"^^xsd:dateTime ;
	ikos:modified "2021-02-18T12:00:00+00:00"^^xsd:dateTime ;
	dct:modified "2021-02-18T12:00:00+00:00"^^xsd:dateTime  ;
	skos:exactMatch <https://www.wikidata.org/entity/Q7210284> ;
	skos:exactMatch subj:16003003 ;
	skos:broader	medtop:11000000 .

medtop:20000649
	rdf:type skos:Concept ;
	skos:prefLabel	"political process"@en-GB ;
	skos:definition	"The art or science of participating in the affairs of government, a state of political party"@en-GB ;
	skos:inScheme <http://cv.iptc.org/newscodes/mediatopic/>  ;
	ikos:created "2009-10-22T02:00:00+00:00"^^xsd:dateTime ;
	dct:created "2009-10-22T02:00:00+00:00"^^xsd:dateTime ;
	ikos:modified "2021-05-05T12:00:00+00:00"^^xsd:dateTime ;
	dct:modified "2021-05-05T12:00:00+00:00"^^xsd:dateTime  ;
	skos:exactMatch subj:11024000 ;
	skos:exactMatch <https://www.wikidata.org/entity/Q11827330> ;
	skos:broader	medtop:11000000 ;
	skos:narrower	medtop:20000650 ;
	skos:narrower	medtop:20000651 ;
	skos:narrower	medtop:20000652 ;
	skos:narrower	medtop:20000653 .

medtop:20000650
	rdf:type skos:Concept ;
	skos:prefLabel	"lobbying"@en-GB ;
	skos:definition	"The attempt by non-government bodies and individuals to affect the outcome of legislation through verbal, or other, persuasion"@en-GB ;
	skos:inScheme <http://cv.iptc.org/newscodes/mediatopic/>  ;
	ikos:created "2009-10-22T02:00:00+00:00"^^xsd:dateTime ;
	dct:created "2009-10-22T02:00:00+00:00"^^xsd:dateTime ;
	ikos:modified "2021-02-18T12:00:00+00:00"^^xsd:dateTime ;
	dct:modified "2021-02-18T12:00:00+00:00"^^xsd:dateTime  ;
	skos:exactMatch subj:11021000 ;
	skos:exactMatch <https://www.wikidata.org/entity/Q187117> ;
	skos:broader	medtop:20000649 .

medtop:20000651
	rdf:type skos:Concept ;
	skos:prefLabel	"political parties and movements"@en-GB ;
	skos:definition	"Covers both formally recognised and informal political associations"@en-GB ;
	skos:inScheme <http://cv.iptc.org/newscodes/mediatopic/>  ;
	ikos:created "2009-10-22T02:00:00+00:00"^^xsd:dateTime ;
	dct:created "2009-10-22T02:00:00+00:00"^^xsd:dateTime ;
	ikos:modified "2021-02-18T12:00:00+00:00"^^xsd:dateTime ;
	dct:modified "2021-02-18T12:00:00+00:00"^^xsd:dateTime  ;
	skos:exactMatch subj:11010000 ;
	skos:exactMatch <https://www.wikidata.org/entity/Q7278> ;
	skos:broader	medtop:20000649 ;
	skos:narrower	medtop:20001312 .

medtop:20000652
	rdf:type skos:Concept ;
	skos:prefLabel	"political development"@en-GB ;
	skos:definition	"The creation and rise of political systems and the history of the people and nations that are associated with those systems."@en-GB ;
	skos:inScheme <http://cv.iptc.org/newscodes/mediatopic/>  ;
	ikos:created "2009-10-22T02:00:00+00:00"^^xsd:dateTime ;
	dct:created "2009-10-22T02:00:00+00:00"^^xsd:dateTime ;
	ikos:modified "2021-02-18T12:00:00+00:00"^^xsd:dateTime ;
	dct:modified "2021-02-18T12:00:00+00:00"^^xsd:dateTime  ;
	skos:exactMatch subj:11024003 ;
	skos:broader	medtop:20000649 .

medtop:20000653
	rdf:type skos:Concept ;
	skos:prefLabel	"political system"@en-GB ;
	skos:definition	"System designed to provide order to government"@en-GB ;
	skos:inScheme <http://cv.iptc.org/newscodes/mediatopic/>  ;
	ikos:created "2009-10-22T02:00:00+00:00"^^xsd:dateTime ;
	dct:created "2009-10-22T02:00:00+00:00"^^xsd:dateTime ;
	ikos:modified "2021-02-18T12:00:00+00:00"^^xsd:dateTime ;
	dct:modified "2021-02-18T12:00:00+00:00"^^xsd:dateTime  ;
	skos:exactMatch subj:11024001 ;
	skos:exactMatch <https://www.wikidata.org/entity/Q28108> ;
	skos:broader	medtop:20000649 ;
	skos:narrower	medtop:20000654 ;
	skos:narrower	medtop:20000655 .

medtop:20000654
	rdf:type skos:Concept ;
	skos:prefLabel	"democracy"@en-GB ;
	skos:definition	"Government in which the people hold the power either directly, or through elected officials."@en-GB ;
	skos:inScheme <http://cv.iptc.org/newscodes/mediatopic/>  ;
	ikos:created "2009-10-22T02:00:00+00:00"^^xsd:dateTime ;
	dct:created "2009-10-22T02:00:00+00:00"^^xsd:dateTime ;
	ikos:modified "2021-02-18T12:00:00+00:00"^^xsd:dateTime ;
	dct:modified "2021-02-18T12:00:00+00:00"^^xsd:dateTime  ;
	skos:exactMatch subj:11024002 ;
	skos:exactMatch <https://www.wikidata.org/entity/Q7174> ;
	skos:broader	medtop:20000653 .

medtop:20000655
	rdf:type skos:Concept ;
	skos:prefLabel	"dictatorship"@en-GB ;
	skos:definition	"Government in which a single individual or a small group of individuals hold power without consent of the people"@en-GB ;
	skos:inScheme <http://cv.iptc.org/newscodes/mediatopic/>  ;
	ikos:created "2009-10-22T02:00:00+00:00"^^xsd:dateTime ;
	dct:created "2009-10-22T02:00:00+00:00"^^xsd:dateTime ;
	ikos:modified "2021-02-18T12:00:00+00:00"^^xsd:dateTime ;
	dct:modified "2021-02-18T12:00:00+00:00"^^xsd:dateTime  ;
	skos:broadMatch subj:11006000 ;
	skos:exactMatch <https://www.wikidata.org/entity/Q317> ;
	skos:broader	medtop:20000653 .

medtop:20000657
	rdf:type skos:Concept ;
	skos:prefLabel	"belief systems"@en-GB ;
	skos:definition	"A set of beliefs prescribed by an institution or text often focusing on the worship of a higher power and the outlining of moral guidelines"@en-GB ;
	skos:inScheme <http://cv.iptc.org/newscodes/mediatopic/>  ;
	ikos:created "2009-10-22T02:00:00+00:00"^^xsd:dateTime ;
	dct:created "2009-10-22T02:00:00+00:00"^^xsd:dateTime ;
	ikos:modified "2021-12-21T12:00:00+00:00"^^xsd:dateTime ;
	dct:modified "2021-12-21T12:00:00+00:00"^^xsd:dateTime  ;
	skos:exactMatch <https://www.wikidata.org/entity/Q2728698> ;
	skos:exactMatch subj:12002000 ;
	skos:broader	medtop:12000000 ;
	skos:narrower	medtop:20000658 ;
	skos:narrower	medtop:20000659 ;
	skos:narrower	medtop:20000673 ;
	skos:narrower	medtop:20000674 ;
	skos:narrower	medtop:20000675 ;
	skos:narrower	medtop:20000676 ;
	skos:narrower	medtop:20000677 ;
	skos:narrower	medtop:20000678 ;
	skos:narrower	medtop:20000679 ;
	skos:narrower	medtop:20000680 ;
	skos:narrower	medtop:20000681 ;
	skos:narrower	medtop:20000682 ;
	skos:narrower	medtop:20000683 ;
	skos:narrower	medtop:20000684 ;
	skos:narrower	medtop:20000685 ;
	skos:narrower	medtop:20000686 ;
	skos:narrower	medtop:20001349 .

medtop:20000658
	rdf:type skos:Concept ;
	skos:prefLabel	"Buddhism"@en-GB ;
	skos:definition	"An Asian religion founded in the 6th century BC in India based on the teachings of the Buddha with the goal of overcoming suffering and transcending desire and the individual self to achieve nirvana"@en-GB ;
	skos:inScheme <http://cv.iptc.org/newscodes/mediatopic/>  ;
	ikos:created "2009-10-22T02:00:00+00:00"^^xsd:dateTime ;
	dct:created "2009-10-22T02:00:00+00:00"^^xsd:dateTime ;
	ikos:modified "2021-12-21T12:00:00+00:00"^^xsd:dateTime ;
	dct:modified "2021-12-21T12:00:00+00:00"^^xsd:dateTime  ;
	skos:exactMatch subj:12012000 ;
	skos:exactMatch <https://www.wikidata.org/entity/Q748> ;
	skos:broader	medtop:20000657 .

medtop:20000659
	rdf:type skos:Concept ;
	skos:prefLabel	"Christianity"@en-GB ;
	skos:definition	"Religions that follow the teachings of Jesus Christ and the Bible"@en-GB ;
	skos:inScheme <http://cv.iptc.org/newscodes/mediatopic/>  ;
	ikos:created "2009-10-22T02:00:00+00:00"^^xsd:dateTime ;
	dct:created "2009-10-22T02:00:00+00:00"^^xsd:dateTime ;
	ikos:modified "2021-12-21T12:00:00+00:00"^^xsd:dateTime ;
	dct:modified "2021-12-21T12:00:00+00:00"^^xsd:dateTime  ;
	skos:exactMatch subj:12009000 ;
	skos:exactMatch <https://www.wikidata.org/entity/Q5043> ;
	skos:broader	medtop:20000657 ;
	skos:narrower	medtop:20000660 ;
	skos:narrower	medtop:20000661 ;
	skos:narrower	medtop:20000662 ;
	skos:narrower	medtop:20000663 ;
	skos:narrower	medtop:20000664 ;
	skos:narrower	medtop:20000671 ;
	skos:narrower	medtop:20001344 .

medtop:20000660
	rdf:type skos:Concept ;
	skos:prefLabel	"ecumenism"@en-GB ;
	skos:definition	"Relations between Christian churches"@en-GB ;
	skos:changeNote	"Retired in December 2021. Use Christianity (medtop:20000659) instead."@en-GB ;
	skos:inScheme <http://cv.iptc.org/newscodes/mediatopic/>  ;
	ikos:created "2009-10-22T02:00:00+00:00"^^xsd:dateTime ;
	dct:created "2009-10-22T02:00:00+00:00"^^xsd:dateTime ;
	ikos:modified "2021-02-18T12:00:00+00:00"^^xsd:dateTime ;
	dct:modified "2021-02-18T12:00:00+00:00"^^xsd:dateTime  ; 
	ikos:retired "2021-12-17T12:00:00+00:00"^^xsd:dateTime ;
	skos:exactMatch subj:12027000 ;
	skos:exactMatch <https://www.wikidata.org/entity/Q156112> ;
	skos:broader	medtop:20000659 .

medtop:20000661
	rdf:type skos:Concept ;
	skos:prefLabel	"Mormonism"@en-GB ;
	skos:definition	"Christian religion founded in New York State in the 1820s that follows the teachings of Joseph Smith and the *Book of Mormon*"@en-GB ;
	skos:inScheme <http://cv.iptc.org/newscodes/mediatopic/>  ;
	ikos:created "2009-10-22T02:00:00+00:00"^^xsd:dateTime ;
	dct:created "2009-10-22T02:00:00+00:00"^^xsd:dateTime ;
	ikos:modified "2021-12-21T12:00:00+00:00"^^xsd:dateTime ;
	dct:modified "2021-12-21T12:00:00+00:00"^^xsd:dateTime  ;
	skos:exactMatch subj:12009009 ;
	skos:exactMatch <https://www.wikidata.org/entity/Q747802> ;
	skos:broader	medtop:20000659 .

medtop:20000662
	rdf:type skos:Concept ;
	skos:prefLabel	"Old Catholic"@en-GB ;
	skos:definition	"Members of a catholic church which started in 1870 and denies the dogma of the infallibility of the pope"@en-GB ;
	skos:changeNote	"Retired in December 2021. Use Catholicism (medtop:20001344) instead."@en-GB ;
	skos:inScheme <http://cv.iptc.org/newscodes/mediatopic/>  ;
	ikos:created "2009-10-22T02:00:00+00:00"^^xsd:dateTime ;
	dct:created "2009-10-22T02:00:00+00:00"^^xsd:dateTime ;
	ikos:modified "2021-02-18T12:00:00+00:00"^^xsd:dateTime ;
	dct:modified "2021-02-18T12:00:00+00:00"^^xsd:dateTime  ; 
	ikos:retired "2021-12-17T12:00:00+00:00"^^xsd:dateTime ;
	skos:exactMatch subj:12009011 ;
	skos:exactMatch <https://www.wikidata.org/entity/Q5169816> ;
	skos:broader	medtop:20000659 .

medtop:20000663
	rdf:type skos:Concept ;
	skos:prefLabel	"Christian Orthodoxy"@en-GB ;
	skos:definition	"Eastern rite churches which are characterised by their continuity with the apostolic church, their liturgy and their territorial churches, mainly in eastern and south-eastern Europe and the Middle East"@en-GB ;
	skos:inScheme <http://cv.iptc.org/newscodes/mediatopic/>  ;
	ikos:created "2009-10-22T02:00:00+00:00"^^xsd:dateTime ;
	dct:created "2009-10-22T02:00:00+00:00"^^xsd:dateTime ;
	ikos:modified "2021-12-17T12:00:00+00:00"^^xsd:dateTime ;
	dct:modified "2021-12-17T12:00:00+00:00"^^xsd:dateTime  ;
	skos:exactMatch subj:12009012 ;
	skos:exactMatch <https://www.wikidata.org/entity/Q3333484> ;
	skos:broader	medtop:20000659 .

medtop:20000664
	rdf:type skos:Concept ;
	skos:prefLabel	"Protestantism"@en-GB ;
	skos:definition	"Christian denominations that were formed through the 16th century Reformation movement"@en-GB ;
	skos:inScheme <http://cv.iptc.org/newscodes/mediatopic/>  ;
	ikos:created "2009-10-22T02:00:00+00:00"^^xsd:dateTime ;
	dct:created "2009-10-22T02:00:00+00:00"^^xsd:dateTime ;
	ikos:modified "2021-12-17T12:00:00+00:00"^^xsd:dateTime ;
	dct:modified "2021-12-17T12:00:00+00:00"^^xsd:dateTime  ;
	skos:exactMatch subj:12009001 ;
	skos:exactMatch <https://www.wikidata.org/entity/Q23540> ;
	skos:broader	medtop:20000659 ;
	skos:narrower	medtop:20000665 ;
	skos:narrower	medtop:20000666 ;
	skos:narrower	medtop:20000667 ;
	skos:narrower	medtop:20000668 ;
	skos:narrower	medtop:20000669 ;
	skos:narrower	medtop:20000670 .

medtop:20000665
	rdf:type skos:Concept ;
	skos:prefLabel	"Anglican"@en-GB ;
	skos:definition	"Members of the worldwide Anglican communion which started in the 16th century in England as a breakaway church from the roman catholic church"@en-GB ;
	skos:changeNote	"Retired in December 2021. Use Protestantism (medtop:20000664) instead."@en-GB ;
	skos:inScheme <http://cv.iptc.org/newscodes/mediatopic/>  ;
	ikos:created "2009-10-22T02:00:00+00:00"^^xsd:dateTime ;
	dct:created "2009-10-22T02:00:00+00:00"^^xsd:dateTime ;
	ikos:modified "2021-02-18T12:00:00+00:00"^^xsd:dateTime ;
	dct:modified "2021-02-18T12:00:00+00:00"^^xsd:dateTime  ; 
	ikos:retired "2021-12-17T12:00:00+00:00"^^xsd:dateTime ;
	skos:exactMatch subj:12009004 ;
	skos:exactMatch <https://www.wikidata.org/entity/Q6423963> ;
	skos:broader	medtop:20000664 .

medtop:20000666
	rdf:type skos:Concept ;
	skos:prefLabel	"Baptist"@en-GB ;
	skos:definition	"Members of a Christian church which only baptises adults who truly believe in Christ"@en-GB ;
	skos:changeNote	"Retired in December 2021. Use Protestantism (medtop:20000664) instead."@en-GB ;
	skos:inScheme <http://cv.iptc.org/newscodes/mediatopic/>  ;
	ikos:created "2009-10-22T02:00:00+00:00"^^xsd:dateTime ;
	dct:created "2009-10-22T02:00:00+00:00"^^xsd:dateTime ;
	ikos:modified "2021-07-12T12:00:00+00:00"^^xsd:dateTime ;
	dct:modified "2021-07-12T12:00:00+00:00"^^xsd:dateTime  ; 
	ikos:retired "2021-12-17T12:00:00+00:00"^^xsd:dateTime ;
	skos:exactMatch subj:12009006 ;
	skos:exactMatch <https://www.wikidata.org/entity/Q93191> ;
	skos:broader	medtop:20000664 .

medtop:20000667
	rdf:type skos:Concept ;
	skos:prefLabel	"Lutheran"@en-GB ;
	skos:definition	"Christians who follow the teaching of reformer Martin Luther"@en-GB ;
	skos:changeNote	"Retired in December 2021. Use Protestantism (medtop:20000664) instead."@en-GB ;
	skos:inScheme <http://cv.iptc.org/newscodes/mediatopic/>  ;
	ikos:created "2009-10-22T02:00:00+00:00"^^xsd:dateTime ;
	dct:created "2009-10-22T02:00:00+00:00"^^xsd:dateTime ;
	ikos:modified "2021-02-18T12:00:00+00:00"^^xsd:dateTime ;
	dct:modified "2021-02-18T12:00:00+00:00"^^xsd:dateTime  ; 
	ikos:retired "2021-12-17T12:00:00+00:00"^^xsd:dateTime ;
	skos:exactMatch subj:12009002 ;
	skos:exactMatch <https://www.wikidata.org/entity/Q75809> ;
	skos:broader	medtop:20000664 .

medtop:20000668
	rdf:type skos:Concept ;
	skos:prefLabel	"Mennonite"@en-GB ;
	skos:definition	"Members of a 16th century Christian church which is against military service and baptising infants"@en-GB ;
	skos:changeNote	"Retired in December 2021. Use Protestantism (medtop:20000664) instead."@en-GB ;
	skos:inScheme <http://cv.iptc.org/newscodes/mediatopic/>  ;
	ikos:created "2009-10-22T02:00:00+00:00"^^xsd:dateTime ;
	dct:created "2009-10-22T02:00:00+00:00"^^xsd:dateTime ;
	ikos:modified "2021-12-17T12:00:00+00:00"^^xsd:dateTime ;
	dct:modified "2021-12-17T12:00:00+00:00"^^xsd:dateTime  ; 
	ikos:retired "2021-12-17T12:00:00+00:00"^^xsd:dateTime ;
	skos:exactMatch subj:12009007 ;
	skos:exactMatch <https://www.wikidata.org/entity/Q110223> ;
	skos:broader	medtop:20000664 .

medtop:20000669
	rdf:type skos:Concept ;
	skos:prefLabel	"Methodist"@en-GB ;
	skos:definition	"Followers of John and Charles Wesley who tried to reform the Church of England in the 18th century and turned into a separate church"@en-GB ;
	skos:changeNote	"Retired in December 2021. Use Protestantism (medtop:20000664) instead."@en-GB ;
	skos:inScheme <http://cv.iptc.org/newscodes/mediatopic/>  ;
	ikos:created "2009-10-22T02:00:00+00:00"^^xsd:dateTime ;
	dct:created "2009-10-22T02:00:00+00:00"^^xsd:dateTime ;
	ikos:modified "2021-02-18T12:00:00+00:00"^^xsd:dateTime ;
	dct:modified "2021-02-18T12:00:00+00:00"^^xsd:dateTime  ; 
	ikos:retired "2021-12-17T12:00:00+00:00"^^xsd:dateTime ;
	skos:exactMatch subj:12009005 ;
	skos:exactMatch <https://www.wikidata.org/entity/Q33203> ;
	skos:broader	medtop:20000664 .

medtop:20000670
	rdf:type skos:Concept ;
	skos:prefLabel	"Reformed"@en-GB ;
	skos:definition	"Christians who follow the teaching of reformers Johannes Calvin and Ulrich Zwingli"@en-GB ;
	skos:changeNote	"Retired in December 2021. Use Protestantism (medtop:20000664) instead."@en-GB ;
	skos:inScheme <http://cv.iptc.org/newscodes/mediatopic/>  ;
	ikos:created "2009-10-22T02:00:00+00:00"^^xsd:dateTime ;
	dct:created "2009-10-22T02:00:00+00:00"^^xsd:dateTime ;
	ikos:modified "2021-02-18T12:00:00+00:00"^^xsd:dateTime ;
	dct:modified "2021-02-18T12:00:00+00:00"^^xsd:dateTime  ; 
	ikos:retired "2021-12-17T12:00:00+00:00"^^xsd:dateTime ;
	skos:exactMatch subj:12009003 ;
	skos:exactMatch <https://www.wikidata.org/entity/Q101849> ;
	skos:broader	medtop:20000664 .

medtop:20000671
	rdf:type skos:Concept ;
	skos:prefLabel	"Roman Catholic"@en-GB ;
	skos:definition	"Biggest Christian church worldwide tracing its origins back to Jesus Christ"@en-GB ;
	skos:changeNote	"Retired in December 2021. Use Catholicism (medtop:20001344) instead."@en-GB ;
	skos:inScheme <http://cv.iptc.org/newscodes/mediatopic/>  ;
	ikos:created "2009-10-22T02:00:00+00:00"^^xsd:dateTime ;
	dct:created "2009-10-22T02:00:00+00:00"^^xsd:dateTime ;
	ikos:modified "2021-02-18T12:00:00+00:00"^^xsd:dateTime ;
	dct:modified "2021-02-18T12:00:00+00:00"^^xsd:dateTime  ; 
	ikos:retired "2021-12-17T12:00:00+00:00"^^xsd:dateTime ;
	skos:exactMatch subj:12009010 ;
	skos:exactMatch <https://www.wikidata.org/entity/Q9592> ;
	skos:broader	medtop:20000659 ;
	skos:narrower	medtop:20000672 .

medtop:20000672
	rdf:type skos:Concept ;
	skos:prefLabel	"concordat"@en-GB ;
	skos:definition	"Treaty between the Holy See and another country for the regulation of ecclesiastical affairs in the territory of the latter"@en-GB ;
	skos:changeNote	"Retired in December 2021. Use Catholicism (medtop:20001344) instead."@en-GB ;
	skos:inScheme <http://cv.iptc.org/newscodes/mediatopic/>  ;
	ikos:created "2009-10-22T02:00:00+00:00"^^xsd:dateTime ;
	dct:created "2009-10-22T02:00:00+00:00"^^xsd:dateTime ;
	ikos:modified "2021-12-17T12:00:00+00:00"^^xsd:dateTime ;
	dct:modified "2021-12-17T12:00:00+00:00"^^xsd:dateTime  ; 
	ikos:retired "2021-12-17T12:00:00+00:00"^^xsd:dateTime ;
	skos:exactMatch subj:12026000 ;
	skos:exactMatch <https://www.wikidata.org/entity/Q213541> ;
	skos:broader	medtop:20000671 .

medtop:20000673
	rdf:type skos:Concept ;
	skos:prefLabel	"Confucianism"@en-GB ;
	skos:definition	"A system of thought and behavior originating in ancient China and based on the teachings of the philosopher Confucius"@en-GB ;
	skos:inScheme <http://cv.iptc.org/newscodes/mediatopic/>  ;
	ikos:created "2009-10-22T02:00:00+00:00"^^xsd:dateTime ;
	dct:created "2009-10-22T02:00:00+00:00"^^xsd:dateTime ;
	ikos:modified "2021-12-17T12:00:00+00:00"^^xsd:dateTime ;
	dct:modified "2021-12-17T12:00:00+00:00"^^xsd:dateTime  ;
	skos:exactMatch subj:12022000 ;
	skos:exactMatch <https://www.wikidata.org/entity/Q9581> ;
	skos:broader	medtop:20000657 .

medtop:20000674
	rdf:type skos:Concept ;
	skos:prefLabel	"cult"@en-GB ;
	skos:definition	"A group that consists of followers who are fully devoted to a charismatic leader. Members are sometimes exploited financially or subject to emotional or physical harm"@en-GB ;
	skos:inScheme <http://cv.iptc.org/newscodes/mediatopic/>  ;
	ikos:created "2009-10-22T02:00:00+00:00"^^xsd:dateTime ;
	dct:created "2009-10-22T02:00:00+00:00"^^xsd:dateTime ;
	ikos:modified "2021-12-21T12:00:00+00:00"^^xsd:dateTime ;
	dct:modified "2021-12-21T12:00:00+00:00"^^xsd:dateTime  ;
	skos:exactMatch subj:12001000 ;
	skos:exactMatch <https://www.wikidata.org/entity/Q11038979> ;
	skos:broader	medtop:20000657 .

medtop:20000675
	rdf:type skos:Concept ;
	skos:prefLabel	"Freemasonry"@en-GB ;
	skos:definition	"A secret international society based on the principles of brotherhood, charity and mutual aid"@en-GB ;
	skos:changeNote	"Retired in December 2021"@en-GB ;
	skos:inScheme <http://cv.iptc.org/newscodes/mediatopic/>  ;
	ikos:created "2009-10-22T02:00:00+00:00"^^xsd:dateTime ;
	dct:created "2009-10-22T02:00:00+00:00"^^xsd:dateTime ;
	ikos:modified "2021-12-17T12:00:00+00:00"^^xsd:dateTime ;
	dct:modified "2021-12-17T12:00:00+00:00"^^xsd:dateTime  ; 
	ikos:retired "2021-12-17T12:00:00+00:00"^^xsd:dateTime ;
	skos:exactMatch subj:12003000 ;
	skos:exactMatch <https://www.wikidata.org/entity/Q41726> ;
	skos:broader	medtop:20000657 .

medtop:20000676
	rdf:type skos:Concept ;
	skos:prefLabel	"Hinduism"@en-GB ;
	skos:definition	"A religion and social system originating in India that includes a caste system, a belief in reincarnation and the worship of multiple deities"@en-GB ;
	skos:inScheme <http://cv.iptc.org/newscodes/mediatopic/>  ;
	ikos:created "2009-10-22T02:00:00+00:00"^^xsd:dateTime ;
	dct:created "2009-10-22T02:00:00+00:00"^^xsd:dateTime ;
	ikos:modified "2021-12-21T12:00:00+00:00"^^xsd:dateTime ;
	dct:modified "2021-12-21T12:00:00+00:00"^^xsd:dateTime  ;
	skos:exactMatch subj:12013000 ;
	skos:exactMatch <https://www.wikidata.org/entity/Q9089> ;
	skos:broader	medtop:20000657 .

medtop:20000677
	rdf:type skos:Concept ;
	skos:prefLabel	"Islam"@en-GB ;
	skos:definition	"Monotheistic religion that considers Muhammad as a prophet and the Qur'an as holy scripture"@en-GB ;
	skos:inScheme <http://cv.iptc.org/newscodes/mediatopic/>  ;
	ikos:created "2009-10-22T02:00:00+00:00"^^xsd:dateTime ;
	dct:created "2009-10-22T02:00:00+00:00"^^xsd:dateTime ;
	ikos:modified "2021-12-17T12:00:00+00:00"^^xsd:dateTime ;
	dct:modified "2021-12-17T12:00:00+00:00"^^xsd:dateTime  ;
	skos:exactMatch subj:12010000 ;
	skos:exactMatch <https://www.wikidata.org/entity/Q432> ;
	skos:broader	medtop:20000657 ;
	skos:narrower	medtop:20001347 ;
	skos:narrower	medtop:20001348 .

medtop:20000678
	rdf:type skos:Concept ;
	skos:prefLabel	"Jainism"@en-GB ;
	skos:definition	"A religion beginning in the 7th-5th century BC in India that teaches a path to spiritual purity and enlightenment through a disciplined mode of life founded upon the tradition of ahimsa, nonviolence to all living creatures"@en-GB ;
	skos:inScheme <http://cv.iptc.org/newscodes/mediatopic/>  ;
	ikos:created "2009-10-22T02:00:00+00:00"^^xsd:dateTime ;
	dct:created "2009-10-22T02:00:00+00:00"^^xsd:dateTime ;
	ikos:modified "2021-12-21T12:00:00+00:00"^^xsd:dateTime ;
	dct:modified "2021-12-21T12:00:00+00:00"^^xsd:dateTime  ;
	skos:exactMatch subj:12020000 ;
	skos:exactMatch <https://www.wikidata.org/entity/Q9232> ;
	skos:broader	medtop:20000657 .

medtop:20000679
	rdf:type skos:Concept ;
	skos:prefLabel	"Judaism"@en-GB ;
	skos:definition	"A monotheistic religion and culture that follows the teachings of the Torah"@en-GB ;
	skos:inScheme <http://cv.iptc.org/newscodes/mediatopic/>  ;
	ikos:created "2009-10-22T02:00:00+00:00"^^xsd:dateTime ;
	dct:created "2009-10-22T02:00:00+00:00"^^xsd:dateTime ;
	ikos:modified "2021-12-21T12:00:00+00:00"^^xsd:dateTime ;
	dct:modified "2021-12-21T12:00:00+00:00"^^xsd:dateTime  ;
	skos:exactMatch subj:12011000 ;
	skos:exactMatch <https://www.wikidata.org/entity/Q9268> ;
	skos:broader	medtop:20000657 ;
	skos:narrower	medtop:20001351 .

medtop:20000680
	rdf:type skos:Concept ;
	skos:prefLabel	"nature religion"@en-GB ;
	skos:definition	"Religions that believe nature and the natural world is an embodiment of divinity, sacredness or spiritual power, including indigenous religions practiced in various parts of the world, and modern Pagan faiths, such as Wicca"@en-GB ;
	skos:inScheme <http://cv.iptc.org/newscodes/mediatopic/>  ;
	ikos:created "2009-10-22T02:00:00+00:00"^^xsd:dateTime ;
	dct:created "2009-10-22T02:00:00+00:00"^^xsd:dateTime ;
	ikos:modified "2021-12-21T12:00:00+00:00"^^xsd:dateTime ;
	dct:modified "2021-12-21T12:00:00+00:00"^^xsd:dateTime  ;
	skos:exactMatch subj:12016000 ;
	skos:exactMatch <https://www.wikidata.org/entity/Q12291451> ;
	skos:broader	medtop:20000657 .

medtop:20000681
	rdf:type skos:Concept ;
	skos:prefLabel	"Zoroastrianism"@en-GB ;
	skos:definition	"A religion originating in ancient Iran following the teachings of the prophet Zoroaster, predicting the triumph of good over evil and exalting the benevolent deity of wisdom, Ahura Mazda (Wise Lord), as its supreme being"@en-GB ;
	skos:inScheme <http://cv.iptc.org/newscodes/mediatopic/>  ;
	ikos:created "2009-10-22T02:00:00+00:00"^^xsd:dateTime ;
	dct:created "2009-10-22T02:00:00+00:00"^^xsd:dateTime ;
	ikos:modified "2021-12-17T12:00:00+00:00"^^xsd:dateTime ;
	dct:modified "2021-12-17T12:00:00+00:00"^^xsd:dateTime  ;
	skos:exactMatch subj:12021000 ;
	skos:exactMatch <https://www.wikidata.org/entity/Q9601> ;
	skos:broader	medtop:20000657 .

medtop:20000682
	rdf:type skos:Concept ;
	skos:prefLabel	"Scientology"@en-GB ;
	skos:definition	"A set of beliefs and practices invented by American science fiction author L. Ron Hubbard asserting that a human is an immortal, spiritual being (Thetan) that is resident in a physical body"@en-GB ;
	skos:inScheme <http://cv.iptc.org/newscodes/mediatopic/>  ;
	ikos:created "2009-10-22T02:00:00+00:00"^^xsd:dateTime ;
	dct:created "2009-10-22T02:00:00+00:00"^^xsd:dateTime ;
	ikos:modified "2021-12-21T12:00:00+00:00"^^xsd:dateTime ;
	dct:modified "2021-12-21T12:00:00+00:00"^^xsd:dateTime  ;
	skos:exactMatch subj:12002002 ;
	skos:exactMatch <https://www.wikidata.org/entity/Q131036> ;
	skos:broader	medtop:20000657 .

medtop:20000683
	rdf:type skos:Concept ;
	skos:prefLabel	"Shintoism"@en-GB ;
	skos:definition	"An indigenous Japanese polytheistic religion that revolves around kami, supernatural entities believed to inhabit all things"@en-GB ;
	skos:inScheme <http://cv.iptc.org/newscodes/mediatopic/>  ;
	ikos:created "2009-10-22T02:00:00+00:00"^^xsd:dateTime ;
	dct:created "2009-10-22T02:00:00+00:00"^^xsd:dateTime ;
	ikos:modified "2021-12-17T12:00:00+00:00"^^xsd:dateTime ;
	dct:modified "2021-12-17T12:00:00+00:00"^^xsd:dateTime  ;
	skos:exactMatch subj:12018000 ;
	skos:exactMatch <https://www.wikidata.org/entity/Q812767> ;
	skos:broader	medtop:20000657 .

medtop:20000684
	rdf:type skos:Concept ;
	skos:prefLabel	"Sikhism"@en-GB ;
	skos:definition	"An Indian Dharmic religion that originated at the end of the 15th century CE in the Punjab region, developed from the spiritual teachings of Guru Nanak"@en-GB ;
	skos:inScheme <http://cv.iptc.org/newscodes/mediatopic/>  ;
	ikos:created "2009-10-22T02:00:00+00:00"^^xsd:dateTime ;
	dct:created "2009-10-22T02:00:00+00:00"^^xsd:dateTime ;
	ikos:modified "2021-12-17T12:00:00+00:00"^^xsd:dateTime ;
	dct:modified "2021-12-17T12:00:00+00:00"^^xsd:dateTime  ;
	skos:exactMatch subj:12019000 ;
	skos:exactMatch <https://www.wikidata.org/entity/Q9316> ;
	skos:broader	medtop:20000657 .

medtop:20000685
	rdf:type skos:Concept ;
	skos:prefLabel	"Taoism"@en-GB ;
	skos:definition	"A philosophical and spiritual tradition originating in the 4th century BCE in China which emphasizes living in harmony with the Tao, the source, pattern and substance of everything that exists"@en-GB ;
	skos:inScheme <http://cv.iptc.org/newscodes/mediatopic/>  ;
	ikos:created "2009-10-22T02:00:00+00:00"^^xsd:dateTime ;
	dct:created "2009-10-22T02:00:00+00:00"^^xsd:dateTime ;
	ikos:modified "2021-12-17T12:00:00+00:00"^^xsd:dateTime ;
	dct:modified "2021-12-17T12:00:00+00:00"^^xsd:dateTime  ;
	skos:exactMatch subj:12017000 ;
	skos:exactMatch <https://www.wikidata.org/entity/Q9598> ;
	skos:broader	medtop:20000657 .

medtop:20000686
	rdf:type skos:Concept ;
	skos:prefLabel	"Unificationism"@en-GB ;
	skos:definition	"A religion founded in 1954 in South Korea following the teachings of Rev. Syn Myung Moon and known for its mass wedding ceremonies"@en-GB ;
	skos:inScheme <http://cv.iptc.org/newscodes/mediatopic/>  ;
	ikos:created "2009-10-22T02:00:00+00:00"^^xsd:dateTime ;
	dct:created "2009-10-22T02:00:00+00:00"^^xsd:dateTime ;
	ikos:modified "2021-12-17T12:00:00+00:00"^^xsd:dateTime ;
	dct:modified "2021-12-17T12:00:00+00:00"^^xsd:dateTime  ;
	skos:exactMatch subj:12002001 ;
	skos:exactMatch <https://www.wikidata.org/entity/Q217059> ;
	skos:broader	medtop:20000657 .

medtop:20000687
	rdf:type skos:Concept ;
	skos:prefLabel	"interreligious dialogue"@en-GB ;
	skos:definition	"Any form of communication between religions"@en-GB ;
	skos:changeNote	"Retired in December 2021. Use religion (medtop:12000000) instead."@en-GB ;
	skos:inScheme <http://cv.iptc.org/newscodes/mediatopic/>  ;
	ikos:created "2009-10-22T02:00:00+00:00"^^xsd:dateTime ;
	dct:created "2009-10-22T02:00:00+00:00"^^xsd:dateTime ;
	ikos:modified "2021-02-18T12:00:00+00:00"^^xsd:dateTime ;
	dct:modified "2021-02-18T12:00:00+00:00"^^xsd:dateTime  ; 
	ikos:retired "2021-12-17T12:00:00+00:00"^^xsd:dateTime ;
	skos:exactMatch subj:12024000 ;
	skos:exactMatch <https://www.wikidata.org/entity/Q1304214> ;
	skos:broader	medtop:12000000 .

medtop:20000688
	rdf:type skos:Concept ;
	skos:prefLabel	"religious conflict"@en-GB ;
	skos:definition	"Conflicts involving religious differences"@en-GB ;
	skos:inScheme <http://cv.iptc.org/newscodes/mediatopic/>  ;
	ikos:created "2009-10-22T02:00:00+00:00"^^xsd:dateTime ;
	dct:created "2009-10-22T02:00:00+00:00"^^xsd:dateTime ;
	ikos:modified "2021-02-18T12:00:00+00:00"^^xsd:dateTime ;
	dct:modified "2021-02-18T12:00:00+00:00"^^xsd:dateTime  ;
	skos:exactMatch subj:16003004 ;
	skos:exactMatch <https://www.wikidata.org/entity/Q7311342> ;
	skos:broader	medtop:12000000 .

medtop:20000689
	rdf:type skos:Concept ;
	skos:prefLabel	"religious event"@en-GB ;
	skos:definition	"News regarding a religious event but not a festival or holiday"@en-GB ;
	skos:changeNote	"Retired in December 2021. Use religion (medtop:12000000) instead."@en-GB ;
	skos:inScheme <http://cv.iptc.org/newscodes/mediatopic/>  ;
	ikos:created "2009-10-22T02:00:00+00:00"^^xsd:dateTime ;
	dct:created "2009-10-22T02:00:00+00:00"^^xsd:dateTime ;
	ikos:modified "2021-07-12T12:00:00+00:00"^^xsd:dateTime ;
	dct:modified "2021-07-12T12:00:00+00:00"^^xsd:dateTime  ; 
	ikos:retired "2021-12-17T12:00:00+00:00"^^xsd:dateTime ;
	skos:exactMatch subj:12025000 ;
	skos:broader	medtop:12000000 .

medtop:20000690
	rdf:type skos:Concept ;
	skos:prefLabel	"religious festival and holiday"@en-GB ;
	skos:definition	"Holy day or period of observance in a religion which is sometimes a public holiday"@en-GB ;
	skos:inScheme <http://cv.iptc.org/newscodes/mediatopic/>  ;
	ikos:created "2009-10-22T02:00:00+00:00"^^xsd:dateTime ;
	dct:created "2009-10-22T02:00:00+00:00"^^xsd:dateTime ;
	ikos:modified "2021-12-17T12:00:00+00:00"^^xsd:dateTime ;
	dct:modified "2021-12-17T12:00:00+00:00"^^xsd:dateTime  ;
	skos:exactMatch subj:12014000 ;
	skos:exactMatch <https://www.wikidata.org/entity/Q375011> ;
	skos:broader	medtop:12000000 ;
	skos:narrower	medtop:20000691 ;
	skos:narrower	medtop:20000692 ;
	skos:narrower	medtop:20000693 ;
	skos:narrower	medtop:20000694 ;
	skos:narrower	medtop:20000695 ;
	skos:narrower	medtop:20001271 ;
	skos:narrower	medtop:20001272 ;
	skos:narrower	medtop:20001350 ;
	skos:narrower	medtop:20001352 .

medtop:20000691
	rdf:type skos:Concept ;
	skos:prefLabel	"Christmas"@en-GB ;
	skos:definition	"Christian holiday that celebrates the birth of Jesus Christ. Is also celebrated by many as a secular holiday."@en-GB ;
	skos:inScheme <http://cv.iptc.org/newscodes/mediatopic/>  ;
	ikos:created "2009-10-22T02:00:00+00:00"^^xsd:dateTime ;
	dct:created "2009-10-22T02:00:00+00:00"^^xsd:dateTime ;
	ikos:modified "2021-12-21T12:00:00+00:00"^^xsd:dateTime ;
	dct:modified "2021-12-21T12:00:00+00:00"^^xsd:dateTime  ;
	skos:exactMatch subj:12014001 ;
	skos:exactMatch <https://www.wikidata.org/entity/Q19809> ;
	skos:broader	medtop:20000690 .

medtop:20000692
	rdf:type skos:Concept ;
	skos:prefLabel	"Easter"@en-GB ;
	skos:definition	"Christian festival commemorating the resurrection of Jesus Christ. Is also celebrated by many as a secular holiday."@en-GB ;
	skos:inScheme <http://cv.iptc.org/newscodes/mediatopic/>  ;
	ikos:created "2009-10-22T02:00:00+00:00"^^xsd:dateTime ;
	dct:created "2009-10-22T02:00:00+00:00"^^xsd:dateTime ;
	ikos:modified "2021-12-17T12:00:00+00:00"^^xsd:dateTime ;
	dct:modified "2021-12-17T12:00:00+00:00"^^xsd:dateTime  ;
	skos:exactMatch subj:12014002 ;
	skos:exactMatch <https://www.wikidata.org/entity/Q21196> ;
	skos:broader	medtop:20000690 .

medtop:20000693
	rdf:type skos:Concept ;
	skos:prefLabel	"Pentecost"@en-GB ;
	skos:definition	"Christian festival, celebrated on the 50th day after Easter commemorating the descent of the Holy Spirit, also known as Whitsun"@en-GB ;
	skos:inScheme <http://cv.iptc.org/newscodes/mediatopic/>  ;
	ikos:created "2009-10-22T02:00:00+00:00"^^xsd:dateTime ;
	dct:created "2009-10-22T02:00:00+00:00"^^xsd:dateTime ;
	ikos:modified "2021-12-17T12:00:00+00:00"^^xsd:dateTime ;
	dct:modified "2021-12-17T12:00:00+00:00"^^xsd:dateTime  ;
	skos:exactMatch subj:12014003 ;
	skos:exactMatch <https://www.wikidata.org/entity/Q39864> ;
	skos:broader	medtop:20000690 .

medtop:20000694
	rdf:type skos:Concept ;
	skos:prefLabel	"Ramadan"@en-GB ;
	skos:definition	"Holy month of fasting in Islam concluding in Eid al-Fitr"@en-GB ;
	skos:inScheme <http://cv.iptc.org/newscodes/mediatopic/>  ;
	ikos:created "2009-10-22T02:00:00+00:00"^^xsd:dateTime ;
	dct:created "2009-10-22T02:00:00+00:00"^^xsd:dateTime ;
	ikos:modified "2021-12-17T12:00:00+00:00"^^xsd:dateTime ;
	dct:modified "2021-12-17T12:00:00+00:00"^^xsd:dateTime  ;
	skos:exactMatch subj:12014004 ;
	skos:exactMatch <https://www.wikidata.org/entity/Q41662> ;
	skos:broader	medtop:20000690 .

medtop:20000695
	rdf:type skos:Concept ;
	skos:prefLabel	"Yom Kippur"@en-GB ;
	skos:definition	"Most solemn of Jewish religious holidays, observed on the 10th day of the lunar month of tishri by fasting and prayer from sunset to sundown the following day"@en-GB ;
	skos:inScheme <http://cv.iptc.org/newscodes/mediatopic/>  ;
	ikos:created "2009-10-22T02:00:00+00:00"^^xsd:dateTime ;
	dct:created "2009-10-22T02:00:00+00:00"^^xsd:dateTime ;
	ikos:modified "2021-12-17T12:00:00+00:00"^^xsd:dateTime ;
	dct:modified "2021-12-17T12:00:00+00:00"^^xsd:dateTime  ;
	skos:exactMatch subj:12014005 ;
	skos:exactMatch <https://www.wikidata.org/entity/Q132994> ;
	skos:broader	medtop:20000690 .

medtop:20000696
	rdf:type skos:Concept ;
	skos:prefLabel	"religious ritual"@en-GB ;
	skos:definition	"Established religious rituals such as mass, baptism, prayer meetings and bar and bat mitzvah"@en-GB ;
	skos:inScheme <http://cv.iptc.org/newscodes/mediatopic/>  ;
	ikos:created "2009-10-22T02:00:00+00:00"^^xsd:dateTime ;
	dct:created "2009-10-22T02:00:00+00:00"^^xsd:dateTime ;
	ikos:modified "2021-12-17T12:00:00+00:00"^^xsd:dateTime ;
	dct:modified "2021-12-17T12:00:00+00:00"^^xsd:dateTime  ;
	skos:exactMatch subj:12025004 ;
	skos:exactMatch <https://www.wikidata.org/entity/Q2110808> ;
	skos:broader	medtop:12000000 ;
	skos:narrower	medtop:20001273 ;
	skos:narrower	medtop:20001345 ;
	skos:narrower	medtop:20001346 .

medtop:20000697
	rdf:type skos:Concept ;
	skos:prefLabel	"religious facility"@en-GB ;
	skos:definition	"Any facility where a group carries out its religious rites"@en-GB ;
	skos:inScheme <http://cv.iptc.org/newscodes/mediatopic/>  ;
	ikos:created "2009-10-22T02:00:00+00:00"^^xsd:dateTime ;
	dct:created "2009-10-22T02:00:00+00:00"^^xsd:dateTime ;
	ikos:modified "2021-12-17T12:00:00+00:00"^^xsd:dateTime ;
	dct:modified "2021-12-17T12:00:00+00:00"^^xsd:dateTime  ;
	skos:broadMatch subj:12000000 ;
	skos:exactMatch <https://www.wikidata.org/entity/Q24398318> ;
	skos:broader	medtop:12000000 ;
	skos:narrower	medtop:20000698 ;
	skos:narrower	medtop:20000699 ;
	skos:narrower	medtop:20000700 ;
	skos:narrower	medtop:20000701 .

medtop:20000698
	rdf:type skos:Concept ;
	skos:prefLabel	"church"@en-GB ;
	skos:definition	"A building used as a place of worship for the Christian religion"@en-GB ;
	skos:inScheme <http://cv.iptc.org/newscodes/mediatopic/>  ;
	ikos:created "2009-10-22T02:00:00+00:00"^^xsd:dateTime ;
	dct:created "2009-10-22T02:00:00+00:00"^^xsd:dateTime ;
	ikos:modified "2021-12-17T12:00:00+00:00"^^xsd:dateTime ;
	dct:modified "2021-12-17T12:00:00+00:00"^^xsd:dateTime  ;
	skos:broadMatch subj:12000000 ;
	skos:exactMatch <https://www.wikidata.org/entity/Q16970> ;
	skos:broader	medtop:20000697 .

medtop:20000699
	rdf:type skos:Concept ;
	skos:prefLabel	"mosque"@en-GB ;
	skos:definition	"A building used as a place of worship for the Islamic religion"@en-GB ;
	skos:inScheme <http://cv.iptc.org/newscodes/mediatopic/>  ;
	ikos:created "2009-10-22T02:00:00+00:00"^^xsd:dateTime ;
	dct:created "2009-10-22T02:00:00+00:00"^^xsd:dateTime ;
	ikos:modified "2021-12-17T12:00:00+00:00"^^xsd:dateTime ;
	dct:modified "2021-12-17T12:00:00+00:00"^^xsd:dateTime  ;
	skos:broadMatch subj:12000000 ;
	skos:exactMatch <https://www.wikidata.org/entity/Q32815> ;
	skos:broader	medtop:20000697 .

medtop:20000700
	rdf:type skos:Concept ;
	skos:prefLabel	"synagogue"@en-GB ;
	skos:definition	"A building used as a place of worship for the Jewish religion"@en-GB ;
	skos:inScheme <http://cv.iptc.org/newscodes/mediatopic/>  ;
	ikos:created "2009-10-22T02:00:00+00:00"^^xsd:dateTime ;
	dct:created "2009-10-22T02:00:00+00:00"^^xsd:dateTime ;
	ikos:modified "2021-12-17T12:00:00+00:00"^^xsd:dateTime ;
	dct:modified "2021-12-17T12:00:00+00:00"^^xsd:dateTime  ;
	skos:broadMatch subj:12000000 ;
	skos:exactMatch <https://www.wikidata.org/entity/Q34627> ;
	skos:broader	medtop:20000697 .

medtop:20000701
	rdf:type skos:Concept ;
	skos:prefLabel	"temple"@en-GB ;
	skos:definition	"Generally an edifice identifiable as a place of worship"@en-GB ;
	skos:changeNote	"Retired in December 2021. Use religious facility (medtop:20000697) instead."@en-GB ;
	skos:inScheme <http://cv.iptc.org/newscodes/mediatopic/>  ;
	ikos:created "2009-10-22T02:00:00+00:00"^^xsd:dateTime ;
	dct:created "2009-10-22T02:00:00+00:00"^^xsd:dateTime ;
	ikos:modified "2021-02-18T12:00:00+00:00"^^xsd:dateTime ;
	dct:modified "2021-02-18T12:00:00+00:00"^^xsd:dateTime  ; 
	ikos:retired "2021-12-17T12:00:00+00:00"^^xsd:dateTime ;
	skos:broadMatch subj:12000000 ;
	skos:exactMatch <https://www.wikidata.org/entity/Q44539> ;
	skos:broader	medtop:20000697 .

medtop:20000702
	rdf:type skos:Concept ;
	skos:prefLabel	"relations between religion and government"@en-GB ;
	skos:definition	"Matters arising from the relationship between religions and a government, including the question of whether churches should pay taxes, the push to keep religion out of publicly funded institutions and the freedom, or lack of to waer religious symbols in a school setting"@en-GB ;
	skos:inScheme <http://cv.iptc.org/newscodes/mediatopic/>  ;
	ikos:created "2009-10-22T02:00:00+00:00"^^xsd:dateTime ;
	dct:created "2009-10-22T02:00:00+00:00"^^xsd:dateTime ;
	ikos:modified "2021-12-21T12:00:00+00:00"^^xsd:dateTime ;
	dct:modified "2021-12-21T12:00:00+00:00"^^xsd:dateTime  ;
	skos:exactMatch subj:12007000 ;
	skos:exactMatch <https://www.wikidata.org/entity/Q753623> ;
	skos:broader	medtop:12000000 .

medtop:20000703
	rdf:type skos:Concept ;
	skos:prefLabel	"religious leader"@en-GB ;
	skos:definition	"Person or persons who have a ritual, juridical or otherwise leading role in their respective church or religion"@en-GB ;
	skos:inScheme <http://cv.iptc.org/newscodes/mediatopic/>  ;
	ikos:created "2009-10-22T02:00:00+00:00"^^xsd:dateTime ;
	dct:created "2009-10-22T02:00:00+00:00"^^xsd:dateTime ;
	ikos:modified "2021-02-18T12:00:00+00:00"^^xsd:dateTime ;
	dct:modified "2021-02-18T12:00:00+00:00"^^xsd:dateTime  ;
	skos:exactMatch subj:12015000 ;
	skos:exactMatch <https://www.wikidata.org/entity/Q15995642> ;
	skos:broader	medtop:12000000 ;
	skos:narrower	medtop:20000704 .

medtop:20000704
	rdf:type skos:Concept ;
	skos:prefLabel	"pope"@en-GB ;
	skos:definition	"Head of the Roman Catholic Church worldwide"@en-GB ;
	skos:inScheme <http://cv.iptc.org/newscodes/mediatopic/>  ;
	ikos:created "2009-10-22T02:00:00+00:00"^^xsd:dateTime ;
	dct:created "2009-10-22T02:00:00+00:00"^^xsd:dateTime ;
	ikos:modified "2021-12-17T12:00:00+00:00"^^xsd:dateTime ;
	dct:modified "2021-12-17T12:00:00+00:00"^^xsd:dateTime  ;
	skos:exactMatch subj:12015001 ;
	skos:exactMatch <https://www.wikidata.org/entity/Q19546> ;
	skos:broader	medtop:20000703 .

medtop:20000705
	rdf:type skos:Concept ;
	skos:prefLabel	"religious text"@en-GB ;
	skos:definition	"Texts regarded as holy or important by a religion"@en-GB ;
	skos:inScheme <http://cv.iptc.org/newscodes/mediatopic/>  ;
	ikos:created "2009-10-22T02:00:00+00:00"^^xsd:dateTime ;
	dct:created "2009-10-22T02:00:00+00:00"^^xsd:dateTime ;
	ikos:modified "2021-12-17T12:00:00+00:00"^^xsd:dateTime ;
	dct:modified "2021-12-17T12:00:00+00:00"^^xsd:dateTime  ;
	skos:exactMatch subj:12023000 ;
	skos:exactMatch <https://www.wikidata.org/entity/Q179461> ;
	skos:broader	medtop:12000000 ;
	skos:narrower	medtop:20000706 ;
	skos:narrower	medtop:20000707 ;
	skos:narrower	medtop:20000708 .

medtop:20000706
	rdf:type skos:Concept ;
	skos:prefLabel	"Bible"@en-GB ;
	skos:definition	"Holy book of Christianity"@en-GB ;
	skos:inScheme <http://cv.iptc.org/newscodes/mediatopic/>  ;
	ikos:created "2009-10-22T02:00:00+00:00"^^xsd:dateTime ;
	dct:created "2009-10-22T02:00:00+00:00"^^xsd:dateTime ;
	ikos:modified "2021-12-17T12:00:00+00:00"^^xsd:dateTime ;
	dct:modified "2021-12-17T12:00:00+00:00"^^xsd:dateTime  ;
	skos:exactMatch subj:12023001 ;
	skos:exactMatch <https://www.wikidata.org/entity/Q1845> ;
	skos:broader	medtop:20000705 .

medtop:20000707
	rdf:type skos:Concept ;
	skos:prefLabel	"Qur'an"@en-GB ;
	skos:definition	"Holy book of Islam"@en-GB ;
	skos:inScheme <http://cv.iptc.org/newscodes/mediatopic/>  ;
	ikos:created "2009-10-22T02:00:00+00:00"^^xsd:dateTime ;
	dct:created "2009-10-22T02:00:00+00:00"^^xsd:dateTime ;
	ikos:modified "2021-02-18T12:00:00+00:00"^^xsd:dateTime ;
	dct:modified "2021-02-18T12:00:00+00:00"^^xsd:dateTime  ;
	skos:exactMatch subj:12023002 ;
	skos:exactMatch <https://www.wikidata.org/entity/Q428> ;
	skos:broader	medtop:20000705 .

medtop:20000708
	rdf:type skos:Concept ;
	skos:prefLabel	"Torah"@en-GB ;
	skos:definition	"Holy book of Judaism"@en-GB ;
	skos:inScheme <http://cv.iptc.org/newscodes/mediatopic/>  ;
	ikos:created "2009-10-22T02:00:00+00:00"^^xsd:dateTime ;
	dct:created "2009-10-22T02:00:00+00:00"^^xsd:dateTime ;
	ikos:modified "2021-12-17T12:00:00+00:00"^^xsd:dateTime ;
	dct:modified "2021-12-17T12:00:00+00:00"^^xsd:dateTime  ;
	skos:exactMatch subj:12023003 ;
	skos:exactMatch <https://www.wikidata.org/entity/Q34990> ;
	skos:broader	medtop:20000705 .

medtop:20000710
	rdf:type skos:Concept ;
	skos:prefLabel	"biomedical science"@en-GB ;
	skos:definition	"The application of biology-based science to medical fields such as research, health monitoring or medical treatment"@en-GB ;
	skos:inScheme <http://cv.iptc.org/newscodes/mediatopic/>  ;
	ikos:created "2009-10-22T02:00:00+00:00"^^xsd:dateTime ;
	dct:created "2009-10-22T02:00:00+00:00"^^xsd:dateTime ;
	ikos:modified "2021-02-18T12:00:00+00:00"^^xsd:dateTime ;
	dct:modified "2021-02-18T12:00:00+00:00"^^xsd:dateTime  ;
	skos:broadMatch subj:13019000 ;
	skos:exactMatch <https://www.wikidata.org/entity/Q16745563> ;
	skos:broader	medtop:13000000 ;
	skos:narrower	medtop:20000711 .

medtop:20000711
	rdf:type skos:Concept ;
	skos:prefLabel	"biotechnology"@en-GB ;
	skos:definition	"The scientific manipulation of living organisms and biological processes for scientific, medical or agricultural purposes"@en-GB ;
	skos:inScheme <http://cv.iptc.org/newscodes/mediatopic/>  ;
	ikos:created "2009-10-22T02:00:00+00:00"^^xsd:dateTime ;
	dct:created "2009-10-22T02:00:00+00:00"^^xsd:dateTime ;
	ikos:modified "2021-02-18T12:00:00+00:00"^^xsd:dateTime ;
	dct:modified "2021-02-18T12:00:00+00:00"^^xsd:dateTime  ;
	skos:exactMatch subj:13019000 ;
	skos:exactMatch <https://www.wikidata.org/entity/Q7108> ;
	skos:broader	medtop:20000710 .

medtop:20000712
	rdf:type skos:Concept ;
	skos:prefLabel	"dentistry"@en-GB ;
	skos:definition	"The medical profession and field of study devoted to diagnosing, preventing and treating oral conditions"@en-GB ;
	skos:inScheme <http://cv.iptc.org/newscodes/mediatopic/>  ;
	ikos:created "2009-10-22T02:00:00+00:00"^^xsd:dateTime ;
	dct:created "2009-10-22T02:00:00+00:00"^^xsd:dateTime ;
	ikos:modified "2021-02-18T12:00:00+00:00"^^xsd:dateTime ;
	dct:modified "2021-02-18T12:00:00+00:00"^^xsd:dateTime  ;
	skos:broadMatch subj:13019000 ;
	skos:exactMatch <https://www.wikidata.org/entity/Q12128> ;
	skos:broader	medtop:20000487 .

medtop:20000713
	rdf:type skos:Concept ;
	skos:prefLabel	"pharmacology"@en-GB ;
	skos:definition	"The medical profession and field of study concerned with the uses, modes of action and effects of pharmaceutical agents"@en-GB ;
	skos:changeNote	"Retired. Use medtop:20000468 prescription drugs instead."@en-GB ;
	skos:inScheme <http://cv.iptc.org/newscodes/mediatopic/>  ;
	ikos:created "2009-10-22T02:00:00+00:00"^^xsd:dateTime ;
	dct:created "2009-10-22T02:00:00+00:00"^^xsd:dateTime ;
	ikos:modified "2022-06-14T12:00:00+00:00"^^xsd:dateTime ;
	dct:modified "2022-06-14T12:00:00+00:00"^^xsd:dateTime  ; 
	ikos:retired "2022-06-14T12:00:00+00:00"^^xsd:dateTime ;
	skos:broadMatch subj:13019000 ;
	skos:exactMatch <https://www.wikidata.org/entity/Q128406> ;
	skos:broader	medtop:20000487 .

medtop:20000714
	rdf:type skos:Concept ;
	skos:prefLabel	"veterinary medicine"@en-GB ;
	skos:definition	"The medical profession and field of study devoted to diagnosis, prevention and treatment of medical conditions in animals"@en-GB ;
	skos:inScheme <http://cv.iptc.org/newscodes/mediatopic/>  ;
	ikos:created "2009-10-22T02:00:00+00:00"^^xsd:dateTime ;
	dct:created "2009-10-22T02:00:00+00:00"^^xsd:dateTime ;
	ikos:modified "2021-02-18T12:00:00+00:00"^^xsd:dateTime ;
	dct:modified "2021-02-18T12:00:00+00:00"^^xsd:dateTime  ;
	skos:broadMatch subj:13019000 ;
	skos:exactMatch <https://www.wikidata.org/entity/Q170201> ;
	skos:broader	medtop:20000487 .

medtop:20000715
	rdf:type skos:Concept ;
	skos:prefLabel	"mathematics"@en-GB ;
	skos:definition	"The study of structure, space, change and number in abstract, often using symbolic logic and language, and including subjects such as geometry, algebra or trigonometry"@en-GB ;
	skos:inScheme <http://cv.iptc.org/newscodes/mediatopic/>  ;
	ikos:created "2009-10-22T02:00:00+00:00"^^xsd:dateTime ;
	dct:created "2009-10-22T02:00:00+00:00"^^xsd:dateTime ;
	ikos:modified "2021-02-18T12:00:00+00:00"^^xsd:dateTime ;
	dct:modified "2021-02-18T12:00:00+00:00"^^xsd:dateTime  ;
	skos:exactMatch subj:13018000 ;
	skos:exactMatch <https://www.wikidata.org/entity/Q395> ;
	skos:broader	medtop:13000000 .

medtop:20000716
	rdf:type skos:Concept ;
	skos:prefLabel	"mechanical engineering"@en-GB ;
	skos:definition	"The study and application of the design, construction and operation of mechanical systems"@en-GB ;
	skos:inScheme <http://cv.iptc.org/newscodes/mediatopic/>  ;
	ikos:created "2009-10-22T02:00:00+00:00"^^xsd:dateTime ;
	dct:created "2009-10-22T02:00:00+00:00"^^xsd:dateTime ;
	ikos:modified "2021-02-18T12:00:00+00:00"^^xsd:dateTime ;
	dct:modified "2021-02-18T12:00:00+00:00"^^xsd:dateTime  ;
	skos:broadMatch subj:13002000 ;
	skos:exactMatch <https://www.wikidata.org/entity/Q101333> ;
	skos:broader	medtop:20000756 .

medtop:20000717
	rdf:type skos:Concept ;
	skos:prefLabel	"natural science"@en-GB ;
	skos:definition	"The sciences that deal with matter, energy and the physical world, including physics, biology, chemistry and astronomy"@en-GB ;
	skos:inScheme <http://cv.iptc.org/newscodes/mediatopic/>  ;
	ikos:created "2009-10-22T02:00:00+00:00"^^xsd:dateTime ;
	dct:created "2009-10-22T02:00:00+00:00"^^xsd:dateTime ;
	ikos:modified "2021-02-18T12:00:00+00:00"^^xsd:dateTime ;
	dct:modified "2021-02-18T12:00:00+00:00"^^xsd:dateTime  ;
	skos:exactMatch subj:13004000 ;
	skos:exactMatch <https://www.wikidata.org/entity/Q7991> ;
	skos:broader	medtop:13000000 ;
	skos:narrower	medtop:20000718 ;
	skos:narrower	medtop:20000719 ;
	skos:narrower	medtop:20000725 ;
	skos:narrower	medtop:20000726 ;
	skos:narrower	medtop:20000727 ;
	skos:narrower	medtop:20000728 ;
	skos:narrower	medtop:20000729 ;
	skos:narrower	medtop:20000730 ;
	skos:narrower	medtop:20000731 .

medtop:20000718
	rdf:type skos:Concept ;
	skos:prefLabel	"astronomy"@en-GB ;
	skos:definition	"The study of celestial objects through direct observation and theoretical models"@en-GB ;
	skos:inScheme <http://cv.iptc.org/newscodes/mediatopic/>  ;
	ikos:created "2009-10-22T02:00:00+00:00"^^xsd:dateTime ;
	dct:created "2009-10-22T02:00:00+00:00"^^xsd:dateTime ;
	ikos:modified "2021-02-18T12:00:00+00:00"^^xsd:dateTime ;
	dct:modified "2021-02-18T12:00:00+00:00"^^xsd:dateTime  ;
	skos:exactMatch subj:13004007 ;
	skos:exactMatch <https://www.wikidata.org/entity/Q333> ;
	skos:broader	medtop:20000717 .

medtop:20000719
	rdf:type skos:Concept ;
	skos:prefLabel	"biology"@en-GB ;
	skos:definition	"The study of the anatomy, behaviour, origin, physiology and other aspects of living organisms"@en-GB ;
	skos:inScheme <http://cv.iptc.org/newscodes/mediatopic/>  ;
	ikos:created "2009-10-22T02:00:00+00:00"^^xsd:dateTime ;
	dct:created "2009-10-22T02:00:00+00:00"^^xsd:dateTime ;
	ikos:modified "2021-02-18T12:00:00+00:00"^^xsd:dateTime ;
	dct:modified "2021-02-18T12:00:00+00:00"^^xsd:dateTime  ;
	skos:exactMatch subj:13004008 ;
	skos:exactMatch <https://www.wikidata.org/entity/Q420> ;
	skos:broader	medtop:20000717 ;
	skos:narrower	medtop:20000720 ;
	skos:narrower	medtop:20000721 ;
	skos:narrower	medtop:20000722 ;
	skos:narrower	medtop:20000723 ;
	skos:narrower	medtop:20000724 .

medtop:20000720
	rdf:type skos:Concept ;
	skos:prefLabel	"botany"@en-GB ;
	skos:definition	"The study of the physical and physiological structure, genetics, ecology and other aspects of plants"@en-GB ;
	skos:inScheme <http://cv.iptc.org/newscodes/mediatopic/>  ;
	ikos:created "2009-10-22T02:00:00+00:00"^^xsd:dateTime ;
	dct:created "2009-10-22T02:00:00+00:00"^^xsd:dateTime ;
	ikos:modified "2021-02-18T12:00:00+00:00"^^xsd:dateTime ;
	dct:modified "2021-02-18T12:00:00+00:00"^^xsd:dateTime  ;
	skos:exactMatch subj:13004004 ;
	skos:exactMatch <https://www.wikidata.org/entity/Q441> ;
	skos:broader	medtop:20000719 .

medtop:20000721
	rdf:type skos:Concept ;
	skos:prefLabel	"genetics"@en-GB ;
	skos:definition	"The study of genes in living organisms, and of their role in heredity, development or genetic adaptation"@en-GB ;
	skos:inScheme <http://cv.iptc.org/newscodes/mediatopic/>  ;
	ikos:created "2009-10-22T02:00:00+00:00"^^xsd:dateTime ;
	dct:created "2009-10-22T02:00:00+00:00"^^xsd:dateTime ;
	ikos:modified "2021-02-18T12:00:00+00:00"^^xsd:dateTime ;
	dct:modified "2021-02-18T12:00:00+00:00"^^xsd:dateTime  ;
	skos:exactMatch subj:07014004 ;
	skos:exactMatch <https://www.wikidata.org/entity/Q7162> ;
	skos:broader	medtop:20000719 .

medtop:20000722
	rdf:type skos:Concept ;
	skos:prefLabel	"palaeontology"@en-GB ;
	skos:definition	"The study of prehistoric life forms, geological periods and fossils"@en-GB ;
	skos:inScheme <http://cv.iptc.org/newscodes/mediatopic/>  ;
	ikos:created "2009-10-22T02:00:00+00:00"^^xsd:dateTime ;
	dct:created "2009-10-22T02:00:00+00:00"^^xsd:dateTime ;
	ikos:modified "2021-02-18T12:00:00+00:00"^^xsd:dateTime ;
	dct:modified "2021-02-18T12:00:00+00:00"^^xsd:dateTime  ;
	skos:exactMatch subj:13004002 ;
	skos:exactMatch <https://www.wikidata.org/entity/Q7205> ;
	skos:broader	medtop:20000719 .

medtop:20000723
	rdf:type skos:Concept ;
	skos:prefLabel	"physiology"@en-GB ;
	skos:definition	"The study of the vital processes, internal organs or functional mechanisms of living organisms"@en-GB ;
	skos:inScheme <http://cv.iptc.org/newscodes/mediatopic/>  ;
	ikos:created "2009-10-22T02:00:00+00:00"^^xsd:dateTime ;
	dct:created "2009-10-22T02:00:00+00:00"^^xsd:dateTime ;
	ikos:modified "2021-02-18T12:00:00+00:00"^^xsd:dateTime ;
	dct:modified "2021-02-18T12:00:00+00:00"^^xsd:dateTime  ;
	skos:exactMatch subj:13004006 ;
	skos:exactMatch <https://www.wikidata.org/entity/Q521> ;
	skos:broader	medtop:20000719 .

medtop:20000724
	rdf:type skos:Concept ;
	skos:prefLabel	"zoology"@en-GB ;
	skos:definition	"The study of the biology, physiology, development, behaviour or other aspects of animals"@en-GB ;
	skos:inScheme <http://cv.iptc.org/newscodes/mediatopic/>  ;
	ikos:created "2009-10-22T02:00:00+00:00"^^xsd:dateTime ;
	dct:created "2009-10-22T02:00:00+00:00"^^xsd:dateTime ;
	ikos:modified "2021-02-18T12:00:00+00:00"^^xsd:dateTime ;
	dct:modified "2021-02-18T12:00:00+00:00"^^xsd:dateTime  ;
	skos:exactMatch subj:13004005 ;
	skos:exactMatch <https://www.wikidata.org/entity/Q431> ;
	skos:broader	medtop:20000719 .

medtop:20000725
	rdf:type skos:Concept ;
	skos:prefLabel	"chemistry"@en-GB ;
	skos:definition	"The study of the composition and properties of matter on the scale of atoms and molecules, and of the reactions between compounds"@en-GB ;
	skos:inScheme <http://cv.iptc.org/newscodes/mediatopic/>  ;
	ikos:created "2009-10-22T02:00:00+00:00"^^xsd:dateTime ;
	dct:created "2009-10-22T02:00:00+00:00"^^xsd:dateTime ;
	ikos:modified "2021-02-18T12:00:00+00:00"^^xsd:dateTime ;
	dct:modified "2021-02-18T12:00:00+00:00"^^xsd:dateTime  ;
	skos:exactMatch subj:13001002 ;
	skos:exactMatch <https://www.wikidata.org/entity/Q2329> ;
	skos:broader	medtop:20000717 .

medtop:20000726
	rdf:type skos:Concept ;
	skos:prefLabel	"cosmology"@en-GB ;
	skos:definition	"The study of the origin, evolution, organisation and structure of the universe"@en-GB ;
	skos:inScheme <http://cv.iptc.org/newscodes/mediatopic/>  ;
	ikos:created "2009-10-22T02:00:00+00:00"^^xsd:dateTime ;
	dct:created "2009-10-22T02:00:00+00:00"^^xsd:dateTime ;
	ikos:modified "2021-02-18T12:00:00+00:00"^^xsd:dateTime ;
	dct:modified "2021-02-18T12:00:00+00:00"^^xsd:dateTime  ;
	skos:exactMatch subj:13001003 ;
	skos:exactMatch <https://www.wikidata.org/entity/Q338> ;
	skos:broader	medtop:20000717 .

medtop:20000727
	rdf:type skos:Concept ;
	skos:prefLabel	"geology"@en-GB ;
	skos:definition	"The study of Earth's physical processes, material structures and its properties"@en-GB ;
	skos:inScheme <http://cv.iptc.org/newscodes/mediatopic/>  ;
	ikos:created "2009-10-22T02:00:00+00:00"^^xsd:dateTime ;
	dct:created "2009-10-22T02:00:00+00:00"^^xsd:dateTime ;
	ikos:modified "2021-02-18T12:00:00+00:00"^^xsd:dateTime ;
	dct:modified "2021-02-18T12:00:00+00:00"^^xsd:dateTime  ;
	skos:exactMatch subj:13004001 ;
	skos:exactMatch <https://www.wikidata.org/entity/Q1069> ;
	skos:broader	medtop:20000717 .

medtop:20000728
	rdf:type skos:Concept ;
	skos:prefLabel	"horticulture"@en-GB ;
	skos:definition	"The study and art of plant cultivation, including landscape and garden design and plant conservation"@en-GB ;
	skos:inScheme <http://cv.iptc.org/newscodes/mediatopic/>  ;
	ikos:created "2009-10-22T02:00:00+00:00"^^xsd:dateTime ;
	dct:created "2009-10-22T02:00:00+00:00"^^xsd:dateTime ;
	ikos:modified "2021-02-18T12:00:00+00:00"^^xsd:dateTime ;
	dct:modified "2021-02-18T12:00:00+00:00"^^xsd:dateTime  ;
	skos:broadMatch subj:13004000 ;
	skos:exactMatch <https://www.wikidata.org/entity/Q48803> ;
	skos:broader	medtop:20000717 .

medtop:20000729
	rdf:type skos:Concept ;
	skos:prefLabel	"marine science"@en-GB ;
	skos:definition	"The study of living organisms and environments in saltwater ecosystems"@en-GB ;
	skos:inScheme <http://cv.iptc.org/newscodes/mediatopic/>  ;
	ikos:created "2009-10-22T02:00:00+00:00"^^xsd:dateTime ;
	dct:created "2009-10-22T02:00:00+00:00"^^xsd:dateTime ;
	ikos:modified "2021-02-18T12:00:00+00:00"^^xsd:dateTime ;
	dct:modified "2021-02-18T12:00:00+00:00"^^xsd:dateTime  ;
	skos:exactMatch subj:13014000 ;
	skos:exactMatch <https://www.wikidata.org/entity/Q24577909> ;
	skos:broader	medtop:20000717 .

medtop:20000730
	rdf:type skos:Concept ;
	skos:prefLabel	"meteorology"@en-GB ;
	skos:definition	"The study of atmospheric chemistry and physics, with a focus on weather forecasting"@en-GB ;
	skos:inScheme <http://cv.iptc.org/newscodes/mediatopic/>  ;
	ikos:created "2009-10-22T02:00:00+00:00"^^xsd:dateTime ;
	dct:created "2009-10-22T02:00:00+00:00"^^xsd:dateTime ;
	ikos:modified "2021-02-18T12:00:00+00:00"^^xsd:dateTime ;
	dct:modified "2021-02-18T12:00:00+00:00"^^xsd:dateTime  ;
	skos:exactMatch subj:13015000 ;
	skos:exactMatch <https://www.wikidata.org/entity/Q25261> ;
	skos:broader	medtop:20000717 .

medtop:20000731
	rdf:type skos:Concept ;
	skos:prefLabel	"physics"@en-GB ;
	skos:definition	"The study of the movement and structure of matter, and how it relates to energy"@en-GB ;
	skos:inScheme <http://cv.iptc.org/newscodes/mediatopic/>  ;
	ikos:created "2009-10-22T02:00:00+00:00"^^xsd:dateTime ;
	dct:created "2009-10-22T02:00:00+00:00"^^xsd:dateTime ;
	ikos:modified "2021-02-18T12:00:00+00:00"^^xsd:dateTime ;
	dct:modified "2021-02-18T12:00:00+00:00"^^xsd:dateTime  ;
	skos:exactMatch subj:13001001 ;
	skos:exactMatch <https://www.wikidata.org/entity/Q413> ;
	skos:broader	medtop:20000717 ;
	skos:narrower	medtop:20000732 ;
	skos:narrower	medtop:20000733 .

medtop:20000732
	rdf:type skos:Concept ;
	skos:prefLabel	"electromagnetism"@en-GB ;
	skos:definition	"The study of the physical interactions between electrically charged particles and magnetic fields"@en-GB ;
	skos:inScheme <http://cv.iptc.org/newscodes/mediatopic/>  ;
	ikos:created "2009-10-22T02:00:00+00:00"^^xsd:dateTime ;
	dct:created "2009-10-22T02:00:00+00:00"^^xsd:dateTime ;
	ikos:modified "2021-07-12T12:00:00+00:00"^^xsd:dateTime ;
	dct:modified "2021-07-12T12:00:00+00:00"^^xsd:dateTime  ;
	skos:broadMatch subj:13001001 ;
	skos:exactMatch <https://www.wikidata.org/entity/Q11406> ;
	skos:broader	medtop:20000731 .

medtop:20000733
	rdf:type skos:Concept ;
	skos:prefLabel	"nuclear physics"@en-GB ;
	skos:definition	"The study of the structure and behaviour of atomic nuclei"@en-GB ;
	skos:inScheme <http://cv.iptc.org/newscodes/mediatopic/>  ;
	ikos:created "2009-10-22T02:00:00+00:00"^^xsd:dateTime ;
	dct:created "2009-10-22T02:00:00+00:00"^^xsd:dateTime ;
	ikos:modified "2021-02-18T12:00:00+00:00"^^xsd:dateTime ;
	dct:modified "2021-02-18T12:00:00+00:00"^^xsd:dateTime  ;
	skos:broadMatch subj:13001001 ;
	skos:exactMatch <https://www.wikidata.org/entity/Q81197> ;
	skos:broader	medtop:20000731 ;
	skos:narrower	medtop:20000734 .

medtop:20000734
	rdf:type skos:Concept ;
	skos:prefLabel	"particle physics"@en-GB ;
	skos:definition	"The study of the nature, properties and interactions of the elementary particles that constitute matter"@en-GB ;
	skos:inScheme <http://cv.iptc.org/newscodes/mediatopic/>  ;
	ikos:created "2009-10-22T02:00:00+00:00"^^xsd:dateTime ;
	dct:created "2009-10-22T02:00:00+00:00"^^xsd:dateTime ;
	ikos:modified "2021-02-18T12:00:00+00:00"^^xsd:dateTime ;
	dct:modified "2021-02-18T12:00:00+00:00"^^xsd:dateTime  ;
	skos:exactMatch subj:13001004 ;
	skos:exactMatch <https://www.wikidata.org/entity/Q18334> ;
	skos:broader	medtop:20000733 .

medtop:20000735
	rdf:type skos:Concept ;
	skos:prefLabel	"scientific research"@en-GB ;
	skos:definition	"The scientific and methodical investigation of events, procedures and interactions to explain why they occur, or to find solutions for problems"@en-GB ;
	skos:inScheme <http://cv.iptc.org/newscodes/mediatopic/>  ;
	ikos:created "2009-10-22T02:00:00+00:00"^^xsd:dateTime ;
	dct:created "2009-10-22T02:00:00+00:00"^^xsd:dateTime ;
	ikos:modified "2021-02-18T12:00:00+00:00"^^xsd:dateTime ;
	dct:modified "2021-02-18T12:00:00+00:00"^^xsd:dateTime  ;
	skos:exactMatch subj:13006000 ;
	skos:exactMatch <https://www.wikidata.org/entity/Q42240> ;
	skos:broader	medtop:13000000 ;
	skos:narrower	medtop:20000736 ;
	skos:narrower	medtop:20000737 ;
	skos:narrower	medtop:20000738 ;
	skos:narrower	medtop:20000740 .

medtop:20000736
	rdf:type skos:Concept ;
	skos:prefLabel	"scientific innovation"@en-GB ;
	skos:definition	"The development or creation of new scientific or technological products or processes, such as biotech or artificial intelligence applications, robotic limbs or nanoscale cameras"@en-GB ;
	skos:inScheme <http://cv.iptc.org/newscodes/mediatopic/>  ;
	ikos:created "2009-10-22T02:00:00+00:00"^^xsd:dateTime ;
	dct:created "2009-10-22T02:00:00+00:00"^^xsd:dateTime ;
	ikos:modified "2021-02-18T12:00:00+00:00"^^xsd:dateTime ;
	dct:modified "2021-02-18T12:00:00+00:00"^^xsd:dateTime  ;
	skos:broadMatch subj:13006000 ;
	skos:exactMatch <https://www.wikidata.org/entity/Q174165> ;
	skos:broader	medtop:20000735 .

medtop:20000737
	rdf:type skos:Concept ;
	skos:prefLabel	"medical research"@en-GB ;
	skos:definition	"Investigation conducted in the fields of health and medicine, such as genetic studies, disease research or pharmaceutical drug trials"@en-GB ;
	skos:inScheme <http://cv.iptc.org/newscodes/mediatopic/>  ;
	ikos:created "2009-10-22T02:00:00+00:00"^^xsd:dateTime ;
	dct:created "2009-10-22T02:00:00+00:00"^^xsd:dateTime ;
	ikos:modified "2021-02-18T12:00:00+00:00"^^xsd:dateTime ;
	dct:modified "2021-02-18T12:00:00+00:00"^^xsd:dateTime  ;
	skos:exactMatch subj:07005000 ;
	skos:exactMatch <https://www.wikidata.org/entity/Q2752427> ;
	skos:broader	medtop:20000735 .

medtop:20000738
	rdf:type skos:Concept ;
	skos:prefLabel	"scientific exploration"@en-GB ;
	skos:definition	"Land, sea or space journeys undertaken to discover new information"@en-GB ;
	skos:inScheme <http://cv.iptc.org/newscodes/mediatopic/>  ;
	ikos:created "2009-10-22T02:00:00+00:00"^^xsd:dateTime ;
	dct:created "2009-10-22T02:00:00+00:00"^^xsd:dateTime ;
	ikos:modified "2021-02-18T12:00:00+00:00"^^xsd:dateTime ;
	dct:modified "2021-02-18T12:00:00+00:00"^^xsd:dateTime  ;
	skos:exactMatch subj:13007000 ;
	skos:exactMatch <https://www.wikidata.org/entity/Q6502154> ;
	skos:broader	medtop:20000735 ;
	skos:narrower	medtop:20000739 .

medtop:20000739
	rdf:type skos:Concept ;
	skos:prefLabel	"space exploration"@en-GB ;
	skos:definition	"The scientific exploration of outer space through manned and unmanned missions"@en-GB ;
	skos:inScheme <http://cv.iptc.org/newscodes/mediatopic/>  ;
	ikos:created "2009-10-22T02:00:00+00:00"^^xsd:dateTime ;
	dct:created "2009-10-22T02:00:00+00:00"^^xsd:dateTime ;
	ikos:modified "2021-02-18T12:00:00+00:00"^^xsd:dateTime ;
	dct:modified "2021-02-18T12:00:00+00:00"^^xsd:dateTime  ;
	skos:exactMatch subj:13008000 ;
	skos:exactMatch <https://www.wikidata.org/entity/Q180046> ;
	skos:broader	medtop:20000738 .

medtop:20000740
	rdf:type skos:Concept ;
	skos:prefLabel	"scientific publication"@en-GB ;
	skos:definition	"Academic research findings published in a journal, book or thesis"@en-GB ;
	skos:inScheme <http://cv.iptc.org/newscodes/mediatopic/>  ;
	ikos:created "2009-10-22T02:00:00+00:00"^^xsd:dateTime ;
	dct:created "2009-10-22T02:00:00+00:00"^^xsd:dateTime ;
	ikos:modified "2021-02-18T12:00:00+00:00"^^xsd:dateTime ;
	dct:modified "2021-02-18T12:00:00+00:00"^^xsd:dateTime  ;
	skos:broadMatch subj:13006000 ;
	skos:exactMatch <https://www.wikidata.org/entity/Q591041> ;
	skos:broader	medtop:20000735 .

medtop:20000741
	rdf:type skos:Concept ;
	skos:prefLabel	"scientific institution"@en-GB ;
	skos:definition	"Institution that carries out or governs scientific work, such as the National Academy of Arts and Sciences"@en-GB ;
	skos:inScheme <http://cv.iptc.org/newscodes/mediatopic/>  ;
	ikos:created "2009-10-22T02:00:00+00:00"^^xsd:dateTime ;
	dct:created "2009-10-22T02:00:00+00:00"^^xsd:dateTime ;
	ikos:modified "2021-02-18T12:00:00+00:00"^^xsd:dateTime ;
	dct:modified "2021-02-18T12:00:00+00:00"^^xsd:dateTime  ;
	skos:exactMatch subj:13023000 ;
	skos:exactMatch <https://www.wikidata.org/entity/Q31855> ;
	skos:broader	medtop:13000000 .

medtop:20000742
	rdf:type skos:Concept ;
	skos:prefLabel	"social sciences"@en-GB ;
	skos:definition	"The study of human society in such aspects as linguistics, anthropology, economics or sociology"@en-GB ;
	skos:inScheme <http://cv.iptc.org/newscodes/mediatopic/>  ;
	ikos:created "2009-10-22T02:00:00+00:00"^^xsd:dateTime ;
	dct:created "2009-10-22T02:00:00+00:00"^^xsd:dateTime ;
	ikos:modified "2021-02-18T12:00:00+00:00"^^xsd:dateTime ;
	dct:modified "2021-02-18T12:00:00+00:00"^^xsd:dateTime  ;
	skos:exactMatch <https://www.wikidata.org/entity/Q34749> ;
	skos:exactMatch subj:13003001 ;
	skos:broader	medtop:13000000 ;
	skos:narrower	medtop:20000743 ;
	skos:narrower	medtop:20000744 ;
	skos:narrower	medtop:20000745 ;
	skos:narrower	medtop:20000746 ;
	skos:narrower	medtop:20000747 ;
	skos:narrower	medtop:20000748 ;
	skos:narrower	medtop:20000749 ;
	skos:narrower	medtop:20000750 ;
	skos:narrower	medtop:20000751 ;
	skos:narrower	medtop:20000752 ;
	skos:narrower	medtop:20000753 ;
	skos:narrower	medtop:20000754 .

medtop:20000743
	rdf:type skos:Concept ;
	skos:prefLabel	"anthropology"@en-GB ;
	skos:definition	"The study of human behaviour and social interactions across time"@en-GB ;
	skos:inScheme <http://cv.iptc.org/newscodes/mediatopic/>  ;
	ikos:created "2009-10-22T02:00:00+00:00"^^xsd:dateTime ;
	dct:created "2009-10-22T02:00:00+00:00"^^xsd:dateTime ;
	ikos:modified "2021-02-18T12:00:00+00:00"^^xsd:dateTime ;
	dct:modified "2021-02-18T12:00:00+00:00"^^xsd:dateTime  ;
	skos:exactMatch subj:13003005 ;
	skos:exactMatch <https://www.wikidata.org/entity/Q23404> ;
	skos:broader	medtop:20000742 .

medtop:20000744
	rdf:type skos:Concept ;
	skos:prefLabel	"archaeology"@en-GB ;
	skos:definition	"The study of human activity throughout time and cultural history, using artefacts left behind by ancient peoples"@en-GB ;
	skos:inScheme <http://cv.iptc.org/newscodes/mediatopic/>  ;
	ikos:created "2009-10-22T02:00:00+00:00"^^xsd:dateTime ;
	dct:created "2009-10-22T02:00:00+00:00"^^xsd:dateTime ;
	ikos:modified "2021-02-18T12:00:00+00:00"^^xsd:dateTime ;
	dct:modified "2021-02-18T12:00:00+00:00"^^xsd:dateTime  ;
	skos:exactMatch subj:01001000 ;
	skos:exactMatch <https://www.wikidata.org/entity/Q23498> ;
	skos:broader	medtop:20000742 .

medtop:20000745
	rdf:type skos:Concept ;
	skos:prefLabel	"economics"@en-GB ;
	skos:definition	"The study of the laws and principles of economies, such as the production and distribution of goods and services"@en-GB ;
	skos:inScheme <http://cv.iptc.org/newscodes/mediatopic/>  ;
	ikos:created "2009-10-22T02:00:00+00:00"^^xsd:dateTime ;
	dct:created "2009-10-22T02:00:00+00:00"^^xsd:dateTime ;
	ikos:modified "2021-02-18T12:00:00+00:00"^^xsd:dateTime ;
	dct:modified "2021-02-18T12:00:00+00:00"^^xsd:dateTime  ;
	skos:broadMatch subj:04017000 ;
	skos:exactMatch <https://www.wikidata.org/entity/Q8134> ;
	skos:broader	medtop:20000742 .

medtop:20000746
	rdf:type skos:Concept ;
	skos:prefLabel	"geography"@en-GB ;
	skos:definition	"The study of the physical features of the surface of Earth and its political divisions"@en-GB ;
	skos:inScheme <http://cv.iptc.org/newscodes/mediatopic/>  ;
	ikos:created "2009-10-22T02:00:00+00:00"^^xsd:dateTime ;
	dct:created "2009-10-22T02:00:00+00:00"^^xsd:dateTime ;
	ikos:modified "2021-02-18T12:00:00+00:00"^^xsd:dateTime ;
	dct:modified "2021-02-18T12:00:00+00:00"^^xsd:dateTime  ;
	skos:exactMatch subj:13004003 ;
	skos:exactMatch <https://www.wikidata.org/entity/Q1071> ;
	skos:broader	medtop:20000742 .

medtop:20000747
	rdf:type skos:Concept ;
	skos:prefLabel	"history"@en-GB ;
	skos:definition	"The study of human events of the past"@en-GB ;
	skos:inScheme <http://cv.iptc.org/newscodes/mediatopic/>  ;
	ikos:created "2009-10-22T02:00:00+00:00"^^xsd:dateTime ;
	dct:created "2009-10-22T02:00:00+00:00"^^xsd:dateTime ;
	ikos:modified "2021-02-18T12:00:00+00:00"^^xsd:dateTime ;
	dct:modified "2021-02-18T12:00:00+00:00"^^xsd:dateTime  ;
	skos:exactMatch subj:13003002 ;
	skos:exactMatch <https://www.wikidata.org/entity/Q1066186> ;
	skos:broader	medtop:20000742 .

medtop:20000748
	rdf:type skos:Concept ;
	skos:prefLabel	"information science"@en-GB ;
	skos:definition	"The study and practice of collecting, classifying, storing, retrieving and disseminating information"@en-GB ;
	skos:inScheme <http://cv.iptc.org/newscodes/mediatopic/>  ;
	ikos:created "2009-10-22T02:00:00+00:00"^^xsd:dateTime ;
	dct:created "2009-10-22T02:00:00+00:00"^^xsd:dateTime ;
	ikos:modified "2021-02-18T12:00:00+00:00"^^xsd:dateTime ;
	dct:modified "2021-02-18T12:00:00+00:00"^^xsd:dateTime  ;
	skos:broadMatch subj:13003001 ;
	skos:exactMatch <https://www.wikidata.org/entity/Q16387> ;
	skos:broader	medtop:20000742 .

medtop:20000749
	rdf:type skos:Concept ;
	skos:prefLabel	"study of law"@en-GB ;
	skos:definition	"The study of legal systems and the philosophy of law"@en-GB ;
	skos:inScheme <http://cv.iptc.org/newscodes/mediatopic/>  ;
	ikos:created "2009-10-22T02:00:00+00:00"^^xsd:dateTime ;
	dct:created "2009-10-22T02:00:00+00:00"^^xsd:dateTime ;
	ikos:modified "2023-10-02T12:00:00+00:00"^^xsd:dateTime ;
	dct:modified "2023-10-02T12:00:00+00:00"^^xsd:dateTime  ;
	skos:broadMatch subj:13003001 ;
	skos:exactMatch <https://www.wikidata.org/entity/Q4932206> ;
	skos:broader	medtop:20000742 .

medtop:20000750
	rdf:type skos:Concept ;
	skos:prefLabel	"linguistics"@en-GB ;
	skos:definition	"The study of all aspects of human language such as syntax, phonetics, written and spoken forms and variations over time"@en-GB ;
	skos:inScheme <http://cv.iptc.org/newscodes/mediatopic/>  ;
	ikos:created "2009-10-22T02:00:00+00:00"^^xsd:dateTime ;
	dct:created "2009-10-22T02:00:00+00:00"^^xsd:dateTime ;
	ikos:modified "2021-02-18T12:00:00+00:00"^^xsd:dateTime ;
	dct:modified "2021-02-18T12:00:00+00:00"^^xsd:dateTime  ;
	skos:broadMatch subj:13000000 ;
	skos:exactMatch <https://www.wikidata.org/entity/Q8162> ;
	skos:broader	medtop:20000742 .

medtop:20000751
	rdf:type skos:Concept ;
	skos:prefLabel	"philosophy"@en-GB ;
	skos:definition	"The study of the principles and fundamental questions about matters such as the mind, reason, morality or values"@en-GB ;
	skos:inScheme <http://cv.iptc.org/newscodes/mediatopic/>  ;
	ikos:created "2009-10-22T02:00:00+00:00"^^xsd:dateTime ;
	dct:created "2009-10-22T02:00:00+00:00"^^xsd:dateTime ;
	ikos:modified "2021-02-18T12:00:00+00:00"^^xsd:dateTime ;
	dct:modified "2021-02-18T12:00:00+00:00"^^xsd:dateTime  ;
	skos:closeMatch subj:12008000 ;
	skos:exactMatch <https://www.wikidata.org/entity/Q5891> ;
	skos:broader	medtop:20000742 .

medtop:20000752
	rdf:type skos:Concept ;
	skos:prefLabel	"political science"@en-GB ;
	skos:definition	"The study of the principles of political and governmental systems, political thought and practices"@en-GB ;
	skos:inScheme <http://cv.iptc.org/newscodes/mediatopic/>  ;
	ikos:created "2009-10-22T02:00:00+00:00"^^xsd:dateTime ;
	dct:created "2009-10-22T02:00:00+00:00"^^xsd:dateTime ;
	ikos:modified "2021-02-18T12:00:00+00:00"^^xsd:dateTime ;
	dct:modified "2021-02-18T12:00:00+00:00"^^xsd:dateTime  ;
	skos:broadMatch subj:13000000 ;
	skos:exactMatch <https://www.wikidata.org/entity/Q36442> ;
	skos:broader	medtop:20000742 .

medtop:20000753
	rdf:type skos:Concept ;
	skos:prefLabel	"psychology"@en-GB ;
	skos:definition	"The study of the human mind, mental characteristics and emotional processes"@en-GB ;
	skos:inScheme <http://cv.iptc.org/newscodes/mediatopic/>  ;
	ikos:created "2009-10-22T02:00:00+00:00"^^xsd:dateTime ;
	dct:created "2009-10-22T02:00:00+00:00"^^xsd:dateTime ;
	ikos:modified "2021-02-18T12:00:00+00:00"^^xsd:dateTime ;
	dct:modified "2021-02-18T12:00:00+00:00"^^xsd:dateTime  ;
	skos:exactMatch subj:13003003 ;
	skos:exactMatch <https://www.wikidata.org/entity/Q9418> ;
	skos:broader	medtop:20000742 .

medtop:20000754
	rdf:type skos:Concept ;
	skos:prefLabel	"sociology"@en-GB ;
	skos:definition	"The study of human social organisation, social relationships and societal changes"@en-GB ;
	skos:inScheme <http://cv.iptc.org/newscodes/mediatopic/>  ;
	ikos:created "2009-10-22T02:00:00+00:00"^^xsd:dateTime ;
	dct:created "2009-10-22T02:00:00+00:00"^^xsd:dateTime ;
	ikos:modified "2021-02-18T12:00:00+00:00"^^xsd:dateTime ;
	dct:modified "2021-02-18T12:00:00+00:00"^^xsd:dateTime  ;
	skos:exactMatch subj:13003004 ;
	skos:exactMatch <https://www.wikidata.org/entity/Q21201> ;
	skos:broader	medtop:20000742 .

medtop:20000755
	rdf:type skos:Concept ;
	skos:prefLabel	"scientific standards"@en-GB ;
	skos:definition	"Nationally or internationally established rules governing scientific and technological study and development, such as calibration standards for scientific tools or equipment"@en-GB ;
	skos:inScheme <http://cv.iptc.org/newscodes/mediatopic/>  ;
	ikos:created "2009-10-22T02:00:00+00:00"^^xsd:dateTime ;
	dct:created "2009-10-22T02:00:00+00:00"^^xsd:dateTime ;
	ikos:modified "2021-02-18T12:00:00+00:00"^^xsd:dateTime ;
	dct:modified "2021-02-18T12:00:00+00:00"^^xsd:dateTime  ;
	skos:exactMatch subj:13011000 ;
	skos:exactMatch <https://www.wikidata.org/entity/Q1334738> ;
	skos:broader	medtop:13000000 .

medtop:20000756
	rdf:type skos:Concept ;
	skos:prefLabel	"technology and engineering"@en-GB ;
	skos:definition	"The study and practice of industrial or applied sciences such as physics, hydrodynamics or thermodynamics"@en-GB ;
	skos:inScheme <http://cv.iptc.org/newscodes/mediatopic/>  ;
	ikos:created "2009-10-22T02:00:00+00:00"^^xsd:dateTime ;
	dct:created "2009-10-22T02:00:00+00:00"^^xsd:dateTime ;
	ikos:modified "2021-02-18T12:00:00+00:00"^^xsd:dateTime ;
	dct:modified "2021-02-18T12:00:00+00:00"^^xsd:dateTime  ;
	skos:broadMatch subj:13000000 ;
	skos:exactMatch <https://www.wikidata.org/entity/Q11016> ;
	skos:broader	medtop:13000000 ;
	skos:narrower	medtop:20000716 ;
	skos:narrower	medtop:20000757 ;
	skos:narrower	medtop:20000759 ;
	skos:narrower	medtop:20000760 ;
	skos:narrower	medtop:20000761 ;
	skos:narrower	medtop:20000762 ;
	skos:narrower	medtop:20000763 ;
	skos:narrower	medtop:20000764 ;
	skos:narrower	medtop:20000765 .

medtop:20000757
	rdf:type skos:Concept ;
	skos:prefLabel	"aerospace engineering"@en-GB ;
	skos:definition	"The study, design, development and construction of aircraft, spacecraft and missile systems"@en-GB ;
	skos:inScheme <http://cv.iptc.org/newscodes/mediatopic/>  ;
	ikos:created "2009-10-22T02:00:00+00:00"^^xsd:dateTime ;
	dct:created "2009-10-22T02:00:00+00:00"^^xsd:dateTime ;
	ikos:modified "2021-02-18T12:00:00+00:00"^^xsd:dateTime ;
	dct:modified "2021-02-18T12:00:00+00:00"^^xsd:dateTime  ;
	skos:broadMatch subj:04011001 ;
	skos:exactMatch <https://www.wikidata.org/entity/Q3798668> ;
	skos:broader	medtop:20000756 ;
	skos:narrower	medtop:20000758 .

medtop:20000758
	rdf:type skos:Concept ;
	skos:prefLabel	"rocketry"@en-GB ;
	skos:definition	"The study, design, development and construction of rockets"@en-GB ;
	skos:inScheme <http://cv.iptc.org/newscodes/mediatopic/>  ;
	ikos:created "2009-10-22T02:00:00+00:00"^^xsd:dateTime ;
	dct:created "2009-10-22T02:00:00+00:00"^^xsd:dateTime ;
	ikos:modified "2021-02-18T12:00:00+00:00"^^xsd:dateTime ;
	dct:modified "2021-02-18T12:00:00+00:00"^^xsd:dateTime  ;
	skos:exactMatch subj:13010001 ;
	skos:exactMatch <https://www.wikidata.org/entity/Q23064627> ;
	skos:broader	medtop:20000757 .

medtop:20000759
	rdf:type skos:Concept ;
	skos:prefLabel	"agricultural technology"@en-GB ;
	skos:definition	"The study and development of techniques and machinery to improve agricultural management and productivity"@en-GB ;
	skos:inScheme <http://cv.iptc.org/newscodes/mediatopic/>  ;
	ikos:created "2009-10-22T02:00:00+00:00"^^xsd:dateTime ;
	dct:created "2009-10-22T02:00:00+00:00"^^xsd:dateTime ;
	ikos:modified "2021-05-05T12:00:00+00:00"^^xsd:dateTime ;
	dct:modified "2021-05-05T12:00:00+00:00"^^xsd:dateTime  ;
	skos:broadMatch subj:13020000 ;
	skos:exactMatch <https://www.wikidata.org/entity/Q25324295> ;
	skos:broader	medtop:20000756 .

medtop:20000760
	rdf:type skos:Concept ;
	skos:prefLabel	"civil engineering"@en-GB ;
	skos:definition	"The study, design, development and construction of structures such as buildings, bridges, tunnels, irrigation and sewage systems, streets or railroads"@en-GB ;
	skos:inScheme <http://cv.iptc.org/newscodes/mediatopic/>  ;
	ikos:created "2009-10-22T02:00:00+00:00"^^xsd:dateTime ;
	dct:created "2009-10-22T02:00:00+00:00"^^xsd:dateTime ;
	ikos:modified "2021-02-18T12:00:00+00:00"^^xsd:dateTime ;
	dct:modified "2021-02-18T12:00:00+00:00"^^xsd:dateTime  ;
	skos:broadMatch subj:13002000 ;
	skos:exactMatch <https://www.wikidata.org/entity/Q77590> ;
	skos:broader	medtop:20000756 .

medtop:20000761
	rdf:type skos:Concept ;
	skos:prefLabel	"electronic engineering"@en-GB ;
	skos:definition	"The study, design, development and application of systems built on the exchange of electrical charges, such as consumer devices, communications systems or industrial computers"@en-GB ;
	skos:inScheme <http://cv.iptc.org/newscodes/mediatopic/>  ;
	ikos:created "2009-10-22T02:00:00+00:00"^^xsd:dateTime ;
	dct:created "2009-10-22T02:00:00+00:00"^^xsd:dateTime ;
	ikos:modified "2021-02-18T12:00:00+00:00"^^xsd:dateTime ;
	dct:modified "2021-02-18T12:00:00+00:00"^^xsd:dateTime  ;
	skos:exactMatch subj:13016000 ;
	skos:exactMatch <https://www.wikidata.org/entity/Q126095> ;
	skos:broader	medtop:20000756 .

medtop:20000762
	rdf:type skos:Concept ;
	skos:prefLabel	"identification technology"@en-GB ;
	skos:definition	"The study, development, application and ethical considerations of technological methods for identifying products, animals or people; including radio frequency, biometrics or face recognition"@en-GB ;
	skos:inScheme <http://cv.iptc.org/newscodes/mediatopic/>  ;
	ikos:created "2009-10-22T02:00:00+00:00"^^xsd:dateTime ;
	dct:created "2009-10-22T02:00:00+00:00"^^xsd:dateTime ;
	ikos:modified "2021-02-18T12:00:00+00:00"^^xsd:dateTime ;
	dct:modified "2021-02-18T12:00:00+00:00"^^xsd:dateTime  ;
	skos:exactMatch subj:13017000 ;
	skos:exactMatch <https://www.wikidata.org/entity/Q787282> ;
	skos:broader	medtop:20000756 .

medtop:20000763
	rdf:type skos:Concept ;
	skos:prefLabel	"information technology and computer science"@en-GB ;
	skos:definition	"The study and design of computer systems, software and networks"@en-GB ;
	skos:inScheme <http://cv.iptc.org/newscodes/mediatopic/>  ;
	ikos:created "2009-10-22T02:00:00+00:00"^^xsd:dateTime ;
	dct:created "2009-10-22T02:00:00+00:00"^^xsd:dateTime ;
	ikos:modified "2021-02-18T12:00:00+00:00"^^xsd:dateTime ;
	dct:modified "2021-02-18T12:00:00+00:00"^^xsd:dateTime  ;
	skos:exactMatch subj:13022000 ;
	skos:exactMatch <https://www.wikidata.org/entity/Q11661> ;
	skos:broader	medtop:20000756 ;
	skos:narrower	medtop:20001298 .

medtop:20000764
	rdf:type skos:Concept ;
	skos:prefLabel	"materials science"@en-GB ;
	skos:definition	"The study of the composition, structure and properties of materials for their use in industry and manufacturing"@en-GB ;
	skos:inScheme <http://cv.iptc.org/newscodes/mediatopic/>  ;
	ikos:created "2009-10-22T02:00:00+00:00"^^xsd:dateTime ;
	dct:created "2009-10-22T02:00:00+00:00"^^xsd:dateTime ;
	ikos:modified "2021-02-18T12:00:00+00:00"^^xsd:dateTime ;
	dct:modified "2021-02-18T12:00:00+00:00"^^xsd:dateTime  ;
	skos:exactMatch subj:13002001 ;
	skos:exactMatch <https://www.wikidata.org/entity/Q228736> ;
	skos:broader	medtop:20000756 .

medtop:20000765
	rdf:type skos:Concept ;
	skos:prefLabel	"micro science"@en-GB ;
	skos:definition	"The study of and technologies built at a microscopic scale, such as microbiology or microcomputing"@en-GB ;
	skos:inScheme <http://cv.iptc.org/newscodes/mediatopic/>  ;
	ikos:created "2009-10-22T02:00:00+00:00"^^xsd:dateTime ;
	dct:created "2009-10-22T02:00:00+00:00"^^xsd:dateTime ;
	ikos:modified "2021-02-18T12:00:00+00:00"^^xsd:dateTime ;
	dct:modified "2021-02-18T12:00:00+00:00"^^xsd:dateTime  ;
	skos:exactMatch subj:13013000 ;
	skos:broader	medtop:20000756 ;
	skos:narrower	medtop:20000766 .

medtop:20000766
	rdf:type skos:Concept ;
	skos:prefLabel	"nanotechnology"@en-GB ;
	skos:definition	"Manipulating objects at the molecular scale"@en-GB ;
	skos:inScheme <http://cv.iptc.org/newscodes/mediatopic/>  ;
	ikos:created "2009-10-22T02:00:00+00:00"^^xsd:dateTime ;
	dct:created "2009-10-22T02:00:00+00:00"^^xsd:dateTime ;
	ikos:modified "2021-02-18T12:00:00+00:00"^^xsd:dateTime ;
	dct:modified "2021-02-18T12:00:00+00:00"^^xsd:dateTime  ;
	skos:exactMatch subj:13021000 ;
	skos:exactMatch <https://www.wikidata.org/entity/Q11468> ;
	skos:broader	medtop:20000765 .

medtop:20000768
	rdf:type skos:Concept ;
	skos:prefLabel	"communities"@en-GB ;
	skos:definition	"A group of individuals actively sharing a common value or interest"@en-GB ;
	skos:inScheme <http://cv.iptc.org/newscodes/mediatopic/>  ;
	ikos:created "2009-10-22T02:00:00+00:00"^^xsd:dateTime ;
	dct:created "2009-10-22T02:00:00+00:00"^^xsd:dateTime ;
	ikos:modified "2021-02-18T12:00:00+00:00"^^xsd:dateTime ;
	dct:modified "2021-02-18T12:00:00+00:00"^^xsd:dateTime  ;
	skos:exactMatch <https://www.wikidata.org/entity/Q177634> ;
	skos:broadMatch subj:14024000 ;
	skos:broader	medtop:14000000 ;
	skos:narrower	medtop:20000769 ;
	skos:narrower	medtop:20001360 .

medtop:20000769
	rdf:type skos:Concept ;
	skos:prefLabel	"social networking"@en-GB ;
	skos:definition	"Social interactions, either in person or online, intended to share information and build relationships around common interests"@en-GB ;
	skos:inScheme <http://cv.iptc.org/newscodes/mediatopic/>  ;
	ikos:created "2009-10-22T02:00:00+00:00"^^xsd:dateTime ;
	dct:created "2009-10-22T02:00:00+00:00"^^xsd:dateTime ;
	ikos:modified "2021-02-18T12:00:00+00:00"^^xsd:dateTime ;
	dct:modified "2021-02-18T12:00:00+00:00"^^xsd:dateTime  ;
	skos:broadMatch subj:14000000 ;
	skos:exactMatch <https://www.wikidata.org/entity/Q19368491> ;
	skos:broader	medtop:20000768 .

medtop:20000770
	rdf:type skos:Concept ;
	skos:prefLabel	"demographics"@en-GB ;
	skos:definition	"The study of human populations and their characteristics, for example statistics or trends around aging populations in a particular geographic region"@en-GB ;
	skos:inScheme <http://cv.iptc.org/newscodes/mediatopic/>  ;
	ikos:created "2009-10-22T02:00:00+00:00"^^xsd:dateTime ;
	dct:created "2009-10-22T02:00:00+00:00"^^xsd:dateTime ;
	ikos:modified "2021-02-18T12:00:00+00:00"^^xsd:dateTime ;
	dct:modified "2021-02-18T12:00:00+00:00"^^xsd:dateTime  ;
	skos:exactMatch subj:14003000 ;
	skos:exactMatch <https://www.wikidata.org/entity/Q37732> ;
	skos:broader	medtop:14000000 ;
	skos:narrower	medtop:20000774 .

medtop:20000771
	rdf:type skos:Concept ;
	skos:prefLabel	"immigration"@en-GB ;
	skos:definition	"The movement of individuals or groups of people from one country to another"@en-GB ;
	skos:inScheme <http://cv.iptc.org/newscodes/mediatopic/>  ;
	ikos:created "2009-10-22T02:00:00+00:00"^^xsd:dateTime ;
	dct:created "2009-10-22T02:00:00+00:00"^^xsd:dateTime ;
	ikos:modified "2021-02-18T12:00:00+00:00"^^xsd:dateTime ;
	dct:modified "2021-02-18T12:00:00+00:00"^^xsd:dateTime  ;
	skos:exactMatch subj:14003002 ;
	skos:exactMatch <https://www.wikidata.org/entity/Q131288> ;
	skos:broader	medtop:14000000 ;
	skos:narrower	medtop:20000773 .

medtop:20000772
	rdf:type skos:Concept ;
	skos:prefLabel	"emigration"@en-GB ;
	skos:definition	"Leaving one's country of residence to settle permanently elsewhere"@en-GB ;
	skos:inScheme <http://cv.iptc.org/newscodes/mediatopic/>  ;
	ikos:created "2009-10-22T02:00:00+00:00"^^xsd:dateTime ;
	dct:created "2009-10-22T02:00:00+00:00"^^xsd:dateTime ;
	ikos:modified "2021-07-12T12:00:00+00:00"^^xsd:dateTime ;
	dct:modified "2021-07-12T12:00:00+00:00"^^xsd:dateTime  ;
	skos:exactMatch subj:14003004 ;
	skos:exactMatch <https://www.wikidata.org/entity/Q187668> ;
	skos:broader	medtop:14000000 .

medtop:20000773
	rdf:type skos:Concept ;
	skos:prefLabel	"illegal immigration"@en-GB ;
	skos:definition	"The movement of individuals or groups of people from one country to another without legal authorisation from the destination country"@en-GB ;
	skos:inScheme <http://cv.iptc.org/newscodes/mediatopic/>  ;
	ikos:created "2009-10-22T02:00:00+00:00"^^xsd:dateTime ;
	dct:created "2009-10-22T02:00:00+00:00"^^xsd:dateTime ;
	ikos:modified "2021-02-18T12:00:00+00:00"^^xsd:dateTime ;
	dct:modified "2021-02-18T12:00:00+00:00"^^xsd:dateTime  ;
	skos:exactMatch subj:14003003 ;
	skos:exactMatch <https://www.wikidata.org/entity/Q2368859> ;
	skos:broader	medtop:20000771 .

medtop:20000774
	rdf:type skos:Concept ;
	skos:prefLabel	"population and census"@en-GB ;
	skos:definition	"The official count of people living in a given geopolitical area, usually carried out by a governmental body"@en-GB ;
	skos:inScheme <http://cv.iptc.org/newscodes/mediatopic/>  ;
	ikos:created "2009-10-22T02:00:00+00:00"^^xsd:dateTime ;
	dct:created "2009-10-22T02:00:00+00:00"^^xsd:dateTime ;
	ikos:modified "2021-05-05T12:00:00+00:00"^^xsd:dateTime ;
	dct:modified "2021-05-05T12:00:00+00:00"^^xsd:dateTime  ;
	skos:exactMatch subj:14003001 ;
	skos:exactMatch <https://www.wikidata.org/entity/Q39825> ;
	skos:broader	medtop:20000770 .

medtop:20000775
	rdf:type skos:Concept ;
	skos:prefLabel	"discrimination"@en-GB ;
	skos:definition	"Unfair treatment of, or policies or practices against, individuals or groups of people on the basis of real or perceived membership in a group, such as race, sexual orientation, political or religious beliefs, age or height"@en-GB ;
	skos:inScheme <http://cv.iptc.org/newscodes/mediatopic/>  ;
	ikos:created "2009-10-22T02:00:00+00:00"^^xsd:dateTime ;
	dct:created "2009-10-22T02:00:00+00:00"^^xsd:dateTime ;
	ikos:modified "2021-02-18T12:00:00+00:00"^^xsd:dateTime ;
	dct:modified "2021-02-18T12:00:00+00:00"^^xsd:dateTime  ;
	skos:exactMatch <https://www.wikidata.org/entity/Q169207> ;
	skos:exactMatch subj:14025003 ;
	skos:broader	medtop:14000000 ;
	skos:narrower	medtop:20000776 ;
	skos:narrower	medtop:20000777 ;
	skos:narrower	medtop:20000778 ;
	skos:narrower	medtop:20000779 .

medtop:20000776
	rdf:type skos:Concept ;
	skos:prefLabel	"ageism"@en-GB ;
	skos:definition	"Discrimination against individuals or groups of people on the basis of age"@en-GB ;
	skos:inScheme <http://cv.iptc.org/newscodes/mediatopic/>  ;
	ikos:created "2009-10-22T02:00:00+00:00"^^xsd:dateTime ;
	dct:created "2009-10-22T02:00:00+00:00"^^xsd:dateTime ;
	ikos:modified "2021-02-18T12:00:00+00:00"^^xsd:dateTime ;
	dct:modified "2021-02-18T12:00:00+00:00"^^xsd:dateTime  ;
	skos:broadMatch subj:14025003 ;
	skos:exactMatch <https://www.wikidata.org/entity/Q438946> ;
	skos:broader	medtop:20000775 .

medtop:20000777
	rdf:type skos:Concept ;
	skos:prefLabel	"racism"@en-GB ;
	skos:definition	"Discrimination against individuals or groups of people on the basis of race"@en-GB ;
	skos:inScheme <http://cv.iptc.org/newscodes/mediatopic/>  ;
	ikos:created "2009-10-22T02:00:00+00:00"^^xsd:dateTime ;
	dct:created "2009-10-22T02:00:00+00:00"^^xsd:dateTime ;
	ikos:modified "2021-02-18T12:00:00+00:00"^^xsd:dateTime ;
	dct:modified "2021-02-18T12:00:00+00:00"^^xsd:dateTime  ;
	skos:exactMatch subj:14014000 ;
	skos:exactMatch <https://www.wikidata.org/entity/Q8461> ;
	skos:broader	medtop:20000775 .

medtop:20000778
	rdf:type skos:Concept ;
	skos:prefLabel	"religious discrimination"@en-GB ;
	skos:definition	"Unfair treatment of individuals or groups of people on the basis of their religious belief"@en-GB ;
	skos:inScheme <http://cv.iptc.org/newscodes/mediatopic/>  ;
	ikos:created "2009-10-22T02:00:00+00:00"^^xsd:dateTime ;
	dct:created "2009-10-22T02:00:00+00:00"^^xsd:dateTime ;
	ikos:modified "2021-02-18T12:00:00+00:00"^^xsd:dateTime ;
	dct:modified "2021-02-18T12:00:00+00:00"^^xsd:dateTime  ;
	skos:broadMatch subj:14025003 ;
	skos:exactMatch <https://www.wikidata.org/entity/Q2029282> ;
	skos:broader	medtop:20000775 .

medtop:20000779
	rdf:type skos:Concept ;
	skos:prefLabel	"sexism"@en-GB ;
	skos:definition	"Discrimination against individuals or groups of people, usually women, on the basis of gender"@en-GB ;
	skos:inScheme <http://cv.iptc.org/newscodes/mediatopic/>  ;
	ikos:created "2009-10-22T02:00:00+00:00"^^xsd:dateTime ;
	dct:created "2009-10-22T02:00:00+00:00"^^xsd:dateTime ;
	ikos:modified "2021-09-30T12:00:00+00:00"^^xsd:dateTime ;
	dct:modified "2021-09-30T12:00:00+00:00"^^xsd:dateTime  ;
	skos:broadMatch subj:14025003 ;
	skos:exactMatch <https://www.wikidata.org/entity/Q93200> ;
	skos:broader	medtop:20000775 .

medtop:20000780
	rdf:type skos:Concept ;
	skos:prefLabel	"family"@en-GB ;
	skos:definition	"A group of people related genetically or by a legal bond, or who consider themselves part of a familial unit regardless of genetic or legal status"@en-GB ;
	skos:inScheme <http://cv.iptc.org/newscodes/mediatopic/>  ;
	ikos:created "2009-10-22T02:00:00+00:00"^^xsd:dateTime ;
	dct:created "2009-10-22T02:00:00+00:00"^^xsd:dateTime ;
	ikos:modified "2021-02-18T12:00:00+00:00"^^xsd:dateTime ;
	dct:modified "2021-02-18T12:00:00+00:00"^^xsd:dateTime  ;
	skos:exactMatch <https://www.wikidata.org/entity/Q8436> ;
	skos:exactMatch subj:14006000 ;
	skos:broader	medtop:14000000 ;
	skos:narrower	medtop:20000781 ;
	skos:narrower	medtop:20000782 ;
	skos:narrower	medtop:20000783 ;
	skos:narrower	medtop:20000784 ;
	skos:narrower	medtop:20000786 ;
	skos:narrower	medtop:20000787 ;
	skos:narrower	medtop:20001359 .

medtop:20000781
	rdf:type skos:Concept ;
	skos:prefLabel	"adoption"@en-GB ;
	skos:definition	"The legal process of transferring parental rights to someone other than a person's birth parents, that person usually being a child"@en-GB ;
	skos:inScheme <http://cv.iptc.org/newscodes/mediatopic/>  ;
	ikos:created "2009-10-22T02:00:00+00:00"^^xsd:dateTime ;
	dct:created "2009-10-22T02:00:00+00:00"^^xsd:dateTime ;
	ikos:modified "2021-02-18T12:00:00+00:00"^^xsd:dateTime ;
	dct:modified "2021-02-18T12:00:00+00:00"^^xsd:dateTime  ;
	skos:exactMatch subj:14006002 ;
	skos:exactMatch <https://www.wikidata.org/entity/Q180472> ;
	skos:broader	medtop:20000780 .

medtop:20000782
	rdf:type skos:Concept ;
	skos:prefLabel	"Dating and Relationships"@en-GB ;
	skos:definition	"The development of an intimate connection between individuals, through various forms of activities enjoyed together, often leading to a legal or permanent union such as marriage"@en-GB ;
	skos:inScheme <http://cv.iptc.org/newscodes/mediatopic/>  ;
	ikos:created "2009-10-22T02:00:00+00:00"^^xsd:dateTime ;
	dct:created "2009-10-22T02:00:00+00:00"^^xsd:dateTime ;
	ikos:modified "2021-07-12T12:00:00+00:00"^^xsd:dateTime ;
	dct:modified "2021-07-12T12:00:00+00:00"^^xsd:dateTime  ;
	skos:exactMatch subj:14006006 ;
	skos:exactMatch <https://www.wikidata.org/entity/Q376596> ;
	skos:broader	medtop:20000780 .

medtop:20000783
	rdf:type skos:Concept ;
	skos:prefLabel	"divorce"@en-GB ;
	skos:definition	"The process by which a marriage is legally dissolved"@en-GB ;
	skos:inScheme <http://cv.iptc.org/newscodes/mediatopic/>  ;
	ikos:created "2009-10-22T02:00:00+00:00"^^xsd:dateTime ;
	dct:created "2009-10-22T02:00:00+00:00"^^xsd:dateTime ;
	ikos:modified "2022-06-14T12:00:00+00:00"^^xsd:dateTime ;
	dct:modified "2022-06-14T12:00:00+00:00"^^xsd:dateTime  ;
	skos:exactMatch subj:14006004 ;
	skos:exactMatch <https://www.wikidata.org/entity/Q93190> ;
	skos:broader	medtop:20000780 .

medtop:20000784
	rdf:type skos:Concept ;
	skos:prefLabel	"family planning"@en-GB ;
	skos:definition	"Services and education aimed at informing individual decisions about reproduction, such as fertility, in vitro fertilisation, contraception or abortion"@en-GB ;
	skos:inScheme <http://cv.iptc.org/newscodes/mediatopic/>  ;
	ikos:created "2009-10-22T02:00:00+00:00"^^xsd:dateTime ;
	dct:created "2009-10-22T02:00:00+00:00"^^xsd:dateTime ;
	ikos:modified "2022-06-14T12:00:00+00:00"^^xsd:dateTime ;
	dct:modified "2022-06-14T12:00:00+00:00"^^xsd:dateTime  ;
	skos:exactMatch subj:14007000 ;
	skos:exactMatch <https://www.wikidata.org/entity/Q1280670> ;
	skos:broader	medtop:20000780 ;
	skos:narrower	medtop:20000785 ;
	skos:narrower	medtop:20001274 .

medtop:20000785
	rdf:type skos:Concept ;
	skos:prefLabel	"abortion"@en-GB ;
	skos:definition	"The intentional termination of a pregnancy for elective or medical reasons"@en-GB ;
	skos:inScheme <http://cv.iptc.org/newscodes/mediatopic/>  ;
	ikos:created "2009-10-22T02:00:00+00:00"^^xsd:dateTime ;
	dct:created "2009-10-22T02:00:00+00:00"^^xsd:dateTime ;
	ikos:modified "2021-02-18T12:00:00+00:00"^^xsd:dateTime ;
	dct:modified "2021-02-18T12:00:00+00:00"^^xsd:dateTime  ;
	skos:exactMatch subj:14016000 ;
	skos:exactMatch <https://www.wikidata.org/entity/Q8452> ;
	skos:broader	medtop:20000784 .

medtop:20000786
	rdf:type skos:Concept ;
	skos:prefLabel	"marriage"@en-GB ;
	skos:definition	"The legal or socially recognised union of individuals, which establishes rights and obligations between them"@en-GB ;
	skos:inScheme <http://cv.iptc.org/newscodes/mediatopic/>  ;
	ikos:created "2009-10-22T02:00:00+00:00"^^xsd:dateTime ;
	dct:created "2009-10-22T02:00:00+00:00"^^xsd:dateTime ;
	ikos:modified "2021-03-15T12:00:00+00:00"^^xsd:dateTime ;
	dct:modified "2021-03-15T12:00:00+00:00"^^xsd:dateTime  ;
	skos:exactMatch subj:14006003 ;
	skos:exactMatch <https://www.wikidata.org/entity/Q8445> ;
	skos:broader	medtop:20000780 .

medtop:20000787
	rdf:type skos:Concept ;
	skos:prefLabel	"parenting"@en-GB ;
	skos:definition	"The caring for and support of a child's physical, emotional, developmental and social needs from birth to adulthood"@en-GB ;
	skos:inScheme <http://cv.iptc.org/newscodes/mediatopic/>  ;
	ikos:created "2009-10-22T02:00:00+00:00"^^xsd:dateTime ;
	dct:created "2009-10-22T02:00:00+00:00"^^xsd:dateTime ;
	ikos:modified "2021-02-18T12:00:00+00:00"^^xsd:dateTime ;
	dct:modified "2021-02-18T12:00:00+00:00"^^xsd:dateTime  ;
	skos:exactMatch subj:14006001 ;
	skos:exactMatch <https://www.wikidata.org/entity/Q5362237> ;
	skos:broader	medtop:20000780 .

medtop:20000788
	rdf:type skos:Concept ;
	skos:prefLabel	"mankind"@en-GB ;
	skos:definition	"Human beings taken as a whole, or described as members of particular groups such as teenagers, women, or people with disabilities"@en-GB ;
	skos:inScheme <http://cv.iptc.org/newscodes/mediatopic/>  ;
	ikos:created "2009-10-22T02:00:00+00:00"^^xsd:dateTime ;
	dct:created "2009-10-22T02:00:00+00:00"^^xsd:dateTime ;
	ikos:modified "2021-02-18T12:00:00+00:00"^^xsd:dateTime ;
	dct:modified "2021-02-18T12:00:00+00:00"^^xsd:dateTime  ;
	skos:exactMatch subj:14024000 ;
	skos:exactMatch <https://www.wikidata.org/entity/Q1156970> ;
	skos:broader	medtop:14000000 ;
	skos:narrower	medtop:20000789 ;
	skos:narrower	medtop:20000790 ;
	skos:narrower	medtop:20000791 ;
	skos:narrower	medtop:20000792 ;
	skos:narrower	medtop:20000793 ;
	skos:narrower	medtop:20000794 ;
	skos:narrower	medtop:20000795 ;
	skos:narrower	medtop:20000796 ;
	skos:narrower	medtop:20000797 ;
	skos:narrower	medtop:20000798 ;
	skos:narrower	medtop:20001288 ;
	skos:narrower	medtop:20001327 ;
	skos:narrower	medtop:20001328 .

medtop:20000789
	rdf:type skos:Concept ;
	skos:prefLabel	"adults"@en-GB ;
	skos:definition	"People above an age set by law that entitles them to full liability and certain privileges such as the legal right to drink alcoholic beverages and to vote"@en-GB ;
	skos:inScheme <http://cv.iptc.org/newscodes/mediatopic/>  ;
	ikos:created "2009-10-22T02:00:00+00:00"^^xsd:dateTime ;
	dct:created "2009-10-22T02:00:00+00:00"^^xsd:dateTime ;
	ikos:modified "2021-02-18T12:00:00+00:00"^^xsd:dateTime ;
	dct:modified "2021-02-18T12:00:00+00:00"^^xsd:dateTime  ;
	skos:exactMatch subj:14024004 ;
	skos:exactMatch <https://www.wikidata.org/entity/Q9584157> ;
	skos:broader	medtop:20000788 .

medtop:20000790
	rdf:type skos:Concept ;
	skos:prefLabel	"children"@en-GB ;
	skos:definition	"Young people, usually pre-pubescent, who are legally considered minors and are in a guardianship relationship with adults"@en-GB ;
	skos:inScheme <http://cv.iptc.org/newscodes/mediatopic/>  ;
	ikos:created "2009-10-22T02:00:00+00:00"^^xsd:dateTime ;
	dct:created "2009-10-22T02:00:00+00:00"^^xsd:dateTime ;
	ikos:modified "2021-02-18T12:00:00+00:00"^^xsd:dateTime ;
	dct:modified "2021-02-18T12:00:00+00:00"^^xsd:dateTime  ;
	skos:exactMatch subj:14024001 ;
	skos:exactMatch <https://www.wikidata.org/entity/Q7569> ;
	skos:broader	medtop:20000788 .

medtop:20000791
	rdf:type skos:Concept ;
	skos:prefLabel	"disabilities"@en-GB ;
	skos:definition	"Physical or mental conditions that limits a person's movements, senses, or activities"@en-GB ;
	skos:inScheme <http://cv.iptc.org/newscodes/mediatopic/>  ;
	ikos:created "2009-10-22T02:00:00+00:00"^^xsd:dateTime ;
	dct:created "2009-10-22T02:00:00+00:00"^^xsd:dateTime ;
	ikos:modified "2023-06-05T12:00:00+00:00"^^xsd:dateTime ;
	dct:modified "2023-06-05T12:00:00+00:00"^^xsd:dateTime  ;
	skos:exactMatch subj:14004000 ;
	skos:exactMatch <https://www.wikidata.org/entity/Q12131> ;
	skos:broader	medtop:20000788 .

medtop:20000792
	rdf:type skos:Concept ;
	skos:prefLabel	"LGBTQ"@en-GB ;
	skos:definition	"People who identify as lesbian, gay, bisexual, transgender or queer"@en-GB ;
	skos:inScheme <http://cv.iptc.org/newscodes/mediatopic/>  ;
	ikos:created "2009-10-22T02:00:00+00:00"^^xsd:dateTime ;
	dct:created "2009-10-22T02:00:00+00:00"^^xsd:dateTime ;
	ikos:modified "2021-05-05T12:00:00+00:00"^^xsd:dateTime ;
	dct:modified "2021-05-05T12:00:00+00:00"^^xsd:dateTime  ;
	skos:exactMatch subj:14010001 ;
	skos:exactMatch <https://www.wikidata.org/entity/Q17884> ;
	skos:broader	medtop:20000788 .

medtop:20000793
	rdf:type skos:Concept ;
	skos:prefLabel	"gender"@en-GB ;
	skos:definition	"The classification of individuals as male, female, or a non-binary designation"@en-GB ;
	skos:inScheme <http://cv.iptc.org/newscodes/mediatopic/>  ;
	ikos:created "2009-10-22T02:00:00+00:00"^^xsd:dateTime ;
	dct:created "2009-10-22T02:00:00+00:00"^^xsd:dateTime ;
	ikos:modified "2021-02-18T12:00:00+00:00"^^xsd:dateTime ;
	dct:modified "2021-02-18T12:00:00+00:00"^^xsd:dateTime  ;
	skos:broadMatch subj:14024000 ;
	skos:exactMatch <https://www.wikidata.org/entity/Q48277> ;
	skos:broader	medtop:20000788 .

medtop:20000794
	rdf:type skos:Concept ;
	skos:prefLabel	"infants"@en-GB ;
	skos:definition	"Very young people, usually defined as being just born up to the age of two"@en-GB ;
	skos:inScheme <http://cv.iptc.org/newscodes/mediatopic/>  ;
	ikos:created "2009-10-22T02:00:00+00:00"^^xsd:dateTime ;
	dct:created "2009-10-22T02:00:00+00:00"^^xsd:dateTime ;
	ikos:modified "2021-02-18T12:00:00+00:00"^^xsd:dateTime ;
	dct:modified "2021-02-18T12:00:00+00:00"^^xsd:dateTime  ;
	skos:exactMatch subj:14024002 ;
	skos:exactMatch <https://www.wikidata.org/entity/Q998> ;
	skos:broader	medtop:20000788 .

medtop:20000795
	rdf:type skos:Concept ;
	skos:prefLabel	"national or ethnic minority"@en-GB ;
	skos:definition	"Groups of people that form a minority on an ethnic or national basis, and their status or issues relating to the majority"@en-GB ;
	skos:inScheme <http://cv.iptc.org/newscodes/mediatopic/>  ;
	ikos:created "2009-10-22T02:00:00+00:00"^^xsd:dateTime ;
	dct:created "2009-10-22T02:00:00+00:00"^^xsd:dateTime ;
	ikos:modified "2021-02-18T12:00:00+00:00"^^xsd:dateTime ;
	dct:modified "2021-02-18T12:00:00+00:00"^^xsd:dateTime  ;
	skos:exactMatch subj:14010002 ;
	skos:exactMatch <https://www.wikidata.org/entity/Q769696> ;
	skos:broader	medtop:20000788 .

medtop:20000796
	rdf:type skos:Concept ;
	skos:prefLabel	"nuclear radiation victims"@en-GB ;
	skos:definition	"Includes antinuclear movements and compensation for atomic blast victims."@en-GB ;
	skos:changeNote	"2019-10-07: Retired. Use nuclear accident and incident (20000142) instead."@en-GB ;
	skos:inScheme <http://cv.iptc.org/newscodes/mediatopic/>  ;
	ikos:created "2009-10-22T02:00:00+00:00"^^xsd:dateTime ;
	dct:created "2009-10-22T02:00:00+00:00"^^xsd:dateTime ;
	ikos:modified "2021-02-18T12:00:00+00:00"^^xsd:dateTime ;
	dct:modified "2021-02-18T12:00:00+00:00"^^xsd:dateTime  ; 
	ikos:retired "2019-10-07T12:00:00+00:00"^^xsd:dateTime ;
	skos:exactMatch subj:14020000 ;
	skos:broader	medtop:20000788 .

medtop:20000797
	rdf:type skos:Concept ;
	skos:prefLabel	"senior citizens"@en-GB ;
	skos:definition	"People having passed the age of retirement"@en-GB ;
	skos:inScheme <http://cv.iptc.org/newscodes/mediatopic/>  ;
	ikos:created "2009-10-22T02:00:00+00:00"^^xsd:dateTime ;
	dct:created "2009-10-22T02:00:00+00:00"^^xsd:dateTime ;
	ikos:modified "2021-02-18T12:00:00+00:00"^^xsd:dateTime ;
	dct:modified "2021-02-18T12:00:00+00:00"^^xsd:dateTime  ;
	skos:exactMatch subj:14024005 ;
	skos:exactMatch <https://www.wikidata.org/entity/Q1358789> ;
	skos:broader	medtop:20000788 .

medtop:20000798
	rdf:type skos:Concept ;
	skos:prefLabel	"teenagers"@en-GB ;
	skos:definition	"Young people between the ages that describe childhood and adulthood"@en-GB ;
	skos:inScheme <http://cv.iptc.org/newscodes/mediatopic/>  ;
	ikos:created "2009-10-22T02:00:00+00:00"^^xsd:dateTime ;
	dct:created "2009-10-22T02:00:00+00:00"^^xsd:dateTime ;
	ikos:modified "2021-02-18T12:00:00+00:00"^^xsd:dateTime ;
	dct:modified "2021-02-18T12:00:00+00:00"^^xsd:dateTime  ;
	skos:exactMatch subj:14024003 ;
	skos:exactMatch <https://www.wikidata.org/entity/Q1492760> ;
	skos:broader	medtop:20000788 .

medtop:20000799
	rdf:type skos:Concept ;
	skos:prefLabel	"social condition"@en-GB ;
	skos:definition	"The circumstances or state of affairs affecting a person's life, welfare and relations with others in a society"@en-GB ;
	skos:inScheme <http://cv.iptc.org/newscodes/mediatopic/>  ;
	ikos:created "2009-10-22T02:00:00+00:00"^^xsd:dateTime ;
	dct:created "2009-10-22T02:00:00+00:00"^^xsd:dateTime ;
	ikos:modified "2021-05-05T12:00:00+00:00"^^xsd:dateTime ;
	dct:modified "2021-05-05T12:00:00+00:00"^^xsd:dateTime  ;
	skos:exactMatch subj:14025001 ;
	skos:exactMatch <https://www.wikidata.org/entity/Q189970> ;
	skos:broader	medtop:14000000 ;
	skos:narrower	medtop:20000800 ;
	skos:narrower	medtop:20000801 .

medtop:20000800
	rdf:type skos:Concept ;
	skos:prefLabel	"homelessness"@en-GB ;
	skos:definition	"The social condition defined by lack of permanent residence, living in shelters or on streets, and the issues and problems associated with it"@en-GB ;
	skos:inScheme <http://cv.iptc.org/newscodes/mediatopic/>  ;
	ikos:created "2009-10-22T02:00:00+00:00"^^xsd:dateTime ;
	dct:created "2009-10-22T02:00:00+00:00"^^xsd:dateTime ;
	ikos:modified "2021-02-18T12:00:00+00:00"^^xsd:dateTime ;
	dct:modified "2021-02-18T12:00:00+00:00"^^xsd:dateTime  ;
	skos:exactMatch subj:14009000 ;
	skos:exactMatch <https://www.wikidata.org/entity/Q131327> ;
	skos:broader	medtop:20000799 .

medtop:20000801
	rdf:type skos:Concept ;
	skos:prefLabel	"poverty"@en-GB ;
	skos:definition	"The lack of sufficient resources and means to provide basic needs such as food, clothing or shelter for oneself and one's family"@en-GB ;
	skos:inScheme <http://cv.iptc.org/newscodes/mediatopic/>  ;
	ikos:created "2009-10-22T02:00:00+00:00"^^xsd:dateTime ;
	dct:created "2009-10-22T02:00:00+00:00"^^xsd:dateTime ;
	ikos:modified "2021-02-18T12:00:00+00:00"^^xsd:dateTime ;
	dct:modified "2021-02-18T12:00:00+00:00"^^xsd:dateTime  ;
	skos:exactMatch subj:14012000 ;
	skos:exactMatch <https://www.wikidata.org/entity/Q10294> ;
	skos:broader	medtop:20000799 .

medtop:20000802
	rdf:type skos:Concept ;
	skos:prefLabel	"social problem"@en-GB ;
	skos:definition	"Issues related to human rights, human welfare and other areas of societal concern"@en-GB ;
	skos:inScheme <http://cv.iptc.org/newscodes/mediatopic/>  ;
	ikos:created "2009-10-22T02:00:00+00:00"^^xsd:dateTime ;
	dct:created "2009-10-22T02:00:00+00:00"^^xsd:dateTime ;
	ikos:modified "2021-02-18T12:00:00+00:00"^^xsd:dateTime ;
	dct:modified "2021-02-18T12:00:00+00:00"^^xsd:dateTime  ;
	skos:exactMatch <https://www.wikidata.org/entity/Q1920219> ;
	skos:broadMatch subj:14025002 ;
	skos:broader	medtop:14000000 ;
	skos:narrower	medtop:20000803 ;
	skos:narrower	medtop:20000804 ;
	skos:narrower	medtop:20000805 ;
	skos:narrower	medtop:20000806 ;
	skos:narrower	medtop:20000807 ;
	skos:narrower	medtop:20001193 ;
	skos:narrower	medtop:20001284 .

medtop:20000803
	rdf:type skos:Concept ;
	skos:prefLabel	"abusive behaviour"@en-GB ;
	skos:definition	"Actions that intentionally harm another person or people, often on an ongoing basis, such as psychological or mental abuse, negligence, physical or sexual abuse and torture"@en-GB ;
	skos:inScheme <http://cv.iptc.org/newscodes/mediatopic/>  ;
	ikos:created "2009-10-22T02:00:00+00:00"^^xsd:dateTime ;
	dct:created "2009-10-22T02:00:00+00:00"^^xsd:dateTime ;
	ikos:modified "2021-02-18T12:00:00+00:00"^^xsd:dateTime ;
	dct:modified "2021-02-18T12:00:00+00:00"^^xsd:dateTime  ;
	skos:exactMatch subj:14022000 ;
	skos:exactMatch <https://www.wikidata.org/entity/Q600571> ;
	skos:broader	medtop:20000802 .

medtop:20000804
	rdf:type skos:Concept ;
	skos:prefLabel	"addiction"@en-GB ;
	skos:definition	"The habitual and compulsive use of substances such as alcohol or drugs, or behaviour such as gambling, gaming or sex, often causing detrimental effects on the body, brain, and relationships with others"@en-GB ;
	skos:inScheme <http://cv.iptc.org/newscodes/mediatopic/>  ;
	ikos:created "2009-10-22T02:00:00+00:00"^^xsd:dateTime ;
	dct:created "2009-10-22T02:00:00+00:00"^^xsd:dateTime ;
	ikos:modified "2021-02-18T12:00:00+00:00"^^xsd:dateTime ;
	dct:modified "2021-02-18T12:00:00+00:00"^^xsd:dateTime  ;
	skos:exactMatch subj:14001000 ;
	skos:exactMatch <https://www.wikidata.org/entity/Q12029> ;
	skos:broader	medtop:20000802 .

medtop:20000805
	rdf:type skos:Concept ;
	skos:prefLabel	"juvenile delinquency"@en-GB ;
	skos:definition	"Unlawful conduct perpetrated by minors, often on a repeated basis"@en-GB ;
	skos:inScheme <http://cv.iptc.org/newscodes/mediatopic/>  ;
	ikos:created "2009-10-22T02:00:00+00:00"^^xsd:dateTime ;
	dct:created "2009-10-22T02:00:00+00:00"^^xsd:dateTime ;
	ikos:modified "2021-02-18T12:00:00+00:00"^^xsd:dateTime ;
	dct:modified "2021-02-18T12:00:00+00:00"^^xsd:dateTime  ;
	skos:exactMatch subj:14019000 ;
	skos:exactMatch <https://www.wikidata.org/entity/Q1001125> ;
	skos:broader	medtop:20000802 .

medtop:20000806
	rdf:type skos:Concept ;
	skos:prefLabel	"prostitution"@en-GB ;
	skos:definition	"The business of engaging in sexual activity in exchange for payment"@en-GB ;
	skos:inScheme <http://cv.iptc.org/newscodes/mediatopic/>  ;
	ikos:created "2009-10-22T02:00:00+00:00"^^xsd:dateTime ;
	dct:created "2009-10-22T02:00:00+00:00"^^xsd:dateTime ;
	ikos:modified "2021-02-18T12:00:00+00:00"^^xsd:dateTime ;
	dct:modified "2021-02-18T12:00:00+00:00"^^xsd:dateTime  ;
	skos:exactMatch subj:14013000 ;
	skos:exactMatch <https://www.wikidata.org/entity/Q36633> ;
	skos:broader	medtop:20000802 .

medtop:20000807
	rdf:type skos:Concept ;
	skos:prefLabel	"slavery"@en-GB ;
	skos:definition	"The ownership of people as property, and the involuntary servitude of those people to their owners, which includes unpaid labour and coerced actions"@en-GB ;
	skos:inScheme <http://cv.iptc.org/newscodes/mediatopic/>  ;
	ikos:created "2009-10-22T02:00:00+00:00"^^xsd:dateTime ;
	dct:created "2009-10-22T02:00:00+00:00"^^xsd:dateTime ;
	ikos:modified "2021-02-18T12:00:00+00:00"^^xsd:dateTime ;
	dct:modified "2021-02-18T12:00:00+00:00"^^xsd:dateTime  ;
	skos:exactMatch subj:14021000 ;
	skos:exactMatch <https://www.wikidata.org/entity/Q8463> ;
	skos:broader	medtop:20000802 .

medtop:20000808
	rdf:type skos:Concept ;
	skos:prefLabel	"values"@en-GB ;
	skos:definition	"A person's or group's principles or standards of behaviour, which guide their way of living and choices made"@en-GB ;
	skos:inScheme <http://cv.iptc.org/newscodes/mediatopic/>  ;
	ikos:created "2009-10-22T02:00:00+00:00"^^xsd:dateTime ;
	dct:created "2009-10-22T02:00:00+00:00"^^xsd:dateTime ;
	ikos:modified "2021-02-18T12:00:00+00:00"^^xsd:dateTime ;
	dct:modified "2021-02-18T12:00:00+00:00"^^xsd:dateTime  ;
	skos:exactMatch subj:12006000 ;
	skos:exactMatch <https://www.wikidata.org/entity/Q831695> ;
	skos:broader	medtop:14000000 ;
	skos:narrower	medtop:20000809 ;
	skos:narrower	medtop:20000810 ;
	skos:narrower	medtop:20000814 ;
	skos:narrower	medtop:20000815 ;
	skos:narrower	medtop:20000816 .

medtop:20000809
	rdf:type skos:Concept ;
	skos:prefLabel	"corrupt practices"@en-GB ;
	skos:definition	"Any action which is harmful to others"@en-GB ;
	skos:changeNote	"2019-10-07: Retired. Use corruption (20000093) instead."@en-GB ;
	skos:inScheme <http://cv.iptc.org/newscodes/mediatopic/>  ;
	ikos:created "2009-10-22T02:00:00+00:00"^^xsd:dateTime ;
	dct:created "2009-10-22T02:00:00+00:00"^^xsd:dateTime ;
	ikos:modified "2021-02-18T12:00:00+00:00"^^xsd:dateTime ;
	dct:modified "2021-02-18T12:00:00+00:00"^^xsd:dateTime  ; 
	ikos:retired "2019-10-07T12:00:00+00:00"^^xsd:dateTime ;
	skos:exactMatch subj:12006002 ;
	skos:exactMatch <https://www.wikidata.org/entity/Q5173053> ;
	skos:broader	medtop:20000808 .

medtop:20000810
	rdf:type skos:Concept ;
	skos:prefLabel	"death and dying"@en-GB ;
	skos:definition	"Social, medical and mental health issues relating to people at the end of their lives"@en-GB ;
	skos:inScheme <http://cv.iptc.org/newscodes/mediatopic/>  ;
	ikos:created "2009-10-22T02:00:00+00:00"^^xsd:dateTime ;
	dct:created "2009-10-22T02:00:00+00:00"^^xsd:dateTime ;
	ikos:modified "2021-02-18T12:00:00+00:00"^^xsd:dateTime ;
	dct:modified "2021-02-18T12:00:00+00:00"^^xsd:dateTime  ;
	skos:closeMatch subj:14023000 ;
	skos:exactMatch <https://www.wikidata.org/entity/Q4> ;
	skos:broader	medtop:20000808 ;
	skos:narrower	medtop:20000811 ;
	skos:narrower	medtop:20000813 .

medtop:20000811
	rdf:type skos:Concept ;
	skos:prefLabel	"euthanasia"@en-GB ;
	skos:definition	"The practice of humanely ending the life of a person suffering from a terminal illness"@en-GB ;
	skos:inScheme <http://cv.iptc.org/newscodes/mediatopic/>  ;
	ikos:created "2009-10-22T02:00:00+00:00"^^xsd:dateTime ;
	dct:created "2009-10-22T02:00:00+00:00"^^xsd:dateTime ;
	ikos:modified "2021-02-18T12:00:00+00:00"^^xsd:dateTime ;
	dct:modified "2021-02-18T12:00:00+00:00"^^xsd:dateTime  ;
	skos:exactMatch subj:14005000 ;
	skos:exactMatch <https://www.wikidata.org/entity/Q100159> ;
	skos:broader	medtop:20000810 ;
	skos:narrower	medtop:20000812 .

medtop:20000812
	rdf:type skos:Concept ;
	skos:prefLabel	"assisted suicide"@en-GB ;
	skos:definition	"The practice of assisting a person suffering from a terminal illness in the process of suicide, often with a physician's oversight"@en-GB ;
	skos:inScheme <http://cv.iptc.org/newscodes/mediatopic/>  ;
	ikos:created "2009-10-22T02:00:00+00:00"^^xsd:dateTime ;
	dct:created "2009-10-22T02:00:00+00:00"^^xsd:dateTime ;
	ikos:modified "2021-02-18T12:00:00+00:00"^^xsd:dateTime ;
	dct:modified "2021-02-18T12:00:00+00:00"^^xsd:dateTime  ;
	skos:broadMatch subj:14005000 ;
	skos:exactMatch <https://www.wikidata.org/entity/Q689846> ;
	skos:broader	medtop:20000811 .

medtop:20000813
	rdf:type skos:Concept ;
	skos:prefLabel	"suicide"@en-GB ;
	skos:definition	"The intentional taking of one's own life"@en-GB ;
	skos:inScheme <http://cv.iptc.org/newscodes/mediatopic/>  ;
	ikos:created "2009-10-22T02:00:00+00:00"^^xsd:dateTime ;
	dct:created "2009-10-22T02:00:00+00:00"^^xsd:dateTime ;
	ikos:modified "2021-02-18T12:00:00+00:00"^^xsd:dateTime ;
	dct:modified "2021-02-18T12:00:00+00:00"^^xsd:dateTime  ;
	skos:exactMatch subj:14005001 ;
	skos:exactMatch <https://www.wikidata.org/entity/Q10737> ;
	skos:broader	medtop:20000810 .

medtop:20000814
	rdf:type skos:Concept ;
	skos:prefLabel	"ethics"@en-GB ;
	skos:definition	"The moral values and standards that define right and wrong actions or decisions"@en-GB ;
	skos:inScheme <http://cv.iptc.org/newscodes/mediatopic/>  ;
	ikos:created "2009-10-22T02:00:00+00:00"^^xsd:dateTime ;
	dct:created "2009-10-22T02:00:00+00:00"^^xsd:dateTime ;
	ikos:modified "2021-07-12T12:00:00+00:00"^^xsd:dateTime ;
	dct:modified "2021-07-12T12:00:00+00:00"^^xsd:dateTime  ;
	skos:exactMatch subj:12006001 ;
	skos:exactMatch <https://www.wikidata.org/entity/Q9465> ;
	skos:broader	medtop:20000808 .

medtop:20000815
	rdf:type skos:Concept ;
	skos:prefLabel	"pornography"@en-GB ;
	skos:definition	"The depiction of sexually explicit acts in various media renditions, such as video or photos, often considered obscene or immoral"@en-GB ;
	skos:inScheme <http://cv.iptc.org/newscodes/mediatopic/>  ;
	ikos:created "2009-10-22T02:00:00+00:00"^^xsd:dateTime ;
	dct:created "2009-10-22T02:00:00+00:00"^^xsd:dateTime ;
	ikos:modified "2021-02-18T12:00:00+00:00"^^xsd:dateTime ;
	dct:modified "2021-02-18T12:00:00+00:00"^^xsd:dateTime  ;
	skos:exactMatch subj:14011000 ;
	skos:exactMatch <https://www.wikidata.org/entity/Q291> ;
	skos:broader	medtop:20000808 .

medtop:20000816
	rdf:type skos:Concept ;
	skos:prefLabel	"sexual behaviour"@en-GB ;
	skos:definition	"The manner in which people express their sexuality in physical acts"@en-GB ;
	skos:inScheme <http://cv.iptc.org/newscodes/mediatopic/>  ;
	ikos:created "2009-10-22T02:00:00+00:00"^^xsd:dateTime ;
	dct:created "2009-10-22T02:00:00+00:00"^^xsd:dateTime ;
	ikos:modified "2021-02-18T12:00:00+00:00"^^xsd:dateTime ;
	dct:modified "2021-02-18T12:00:00+00:00"^^xsd:dateTime  ;
	skos:broadMatch subj:12006000 ;
	skos:exactMatch <https://www.wikidata.org/entity/Q608> ;
	skos:broader	medtop:20000808 .

medtop:20000817
	rdf:type skos:Concept ;
	skos:prefLabel	"welfare"@en-GB ;
	skos:definition	"Help for those in need of food, housing, health and other services"@en-GB ;
	skos:inScheme <http://cv.iptc.org/newscodes/mediatopic/>  ;
	ikos:created "2009-10-22T02:00:00+00:00"^^xsd:dateTime ;
	dct:created "2009-10-22T02:00:00+00:00"^^xsd:dateTime ;
	ikos:modified "2021-02-18T12:00:00+00:00"^^xsd:dateTime ;
	dct:modified "2021-02-18T12:00:00+00:00"^^xsd:dateTime  ;
	skos:exactMatch subj:14015000 ;
	skos:exactMatch <https://www.wikidata.org/entity/Q180043> ;
	skos:broader	medtop:14000000 ;
	skos:narrower	medtop:20000818 ;
	skos:narrower	medtop:20000819 ;
	skos:narrower	medtop:20000820 ;
	skos:narrower	medtop:20001232 ;
	skos:narrower	medtop:20001290 ;
	skos:narrower	medtop:20001317 .

medtop:20000818
	rdf:type skos:Concept ;
	skos:prefLabel	"charity"@en-GB ;
	skos:definition	"The voluntary giving of money, food or other necessities to those in need"@en-GB ;
	skos:inScheme <http://cv.iptc.org/newscodes/mediatopic/>  ;
	ikos:created "2009-10-22T02:00:00+00:00"^^xsd:dateTime ;
	dct:created "2009-10-22T02:00:00+00:00"^^xsd:dateTime ;
	ikos:modified "2021-05-05T12:00:00+00:00"^^xsd:dateTime ;
	dct:modified "2021-05-05T12:00:00+00:00"^^xsd:dateTime  ;
	skos:exactMatch subj:14002000 ;
	skos:exactMatch <https://www.wikidata.org/wiki/Q1077064> ;
	skos:broader	medtop:20000817 .

medtop:20000819
	rdf:type skos:Concept ;
	skos:prefLabel	"long-term care"@en-GB ;
	skos:definition	"Services provided on an extended and ongoing basis to patients suffering from chronic illness or disability"@en-GB ;
	skos:inScheme <http://cv.iptc.org/newscodes/mediatopic/>  ;
	ikos:created "2009-10-22T02:00:00+00:00"^^xsd:dateTime ;
	dct:created "2009-10-22T02:00:00+00:00"^^xsd:dateTime ;
	ikos:modified "2021-05-05T12:00:00+00:00"^^xsd:dateTime ;
	dct:modified "2021-05-05T12:00:00+00:00"^^xsd:dateTime  ;
	skos:exactMatch subj:14018000 ;
	skos:exactMatch <https://www.wikidata.org/entity/Q6672123> ;
	skos:broader	medtop:20000817 .

medtop:20000820
	rdf:type skos:Concept ;
	skos:prefLabel	"social services"@en-GB ;
	skos:definition	"Social programmes, usually publicly sponsored, aimed at promoting people's welfare, such as housing, health care or education services"@en-GB ;
	skos:inScheme <http://cv.iptc.org/newscodes/mediatopic/>  ;
	ikos:created "2009-10-22T02:00:00+00:00"^^xsd:dateTime ;
	dct:created "2009-10-22T02:00:00+00:00"^^xsd:dateTime ;
	ikos:modified "2021-02-18T12:00:00+00:00"^^xsd:dateTime ;
	dct:modified "2021-02-18T12:00:00+00:00"^^xsd:dateTime  ;
	skos:closeMatch subj:14025004 ;
	skos:exactMatch <https://www.wikidata.org/entity/Q12055245> ;
	skos:broader	medtop:20000817 .

medtop:20000822
	rdf:type skos:Concept ;
	skos:prefLabel	"competition discipline"@en-GB ;
	skos:definition	"Different types of sport which can be executed in competitions"@en-GB ;
	skos:inScheme <http://cv.iptc.org/newscodes/mediatopic/>  ;
	ikos:created "2009-10-22T02:00:00+00:00"^^xsd:dateTime ;
	dct:created "2009-10-22T02:00:00+00:00"^^xsd:dateTime ;
	ikos:modified "2021-02-18T12:00:00+00:00"^^xsd:dateTime ;
	dct:modified "2021-02-18T12:00:00+00:00"^^xsd:dateTime  ;
	ikos:hasFacet aspfacet:distance ;
	ikos:hasFacet aspfacet:racetime ;
	skos:broadMatch subj:15000000 ;
	ikos:hasFacet aspfacet:teamsize ;
	ikos:hasFacet aspfacet:parasporttype ;
	ikos:hasFacet aspfacet:ageclass ;
	ikos:hasFacet aspfacet:parasport ;
	ikos:hasFacet aspfacet:racetype ;
	ikos:hasFacet aspfacet:gender ;
	skos:exactMatch <https://www.wikidata.org/entity/Q2312410> ;
	skos:broader	medtop:15000000 ;
	skos:narrower	medtop:20000823 ;
	skos:narrower	medtop:20000824 ;
	skos:narrower	medtop:20000827 ;
	skos:narrower	medtop:20000846 ;
	skos:narrower	medtop:20000847 ;
	skos:narrower	medtop:20000848 ;
	skos:narrower	medtop:20000849 ;
	skos:narrower	medtop:20000851 ;
	skos:narrower	medtop:20000852 ;
	skos:narrower	medtop:20000853 ;
	skos:narrower	medtop:20000854 ;
	skos:narrower	medtop:20000855 ;
	skos:narrower	medtop:20000856 ;
	skos:narrower	medtop:20000875 ;
	skos:narrower	medtop:20000876 ;
	skos:narrower	medtop:20000877 ;
	skos:narrower	medtop:20000883 ;
	skos:narrower	medtop:20000884 ;
	skos:narrower	medtop:20000887 ;
	skos:narrower	medtop:20000888 ;
	skos:narrower	medtop:20000889 ;
	skos:narrower	medtop:20000890 ;
	skos:narrower	medtop:20000892 ;
	skos:narrower	medtop:20000911 ;
	skos:narrower	medtop:20000912 ;
	skos:narrower	medtop:20000913 ;
	skos:narrower	medtop:20000918 ;
	skos:narrower	medtop:20000919 ;
	skos:narrower	medtop:20000922 ;
	skos:narrower	medtop:20000923 ;
	skos:narrower	medtop:20000929 ;
	skos:narrower	medtop:20000933 ;
	skos:narrower	medtop:20000934 ;
	skos:narrower	medtop:20000936 ;
	skos:narrower	medtop:20000937 ;
	skos:narrower	medtop:20000938 ;
	skos:narrower	medtop:20000939 ;
	skos:narrower	medtop:20000940 ;
	skos:narrower	medtop:20000942 ;
	skos:narrower	medtop:20000958 ;
	skos:narrower	medtop:20000959 ;
	skos:narrower	medtop:20000960 ;
	skos:narrower	medtop:20000964 ;
	skos:narrower	medtop:20000965 ;
	skos:narrower	medtop:20000967 ;
	skos:narrower	medtop:20000968 ;
	skos:narrower	medtop:20000978 ;
	skos:narrower	medtop:20000979 ;
	skos:narrower	medtop:20000986 ;
	skos:narrower	medtop:20000987 ;
	skos:narrower	medtop:20000988 ;
	skos:narrower	medtop:20000989 ;
	skos:narrower	medtop:20000990 ;
	skos:narrower	medtop:20000991 ;
	skos:narrower	medtop:20000998 ;
	skos:narrower	medtop:20001010 ;
	skos:narrower	medtop:20001011 ;
	skos:narrower	medtop:20001013 ;
	skos:narrower	medtop:20001014 ;
	skos:narrower	medtop:20001015 ;
	skos:narrower	medtop:20001016 ;
	skos:narrower	medtop:20001017 ;
	skos:narrower	medtop:20001026 ;
	skos:narrower	medtop:20001038 ;
	skos:narrower	medtop:20001047 ;
	skos:narrower	medtop:20001048 ;
	skos:narrower	medtop:20001049 ;
	skos:narrower	medtop:20001055 ;
	skos:narrower	medtop:20001056 ;
	skos:narrower	medtop:20001062 ;
	skos:narrower	medtop:20001063 ;
	skos:narrower	medtop:20001064 ;
	skos:narrower	medtop:20001065 ;
	skos:narrower	medtop:20001066 ;
	skos:narrower	medtop:20001067 ;
	skos:narrower	medtop:20001068 ;
	skos:narrower	medtop:20001069 ;
	skos:narrower	medtop:20001070 ;
	skos:narrower	medtop:20001071 ;
	skos:narrower	medtop:20001083 ;
	skos:narrower	medtop:20001085 ;
	skos:narrower	medtop:20001086 ;
	skos:narrower	medtop:20001087 ;
	skos:narrower	medtop:20001088 ;
	skos:narrower	medtop:20001089 ;
	skos:narrower	medtop:20001091 ;
	skos:narrower	medtop:20001092 ;
	skos:narrower	medtop:20001093 ;
	skos:narrower	medtop:20001097 ;
	skos:narrower	medtop:20001098 ;
	skos:narrower	medtop:20001151 ;
	skos:narrower	medtop:20001154 ;
	skos:narrower	medtop:20001155 ;
	skos:narrower	medtop:20001157 ;
	skos:narrower	medtop:20001175 ;
	skos:narrower	medtop:20001176 ;
	skos:narrower	medtop:20001183 ;
	skos:narrower	medtop:20001240 ;
	skos:narrower	medtop:20001281 ;
	skos:narrower	medtop:20001282 ;
	skos:narrower	medtop:20001286 ;
	skos:narrower	medtop:20001305 ;
	skos:narrower	medtop:20001306 ;
	skos:narrower	medtop:20001307 ;
	skos:narrower	medtop:20001309 ;
	skos:narrower	medtop:20001329 ;
	skos:narrower	medtop:20001330 ;
	skos:narrower	medtop:20001331 ;
	skos:narrower	medtop:20001332 ;
	skos:narrower	medtop:20001333 ;
	skos:narrower	medtop:20001334 ;
	skos:narrower	medtop:20001335 ;
	skos:narrower	medtop:20001336 .

medtop:20000823
	rdf:type skos:Concept ;
	skos:prefLabel	"American football"@en-GB ;
	skos:definition	"Team ball game that opposes two teams of 11 that have offence and defence sections. Each offence attempts to move an oval ball down the 120 yards long field. Points are scored by advancing the ball into the opposing team s end zone."@en-GB ;
	skos:changeNote	"2016-04-06: definition rephrased."@en-GB ;
	skos:inScheme <http://cv.iptc.org/newscodes/mediatopic/>  ;
	ikos:created "2009-10-22T02:00:00+00:00"^^xsd:dateTime ;
	dct:created "2009-10-22T02:00:00+00:00"^^xsd:dateTime ;
	ikos:modified "2021-02-18T12:00:00+00:00"^^xsd:dateTime ;
	dct:modified "2021-02-18T12:00:00+00:00"^^xsd:dateTime  ;
	skos:exactMatch subj:15003000 ;
	skos:exactMatch <https://www.wikidata.org/entity/Q41323> ;
	skos:broader	medtop:20000822 .

medtop:20000824
	rdf:type skos:Concept ;
	skos:prefLabel	"archery"@en-GB ;
	skos:definition	"Archers use bows and arrows to aim at targets 1.22 metres in diameter which are on average 70 metres distant."@en-GB ;
	skos:inScheme <http://cv.iptc.org/newscodes/mediatopic/>  ;
	ikos:created "2009-10-22T02:00:00+00:00"^^xsd:dateTime ;
	dct:created "2009-10-22T02:00:00+00:00"^^xsd:dateTime ;
	ikos:modified "2021-02-18T12:00:00+00:00"^^xsd:dateTime ;
	dct:modified "2021-02-18T12:00:00+00:00"^^xsd:dateTime  ;
	skos:exactMatch subj:15004000 ;
	skos:exactMatch <https://www.wikidata.org/entity/Q108429> ;
	skos:broader	medtop:20000822 ;
	skos:narrower	medtop:20000825 ;
	skos:narrower	medtop:20000826 .

medtop:20000825
	rdf:type skos:Concept ;
	skos:prefLabel	"crossbow shooting"@en-GB ;
	skos:definition	"Shooting with crossbow on targets from different distances"@en-GB ;
	skos:inScheme <http://cv.iptc.org/newscodes/mediatopic/>  ;
	ikos:created "2009-10-22T02:00:00+00:00"^^xsd:dateTime ;
	dct:created "2009-10-22T02:00:00+00:00"^^xsd:dateTime ;
	ikos:modified "2021-02-18T12:00:00+00:00"^^xsd:dateTime ;
	dct:modified "2021-02-18T12:00:00+00:00"^^xsd:dateTime  ;
	skos:exactMatch subj:15004002 ;
	skos:exactMatch <https://www.wikidata.org/entity/Q18089113> ;
	skos:broader	medtop:20000824 .

medtop:20000826
	rdf:type skos:Concept ;
	skos:prefLabel	"longbow"@en-GB ;
	skos:definition	"Shooting with longbow on targets from different distances. The competition is held outdoors on an open (flat) field."@en-GB ;
	skos:inScheme <http://cv.iptc.org/newscodes/mediatopic/>  ;
	ikos:created "2009-10-22T02:00:00+00:00"^^xsd:dateTime ;
	dct:created "2009-10-22T02:00:00+00:00"^^xsd:dateTime ;
	ikos:modified "2021-05-05T12:00:00+00:00"^^xsd:dateTime ;
	dct:modified "2021-05-05T12:00:00+00:00"^^xsd:dateTime  ;
	skos:broadMatch subj:15004000 ;
	skos:exactMatch <https://www.wikidata.org/entity/Q6673620> ;
	skos:broader	medtop:20000824 .

medtop:20000827
	rdf:type skos:Concept ;
	skos:prefLabel	"athletics"@en-GB ;
	skos:definition	"Competitions involving foot races, jumping and throwing which can be on a track inside a stadium or on outside roads"@en-GB ;
	skos:inScheme <http://cv.iptc.org/newscodes/mediatopic/>  ;
	ikos:created "2009-10-22T02:00:00+00:00"^^xsd:dateTime ;
	dct:created "2009-10-22T02:00:00+00:00"^^xsd:dateTime ;
	ikos:modified "2021-05-05T12:00:00+00:00"^^xsd:dateTime ;
	dct:modified "2021-05-05T12:00:00+00:00"^^xsd:dateTime  ;
	skos:exactMatch subj:15005000 ;
	skos:exactMatch <https://www.wikidata.org/entity/Q3312129> ;
	skos:broader	medtop:20000822 ;
	skos:narrower	medtop:20000828 ;
	skos:narrower	medtop:20000829 ;
	skos:narrower	medtop:20000830 ;
	skos:narrower	medtop:20000831 ;
	skos:narrower	medtop:20000832 ;
	skos:narrower	medtop:20000833 ;
	skos:narrower	medtop:20000834 ;
	skos:narrower	medtop:20000835 ;
	skos:narrower	medtop:20000836 ;
	skos:narrower	medtop:20000837 ;
	skos:narrower	medtop:20000838 ;
	skos:narrower	medtop:20000839 ;
	skos:narrower	medtop:20000840 ;
	skos:narrower	medtop:20000841 ;
	skos:narrower	medtop:20000842 ;
	skos:narrower	medtop:20000843 ;
	skos:narrower	medtop:20000844 ;
	skos:narrower	medtop:20000845 ;
	skos:narrower	medtop:20001242 .

medtop:20000828
	rdf:type skos:Concept ;
	skos:prefLabel	"cross-country run"@en-GB ;
	skos:definition	"Competitors run over rough ground and not on a track"@en-GB ;
	skos:inScheme <http://cv.iptc.org/newscodes/mediatopic/>  ;
	ikos:created "2009-10-22T02:00:00+00:00"^^xsd:dateTime ;
	dct:created "2009-10-22T02:00:00+00:00"^^xsd:dateTime ;
	ikos:modified "2021-05-05T12:00:00+00:00"^^xsd:dateTime ;
	dct:modified "2021-05-05T12:00:00+00:00"^^xsd:dateTime  ;
	skos:broadMatch subj:15005000 ;
	skos:exactMatch <https://www.wikidata.org/entity/Q500050> ;
	skos:broader	medtop:20000827 .

medtop:20000829
	rdf:type skos:Concept ;
	skos:prefLabel	"decathlon"@en-GB ;
	skos:definition	"Individual men's competition which involves accumulating points in 10 different disciplines over two days: 1st day - 100m, long-jump, shot-putt, high-jump, 400m. 2nd day - 110m hurdles, discus, pole-vault, javelin and 1,500 metres."@en-GB ;
	skos:inScheme <http://cv.iptc.org/newscodes/mediatopic/>  ;
	ikos:created "2009-10-22T02:00:00+00:00"^^xsd:dateTime ;
	dct:created "2009-10-22T02:00:00+00:00"^^xsd:dateTime ;
	ikos:modified "2021-02-18T12:00:00+00:00"^^xsd:dateTime ;
	dct:modified "2021-02-18T12:00:00+00:00"^^xsd:dateTime  ;
	skos:exactMatch subj:15005027 ;
	skos:exactMatch <https://www.wikidata.org/entity/Q184654> ;
	skos:broader	medtop:20000827 .

medtop:20000830
	rdf:type skos:Concept ;
	skos:prefLabel	"discus throw"@en-GB ;
	skos:definition	"Competitors stand in a netted circle with a 2.50 metres diameter and with a turning motion attempt to throw a discus weighing 2kg for men and 1kg for women as far as possible"@en-GB ;
	skos:inScheme <http://cv.iptc.org/newscodes/mediatopic/>  ;
	ikos:created "2009-10-22T02:00:00+00:00"^^xsd:dateTime ;
	dct:created "2009-10-22T02:00:00+00:00"^^xsd:dateTime ;
	ikos:modified "2021-02-18T12:00:00+00:00"^^xsd:dateTime ;
	dct:modified "2021-02-18T12:00:00+00:00"^^xsd:dateTime  ;
	skos:exactMatch subj:15005024 ;
	skos:exactMatch <https://www.wikidata.org/entity/Q182570> ;
	skos:broader	medtop:20000827 .

medtop:20000831
	rdf:type skos:Concept ;
	skos:prefLabel	"hammer throw"@en-GB ;
	skos:definition	"Competitors throw a hammer consisting of a metal ball, chain and handle as far as they can from a netted circle which is 2.13 metres in diameter. The hammer weighs 7.26kg for men and 4kg for women"@en-GB ;
	skos:inScheme <http://cv.iptc.org/newscodes/mediatopic/>  ;
	ikos:created "2009-10-22T02:00:00+00:00"^^xsd:dateTime ;
	dct:created "2009-10-22T02:00:00+00:00"^^xsd:dateTime ;
	ikos:modified "2021-02-18T12:00:00+00:00"^^xsd:dateTime ;
	dct:modified "2021-02-18T12:00:00+00:00"^^xsd:dateTime  ;
	skos:exactMatch subj:15005025 ;
	skos:exactMatch <https://www.wikidata.org/entity/Q184865> ;
	skos:broader	medtop:20000827 .

medtop:20000832
	rdf:type skos:Concept ;
	skos:prefLabel	"heptathlon"@en-GB ;
	skos:definition	"Competition involving seven separate disciplines over two days. 1st day - 100m hurdles, high jump, shot put, 200 metres. 2nd day - long-jump, javelin, 800 metres"@en-GB ;
	skos:inScheme <http://cv.iptc.org/newscodes/mediatopic/>  ;
	ikos:created "2009-10-22T02:00:00+00:00"^^xsd:dateTime ;
	dct:created "2009-10-22T02:00:00+00:00"^^xsd:dateTime ;
	ikos:modified "2021-02-18T12:00:00+00:00"^^xsd:dateTime ;
	dct:modified "2021-02-18T12:00:00+00:00"^^xsd:dateTime  ;
	skos:exactMatch subj:15005042 ;
	skos:exactMatch <https://www.wikidata.org/entity/Q243264> ;
	skos:broader	medtop:20000827 .

medtop:20000833
	rdf:type skos:Concept ;
	skos:prefLabel	"high jump"@en-GB ;
	skos:definition	"Competitors build up speed over a short sprint and then jump as high as possible over a horizontal bar"@en-GB ;
	skos:inScheme <http://cv.iptc.org/newscodes/mediatopic/>  ;
	ikos:created "2009-10-22T02:00:00+00:00"^^xsd:dateTime ;
	dct:created "2009-10-22T02:00:00+00:00"^^xsd:dateTime ;
	ikos:modified "2021-02-18T12:00:00+00:00"^^xsd:dateTime ;
	dct:modified "2021-02-18T12:00:00+00:00"^^xsd:dateTime  ;
	skos:exactMatch subj:15005019 ;
	skos:exactMatch <https://www.wikidata.org/entity/Q165704> ;
	skos:broader	medtop:20000827 .

medtop:20000834
	rdf:type skos:Concept ;
	skos:prefLabel	"hurdles"@en-GB ;
	skos:definition	"A sprint running race where athletes jump over a series of upright frames"@en-GB ;
	skos:inScheme <http://cv.iptc.org/newscodes/mediatopic/>  ;
	ikos:created "2009-10-22T02:00:00+00:00"^^xsd:dateTime ;
	dct:created "2009-10-22T02:00:00+00:00"^^xsd:dateTime ;
	ikos:modified "2021-05-05T12:00:00+00:00"^^xsd:dateTime ;
	dct:modified "2021-05-05T12:00:00+00:00"^^xsd:dateTime  ;
	skos:broadMatch subj:15005000 ;
	skos:exactMatch <https://www.wikidata.org/entity/Q537769> ;
	skos:broader	medtop:20000827 .

medtop:20000835
	rdf:type skos:Concept ;
	skos:prefLabel	"javelin throw"@en-GB ;
	skos:definition	"Competitors in a specially-designated throwing area attempt to fling a spear-like javelin as far as possible. The javelin weighs 800 grams for men and 600 grams for women."@en-GB ;
	skos:inScheme <http://cv.iptc.org/newscodes/mediatopic/>  ;
	ikos:created "2009-10-22T02:00:00+00:00"^^xsd:dateTime ;
	dct:created "2009-10-22T02:00:00+00:00"^^xsd:dateTime ;
	ikos:modified "2021-02-18T12:00:00+00:00"^^xsd:dateTime ;
	dct:modified "2021-02-18T12:00:00+00:00"^^xsd:dateTime  ;
	skos:exactMatch subj:15005026 ;
	skos:exactMatch <https://www.wikidata.org/entity/Q178108> ;
	skos:broader	medtop:20000827 .

medtop:20000836
	rdf:type skos:Concept ;
	skos:prefLabel	"long distance run"@en-GB ;
	skos:definition	"A running race at distances for more than 1500 metres"@en-GB ;
	skos:inScheme <http://cv.iptc.org/newscodes/mediatopic/>  ;
	ikos:created "2009-10-22T02:00:00+00:00"^^xsd:dateTime ;
	dct:created "2009-10-22T02:00:00+00:00"^^xsd:dateTime ;
	ikos:modified "2021-02-18T12:00:00+00:00"^^xsd:dateTime ;
	dct:modified "2021-02-18T12:00:00+00:00"^^xsd:dateTime  ;
	skos:broadMatch subj:15005000 ;
	skos:exactMatch <https://www.wikidata.org/entity/Q917206> ;
	skos:broader	medtop:20000827 .

medtop:20000837
	rdf:type skos:Concept ;
	skos:prefLabel	"long jump"@en-GB ;
	skos:definition	"Competitors build up speed over a short sprint and then jump in one leap as far as possible"@en-GB ;
	skos:inScheme <http://cv.iptc.org/newscodes/mediatopic/>  ;
	ikos:created "2009-10-22T02:00:00+00:00"^^xsd:dateTime ;
	dct:created "2009-10-22T02:00:00+00:00"^^xsd:dateTime ;
	ikos:modified "2021-02-18T12:00:00+00:00"^^xsd:dateTime ;
	dct:modified "2021-02-18T12:00:00+00:00"^^xsd:dateTime  ;
	skos:exactMatch subj:15005021 ;
	skos:exactMatch <https://www.wikidata.org/entity/Q170737> ;
	skos:broader	medtop:20000827 .

medtop:20000838
	rdf:type skos:Concept ;
	skos:prefLabel	"middle distance run"@en-GB ;
	skos:definition	"A running race at distances for more than 400 metres and up to and including 1500 metres"@en-GB ;
	skos:inScheme <http://cv.iptc.org/newscodes/mediatopic/>  ;
	ikos:created "2009-10-22T02:00:00+00:00"^^xsd:dateTime ;
	dct:created "2009-10-22T02:00:00+00:00"^^xsd:dateTime ;
	ikos:modified "2021-02-18T12:00:00+00:00"^^xsd:dateTime ;
	dct:modified "2021-02-18T12:00:00+00:00"^^xsd:dateTime  ;
	skos:broadMatch subj:15005000 ;
	skos:exactMatch <https://www.wikidata.org/entity/Q1163256> ;
	skos:broader	medtop:20000827 .

medtop:20000839
	rdf:type skos:Concept ;
	skos:prefLabel	"pentathlon"@en-GB ;
	skos:definition	"Only indoor, 60m hurdles, high jump, shot put, long jump, 800 m"@en-GB ;
	skos:inScheme <http://cv.iptc.org/newscodes/mediatopic/>  ;
	ikos:created "2009-10-22T02:00:00+00:00"^^xsd:dateTime ;
	dct:created "2009-10-22T02:00:00+00:00"^^xsd:dateTime ;
	ikos:modified "2021-02-18T12:00:00+00:00"^^xsd:dateTime ;
	dct:modified "2021-02-18T12:00:00+00:00"^^xsd:dateTime  ;
	skos:exactMatch subj:15005069 ;
	skos:exactMatch <https://www.wikidata.org/entity/Q1163125> ;
	skos:broader	medtop:20000827 .

medtop:20000840
	rdf:type skos:Concept ;
	skos:prefLabel	"pole vault"@en-GB ;
	skos:definition	"Competitors use a flexible pole to propel themselves feet-first into the air and clear a bar which is raised higher at each round of jumps."@en-GB ;
	skos:inScheme <http://cv.iptc.org/newscodes/mediatopic/>  ;
	ikos:created "2009-10-22T02:00:00+00:00"^^xsd:dateTime ;
	dct:created "2009-10-22T02:00:00+00:00"^^xsd:dateTime ;
	ikos:modified "2021-02-18T12:00:00+00:00"^^xsd:dateTime ;
	dct:modified "2021-02-18T12:00:00+00:00"^^xsd:dateTime  ;
	skos:exactMatch subj:15005020 ;
	skos:exactMatch <https://www.wikidata.org/entity/Q185027> ;
	skos:broader	medtop:20000827 .

medtop:20000841
	rdf:type skos:Concept ;
	skos:prefLabel	"race walking"@en-GB ;
	skos:definition	"A race requiring the competitor to have always one foot on the ground"@en-GB ;
	skos:inScheme <http://cv.iptc.org/newscodes/mediatopic/>  ;
	ikos:created "2009-10-22T02:00:00+00:00"^^xsd:dateTime ;
	dct:created "2009-10-22T02:00:00+00:00"^^xsd:dateTime ;
	ikos:modified "2021-02-18T12:00:00+00:00"^^xsd:dateTime ;
	dct:modified "2021-02-18T12:00:00+00:00"^^xsd:dateTime  ;
	skos:broadMatch subj:15005000 ;
	skos:exactMatch <https://www.wikidata.org/entity/Q202391> ;
	skos:broader	medtop:20000827 .

medtop:20000842
	rdf:type skos:Concept ;
	skos:prefLabel	"relay run"@en-GB ;
	skos:definition	"A team of athletes run a relay over identical distances"@en-GB ;
	skos:inScheme <http://cv.iptc.org/newscodes/mediatopic/>  ;
	ikos:created "2009-10-22T02:00:00+00:00"^^xsd:dateTime ;
	dct:created "2009-10-22T02:00:00+00:00"^^xsd:dateTime ;
	ikos:modified "2021-02-18T12:00:00+00:00"^^xsd:dateTime ;
	dct:modified "2021-02-18T12:00:00+00:00"^^xsd:dateTime  ;
	skos:broadMatch subj:15005000 ;
	skos:exactMatch <https://www.wikidata.org/entity/Q12469953> ;
	skos:broader	medtop:20000827 .

medtop:20000843
	rdf:type skos:Concept ;
	skos:prefLabel	"shot put"@en-GB ;
	skos:definition	"Competitors stand in a circle with a 2.13 metres diameter and attempt to throw a metal ball weighing 7.26 kg for men and 4kg for women as far as possible. The longest throw wins."@en-GB ;
	skos:inScheme <http://cv.iptc.org/newscodes/mediatopic/>  ;
	ikos:created "2009-10-22T02:00:00+00:00"^^xsd:dateTime ;
	dct:created "2009-10-22T02:00:00+00:00"^^xsd:dateTime ;
	ikos:modified "2021-02-18T12:00:00+00:00"^^xsd:dateTime ;
	dct:modified "2021-02-18T12:00:00+00:00"^^xsd:dateTime  ;
	skos:exactMatch subj:15005023 ;
	skos:exactMatch <https://www.wikidata.org/entity/Q180935> ;
	skos:broader	medtop:20000827 .

medtop:20000844
	rdf:type skos:Concept ;
	skos:prefLabel	"sprint run"@en-GB ;
	skos:definition	"A running race at distances of up to and including 400 metres"@en-GB ;
	skos:inScheme <http://cv.iptc.org/newscodes/mediatopic/>  ;
	ikos:created "2009-10-22T02:00:00+00:00"^^xsd:dateTime ;
	dct:created "2009-10-22T02:00:00+00:00"^^xsd:dateTime ;
	ikos:modified "2021-02-18T12:00:00+00:00"^^xsd:dateTime ;
	dct:modified "2021-02-18T12:00:00+00:00"^^xsd:dateTime  ;
	skos:closeMatch subj:15005000 ;
	skos:exactMatch <https://www.wikidata.org/entity/Q624482> ;
	skos:broader	medtop:20000827 .

medtop:20000845
	rdf:type skos:Concept ;
	skos:prefLabel	"triple jump"@en-GB ;
	skos:definition	"Competitors build up speed over a short sprint and then attempt to jump as far forward as they can using a hop, skip and a jump technique."@en-GB ;
	skos:inScheme <http://cv.iptc.org/newscodes/mediatopic/>  ;
	ikos:created "2009-10-22T02:00:00+00:00"^^xsd:dateTime ;
	dct:created "2009-10-22T02:00:00+00:00"^^xsd:dateTime ;
	ikos:modified "2021-02-18T12:00:00+00:00"^^xsd:dateTime ;
	dct:modified "2021-02-18T12:00:00+00:00"^^xsd:dateTime  ;
	skos:exactMatch subj:15005022 ;
	skos:exactMatch <https://www.wikidata.org/entity/Q187204> ;
	skos:broader	medtop:20000827 .

medtop:20000846
	rdf:type skos:Concept ;
	skos:prefLabel	"Australian rules football"@en-GB ;
	skos:definition	"A form of football played by two teams of 18 competing on a pitch by running with and passing an oval ball. Points are scored by moving the ball between goal posts. Governed by the Australian Football League."@en-GB ;
	skos:changeNote	"2016-04-06: definition rephrased."@en-GB ;
	skos:inScheme <http://cv.iptc.org/newscodes/mediatopic/>  ;
	ikos:created "2009-10-22T02:00:00+00:00"^^xsd:dateTime ;
	dct:created "2009-10-22T02:00:00+00:00"^^xsd:dateTime ;
	ikos:modified "2021-02-18T12:00:00+00:00"^^xsd:dateTime ;
	dct:modified "2021-02-18T12:00:00+00:00"^^xsd:dateTime  ;
	skos:exactMatch subj:15084000 ;
	skos:exactMatch <https://www.wikidata.org/entity/Q50776> ;
	skos:broader	medtop:20000822 .

medtop:20000847
	rdf:type skos:Concept ;
	skos:prefLabel	"badminton"@en-GB ;
	skos:definition	"Two players or two teams of two compete by hitting a shuttlecock weighing approximately five grams over a high net. The aim for each player/team is to prevent the shuttlecock landing on their side of the court."@en-GB ;
	skos:inScheme <http://cv.iptc.org/newscodes/mediatopic/>  ;
	ikos:created "2009-10-22T02:00:00+00:00"^^xsd:dateTime ;
	dct:created "2009-10-22T02:00:00+00:00"^^xsd:dateTime ;
	ikos:modified "2021-02-18T12:00:00+00:00"^^xsd:dateTime ;
	dct:modified "2021-02-18T12:00:00+00:00"^^xsd:dateTime  ;
	skos:exactMatch subj:15006000 ;
	skos:exactMatch <https://www.wikidata.org/entity/Q7291> ;
	skos:broader	medtop:20000822 .

medtop:20000848
	rdf:type skos:Concept ;
	skos:prefLabel	"bandy"@en-GB ;
	skos:definition	"Played outdoors on ice. The size of the ice rink is about the size of a soccer field. Skates like ice hockey. A small hard ball is used for playing. Players play with sticks, much like in ice hockey, but the sticks are shorter and more rounded than in ice"@en-GB ;
	skos:inScheme <http://cv.iptc.org/newscodes/mediatopic/>  ;
	ikos:created "2009-10-22T02:00:00+00:00"^^xsd:dateTime ;
	dct:created "2009-10-22T02:00:00+00:00"^^xsd:dateTime ;
	ikos:modified "2021-02-18T12:00:00+00:00"^^xsd:dateTime ;
	dct:modified "2021-02-18T12:00:00+00:00"^^xsd:dateTime  ;
	skos:exactMatch subj:15076000 ;
	skos:exactMatch <https://www.wikidata.org/entity/Q183018> ;
	skos:broader	medtop:20000822 .

medtop:20000849
	rdf:type skos:Concept ;
	skos:prefLabel	"baseball"@en-GB ;
	skos:definition	"A game between two teams of nine played on an enclosed ground. The team which scores the most points wins. A point is scored when a player runs around the ground marked out by four bases. To do this he has to hit the ball thrown at him by a rival player."@en-GB ;
	skos:inScheme <http://cv.iptc.org/newscodes/mediatopic/>  ;
	ikos:created "2009-10-22T02:00:00+00:00"^^xsd:dateTime ;
	dct:created "2009-10-22T02:00:00+00:00"^^xsd:dateTime ;
	ikos:modified "2021-02-18T12:00:00+00:00"^^xsd:dateTime ;
	dct:modified "2021-02-18T12:00:00+00:00"^^xsd:dateTime  ;
	skos:exactMatch subj:15007000 ;
	skos:exactMatch <https://www.wikidata.org/entity/Q5369> ;
	skos:broader	medtop:20000822 ;
	skos:narrower	medtop:20000850 .

medtop:20000850
	rdf:type skos:Concept ;
	skos:prefLabel	"rubberball baseball"@en-GB ;
	skos:definition	"Sometimes called ''soft baseball,'' the game is played with a rubber baseball of varying degrees of hardness depending upon the age and level of the players."@en-GB ;
	skos:inScheme <http://cv.iptc.org/newscodes/mediatopic/>  ;
	ikos:created "2009-10-22T02:00:00+00:00"^^xsd:dateTime ;
	dct:created "2009-10-22T02:00:00+00:00"^^xsd:dateTime ;
	ikos:modified "2021-05-05T12:00:00+00:00"^^xsd:dateTime ;
	dct:modified "2021-05-05T12:00:00+00:00"^^xsd:dateTime  ;
	skos:exactMatch subj:15007004 ;
	skos:exactMatch <https://www.wikidata.org/entity/Q171038> ;
	skos:broader	medtop:20000849 .

medtop:20000851
	rdf:type skos:Concept ;
	skos:prefLabel	"basketball"@en-GB ;
	skos:definition	"Game played between two teams of five - points are scored by placing the large inflated ball into a net fixed on a ring 3.05m above the ground."@en-GB ;
	skos:inScheme <http://cv.iptc.org/newscodes/mediatopic/>  ;
	ikos:created "2009-10-22T02:00:00+00:00"^^xsd:dateTime ;
	dct:created "2009-10-22T02:00:00+00:00"^^xsd:dateTime ;
	ikos:modified "2021-02-18T12:00:00+00:00"^^xsd:dateTime ;
	dct:modified "2021-02-18T12:00:00+00:00"^^xsd:dateTime  ;
	skos:exactMatch subj:15008000 ;
	skos:exactMatch <https://www.wikidata.org/entity/Q5372> ;
	skos:broader	medtop:20000822 .

medtop:20000852
	rdf:type skos:Concept ;
	skos:prefLabel	"biathlon"@en-GB ;
	skos:definition	"A combination of cross-country skiing and target shooting on a 12.5 K course in a pursuit format."@en-GB ;
	skos:inScheme <http://cv.iptc.org/newscodes/mediatopic/>  ;
	ikos:created "2009-10-22T02:00:00+00:00"^^xsd:dateTime ;
	dct:created "2009-10-22T02:00:00+00:00"^^xsd:dateTime ;
	ikos:modified "2021-05-05T12:00:00+00:00"^^xsd:dateTime ;
	dct:modified "2021-05-05T12:00:00+00:00"^^xsd:dateTime  ;
	skos:exactMatch subj:15009000 ;
	skos:exactMatch <https://www.wikidata.org/entity/Q166788> ;
	skos:broader	medtop:20000822 .

medtop:20000853
	rdf:type skos:Concept ;
	skos:prefLabel	"billiards"@en-GB ;
	skos:definition	"A cue sport with balls on a table without a specific order to play them"@en-GB ;
	skos:inScheme <http://cv.iptc.org/newscodes/mediatopic/>  ;
	ikos:created "2009-10-22T02:00:00+00:00"^^xsd:dateTime ;
	dct:created "2009-10-22T02:00:00+00:00"^^xsd:dateTime ;
	ikos:modified "2021-02-18T12:00:00+00:00"^^xsd:dateTime ;
	dct:modified "2021-02-18T12:00:00+00:00"^^xsd:dateTime  ;
	skos:broadMatch subj:15010000 ;
	ikos:hasFacet aspfacet:billiardtype ;
	skos:exactMatch <https://www.wikidata.org/entity/Q3341285> ;
	skos:broader	medtop:20000822 .

medtop:20000854
	rdf:type skos:Concept ;
	skos:prefLabel	"bobsleigh"@en-GB ;
	skos:definition	"One, two or four people racing down a course in a sled that consists of a main hull, a frame, two axles and sets of runners. The total time of all heats in a competition is added together to determine the winner."@en-GB ;
	skos:inScheme <http://cv.iptc.org/newscodes/mediatopic/>  ;
	ikos:created "2009-10-22T02:00:00+00:00"^^xsd:dateTime ;
	dct:created "2009-10-22T02:00:00+00:00"^^xsd:dateTime ;
	ikos:modified "2022-02-03T12:00:00+00:00"^^xsd:dateTime ;
	dct:modified "2022-02-03T12:00:00+00:00"^^xsd:dateTime  ;
	skos:exactMatch subj:15011000 ;
	skos:exactMatch <https://www.wikidata.org/entity/Q177275> ;
	skos:broader	medtop:20000822 .

medtop:20000855
	rdf:type skos:Concept ;
	skos:prefLabel	"boules"@en-GB ;
	skos:definition	"Collective name of a number of games where the common goal is to move the competitor's balls as close to a small target ball as possible, played on a grass or sand surface. Balls are thrown (as in petanque and boules) or rolled (as in lawn bowls or bocce)."@en-GB ;
	skos:inScheme <http://cv.iptc.org/newscodes/mediatopic/>  ;
	ikos:created "2009-10-22T02:00:00+00:00"^^xsd:dateTime ;
	dct:created "2009-10-22T02:00:00+00:00"^^xsd:dateTime ;
	ikos:modified "2021-05-05T12:00:00+00:00"^^xsd:dateTime ;
	dct:modified "2021-05-05T12:00:00+00:00"^^xsd:dateTime  ;
	skos:exactMatch subj:15013000 ;
	skos:exactMatch <https://www.wikidata.org/entity/Q895060> ;
	skos:broader	medtop:20000822 .

medtop:20000856
	rdf:type skos:Concept ;
	skos:prefLabel	"boxing"@en-GB ;
	skos:definition	"Combat sport in which two men/women fight using only their fists covered by padded gloves in a square ring measuring 6m a side. The fight is usually split into 12 rounds of three minutes each."@en-GB ;
	skos:inScheme <http://cv.iptc.org/newscodes/mediatopic/>  ;
	ikos:created "2009-10-22T02:00:00+00:00"^^xsd:dateTime ;
	dct:created "2009-10-22T02:00:00+00:00"^^xsd:dateTime ;
	ikos:modified "2021-02-18T12:00:00+00:00"^^xsd:dateTime ;
	dct:modified "2021-02-18T12:00:00+00:00"^^xsd:dateTime  ;
	skos:exactMatch subj:15014000 ;
	ikos:hasFacet aspfacet:weightclasstype ;
	skos:exactMatch <https://www.wikidata.org/entity/Q32112> ;
	skos:broader	medtop:20000822 ;
	skos:narrower	medtop:20000857 ;
	skos:narrower	medtop:20000858 ;
	skos:narrower	medtop:20000859 ;
	skos:narrower	medtop:20000860 ;
	skos:narrower	medtop:20000861 ;
	skos:narrower	medtop:20000862 ;
	skos:narrower	medtop:20000863 ;
	skos:narrower	medtop:20000864 ;
	skos:narrower	medtop:20000865 ;
	skos:narrower	medtop:20000866 ;
	skos:narrower	medtop:20000867 ;
	skos:narrower	medtop:20000868 ;
	skos:narrower	medtop:20000869 ;
	skos:narrower	medtop:20000870 ;
	skos:narrower	medtop:20000871 ;
	skos:narrower	medtop:20000872 ;
	skos:narrower	medtop:20000873 ;
	skos:narrower	medtop:20000874 .

medtop:20000857
	rdf:type skos:Concept ;
	skos:prefLabel	"bantamweight (boxing)"@en-GB ;
	skos:definition	"Weight category which varies according to the federation or the Olympic Games"@en-GB ;
	skos:inScheme <http://cv.iptc.org/newscodes/mediatopic/>  ;
	ikos:created "2009-10-22T02:00:00+00:00"^^xsd:dateTime ;
	dct:created "2009-10-22T02:00:00+00:00"^^xsd:dateTime ;
	ikos:modified "2021-12-21T12:00:00+00:00"^^xsd:dateTime ;
	dct:modified "2021-12-21T12:00:00+00:00"^^xsd:dateTime  ; 
	ikos:retired "2015-02-24T12:00:00+00:00"^^xsd:dateTime ;
	skos:closeMatch subj:15014014 ;
	skos:exactMatch <https://www.wikidata.org/entity/Q948780> ;
	skos:broader	medtop:20000856 .

medtop:20000858
	rdf:type skos:Concept ;
	skos:prefLabel	"cruiserweight (boxing)"@en-GB ;
	skos:definition	"Weight category which varies according to the federation or the Olympic Games"@en-GB ;
	skos:inScheme <http://cv.iptc.org/newscodes/mediatopic/>  ;
	ikos:created "2009-10-22T02:00:00+00:00"^^xsd:dateTime ;
	dct:created "2009-10-22T02:00:00+00:00"^^xsd:dateTime ;
	ikos:modified "2021-12-21T12:00:00+00:00"^^xsd:dateTime ;
	dct:modified "2021-12-21T12:00:00+00:00"^^xsd:dateTime  ; 
	ikos:retired "2015-02-24T12:00:00+00:00"^^xsd:dateTime ;
	skos:closeMatch subj:15014003 ;
	skos:exactMatch <https://www.wikidata.org/entity/Q867600> ;
	skos:broader	medtop:20000856 .

medtop:20000859
	rdf:type skos:Concept ;
	skos:prefLabel	"featherweight (boxing)"@en-GB ;
	skos:definition	"Weight category which varies according to the federation or the Olympic Games"@en-GB ;
	skos:inScheme <http://cv.iptc.org/newscodes/mediatopic/>  ;
	ikos:created "2014-04-08T12:00:00+00:00"^^xsd:dateTime ;
	dct:created "2014-04-08T12:00:00+00:00"^^xsd:dateTime ;
	ikos:modified "2021-12-21T12:00:00+00:00"^^xsd:dateTime ;
	dct:modified "2021-12-21T12:00:00+00:00"^^xsd:dateTime  ; 
	ikos:retired "2015-02-24T12:00:00+00:00"^^xsd:dateTime ;
	skos:closeMatch subj:15014012 ;
	skos:exactMatch <https://www.wikidata.org/entity/Q597315> ;
	skos:broader	medtop:20000856 .

medtop:20000860
	rdf:type skos:Concept ;
	skos:prefLabel	"flyweight (boxing)"@en-GB ;
	skos:definition	"Weight category which varies according to the federation or the Olympic Games"@en-GB ;
	skos:inScheme <http://cv.iptc.org/newscodes/mediatopic/>  ;
	ikos:created "2009-10-22T02:00:00+00:00"^^xsd:dateTime ;
	dct:created "2009-10-22T02:00:00+00:00"^^xsd:dateTime ;
	ikos:modified "2021-12-21T12:00:00+00:00"^^xsd:dateTime ;
	dct:modified "2021-12-21T12:00:00+00:00"^^xsd:dateTime  ; 
	ikos:retired "2015-02-24T12:00:00+00:00"^^xsd:dateTime ;
	skos:closeMatch subj:15014016 ;
	skos:exactMatch <https://www.wikidata.org/entity/Q508484> ;
	skos:broader	medtop:20000856 .

medtop:20000861
	rdf:type skos:Concept ;
	skos:prefLabel	"heavyweight (boxing)"@en-GB ;
	skos:definition	"Weight category which varies according to the federation or the Olympic Games"@en-GB ;
	skos:inScheme <http://cv.iptc.org/newscodes/mediatopic/>  ;
	ikos:created "2009-10-22T02:00:00+00:00"^^xsd:dateTime ;
	dct:created "2009-10-22T02:00:00+00:00"^^xsd:dateTime ;
	ikos:modified "2021-12-21T12:00:00+00:00"^^xsd:dateTime ;
	dct:modified "2021-12-21T12:00:00+00:00"^^xsd:dateTime  ; 
	ikos:retired "2015-02-24T12:00:00+00:00"^^xsd:dateTime ;
	skos:closeMatch subj:15014002 ;
	skos:exactMatch <https://www.wikidata.org/entity/Q281678> ;
	skos:broader	medtop:20000856 .

medtop:20000862
	rdf:type skos:Concept ;
	skos:prefLabel	"light flyweight (boxing)"@en-GB ;
	skos:definition	"Weight category which varies according to the federation or the Olympic Games"@en-GB ;
	skos:inScheme <http://cv.iptc.org/newscodes/mediatopic/>  ;
	ikos:created "2009-10-22T02:00:00+00:00"^^xsd:dateTime ;
	dct:created "2009-10-22T02:00:00+00:00"^^xsd:dateTime ;
	ikos:modified "2021-12-21T12:00:00+00:00"^^xsd:dateTime ;
	dct:modified "2021-12-21T12:00:00+00:00"^^xsd:dateTime  ; 
	ikos:retired "2015-02-24T12:00:00+00:00"^^xsd:dateTime ;
	skos:closeMatch subj:15014017 ;
	skos:exactMatch <https://www.wikidata.org/entity/Q1096810> ;
	skos:broader	medtop:20000856 .

medtop:20000863
	rdf:type skos:Concept ;
	skos:prefLabel	"light-heavyweight (boxing)"@en-GB ;
	skos:definition	"Weight category which varies according to the federation or the Olympic Games"@en-GB ;
	skos:inScheme <http://cv.iptc.org/newscodes/mediatopic/>  ;
	ikos:created "2009-10-22T02:00:00+00:00"^^xsd:dateTime ;
	dct:created "2009-10-22T02:00:00+00:00"^^xsd:dateTime ;
	ikos:modified "2021-12-21T12:00:00+00:00"^^xsd:dateTime ;
	dct:modified "2021-12-21T12:00:00+00:00"^^xsd:dateTime  ; 
	ikos:retired "2015-02-24T12:00:00+00:00"^^xsd:dateTime ;
	skos:closeMatch subj:15014004 ;
	skos:exactMatch <https://www.wikidata.org/entity/Q1004748> ;
	skos:broader	medtop:20000856 .

medtop:20000864
	rdf:type skos:Concept ;
	skos:prefLabel	"light-middleweight (boxing)"@en-GB ;
	skos:definition	"Weight category which varies according to the federation or the Olympic Games"@en-GB ;
	skos:inScheme <http://cv.iptc.org/newscodes/mediatopic/>  ;
	ikos:created "2009-10-22T02:00:00+00:00"^^xsd:dateTime ;
	dct:created "2009-10-22T02:00:00+00:00"^^xsd:dateTime ;
	ikos:modified "2021-12-21T12:00:00+00:00"^^xsd:dateTime ;
	dct:modified "2021-12-21T12:00:00+00:00"^^xsd:dateTime  ; 
	ikos:retired "2015-02-24T12:00:00+00:00"^^xsd:dateTime ;
	skos:closeMatch subj:15014007 ;
	skos:exactMatch <https://www.wikidata.org/entity/Q1215222> ;
	skos:broader	medtop:20000856 .

medtop:20000865
	rdf:type skos:Concept ;
	skos:prefLabel	"light-welterweight (boxing)"@en-GB ;
	skos:definition	"Weight category which varies according to the federation or the Olympic Games"@en-GB ;
	skos:inScheme <http://cv.iptc.org/newscodes/mediatopic/>  ;
	ikos:created "2009-10-22T02:00:00+00:00"^^xsd:dateTime ;
	dct:created "2009-10-22T02:00:00+00:00"^^xsd:dateTime ;
	ikos:modified "2021-12-21T12:00:00+00:00"^^xsd:dateTime ;
	dct:modified "2021-12-21T12:00:00+00:00"^^xsd:dateTime  ; 
	ikos:retired "2015-02-24T12:00:00+00:00"^^xsd:dateTime ;
	skos:closeMatch subj:15014009 ;
	skos:exactMatch <https://www.wikidata.org/entity/Q1112498> ;
	skos:broader	medtop:20000856 .

medtop:20000866
	rdf:type skos:Concept ;
	skos:prefLabel	"lightweight (boxing)"@en-GB ;
	skos:definition	"Weight category which varies according to the federation or the Olympic Games"@en-GB ;
	skos:inScheme <http://cv.iptc.org/newscodes/mediatopic/>  ;
	ikos:created "2009-10-22T02:00:00+00:00"^^xsd:dateTime ;
	dct:created "2009-10-22T02:00:00+00:00"^^xsd:dateTime ;
	ikos:modified "2021-12-21T12:00:00+00:00"^^xsd:dateTime ;
	dct:modified "2021-12-21T12:00:00+00:00"^^xsd:dateTime  ; 
	ikos:retired "2015-02-24T12:00:00+00:00"^^xsd:dateTime ;
	skos:closeMatch subj:15047007 ;
	skos:exactMatch <https://www.wikidata.org/entity/Q1051922> ;
	skos:broader	medtop:20000856 .

medtop:20000867
	rdf:type skos:Concept ;
	skos:prefLabel	"middleweight (boxing)"@en-GB ;
	skos:definition	"Weight category which varies according to the federation or the Olympic Games"@en-GB ;
	skos:inScheme <http://cv.iptc.org/newscodes/mediatopic/>  ;
	ikos:created "2009-10-22T02:00:00+00:00"^^xsd:dateTime ;
	dct:created "2009-10-22T02:00:00+00:00"^^xsd:dateTime ;
	ikos:modified "2021-12-21T12:00:00+00:00"^^xsd:dateTime ;
	dct:modified "2021-12-21T12:00:00+00:00"^^xsd:dateTime  ; 
	ikos:retired "2015-02-24T12:00:00+00:00"^^xsd:dateTime ;
	skos:closeMatch subj:15014006 ;
	skos:exactMatch <https://www.wikidata.org/entity/Q1051530> ;
	skos:broader	medtop:20000856 .

medtop:20000868
	rdf:type skos:Concept ;
	skos:prefLabel	"straw weight (boxing)"@en-GB ;
	skos:definition	"Weight category which varies according to the federation or the Olympic Games"@en-GB ;
	skos:inScheme <http://cv.iptc.org/newscodes/mediatopic/>  ;
	ikos:created "2009-10-22T02:00:00+00:00"^^xsd:dateTime ;
	dct:created "2009-10-22T02:00:00+00:00"^^xsd:dateTime ;
	ikos:modified "2021-12-21T12:00:00+00:00"^^xsd:dateTime ;
	dct:modified "2021-12-21T12:00:00+00:00"^^xsd:dateTime  ; 
	ikos:retired "2015-02-24T12:00:00+00:00"^^xsd:dateTime ;
	skos:broadMatch subj:15014000 ;
	skos:exactMatch <https://www.wikidata.org/entity/Q282168> ;
	skos:broader	medtop:20000856 .

medtop:20000869
	rdf:type skos:Concept ;
	skos:prefLabel	"super-bantamweight (boxing)"@en-GB ;
	skos:definition	"Weight category which varies according to the federation or the Olympic Games"@en-GB ;
	skos:inScheme <http://cv.iptc.org/newscodes/mediatopic/>  ;
	ikos:created "2009-10-22T02:00:00+00:00"^^xsd:dateTime ;
	dct:created "2009-10-22T02:00:00+00:00"^^xsd:dateTime ;
	ikos:modified "2021-12-21T12:00:00+00:00"^^xsd:dateTime ;
	dct:modified "2021-12-21T12:00:00+00:00"^^xsd:dateTime  ; 
	ikos:retired "2015-02-24T12:00:00+00:00"^^xsd:dateTime ;
	skos:closeMatch subj:15014013 ;
	skos:exactMatch <https://www.wikidata.org/entity/Q1048358> ;
	skos:broader	medtop:20000856 .

medtop:20000870
	rdf:type skos:Concept ;
	skos:prefLabel	"super-featherweight (boxing)"@en-GB ;
	skos:definition	"Weight category which varies according to the federation or the Olympic Games"@en-GB ;
	skos:inScheme <http://cv.iptc.org/newscodes/mediatopic/>  ;
	ikos:created "2009-10-22T02:00:00+00:00"^^xsd:dateTime ;
	dct:created "2009-10-22T02:00:00+00:00"^^xsd:dateTime ;
	ikos:modified "2021-12-21T12:00:00+00:00"^^xsd:dateTime ;
	dct:modified "2021-12-21T12:00:00+00:00"^^xsd:dateTime  ; 
	ikos:retired "2015-02-24T12:00:00+00:00"^^xsd:dateTime ;
	skos:closeMatch subj:15014011 ;
	skos:exactMatch <https://www.wikidata.org/entity/Q763947> ;
	skos:broader	medtop:20000856 .

medtop:20000871
	rdf:type skos:Concept ;
	skos:prefLabel	"super-flyweight (boxing)"@en-GB ;
	skos:definition	"Weight category which varies according to the federation or the Olympic Games"@en-GB ;
	skos:inScheme <http://cv.iptc.org/newscodes/mediatopic/>  ;
	ikos:created "2009-10-22T02:00:00+00:00"^^xsd:dateTime ;
	dct:created "2009-10-22T02:00:00+00:00"^^xsd:dateTime ;
	ikos:modified "2021-12-21T12:00:00+00:00"^^xsd:dateTime ;
	dct:modified "2021-12-21T12:00:00+00:00"^^xsd:dateTime  ; 
	ikos:retired "2015-02-24T12:00:00+00:00"^^xsd:dateTime ;
	skos:closeMatch subj:15014015 ;
	skos:exactMatch <https://www.wikidata.org/entity/Q11699026> ;
	skos:broader	medtop:20000856 .

medtop:20000872
	rdf:type skos:Concept ;
	skos:prefLabel	"super-heavyweight (boxing)"@en-GB ;
	skos:definition	"Weight category which varies according to the federation or the Olympic Games"@en-GB ;
	skos:inScheme <http://cv.iptc.org/newscodes/mediatopic/>  ;
	ikos:created "2009-10-22T02:00:00+00:00"^^xsd:dateTime ;
	dct:created "2009-10-22T02:00:00+00:00"^^xsd:dateTime ;
	ikos:modified "2021-12-21T12:00:00+00:00"^^xsd:dateTime ;
	dct:modified "2021-12-21T12:00:00+00:00"^^xsd:dateTime  ; 
	ikos:retired "2015-02-24T12:00:00+00:00"^^xsd:dateTime ;
	skos:closeMatch subj:15014001 ;
	skos:exactMatch <https://www.wikidata.org/entity/Q507205> ;
	skos:broader	medtop:20000856 .

medtop:20000873
	rdf:type skos:Concept ;
	skos:prefLabel	"super-middleweight (boxing)"@en-GB ;
	skos:definition	"Weight category which varies according to the federation or the Olympic Games"@en-GB ;
	skos:inScheme <http://cv.iptc.org/newscodes/mediatopic/>  ;
	ikos:created "2009-10-22T02:00:00+00:00"^^xsd:dateTime ;
	dct:created "2009-10-22T02:00:00+00:00"^^xsd:dateTime ;
	ikos:modified "2021-12-21T12:00:00+00:00"^^xsd:dateTime ;
	dct:modified "2021-12-21T12:00:00+00:00"^^xsd:dateTime  ; 
	ikos:retired "2015-02-24T12:00:00+00:00"^^xsd:dateTime ;
	skos:closeMatch subj:15014005 ;
	skos:exactMatch <https://www.wikidata.org/entity/Q645063> ;
	skos:broader	medtop:20000856 .

medtop:20000874
	rdf:type skos:Concept ;
	skos:prefLabel	"welterweight (boxing)"@en-GB ;
	skos:definition	"Weight category which varies according to the federation or the Olympic Games"@en-GB ;
	skos:inScheme <http://cv.iptc.org/newscodes/mediatopic/>  ;
	ikos:created "2009-10-22T02:00:00+00:00"^^xsd:dateTime ;
	dct:created "2009-10-22T02:00:00+00:00"^^xsd:dateTime ;
	ikos:modified "2021-12-21T12:00:00+00:00"^^xsd:dateTime ;
	dct:modified "2021-12-21T12:00:00+00:00"^^xsd:dateTime  ; 
	ikos:retired "2015-02-24T12:00:00+00:00"^^xsd:dateTime ;
	skos:closeMatch subj:15014008 ;
	skos:exactMatch <https://www.wikidata.org/entity/Q766904> ;
	skos:broader	medtop:20000856 .

medtop:20000875
	rdf:type skos:Concept ;
	skos:prefLabel	"bullfighting"@en-GB ;
	skos:definition	"Classical contest pitting man against the bull"@en-GB ;
	skos:inScheme <http://cv.iptc.org/newscodes/mediatopic/>  ;
	ikos:created "2009-10-22T02:00:00+00:00"^^xsd:dateTime ;
	dct:created "2009-10-22T02:00:00+00:00"^^xsd:dateTime ;
	ikos:modified "2021-02-18T12:00:00+00:00"^^xsd:dateTime ;
	dct:modified "2021-02-18T12:00:00+00:00"^^xsd:dateTime  ;
	skos:exactMatch subj:01003000 ;
	skos:exactMatch <https://www.wikidata.org/entity/Q184940> ;
	skos:broader	medtop:20000822 .

medtop:20000876
	rdf:type skos:Concept ;
	skos:prefLabel	"Canadian football"@en-GB ;
	skos:definition	"Team ball game that opposes two teams of 12 that have offence and defence sections. Each offence attempts to move an oval ball down the 150 yards long field. Points are scored by advancing the ball into the opposing team s end zone."@en-GB ;
	skos:changeNote	"2016-04-06: definition rephrased."@en-GB ;
	skos:inScheme <http://cv.iptc.org/newscodes/mediatopic/>  ;
	ikos:created "2009-10-22T02:00:00+00:00"^^xsd:dateTime ;
	dct:created "2009-10-22T02:00:00+00:00"^^xsd:dateTime ;
	ikos:modified "2021-02-18T12:00:00+00:00"^^xsd:dateTime ;
	dct:modified "2021-02-18T12:00:00+00:00"^^xsd:dateTime  ;
	skos:exactMatch subj:15085000 ;
	skos:exactMatch <https://www.wikidata.org/entity/Q248534> ;
	skos:broader	medtop:20000822 .

medtop:20000877
	rdf:type skos:Concept ;
	skos:prefLabel	"canoeing"@en-GB ;
	skos:definition	"Competition involving canoes which are generally kneeled and paddled with a single-bladed paddle"@en-GB ;
	skos:inScheme <http://cv.iptc.org/newscodes/mediatopic/>  ;
	ikos:created "2009-10-22T02:00:00+00:00"^^xsd:dateTime ;
	dct:created "2009-10-22T02:00:00+00:00"^^xsd:dateTime ;
	ikos:modified "2021-02-18T12:00:00+00:00"^^xsd:dateTime ;
	dct:modified "2021-02-18T12:00:00+00:00"^^xsd:dateTime  ;
	ikos:hasFacet aspfacet:canoekayaktype ;
	skos:broadMatch subj:15015000 ;
	skos:exactMatch <https://www.wikidata.org/entity/Q20856109> ;
	skos:broader	medtop:20000822 ;
	skos:narrower	medtop:20000878 ;
	skos:narrower	medtop:20000879 ;
	skos:narrower	medtop:20000880 ;
	skos:narrower	medtop:20000881 ;
	skos:narrower	medtop:20000882 .

medtop:20000878
	rdf:type skos:Concept ;
	skos:prefLabel	"C1 (canoeing)"@en-GB ;
	skos:definition	"One-seater canoe (open boat with competitor using a single bladed paddle"@en-GB ;
	skos:inScheme <http://cv.iptc.org/newscodes/mediatopic/>  ;
	ikos:created "2009-10-22T02:00:00+00:00"^^xsd:dateTime ;
	dct:created "2009-10-22T02:00:00+00:00"^^xsd:dateTime ;
	ikos:modified "2021-12-21T12:00:00+00:00"^^xsd:dateTime ;
	dct:modified "2021-12-21T12:00:00+00:00"^^xsd:dateTime  ; 
	ikos:retired "2015-02-24T12:00:00+00:00"^^xsd:dateTime ;
	skos:exactMatch subj:15015008 ;
	skos:broader	medtop:20000877 .

medtop:20000879
	rdf:type skos:Concept ;
	skos:prefLabel	"C2 (canoeing)"@en-GB ;
	skos:definition	"Two-seater canoe (open boat) - competitors use a single bladed paddle"@en-GB ;
	skos:inScheme <http://cv.iptc.org/newscodes/mediatopic/>  ;
	ikos:created "2009-10-22T02:00:00+00:00"^^xsd:dateTime ;
	dct:created "2009-10-22T02:00:00+00:00"^^xsd:dateTime ;
	ikos:modified "2021-12-21T12:00:00+00:00"^^xsd:dateTime ;
	dct:modified "2021-12-21T12:00:00+00:00"^^xsd:dateTime  ; 
	ikos:retired "2015-02-24T12:00:00+00:00"^^xsd:dateTime ;
	skos:exactMatch subj:15015009 ;
	skos:broader	medtop:20000877 .

medtop:20000880
	rdf:type skos:Concept ;
	skos:prefLabel	"C4 (canoeing)"@en-GB ;
	skos:definition	"Four-seater canoe (open boat) with each competitor using a single bladed paddle"@en-GB ;
	skos:inScheme <http://cv.iptc.org/newscodes/mediatopic/>  ;
	ikos:created "2009-10-22T02:00:00+00:00"^^xsd:dateTime ;
	dct:created "2009-10-22T02:00:00+00:00"^^xsd:dateTime ;
	ikos:modified "2021-12-21T12:00:00+00:00"^^xsd:dateTime ;
	dct:modified "2021-12-21T12:00:00+00:00"^^xsd:dateTime  ; 
	ikos:retired "2015-02-24T12:00:00+00:00"^^xsd:dateTime ;
	skos:broadMatch subj:15015010 ;
	skos:broader	medtop:20000877 .

medtop:20000881
	rdf:type skos:Concept ;
	skos:prefLabel	"canoe sailing"@en-GB ;
	skos:definition	"A race involving a canoe equipped with a sail."@en-GB ;
	skos:note	"Retired. Use Media Topic canoeing + sports facet canoekayaktype"@en-GB ;
	skos:inScheme <http://cv.iptc.org/newscodes/mediatopic/>  ;
	ikos:created "2009-10-22T02:00:00+00:00"^^xsd:dateTime ;
	dct:created "2009-10-22T02:00:00+00:00"^^xsd:dateTime ;
	ikos:modified "2021-05-05T12:00:00+00:00"^^xsd:dateTime ;
	dct:modified "2021-05-05T12:00:00+00:00"^^xsd:dateTime  ; 
	ikos:retired "2017-07-04T12:00:00+00:00"^^xsd:dateTime ;
	skos:exactMatch subj:15015011 ;
	skos:exactMatch <https://www.wikidata.org/entity/Q440985> ;
	skos:broader	medtop:20000877 .

medtop:20000882
	rdf:type skos:Concept ;
	skos:prefLabel	"pontoniering"@en-GB ;
	skos:definition	"Team sport, military tradition, similar to canoe regatta, in boats"@en-GB ;
	skos:note	"Retired. Use Media Topic canoeing + sports facet canoekayaktype"@en-GB ;
	skos:inScheme <http://cv.iptc.org/newscodes/mediatopic/>  ;
	ikos:created "2009-10-22T02:00:00+00:00"^^xsd:dateTime ;
	dct:created "2009-10-22T02:00:00+00:00"^^xsd:dateTime ;
	ikos:modified "2021-02-18T12:00:00+00:00"^^xsd:dateTime ;
	dct:modified "2021-02-18T12:00:00+00:00"^^xsd:dateTime  ; 
	ikos:retired "2017-07-04T12:00:00+00:00"^^xsd:dateTime ;
	skos:exactMatch subj:15015012 ;
	skos:broader	medtop:20000877 .

medtop:20000883
	rdf:type skos:Concept ;
	skos:prefLabel	"casting (fishing)"@en-GB ;
	skos:definition	"Using fishing equipment to hit a target and score points"@en-GB ;
	skos:inScheme <http://cv.iptc.org/newscodes/mediatopic/>  ;
	ikos:created "2009-10-22T02:00:00+00:00"^^xsd:dateTime ;
	dct:created "2009-10-22T02:00:00+00:00"^^xsd:dateTime ;
	ikos:modified "2021-07-12T12:00:00+00:00"^^xsd:dateTime ;
	dct:modified "2021-07-12T12:00:00+00:00"^^xsd:dateTime  ;
	skos:exactMatch subj:15079000 ;
	skos:exactMatch <https://www.wikidata.org/entity/Q933235> ;
	skos:broader	medtop:20000822 .

medtop:20000884
	rdf:type skos:Concept ;
	skos:prefLabel	"mountain climbing"@en-GB ;
	skos:definition	"Moving up mountains using hands and feet"@en-GB ;
	skos:inScheme <http://cv.iptc.org/newscodes/mediatopic/>  ;
	ikos:created "2009-10-22T02:00:00+00:00"^^xsd:dateTime ;
	dct:created "2009-10-22T02:00:00+00:00"^^xsd:dateTime ;
	ikos:modified "2021-02-18T12:00:00+00:00"^^xsd:dateTime ;
	dct:modified "2021-02-18T12:00:00+00:00"^^xsd:dateTime  ;
	skos:exactMatch subj:15016000 ;
	skos:exactMatch <https://www.wikidata.org/entity/Q820236> ;
	skos:broader	medtop:20000822 ;
	skos:narrower	medtop:20000885 ;
	skos:narrower	medtop:20000886 .

medtop:20000885
	rdf:type skos:Concept ;
	skos:prefLabel	"ice climbing"@en-GB ;
	skos:definition	"Climbing of ice features such as icefalls and frozen cliffs"@en-GB ;
	skos:inScheme <http://cv.iptc.org/newscodes/mediatopic/>  ;
	ikos:created "2009-10-22T02:00:00+00:00"^^xsd:dateTime ;
	dct:created "2009-10-22T02:00:00+00:00"^^xsd:dateTime ;
	ikos:modified "2021-02-18T12:00:00+00:00"^^xsd:dateTime ;
	dct:modified "2021-02-18T12:00:00+00:00"^^xsd:dateTime  ;
	skos:broadMatch subj:15016000 ;
	skos:exactMatch <https://www.wikidata.org/entity/Q1148495> ;
	skos:broader	medtop:20000884 .

medtop:20000886
	rdf:type skos:Concept ;
	skos:prefLabel	"mountaineering"@en-GB ;
	skos:definition	"Competitive alpine climbing"@en-GB ;
	skos:inScheme <http://cv.iptc.org/newscodes/mediatopic/>  ;
	ikos:created "2009-10-22T02:00:00+00:00"^^xsd:dateTime ;
	dct:created "2009-10-22T02:00:00+00:00"^^xsd:dateTime ;
	ikos:modified "2023-10-02T12:00:00+00:00"^^xsd:dateTime ;
	dct:modified "2023-10-02T12:00:00+00:00"^^xsd:dateTime  ;
	skos:exactMatch subj:15016001 ;
	skos:exactMatch <https://www.wikidata.org/entity/Q36908> ;
	skos:broader	medtop:20000884 .

medtop:20000887
	rdf:type skos:Concept ;
	skos:prefLabel	"sport climbing"@en-GB ;
	skos:definition	"Sport climbing as a special category: individual competition, on an artificial wall with time measurement"@en-GB ;
	skos:inScheme <http://cv.iptc.org/newscodes/mediatopic/>  ;
	ikos:created "2009-10-22T02:00:00+00:00"^^xsd:dateTime ;
	dct:created "2009-10-22T02:00:00+00:00"^^xsd:dateTime ;
	ikos:modified "2021-07-12T12:00:00+00:00"^^xsd:dateTime ;
	dct:modified "2021-07-12T12:00:00+00:00"^^xsd:dateTime  ;
	skos:exactMatch subj:15016002 ;
	skos:exactMatch <https://www.wikidata.org/entity/Q1541373> ;
	skos:broader	medtop:20000822 .

medtop:20000888
	rdf:type skos:Concept ;
	skos:prefLabel	"cricket"@en-GB ;
	skos:definition	"Ball sport involving two teams of 11 players, balls, bats and wickets. The aim is to score as many runs as possible, and to get the opposing team 'out'. A 'run' involves a player running between two wickets. The opposing team try to get their rivals 'out'"@en-GB ;
	skos:inScheme <http://cv.iptc.org/newscodes/mediatopic/>  ;
	ikos:created "2009-10-22T02:00:00+00:00"^^xsd:dateTime ;
	dct:created "2009-10-22T02:00:00+00:00"^^xsd:dateTime ;
	ikos:modified "2021-02-18T12:00:00+00:00"^^xsd:dateTime ;
	dct:modified "2021-02-18T12:00:00+00:00"^^xsd:dateTime  ;
	skos:exactMatch subj:15017000 ;
	skos:exactMatch <https://www.wikidata.org/entity/Q5375> ;
	skos:broader	medtop:20000822 .

medtop:20000889
	rdf:type skos:Concept ;
	skos:prefLabel	"croquet"@en-GB ;
	skos:definition	"Using mallets to hit a ball through hoops"@en-GB ;
	skos:inScheme <http://cv.iptc.org/newscodes/mediatopic/>  ;
	ikos:created "2009-10-22T02:00:00+00:00"^^xsd:dateTime ;
	dct:created "2009-10-22T02:00:00+00:00"^^xsd:dateTime ;
	ikos:modified "2021-02-18T12:00:00+00:00"^^xsd:dateTime ;
	dct:modified "2021-02-18T12:00:00+00:00"^^xsd:dateTime  ;
	skos:exactMatch subj:15081000 ;
	skos:exactMatch <https://www.wikidata.org/entity/Q193387> ;
	skos:broader	medtop:20000822 .

medtop:20000890
	rdf:type skos:Concept ;
	skos:prefLabel	"curling"@en-GB ;
	skos:definition	"A game played on ice with large flat round stones. A player throws the stone, aiming at a target. Teammates of the player who has thrown the stone can sweep the ice in front of the stone to help smooth its path towards the target."@en-GB ;
	skos:inScheme <http://cv.iptc.org/newscodes/mediatopic/>  ;
	ikos:created "2009-10-22T02:00:00+00:00"^^xsd:dateTime ;
	dct:created "2009-10-22T02:00:00+00:00"^^xsd:dateTime ;
	ikos:modified "2021-02-18T12:00:00+00:00"^^xsd:dateTime ;
	dct:modified "2021-02-18T12:00:00+00:00"^^xsd:dateTime  ;
	skos:exactMatch subj:15018000 ;
	skos:exactMatch <https://www.wikidata.org/entity/Q136851> ;
	skos:broader	medtop:20000822 ;
	skos:narrower	medtop:20000891 .

medtop:20000891
	rdf:type skos:Concept ;
	skos:prefLabel	"icestock sport"@en-GB ;
	skos:definition	"Similar to curling, played on targets on ice, different stones with straight handle and different rules, played in alpine countries"@en-GB ;
	skos:inScheme <http://cv.iptc.org/newscodes/mediatopic/>  ;
	ikos:created "2009-10-22T02:00:00+00:00"^^xsd:dateTime ;
	dct:created "2009-10-22T02:00:00+00:00"^^xsd:dateTime ;
	ikos:modified "2021-02-18T12:00:00+00:00"^^xsd:dateTime ;
	dct:modified "2021-02-18T12:00:00+00:00"^^xsd:dateTime  ;
	skos:exactMatch subj:15018001 ;
	skos:exactMatch <https://www.wikidata.org/entity/Q1070325> ;
	skos:broader	medtop:20000890 .

medtop:20000892
	rdf:type skos:Concept ;
	skos:prefLabel	"cycling"@en-GB ;
	skos:definition	"A race over a given distance on bicycles."@en-GB ;
	skos:inScheme <http://cv.iptc.org/newscodes/mediatopic/>  ;
	ikos:created "2009-10-22T02:00:00+00:00"^^xsd:dateTime ;
	dct:created "2009-10-22T02:00:00+00:00"^^xsd:dateTime ;
	ikos:modified "2021-02-18T12:00:00+00:00"^^xsd:dateTime ;
	dct:modified "2021-02-18T12:00:00+00:00"^^xsd:dateTime  ;
	ikos:hasFacet aspfacet:cyclingtype ;
	skos:exactMatch subj:15019000 ;
	skos:exactMatch <https://www.wikidata.org/entity/Q2215841> ;
	skos:broader	medtop:20000822 ;
	skos:narrower	medtop:20000893 ;
	skos:narrower	medtop:20000894 ;
	skos:narrower	medtop:20000895 ;
	skos:narrower	medtop:20000896 ;
	skos:narrower	medtop:20000897 ;
	skos:narrower	medtop:20000898 ;
	skos:narrower	medtop:20000899 ;
	skos:narrower	medtop:20000900 ;
	skos:narrower	medtop:20000901 ;
	skos:narrower	medtop:20000902 ;
	skos:narrower	medtop:20000903 ;
	skos:narrower	medtop:20000904 ;
	skos:narrower	medtop:20000905 ;
	skos:narrower	medtop:20000906 ;
	skos:narrower	medtop:20000907 ;
	skos:narrower	medtop:20000908 ;
	skos:narrower	medtop:20000909 ;
	skos:narrower	medtop:20000910 .

medtop:20000893
	rdf:type skos:Concept ;
	skos:prefLabel	"artistic cycling"@en-GB ;
	skos:definition	"Individual or teams on one or two bicycles in an arena. Points are awarded by a jury."@en-GB ;
	skos:inScheme <http://cv.iptc.org/newscodes/mediatopic/>  ;
	ikos:created "2009-10-22T02:00:00+00:00"^^xsd:dateTime ;
	dct:created "2009-10-22T02:00:00+00:00"^^xsd:dateTime ;
	ikos:modified "2021-02-18T12:00:00+00:00"^^xsd:dateTime ;
	dct:modified "2021-02-18T12:00:00+00:00"^^xsd:dateTime  ;
	skos:exactMatch subj:15019020 ;
	skos:exactMatch <https://www.wikidata.org/entity/Q1792605> ;
	skos:broader	medtop:20000892 .

medtop:20000894
	rdf:type skos:Concept ;
	skos:prefLabel	"bi-crossing"@en-GB ;
	skos:definition	"A race where competitors have to cover a circuit with obstacles as quickly as possible."@en-GB ;
	skos:note	"Retired. Use Media Topic cycling + sports facet cyclingtype"@en-GB ;
	skos:inScheme <http://cv.iptc.org/newscodes/mediatopic/>  ;
	ikos:created "2009-10-22T02:00:00+00:00"^^xsd:dateTime ;
	dct:created "2009-10-22T02:00:00+00:00"^^xsd:dateTime ;
	ikos:modified "2021-02-18T12:00:00+00:00"^^xsd:dateTime ;
	dct:modified "2021-02-18T12:00:00+00:00"^^xsd:dateTime  ; 
	ikos:retired "2017-07-04T12:00:00+00:00"^^xsd:dateTime ;
	skos:exactMatch subj:15019018 ;
	skos:exactMatch <https://www.wikidata.org/entity/Q215184> ;
	skos:broader	medtop:20000892 .

medtop:20000895
	rdf:type skos:Concept ;
	skos:prefLabel	"bmx racing"@en-GB ;
	skos:definition	"Bicycle racing in with inline start and various obstacles over off-road circuits."@en-GB ;
	skos:inScheme <http://cv.iptc.org/newscodes/mediatopic/>  ;
	ikos:created "2009-10-22T02:00:00+00:00"^^xsd:dateTime ;
	dct:created "2009-10-22T02:00:00+00:00"^^xsd:dateTime ;
	ikos:modified "2021-07-12T12:00:00+00:00"^^xsd:dateTime ;
	dct:modified "2021-07-12T12:00:00+00:00"^^xsd:dateTime  ;
	ikos:hasFacet aspfacet:bmxfreestyletype ;
	skos:broadMatch subj:15019000 ;
	skos:exactMatch <https://www.wikidata.org/entity/Q215184> ;
	skos:broader	medtop:20000892 .

medtop:20000896
	rdf:type skos:Concept ;
	skos:prefLabel	"cycle ball"@en-GB ;
	skos:definition	"Competitive team sport using bicycles. One team against another with two persons per team. The aim is for competitors to move the ball using the front and rear wheels without letting their feet touch the ground."@en-GB ;
	skos:inScheme <http://cv.iptc.org/newscodes/mediatopic/>  ;
	ikos:created "2009-10-22T02:00:00+00:00"^^xsd:dateTime ;
	dct:created "2009-10-22T02:00:00+00:00"^^xsd:dateTime ;
	ikos:modified "2021-02-18T12:00:00+00:00"^^xsd:dateTime ;
	dct:modified "2021-02-18T12:00:00+00:00"^^xsd:dateTime  ;
	skos:exactMatch subj:15019021 ;
	skos:exactMatch <https://www.wikidata.org/entity/Q8099087> ;
	skos:broader	medtop:20000892 .

medtop:20000897
	rdf:type skos:Concept ;
	skos:prefLabel	"cycle sprint race"@en-GB ;
	skos:definition	"Track cycling race between two cyclists over two or three laps, with a timed sprint finish over the last 200m"@en-GB ;
	skos:note	"Retired. Use Media Topic cycling + sports facet racetype"@en-GB ;
	skos:inScheme <http://cv.iptc.org/newscodes/mediatopic/>  ;
	ikos:created "2009-10-22T02:00:00+00:00"^^xsd:dateTime ;
	dct:created "2009-10-22T02:00:00+00:00"^^xsd:dateTime ;
	ikos:modified "2021-02-18T12:00:00+00:00"^^xsd:dateTime ;
	dct:modified "2021-02-18T12:00:00+00:00"^^xsd:dateTime  ; 
	ikos:retired "2017-07-04T12:00:00+00:00"^^xsd:dateTime ;
	skos:exactMatch subj:15019004 ;
	skos:exactMatch <https://www.wikidata.org/entity/Q352749> ;
	skos:broader	medtop:20000892 .

medtop:20000898
	rdf:type skos:Concept ;
	skos:prefLabel	"cyclo-cross"@en-GB ;
	skos:definition	"Staged on various surfaces - earth, grass, sand or tarmac."@en-GB ;
	skos:note	"Retired. Use Media Topic cycling + sports facet cyclingtype"@en-GB ;
	skos:inScheme <http://cv.iptc.org/newscodes/mediatopic/>  ;
	ikos:created "2009-10-22T02:00:00+00:00"^^xsd:dateTime ;
	dct:created "2009-10-22T02:00:00+00:00"^^xsd:dateTime ;
	ikos:modified "2021-02-18T12:00:00+00:00"^^xsd:dateTime ;
	dct:modified "2021-02-18T12:00:00+00:00"^^xsd:dateTime  ; 
	ikos:retired "2017-07-04T12:00:00+00:00"^^xsd:dateTime ;
	skos:exactMatch subj:15019014 ;
	skos:exactMatch <https://www.wikidata.org/entity/Q335638> ;
	skos:broader	medtop:20000892 .

medtop:20000899
	rdf:type skos:Concept ;
	skos:prefLabel	"individual pursuit (cycling)"@en-GB ;
	skos:definition	"Track cycling event where two cyclists set off from midway down opposite straights and try to make up the gap between them"@en-GB ;
	skos:note	"Retired. Use Media Topic cycling +sports facets racetype + teamsize"@en-GB ;
	skos:inScheme <http://cv.iptc.org/newscodes/mediatopic/>  ;
	ikos:created "2009-10-22T02:00:00+00:00"^^xsd:dateTime ;
	dct:created "2009-10-22T02:00:00+00:00"^^xsd:dateTime ;
	ikos:modified "2021-02-18T12:00:00+00:00"^^xsd:dateTime ;
	dct:modified "2021-02-18T12:00:00+00:00"^^xsd:dateTime  ; 
	ikos:retired "2017-07-04T12:00:00+00:00"^^xsd:dateTime ;
	skos:exactMatch subj:15019002 ;
	skos:exactMatch <https://www.wikidata.org/entity/Q1307101> ;
	skos:broader	medtop:20000892 .

medtop:20000900
	rdf:type skos:Concept ;
	skos:prefLabel	"individual time trial (cycling)"@en-GB ;
	skos:definition	"A race or stage against the clock with each cyclist setting off individually"@en-GB ;
	skos:note	"Retired. Use Media Topic cycling + sports facets racetype + teamsize"@en-GB ;
	skos:inScheme <http://cv.iptc.org/newscodes/mediatopic/>  ;
	ikos:created "2009-10-22T02:00:00+00:00"^^xsd:dateTime ;
	dct:created "2009-10-22T02:00:00+00:00"^^xsd:dateTime ;
	ikos:modified "2021-02-18T12:00:00+00:00"^^xsd:dateTime ;
	dct:modified "2021-02-18T12:00:00+00:00"^^xsd:dateTime  ; 
	ikos:retired "2017-07-04T12:00:00+00:00"^^xsd:dateTime ;
	skos:exactMatch subj:15019012 ;
	skos:exactMatch <https://www.wikidata.org/entity/Q2266066> ;
	skos:broader	medtop:20000892 .

medtop:20000901
	rdf:type skos:Concept ;
	skos:prefLabel	"Keirin"@en-GB ;
	skos:definition	"Sprint between six cyclists where a pacemaker on a moped gradually increases the pace over the first 1400m. When the pacemaker leaves the track the race develops into a sprint finish over the final 6-700m."@en-GB ;
	skos:note	"Retired. Use Media Topic cycling + sports facet cyclingtype"@en-GB ;
	skos:inScheme <http://cv.iptc.org/newscodes/mediatopic/>  ;
	ikos:created "2009-10-22T02:00:00+00:00"^^xsd:dateTime ;
	dct:created "2009-10-22T02:00:00+00:00"^^xsd:dateTime ;
	ikos:modified "2021-02-18T12:00:00+00:00"^^xsd:dateTime ;
	dct:modified "2021-02-18T12:00:00+00:00"^^xsd:dateTime  ; 
	ikos:retired "2017-07-04T12:00:00+00:00"^^xsd:dateTime ;
	skos:exactMatch subj:15019005 ;
	skos:exactMatch <https://www.wikidata.org/entity/Q774176> ;
	skos:broader	medtop:20000892 .

medtop:20000902
	rdf:type skos:Concept ;
	skos:prefLabel	"Madison race"@en-GB ;
	skos:definition	"A points race by teams comprising two cyclists in relay-format"@en-GB ;
	skos:note	"Retired. Use Media Topic cycling + sports facet cyclingtype"@en-GB ;
	skos:inScheme <http://cv.iptc.org/newscodes/mediatopic/>  ;
	ikos:created "2009-10-22T02:00:00+00:00"^^xsd:dateTime ;
	dct:created "2009-10-22T02:00:00+00:00"^^xsd:dateTime ;
	ikos:modified "2021-02-18T12:00:00+00:00"^^xsd:dateTime ;
	dct:modified "2021-02-18T12:00:00+00:00"^^xsd:dateTime  ; 
	ikos:retired "2017-07-04T12:00:00+00:00"^^xsd:dateTime ;
	skos:exactMatch subj:15019007 ;
	skos:exactMatch <https://www.wikidata.org/entity/Q2596614> ;
	skos:broader	medtop:20000892 .

medtop:20000903
	rdf:type skos:Concept ;
	skos:prefLabel	"mountain biking"@en-GB ;
	skos:definition	"All-terrain, off-road bicycle riding requiring endurance and specially adapted mountain bikes"@en-GB ;
	skos:inScheme <http://cv.iptc.org/newscodes/mediatopic/>  ;
	ikos:created "2009-10-22T02:00:00+00:00"^^xsd:dateTime ;
	dct:created "2009-10-22T02:00:00+00:00"^^xsd:dateTime ;
	ikos:modified "2021-02-18T12:00:00+00:00"^^xsd:dateTime ;
	dct:modified "2021-02-18T12:00:00+00:00"^^xsd:dateTime  ;
	ikos:hasFacet aspfacet:mountainbikingtype ;
	skos:broadMatch subj:15019015 ;
	skos:exactMatch <https://www.wikidata.org/entity/Q520611> ;
	skos:broader	medtop:20000892 .

medtop:20000904
	rdf:type skos:Concept ;
	skos:prefLabel	"points race (cycling)"@en-GB ;
	skos:definition	"Cyclists aim to complete the highest number of laps. Bonus points are picked up in intermediate sprints held every 2500m"@en-GB ;
	skos:note	"Retired. Use Media Topic cycling + sports facet cyclingtype"@en-GB ;
	skos:inScheme <http://cv.iptc.org/newscodes/mediatopic/>  ;
	ikos:created "2009-10-22T02:00:00+00:00"^^xsd:dateTime ;
	dct:created "2009-10-22T02:00:00+00:00"^^xsd:dateTime ;
	ikos:modified "2021-02-18T12:00:00+00:00"^^xsd:dateTime ;
	dct:modified "2021-02-18T12:00:00+00:00"^^xsd:dateTime  ; 
	ikos:retired "2017-07-04T12:00:00+00:00"^^xsd:dateTime ;
	skos:exactMatch subj:15019006 ;
	skos:exactMatch <https://www.wikidata.org/entity/Q2597988> ;
	skos:broader	medtop:20000892 .

medtop:20000905
	rdf:type skos:Concept ;
	skos:prefLabel	"road cycling"@en-GB ;
	skos:definition	"Road race with all the competitor starting en masse."@en-GB ;
	skos:note	"Retired. Use Media Topic cycling + sports facet cyclingtype"@en-GB ;
	skos:inScheme <http://cv.iptc.org/newscodes/mediatopic/>  ;
	ikos:created "2009-10-22T02:00:00+00:00"^^xsd:dateTime ;
	dct:created "2009-10-22T02:00:00+00:00"^^xsd:dateTime ;
	ikos:modified "2021-02-18T12:00:00+00:00"^^xsd:dateTime ;
	dct:modified "2021-02-18T12:00:00+00:00"^^xsd:dateTime  ; 
	ikos:retired "2017-07-04T12:00:00+00:00"^^xsd:dateTime ;
	skos:exactMatch subj:15019011 ;
	skos:exactMatch <https://www.wikidata.org/entity/Q3609> ;
	skos:broader	medtop:20000892 .

medtop:20000906
	rdf:type skos:Concept ;
	skos:prefLabel	"cycling staging race"@en-GB ;
	skos:definition	"Race disputed by teams with the classifications determined by the combined times over a day"@en-GB ;
	skos:note	"Retired. Use Media Topic cycling + sports facet racetype"@en-GB ;
	skos:inScheme <http://cv.iptc.org/newscodes/mediatopic/>  ;
	ikos:created "2009-10-22T02:00:00+00:00"^^xsd:dateTime ;
	dct:created "2009-10-22T02:00:00+00:00"^^xsd:dateTime ;
	ikos:modified "2021-05-05T12:00:00+00:00"^^xsd:dateTime ;
	dct:modified "2021-05-05T12:00:00+00:00"^^xsd:dateTime  ; 
	ikos:retired "2017-07-04T12:00:00+00:00"^^xsd:dateTime ;
	skos:exactMatch subj:15019013 ;
	skos:exactMatch <https://www.wikidata.org/entity/Q1318941> ;
	skos:broader	medtop:20000892 .

medtop:20000907
	rdf:type skos:Concept ;
	skos:prefLabel	"team cycle sprint"@en-GB ;
	skos:definition	"A track race where two teams race against each other, starting on opposite sides of the track, following the first lap the first rider pulls away, leaving the second rider to lead the next lap, who then does the same at the last lap, leaving the third rider to finish the race. The team with the fastest time is the winner."@en-GB ;
	skos:note	"Retired. Use Media Topic cycling + sports facet cyclingtype"@en-GB ;
	skos:inScheme <http://cv.iptc.org/newscodes/mediatopic/>  ;
	ikos:created "2009-10-22T02:00:00+00:00"^^xsd:dateTime ;
	dct:created "2009-10-22T02:00:00+00:00"^^xsd:dateTime ;
	ikos:modified "2021-02-18T12:00:00+00:00"^^xsd:dateTime ;
	dct:modified "2021-02-18T12:00:00+00:00"^^xsd:dateTime  ; 
	ikos:retired "2017-07-04T12:00:00+00:00"^^xsd:dateTime ;
	skos:broadMatch subj:15019000 ;
	skos:exactMatch <https://www.wikidata.org/entity/Q1817141> ;
	skos:broader	medtop:20000892 .

medtop:20000908
	rdf:type skos:Concept ;
	skos:prefLabel	"road cycling team pursuit"@en-GB ;
	skos:definition	"Track cycle event where two teams set off from midway down opposite straights and try to make up the gap between them"@en-GB ;
	skos:note	"Retired. Use Media Topic cycling + sports facets racetype + teamsize."@en-GB ;
	skos:inScheme <http://cv.iptc.org/newscodes/mediatopic/>  ;
	ikos:created "2009-10-22T02:00:00+00:00"^^xsd:dateTime ;
	dct:created "2009-10-22T02:00:00+00:00"^^xsd:dateTime ;
	ikos:modified "2021-02-18T12:00:00+00:00"^^xsd:dateTime ;
	dct:modified "2021-02-18T12:00:00+00:00"^^xsd:dateTime  ; 
	ikos:retired "2017-07-04T12:00:00+00:00"^^xsd:dateTime ;
	skos:broadMatch subj:15019000 ;
	skos:exactMatch <https://www.wikidata.org/entity/Q1820070> ;
	skos:broader	medtop:20000892 .

medtop:20000909
	rdf:type skos:Concept ;
	skos:prefLabel	"team time trial (cycling)"@en-GB ;
	skos:definition	"Teams of cyclists race against the clock"@en-GB ;
	skos:note	"Retired. Use Media Topic cycling + sports facets racetype + teamsize."@en-GB ;
	skos:inScheme <http://cv.iptc.org/newscodes/mediatopic/>  ;
	ikos:created "2009-10-22T02:00:00+00:00"^^xsd:dateTime ;
	dct:created "2009-10-22T02:00:00+00:00"^^xsd:dateTime ;
	ikos:modified "2021-02-18T12:00:00+00:00"^^xsd:dateTime ;
	dct:modified "2021-02-18T12:00:00+00:00"^^xsd:dateTime  ; 
	ikos:retired "2017-07-04T12:00:00+00:00"^^xsd:dateTime ;
	skos:broadMatch subj:15019000 ;
	skos:exactMatch <https://www.wikidata.org/entity/Q2348250> ;
	skos:broader	medtop:20000892 .

medtop:20000910
	rdf:type skos:Concept ;
	skos:prefLabel	"track race (cycling)"@en-GB ;
	skos:definition	"A race staged on a track in a velodrome"@en-GB ;
	skos:note	"Retired. Use Media Topic cycling + sports facet cyclingtype"@en-GB ;
	skos:inScheme <http://cv.iptc.org/newscodes/mediatopic/>  ;
	ikos:created "2009-10-22T02:00:00+00:00"^^xsd:dateTime ;
	dct:created "2009-10-22T02:00:00+00:00"^^xsd:dateTime ;
	ikos:modified "2021-02-18T12:00:00+00:00"^^xsd:dateTime ;
	dct:modified "2021-02-18T12:00:00+00:00"^^xsd:dateTime  ; 
	ikos:retired "2017-07-04T12:00:00+00:00"^^xsd:dateTime ;
	skos:exactMatch subj:15019001 ;
	skos:exactMatch <https://www.wikidata.org/entity/Q221635> ;
	skos:broader	medtop:20000892 .

medtop:20000911
	rdf:type skos:Concept ;
	skos:prefLabel	"competitive dancing"@en-GB ;
	skos:definition	"Dancing competition where couples are judged on technique and interpretation."@en-GB ;
	skos:inScheme <http://cv.iptc.org/newscodes/mediatopic/>  ;
	ikos:created "2009-10-22T02:00:00+00:00"^^xsd:dateTime ;
	dct:created "2009-10-22T02:00:00+00:00"^^xsd:dateTime ;
	ikos:modified "2021-02-18T12:00:00+00:00"^^xsd:dateTime ;
	dct:modified "2021-02-18T12:00:00+00:00"^^xsd:dateTime  ;
	skos:exactMatch subj:15020000 ;
	skos:exactMatch <https://www.wikidata.org/entity/Q1415387> ;
	skos:broader	medtop:20000822 .

medtop:20000912
	rdf:type skos:Concept ;
	skos:prefLabel	"darts"@en-GB ;
	skos:definition	"The sport in which small darts are thrown at a dartboard, a circular target divided into numbered sections."@en-GB ;
	skos:inScheme <http://cv.iptc.org/newscodes/mediatopic/>  ;
	ikos:created "2009-10-22T02:00:00+00:00"^^xsd:dateTime ;
	dct:created "2009-10-22T02:00:00+00:00"^^xsd:dateTime ;
	ikos:modified "2021-02-18T12:00:00+00:00"^^xsd:dateTime ;
	dct:modified "2021-02-18T12:00:00+00:00"^^xsd:dateTime  ;
	skos:exactMatch subj:15100000 ;
	skos:exactMatch <https://www.wikidata.org/entity/Q131471> ;
	skos:broader	medtop:20000822 .

medtop:20000913
	rdf:type skos:Concept ;
	skos:prefLabel	"diving"@en-GB ;
	skos:definition	"Competitors dive off a fixed or spring board and are assessed by seven judges giving marks up to ten for their acrobatic moves."@en-GB ;
	skos:inScheme <http://cv.iptc.org/newscodes/mediatopic/>  ;
	ikos:created "2009-10-22T02:00:00+00:00"^^xsd:dateTime ;
	dct:created "2009-10-22T02:00:00+00:00"^^xsd:dateTime ;
	ikos:modified "2021-02-18T12:00:00+00:00"^^xsd:dateTime ;
	dct:modified "2021-02-18T12:00:00+00:00"^^xsd:dateTime  ;
	skos:exactMatch subj:15021000 ;
	skos:exactMatch <https://www.wikidata.org/entity/Q7735> ;
	skos:broader	medtop:20000822 ;
	skos:narrower	medtop:20000914 ;
	skos:narrower	medtop:20000915 ;
	skos:narrower	medtop:20000916 .

medtop:20000914
	rdf:type skos:Concept ;
	skos:prefLabel	"platform diving"@en-GB ;
	skos:definition	"Divers take off from a high platform"@en-GB ;
	skos:inScheme <http://cv.iptc.org/newscodes/mediatopic/>  ;
	ikos:created "2009-10-22T02:00:00+00:00"^^xsd:dateTime ;
	dct:created "2009-10-22T02:00:00+00:00"^^xsd:dateTime ;
	ikos:modified "2021-02-18T12:00:00+00:00"^^xsd:dateTime ;
	dct:modified "2021-02-18T12:00:00+00:00"^^xsd:dateTime  ;
	ikos:hasFacet aspfacet:platformheight ;
	skos:broadMatch subj:15021000 ;
	skos:exactMatch <https://www.wikidata.org/entity/Q16014286> ;
	skos:broader	medtop:20000913 .

medtop:20000915
	rdf:type skos:Concept ;
	skos:prefLabel	"springboard diving"@en-GB ;
	skos:definition	"Divers dive from a high springboard."@en-GB ;
	skos:inScheme <http://cv.iptc.org/newscodes/mediatopic/>  ;
	ikos:created "2009-10-22T02:00:00+00:00"^^xsd:dateTime ;
	dct:created "2009-10-22T02:00:00+00:00"^^xsd:dateTime ;
	ikos:modified "2021-02-18T12:00:00+00:00"^^xsd:dateTime ;
	dct:modified "2021-02-18T12:00:00+00:00"^^xsd:dateTime  ;
	ikos:hasFacet aspfacet:platformheight ;
	skos:broadMatch subj:15021000 ;
	skos:exactMatch <https://www.wikidata.org/entity/Q16014295> ;
	skos:broader	medtop:20000913 .

medtop:20000916
	rdf:type skos:Concept ;
	skos:prefLabel	"synchronised diving"@en-GB ;
	skos:definition	"Two competitors from the same team dive off at the same time from separate platforms or springboards. As well as being judged on the standard criteria they are also awarded marks for synchronisation."@en-GB ;
	skos:inScheme <http://cv.iptc.org/newscodes/mediatopic/>  ;
	ikos:created "2009-10-22T02:00:00+00:00"^^xsd:dateTime ;
	dct:created "2009-10-22T02:00:00+00:00"^^xsd:dateTime ;
	ikos:modified "2021-02-18T12:00:00+00:00"^^xsd:dateTime ;
	dct:modified "2021-02-18T12:00:00+00:00"^^xsd:dateTime  ;
	skos:broadMatch subj:15021004 ;
	ikos:hasFacet aspfacet:platformheight ;
	skos:exactMatch <https://www.wikidata.org/entity/Q638269> ;
	skos:broader	medtop:20000913 .

medtop:20000917
	rdf:type skos:Concept ;
	skos:prefLabel	"scuba diving"@en-GB ;
	skos:definition	"Underwater diving with the use of a self-contained underwater breathing apparatus"@en-GB ;
	skos:inScheme <http://cv.iptc.org/newscodes/mediatopic/>  ;
	ikos:created "2009-10-22T02:00:00+00:00"^^xsd:dateTime ;
	dct:created "2009-10-22T02:00:00+00:00"^^xsd:dateTime ;
	ikos:modified "2021-02-18T12:00:00+00:00"^^xsd:dateTime ;
	dct:modified "2021-02-18T12:00:00+00:00"^^xsd:dateTime  ;
	skos:exactMatch subj:15021006 ;
	skos:exactMatch <https://www.wikidata.org/entity/Q1096878> ;
	skos:broader	medtop:20000560 .

medtop:20000918
	rdf:type skos:Concept ;
	skos:prefLabel	"underwater sports"@en-GB ;
	skos:definition	"Competitive sports played under water"@en-GB ;
	skos:inScheme <http://cv.iptc.org/newscodes/mediatopic/>  ;
	ikos:created "2009-10-22T02:00:00+00:00"^^xsd:dateTime ;
	dct:created "2009-10-22T02:00:00+00:00"^^xsd:dateTime ;
	ikos:modified "2021-02-18T12:00:00+00:00"^^xsd:dateTime ;
	dct:modified "2021-02-18T12:00:00+00:00"^^xsd:dateTime  ;
	skos:exactMatch subj:15021005 ;
	skos:exactMatch <https://www.wikidata.org/entity/Q2369170> ;
	skos:broader	medtop:20000822 .

medtop:20000919
	rdf:type skos:Concept ;
	skos:prefLabel	"dog racing"@en-GB ;
	skos:definition	"Dogs racing around a track"@en-GB ;
	skos:inScheme <http://cv.iptc.org/newscodes/mediatopic/>  ;
	ikos:created "2009-10-22T02:00:00+00:00"^^xsd:dateTime ;
	dct:created "2009-10-22T02:00:00+00:00"^^xsd:dateTime ;
	ikos:modified "2021-02-18T12:00:00+00:00"^^xsd:dateTime ;
	dct:modified "2021-02-18T12:00:00+00:00"^^xsd:dateTime  ;
	skos:exactMatch subj:15082000 ;
	ikos:hasFacet aspfacet:dogracingtype ;
	skos:exactMatch <https://www.wikidata.org/entity/Q57833661> ;
	skos:broader	medtop:20000822 ;
	skos:narrower	medtop:20000920 ;
	skos:narrower	medtop:20000921 .

medtop:20000920
	rdf:type skos:Concept ;
	skos:prefLabel	"oval track dog racing"@en-GB ;
	skos:definition	"Pursuing an artificial rabbit around an oval track"@en-GB ;
	skos:note	"Retired. Use Media Topic dog racing+ sports facet dogracingtype"@en-GB ;
	skos:inScheme <http://cv.iptc.org/newscodes/mediatopic/>  ;
	ikos:created "2009-10-22T02:00:00+00:00"^^xsd:dateTime ;
	dct:created "2009-10-22T02:00:00+00:00"^^xsd:dateTime ;
	ikos:modified "2021-02-18T12:00:00+00:00"^^xsd:dateTime ;
	dct:modified "2021-02-18T12:00:00+00:00"^^xsd:dateTime  ; 
	ikos:retired "2017-07-04T12:00:00+00:00"^^xsd:dateTime ;
	skos:exactMatch subj:15082002 ;
	skos:exactMatch <https://www.wikidata.org/entity/Q1345388> ;
	skos:broader	medtop:20000919 .

medtop:20000921
	rdf:type skos:Concept ;
	skos:prefLabel	"dog sled racing"@en-GB ;
	skos:definition	"Race with dogs harnessed to a sled"@en-GB ;
	skos:note	"Retired. Use Media Topic dog racing+ sports facet dogracingtype"@en-GB ;
	skos:inScheme <http://cv.iptc.org/newscodes/mediatopic/>  ;
	ikos:created "2009-10-22T02:00:00+00:00"^^xsd:dateTime ;
	dct:created "2009-10-22T02:00:00+00:00"^^xsd:dateTime ;
	ikos:modified "2021-02-18T12:00:00+00:00"^^xsd:dateTime ;
	dct:modified "2021-02-18T12:00:00+00:00"^^xsd:dateTime  ; 
	ikos:retired "2017-07-04T12:00:00+00:00"^^xsd:dateTime ;
	skos:exactMatch subj:15082001 ;
	skos:exactMatch <https://www.wikidata.org/entity/Q1968664> ;
	skos:broader	medtop:20000919 .

medtop:20000922
	rdf:type skos:Concept ;
	skos:prefLabel	"duathlon"@en-GB ;
	skos:definition	"An athletic event involving running and cycling"@en-GB ;
	skos:inScheme <http://cv.iptc.org/newscodes/mediatopic/>  ;
	ikos:created "2009-10-22T02:00:00+00:00"^^xsd:dateTime ;
	dct:created "2009-10-22T02:00:00+00:00"^^xsd:dateTime ;
	ikos:modified "2021-02-18T12:00:00+00:00"^^xsd:dateTime ;
	dct:modified "2021-02-18T12:00:00+00:00"^^xsd:dateTime  ;
	skos:exactMatch subj:15086000 ;
	skos:exactMatch <https://www.wikidata.org/entity/Q429006> ;
	skos:broader	medtop:20000822 .

medtop:20000923
	rdf:type skos:Concept ;
	skos:prefLabel	"equestrian"@en-GB ;
	skos:definition	"Horse-based sport disciplines governed by the International Federation for Equestrian Sports, such as dressage, eventing, show jumping and vaulting"@en-GB ;
	skos:inScheme <http://cv.iptc.org/newscodes/mediatopic/>  ;
	ikos:created "2009-10-22T02:00:00+00:00"^^xsd:dateTime ;
	dct:created "2009-10-22T02:00:00+00:00"^^xsd:dateTime ;
	ikos:modified "2021-07-12T12:00:00+00:00"^^xsd:dateTime ;
	dct:modified "2021-07-12T12:00:00+00:00"^^xsd:dateTime  ;
	ikos:hasFacet aspfacet:equestriantype ;
	skos:exactMatch subj:15022000 ;
	skos:exactMatch <https://www.wikidata.org/entity/Q902378> ;
	skos:broader	medtop:20000822 ;
	skos:narrower	medtop:20000924 ;
	skos:narrower	medtop:20000925 ;
	skos:narrower	medtop:20000926 ;
	skos:narrower	medtop:20000927 ;
	skos:narrower	medtop:20000928 .

medtop:20000924
	rdf:type skos:Concept ;
	skos:prefLabel	"cross-country horse riding"@en-GB ;
	skos:definition	"Equestrian event held on a designated circuit in the countryside featuring artificial and natural obstacles."@en-GB ;
	skos:note	"Retired. Use Media Topic equestrianism + sports facet equestriantype."@en-GB ;
	skos:inScheme <http://cv.iptc.org/newscodes/mediatopic/>  ;
	ikos:created "2009-10-22T02:00:00+00:00"^^xsd:dateTime ;
	dct:created "2009-10-22T02:00:00+00:00"^^xsd:dateTime ;
	ikos:modified "2021-05-05T12:00:00+00:00"^^xsd:dateTime ;
	dct:modified "2021-05-05T12:00:00+00:00"^^xsd:dateTime  ; 
	ikos:retired "2017-07-04T12:00:00+00:00"^^xsd:dateTime ;
	skos:exactMatch subj:15022004 ;
	skos:exactMatch <https://www.wikidata.org/entity/Q838781> ;
	skos:broader	medtop:20000923 .

medtop:20000925
	rdf:type skos:Concept ;
	skos:prefLabel	"dressage"@en-GB ;
	skos:definition	"A rider is judged on a series of moves at three different paces - walk, trot and gallop."@en-GB ;
	skos:note	"Retired. Use Media Topic equestrianism + sports facet equestriantype."@en-GB ;
	skos:inScheme <http://cv.iptc.org/newscodes/mediatopic/>  ;
	ikos:created "2009-10-22T02:00:00+00:00"^^xsd:dateTime ;
	dct:created "2009-10-22T02:00:00+00:00"^^xsd:dateTime ;
	ikos:modified "2021-02-18T12:00:00+00:00"^^xsd:dateTime ;
	dct:modified "2021-02-18T12:00:00+00:00"^^xsd:dateTime  ; 
	ikos:retired "2017-07-04T12:00:00+00:00"^^xsd:dateTime ;
	skos:exactMatch subj:15022002 ;
	skos:exactMatch <https://www.wikidata.org/entity/Q216033> ;
	skos:broader	medtop:20000923 .

medtop:20000926
	rdf:type skos:Concept ;
	skos:prefLabel	"horse jumping"@en-GB ;
	skos:definition	"A rider and horse attempt to jump a series of obstacles in an enclosed arena against the clock."@en-GB ;
	skos:note	"Retired. Use Media Topic equestrianism + sports facet equestriantype."@en-GB ;
	skos:inScheme <http://cv.iptc.org/newscodes/mediatopic/>  ;
	ikos:created "2009-10-22T02:00:00+00:00"^^xsd:dateTime ;
	dct:created "2009-10-22T02:00:00+00:00"^^xsd:dateTime ;
	ikos:modified "2021-02-18T12:00:00+00:00"^^xsd:dateTime ;
	dct:modified "2021-02-18T12:00:00+00:00"^^xsd:dateTime  ; 
	ikos:retired "2017-07-04T12:00:00+00:00"^^xsd:dateTime ;
	skos:exactMatch subj:15022003 ;
	skos:exactMatch <https://www.wikidata.org/entity/Q211773> ;
	skos:broader	medtop:20000923 .

medtop:20000927
	rdf:type skos:Concept ;
	skos:prefLabel	"three day eventing"@en-GB ;
	skos:definition	"Equestrian event involving three disciplines - Dressage, cross-country and show jumping"@en-GB ;
	skos:note	"Retired. Use Media Topic equestrianism + sports facet equestriantype."@en-GB ;
	skos:inScheme <http://cv.iptc.org/newscodes/mediatopic/>  ;
	ikos:created "2009-10-22T02:00:00+00:00"^^xsd:dateTime ;
	dct:created "2009-10-22T02:00:00+00:00"^^xsd:dateTime ;
	ikos:modified "2021-02-18T12:00:00+00:00"^^xsd:dateTime ;
	dct:modified "2021-02-18T12:00:00+00:00"^^xsd:dateTime  ; 
	ikos:retired "2017-07-04T12:00:00+00:00"^^xsd:dateTime ;
	skos:exactMatch subj:15022001 ;
	skos:exactMatch <https://www.wikidata.org/entity/Q838781> ;
	skos:broader	medtop:20000923 .

medtop:20000928
	rdf:type skos:Concept ;
	skos:prefLabel	"horse driving"@en-GB ;
	skos:definition	"Equestrian events involving horses being driven in harness, single vehicle around a course."@en-GB ;
	skos:note	"Retired. Use Media Topic equestrianism + sports facet equestriantype."@en-GB ;
	skos:inScheme <http://cv.iptc.org/newscodes/mediatopic/>  ;
	ikos:created "2009-10-22T02:00:00+00:00"^^xsd:dateTime ;
	dct:created "2009-10-22T02:00:00+00:00"^^xsd:dateTime ;
	ikos:modified "2021-02-18T12:00:00+00:00"^^xsd:dateTime ;
	dct:modified "2021-02-18T12:00:00+00:00"^^xsd:dateTime  ; 
	ikos:retired "2017-07-04T12:00:00+00:00"^^xsd:dateTime ;
	skos:broadMatch subj:15022000 ;
	skos:exactMatch <https://www.wikidata.org/entity/Q1194269> ;
	skos:broader	medtop:20000923 .

medtop:20000929
	rdf:type skos:Concept ;
	skos:prefLabel	"fencing"@en-GB ;
	skos:definition	"Combat sport using a sword or foil."@en-GB ;
	skos:inScheme <http://cv.iptc.org/newscodes/mediatopic/>  ;
	ikos:created "2009-10-22T02:00:00+00:00"^^xsd:dateTime ;
	dct:created "2009-10-22T02:00:00+00:00"^^xsd:dateTime ;
	ikos:modified "2021-02-18T12:00:00+00:00"^^xsd:dateTime ;
	dct:modified "2021-02-18T12:00:00+00:00"^^xsd:dateTime  ;
	ikos:hasFacet aspfacet:fencingtype ;
	skos:exactMatch subj:15023000 ;
	skos:exactMatch <https://www.wikidata.org/entity/Q12100> ;
	skos:broader	medtop:20000822 ;
	skos:narrower	medtop:20000930 ;
	skos:narrower	medtop:20000931 ;
	skos:narrower	medtop:20000932 .

medtop:20000930
	rdf:type skos:Concept ;
	skos:prefLabel	"epee"@en-GB ;
	skos:definition	"Category of fencing using a weapon with a triangular cross-section blade and a large bell guard"@en-GB ;
	skos:note	"Retired. Use Media Topic fencing + sports facet fencingtype."@en-GB ;
	skos:inScheme <http://cv.iptc.org/newscodes/mediatopic/>  ;
	ikos:created "2009-10-22T02:00:00+00:00"^^xsd:dateTime ;
	dct:created "2009-10-22T02:00:00+00:00"^^xsd:dateTime ;
	ikos:modified "2021-07-12T12:00:00+00:00"^^xsd:dateTime ;
	dct:modified "2021-07-12T12:00:00+00:00"^^xsd:dateTime  ; 
	ikos:retired "2017-07-04T12:00:00+00:00"^^xsd:dateTime ;
	skos:exactMatch subj:15023001 ;
	skos:exactMatch <https://www.wikidata.org/entity/Q840419> ;
	skos:broader	medtop:20000929 .

medtop:20000931
	rdf:type skos:Concept ;
	skos:prefLabel	"foil"@en-GB ;
	skos:definition	"Category of fencing using a weapon with a rectangular cross-section blade and a small bell guard"@en-GB ;
	skos:note	"Retired. Use Media Topic fencing + sports facet fencingtype."@en-GB ;
	skos:inScheme <http://cv.iptc.org/newscodes/mediatopic/>  ;
	ikos:created "2009-10-22T02:00:00+00:00"^^xsd:dateTime ;
	dct:created "2009-10-22T02:00:00+00:00"^^xsd:dateTime ;
	ikos:modified "2021-02-18T12:00:00+00:00"^^xsd:dateTime ;
	dct:modified "2021-02-18T12:00:00+00:00"^^xsd:dateTime  ; 
	ikos:retired "2017-07-04T12:00:00+00:00"^^xsd:dateTime ;
	skos:exactMatch subj:15023002 ;
	skos:exactMatch <https://www.wikidata.org/entity/Q43396037> ;
	skos:broader	medtop:20000929 .

medtop:20000932
	rdf:type skos:Concept ;
	skos:prefLabel	"sabre"@en-GB ;
	skos:definition	"A fencing weapon with a flat blade and knuckle guard used with cutting or thrusting moves"@en-GB ;
	skos:note	"Retired. Use Media Topic fencing + sports facet fencingtype."@en-GB ;
	skos:inScheme <http://cv.iptc.org/newscodes/mediatopic/>  ;
	ikos:created "2009-10-22T02:00:00+00:00"^^xsd:dateTime ;
	dct:created "2009-10-22T02:00:00+00:00"^^xsd:dateTime ;
	ikos:modified "2021-02-18T12:00:00+00:00"^^xsd:dateTime ;
	dct:modified "2021-02-18T12:00:00+00:00"^^xsd:dateTime  ; 
	ikos:retired "2017-07-04T12:00:00+00:00"^^xsd:dateTime ;
	skos:exactMatch subj:15023003 ;
	skos:exactMatch <https://www.wikidata.org/entity/Q1156606> ;
	skos:broader	medtop:20000929 .

medtop:20000933
	rdf:type skos:Concept ;
	skos:prefLabel	"field hockey"@en-GB ;
	skos:definition	"A ball sport involving two teams of 11 players using curved sticks. The aim is to score as many goals as possible."@en-GB ;
	skos:inScheme <http://cv.iptc.org/newscodes/mediatopic/>  ;
	ikos:created "2009-10-22T02:00:00+00:00"^^xsd:dateTime ;
	dct:created "2009-10-22T02:00:00+00:00"^^xsd:dateTime ;
	ikos:modified "2021-02-18T12:00:00+00:00"^^xsd:dateTime ;
	dct:modified "2021-02-18T12:00:00+00:00"^^xsd:dateTime  ;
	skos:exactMatch subj:15024000 ;
	skos:exactMatch <https://www.wikidata.org/entity/Q1455> ;
	skos:broader	medtop:20000822 .

medtop:20000934
	rdf:type skos:Concept ;
	skos:prefLabel	"figure skating"@en-GB ;
	skos:definition	"To obtain the best marks possible from nine judges who award scores after two prepared sections - both skated to music - during which competitors must attempt to achieve the greatest possible harmony between artistic flair and technical precision."@en-GB ;
	skos:inScheme <http://cv.iptc.org/newscodes/mediatopic/>  ;
	ikos:created "2009-10-22T02:00:00+00:00"^^xsd:dateTime ;
	dct:created "2009-10-22T02:00:00+00:00"^^xsd:dateTime ;
	ikos:modified "2021-02-18T12:00:00+00:00"^^xsd:dateTime ;
	dct:modified "2021-02-18T12:00:00+00:00"^^xsd:dateTime  ;
	skos:exactMatch subj:15025000 ;
	ikos:hasFacet aspfacet:figureskatingtype ;
	skos:exactMatch <https://www.wikidata.org/entity/Q38108> ;
	skos:broader	medtop:20000822 ;
	skos:narrower	medtop:20000935 .

medtop:20000935
	rdf:type skos:Concept ;
	skos:prefLabel	"ice dance"@en-GB ;
	skos:definition	"Takes place over three days with, in order, two compulsory dances, the original dance (2min 30sec) and the free dance (4min)."@en-GB ;
	skos:note	"Retired. Use Media Topic figure skating + sports facet figureskatetype."@en-GB ;
	skos:inScheme <http://cv.iptc.org/newscodes/mediatopic/>  ;
	ikos:created "2009-10-22T02:00:00+00:00"^^xsd:dateTime ;
	dct:created "2009-10-22T02:00:00+00:00"^^xsd:dateTime ;
	ikos:modified "2021-02-18T12:00:00+00:00"^^xsd:dateTime ;
	dct:modified "2021-02-18T12:00:00+00:00"^^xsd:dateTime  ; 
	ikos:retired "2017-07-04T12:00:00+00:00"^^xsd:dateTime ;
	skos:exactMatch subj:15025003 ;
	skos:exactMatch <https://www.wikidata.org/entity/Q926191> ;
	skos:broader	medtop:20000934 .

medtop:20000936
	rdf:type skos:Concept ;
	skos:prefLabel	"fist ball"@en-GB ;
	skos:definition	"Men's team sport similar to volleyball (with a much lower net) executed mainly in gymnastics clubs"@en-GB ;
	skos:inScheme <http://cv.iptc.org/newscodes/mediatopic/>  ;
	ikos:created "2009-10-22T02:00:00+00:00"^^xsd:dateTime ;
	dct:created "2009-10-22T02:00:00+00:00"^^xsd:dateTime ;
	ikos:modified "2021-02-18T12:00:00+00:00"^^xsd:dateTime ;
	dct:modified "2021-02-18T12:00:00+00:00"^^xsd:dateTime  ;
	skos:exactMatch subj:15088000 ;
	skos:exactMatch <https://www.wikidata.org/entity/Q1050588> ;
	skos:broader	medtop:20000822 .

medtop:20000937
	rdf:type skos:Concept ;
	skos:prefLabel	"floorball"@en-GB ;
	skos:definition	"Played indoors in a court the size of a basketball court. 6 players per team, of which one is a goalkeeper. He/she operates kneeling but there is no goal-stick like in ice hockey. The players use plastic clubs and a light plastic ball to pass and shot goal"@en-GB ;
	skos:inScheme <http://cv.iptc.org/newscodes/mediatopic/>  ;
	ikos:created "2009-10-22T02:00:00+00:00"^^xsd:dateTime ;
	dct:created "2009-10-22T02:00:00+00:00"^^xsd:dateTime ;
	ikos:modified "2021-02-18T12:00:00+00:00"^^xsd:dateTime ;
	dct:modified "2021-02-18T12:00:00+00:00"^^xsd:dateTime  ;
	skos:exactMatch subj:15078000 ;
	skos:exactMatch <https://www.wikidata.org/entity/Q206763> ;
	skos:broader	medtop:20000822 .

medtop:20000938
	rdf:type skos:Concept ;
	skos:prefLabel	"flying disc"@en-GB ;
	skos:definition	"A group of events all played with a flying plastic disc. The exact regulation for the disc is different in different events but it has to be unbroken of solid plastic and a production model with no modification. Flying disc is sometimes called Frisbee."@en-GB ;
	skos:inScheme <http://cv.iptc.org/newscodes/mediatopic/>  ;
	ikos:created "2009-10-22T02:00:00+00:00"^^xsd:dateTime ;
	dct:created "2009-10-22T02:00:00+00:00"^^xsd:dateTime ;
	ikos:modified "2021-02-18T12:00:00+00:00"^^xsd:dateTime ;
	dct:modified "2021-02-18T12:00:00+00:00"^^xsd:dateTime  ;
	skos:exactMatch subj:15077000 ;
	ikos:hasFacet aspfacet:flyingdisctype ;
	skos:exactMatch <https://www.wikidata.org/entity/Q27672886> ;
	skos:broader	medtop:20000822 .

medtop:20000939
	rdf:type skos:Concept ;
	skos:prefLabel	"Gaelic football"@en-GB ;
	skos:definition	"A form of football played by two teams of 15 competing on a pitch by running with, kicking and passing a spherical ball. Points are scored by moving the ball between goal posts. Governed by the Gaelic Athletic Association."@en-GB ;
	skos:changeNote	"2016-04-06: definition rephrased."@en-GB ;
	skos:inScheme <http://cv.iptc.org/newscodes/mediatopic/>  ;
	ikos:created "2009-10-22T02:00:00+00:00"^^xsd:dateTime ;
	dct:created "2009-10-22T02:00:00+00:00"^^xsd:dateTime ;
	ikos:modified "2021-02-18T12:00:00+00:00"^^xsd:dateTime ;
	dct:modified "2021-02-18T12:00:00+00:00"^^xsd:dateTime  ;
	skos:broadMatch subj:15000000 ;
	skos:exactMatch <https://www.wikidata.org/entity/Q204632> ;
	skos:broader	medtop:20000822 .

medtop:20000940
	rdf:type skos:Concept ;
	skos:prefLabel	"golf"@en-GB ;
	skos:definition	"A game to hit a small hard ball with different clubs around a course of typically 18 holes varying in distance and during a round. The object, depending on the scoring formulae, is to make the fewest strokes possible"@en-GB ;
	skos:inScheme <http://cv.iptc.org/newscodes/mediatopic/>  ;
	ikos:created "2009-10-22T02:00:00+00:00"^^xsd:dateTime ;
	dct:created "2009-10-22T02:00:00+00:00"^^xsd:dateTime ;
	ikos:modified "2021-02-18T12:00:00+00:00"^^xsd:dateTime ;
	dct:modified "2021-02-18T12:00:00+00:00"^^xsd:dateTime  ;
	skos:exactMatch subj:15027000 ;
	skos:exactMatch <https://www.wikidata.org/entity/Q5377> ;
	skos:broader	medtop:20000822 ;
	skos:narrower	medtop:20000941 .

medtop:20000941
	rdf:type skos:Concept ;
	skos:prefLabel	"mini golf"@en-GB ;
	skos:definition	"A game where small hard balls must be holed on an artificial course in as few strokes from the club as possible"@en-GB ;
	skos:inScheme <http://cv.iptc.org/newscodes/mediatopic/>  ;
	ikos:created "2009-10-22T02:00:00+00:00"^^xsd:dateTime ;
	dct:created "2009-10-22T02:00:00+00:00"^^xsd:dateTime ;
	ikos:modified "2021-02-18T12:00:00+00:00"^^xsd:dateTime ;
	dct:modified "2021-02-18T12:00:00+00:00"^^xsd:dateTime  ;
	skos:exactMatch subj:15075000 ;
	skos:exactMatch <https://www.wikidata.org/entity/Q754796> ;
	skos:broader	medtop:20000940 .

medtop:20000942
	rdf:type skos:Concept ;
	skos:prefLabel	"gymnastics"@en-GB ;
	skos:definition	"A sport consisting of a variety of disciplines in which gymnasts perform artistic and acrobatic moves using different apparatus."@en-GB ;
	skos:inScheme <http://cv.iptc.org/newscodes/mediatopic/>  ;
	ikos:created "2009-10-22T02:00:00+00:00"^^xsd:dateTime ;
	dct:created "2009-10-22T02:00:00+00:00"^^xsd:dateTime ;
	ikos:modified "2021-02-18T12:00:00+00:00"^^xsd:dateTime ;
	dct:modified "2021-02-18T12:00:00+00:00"^^xsd:dateTime  ;
	skos:exactMatch subj:15028000 ;
	skos:exactMatch <https://www.wikidata.org/entity/Q43450> ;
	skos:broader	medtop:20000822 ;
	skos:narrower	medtop:20000951 ;
	skos:narrower	medtop:20000955 ;
	skos:narrower	medtop:20001152 .

medtop:20000943
	rdf:type skos:Concept ;
	skos:prefLabel	"ball (rhythmic gymnastics)"@en-GB ;
	skos:definition	"An exercise based on suppleness of the body using a ball."@en-GB ;
	skos:inScheme <http://cv.iptc.org/newscodes/mediatopic/>  ;
	ikos:created "2009-10-22T02:00:00+00:00"^^xsd:dateTime ;
	dct:created "2009-10-22T02:00:00+00:00"^^xsd:dateTime ;
	ikos:modified "2021-12-21T12:00:00+00:00"^^xsd:dateTime ;
	dct:modified "2021-12-21T12:00:00+00:00"^^xsd:dateTime  ; 
	ikos:retired "2015-02-24T12:00:00+00:00"^^xsd:dateTime ;
	skos:exactMatch subj:15028014 ;
	skos:exactMatch <https://www.wikidata.org/entity/Q2356340> ;
	skos:broader	medtop:20000951 .

medtop:20000944
	rdf:type skos:Concept ;
	skos:prefLabel	"beam (artistic gymnastics)"@en-GB ;
	skos:definition	"Gymnasts perform leaps and flips from the much feared balance beam just 10 cm wide."@en-GB ;
	skos:inScheme <http://cv.iptc.org/newscodes/mediatopic/>  ;
	ikos:created "2009-10-22T02:00:00+00:00"^^xsd:dateTime ;
	dct:created "2009-10-22T02:00:00+00:00"^^xsd:dateTime ;
	ikos:modified "2021-12-21T12:00:00+00:00"^^xsd:dateTime ;
	dct:modified "2021-12-21T12:00:00+00:00"^^xsd:dateTime  ; 
	ikos:retired "2015-02-24T12:00:00+00:00"^^xsd:dateTime ;
	skos:exactMatch subj:15028008 ;
	skos:exactMatch <https://www.wikidata.org/entity/Q89579780> ;
	skos:broader	medtop:20001152 .

medtop:20000945
	rdf:type skos:Concept ;
	skos:prefLabel	"clubs (rhythmic gymnastics)"@en-GB ;
	skos:definition	"Dance and gymnastic moves whilst juggling clubs."@en-GB ;
	skos:inScheme <http://cv.iptc.org/newscodes/mediatopic/>  ;
	ikos:created "2009-10-22T02:00:00+00:00"^^xsd:dateTime ;
	dct:created "2009-10-22T02:00:00+00:00"^^xsd:dateTime ;
	ikos:modified "2021-12-21T12:00:00+00:00"^^xsd:dateTime ;
	dct:modified "2021-12-21T12:00:00+00:00"^^xsd:dateTime  ; 
	ikos:retired "2015-02-24T12:00:00+00:00"^^xsd:dateTime ;
	skos:exactMatch subj:15028010 ;
	skos:broader	medtop:20000951 .

medtop:20000946
	rdf:type skos:Concept ;
	skos:prefLabel	"floor exercise (artistic gymnastics)"@en-GB ;
	skos:definition	"A gymnastics floor exercise on a 12m/sq matt."@en-GB ;
	skos:inScheme <http://cv.iptc.org/newscodes/mediatopic/>  ;
	ikos:created "2009-10-22T02:00:00+00:00"^^xsd:dateTime ;
	dct:created "2009-10-22T02:00:00+00:00"^^xsd:dateTime ;
	ikos:modified "2021-12-21T12:00:00+00:00"^^xsd:dateTime ;
	dct:modified "2021-12-21T12:00:00+00:00"^^xsd:dateTime  ; 
	ikos:retired "2015-02-24T12:00:00+00:00"^^xsd:dateTime ;
	skos:exactMatch subj:15028001 ;
	skos:exactMatch <https://www.wikidata.org/entity/Q89580727> ;
	skos:broader	medtop:20001152 .

medtop:20000947
	rdf:type skos:Concept ;
	skos:prefLabel	"hoop (rhythmic gymnastics)"@en-GB ;
	skos:definition	"A hoop is rolled and thrown whilst performing a dance routine."@en-GB ;
	skos:inScheme <http://cv.iptc.org/newscodes/mediatopic/>  ;
	ikos:created "2009-10-22T02:00:00+00:00"^^xsd:dateTime ;
	dct:created "2009-10-22T02:00:00+00:00"^^xsd:dateTime ;
	ikos:modified "2021-12-21T12:00:00+00:00"^^xsd:dateTime ;
	dct:modified "2021-12-21T12:00:00+00:00"^^xsd:dateTime  ; 
	ikos:retired "2015-02-24T12:00:00+00:00"^^xsd:dateTime ;
	skos:closeMatch subj:15028011 ;
	skos:exactMatch <https://www.wikidata.org/entity/Q2553153> ;
	skos:broader	medtop:20000951 .

medtop:20000948
	rdf:type skos:Concept ;
	skos:prefLabel	"horizontal bar (artistic gymnastics)"@en-GB ;
	skos:definition	"Gymnasts turn, spin and perform pirouettes around the horizontal bar."@en-GB ;
	skos:inScheme <http://cv.iptc.org/newscodes/mediatopic/>  ;
	ikos:created "2009-10-22T02:00:00+00:00"^^xsd:dateTime ;
	dct:created "2009-10-22T02:00:00+00:00"^^xsd:dateTime ;
	ikos:modified "2021-12-21T12:00:00+00:00"^^xsd:dateTime ;
	dct:modified "2021-12-21T12:00:00+00:00"^^xsd:dateTime  ; 
	ikos:retired "2015-02-24T12:00:00+00:00"^^xsd:dateTime ;
	skos:exactMatch subj:15028006 ;
	skos:exactMatch <https://www.wikidata.org/entity/Q623270> ;
	skos:broader	medtop:20001152 .

medtop:20000949
	rdf:type skos:Concept ;
	skos:prefLabel	"parallel bars (artistic gymnastics)"@en-GB ;
	skos:definition	"Gymnasts swing and turn with guile and grace around the parallel bars."@en-GB ;
	skos:inScheme <http://cv.iptc.org/newscodes/mediatopic/>  ;
	ikos:created "2009-10-22T02:00:00+00:00"^^xsd:dateTime ;
	dct:created "2009-10-22T02:00:00+00:00"^^xsd:dateTime ;
	ikos:modified "2021-12-21T12:00:00+00:00"^^xsd:dateTime ;
	dct:modified "2021-12-21T12:00:00+00:00"^^xsd:dateTime  ; 
	ikos:retired "2015-02-24T12:00:00+00:00"^^xsd:dateTime ;
	skos:exactMatch subj:15028005 ;
	skos:exactMatch <https://www.wikidata.org/entity/Q692104> ;
	skos:broader	medtop:20001152 .

medtop:20000950
	rdf:type skos:Concept ;
	skos:prefLabel	"pommel horse (artistic gymnastics)"@en-GB ;
	skos:definition	"Gymnasts perform an uninterrupted swing motion over a handled horse using balance and strength"@en-GB ;
	skos:inScheme <http://cv.iptc.org/newscodes/mediatopic/>  ;
	ikos:created "2009-10-22T02:00:00+00:00"^^xsd:dateTime ;
	dct:created "2009-10-22T02:00:00+00:00"^^xsd:dateTime ;
	ikos:modified "2021-12-21T12:00:00+00:00"^^xsd:dateTime ;
	dct:modified "2021-12-21T12:00:00+00:00"^^xsd:dateTime  ; 
	ikos:retired "2015-02-24T12:00:00+00:00"^^xsd:dateTime ;
	skos:exactMatch subj:15028003 ;
	skos:exactMatch <https://www.wikidata.org/entity/Q840330> ;
	skos:broader	medtop:20001152 .

medtop:20000951
	rdf:type skos:Concept ;
	skos:prefLabel	"rhythmic gymnastics"@en-GB ;
	skos:definition	"Mixture of dance and gymnastic moves"@en-GB ;
	skos:inScheme <http://cv.iptc.org/newscodes/mediatopic/>  ;
	ikos:created "2009-10-22T02:00:00+00:00"^^xsd:dateTime ;
	dct:created "2009-10-22T02:00:00+00:00"^^xsd:dateTime ;
	ikos:modified "2021-02-18T12:00:00+00:00"^^xsd:dateTime ;
	dct:modified "2021-02-18T12:00:00+00:00"^^xsd:dateTime  ;
	skos:exactMatch subj:15028009 ;
	ikos:hasFacet aspfacet:rhythmgymtype ;
	skos:exactMatch <https://www.wikidata.org/entity/Q61465> ;
	skos:broader	medtop:20000942 ;
	skos:narrower	medtop:20000943 ;
	skos:narrower	medtop:20000945 ;
	skos:narrower	medtop:20000947 ;
	skos:narrower	medtop:20000952 ;
	skos:narrower	medtop:20000954 .

medtop:20000952
	rdf:type skos:Concept ;
	skos:prefLabel	"ribbon (rhythmic gymnastics)"@en-GB ;
	skos:definition	"Gymnasts work through a pre-arranged routine whilst manipulating a spectacular length of ribbon."@en-GB ;
	skos:inScheme <http://cv.iptc.org/newscodes/mediatopic/>  ;
	ikos:created "2009-10-22T02:00:00+00:00"^^xsd:dateTime ;
	dct:created "2009-10-22T02:00:00+00:00"^^xsd:dateTime ;
	ikos:modified "2021-12-21T12:00:00+00:00"^^xsd:dateTime ;
	dct:modified "2021-12-21T12:00:00+00:00"^^xsd:dateTime  ; 
	ikos:retired "2015-02-24T12:00:00+00:00"^^xsd:dateTime ;
	skos:exactMatch subj:15028012 ;
	skos:exactMatch <https://www.wikidata.org/entity/Q748773> ;
	skos:broader	medtop:20000951 .

medtop:20000953
	rdf:type skos:Concept ;
	skos:prefLabel	"rings (artistic gymnastics)"@en-GB ;
	skos:definition	"Gymnasts perform feats of balance and strength from two suspended rings."@en-GB ;
	skos:inScheme <http://cv.iptc.org/newscodes/mediatopic/>  ;
	ikos:created "2009-10-22T02:00:00+00:00"^^xsd:dateTime ;
	dct:created "2009-10-22T02:00:00+00:00"^^xsd:dateTime ;
	ikos:modified "2021-12-21T12:00:00+00:00"^^xsd:dateTime ;
	dct:modified "2021-12-21T12:00:00+00:00"^^xsd:dateTime  ; 
	ikos:retired "2015-02-24T12:00:00+00:00"^^xsd:dateTime ;
	skos:exactMatch subj:15028007 ;
	skos:exactMatch <https://www.wikidata.org/entity/Q89582128> ;
	skos:broader	medtop:20001152 .

medtop:20000954
	rdf:type skos:Concept ;
	skos:prefLabel	"rope (rhythmic gymnastics)"@en-GB ;
	skos:definition	"Jump and figure movements are performed while a rope is manipulated."@en-GB ;
	skos:inScheme <http://cv.iptc.org/newscodes/mediatopic/>  ;
	ikos:created "2009-10-22T02:00:00+00:00"^^xsd:dateTime ;
	dct:created "2009-10-22T02:00:00+00:00"^^xsd:dateTime ;
	ikos:modified "2021-12-21T12:00:00+00:00"^^xsd:dateTime ;
	dct:modified "2021-12-21T12:00:00+00:00"^^xsd:dateTime  ; 
	ikos:retired "2015-02-24T12:00:00+00:00"^^xsd:dateTime ;
	skos:exactMatch subj:15028013 ;
	skos:exactMatch <https://www.wikidata.org/entity/Q635343> ;
	skos:broader	medtop:20000951 .

medtop:20000955
	rdf:type skos:Concept ;
	skos:prefLabel	"trampoline"@en-GB ;
	skos:definition	"Competitors perform complicated twists and turns whilst bouncing on the trampoline."@en-GB ;
	skos:inScheme <http://cv.iptc.org/newscodes/mediatopic/>  ;
	ikos:created "2009-10-22T02:00:00+00:00"^^xsd:dateTime ;
	dct:created "2009-10-22T02:00:00+00:00"^^xsd:dateTime ;
	ikos:modified "2021-02-18T12:00:00+00:00"^^xsd:dateTime ;
	dct:modified "2021-02-18T12:00:00+00:00"^^xsd:dateTime  ;
	skos:exactMatch subj:15028015 ;
	skos:exactMatch <https://www.wikidata.org/entity/Q465014> ;
	skos:broader	medtop:20000942 .

medtop:20000956
	rdf:type skos:Concept ;
	skos:prefLabel	"uneven bars (artistic gymnastics)"@en-GB ;
	skos:definition	"Gymnasts run through an airborne routine swinging around and between the uneven bars."@en-GB ;
	skos:inScheme <http://cv.iptc.org/newscodes/mediatopic/>  ;
	ikos:created "2009-10-22T02:00:00+00:00"^^xsd:dateTime ;
	dct:created "2009-10-22T02:00:00+00:00"^^xsd:dateTime ;
	ikos:modified "2021-12-21T12:00:00+00:00"^^xsd:dateTime ;
	dct:modified "2021-12-21T12:00:00+00:00"^^xsd:dateTime  ; 
	ikos:retired "2015-02-24T12:00:00+00:00"^^xsd:dateTime ;
	skos:closeMatch subj:15028004 ;
	skos:exactMatch <https://www.wikidata.org/entity/Q89671012> ;
	skos:broader	medtop:20001152 .

medtop:20000957
	rdf:type skos:Concept ;
	skos:prefLabel	"vault (artistic gymnastics)"@en-GB ;
	skos:definition	"Gymnasts propel themselves by jumping on a trampoline after running quickly down a 25m lane"@en-GB ;
	skos:inScheme <http://cv.iptc.org/newscodes/mediatopic/>  ;
	ikos:created "2009-10-22T02:00:00+00:00"^^xsd:dateTime ;
	dct:created "2009-10-22T02:00:00+00:00"^^xsd:dateTime ;
	ikos:modified "2021-12-21T12:00:00+00:00"^^xsd:dateTime ;
	dct:modified "2021-12-21T12:00:00+00:00"^^xsd:dateTime  ; 
	ikos:retired "2015-02-24T12:00:00+00:00"^^xsd:dateTime ;
	skos:exactMatch subj:15028002 ;
	skos:exactMatch <https://www.wikidata.org/entity/Q598168> ;
	skos:broader	medtop:20001152 .

medtop:20000958
	rdf:type skos:Concept ;
	skos:prefLabel	"handball (team)"@en-GB ;
	skos:definition	"A ball game using the hands contested by two teams of seven trying to throw the ball into the opponents goal."@en-GB ;
	skos:inScheme <http://cv.iptc.org/newscodes/mediatopic/>  ;
	ikos:created "2009-10-22T02:00:00+00:00"^^xsd:dateTime ;
	dct:created "2009-10-22T02:00:00+00:00"^^xsd:dateTime ;
	ikos:modified "2021-02-18T12:00:00+00:00"^^xsd:dateTime ;
	dct:modified "2021-02-18T12:00:00+00:00"^^xsd:dateTime  ;
	skos:exactMatch subj:15029000 ;
	skos:exactMatch <https://www.wikidata.org/entity/Q8418> ;
	skos:broader	medtop:20000822 .

medtop:20000959
	rdf:type skos:Concept ;
	skos:prefLabel	"hornuss"@en-GB ;
	skos:definition	"Swiss team sport with 16 or 18 men per team. A rubber puck is hit towards the field of the adversary team which tries to hit the puck in the air with a wooden board thrown in the air"@en-GB ;
	skos:inScheme <http://cv.iptc.org/newscodes/mediatopic/>  ;
	ikos:created "2009-10-22T02:00:00+00:00"^^xsd:dateTime ;
	dct:created "2009-10-22T02:00:00+00:00"^^xsd:dateTime ;
	ikos:modified "2021-02-18T12:00:00+00:00"^^xsd:dateTime ;
	dct:modified "2021-02-18T12:00:00+00:00"^^xsd:dateTime  ;
	skos:exactMatch subj:15087000 ;
	skos:exactMatch <https://www.wikidata.org/entity/Q669810> ;
	skos:broader	medtop:20000822 .

medtop:20000960
	rdf:type skos:Concept ;
	skos:prefLabel	"horse racing"@en-GB ;
	skos:definition	"Mounted horse races."@en-GB ;
	skos:inScheme <http://cv.iptc.org/newscodes/mediatopic/>  ;
	ikos:created "2009-10-22T02:00:00+00:00"^^xsd:dateTime ;
	dct:created "2009-10-22T02:00:00+00:00"^^xsd:dateTime ;
	ikos:modified "2021-02-18T12:00:00+00:00"^^xsd:dateTime ;
	dct:modified "2021-02-18T12:00:00+00:00"^^xsd:dateTime  ;
	skos:exactMatch subj:15030000 ;
	skos:exactMatch <https://www.wikidata.org/entity/Q187916> ;
	skos:broader	medtop:20000822 ;
	skos:narrower	medtop:20000961 ;
	skos:narrower	medtop:20000962 ;
	skos:narrower	medtop:20000963 .

medtop:20000961
	rdf:type skos:Concept ;
	skos:prefLabel	"flat racing"@en-GB ;
	skos:definition	"A horse race over a flat course."@en-GB ;
	skos:note	"Retired. Use Media Topic horse racing + sports facet equestriantype."@en-GB ;
	skos:inScheme <http://cv.iptc.org/newscodes/mediatopic/>  ;
	ikos:created "2009-10-22T02:00:00+00:00"^^xsd:dateTime ;
	dct:created "2009-10-22T02:00:00+00:00"^^xsd:dateTime ;
	ikos:modified "2021-02-18T12:00:00+00:00"^^xsd:dateTime ;
	dct:modified "2021-02-18T12:00:00+00:00"^^xsd:dateTime  ; 
	ikos:retired "2017-07-04T12:00:00+00:00"^^xsd:dateTime ;
	skos:exactMatch subj:15030001 ;
	skos:exactMatch <https://www.wikidata.org/entity/Q5369934> ;
	skos:broader	medtop:20000960 .

medtop:20000962
	rdf:type skos:Concept ;
	skos:prefLabel	"harness racing"@en-GB ;
	skos:definition	"Horses hitched to a jockeyed buggy race round a flat course. Can be performed at a trotting gait or a pacing gait."@en-GB ;
	skos:note	"Retired. Use Media Topic horse racing + sports facet equestriantype."@en-GB ;
	skos:inScheme <http://cv.iptc.org/newscodes/mediatopic/>  ;
	ikos:created "2009-10-22T02:00:00+00:00"^^xsd:dateTime ;
	dct:created "2009-10-22T02:00:00+00:00"^^xsd:dateTime ;
	ikos:modified "2021-02-18T12:00:00+00:00"^^xsd:dateTime ;
	dct:modified "2021-02-18T12:00:00+00:00"^^xsd:dateTime  ; 
	ikos:retired "2017-07-04T12:00:00+00:00"^^xsd:dateTime ;
	skos:exactMatch subj:15030000 ;
	skos:exactMatch <https://www.wikidata.org/entity/Q1194269> ;
	skos:broader	medtop:20000960 .

medtop:20000963
	rdf:type skos:Concept ;
	skos:prefLabel	"steeple chase"@en-GB ;
	skos:definition	"A mounted horse race over at least eight classic obstacles, four of which must be different, such as the water jump, spruce fences, mud walls etc."@en-GB ;
	skos:note	"Retired. Use Media Topic horse racing + sports facet equestriantype."@en-GB ;
	skos:inScheme <http://cv.iptc.org/newscodes/mediatopic/>  ;
	ikos:created "2009-10-22T02:00:00+00:00"^^xsd:dateTime ;
	dct:created "2009-10-22T02:00:00+00:00"^^xsd:dateTime ;
	ikos:modified "2021-02-18T12:00:00+00:00"^^xsd:dateTime ;
	dct:modified "2021-02-18T12:00:00+00:00"^^xsd:dateTime  ; 
	ikos:retired "2017-07-04T12:00:00+00:00"^^xsd:dateTime ;
	skos:exactMatch subj:15030002 ;
	skos:exactMatch <https://www.wikidata.org/entity/Q2300237> ;
	skos:broader	medtop:20000960 .

medtop:20000964
	rdf:type skos:Concept ;
	skos:prefLabel	"hurling"@en-GB ;
	skos:definition	"A game played by two teams of fifteen each with a curved wooden stick called a hurley. The object is to score a goal by hitting the small ball between the opponents' goalposts either over the crossbar or under it into a net guarded by a goalkeeper."@en-GB ;
	skos:inScheme <http://cv.iptc.org/newscodes/mediatopic/>  ;
	ikos:created "2009-10-22T02:00:00+00:00"^^xsd:dateTime ;
	dct:created "2009-10-22T02:00:00+00:00"^^xsd:dateTime ;
	ikos:modified "2021-02-18T12:00:00+00:00"^^xsd:dateTime ;
	dct:modified "2021-02-18T12:00:00+00:00"^^xsd:dateTime  ;
	skos:broadMatch subj:15000000 ;
	skos:exactMatch <https://www.wikidata.org/entity/Q213711> ;
	skos:broader	medtop:20000822 .

medtop:20000965
	rdf:type skos:Concept ;
	skos:prefLabel	"ice hockey"@en-GB ;
	skos:definition	"Two teams of six heavily padded skaters try and outscore each other by hitting a puck into the opponents goal."@en-GB ;
	skos:inScheme <http://cv.iptc.org/newscodes/mediatopic/>  ;
	ikos:created "2009-10-22T02:00:00+00:00"^^xsd:dateTime ;
	dct:created "2009-10-22T02:00:00+00:00"^^xsd:dateTime ;
	ikos:modified "2021-02-18T12:00:00+00:00"^^xsd:dateTime ;
	dct:modified "2021-02-18T12:00:00+00:00"^^xsd:dateTime  ;
	skos:exactMatch subj:15031000 ;
	skos:exactMatch <https://www.wikidata.org/entity/Q41466> ;
	skos:broader	medtop:20000822 ;
	skos:narrower	medtop:20000966 .

medtop:20000966
	rdf:type skos:Concept ;
	skos:prefLabel	"sledge hockey"@en-GB ;
	skos:definition	"Like ice hockey but instead of skates small sledges are used. Competitors move by pushing with the arms"@en-GB ;
	skos:inScheme <http://cv.iptc.org/newscodes/mediatopic/>  ;
	ikos:created "2009-10-22T02:00:00+00:00"^^xsd:dateTime ;
	dct:created "2009-10-22T02:00:00+00:00"^^xsd:dateTime ;
	ikos:modified "2021-02-18T12:00:00+00:00"^^xsd:dateTime ;
	dct:modified "2021-02-18T12:00:00+00:00"^^xsd:dateTime  ;
	skos:exactMatch subj:15031002 ;
	skos:exactMatch <https://www.wikidata.org/entity/Q963312> ;
	skos:broader	medtop:20000965 .

medtop:20000967
	rdf:type skos:Concept ;
	skos:prefLabel	"inline skating"@en-GB ;
	skos:definition	"Competitive sports using inline skates"@en-GB ;
	skos:changeNote	"Retired. Use roller sports (medtop:20001155)"@en-GB ;
	skos:inScheme <http://cv.iptc.org/newscodes/mediatopic/>  ;
	ikos:created "2009-10-22T02:00:00+00:00"^^xsd:dateTime ;
	dct:created "2009-10-22T02:00:00+00:00"^^xsd:dateTime ;
	ikos:modified "2021-02-18T12:00:00+00:00"^^xsd:dateTime ;
	dct:modified "2021-02-18T12:00:00+00:00"^^xsd:dateTime  ; 
	ikos:retired "2021-02-18T12:00:00+00:00"^^xsd:dateTime ;
	skos:exactMatch subj:15089000 ;
	skos:exactMatch <https://www.wikidata.org/entity/Q6034982> ;
	skos:broader	medtop:20000822 .

medtop:20000968
	rdf:type skos:Concept ;
	skos:prefLabel	"Jai Alai (Pelota)"@en-GB ;
	skos:definition	"A fast ball play using either the bare hand or a wicker scoop in an arena of walls of different outlay and size"@en-GB ;
	skos:inScheme <http://cv.iptc.org/newscodes/mediatopic/>  ;
	ikos:created "2009-10-22T02:00:00+00:00"^^xsd:dateTime ;
	dct:created "2009-10-22T02:00:00+00:00"^^xsd:dateTime ;
	ikos:modified "2021-02-18T12:00:00+00:00"^^xsd:dateTime ;
	dct:modified "2021-02-18T12:00:00+00:00"^^xsd:dateTime  ;
	ikos:hasFacet aspfacet:jaialaitype ;
	skos:exactMatch subj:15032000 ;
	skos:exactMatch <https://www.wikidata.org/entity/Q1193361> ;
	skos:broader	medtop:20000822 .

medtop:20000969
	rdf:type skos:Concept ;
	skos:prefLabel	"judo"@en-GB ;
	skos:definition	"A defensive martial art."@en-GB ;
	skos:changeNote	"Change Note 2015-08-27: broader term changed"@en-GB ;
	skos:inScheme <http://cv.iptc.org/newscodes/mediatopic/>  ;
	ikos:created "2009-10-22T02:00:00+00:00"^^xsd:dateTime ;
	dct:created "2009-10-22T02:00:00+00:00"^^xsd:dateTime ;
	ikos:modified "2021-02-18T12:00:00+00:00"^^xsd:dateTime ;
	dct:modified "2021-02-18T12:00:00+00:00"^^xsd:dateTime  ;
	ikos:hasFacet aspfacet:weightclasstype ;
	skos:exactMatch subj:15033000 ;
	skos:exactMatch <https://www.wikidata.org/entity/Q11420> ;
	skos:broader	medtop:20001157 ;
	skos:narrower	medtop:20000970 ;
	skos:narrower	medtop:20000971 ;
	skos:narrower	medtop:20000972 ;
	skos:narrower	medtop:20000973 ;
	skos:narrower	medtop:20000974 ;
	skos:narrower	medtop:20000975 ;
	skos:narrower	medtop:20000976 .

medtop:20000970
	rdf:type skos:Concept ;
	skos:prefLabel	"extra lightweight (judo)"@en-GB ;
	skos:definition	"Up to 60kg for men and 48kg for women."@en-GB ;
	skos:inScheme <http://cv.iptc.org/newscodes/mediatopic/>  ;
	ikos:created "2009-10-22T02:00:00+00:00"^^xsd:dateTime ;
	dct:created "2009-10-22T02:00:00+00:00"^^xsd:dateTime ;
	ikos:modified "2021-12-21T12:00:00+00:00"^^xsd:dateTime ;
	dct:modified "2021-12-21T12:00:00+00:00"^^xsd:dateTime  ; 
	ikos:retired "2015-02-24T12:00:00+00:00"^^xsd:dateTime ;
	skos:closeMatch subj:15033007 ;
	skos:exactMatch <https://www.wikidata.org/entity/Q77217208> ;
	skos:broader	medtop:20000969 .

medtop:20000971
	rdf:type skos:Concept ;
	skos:prefLabel	"half-heavyweight (judo)"@en-GB ;
	skos:definition	"Up to 100kg for men and 78kg for women."@en-GB ;
	skos:inScheme <http://cv.iptc.org/newscodes/mediatopic/>  ;
	ikos:created "2009-10-22T02:00:00+00:00"^^xsd:dateTime ;
	dct:created "2009-10-22T02:00:00+00:00"^^xsd:dateTime ;
	ikos:modified "2021-12-21T12:00:00+00:00"^^xsd:dateTime ;
	dct:modified "2021-12-21T12:00:00+00:00"^^xsd:dateTime  ; 
	ikos:retired "2015-02-24T12:00:00+00:00"^^xsd:dateTime ;
	skos:exactMatch subj:15033002 ;
	skos:exactMatch <https://www.wikidata.org/entity/Q77217224> ;
	skos:broader	medtop:20000969 .

medtop:20000972
	rdf:type skos:Concept ;
	skos:prefLabel	"half-lightweight (judo)"@en-GB ;
	skos:definition	"Up to 73kg for men and 57kg for women."@en-GB ;
	skos:inScheme <http://cv.iptc.org/newscodes/mediatopic/>  ;
	ikos:created "2009-10-22T02:00:00+00:00"^^xsd:dateTime ;
	dct:created "2009-10-22T02:00:00+00:00"^^xsd:dateTime ;
	ikos:modified "2021-12-21T12:00:00+00:00"^^xsd:dateTime ;
	dct:modified "2021-12-21T12:00:00+00:00"^^xsd:dateTime  ; 
	ikos:retired "2015-02-24T12:00:00+00:00"^^xsd:dateTime ;
	skos:exactMatch subj:15033005 ;
	skos:exactMatch <https://www.wikidata.org/entity/Q77217224> ;
	skos:broader	medtop:20000969 .

medtop:20000973
	rdf:type skos:Concept ;
	skos:prefLabel	"half-middleweight (judo)"@en-GB ;
	skos:definition	"Up to 81kg for men and 63kg for women"@en-GB ;
	skos:inScheme <http://cv.iptc.org/newscodes/mediatopic/>  ;
	ikos:created "2009-10-22T02:00:00+00:00"^^xsd:dateTime ;
	dct:created "2009-10-22T02:00:00+00:00"^^xsd:dateTime ;
	ikos:modified "2021-12-21T12:00:00+00:00"^^xsd:dateTime ;
	dct:modified "2021-12-21T12:00:00+00:00"^^xsd:dateTime  ; 
	ikos:retired "2015-02-24T12:00:00+00:00"^^xsd:dateTime ;
	skos:exactMatch subj:15033004 ;
	skos:exactMatch <https://www.wikidata.org/entity/Q77217215> ;
	skos:broader	medtop:20000969 .

medtop:20000974
	rdf:type skos:Concept ;
	skos:prefLabel	"heavyweight (judo)"@en-GB ;
	skos:definition	"Open but usually over 100kg for men and over 78kg for women"@en-GB ;
	skos:inScheme <http://cv.iptc.org/newscodes/mediatopic/>  ;
	ikos:created "2009-10-22T02:00:00+00:00"^^xsd:dateTime ;
	dct:created "2009-10-22T02:00:00+00:00"^^xsd:dateTime ;
	ikos:modified "2021-12-21T12:00:00+00:00"^^xsd:dateTime ;
	dct:modified "2021-12-21T12:00:00+00:00"^^xsd:dateTime  ; 
	ikos:retired "2015-02-24T12:00:00+00:00"^^xsd:dateTime ;
	skos:exactMatch subj:15033001 ;
	skos:exactMatch <https://www.wikidata.org/entity/Q77217228> ;
	skos:broader	medtop:20000969 .

medtop:20000975
	rdf:type skos:Concept ;
	skos:prefLabel	"lightweight (judo)"@en-GB ;
	skos:definition	"Up to 66kg for men and 52kg for women."@en-GB ;
	skos:inScheme <http://cv.iptc.org/newscodes/mediatopic/>  ;
	ikos:created "2009-10-22T02:00:00+00:00"^^xsd:dateTime ;
	dct:created "2009-10-22T02:00:00+00:00"^^xsd:dateTime ;
	ikos:modified "2021-12-21T12:00:00+00:00"^^xsd:dateTime ;
	dct:modified "2021-12-21T12:00:00+00:00"^^xsd:dateTime  ; 
	ikos:retired "2015-02-24T12:00:00+00:00"^^xsd:dateTime ;
	skos:exactMatch subj:15033006 ;
	skos:exactMatch <https://www.wikidata.org/entity/Q77217210> ;
	skos:broader	medtop:20000969 .

medtop:20000976
	rdf:type skos:Concept ;
	skos:prefLabel	"middleweight (judo)"@en-GB ;
	skos:definition	"Up to 90kg for men and 70kg for women."@en-GB ;
	skos:inScheme <http://cv.iptc.org/newscodes/mediatopic/>  ;
	ikos:created "2009-10-22T02:00:00+00:00"^^xsd:dateTime ;
	dct:created "2009-10-22T02:00:00+00:00"^^xsd:dateTime ;
	ikos:modified "2021-12-21T12:00:00+00:00"^^xsd:dateTime ;
	dct:modified "2021-12-21T12:00:00+00:00"^^xsd:dateTime  ; 
	ikos:retired "2015-02-24T12:00:00+00:00"^^xsd:dateTime ;
	skos:exactMatch subj:15033003 ;
	skos:exactMatch <https://www.wikidata.org/entity/Q77217218> ;
	skos:broader	medtop:20000969 .

medtop:20000977
	rdf:type skos:Concept ;
	skos:prefLabel	"jukendo"@en-GB ;
	skos:definition	"Japanese traditional martial art using a model rifle made of wood. 'Juken' means a rifle or gun with blade (bayonet)"@en-GB ;
	skos:changeNote	"Change Note 2015-08-27: broader term changed"@en-GB ;
	skos:inScheme <http://cv.iptc.org/newscodes/mediatopic/>  ;
	ikos:created "2009-10-22T02:00:00+00:00"^^xsd:dateTime ;
	dct:created "2009-10-22T02:00:00+00:00"^^xsd:dateTime ;
	ikos:modified "2021-02-18T12:00:00+00:00"^^xsd:dateTime ;
	dct:modified "2021-02-18T12:00:00+00:00"^^xsd:dateTime  ;
	skos:exactMatch subj:15094000 ;
	skos:exactMatch <https://www.wikidata.org/entity/Q1717983> ;
	skos:broader	medtop:20001157 .

medtop:20000978
	rdf:type skos:Concept ;
	skos:prefLabel	"kabaddi"@en-GB ;
	skos:definition	"The attacking side scores by touching, and the side to guard scores by capturing. The attacker continues calling it 'kabaddi'."@en-GB ;
	skos:inScheme <http://cv.iptc.org/newscodes/mediatopic/>  ;
	ikos:created "2009-10-22T02:00:00+00:00"^^xsd:dateTime ;
	dct:created "2009-10-22T02:00:00+00:00"^^xsd:dateTime ;
	ikos:modified "2021-02-18T12:00:00+00:00"^^xsd:dateTime ;
	dct:modified "2021-02-18T12:00:00+00:00"^^xsd:dateTime  ;
	skos:exactMatch subj:15097000 ;
	skos:exactMatch <https://www.wikidata.org/entity/Q148636> ;
	skos:broader	medtop:20000822 .

medtop:20000979
	rdf:type skos:Concept ;
	skos:prefLabel	"kayaking"@en-GB ;
	skos:definition	"Competition involving kayaks where the paddler sits with their legs facing forward using a double-bladed paddle"@en-GB ;
	skos:inScheme <http://cv.iptc.org/newscodes/mediatopic/>  ;
	ikos:created "2009-10-22T02:00:00+00:00"^^xsd:dateTime ;
	dct:created "2009-10-22T02:00:00+00:00"^^xsd:dateTime ;
	ikos:modified "2021-02-18T12:00:00+00:00"^^xsd:dateTime ;
	dct:modified "2021-02-18T12:00:00+00:00"^^xsd:dateTime  ;
	skos:broadMatch subj:15015000 ;
	ikos:hasFacet aspfacet:canoekayaktype ;
	skos:exactMatch <https://www.wikidata.org/entity/Q2094083> ;
	skos:broader	medtop:20000822 ;
	skos:narrower	medtop:20000980 ;
	skos:narrower	medtop:20000981 ;
	skos:narrower	medtop:20000982 .

medtop:20000980
	rdf:type skos:Concept ;
	skos:prefLabel	"K1 (kayaking)"@en-GB ;
	skos:definition	"An enclosed boat with the competitor sitting on a fixed seat for one person using a double bladed paddle"@en-GB ;
	skos:inScheme <http://cv.iptc.org/newscodes/mediatopic/>  ;
	ikos:created "2009-10-22T02:00:00+00:00"^^xsd:dateTime ;
	dct:created "2009-10-22T02:00:00+00:00"^^xsd:dateTime ;
	ikos:modified "2021-12-21T12:00:00+00:00"^^xsd:dateTime ;
	dct:modified "2021-12-21T12:00:00+00:00"^^xsd:dateTime  ; 
	ikos:retired "2015-02-24T12:00:00+00:00"^^xsd:dateTime ;
	skos:exactMatch subj:15015005 ;
	skos:broader	medtop:20000979 .

medtop:20000981
	rdf:type skos:Concept ;
	skos:prefLabel	"K2 (kayaking)"@en-GB ;
	skos:definition	"An enclosed boat with the competitor sitting on a fixed seat for two people using double bladed paddles"@en-GB ;
	skos:inScheme <http://cv.iptc.org/newscodes/mediatopic/>  ;
	ikos:created "2009-10-22T02:00:00+00:00"^^xsd:dateTime ;
	dct:created "2009-10-22T02:00:00+00:00"^^xsd:dateTime ;
	ikos:modified "2021-12-21T12:00:00+00:00"^^xsd:dateTime ;
	dct:modified "2021-12-21T12:00:00+00:00"^^xsd:dateTime  ; 
	ikos:retired "2015-02-24T12:00:00+00:00"^^xsd:dateTime ;
	skos:closeMatch subj:15015006 ;
	skos:exactMatch <https://www.wikidata.org/entity/Q232550> ;
	skos:broader	medtop:20000979 .

medtop:20000982
	rdf:type skos:Concept ;
	skos:prefLabel	"K4 (kayaking)"@en-GB ;
	skos:definition	"An enclosed boat with the competitor sitting on a fixed seat for four people using double bladed paddles"@en-GB ;
	skos:inScheme <http://cv.iptc.org/newscodes/mediatopic/>  ;
	ikos:created "2009-10-22T02:00:00+00:00"^^xsd:dateTime ;
	dct:created "2009-10-22T02:00:00+00:00"^^xsd:dateTime ;
	ikos:modified "2021-12-21T12:00:00+00:00"^^xsd:dateTime ;
	dct:modified "2021-12-21T12:00:00+00:00"^^xsd:dateTime  ; 
	ikos:retired "2015-02-24T12:00:00+00:00"^^xsd:dateTime ;
	skos:exactMatch subj:15015007 ;
	skos:broader	medtop:20000979 .

medtop:20000983
	rdf:type skos:Concept ;
	skos:prefLabel	"karate"@en-GB ;
	skos:definition	"A martial art where chops, punches, kicks and throws are used to defeat an opponent."@en-GB ;
	skos:changeNote	"Change Note 2015-08-27: broader term changed"@en-GB ;
	skos:inScheme <http://cv.iptc.org/newscodes/mediatopic/>  ;
	ikos:created "2009-10-22T02:00:00+00:00"^^xsd:dateTime ;
	dct:created "2009-10-22T02:00:00+00:00"^^xsd:dateTime ;
	ikos:modified "2021-02-18T12:00:00+00:00"^^xsd:dateTime ;
	dct:modified "2021-02-18T12:00:00+00:00"^^xsd:dateTime  ;
	skos:exactMatch subj:15034000 ;
	skos:exactMatch <https://www.wikidata.org/entity/Q11419> ;
	skos:broader	medtop:20001157 .

medtop:20000984
	rdf:type skos:Concept ;
	skos:prefLabel	"kendo"@en-GB ;
	skos:definition	"Japanese traditional martial art using a bamboo sword, sometimes called Japanese fencing"@en-GB ;
	skos:changeNote	"Change Note 2015-08-27: broader term changed"@en-GB ;
	skos:inScheme <http://cv.iptc.org/newscodes/mediatopic/>  ;
	ikos:created "2009-10-22T02:00:00+00:00"^^xsd:dateTime ;
	dct:created "2009-10-22T02:00:00+00:00"^^xsd:dateTime ;
	ikos:modified "2021-03-15T12:00:00+00:00"^^xsd:dateTime ;
	dct:modified "2021-03-15T12:00:00+00:00"^^xsd:dateTime  ;
	skos:exactMatch subj:15093000 ;
	skos:exactMatch <https://www.wikidata.org/entity/Q170931> ;
	skos:broader	medtop:20001157 .

medtop:20000985
	rdf:type skos:Concept ;
	skos:prefLabel	"kyudo"@en-GB ;
	skos:definition	"Japanese traditional martial art using a bamboo bow and arrows, sometimes called Japanese archery"@en-GB ;
	skos:changeNote	"Change Note 2015-08-27: broader term changed"@en-GB ;
	skos:inScheme <http://cv.iptc.org/newscodes/mediatopic/>  ;
	ikos:created "2009-10-22T02:00:00+00:00"^^xsd:dateTime ;
	dct:created "2009-10-22T02:00:00+00:00"^^xsd:dateTime ;
	ikos:modified "2021-02-18T12:00:00+00:00"^^xsd:dateTime ;
	dct:modified "2021-02-18T12:00:00+00:00"^^xsd:dateTime  ;
	skos:exactMatch subj:15096000 ;
	skos:exactMatch <https://www.wikidata.org/entity/Q273125> ;
	skos:broader	medtop:20001157 .

medtop:20000986
	rdf:type skos:Concept ;
	skos:prefLabel	"lacrosse"@en-GB ;
	skos:definition	"Two teams of helmeted and padded players try and outscore each other using a netted stick and hard ball."@en-GB ;
	skos:inScheme <http://cv.iptc.org/newscodes/mediatopic/>  ;
	ikos:created "2009-10-22T02:00:00+00:00"^^xsd:dateTime ;
	dct:created "2009-10-22T02:00:00+00:00"^^xsd:dateTime ;
	ikos:modified "2021-02-18T12:00:00+00:00"^^xsd:dateTime ;
	dct:modified "2021-02-18T12:00:00+00:00"^^xsd:dateTime  ;
	skos:exactMatch subj:15035000 ;
	skos:exactMatch <https://www.wikidata.org/entity/Q185851> ;
	skos:broader	medtop:20000822 .

medtop:20000987
	rdf:type skos:Concept ;
	skos:prefLabel	"luge"@en-GB ;
	skos:definition	"Luge (French word for sled) is competed in singles or doubles. The competitor(s) lay on their back on an open sled and race down a course. The competitor(s) and the sled must be in contact when passing the finishing line. The competitor can steer the sled"@en-GB ;
	skos:inScheme <http://cv.iptc.org/newscodes/mediatopic/>  ;
	ikos:created "2009-10-22T02:00:00+00:00"^^xsd:dateTime ;
	dct:created "2009-10-22T02:00:00+00:00"^^xsd:dateTime ;
	ikos:modified "2021-02-18T12:00:00+00:00"^^xsd:dateTime ;
	dct:modified "2021-02-18T12:00:00+00:00"^^xsd:dateTime  ;
	skos:exactMatch <https://www.wikidata.org/entity/Q273285> ;
	skos:broader	medtop:20000822 .

medtop:20000988
	rdf:type skos:Concept ;
	skos:prefLabel	"marathon"@en-GB ;
	skos:definition	"A road race where competitors run 42.195km, generally through city streets"@en-GB ;
	skos:inScheme <http://cv.iptc.org/newscodes/mediatopic/>  ;
	ikos:created "2009-10-22T02:00:00+00:00"^^xsd:dateTime ;
	dct:created "2009-10-22T02:00:00+00:00"^^xsd:dateTime ;
	ikos:modified "2021-02-18T12:00:00+00:00"^^xsd:dateTime ;
	dct:modified "2021-02-18T12:00:00+00:00"^^xsd:dateTime  ;
	skos:exactMatch subj:15037000 ;
	skos:exactMatch <https://www.wikidata.org/entity/Q40244> ;
	skos:broader	medtop:20000822 .

medtop:20000989
	rdf:type skos:Concept ;
	skos:prefLabel	"modern pentathlon"@en-GB ;
	skos:definition	"The Modern Pentathlon comprises five events run over a single day in the following order: shooting, fencing, swimming, horse riding and running."@en-GB ;
	skos:inScheme <http://cv.iptc.org/newscodes/mediatopic/>  ;
	ikos:created "2009-10-22T02:00:00+00:00"^^xsd:dateTime ;
	dct:created "2009-10-22T02:00:00+00:00"^^xsd:dateTime ;
	ikos:modified "2021-02-18T12:00:00+00:00"^^xsd:dateTime ;
	dct:modified "2021-02-18T12:00:00+00:00"^^xsd:dateTime  ;
	skos:exactMatch subj:15038000 ;
	skos:exactMatch <https://www.wikidata.org/entity/Q32485> ;
	skos:broader	medtop:20000822 .

medtop:20000990
	rdf:type skos:Concept ;
	skos:prefLabel	"motorboat racing"@en-GB ;
	skos:definition	"Racing with boats with engines"@en-GB ;
	skos:inScheme <http://cv.iptc.org/newscodes/mediatopic/>  ;
	ikos:created "2009-10-22T02:00:00+00:00"^^xsd:dateTime ;
	dct:created "2009-10-22T02:00:00+00:00"^^xsd:dateTime ;
	ikos:modified "2021-02-18T12:00:00+00:00"^^xsd:dateTime ;
	dct:modified "2021-02-18T12:00:00+00:00"^^xsd:dateTime  ;
	skos:broadMatch subj:15046000 ;
	skos:exactMatch <https://www.wikidata.org/entity/Q1545308> ;
	skos:broader	medtop:20000822 .

medtop:20000991
	rdf:type skos:Concept ;
	skos:prefLabel	"motor car racing"@en-GB ;
	skos:definition	"Racing with cars"@en-GB ;
	skos:inScheme <http://cv.iptc.org/newscodes/mediatopic/>  ;
	ikos:created "2009-10-22T02:00:00+00:00"^^xsd:dateTime ;
	dct:created "2009-10-22T02:00:00+00:00"^^xsd:dateTime ;
	ikos:modified "2021-02-18T12:00:00+00:00"^^xsd:dateTime ;
	dct:modified "2021-02-18T12:00:00+00:00"^^xsd:dateTime  ;
	skos:exactMatch subj:15039000 ;
	ikos:hasFacet aspfacet:motorcarracingtype ;
	skos:exactMatch <https://www.wikidata.org/entity/Q5386> ;
	skos:broader	medtop:20000822 ;
	skos:narrower	medtop:20000992 ;
	skos:narrower	medtop:20000993 ;
	skos:narrower	medtop:20000994 ;
	skos:narrower	medtop:20000995 ;
	skos:narrower	medtop:20000996 ;
	skos:narrower	medtop:20000997 .

medtop:20000992
	rdf:type skos:Concept ;
	skos:prefLabel	"endurance race"@en-GB ;
	skos:definition	"Races for one or more drivers over a long and set distance or time"@en-GB ;
	skos:note	"Retired. Use Media Topic motor car racing + sports facet motorcarracingtype"@en-GB ;
	skos:inScheme <http://cv.iptc.org/newscodes/mediatopic/>  ;
	ikos:created "2009-10-22T02:00:00+00:00"^^xsd:dateTime ;
	dct:created "2009-10-22T02:00:00+00:00"^^xsd:dateTime ;
	ikos:modified "2021-02-18T12:00:00+00:00"^^xsd:dateTime ;
	dct:modified "2021-02-18T12:00:00+00:00"^^xsd:dateTime  ; 
	ikos:retired "2017-07-04T12:00:00+00:00"^^xsd:dateTime ;
	skos:exactMatch subj:15039003 ;
	skos:exactMatch <https://www.wikidata.org/entity/Q1805420> ;
	skos:broader	medtop:20000991 .

medtop:20000993
	rdf:type skos:Concept ;
	skos:prefLabel	"F3000"@en-GB ;
	skos:definition	"Using less powerful motors than the Formula One, designated construction teams race over varied circuits the world over in speed races for individual and team honours over a season."@en-GB ;
	skos:note	"Retired. Use Media Topic motor car racing + sports facet motorcarracingtype"@en-GB ;
	skos:inScheme <http://cv.iptc.org/newscodes/mediatopic/>  ;
	ikos:created "2009-10-22T02:00:00+00:00"^^xsd:dateTime ;
	dct:created "2009-10-22T02:00:00+00:00"^^xsd:dateTime ;
	ikos:modified "2021-02-18T12:00:00+00:00"^^xsd:dateTime ;
	dct:modified "2021-02-18T12:00:00+00:00"^^xsd:dateTime  ; 
	ikos:retired "2017-07-04T12:00:00+00:00"^^xsd:dateTime ;
	skos:exactMatch subj:15039002 ;
	skos:exactMatch <https://www.wikidata.org/entity/Q744289> ;
	skos:broader	medtop:20000991 .

medtop:20000994
	rdf:type skos:Concept ;
	skos:prefLabel	"Formula One"@en-GB ;
	skos:definition	"Single cockpit car racing where 20 or so competitors race head to head over varied circuits around the world to win Grand Prix points in an individual and constructors championship"@en-GB ;
	skos:note	"Retired. Use Media Topic motor car racing + sports facet motorcarracingtype"@en-GB ;
	skos:inScheme <http://cv.iptc.org/newscodes/mediatopic/>  ;
	ikos:created "2009-10-22T02:00:00+00:00"^^xsd:dateTime ;
	dct:created "2009-10-22T02:00:00+00:00"^^xsd:dateTime ;
	ikos:modified "2021-02-18T12:00:00+00:00"^^xsd:dateTime ;
	dct:modified "2021-02-18T12:00:00+00:00"^^xsd:dateTime  ; 
	ikos:retired "2017-07-04T12:00:00+00:00"^^xsd:dateTime ;
	skos:exactMatch subj:15039001 ;
	skos:exactMatch <https://www.wikidata.org/entity/Q1968> ;
	skos:broader	medtop:20000991 .

medtop:20000995
	rdf:type skos:Concept ;
	skos:prefLabel	"Indy Racing"@en-GB ;
	skos:definition	"North American top range professional league speed racing over circuits."@en-GB ;
	skos:note	"Retired. Use Media Topic motor car racing + sports facet motorcarracingtype"@en-GB ;
	skos:inScheme <http://cv.iptc.org/newscodes/mediatopic/>  ;
	ikos:created "2009-10-22T02:00:00+00:00"^^xsd:dateTime ;
	dct:created "2009-10-22T02:00:00+00:00"^^xsd:dateTime ;
	ikos:modified "2021-02-18T12:00:00+00:00"^^xsd:dateTime ;
	dct:modified "2021-02-18T12:00:00+00:00"^^xsd:dateTime  ; 
	ikos:retired "2017-07-04T12:00:00+00:00"^^xsd:dateTime ;
	skos:exactMatch subj:15039004 ;
	skos:exactMatch <https://www.wikidata.org/entity/Q832052> ;
	skos:broader	medtop:20000991 .

medtop:20000996
	rdf:type skos:Concept ;
	skos:prefLabel	"motor car rallycross"@en-GB ;
	skos:definition	"Stage races over dirt tracks"@en-GB ;
	skos:note	"Retired. Use Media Topic motor car racing + sports facet motorcarracingtype"@en-GB ;
	skos:inScheme <http://cv.iptc.org/newscodes/mediatopic/>  ;
	ikos:created "2009-10-22T02:00:00+00:00"^^xsd:dateTime ;
	dct:created "2009-10-22T02:00:00+00:00"^^xsd:dateTime ;
	ikos:modified "2021-02-18T12:00:00+00:00"^^xsd:dateTime ;
	dct:modified "2021-02-18T12:00:00+00:00"^^xsd:dateTime  ; 
	ikos:retired "2017-07-04T12:00:00+00:00"^^xsd:dateTime ;
	skos:exactMatch subj:15040003 ;
	skos:exactMatch <https://www.wikidata.org/entity/Q599204> ;
	skos:broader	medtop:20000991 .

medtop:20000997
	rdf:type skos:Concept ;
	skos:prefLabel	"motor car rallying"@en-GB ;
	skos:definition	"A season of endurance races over closed circuits including dirt tracks, roads and even snowy conditions featuring specials using adapted road cars with a driver and co-pilot."@en-GB ;
	skos:note	"Retired. Use Media Topic motor car racing + sports facet motorcarracingtype"@en-GB ;
	skos:inScheme <http://cv.iptc.org/newscodes/mediatopic/>  ;
	ikos:created "2009-10-22T02:00:00+00:00"^^xsd:dateTime ;
	dct:created "2009-10-22T02:00:00+00:00"^^xsd:dateTime ;
	ikos:modified "2021-02-18T12:00:00+00:00"^^xsd:dateTime ;
	dct:modified "2021-02-18T12:00:00+00:00"^^xsd:dateTime  ; 
	ikos:retired "2017-07-04T12:00:00+00:00"^^xsd:dateTime ;
	skos:exactMatch subj:15040000 ;
	skos:exactMatch <https://www.wikidata.org/entity/Q7856> ;
	skos:broader	medtop:20000991 .

medtop:20000998
	rdf:type skos:Concept ;
	skos:prefLabel	"motorcycling"@en-GB ;
	skos:definition	"Races with 2, 3 or 4 wheels vehicles with a saddle and handlebars"@en-GB ;
	skos:inScheme <http://cv.iptc.org/newscodes/mediatopic/>  ;
	ikos:created "2009-10-22T02:00:00+00:00"^^xsd:dateTime ;
	dct:created "2009-10-22T02:00:00+00:00"^^xsd:dateTime ;
	ikos:modified "2021-02-18T12:00:00+00:00"^^xsd:dateTime ;
	dct:modified "2021-02-18T12:00:00+00:00"^^xsd:dateTime  ;
	ikos:hasFacet aspfacet:motorcyclingtype ;
	skos:exactMatch subj:15041000 ;
	skos:exactMatch <https://www.wikidata.org/entity/Q608003> ;
	skos:broader	medtop:20000822 ;
	skos:narrower	medtop:20000999 ;
	skos:narrower	medtop:20001000 ;
	skos:narrower	medtop:20001001 ;
	skos:narrower	medtop:20001002 ;
	skos:narrower	medtop:20001003 ;
	skos:narrower	medtop:20001004 ;
	skos:narrower	medtop:20001005 ;
	skos:narrower	medtop:20001006 ;
	skos:narrower	medtop:20001007 ;
	skos:narrower	medtop:20001008 .

medtop:20000999
	rdf:type skos:Concept ;
	skos:prefLabel	"motorcycle endurance"@en-GB ;
	skos:definition	"A road race of consistency and endurance"@en-GB ;
	skos:note	"Retired. Use Media Topicmotorcycling+ sports facet motorcyclingtype."@en-GB ;
	skos:inScheme <http://cv.iptc.org/newscodes/mediatopic/>  ;
	ikos:created "2009-10-22T02:00:00+00:00"^^xsd:dateTime ;
	dct:created "2009-10-22T02:00:00+00:00"^^xsd:dateTime ;
	ikos:modified "2021-02-18T12:00:00+00:00"^^xsd:dateTime ;
	dct:modified "2021-02-18T12:00:00+00:00"^^xsd:dateTime  ; 
	ikos:retired "2017-07-04T12:00:00+00:00"^^xsd:dateTime ;
	skos:exactMatch subj:15041008 ;
	skos:exactMatch <https://www.wikidata.org/entity/Q15732689> ;
	skos:broader	medtop:20000998 .

medtop:20001000
	rdf:type skos:Concept ;
	skos:prefLabel	"enduro"@en-GB ;
	skos:definition	"A race of speed, endurance and regularity over varied surfaces such as through forests and on dirt tracks"@en-GB ;
	skos:note	"Retired. Use Media Topic motorcycling+ sports facet motorcyclingtype"@en-GB ;
	skos:inScheme <http://cv.iptc.org/newscodes/mediatopic/>  ;
	ikos:created "2009-10-22T02:00:00+00:00"^^xsd:dateTime ;
	dct:created "2009-10-22T02:00:00+00:00"^^xsd:dateTime ;
	ikos:modified "2021-02-18T12:00:00+00:00"^^xsd:dateTime ;
	dct:modified "2021-02-18T12:00:00+00:00"^^xsd:dateTime  ; 
	ikos:retired "2017-07-04T12:00:00+00:00"^^xsd:dateTime ;
	skos:exactMatch subj:15041002 ;
	skos:exactMatch <https://www.wikidata.org/entity/Q853890> ;
	skos:broader	medtop:20000998 .

medtop:20001001
	rdf:type skos:Concept ;
	skos:prefLabel	"grass-track"@en-GB ;
	skos:definition	"A race competed on turf"@en-GB ;
	skos:note	"Retired. Use Media Topicmotorcycling+ sports facet motorcyclingtype"@en-GB ;
	skos:inScheme <http://cv.iptc.org/newscodes/mediatopic/>  ;
	ikos:created "2009-10-22T02:00:00+00:00"^^xsd:dateTime ;
	dct:created "2009-10-22T02:00:00+00:00"^^xsd:dateTime ;
	ikos:modified "2021-02-18T12:00:00+00:00"^^xsd:dateTime ;
	dct:modified "2021-02-18T12:00:00+00:00"^^xsd:dateTime  ; 
	ikos:retired "2017-07-04T12:00:00+00:00"^^xsd:dateTime ;
	skos:exactMatch subj:15041003 ;
	skos:exactMatch <https://www.wikidata.org/entity/Q1474094> ;
	skos:broader	medtop:20000998 .

medtop:20001002
	rdf:type skos:Concept ;
	skos:prefLabel	"moto-ball"@en-GB ;
	skos:definition	"Team sport where drivers play a ball"@en-GB ;
	skos:note	"Retired. Use Media Topic motorcycling+ sports facet racetype."@en-GB ;
	skos:inScheme <http://cv.iptc.org/newscodes/mediatopic/>  ;
	ikos:created "2009-10-22T02:00:00+00:00"^^xsd:dateTime ;
	dct:created "2009-10-22T02:00:00+00:00"^^xsd:dateTime ;
	ikos:modified "2021-02-18T12:00:00+00:00"^^xsd:dateTime ;
	dct:modified "2021-02-18T12:00:00+00:00"^^xsd:dateTime  ; 
	ikos:retired "2017-07-04T12:00:00+00:00"^^xsd:dateTime ;
	skos:exactMatch subj:15041004 ;
	skos:exactMatch <https://www.wikidata.org/entity/Q1826965> ;
	skos:broader	medtop:20000998 .

medtop:20001003
	rdf:type skos:Concept ;
	skos:prefLabel	"moto-cross"@en-GB ;
	skos:definition	"Raced over dirt tracks featuring severe mounds"@en-GB ;
	skos:note	"Retired. Use Media Topic motorcycling+ sports facet racetype."@en-GB ;
	skos:inScheme <http://cv.iptc.org/newscodes/mediatopic/>  ;
	ikos:created "2009-10-22T02:00:00+00:00"^^xsd:dateTime ;
	dct:created "2009-10-22T02:00:00+00:00"^^xsd:dateTime ;
	ikos:modified "2021-02-18T12:00:00+00:00"^^xsd:dateTime ;
	dct:modified "2021-02-18T12:00:00+00:00"^^xsd:dateTime  ; 
	ikos:retired "2017-07-04T12:00:00+00:00"^^xsd:dateTime ;
	skos:exactMatch subj:15041005 ;
	skos:exactMatch <https://www.wikidata.org/entity/Q215862> ;
	skos:broader	medtop:20000998 .

medtop:20001004
	rdf:type skos:Concept ;
	skos:prefLabel	"motoGP"@en-GB ;
	skos:definition	"Capacity class 1000ccm"@en-GB ;
	skos:note	"Retired. Use Media Topic motorcycling+ sports facet racetype."@en-GB ;
	skos:inScheme <http://cv.iptc.org/newscodes/mediatopic/>  ;
	ikos:created "2009-10-22T02:00:00+00:00"^^xsd:dateTime ;
	dct:created "2009-10-22T02:00:00+00:00"^^xsd:dateTime ;
	ikos:modified "2021-02-18T12:00:00+00:00"^^xsd:dateTime ;
	dct:modified "2021-02-18T12:00:00+00:00"^^xsd:dateTime  ; 
	ikos:retired "2017-07-04T12:00:00+00:00"^^xsd:dateTime ;
	skos:exactMatch subj:15041014 ;
	skos:exactMatch <https://www.wikidata.org/entity/Q850292> ;
	skos:broader	medtop:20000998 .

medtop:20001005
	rdf:type skos:Concept ;
	skos:prefLabel	"motorcycle rallying"@en-GB ;
	skos:definition	"Races run over regular roads"@en-GB ;
	skos:note	"Retired. Use Media Topicmotorcycling+ sports facet motorcyclingtype"@en-GB ;
	skos:inScheme <http://cv.iptc.org/newscodes/mediatopic/>  ;
	ikos:created "2009-10-22T02:00:00+00:00"^^xsd:dateTime ;
	dct:created "2009-10-22T02:00:00+00:00"^^xsd:dateTime ;
	ikos:modified "2021-02-18T12:00:00+00:00"^^xsd:dateTime ;
	dct:modified "2021-02-18T12:00:00+00:00"^^xsd:dateTime  ; 
	ikos:retired "2017-07-04T12:00:00+00:00"^^xsd:dateTime ;
	skos:exactMatch subj:15041006 ;
	skos:exactMatch <https://www.wikidata.org/entity/Q2404296> ;
	skos:broader	medtop:20000998 .

medtop:20001006
	rdf:type skos:Concept ;
	skos:prefLabel	"side-cars"@en-GB ;
	skos:definition	"Of different engine sizes but attached to a side car featuring a passenger"@en-GB ;
	skos:note	"Retired. Use Media Topic motorcycling+ sports facet racetype."@en-GB ;
	skos:inScheme <http://cv.iptc.org/newscodes/mediatopic/>  ;
	ikos:created "2009-10-22T02:00:00+00:00"^^xsd:dateTime ;
	dct:created "2009-10-22T02:00:00+00:00"^^xsd:dateTime ;
	ikos:modified "2021-05-05T12:00:00+00:00"^^xsd:dateTime ;
	dct:modified "2021-05-05T12:00:00+00:00"^^xsd:dateTime  ; 
	ikos:retired "2017-07-04T12:00:00+00:00"^^xsd:dateTime ;
	skos:exactMatch subj:15041013 ;
	skos:exactMatch <https://www.wikidata.org/entity/Q1051405> ;
	skos:broader	medtop:20000998 .

medtop:20001007
	rdf:type skos:Concept ;
	skos:prefLabel	"speedway"@en-GB ;
	skos:definition	"Race involving up to six riders competing over a flat oval track. Speedway motorcycles use only one gear and have no brakes"@en-GB ;
	skos:note	"Retired. Use Media Topicmotorcycling+ sports facet motorcyclingtype"@en-GB ;
	skos:inScheme <http://cv.iptc.org/newscodes/mediatopic/>  ;
	ikos:created "2009-10-22T02:00:00+00:00"^^xsd:dateTime ;
	dct:created "2009-10-22T02:00:00+00:00"^^xsd:dateTime ;
	ikos:modified "2021-02-18T12:00:00+00:00"^^xsd:dateTime ;
	dct:modified "2021-02-18T12:00:00+00:00"^^xsd:dateTime  ; 
	ikos:retired "2017-07-04T12:00:00+00:00"^^xsd:dateTime ;
	skos:exactMatch subj:15057000 ;
	skos:exactMatch <https://www.wikidata.org/entity/Q750080> ;
	skos:broader	medtop:20000998 .

medtop:20001008
	rdf:type skos:Concept ;
	skos:prefLabel	"motorcycling trial"@en-GB ;
	skos:definition	"A race of consistency and endurance over varied terrain"@en-GB ;
	skos:note	"Retired. Use Media Topic motorcycling+ sports facet racetype."@en-GB ;
	skos:inScheme <http://cv.iptc.org/newscodes/mediatopic/>  ;
	ikos:created "2009-10-22T02:00:00+00:00"^^xsd:dateTime ;
	dct:created "2009-10-22T02:00:00+00:00"^^xsd:dateTime ;
	ikos:modified "2021-02-18T12:00:00+00:00"^^xsd:dateTime ;
	dct:modified "2021-02-18T12:00:00+00:00"^^xsd:dateTime  ; 
	ikos:retired "2017-07-04T12:00:00+00:00"^^xsd:dateTime ;
	skos:exactMatch subj:15041007 ;
	skos:exactMatch <https://www.wikidata.org/entity/Q1413550> ;
	skos:broader	medtop:20000998 .

medtop:20001009
	rdf:type skos:Concept ;
	skos:prefLabel	"naginata"@en-GB ;
	skos:definition	"Japanese traditional martial art using a pole sword made of wood. 'Naginata' means a spear with a curved blade"@en-GB ;
	skos:changeNote	"Change Note 2015-08-27: broader term changed"@en-GB ;
	skos:inScheme <http://cv.iptc.org/newscodes/mediatopic/>  ;
	ikos:created "2009-10-22T02:00:00+00:00"^^xsd:dateTime ;
	dct:created "2009-10-22T02:00:00+00:00"^^xsd:dateTime ;
	ikos:modified "2021-02-18T12:00:00+00:00"^^xsd:dateTime ;
	dct:modified "2021-02-18T12:00:00+00:00"^^xsd:dateTime  ;
	skos:exactMatch subj:15095000 ;
	skos:exactMatch <https://www.wikidata.org/entity/Q1757215> ;
	skos:broader	medtop:20001157 .

medtop:20001010
	rdf:type skos:Concept ;
	skos:prefLabel	"netball"@en-GB ;
	skos:definition	"A woman's sport similar to basketball though without a board behind the basket"@en-GB ;
	skos:inScheme <http://cv.iptc.org/newscodes/mediatopic/>  ;
	ikos:created "2009-10-22T02:00:00+00:00"^^xsd:dateTime ;
	dct:created "2009-10-22T02:00:00+00:00"^^xsd:dateTime ;
	ikos:modified "2021-02-18T12:00:00+00:00"^^xsd:dateTime ;
	dct:modified "2021-02-18T12:00:00+00:00"^^xsd:dateTime  ;
	skos:exactMatch subj:15042000 ;
	skos:exactMatch <https://www.wikidata.org/entity/Q231200> ;
	skos:broader	medtop:20000822 .

medtop:20001011
	rdf:type skos:Concept ;
	skos:prefLabel	"orienteering"@en-GB ;
	skos:definition	"An individual time-trial over a route marked out by beacons. The competitor has to search out and find in a specific order. The contestant makes his way with the help of a compass and map"@en-GB ;
	skos:inScheme <http://cv.iptc.org/newscodes/mediatopic/>  ;
	ikos:created "2009-10-22T02:00:00+00:00"^^xsd:dateTime ;
	dct:created "2009-10-22T02:00:00+00:00"^^xsd:dateTime ;
	ikos:modified "2021-02-18T12:00:00+00:00"^^xsd:dateTime ;
	dct:modified "2021-02-18T12:00:00+00:00"^^xsd:dateTime  ;
	skos:exactMatch subj:15044000 ;
	skos:exactMatch <https://www.wikidata.org/entity/Q29358> ;
	skos:broader	medtop:20000822 ;
	skos:narrower	medtop:20001012 .

medtop:20001012
	rdf:type skos:Concept ;
	skos:prefLabel	"ski orienteering"@en-GB ;
	skos:definition	"An individual ski time-trial over a route marked out by beacons, that the competitor has to search out and find in a specific order. The contestant makes his way with the help of a compass and map"@en-GB ;
	skos:inScheme <http://cv.iptc.org/newscodes/mediatopic/>  ;
	ikos:created "2009-10-22T02:00:00+00:00"^^xsd:dateTime ;
	dct:created "2009-10-22T02:00:00+00:00"^^xsd:dateTime ;
	ikos:modified "2021-02-18T12:00:00+00:00"^^xsd:dateTime ;
	dct:modified "2021-02-18T12:00:00+00:00"^^xsd:dateTime  ;
	skos:exactMatch subj:15044001 ;
	skos:exactMatch <https://www.wikidata.org/entity/Q428242> ;
	skos:broader	medtop:20001011 .

medtop:20001013
	rdf:type skos:Concept ;
	skos:prefLabel	"parachuting"@en-GB ;
	skos:definition	"Jumping from an aeroplane using a parachute, competitions are precision landings, voltige, individual and team"@en-GB ;
	skos:inScheme <http://cv.iptc.org/newscodes/mediatopic/>  ;
	ikos:created "2009-10-22T02:00:00+00:00"^^xsd:dateTime ;
	dct:created "2009-10-22T02:00:00+00:00"^^xsd:dateTime ;
	ikos:modified "2021-02-18T12:00:00+00:00"^^xsd:dateTime ;
	dct:modified "2021-02-18T12:00:00+00:00"^^xsd:dateTime  ;
	skos:exactMatch subj:15001001 ;
	skos:exactMatch <https://www.wikidata.org/entity/Q193210> ;
	skos:broader	medtop:20000822 .

medtop:20001014
	rdf:type skos:Concept ;
	skos:prefLabel	"polo"@en-GB ;
	skos:definition	"With the aid of a mallet two teams of four horsemen try and knock a bamboo ball into the opponents goal over a pitch 250m long and 150m wide. The game is divided into 4, 6, or 8 time periods of 7min 30sec called chukkas."@en-GB ;
	skos:inScheme <http://cv.iptc.org/newscodes/mediatopic/>  ;
	ikos:created "2009-10-22T02:00:00+00:00"^^xsd:dateTime ;
	dct:created "2009-10-22T02:00:00+00:00"^^xsd:dateTime ;
	ikos:modified "2021-02-18T12:00:00+00:00"^^xsd:dateTime ;
	dct:modified "2021-02-18T12:00:00+00:00"^^xsd:dateTime  ;
	skos:exactMatch subj:15045000 ;
	skos:exactMatch <https://www.wikidata.org/entity/Q134211> ;
	skos:broader	medtop:20000822 .

medtop:20001015
	rdf:type skos:Concept ;
	skos:prefLabel	"pool"@en-GB ;
	skos:definition	"A cue sport on a table with pockets, played with different numbers of balls"@en-GB ;
	skos:inScheme <http://cv.iptc.org/newscodes/mediatopic/>  ;
	ikos:created "2009-10-22T02:00:00+00:00"^^xsd:dateTime ;
	dct:created "2009-10-22T02:00:00+00:00"^^xsd:dateTime ;
	ikos:modified "2021-02-18T12:00:00+00:00"^^xsd:dateTime ;
	dct:modified "2021-02-18T12:00:00+00:00"^^xsd:dateTime  ;
	skos:broadMatch subj:15010000 ;
	ikos:hasFacet aspfacet:billiardtype ;
	skos:exactMatch <https://www.wikidata.org/entity/Q11020> ;
	skos:broader	medtop:20000822 .

medtop:20001016
	rdf:type skos:Concept ;
	skos:prefLabel	"power boating"@en-GB ;
	skos:definition	"Races between motor boats on rivers or lakes"@en-GB ;
	skos:inScheme <http://cv.iptc.org/newscodes/mediatopic/>  ;
	ikos:created "2009-10-22T02:00:00+00:00"^^xsd:dateTime ;
	dct:created "2009-10-22T02:00:00+00:00"^^xsd:dateTime ;
	ikos:modified "2021-02-18T12:00:00+00:00"^^xsd:dateTime ;
	dct:modified "2021-02-18T12:00:00+00:00"^^xsd:dateTime  ;
	skos:exactMatch subj:15046000 ;
	skos:exactMatch <https://www.wikidata.org/entity/Q1545308> ;
	skos:broader	medtop:20000822 .

medtop:20001017
	rdf:type skos:Concept ;
	skos:prefLabel	"rodeo"@en-GB ;
	skos:definition	"A discipline where wild horses or bulls must be mounted and mastered"@en-GB ;
	skos:inScheme <http://cv.iptc.org/newscodes/mediatopic/>  ;
	ikos:created "2009-10-22T02:00:00+00:00"^^xsd:dateTime ;
	dct:created "2009-10-22T02:00:00+00:00"^^xsd:dateTime ;
	ikos:modified "2021-02-18T12:00:00+00:00"^^xsd:dateTime ;
	dct:modified "2021-02-18T12:00:00+00:00"^^xsd:dateTime  ;
	skos:exactMatch subj:15074000 ;
	skos:exactMatch <https://www.wikidata.org/entity/Q207703> ;
	skos:broader	medtop:20000822 ;
	skos:narrower	medtop:20001018 ;
	skos:narrower	medtop:20001019 ;
	skos:narrower	medtop:20001020 ;
	skos:narrower	medtop:20001021 ;
	skos:narrower	medtop:20001022 ;
	skos:narrower	medtop:20001023 ;
	skos:narrower	medtop:20001024 .

medtop:20001018
	rdf:type skos:Concept ;
	skos:prefLabel	"bareback bronc"@en-GB ;
	skos:definition	"Rodeo discipline"@en-GB ;
	skos:inScheme <http://cv.iptc.org/newscodes/mediatopic/>  ;
	ikos:created "2009-10-22T02:00:00+00:00"^^xsd:dateTime ;
	dct:created "2009-10-22T02:00:00+00:00"^^xsd:dateTime ;
	ikos:modified "2021-07-12T12:00:00+00:00"^^xsd:dateTime ;
	dct:modified "2021-07-12T12:00:00+00:00"^^xsd:dateTime  ;
	skos:exactMatch subj:15074006 ;
	skos:broader	medtop:20001017 .

medtop:20001019
	rdf:type skos:Concept ;
	skos:prefLabel	"barrel racing"@en-GB ;
	skos:definition	"Rodeo discipline"@en-GB ;
	skos:inScheme <http://cv.iptc.org/newscodes/mediatopic/>  ;
	ikos:created "2009-10-22T02:00:00+00:00"^^xsd:dateTime ;
	dct:created "2009-10-22T02:00:00+00:00"^^xsd:dateTime ;
	ikos:modified "2021-07-12T12:00:00+00:00"^^xsd:dateTime ;
	dct:modified "2021-07-12T12:00:00+00:00"^^xsd:dateTime  ;
	skos:exactMatch subj:15074001 ;
	skos:exactMatch <https://www.wikidata.org/entity/Q2529836> ;
	skos:broader	medtop:20001017 .

medtop:20001020
	rdf:type skos:Concept ;
	skos:prefLabel	"bull riding"@en-GB ;
	skos:definition	"Rodeo discipline"@en-GB ;
	skos:inScheme <http://cv.iptc.org/newscodes/mediatopic/>  ;
	ikos:created "2009-10-22T02:00:00+00:00"^^xsd:dateTime ;
	dct:created "2009-10-22T02:00:00+00:00"^^xsd:dateTime ;
	ikos:modified "2021-07-12T12:00:00+00:00"^^xsd:dateTime ;
	dct:modified "2021-07-12T12:00:00+00:00"^^xsd:dateTime  ;
	skos:exactMatch subj:15074003 ;
	skos:exactMatch <https://www.wikidata.org/entity/Q696267> ;
	skos:broader	medtop:20001017 .

medtop:20001021
	rdf:type skos:Concept ;
	skos:prefLabel	"bulldogging"@en-GB ;
	skos:definition	"Rodeo discipline"@en-GB ;
	skos:inScheme <http://cv.iptc.org/newscodes/mediatopic/>  ;
	ikos:created "2009-10-22T02:00:00+00:00"^^xsd:dateTime ;
	dct:created "2009-10-22T02:00:00+00:00"^^xsd:dateTime ;
	ikos:modified "2021-07-12T12:00:00+00:00"^^xsd:dateTime ;
	dct:modified "2021-07-12T12:00:00+00:00"^^xsd:dateTime  ;
	skos:exactMatch subj:15074004 ;
	skos:exactMatch <https://www.wikidata.org/entity/Q7605950> ;
	skos:broader	medtop:20001017 .

medtop:20001022
	rdf:type skos:Concept ;
	skos:prefLabel	"calf roping"@en-GB ;
	skos:definition	"Rodeo discipline"@en-GB ;
	skos:inScheme <http://cv.iptc.org/newscodes/mediatopic/>  ;
	ikos:created "2009-10-22T02:00:00+00:00"^^xsd:dateTime ;
	dct:created "2009-10-22T02:00:00+00:00"^^xsd:dateTime ;
	ikos:modified "2021-07-12T12:00:00+00:00"^^xsd:dateTime ;
	dct:modified "2021-07-12T12:00:00+00:00"^^xsd:dateTime  ;
	skos:exactMatch subj:15074002 ;
	skos:exactMatch <https://www.wikidata.org/entity/Q5019578> ;
	skos:broader	medtop:20001017 .

medtop:20001023
	rdf:type skos:Concept ;
	skos:prefLabel	"goat roping"@en-GB ;
	skos:definition	"Rodeo discipline"@en-GB ;
	skos:inScheme <http://cv.iptc.org/newscodes/mediatopic/>  ;
	ikos:created "2009-10-22T02:00:00+00:00"^^xsd:dateTime ;
	dct:created "2009-10-22T02:00:00+00:00"^^xsd:dateTime ;
	ikos:modified "2021-07-12T12:00:00+00:00"^^xsd:dateTime ;
	dct:modified "2021-07-12T12:00:00+00:00"^^xsd:dateTime  ;
	skos:exactMatch subj:15074007 ;
	skos:exactMatch <https://www.wikidata.org/entity/Q5575349> ;
	skos:broader	medtop:20001017 .

medtop:20001024
	rdf:type skos:Concept ;
	skos:prefLabel	"saddle bronc"@en-GB ;
	skos:definition	"Rodeo discipline"@en-GB ;
	skos:inScheme <http://cv.iptc.org/newscodes/mediatopic/>  ;
	ikos:created "2009-10-22T02:00:00+00:00"^^xsd:dateTime ;
	dct:created "2009-10-22T02:00:00+00:00"^^xsd:dateTime ;
	ikos:modified "2021-07-12T12:00:00+00:00"^^xsd:dateTime ;
	dct:modified "2021-07-12T12:00:00+00:00"^^xsd:dateTime  ;
	skos:exactMatch subj:15074005 ;
	skos:broader	medtop:20001017 .

medtop:20001025
	rdf:type skos:Concept ;
	skos:prefLabel	"roller hockey"@en-GB ;
	skos:definition	"Team sport similar to ice hockey, executed on 4 wheel roller skates with sticks and a ball"@en-GB ;
	skos:inScheme <http://cv.iptc.org/newscodes/mediatopic/>  ;
	ikos:created "2009-10-22T02:00:00+00:00"^^xsd:dateTime ;
	dct:created "2009-10-22T02:00:00+00:00"^^xsd:dateTime ;
	ikos:modified "2021-02-18T12:00:00+00:00"^^xsd:dateTime ;
	dct:modified "2021-02-18T12:00:00+00:00"^^xsd:dateTime  ;
	skos:exactMatch subj:15024001 ;
	skos:exactMatch <https://www.wikidata.org/entity/Q1748406> ;
	skos:broader	medtop:20001155 .

medtop:20001026
	rdf:type skos:Concept ;
	skos:prefLabel	"rowing"@en-GB ;
	skos:definition	"Boat racing usually on flat calm waters with boats for 1, 2, 4 or 8 rowers"@en-GB ;
	skos:inScheme <http://cv.iptc.org/newscodes/mediatopic/>  ;
	ikos:created "2009-10-22T02:00:00+00:00"^^xsd:dateTime ;
	dct:created "2009-10-22T02:00:00+00:00"^^xsd:dateTime ;
	ikos:modified "2021-02-18T12:00:00+00:00"^^xsd:dateTime ;
	dct:modified "2021-02-18T12:00:00+00:00"^^xsd:dateTime  ;
	ikos:hasFacet aspfacet:rowingtype ;
	skos:exactMatch subj:15047000 ;
	skos:exactMatch <https://www.wikidata.org/entity/Q159354> ;
	skos:broader	medtop:20000822 ;
	skos:narrower	medtop:20001027 ;
	skos:narrower	medtop:20001028 ;
	skos:narrower	medtop:20001029 ;
	skos:narrower	medtop:20001030 ;
	skos:narrower	medtop:20001031 ;
	skos:narrower	medtop:20001032 ;
	skos:narrower	medtop:20001033 ;
	skos:narrower	medtop:20001034 .

medtop:20001027
	rdf:type skos:Concept ;
	skos:prefLabel	"coxed four"@en-GB ;
	skos:definition	"Four person boats with just one oar each and with a team mate to give directions"@en-GB ;
	skos:inScheme <http://cv.iptc.org/newscodes/mediatopic/>  ;
	ikos:created "2009-10-22T02:00:00+00:00"^^xsd:dateTime ;
	dct:created "2009-10-22T02:00:00+00:00"^^xsd:dateTime ;
	ikos:modified "2021-12-21T12:00:00+00:00"^^xsd:dateTime ;
	dct:modified "2021-12-21T12:00:00+00:00"^^xsd:dateTime  ; 
	ikos:retired "2015-02-24T12:00:00+00:00"^^xsd:dateTime ;
	skos:broadMatch subj:15047000 ;
	skos:exactMatch <https://www.wikidata.org/entity/Q1992528> ;
	skos:broader	medtop:20001026 .

medtop:20001028
	rdf:type skos:Concept ;
	skos:prefLabel	"coxed pair"@en-GB ;
	skos:definition	"Two person boats with just one oar each and with a team mate to give directions"@en-GB ;
	skos:inScheme <http://cv.iptc.org/newscodes/mediatopic/>  ;
	ikos:created "2009-10-22T02:00:00+00:00"^^xsd:dateTime ;
	dct:created "2009-10-22T02:00:00+00:00"^^xsd:dateTime ;
	ikos:modified "2021-12-21T12:00:00+00:00"^^xsd:dateTime ;
	dct:modified "2021-12-21T12:00:00+00:00"^^xsd:dateTime  ; 
	ikos:retired "2015-02-24T12:00:00+00:00"^^xsd:dateTime ;
	skos:broadMatch subj:15047000 ;
	skos:exactMatch <https://www.wikidata.org/entity/Q232557> ;
	skos:broader	medtop:20001026 .

medtop:20001029
	rdf:type skos:Concept ;
	skos:prefLabel	"coxless four"@en-GB ;
	skos:definition	"Four person boats with just one oar each and without a team mate to give directions"@en-GB ;
	skos:inScheme <http://cv.iptc.org/newscodes/mediatopic/>  ;
	ikos:created "2009-10-22T02:00:00+00:00"^^xsd:dateTime ;
	dct:created "2009-10-22T02:00:00+00:00"^^xsd:dateTime ;
	ikos:modified "2021-12-21T12:00:00+00:00"^^xsd:dateTime ;
	dct:modified "2021-12-21T12:00:00+00:00"^^xsd:dateTime  ; 
	ikos:retired "2015-02-24T12:00:00+00:00"^^xsd:dateTime ;
	skos:exactMatch subj:15047005 ;
	skos:exactMatch <https://www.wikidata.org/entity/Q232557> ;
	skos:broader	medtop:20001026 .

medtop:20001030
	rdf:type skos:Concept ;
	skos:prefLabel	"coxless pair"@en-GB ;
	skos:definition	"Two person boats with just one oar each and without a team mate to give directions"@en-GB ;
	skos:inScheme <http://cv.iptc.org/newscodes/mediatopic/>  ;
	ikos:created "2009-10-22T02:00:00+00:00"^^xsd:dateTime ;
	dct:created "2009-10-22T02:00:00+00:00"^^xsd:dateTime ;
	ikos:modified "2021-12-21T12:00:00+00:00"^^xsd:dateTime ;
	dct:modified "2021-12-21T12:00:00+00:00"^^xsd:dateTime  ; 
	ikos:retired "2015-02-24T12:00:00+00:00"^^xsd:dateTime ;
	skos:exactMatch subj:15047004 ;
	skos:exactMatch <https://www.wikidata.org/entity/Q232563> ;
	skos:broader	medtop:20001026 .

medtop:20001031
	rdf:type skos:Concept ;
	skos:prefLabel	"double sculls"@en-GB ;
	skos:definition	"Two person boats with two oars each"@en-GB ;
	skos:inScheme <http://cv.iptc.org/newscodes/mediatopic/>  ;
	ikos:created "2009-10-22T02:00:00+00:00"^^xsd:dateTime ;
	dct:created "2009-10-22T02:00:00+00:00"^^xsd:dateTime ;
	ikos:modified "2021-12-21T12:00:00+00:00"^^xsd:dateTime ;
	dct:modified "2021-12-21T12:00:00+00:00"^^xsd:dateTime  ; 
	ikos:retired "2015-02-24T12:00:00+00:00"^^xsd:dateTime ;
	skos:exactMatch subj:15047002 ;
	skos:exactMatch <https://www.wikidata.org/entity/Q1243495> ;
	skos:broader	medtop:20001026 .

medtop:20001032
	rdf:type skos:Concept ;
	skos:prefLabel	"coxed eight"@en-GB ;
	skos:definition	"Eight person boats with just one oar each and with a team mate to give directions"@en-GB ;
	skos:inScheme <http://cv.iptc.org/newscodes/mediatopic/>  ;
	ikos:created "2009-10-22T02:00:00+00:00"^^xsd:dateTime ;
	dct:created "2009-10-22T02:00:00+00:00"^^xsd:dateTime ;
	ikos:modified "2021-12-21T12:00:00+00:00"^^xsd:dateTime ;
	dct:modified "2021-12-21T12:00:00+00:00"^^xsd:dateTime  ; 
	ikos:retired "2015-02-24T12:00:00+00:00"^^xsd:dateTime ;
	skos:broadMatch subj:15047006 ;
	skos:exactMatch <https://www.wikidata.org/entity/Q81050> ;
	skos:broader	medtop:20001026 .

medtop:20001033
	rdf:type skos:Concept ;
	skos:prefLabel	"quadruple sculls"@en-GB ;
	skos:definition	"Four person boats with two oars each and without a team mate to give directions"@en-GB ;
	skos:inScheme <http://cv.iptc.org/newscodes/mediatopic/>  ;
	ikos:created "2009-10-22T02:00:00+00:00"^^xsd:dateTime ;
	dct:created "2009-10-22T02:00:00+00:00"^^xsd:dateTime ;
	ikos:modified "2021-12-21T12:00:00+00:00"^^xsd:dateTime ;
	dct:modified "2021-12-21T12:00:00+00:00"^^xsd:dateTime  ; 
	ikos:retired "2015-02-24T12:00:00+00:00"^^xsd:dateTime ;
	skos:exactMatch subj:15047003 ;
	skos:exactMatch <https://www.wikidata.org/entity/Q507520> ;
	skos:broader	medtop:20001026 .

medtop:20001034
	rdf:type skos:Concept ;
	skos:prefLabel	"single sculls"@en-GB ;
	skos:definition	"Single person boats with two oars"@en-GB ;
	skos:inScheme <http://cv.iptc.org/newscodes/mediatopic/>  ;
	ikos:created "2009-10-22T02:00:00+00:00"^^xsd:dateTime ;
	dct:created "2009-10-22T02:00:00+00:00"^^xsd:dateTime ;
	ikos:modified "2021-12-21T12:00:00+00:00"^^xsd:dateTime ;
	dct:modified "2021-12-21T12:00:00+00:00"^^xsd:dateTime  ; 
	ikos:retired "2015-02-24T12:00:00+00:00"^^xsd:dateTime ;
	skos:exactMatch subj:15047001 ;
	skos:exactMatch <https://www.wikidata.org/entity/Q1307021> ;
	skos:broader	medtop:20001026 .

medtop:20001035
	rdf:type skos:Concept ;
	skos:prefLabel	"rugby league"@en-GB ;
	skos:definition	"A type of rugby where two teams of 13 compete on a pitch by running with and passing an oval ball. Points are scored by touching down the ball behind the goal line or kicking it between goal posts. Governed by Rugby League International Federation."@en-GB ;
	skos:changeNote	"2016-04-05: Broader concept changed, definition slightly modified."@en-GB ;
	skos:inScheme <http://cv.iptc.org/newscodes/mediatopic/>  ;
	ikos:created "2009-10-22T02:00:00+00:00"^^xsd:dateTime ;
	dct:created "2009-10-22T02:00:00+00:00"^^xsd:dateTime ;
	ikos:modified "2021-07-12T12:00:00+00:00"^^xsd:dateTime ;
	dct:modified "2021-07-12T12:00:00+00:00"^^xsd:dateTime  ;
	skos:exactMatch subj:15048000 ;
	skos:exactMatch <https://www.wikidata.org/entity/Q10962> ;
	skos:broader	medtop:20001176 .

medtop:20001036
	rdf:type skos:Concept ;
	skos:prefLabel	"rugby union"@en-GB ;
	skos:definition	"A type of rugby where two teams of 15 compete on a pitch by running with and passing an oval ball. Points are scored by touching down the ball behind the goal line or kicking it between goal posts. Governed by the World Rugby organization."@en-GB ;
	skos:changeNote	"2016-04-05: Broader concept changed, definition slightly modified."@en-GB ;
	skos:inScheme <http://cv.iptc.org/newscodes/mediatopic/>  ;
	ikos:created "2009-10-22T02:00:00+00:00"^^xsd:dateTime ;
	dct:created "2009-10-22T02:00:00+00:00"^^xsd:dateTime ;
	ikos:modified "2021-02-18T12:00:00+00:00"^^xsd:dateTime ;
	dct:modified "2021-02-18T12:00:00+00:00"^^xsd:dateTime  ;
	skos:exactMatch subj:15049000 ;
	skos:exactMatch <https://www.wikidata.org/entity/Q5849> ;
	skos:broader	medtop:20001176 .

medtop:20001037
	rdf:type skos:Concept ;
	skos:prefLabel	"rugby sevens"@en-GB ;
	skos:definition	"A type of rugby union where two teams of 7 compete on a pitch by running with and passing an oval ball. Points are scored by touching down the ball behind the goal line or kicking it between goal posts. Governed by the World Rugby organization."@en-GB ;
	skos:changeNote	"2016-04-05: Broader concept changed, definition slightly modified."@en-GB ;
	skos:inScheme <http://cv.iptc.org/newscodes/mediatopic/>  ;
	ikos:created "2009-10-22T02:00:00+00:00"^^xsd:dateTime ;
	dct:created "2009-10-22T02:00:00+00:00"^^xsd:dateTime ;
	ikos:modified "2021-07-12T12:00:00+00:00"^^xsd:dateTime ;
	dct:modified "2021-07-12T12:00:00+00:00"^^xsd:dateTime  ;
	skos:exactMatch subj:15049001 ;
	skos:exactMatch <https://www.wikidata.org/entity/Q270102> ;
	skos:broader	medtop:20001176 .

medtop:20001038
	rdf:type skos:Concept ;
	skos:prefLabel	"sailing"@en-GB ;
	skos:definition	"Sailing boat racing over a route"@en-GB ;
	skos:inScheme <http://cv.iptc.org/newscodes/mediatopic/>  ;
	ikos:created "2009-10-22T02:00:00+00:00"^^xsd:dateTime ;
	dct:created "2009-10-22T02:00:00+00:00"^^xsd:dateTime ;
	ikos:modified "2021-02-18T12:00:00+00:00"^^xsd:dateTime ;
	dct:modified "2021-02-18T12:00:00+00:00"^^xsd:dateTime  ;
	ikos:hasFacet aspfacet:sailingtype ;
	skos:exactMatch subj:15050000 ;
	skos:exactMatch <https://www.wikidata.org/entity/Q14085739> ;
	skos:broader	medtop:20000822 ;
	skos:narrower	medtop:20001039 ;
	skos:narrower	medtop:20001040 ;
	skos:narrower	medtop:20001041 ;
	skos:narrower	medtop:20001042 ;
	skos:narrower	medtop:20001043 ;
	skos:narrower	medtop:20001044 ;
	skos:narrower	medtop:20001045 ;
	skos:narrower	medtop:20001046 .

medtop:20001039
	rdf:type skos:Concept ;
	skos:prefLabel	"multihull"@en-GB ;
	skos:definition	"Sailing boats with multiple hulls"@en-GB ;
	skos:note	"Retired. Use Media Topic sailing + sports facet sailingtype."@en-GB ;
	skos:inScheme <http://cv.iptc.org/newscodes/mediatopic/>  ;
	ikos:created "2009-10-22T02:00:00+00:00"^^xsd:dateTime ;
	dct:created "2009-10-22T02:00:00+00:00"^^xsd:dateTime ;
	ikos:modified "2021-05-05T12:00:00+00:00"^^xsd:dateTime ;
	dct:modified "2021-05-05T12:00:00+00:00"^^xsd:dateTime  ; 
	ikos:retired "2017-07-04T12:00:00+00:00"^^xsd:dateTime ;
	skos:exactMatch subj:15050014 ;
	skos:exactMatch <https://www.wikidata.org/entity/Q1642862> ;
	skos:broader	medtop:20001038 .

medtop:20001040
	rdf:type skos:Concept ;
	skos:prefLabel	"dinghy"@en-GB ;
	skos:definition	"Single hulled vessel without a fixed keel"@en-GB ;
	skos:note	"Retired. Use Media Topic sailing + sports facet sailingtype."@en-GB ;
	skos:inScheme <http://cv.iptc.org/newscodes/mediatopic/>  ;
	ikos:created "2009-10-22T02:00:00+00:00"^^xsd:dateTime ;
	dct:created "2009-10-22T02:00:00+00:00"^^xsd:dateTime ;
	ikos:modified "2021-02-18T12:00:00+00:00"^^xsd:dateTime ;
	dct:modified "2021-02-18T12:00:00+00:00"^^xsd:dateTime  ; 
	ikos:retired "2017-07-04T12:00:00+00:00"^^xsd:dateTime ;
	skos:broadMatch subj:15050013 ;
	skos:exactMatch <https://www.wikidata.org/entity/Q5278203> ;
	skos:broader	medtop:20001038 .

medtop:20001041
	rdf:type skos:Concept ;
	skos:prefLabel	"keelboat"@en-GB ;
	skos:definition	"Single hulled vessel with a fixed keel"@en-GB ;
	skos:note	"Retired. Use Media Topic sailing + sports facet sailingtype."@en-GB ;
	skos:inScheme <http://cv.iptc.org/newscodes/mediatopic/>  ;
	ikos:created "2009-10-22T02:00:00+00:00"^^xsd:dateTime ;
	dct:created "2009-10-22T02:00:00+00:00"^^xsd:dateTime ;
	ikos:modified "2021-05-05T12:00:00+00:00"^^xsd:dateTime ;
	dct:modified "2021-05-05T12:00:00+00:00"^^xsd:dateTime  ; 
	ikos:retired "2017-07-04T12:00:00+00:00"^^xsd:dateTime ;
	skos:broadMatch subj:15050013 ;
	skos:exactMatch <https://www.wikidata.org/entity/Q474161> ;
	skos:broader	medtop:20001038 .

medtop:20001042
	rdf:type skos:Concept ;
	skos:prefLabel	"sailing regatta"@en-GB ;
	skos:definition	"Sailing event"@en-GB ;
	skos:note	"Retired. Use Media Topic sailing + sports facet sailingtype."@en-GB ;
	skos:inScheme <http://cv.iptc.org/newscodes/mediatopic/>  ;
	ikos:created "2009-10-22T02:00:00+00:00"^^xsd:dateTime ;
	dct:created "2009-10-22T02:00:00+00:00"^^xsd:dateTime ;
	ikos:modified "2021-05-05T12:00:00+00:00"^^xsd:dateTime ;
	dct:modified "2021-05-05T12:00:00+00:00"^^xsd:dateTime  ; 
	ikos:retired "2017-07-04T12:00:00+00:00"^^xsd:dateTime ;
	skos:broadMatch subj:15050000 ;
	skos:exactMatch <https://www.wikidata.org/entity/Q126701> ;
	skos:broader	medtop:20001038 .

medtop:20001043
	rdf:type skos:Concept ;
	skos:prefLabel	"ocean sailing"@en-GB ;
	skos:definition	"Sailing vessels across oceans as part of a competitive race."@en-GB ;
	skos:note	"Retired. Use Media Topic sailing + sports facet sailingtype."@en-GB ;
	skos:inScheme <http://cv.iptc.org/newscodes/mediatopic/>  ;
	ikos:created "2009-10-22T02:00:00+00:00"^^xsd:dateTime ;
	dct:created "2009-10-22T02:00:00+00:00"^^xsd:dateTime ;
	ikos:modified "2021-05-05T12:00:00+00:00"^^xsd:dateTime ;
	dct:modified "2021-05-05T12:00:00+00:00"^^xsd:dateTime  ; 
	ikos:retired "2017-07-04T12:00:00+00:00"^^xsd:dateTime ;
	skos:broadMatch subj:15050000 ;
	skos:exactMatch <https://www.wikidata.org/entity/Q8046440> ;
	skos:broader	medtop:20001038 .

medtop:20001044
	rdf:type skos:Concept ;
	skos:prefLabel	"round the world race"@en-GB ;
	skos:definition	"Sailing vessels around the world as a race"@en-GB ;
	skos:note	"Retired. Use Media Topic sailing + sports facet sailingtype."@en-GB ;
	skos:inScheme <http://cv.iptc.org/newscodes/mediatopic/>  ;
	ikos:created "2009-10-22T02:00:00+00:00"^^xsd:dateTime ;
	dct:created "2009-10-22T02:00:00+00:00"^^xsd:dateTime ;
	ikos:modified "2021-05-05T12:00:00+00:00"^^xsd:dateTime ;
	dct:modified "2021-05-05T12:00:00+00:00"^^xsd:dateTime  ; 
	ikos:retired "2017-07-04T12:00:00+00:00"^^xsd:dateTime ;
	skos:exactMatch subj:15050012 ;
	skos:exactMatch <https://www.wikidata.org/entity/Q3422424> ;
	skos:broader	medtop:20001038 .

medtop:20001045
	rdf:type skos:Concept ;
	skos:prefLabel	"solo ocean sailing"@en-GB ;
	skos:definition	"Sailing oceans as an individual, as part of a race."@en-GB ;
	skos:note	"Retired. Use Media Topic sailing + sports facet sailingtype."@en-GB ;
	skos:inScheme <http://cv.iptc.org/newscodes/mediatopic/>  ;
	ikos:created "2009-10-22T02:00:00+00:00"^^xsd:dateTime ;
	dct:created "2009-10-22T02:00:00+00:00"^^xsd:dateTime ;
	ikos:modified "2021-05-05T12:00:00+00:00"^^xsd:dateTime ;
	dct:modified "2021-05-05T12:00:00+00:00"^^xsd:dateTime  ; 
	ikos:retired "2017-07-04T12:00:00+00:00"^^xsd:dateTime ;
	skos:broadMatch subj:15050000 ;
	skos:exactMatch <https://www.wikidata.org/entity/Q1307611> ;
	skos:broader	medtop:20001038 .

medtop:20001046
	rdf:type skos:Concept ;
	skos:prefLabel	"non-stop solo race"@en-GB ;
	skos:definition	"Races either clockwise or anti clockwise around the globe without stopping at any ports between start and finish of race."@en-GB ;
	skos:note	"Retired. Use Media Topic sailing + sports facet sailingtype."@en-GB ;
	skos:inScheme <http://cv.iptc.org/newscodes/mediatopic/>  ;
	ikos:created "2009-10-22T02:00:00+00:00"^^xsd:dateTime ;
	dct:created "2009-10-22T02:00:00+00:00"^^xsd:dateTime ;
	ikos:modified "2021-02-18T12:00:00+00:00"^^xsd:dateTime ;
	dct:modified "2021-02-18T12:00:00+00:00"^^xsd:dateTime  ; 
	ikos:retired "2017-07-04T12:00:00+00:00"^^xsd:dateTime ;
	skos:broadMatch subj:15050012 ;
	skos:broader	medtop:20001038 .

medtop:20001047
	rdf:type skos:Concept ;
	skos:prefLabel	"sepak takraw"@en-GB ;
	skos:definition	"A game like volleyball where hands must not be used, using a ball made of rattan"@en-GB ;
	skos:inScheme <http://cv.iptc.org/newscodes/mediatopic/>  ;
	ikos:created "2009-10-22T02:00:00+00:00"^^xsd:dateTime ;
	dct:created "2009-10-22T02:00:00+00:00"^^xsd:dateTime ;
	ikos:modified "2021-02-18T12:00:00+00:00"^^xsd:dateTime ;
	dct:modified "2021-02-18T12:00:00+00:00"^^xsd:dateTime  ;
	skos:exactMatch subj:15098000 ;
	skos:exactMatch <https://www.wikidata.org/entity/Q188818> ;
	skos:broader	medtop:20000822 .

medtop:20001048
	rdf:type skos:Concept ;
	skos:prefLabel	"shinty"@en-GB ;
	skos:definition	"A ball game involving 2 teams with curved sticks called camans. The object is to score goals by hitting the small leather ball through the goals."@en-GB ;
	skos:inScheme <http://cv.iptc.org/newscodes/mediatopic/>  ;
	ikos:created "2009-10-22T02:00:00+00:00"^^xsd:dateTime ;
	dct:created "2009-10-22T02:00:00+00:00"^^xsd:dateTime ;
	ikos:modified "2021-02-18T12:00:00+00:00"^^xsd:dateTime ;
	dct:modified "2021-02-18T12:00:00+00:00"^^xsd:dateTime  ;
	skos:broadMatch subj:15000000 ;
	skos:exactMatch <https://www.wikidata.org/entity/Q850256> ;
	skos:broader	medtop:20000822 .

medtop:20001049
	rdf:type skos:Concept ;
	skos:prefLabel	"sport shooting"@en-GB ;
	skos:definition	"Precision sport using a hand gun, rifle or shotgun"@en-GB ;
	skos:inScheme <http://cv.iptc.org/newscodes/mediatopic/>  ;
	ikos:created "2009-10-22T02:00:00+00:00"^^xsd:dateTime ;
	dct:created "2009-10-22T02:00:00+00:00"^^xsd:dateTime ;
	ikos:modified "2023-10-02T12:00:00+00:00"^^xsd:dateTime ;
	dct:modified "2023-10-02T12:00:00+00:00"^^xsd:dateTime  ;
	skos:exactMatch subj:15051000 ;
	ikos:hasFacet aspfacet:shootingtype ;
	skos:exactMatch <https://www.wikidata.org/entity/Q206989> ;
	skos:broader	medtop:20000822 ;
	skos:narrower	medtop:20001050 ;
	skos:narrower	medtop:20001051 ;
	skos:narrower	medtop:20001052 ;
	skos:narrower	medtop:20001053 ;
	skos:narrower	medtop:20001054 .

medtop:20001050
	rdf:type skos:Concept ;
	skos:prefLabel	"pistol shooting"@en-GB ;
	skos:definition	"Shooting event using a pistol"@en-GB ;
	skos:note	"Retired. Use Media Topic sport shooting + sports facet shootingtype."@en-GB ;
	skos:inScheme <http://cv.iptc.org/newscodes/mediatopic/>  ;
	ikos:created "2009-10-22T02:00:00+00:00"^^xsd:dateTime ;
	dct:created "2009-10-22T02:00:00+00:00"^^xsd:dateTime ;
	ikos:modified "2021-02-18T12:00:00+00:00"^^xsd:dateTime ;
	dct:modified "2021-02-18T12:00:00+00:00"^^xsd:dateTime  ; 
	ikos:retired "2017-07-04T12:00:00+00:00"^^xsd:dateTime ;
	skos:broadMatch subj:15051001 ;
	skos:exactMatch <https://www.wikidata.org/entity/Q4632203> ;
	skos:broader	medtop:20001049 .

medtop:20001051
	rdf:type skos:Concept ;
	skos:prefLabel	"rifle shooting"@en-GB ;
	skos:definition	"Shooting event using a rifle"@en-GB ;
	skos:note	"Retired. Use Media Topic sport shooting + sports facet shootingtype."@en-GB ;
	skos:inScheme <http://cv.iptc.org/newscodes/mediatopic/>  ;
	ikos:created "2009-10-22T02:00:00+00:00"^^xsd:dateTime ;
	dct:created "2009-10-22T02:00:00+00:00"^^xsd:dateTime ;
	ikos:modified "2021-05-05T12:00:00+00:00"^^xsd:dateTime ;
	dct:modified "2021-05-05T12:00:00+00:00"^^xsd:dateTime  ; 
	ikos:retired "2017-07-04T12:00:00+00:00"^^xsd:dateTime ;
	skos:broadMatch subj:15051002 ;
	skos:exactMatch <https://www.wikidata.org/entity/Q69387590> ;
	skos:broader	medtop:20001049 .

medtop:20001052
	rdf:type skos:Concept ;
	skos:prefLabel	"running target shooting"@en-GB ;
	skos:definition	"Shooting event with an airgun and a target that moves sideways"@en-GB ;
	skos:note	"Retired. Use Media Topic sport shooting + sports facet shootingtype."@en-GB ;
	skos:inScheme <http://cv.iptc.org/newscodes/mediatopic/>  ;
	ikos:created "2009-10-22T02:00:00+00:00"^^xsd:dateTime ;
	dct:created "2009-10-22T02:00:00+00:00"^^xsd:dateTime ;
	ikos:modified "2021-05-05T12:00:00+00:00"^^xsd:dateTime ;
	dct:modified "2021-05-05T12:00:00+00:00"^^xsd:dateTime  ; 
	ikos:retired "2017-07-04T12:00:00+00:00"^^xsd:dateTime ;
	skos:broadMatch subj:15051003 ;
	skos:exactMatch <https://www.wikidata.org/entity/Q40679812> ;
	skos:broader	medtop:20001049 .

medtop:20001053
	rdf:type skos:Concept ;
	skos:prefLabel	"shotgun shooting"@en-GB ;
	skos:definition	"Shooting event using a shotgun"@en-GB ;
	skos:note	"Retired. Use Media Topic sport shooting + sports facet shootingtype."@en-GB ;
	skos:inScheme <http://cv.iptc.org/newscodes/mediatopic/>  ;
	ikos:created "2009-10-22T02:00:00+00:00"^^xsd:dateTime ;
	dct:created "2009-10-22T02:00:00+00:00"^^xsd:dateTime ;
	ikos:modified "2021-05-05T12:00:00+00:00"^^xsd:dateTime ;
	dct:modified "2021-05-05T12:00:00+00:00"^^xsd:dateTime  ; 
	ikos:retired "2017-07-04T12:00:00+00:00"^^xsd:dateTime ;
	skos:broadMatch subj:15051004 ;
	skos:exactMatch <https://www.wikidata.org/entity/Q96293020> ;
	skos:broader	medtop:20001049 .

medtop:20001054
	rdf:type skos:Concept ;
	skos:prefLabel	"clay pigeon shooting"@en-GB ;
	skos:definition	"Shooting event which involves shooting at special flying targets, known as clay pigeons or clay targets"@en-GB ;
	skos:note	"Retired. Use Media Topic sport shooting + sports facet shootingtype."@en-GB ;
	skos:inScheme <http://cv.iptc.org/newscodes/mediatopic/>  ;
	ikos:created "2009-10-22T02:00:00+00:00"^^xsd:dateTime ;
	dct:created "2009-10-22T02:00:00+00:00"^^xsd:dateTime ;
	ikos:modified "2021-05-05T12:00:00+00:00"^^xsd:dateTime ;
	dct:modified "2021-05-05T12:00:00+00:00"^^xsd:dateTime  ; 
	ikos:retired "2017-07-04T12:00:00+00:00"^^xsd:dateTime ;
	skos:broadMatch subj:15051005 ;
	skos:exactMatch <https://www.wikidata.org/entity/Q5130059> ;
	skos:broader	medtop:20001049 .

medtop:20001055
	rdf:type skos:Concept ;
	skos:prefLabel	"skeleton"@en-GB ;
	skos:definition	"In skeleton the competitor lies on his/her stomach when racing down the course. The competitor must be on the sled when crossing the finishing line."@en-GB ;
	skos:inScheme <http://cv.iptc.org/newscodes/mediatopic/>  ;
	ikos:created "2009-10-22T02:00:00+00:00"^^xsd:dateTime ;
	dct:created "2009-10-22T02:00:00+00:00"^^xsd:dateTime ;
	ikos:modified "2021-02-18T12:00:00+00:00"^^xsd:dateTime ;
	dct:modified "2021-02-18T12:00:00+00:00"^^xsd:dateTime  ;
	skos:exactMatch subj:15083000 ;
	skos:exactMatch <https://www.wikidata.org/entity/Q186190> ;
	skos:broader	medtop:20000822 .

medtop:20001056
	rdf:type skos:Concept ;
	skos:prefLabel	"skiing"@en-GB ;
	skos:definition	"A winter sport using different types of skis"@en-GB ;
	skos:inScheme <http://cv.iptc.org/newscodes/mediatopic/>  ;
	ikos:created "2009-10-22T02:00:00+00:00"^^xsd:dateTime ;
	dct:created "2009-10-22T02:00:00+00:00"^^xsd:dateTime ;
	ikos:modified "2021-02-18T12:00:00+00:00"^^xsd:dateTime ;
	dct:modified "2021-02-18T12:00:00+00:00"^^xsd:dateTime  ;
	skos:broadMatch subj:15000000 ;
	skos:exactMatch <https://www.wikidata.org/entity/Q130949> ;
	skos:broader	medtop:20000822 ;
	skos:narrower	medtop:20001057 ;
	skos:narrower	medtop:20001058 ;
	skos:narrower	medtop:20001059 ;
	skos:narrower	medtop:20001060 ;
	skos:narrower	medtop:20001061 ;
	skos:narrower	medtop:20001149 ;
	skos:narrower	medtop:20001150 ;
	skos:narrower	medtop:20001153 .

medtop:20001057
	rdf:type skos:Concept ;
	skos:prefLabel	"alpine skiing"@en-GB ;
	skos:definition	"Racing downhill on snow-covered slopes using alpine techniques and equipment. The slopes contain intermediate gates which are spaced according to the discipline involved."@en-GB ;
	skos:inScheme <http://cv.iptc.org/newscodes/mediatopic/>  ;
	ikos:created "2009-10-22T02:00:00+00:00"^^xsd:dateTime ;
	dct:created "2009-10-22T02:00:00+00:00"^^xsd:dateTime ;
	ikos:modified "2021-02-18T12:00:00+00:00"^^xsd:dateTime ;
	dct:modified "2021-02-18T12:00:00+00:00"^^xsd:dateTime  ;
	skos:exactMatch subj:15002000 ;
	ikos:hasFacet aspfacet:alpineskiingtype ;
	skos:exactMatch <https://www.wikidata.org/entity/Q186222> ;
	skos:broader	medtop:20001056 .

medtop:20001058
	rdf:type skos:Concept ;
	skos:prefLabel	"freestyle skiing"@en-GB ;
	skos:definition	"Skiing competitions which, in contrast to alpine skiing, incorporate acrobatic moves and jumps. Events include aerials, halfpipe, slopestyle, ski cross, moguls and big air."@en-GB ;
	skos:inScheme <http://cv.iptc.org/newscodes/mediatopic/>  ;
	ikos:created "2009-10-22T02:00:00+00:00"^^xsd:dateTime ;
	dct:created "2009-10-22T02:00:00+00:00"^^xsd:dateTime ;
	ikos:modified "2022-02-03T12:00:00+00:00"^^xsd:dateTime ;
	dct:modified "2022-02-03T12:00:00+00:00"^^xsd:dateTime  ;
	ikos:hasFacet aspfacet:freestyleskiingtype ;
	skos:exactMatch subj:15026000 ;
	skos:exactMatch <https://www.wikidata.org/entity/Q189472> ;
	skos:broader	medtop:20001056 .

medtop:20001059
	rdf:type skos:Concept ;
	skos:prefLabel	"grass skiing"@en-GB ;
	skos:definition	"Alpine skiing on roller skis and grass"@en-GB ;
	skos:inScheme <http://cv.iptc.org/newscodes/mediatopic/>  ;
	ikos:created "2009-10-22T02:00:00+00:00"^^xsd:dateTime ;
	dct:created "2009-10-22T02:00:00+00:00"^^xsd:dateTime ;
	ikos:modified "2021-02-18T12:00:00+00:00"^^xsd:dateTime ;
	dct:modified "2021-02-18T12:00:00+00:00"^^xsd:dateTime  ;
	skos:exactMatch subj:15090000 ;
	skos:exactMatch <https://www.wikidata.org/entity/Q637186> ;
	skos:broader	medtop:20001056 .

medtop:20001060
	rdf:type skos:Concept ;
	skos:prefLabel	"Nordic skiing"@en-GB ;
	skos:definition	"Practiced in relatively-flat, snowy countryside and based on power and endurance."@en-GB ;
	skos:inScheme <http://cv.iptc.org/newscodes/mediatopic/>  ;
	ikos:created "2009-10-22T02:00:00+00:00"^^xsd:dateTime ;
	dct:created "2009-10-22T02:00:00+00:00"^^xsd:dateTime ;
	ikos:modified "2021-02-18T12:00:00+00:00"^^xsd:dateTime ;
	dct:modified "2021-02-18T12:00:00+00:00"^^xsd:dateTime  ; 
	ikos:retired "2019-08-01T12:00:00+00:00"^^xsd:dateTime ;
	ikos:hasFacet aspfacet:nordicskiingtype ;
	skos:exactMatch subj:15043000 ;
	skos:exactMatch <https://www.wikidata.org/entity/Q216613> ;
	skos:broader	medtop:20001056 .

medtop:20001061
	rdf:type skos:Concept ;
	skos:prefLabel	"ski jumping"@en-GB ;
	skos:definition	"Competitors descend a snow covered elevated ramp on skis and try to fly off it as far as possible, receiving marks for distance, style of flight and landing"@en-GB ;
	skos:inScheme <http://cv.iptc.org/newscodes/mediatopic/>  ;
	ikos:created "2009-10-22T02:00:00+00:00"^^xsd:dateTime ;
	dct:created "2009-10-22T02:00:00+00:00"^^xsd:dateTime ;
	ikos:modified "2021-02-18T12:00:00+00:00"^^xsd:dateTime ;
	dct:modified "2021-02-18T12:00:00+00:00"^^xsd:dateTime  ;
	skos:exactMatch subj:15052000 ;
	skos:exactMatch <https://www.wikidata.org/entity/Q7718> ;
	skos:broader	medtop:20001056 .

medtop:20001062
	rdf:type skos:Concept ;
	skos:prefLabel	"sky diving"@en-GB ;
	skos:definition	"Parachuting competitions with long distance falls without using a parachute"@en-GB ;
	skos:inScheme <http://cv.iptc.org/newscodes/mediatopic/>  ;
	ikos:created "2009-10-22T02:00:00+00:00"^^xsd:dateTime ;
	dct:created "2009-10-22T02:00:00+00:00"^^xsd:dateTime ;
	ikos:modified "2021-02-18T12:00:00+00:00"^^xsd:dateTime ;
	dct:modified "2021-02-18T12:00:00+00:00"^^xsd:dateTime  ;
	skos:exactMatch subj:15001002 ;
	skos:exactMatch <https://www.wikidata.org/entity/Q193210> ;
	skos:broader	medtop:20000822 .

medtop:20001063
	rdf:type skos:Concept ;
	skos:prefLabel	"snooker"@en-GB ;
	skos:definition	"A cue sport with balls on a table to be potted in a specific order"@en-GB ;
	skos:inScheme <http://cv.iptc.org/newscodes/mediatopic/>  ;
	ikos:created "2009-10-22T02:00:00+00:00"^^xsd:dateTime ;
	dct:created "2009-10-22T02:00:00+00:00"^^xsd:dateTime ;
	ikos:modified "2021-02-18T12:00:00+00:00"^^xsd:dateTime ;
	dct:modified "2021-02-18T12:00:00+00:00"^^xsd:dateTime  ;
	skos:exactMatch subj:15010006 ;
	ikos:hasFacet aspfacet:billiardtype ;
	skos:exactMatch <https://www.wikidata.org/entity/Q11015> ;
	skos:broader	medtop:20000822 .

medtop:20001064
	rdf:type skos:Concept ;
	skos:prefLabel	"snowboarding"@en-GB ;
	skos:definition	"Practiced with a single board (rather than two skis)"@en-GB ;
	skos:inScheme <http://cv.iptc.org/newscodes/mediatopic/>  ;
	ikos:created "2009-10-22T02:00:00+00:00"^^xsd:dateTime ;
	dct:created "2009-10-22T02:00:00+00:00"^^xsd:dateTime ;
	ikos:modified "2021-02-18T12:00:00+00:00"^^xsd:dateTime ;
	dct:modified "2021-02-18T12:00:00+00:00"^^xsd:dateTime  ;
	ikos:hasFacet aspfacet:snowboardingtype ;
	skos:exactMatch subj:15053000 ;
	skos:exactMatch <https://www.wikidata.org/entity/Q178131> ;
	skos:broader	medtop:20000822 .

medtop:20001065
	rdf:type skos:Concept ;
	skos:prefLabel	"soccer"@en-GB ;
	skos:definition	"A form of football played by two teams competing on a pitch by kicking a spherical ball. Points are scored by kicking or heading the ball into a goal. Governed by the Fédération Internationale de Football Association"@en-GB ;
	skos:changeNote	"2016-04-06: definition rephrased."@en-GB ;
	skos:inScheme <http://cv.iptc.org/newscodes/mediatopic/>  ;
	ikos:created "2009-10-22T02:00:00+00:00"^^xsd:dateTime ;
	dct:created "2009-10-22T02:00:00+00:00"^^xsd:dateTime ;
	ikos:modified "2021-02-18T12:00:00+00:00"^^xsd:dateTime ;
	dct:modified "2021-02-18T12:00:00+00:00"^^xsd:dateTime  ;
	skos:exactMatch subj:15054000 ;
	skos:exactMatch <https://www.wikidata.org/entity/Q2736> ;
	skos:broader	medtop:20000822 .

medtop:20001066
	rdf:type skos:Concept ;
	skos:prefLabel	"softball"@en-GB ;
	skos:definition	"Similar to baseball but with a larger and softer ball, a thinner bat, shorter gaps between bases and less innings"@en-GB ;
	skos:inScheme <http://cv.iptc.org/newscodes/mediatopic/>  ;
	ikos:created "2009-10-22T02:00:00+00:00"^^xsd:dateTime ;
	dct:created "2009-10-22T02:00:00+00:00"^^xsd:dateTime ;
	ikos:modified "2021-02-18T12:00:00+00:00"^^xsd:dateTime ;
	dct:modified "2021-02-18T12:00:00+00:00"^^xsd:dateTime  ;
	skos:exactMatch subj:15055000 ;
	skos:exactMatch <https://www.wikidata.org/entity/Q171038> ;
	skos:broader	medtop:20000822 .

medtop:20001067
	rdf:type skos:Concept ;
	skos:prefLabel	"speed skating"@en-GB ;
	skos:definition	"Timed races competed by two or more skaters at a time on an oval ice track"@en-GB ;
	skos:inScheme <http://cv.iptc.org/newscodes/mediatopic/>  ;
	ikos:created "2009-10-22T02:00:00+00:00"^^xsd:dateTime ;
	dct:created "2009-10-22T02:00:00+00:00"^^xsd:dateTime ;
	ikos:modified "2021-03-31T12:00:00+00:00"^^xsd:dateTime ;
	dct:modified "2021-03-31T12:00:00+00:00"^^xsd:dateTime  ;
	skos:exactMatch subj:15056000 ;
	skos:exactMatch <https://www.wikidata.org/entity/Q192431> ;
	skos:broader	medtop:20000822 .

medtop:20001068
	rdf:type skos:Concept ;
	skos:prefLabel	"squash"@en-GB ;
	skos:definition	"A racquet sport of strategy and endurance played by singles or doubles teams in a walled court with a small rubber ball"@en-GB ;
	skos:inScheme <http://cv.iptc.org/newscodes/mediatopic/>  ;
	ikos:created "2009-10-22T02:00:00+00:00"^^xsd:dateTime ;
	dct:created "2009-10-22T02:00:00+00:00"^^xsd:dateTime ;
	ikos:modified "2021-02-18T12:00:00+00:00"^^xsd:dateTime ;
	dct:modified "2021-02-18T12:00:00+00:00"^^xsd:dateTime  ;
	skos:exactMatch subj:15059000 ;
	skos:exactMatch <https://www.wikidata.org/entity/Q133201> ;
	skos:broader	medtop:20000822 .

medtop:20001069
	rdf:type skos:Concept ;
	skos:prefLabel	"sumo wrestling"@en-GB ;
	skos:definition	"A combat sport of speed and rapidity with much ceremony where two contestants try to throw or slap a competitor out of a marked area. Generally practiced in Japan by large men."@en-GB ;
	skos:inScheme <http://cv.iptc.org/newscodes/mediatopic/>  ;
	ikos:created "2009-10-22T02:00:00+00:00"^^xsd:dateTime ;
	dct:created "2009-10-22T02:00:00+00:00"^^xsd:dateTime ;
	ikos:modified "2021-02-18T12:00:00+00:00"^^xsd:dateTime ;
	dct:modified "2021-02-18T12:00:00+00:00"^^xsd:dateTime  ;
	skos:exactMatch subj:15060000 ;
	skos:exactMatch <https://www.wikidata.org/entity/Q40561> ;
	skos:broader	medtop:20000822 .

medtop:20001070
	rdf:type skos:Concept ;
	skos:prefLabel	"surfing"@en-GB ;
	skos:definition	"Water sport where contestants catch and ride waves upright on a surfboard"@en-GB ;
	skos:inScheme <http://cv.iptc.org/newscodes/mediatopic/>  ;
	ikos:created "2009-10-22T02:00:00+00:00"^^xsd:dateTime ;
	dct:created "2009-10-22T02:00:00+00:00"^^xsd:dateTime ;
	ikos:modified "2021-02-18T12:00:00+00:00"^^xsd:dateTime ;
	dct:modified "2021-02-18T12:00:00+00:00"^^xsd:dateTime  ;
	skos:exactMatch subj:15061000 ;
	skos:exactMatch <https://www.wikidata.org/entity/Q159992> ;
	skos:broader	medtop:20000822 .

medtop:20001071
	rdf:type skos:Concept ;
	skos:prefLabel	"swimming"@en-GB ;
	skos:definition	"A water sport where contestants swim as fast as possible in a given style and win races by being the first to touch home"@en-GB ;
	skos:inScheme <http://cv.iptc.org/newscodes/mediatopic/>  ;
	ikos:created "2009-10-22T02:00:00+00:00"^^xsd:dateTime ;
	dct:created "2009-10-22T02:00:00+00:00"^^xsd:dateTime ;
	ikos:modified "2021-02-18T12:00:00+00:00"^^xsd:dateTime ;
	dct:modified "2021-02-18T12:00:00+00:00"^^xsd:dateTime  ;
	ikos:hasFacet aspfacet:swimmingtype ;
	skos:exactMatch subj:15062000 ;
	skos:exactMatch <https://www.wikidata.org/entity/Q31920> ;
	skos:broader	medtop:20000822 ;
	skos:narrower	medtop:20001072 ;
	skos:narrower	medtop:20001073 ;
	skos:narrower	medtop:20001074 ;
	skos:narrower	medtop:20001075 ;
	skos:narrower	medtop:20001076 ;
	skos:narrower	medtop:20001077 ;
	skos:narrower	medtop:20001078 ;
	skos:narrower	medtop:20001079 ;
	skos:narrower	medtop:20001080 .

medtop:20001072
	rdf:type skos:Concept ;
	skos:prefLabel	"backstroke"@en-GB ;
	skos:definition	"Swimming style, on the back, legs move in flapping motion whilst arms propel the swimmer forward"@en-GB ;
	skos:inScheme <http://cv.iptc.org/newscodes/mediatopic/>  ;
	ikos:created "2009-10-22T02:00:00+00:00"^^xsd:dateTime ;
	dct:created "2009-10-22T02:00:00+00:00"^^xsd:dateTime ;
	ikos:modified "2021-12-21T12:00:00+00:00"^^xsd:dateTime ;
	dct:modified "2021-12-21T12:00:00+00:00"^^xsd:dateTime  ; 
	ikos:retired "2015-02-24T12:00:00+00:00"^^xsd:dateTime ;
	skos:broadMatch subj:15062000 ;
	skos:exactMatch <https://www.wikidata.org/entity/Q275115> ;
	skos:broader	medtop:20001071 .

medtop:20001073
	rdf:type skos:Concept ;
	skos:prefLabel	"breaststroke"@en-GB ;
	skos:definition	"Swimming style , on the front, effecting forward and outward push movements with the arms and backward and outward pushes with the legs"@en-GB ;
	skos:inScheme <http://cv.iptc.org/newscodes/mediatopic/>  ;
	ikos:created "2009-10-22T02:00:00+00:00"^^xsd:dateTime ;
	dct:created "2009-10-22T02:00:00+00:00"^^xsd:dateTime ;
	ikos:modified "2021-12-21T12:00:00+00:00"^^xsd:dateTime ;
	dct:modified "2021-12-21T12:00:00+00:00"^^xsd:dateTime  ; 
	ikos:retired "2015-02-24T12:00:00+00:00"^^xsd:dateTime ;
	skos:broadMatch subj:15062000 ;
	skos:exactMatch <https://www.wikidata.org/entity/Q326163> ;
	skos:broader	medtop:20001071 .

medtop:20001074
	rdf:type skos:Concept ;
	skos:prefLabel	"butterfly swimming"@en-GB ;
	skos:definition	"Swimming style , swum on the front with the shoulders remaining parallel to the water both arms moving in simultaneous windmill fashion, the legs remain together and are moved in a flapping motion. The most physical of all styles."@en-GB ;
	skos:inScheme <http://cv.iptc.org/newscodes/mediatopic/>  ;
	ikos:created "2009-10-22T02:00:00+00:00"^^xsd:dateTime ;
	dct:created "2009-10-22T02:00:00+00:00"^^xsd:dateTime ;
	ikos:modified "2021-12-21T12:00:00+00:00"^^xsd:dateTime ;
	dct:modified "2021-12-21T12:00:00+00:00"^^xsd:dateTime  ; 
	ikos:retired "2015-02-24T12:00:00+00:00"^^xsd:dateTime ;
	skos:broadMatch subj:15062000 ;
	skos:exactMatch <https://www.wikidata.org/entity/Q245249> ;
	skos:broader	medtop:20001071 .

medtop:20001075
	rdf:type skos:Concept ;
	skos:prefLabel	"freestyle swimming"@en-GB ;
	skos:definition	"Any swimming style may be employed, though front crawl is universally employed"@en-GB ;
	skos:inScheme <http://cv.iptc.org/newscodes/mediatopic/>  ;
	ikos:created "2009-10-22T02:00:00+00:00"^^xsd:dateTime ;
	dct:created "2009-10-22T02:00:00+00:00"^^xsd:dateTime ;
	ikos:modified "2021-12-21T12:00:00+00:00"^^xsd:dateTime ;
	dct:modified "2021-12-21T12:00:00+00:00"^^xsd:dateTime  ; 
	ikos:retired "2015-02-24T12:00:00+00:00"^^xsd:dateTime ;
	skos:closeMatch subj:15062000 ;
	skos:exactMatch <https://www.wikidata.org/entity/Q31987> ;
	skos:broader	medtop:20001071 .

medtop:20001076
	rdf:type skos:Concept ;
	skos:prefLabel	"medley swimming"@en-GB ;
	skos:definition	"A combination of four different swimming styles in one race"@en-GB ;
	skos:inScheme <http://cv.iptc.org/newscodes/mediatopic/>  ;
	ikos:created "2009-10-22T02:00:00+00:00"^^xsd:dateTime ;
	dct:created "2009-10-22T02:00:00+00:00"^^xsd:dateTime ;
	ikos:modified "2021-12-21T12:00:00+00:00"^^xsd:dateTime ;
	dct:modified "2021-12-21T12:00:00+00:00"^^xsd:dateTime  ; 
	ikos:retired "2015-02-24T12:00:00+00:00"^^xsd:dateTime ;
	skos:broadMatch subj:15062000 ;
	skos:exactMatch <https://www.wikidata.org/entity/Q657196> ;
	skos:broader	medtop:20001071 .

medtop:20001077
	rdf:type skos:Concept ;
	skos:prefLabel	"marathon swimming"@en-GB ;
	skos:definition	"A long distance open water swimming"@en-GB ;
	skos:note	"Retired in 2017 in favour of sports facet, but then un-retired in 2021 so all top-level Olympics sports have a valid Media Topics term."@en-GB ;
	skos:inScheme <http://cv.iptc.org/newscodes/mediatopic/>  ;
	ikos:created "2009-10-22T02:00:00+00:00"^^xsd:dateTime ;
	dct:created "2009-10-22T02:00:00+00:00"^^xsd:dateTime ;
	ikos:modified "2021-07-12T12:00:00+00:00"^^xsd:dateTime ;
	dct:modified "2021-07-12T12:00:00+00:00"^^xsd:dateTime  ;
	skos:broadMatch subj:15062000 ;
	skos:exactMatch <https://www.wikidata.org/entity/Q17143662> ;
	skos:broader	medtop:20001071 .

medtop:20001078
	rdf:type skos:Concept ;
	skos:prefLabel	"relay freestyle swimming"@en-GB ;
	skos:definition	"Team of swimmers swim a relay in the swimming style of their choice"@en-GB ;
	skos:inScheme <http://cv.iptc.org/newscodes/mediatopic/>  ;
	ikos:created "2009-10-22T02:00:00+00:00"^^xsd:dateTime ;
	dct:created "2009-10-22T02:00:00+00:00"^^xsd:dateTime ;
	ikos:modified "2021-12-21T12:00:00+00:00"^^xsd:dateTime ;
	dct:modified "2021-12-21T12:00:00+00:00"^^xsd:dateTime  ; 
	ikos:retired "2015-02-24T12:00:00+00:00"^^xsd:dateTime ;
	skos:broadMatch subj:15062000 ;
	skos:exactMatch <https://www.wikidata.org/entity/Q10855252> ;
	skos:broader	medtop:20001071 .

medtop:20001079
	rdf:type skos:Concept ;
	skos:prefLabel	"relay medley swimming"@en-GB ;
	skos:definition	"Team relay race involving a combination of four different swimming styles"@en-GB ;
	skos:inScheme <http://cv.iptc.org/newscodes/mediatopic/>  ;
	ikos:created "2009-10-22T02:00:00+00:00"^^xsd:dateTime ;
	dct:created "2009-10-22T02:00:00+00:00"^^xsd:dateTime ;
	ikos:modified "2021-12-21T12:00:00+00:00"^^xsd:dateTime ;
	dct:modified "2021-12-21T12:00:00+00:00"^^xsd:dateTime  ; 
	ikos:retired "2015-02-24T12:00:00+00:00"^^xsd:dateTime ;
	skos:broadMatch subj:15062000 ;
	skos:exactMatch <https://www.wikidata.org/entity/Q657196> ;
	skos:broader	medtop:20001071 .

medtop:20001080
	rdf:type skos:Concept ;
	skos:prefLabel	"short course swimming"@en-GB ;
	skos:definition	"Races competed in a 25m length pool"@en-GB ;
	skos:inScheme <http://cv.iptc.org/newscodes/mediatopic/>  ;
	ikos:created "2009-10-22T02:00:00+00:00"^^xsd:dateTime ;
	dct:created "2009-10-22T02:00:00+00:00"^^xsd:dateTime ;
	ikos:modified "2021-12-21T12:00:00+00:00"^^xsd:dateTime ;
	dct:modified "2021-12-21T12:00:00+00:00"^^xsd:dateTime  ; 
	ikos:retired "2015-02-24T12:00:00+00:00"^^xsd:dateTime ;
	skos:broadMatch subj:15062000 ;
	skos:exactMatch <https://www.wikidata.org/entity/Q4008851> ;
	skos:broader	medtop:20001071 .

medtop:20001081
	rdf:type skos:Concept ;
	skos:prefLabel	"synchronised free routine"@en-GB ;
	skos:definition	"In the free programme, music, movements and their order of execution are not restricted."@en-GB ;
	skos:changeNote	"2016-04-05: Broader concept changed."@en-GB ;
	skos:inScheme <http://cv.iptc.org/newscodes/mediatopic/>  ;
	ikos:created "2009-10-22T02:00:00+00:00"^^xsd:dateTime ;
	dct:created "2009-10-22T02:00:00+00:00"^^xsd:dateTime ;
	ikos:modified "2021-02-18T12:00:00+00:00"^^xsd:dateTime ;
	dct:modified "2021-02-18T12:00:00+00:00"^^xsd:dateTime  ;
	skos:exactMatch subj:15062026 ;
	skos:broader	medtop:20001175 .

medtop:20001082
	rdf:type skos:Concept ;
	skos:prefLabel	"synchronised technical routine"@en-GB ;
	skos:definition	"Contestants obtain points from 10 sitting judges by executing certain synchronised artistic shapes and movements in the water. In the technical programme, competitors must execute a range of specific moves in a given order."@en-GB ;
	skos:changeNote	"2016-04-05: Broader concept changed"@en-GB ;
	skos:inScheme <http://cv.iptc.org/newscodes/mediatopic/>  ;
	ikos:created "2009-10-22T02:00:00+00:00"^^xsd:dateTime ;
	dct:created "2009-10-22T02:00:00+00:00"^^xsd:dateTime ;
	ikos:modified "2021-02-18T12:00:00+00:00"^^xsd:dateTime ;
	dct:modified "2021-02-18T12:00:00+00:00"^^xsd:dateTime  ;
	skos:exactMatch subj:15062025 ;
	skos:broader	medtop:20001175 .

medtop:20001083
	rdf:type skos:Concept ;
	skos:prefLabel	"table tennis"@en-GB ;
	skos:definition	"A racquet sport for two or four (in doubles), who compete at a table divided by a net using a small bat to play a lightweight ball"@en-GB ;
	skos:inScheme <http://cv.iptc.org/newscodes/mediatopic/>  ;
	ikos:created "2009-10-22T02:00:00+00:00"^^xsd:dateTime ;
	dct:created "2009-10-22T02:00:00+00:00"^^xsd:dateTime ;
	ikos:modified "2021-03-15T12:00:00+00:00"^^xsd:dateTime ;
	dct:modified "2021-03-15T12:00:00+00:00"^^xsd:dateTime  ;
	skos:exactMatch subj:15063000 ;
	skos:exactMatch <https://www.wikidata.org/entity/Q3930> ;
	skos:broader	medtop:20000822 .

medtop:20001084
	rdf:type skos:Concept ;
	skos:prefLabel	"Taekwon-Do"@en-GB ;
	skos:definition	"A martial art of Korean origin"@en-GB ;
	skos:changeNote	"Change Note 2015-08-27: broader term changed"@en-GB ;
	skos:inScheme <http://cv.iptc.org/newscodes/mediatopic/>  ;
	ikos:created "2009-10-22T02:00:00+00:00"^^xsd:dateTime ;
	dct:created "2009-10-22T02:00:00+00:00"^^xsd:dateTime ;
	ikos:modified "2021-02-18T12:00:00+00:00"^^xsd:dateTime ;
	dct:modified "2021-02-18T12:00:00+00:00"^^xsd:dateTime  ;
	skos:exactMatch subj:15064000 ;
	skos:exactMatch <https://www.wikidata.org/entity/Q36389> ;
	skos:broader	medtop:20001157 .

medtop:20001085
	rdf:type skos:Concept ;
	skos:prefLabel	"tennis"@en-GB ;
	skos:definition	"A sport where two players, four in doubles, equipped with a racket compete by hitting the ball over a net into the opponent's side of the court with the aim of putting it out of reach within the regulation lines, thus winning points."@en-GB ;
	skos:inScheme <http://cv.iptc.org/newscodes/mediatopic/>  ;
	ikos:created "2009-10-22T02:00:00+00:00"^^xsd:dateTime ;
	dct:created "2009-10-22T02:00:00+00:00"^^xsd:dateTime ;
	ikos:modified "2021-02-18T12:00:00+00:00"^^xsd:dateTime ;
	dct:modified "2021-02-18T12:00:00+00:00"^^xsd:dateTime  ;
	skos:exactMatch subj:15065000 ;
	skos:exactMatch <https://www.wikidata.org/entity/Q847> ;
	skos:broader	medtop:20000822 .

medtop:20001086
	rdf:type skos:Concept ;
	skos:prefLabel	"ten pin bowling"@en-GB ;
	skos:definition	"A game in which a player scores points by trying to knock down ten 'pins' using a ball - if unsuccessful the player has a second attempt. A game consists of ten frames."@en-GB ;
	skos:inScheme <http://cv.iptc.org/newscodes/mediatopic/>  ;
	ikos:created "2009-10-22T02:00:00+00:00"^^xsd:dateTime ;
	dct:created "2009-10-22T02:00:00+00:00"^^xsd:dateTime ;
	ikos:modified "2021-02-18T12:00:00+00:00"^^xsd:dateTime ;
	dct:modified "2021-02-18T12:00:00+00:00"^^xsd:dateTime  ;
	skos:exactMatch subj:15012000 ;
	skos:exactMatch <https://www.wikidata.org/entity/Q172809> ;
	skos:broader	medtop:20000822 .

medtop:20001087
	rdf:type skos:Concept ;
	skos:prefLabel	"triathlon"@en-GB ;
	skos:definition	"An endurance multi-sport where competitors first swim, then cycle and then run a road race. Distances vary according to the competition."@en-GB ;
	skos:inScheme <http://cv.iptc.org/newscodes/mediatopic/>  ;
	ikos:created "2009-10-22T02:00:00+00:00"^^xsd:dateTime ;
	dct:created "2009-10-22T02:00:00+00:00"^^xsd:dateTime ;
	ikos:modified "2021-02-18T12:00:00+00:00"^^xsd:dateTime ;
	dct:modified "2021-02-18T12:00:00+00:00"^^xsd:dateTime  ;
	skos:exactMatch subj:15066000 ;
	skos:exactMatch <https://www.wikidata.org/entity/Q10980> ;
	skos:broader	medtop:20000822 .

medtop:20001088
	rdf:type skos:Concept ;
	skos:prefLabel	"tug-of-war"@en-GB ;
	skos:definition	"Two teams pulling against each other on a rope"@en-GB ;
	skos:inScheme <http://cv.iptc.org/newscodes/mediatopic/>  ;
	ikos:created "2009-10-22T02:00:00+00:00"^^xsd:dateTime ;
	dct:created "2009-10-22T02:00:00+00:00"^^xsd:dateTime ;
	ikos:modified "2021-02-18T12:00:00+00:00"^^xsd:dateTime ;
	dct:modified "2021-02-18T12:00:00+00:00"^^xsd:dateTime  ;
	skos:exactMatch subj:15080000 ;
	skos:exactMatch <https://www.wikidata.org/entity/Q102843> ;
	skos:broader	medtop:20000822 .

medtop:20001089
	rdf:type skos:Concept ;
	skos:prefLabel	"volleyball"@en-GB ;
	skos:definition	"Two teams of six record points by hitting a ball over a net into the opponent's half of the court, keeping it in the air at all times. Points are won when opponents fail to return the ball."@en-GB ;
	skos:inScheme <http://cv.iptc.org/newscodes/mediatopic/>  ;
	ikos:created "2009-10-22T02:00:00+00:00"^^xsd:dateTime ;
	dct:created "2009-10-22T02:00:00+00:00"^^xsd:dateTime ;
	ikos:modified "2021-02-18T12:00:00+00:00"^^xsd:dateTime ;
	dct:modified "2021-02-18T12:00:00+00:00"^^xsd:dateTime  ;
	skos:exactMatch subj:15067000 ;
	skos:exactMatch <https://www.wikidata.org/entity/Q1734> ;
	skos:broader	medtop:20000822 ;
	skos:narrower	medtop:20001090 .

medtop:20001090
	rdf:type skos:Concept ;
	skos:prefLabel	"beach volleyball"@en-GB ;
	skos:definition	"Two teams of two players compete on a sand court. Unlike indoor volleyball, points are scored only when the serving team wins a rally or forces an error. The sand surface makes it more physically demanding than volleyball"@en-GB ;
	skos:inScheme <http://cv.iptc.org/newscodes/mediatopic/>  ;
	ikos:created "2009-10-22T02:00:00+00:00"^^xsd:dateTime ;
	dct:created "2009-10-22T02:00:00+00:00"^^xsd:dateTime ;
	ikos:modified "2021-02-18T12:00:00+00:00"^^xsd:dateTime ;
	dct:modified "2021-02-18T12:00:00+00:00"^^xsd:dateTime  ;
	skos:exactMatch subj:15067001 ;
	skos:exactMatch <https://www.wikidata.org/entity/Q4543> ;
	skos:broader	medtop:20001089 .

medtop:20001091
	rdf:type skos:Concept ;
	skos:prefLabel	"water polo"@en-GB ;
	skos:definition	"Played in a pool between two teams of 7, who must stay afloat and can only use one hand to pass the ball or swim with it before trying to throw it into the opponents net to score goals."@en-GB ;
	skos:inScheme <http://cv.iptc.org/newscodes/mediatopic/>  ;
	ikos:created "2009-10-22T02:00:00+00:00"^^xsd:dateTime ;
	dct:created "2009-10-22T02:00:00+00:00"^^xsd:dateTime ;
	ikos:modified "2021-02-18T12:00:00+00:00"^^xsd:dateTime ;
	dct:modified "2021-02-18T12:00:00+00:00"^^xsd:dateTime  ;
	skos:exactMatch subj:15068000 ;
	skos:exactMatch <https://www.wikidata.org/entity/Q7707> ;
	skos:broader	medtop:20000822 .

medtop:20001092
	rdf:type skos:Concept ;
	skos:prefLabel	"water skiing"@en-GB ;
	skos:definition	"On one or two skis contestants are pulled by a power boat along the water's surface"@en-GB ;
	skos:inScheme <http://cv.iptc.org/newscodes/mediatopic/>  ;
	ikos:created "2009-10-22T02:00:00+00:00"^^xsd:dateTime ;
	dct:created "2009-10-22T02:00:00+00:00"^^xsd:dateTime ;
	ikos:modified "2021-02-18T12:00:00+00:00"^^xsd:dateTime ;
	dct:modified "2021-02-18T12:00:00+00:00"^^xsd:dateTime  ;
	ikos:hasFacet aspfacet:waterskiingtype ;
	skos:exactMatch subj:15069000 ;
	skos:exactMatch <https://www.wikidata.org/entity/Q472827> ;
	skos:broader	medtop:20000822 .

medtop:20001093
	rdf:type skos:Concept ;
	skos:prefLabel	"weightlifting and powerlifting"@en-GB ;
	skos:definition	"A strength test where competitors lift as heavy a weight as possible"@en-GB ;
	skos:inScheme <http://cv.iptc.org/newscodes/mediatopic/>  ;
	ikos:created "2009-10-22T02:00:00+00:00"^^xsd:dateTime ;
	dct:created "2009-10-22T02:00:00+00:00"^^xsd:dateTime ;
	ikos:modified "2021-07-12T12:00:00+00:00"^^xsd:dateTime ;
	dct:modified "2021-07-12T12:00:00+00:00"^^xsd:dateTime  ;
	skos:exactMatch subj:15070000 ;
	ikos:hasFacet aspfacet:weightliftingtype ;
	skos:exactMatch <https://www.wikidata.org/entity/Q83462> ;
	skos:broader	medtop:20000822 ;
	skos:narrower	medtop:20001094 ;
	skos:narrower	medtop:20001095 ;
	skos:narrower	medtop:20001096 .

medtop:20001094
	rdf:type skos:Concept ;
	skos:prefLabel	"clean and jerk (weightlifting)"@en-GB ;
	skos:definition	"The bar is first lifted to the shoulders and then jerk it above the head and keep it there while maintaining straight legs"@en-GB ;
	skos:note	"Retired. Use Media Topic weightlifting+ sports facet weightliftingtype."@en-GB ;
	skos:inScheme <http://cv.iptc.org/newscodes/mediatopic/>  ;
	ikos:created "2009-10-22T02:00:00+00:00"^^xsd:dateTime ;
	dct:created "2009-10-22T02:00:00+00:00"^^xsd:dateTime ;
	ikos:modified "2021-07-12T12:00:00+00:00"^^xsd:dateTime ;
	dct:modified "2021-07-12T12:00:00+00:00"^^xsd:dateTime  ; 
	ikos:retired "2017-07-04T12:00:00+00:00"^^xsd:dateTime ;
	skos:exactMatch subj:15070002 ;
	skos:exactMatch <https://www.wikidata.org/entity/Q6531690> ;
	skos:broader	medtop:20001093 .

medtop:20001095
	rdf:type skos:Concept ;
	skos:prefLabel	"powerlifting"@en-GB ;
	skos:definition	"A strength test where competitors lift as heavy a weight as possible"@en-GB ;
	skos:note	"Retired. Use Media Topic weightlifting+ sports facet weightliftingtype."@en-GB ;
	skos:inScheme <http://cv.iptc.org/newscodes/mediatopic/>  ;
	ikos:created "2009-10-22T02:00:00+00:00"^^xsd:dateTime ;
	dct:created "2009-10-22T02:00:00+00:00"^^xsd:dateTime ;
	ikos:modified "2021-02-18T12:00:00+00:00"^^xsd:dateTime ;
	dct:modified "2021-02-18T12:00:00+00:00"^^xsd:dateTime  ; 
	ikos:retired "2017-07-04T12:00:00+00:00"^^xsd:dateTime ;
	skos:exactMatch subj:15070016 ;
	skos:exactMatch <https://www.wikidata.org/entity/Q213796> ;
	skos:broader	medtop:20001093 .

medtop:20001096
	rdf:type skos:Concept ;
	skos:prefLabel	"snatch (weightlifting)"@en-GB ;
	skos:definition	"The bar must be lifted from floor to above the head in one movement"@en-GB ;
	skos:note	"Retired. Use Media Topicweightlifting+ sports facet weightliftingtype."@en-GB ;
	skos:inScheme <http://cv.iptc.org/newscodes/mediatopic/>  ;
	ikos:created "2009-10-22T02:00:00+00:00"^^xsd:dateTime ;
	dct:created "2009-10-22T02:00:00+00:00"^^xsd:dateTime ;
	ikos:modified "2021-07-12T12:00:00+00:00"^^xsd:dateTime ;
	dct:modified "2021-07-12T12:00:00+00:00"^^xsd:dateTime  ; 
	ikos:retired "2017-07-04T12:00:00+00:00"^^xsd:dateTime ;
	skos:exactMatch subj:15070001 ;
	skos:exactMatch <https://www.wikidata.org/entity/Q14786282> ;
	skos:broader	medtop:20001093 .

medtop:20001097
	rdf:type skos:Concept ;
	skos:prefLabel	"windsurfing"@en-GB ;
	skos:definition	"Contestants must complete a marked out course as fast as possible on a windsurf board"@en-GB ;
	skos:inScheme <http://cv.iptc.org/newscodes/mediatopic/>  ;
	ikos:created "2009-10-22T02:00:00+00:00"^^xsd:dateTime ;
	dct:created "2009-10-22T02:00:00+00:00"^^xsd:dateTime ;
	ikos:modified "2021-02-18T12:00:00+00:00"^^xsd:dateTime ;
	dct:modified "2021-02-18T12:00:00+00:00"^^xsd:dateTime  ;
	ikos:hasFacet aspfacet:windsurfingtype ;
	skos:exactMatch subj:15071000 ;
	skos:exactMatch <https://www.wikidata.org/entity/Q191051> ;
	skos:broader	medtop:20000822 .

medtop:20001098
	rdf:type skos:Concept ;
	skos:prefLabel	"wrestling"@en-GB ;
	skos:definition	"Combat sport where each wrestler attempts to win over his adversary, by holding both shoulders on the ground (fall) long enough to be in control. Points can also be decisive."@en-GB ;
	skos:inScheme <http://cv.iptc.org/newscodes/mediatopic/>  ;
	ikos:created "2009-10-22T02:00:00+00:00"^^xsd:dateTime ;
	dct:created "2009-10-22T02:00:00+00:00"^^xsd:dateTime ;
	ikos:modified "2021-02-18T12:00:00+00:00"^^xsd:dateTime ;
	dct:modified "2021-02-18T12:00:00+00:00"^^xsd:dateTime  ;
	skos:exactMatch subj:15072000 ;
	ikos:hasFacet aspfacet:weightclasstype ;
	skos:exactMatch <https://www.wikidata.org/entity/Q42486> ;
	skos:broader	medtop:20000822 ;
	skos:narrower	medtop:20001099 ;
	skos:narrower	medtop:20001100 ;
	skos:narrower	medtop:20001101 .

medtop:20001099
	rdf:type skos:Concept ;
	skos:prefLabel	"freestyle wrestling"@en-GB ;
	skos:definition	"A style where leg holds are allowed"@en-GB ;
	skos:inScheme <http://cv.iptc.org/newscodes/mediatopic/>  ;
	ikos:created "2009-10-22T02:00:00+00:00"^^xsd:dateTime ;
	dct:created "2009-10-22T02:00:00+00:00"^^xsd:dateTime ;
	ikos:modified "2021-02-18T12:00:00+00:00"^^xsd:dateTime ;
	dct:modified "2021-02-18T12:00:00+00:00"^^xsd:dateTime  ;
	skos:exactMatch subj:15072001 ;
	skos:exactMatch <https://www.wikidata.org/entity/Q327223> ;
	skos:broader	medtop:20001098 .

medtop:20001100
	rdf:type skos:Concept ;
	skos:prefLabel	"greco-roman"@en-GB ;
	skos:definition	"A style where the only holds allowed are those between the head and the belt"@en-GB ;
	skos:inScheme <http://cv.iptc.org/newscodes/mediatopic/>  ;
	ikos:created "2009-10-22T02:00:00+00:00"^^xsd:dateTime ;
	dct:created "2009-10-22T02:00:00+00:00"^^xsd:dateTime ;
	ikos:modified "2021-02-18T12:00:00+00:00"^^xsd:dateTime ;
	dct:modified "2021-02-18T12:00:00+00:00"^^xsd:dateTime  ;
	skos:exactMatch subj:15072002 ;
	skos:exactMatch <https://www.wikidata.org/entity/Q389654> ;
	skos:broader	medtop:20001098 .

medtop:20001101
	rdf:type skos:Concept ;
	skos:prefLabel	"Swiss wrestling"@en-GB ;
	skos:definition	"Traditional Swiss sport similar to wrestling with specific rules"@en-GB ;
	skos:inScheme <http://cv.iptc.org/newscodes/mediatopic/>  ;
	ikos:created "2009-10-22T02:00:00+00:00"^^xsd:dateTime ;
	dct:created "2009-10-22T02:00:00+00:00"^^xsd:dateTime ;
	ikos:modified "2021-02-18T12:00:00+00:00"^^xsd:dateTime ;
	dct:modified "2021-02-18T12:00:00+00:00"^^xsd:dateTime  ;
	skos:exactMatch subj:15072012 ;
	skos:exactMatch <https://www.wikidata.org/entity/Q685078> ;
	skos:broader	medtop:20001098 .

medtop:20001102
	rdf:type skos:Concept ;
	skos:prefLabel	"wushu"@en-GB ;
	skos:definition	"Chinese traditional martial art"@en-GB ;
	skos:changeNote	"Change Note 2015-08-27: broader term changed"@en-GB ;
	skos:inScheme <http://cv.iptc.org/newscodes/mediatopic/>  ;
	ikos:created "2009-10-22T02:00:00+00:00"^^xsd:dateTime ;
	dct:created "2009-10-22T02:00:00+00:00"^^xsd:dateTime ;
	ikos:modified "2021-02-18T12:00:00+00:00"^^xsd:dateTime ;
	dct:modified "2021-02-18T12:00:00+00:00"^^xsd:dateTime  ;
	skos:exactMatch subj:15099000 ;
	skos:exactMatch <https://www.wikidata.org/entity/Q3479346> ;
	skos:broader	medtop:20001157 .

medtop:20001103
	rdf:type skos:Concept ;
	skos:prefLabel	"disciplinary action in sport"@en-GB ;
	skos:definition	"Actions, including fines and suspensions levied by sports organisations and teams"@en-GB ;
	skos:inScheme <http://cv.iptc.org/newscodes/mediatopic/>  ;
	ikos:created "2009-10-22T02:00:00+00:00"^^xsd:dateTime ;
	dct:created "2009-10-22T02:00:00+00:00"^^xsd:dateTime ;
	ikos:modified "2021-02-18T12:00:00+00:00"^^xsd:dateTime ;
	dct:modified "2021-02-18T12:00:00+00:00"^^xsd:dateTime  ;
	skos:exactMatch subj:15102000 ;
	skos:broader	medtop:15000000 .

medtop:20001104
	rdf:type skos:Concept ;
	skos:prefLabel	"drug use in sport"@en-GB ;
	skos:definition	"Drug use associated with sport activities, including doping, abuse, testing and permitted medical uses"@en-GB ;
	skos:inScheme <http://cv.iptc.org/newscodes/mediatopic/>  ;
	ikos:created "2009-10-22T02:00:00+00:00"^^xsd:dateTime ;
	dct:created "2009-10-22T02:00:00+00:00"^^xsd:dateTime ;
	ikos:modified "2022-09-23T12:00:00+00:00"^^xsd:dateTime ;
	dct:modified "2022-09-23T12:00:00+00:00"^^xsd:dateTime  ;
	skos:broadMatch subj:15000000 ;
	skos:broader	medtop:15000000 ;
	skos:narrower	medtop:20001105 ;
	skos:narrower	medtop:20001106 ;
	skos:narrower	medtop:20001107 .

medtop:20001105
	rdf:type skos:Concept ;
	skos:prefLabel	"drug abuse in sport"@en-GB ;
	skos:definition	"Using drugs to improve competitiveness in sports"@en-GB ;
	skos:changeNote	"Retired. Use medtop:20001104: drug use in sport instead"@en-GB ;
	skos:inScheme <http://cv.iptc.org/newscodes/mediatopic/>  ;
	ikos:created "2009-10-22T02:00:00+00:00"^^xsd:dateTime ;
	dct:created "2009-10-22T02:00:00+00:00"^^xsd:dateTime ;
	ikos:modified "2022-09-23T12:00:00+00:00"^^xsd:dateTime ;
	dct:modified "2022-09-23T12:00:00+00:00"^^xsd:dateTime  ; 
	ikos:retired "2022-09-23T12:00:00+00:00"^^xsd:dateTime ;
	skos:broadMatch subj:15000000 ;
	skos:exactMatch <https://www.wikidata.org/entity/Q166376> ;
	skos:broader	medtop:20001104 .

medtop:20001106
	rdf:type skos:Concept ;
	skos:prefLabel	"drug testing in sport"@en-GB ;
	skos:definition	"Means and ways to check the use of drugs in sports"@en-GB ;
	skos:changeNote	"Retired. Use medtop:20001104: drug use in sport instead"@en-GB ;
	skos:inScheme <http://cv.iptc.org/newscodes/mediatopic/>  ;
	ikos:created "2009-10-22T02:00:00+00:00"^^xsd:dateTime ;
	dct:created "2009-10-22T02:00:00+00:00"^^xsd:dateTime ;
	ikos:modified "2022-09-23T12:00:00+00:00"^^xsd:dateTime ;
	dct:modified "2022-09-23T12:00:00+00:00"^^xsd:dateTime  ; 
	ikos:retired "2022-09-23T12:00:00+00:00"^^xsd:dateTime ;
	skos:broadMatch subj:15000000 ;
	skos:broader	medtop:20001104 .

medtop:20001107
	rdf:type skos:Concept ;
	skos:prefLabel	"medical drug use in sport"@en-GB ;
	skos:definition	"Use of drugs for medical reasons as permitted by sport regulators"@en-GB ;
	skos:changeNote	"Retired. Use medtop:20001104: drug use in sport instead"@en-GB ;
	skos:inScheme <http://cv.iptc.org/newscodes/mediatopic/>  ;
	ikos:created "2009-10-22T02:00:00+00:00"^^xsd:dateTime ;
	dct:created "2009-10-22T02:00:00+00:00"^^xsd:dateTime ;
	ikos:modified "2022-09-23T12:00:00+00:00"^^xsd:dateTime ;
	dct:modified "2022-09-23T12:00:00+00:00"^^xsd:dateTime  ; 
	ikos:retired "2022-09-23T12:00:00+00:00"^^xsd:dateTime ;
	skos:broadMatch subj:15000000 ;
	skos:broader	medtop:20001104 .

medtop:20001108
	rdf:type skos:Concept ;
	skos:prefLabel	"sport event"@en-GB ;
	skos:definition	"An event featuring one or more sport competitions"@en-GB ;
	skos:inScheme <http://cv.iptc.org/newscodes/mediatopic/>  ;
	ikos:created "2009-10-22T02:00:00+00:00"^^xsd:dateTime ;
	dct:created "2009-10-22T02:00:00+00:00"^^xsd:dateTime ;
	ikos:modified "2021-07-12T12:00:00+00:00"^^xsd:dateTime ;
	dct:modified "2021-07-12T12:00:00+00:00"^^xsd:dateTime  ;
	skos:exactMatch <https://www.wikidata.org/entity/Q167170> ;
	skos:exactMatch subj:15073000 ;
	skos:broader	medtop:15000000 ;
	skos:narrower	medtop:20001109 ;
	skos:narrower	medtop:20001110 ;
	skos:narrower	medtop:20001111 ;
	skos:narrower	medtop:20001112 ;
	skos:narrower	medtop:20001113 ;
	skos:narrower	medtop:20001114 ;
	skos:narrower	medtop:20001115 ;
	skos:narrower	medtop:20001116 ;
	skos:narrower	medtop:20001117 ;
	skos:narrower	medtop:20001118 ;
	skos:narrower	medtop:20001119 ;
	skos:narrower	medtop:20001120 ;
	skos:narrower	medtop:20001121 ;
	skos:narrower	medtop:20001122 ;
	skos:narrower	medtop:20001123 ;
	skos:narrower	medtop:20001177 ;
	skos:narrower	medtop:20001178 ;
	skos:narrower	medtop:20001341 ;
	skos:narrower	medtop:20001342 ;
	skos:narrower	medtop:20001343 .

medtop:20001109
	rdf:type skos:Concept ;
	skos:prefLabel	"continental championship"@en-GB ;
	skos:definition	"A competition where individuals or teams from countries from one continent may participate. Called a *Championship*"@en-GB ;
	skos:note	"Retired December 2021."@en-GB ;
	skos:inScheme <http://cv.iptc.org/newscodes/mediatopic/>  ;
	ikos:created "2009-10-22T02:00:00+00:00"^^xsd:dateTime ;
	dct:created "2009-10-22T02:00:00+00:00"^^xsd:dateTime ;
	ikos:modified "2021-12-17T12:00:00+00:00"^^xsd:dateTime ;
	dct:modified "2021-12-17T12:00:00+00:00"^^xsd:dateTime  ; 
	ikos:retired "2021-12-17T12:00:00+00:00"^^xsd:dateTime ;
	skos:broadMatch subj:15073028 ;
	skos:exactMatch <https://www.wikidata.org/entity/Q5165329> ;
	skos:broader	medtop:20001108 .

medtop:20001110
	rdf:type skos:Concept ;
	skos:prefLabel	"continental cup"@en-GB ;
	skos:definition	"A competition where individuals or teams from countries from one continent may participate. Called a *Cup*"@en-GB ;
	skos:note	"Retired December 2021."@en-GB ;
	skos:inScheme <http://cv.iptc.org/newscodes/mediatopic/>  ;
	ikos:created "2009-10-22T02:00:00+00:00"^^xsd:dateTime ;
	dct:created "2009-10-22T02:00:00+00:00"^^xsd:dateTime ;
	ikos:modified "2021-12-17T12:00:00+00:00"^^xsd:dateTime ;
	dct:modified "2021-12-17T12:00:00+00:00"^^xsd:dateTime  ; 
	ikos:retired "2021-12-17T12:00:00+00:00"^^xsd:dateTime ;
	skos:exactMatch subj:15073020 ;
	skos:exactMatch <https://www.wikidata.org/entity/Q340966> ;
	skos:broader	medtop:20001108 .

medtop:20001111
	rdf:type skos:Concept ;
	skos:prefLabel	"continental games"@en-GB ;
	skos:definition	"A competition where individuals or teams from countries from one continent may participate. Called *Games*"@en-GB ;
	skos:note	"Retired December 2021."@en-GB ;
	skos:inScheme <http://cv.iptc.org/newscodes/mediatopic/>  ;
	ikos:created "2009-10-22T02:00:00+00:00"^^xsd:dateTime ;
	dct:created "2009-10-22T02:00:00+00:00"^^xsd:dateTime ;
	ikos:modified "2021-12-17T12:00:00+00:00"^^xsd:dateTime ;
	dct:modified "2021-12-17T12:00:00+00:00"^^xsd:dateTime  ; 
	ikos:retired "2021-12-17T12:00:00+00:00"^^xsd:dateTime ;
	skos:broadMatch subj:15073000 ;
	skos:broader	medtop:20001108 .

medtop:20001112
	rdf:type skos:Concept ;
	skos:prefLabel	"international championship"@en-GB ;
	skos:definition	"A competition where individuals or teams from different countries may participate. Called a *Championship*"@en-GB ;
	skos:note	"Retired December 2021."@en-GB ;
	skos:inScheme <http://cv.iptc.org/newscodes/mediatopic/>  ;
	ikos:created "2009-10-22T02:00:00+00:00"^^xsd:dateTime ;
	dct:created "2009-10-22T02:00:00+00:00"^^xsd:dateTime ;
	ikos:modified "2021-12-17T12:00:00+00:00"^^xsd:dateTime ;
	dct:modified "2021-12-17T12:00:00+00:00"^^xsd:dateTime  ; 
	ikos:retired "2021-12-17T12:00:00+00:00"^^xsd:dateTime ;
	skos:broadMatch subj:15073000 ;
	skos:exactMatch <https://www.wikidata.org/entity/Q1344963> ;
	skos:broader	medtop:20001108 .

medtop:20001113
	rdf:type skos:Concept ;
	skos:prefLabel	"international cup"@en-GB ;
	skos:definition	"A competition where individuals or teams from different countries may participate. Called a *Cup*"@en-GB ;
	skos:note	"Retired December 2021."@en-GB ;
	skos:inScheme <http://cv.iptc.org/newscodes/mediatopic/>  ;
	ikos:created "2009-10-22T02:00:00+00:00"^^xsd:dateTime ;
	dct:created "2009-10-22T02:00:00+00:00"^^xsd:dateTime ;
	ikos:modified "2021-12-17T12:00:00+00:00"^^xsd:dateTime ;
	dct:modified "2021-12-17T12:00:00+00:00"^^xsd:dateTime  ; 
	ikos:retired "2021-12-17T12:00:00+00:00"^^xsd:dateTime ;
	skos:exactMatch subj:15073021 ;
	skos:exactMatch <https://www.wikidata.org/entity/Q1936368> ;
	skos:broader	medtop:20001108 .

medtop:20001114
	rdf:type skos:Concept ;
	skos:prefLabel	"international games"@en-GB ;
	skos:definition	"A competition where individuals or teams from different countries may participate. Called *Games*"@en-GB ;
	skos:note	"Retired December 2021."@en-GB ;
	skos:inScheme <http://cv.iptc.org/newscodes/mediatopic/>  ;
	ikos:created "2009-10-22T02:00:00+00:00"^^xsd:dateTime ;
	dct:created "2009-10-22T02:00:00+00:00"^^xsd:dateTime ;
	ikos:modified "2021-12-17T12:00:00+00:00"^^xsd:dateTime ;
	dct:modified "2021-12-17T12:00:00+00:00"^^xsd:dateTime  ; 
	ikos:retired "2021-12-17T12:00:00+00:00"^^xsd:dateTime ;
	skos:broadMatch subj:15073000 ;
	skos:broader	medtop:20001108 .

medtop:20001115
	rdf:type skos:Concept ;
	skos:prefLabel	"national championship"@en-GB ;
	skos:definition	"A competition where individuals or teams from one country may participate. Called a *Championship*"@en-GB ;
	skos:note	"Retired December 2021."@en-GB ;
	skos:inScheme <http://cv.iptc.org/newscodes/mediatopic/>  ;
	ikos:created "2009-10-22T02:00:00+00:00"^^xsd:dateTime ;
	dct:created "2009-10-22T02:00:00+00:00"^^xsd:dateTime ;
	ikos:modified "2021-12-17T12:00:00+00:00"^^xsd:dateTime ;
	dct:modified "2021-12-17T12:00:00+00:00"^^xsd:dateTime  ; 
	ikos:retired "2021-12-17T12:00:00+00:00"^^xsd:dateTime ;
	skos:broadMatch subj:15073000 ;
	skos:exactMatch <https://www.wikidata.org/entity/Q3270632> ;
	skos:broader	medtop:20001108 .

medtop:20001116
	rdf:type skos:Concept ;
	skos:prefLabel	"national cup"@en-GB ;
	skos:definition	"A competition where individuals or teams from one country may participate. Called a *Cup*"@en-GB ;
	skos:note	"Retired December 2021."@en-GB ;
	skos:inScheme <http://cv.iptc.org/newscodes/mediatopic/>  ;
	ikos:created "2009-10-22T02:00:00+00:00"^^xsd:dateTime ;
	dct:created "2009-10-22T02:00:00+00:00"^^xsd:dateTime ;
	ikos:modified "2021-12-17T12:00:00+00:00"^^xsd:dateTime ;
	dct:modified "2021-12-17T12:00:00+00:00"^^xsd:dateTime  ; 
	ikos:retired "2021-12-17T12:00:00+00:00"^^xsd:dateTime ;
	skos:exactMatch subj:15073022 ;
	skos:broader	medtop:20001108 .

medtop:20001117
	rdf:type skos:Concept ;
	skos:prefLabel	"national games"@en-GB ;
	skos:definition	"A competition where individuals or teams from one country may participate. Called *Games*"@en-GB ;
	skos:note	"Retired December 2021."@en-GB ;
	skos:inScheme <http://cv.iptc.org/newscodes/mediatopic/>  ;
	ikos:created "2009-10-22T02:00:00+00:00"^^xsd:dateTime ;
	dct:created "2009-10-22T02:00:00+00:00"^^xsd:dateTime ;
	ikos:modified "2021-12-17T12:00:00+00:00"^^xsd:dateTime ;
	dct:modified "2021-12-17T12:00:00+00:00"^^xsd:dateTime  ; 
	ikos:retired "2021-12-17T12:00:00+00:00"^^xsd:dateTime ;
	skos:broadMatch subj:15073000 ;
	skos:broader	medtop:20001108 .

medtop:20001118
	rdf:type skos:Concept ;
	skos:prefLabel	"regional championship"@en-GB ;
	skos:definition	"A competition where individuals or teams from a region of a country may participate. Called a *Championship*"@en-GB ;
	skos:note	"Retired December 2021."@en-GB ;
	skos:inScheme <http://cv.iptc.org/newscodes/mediatopic/>  ;
	ikos:created "2009-10-22T02:00:00+00:00"^^xsd:dateTime ;
	dct:created "2009-10-22T02:00:00+00:00"^^xsd:dateTime ;
	ikos:modified "2021-12-17T12:00:00+00:00"^^xsd:dateTime ;
	dct:modified "2021-12-17T12:00:00+00:00"^^xsd:dateTime  ; 
	ikos:retired "2021-12-17T12:00:00+00:00"^^xsd:dateTime ;
	skos:exactMatch subj:15073035 ;
	skos:broader	medtop:20001108 .

medtop:20001119
	rdf:type skos:Concept ;
	skos:prefLabel	"regional cup"@en-GB ;
	skos:definition	"A competition where individuals or teams from a region of a country may participate. Called a *Cup*"@en-GB ;
	skos:note	"Retired December 2021."@en-GB ;
	skos:inScheme <http://cv.iptc.org/newscodes/mediatopic/>  ;
	ikos:created "2009-10-22T02:00:00+00:00"^^xsd:dateTime ;
	dct:created "2009-10-22T02:00:00+00:00"^^xsd:dateTime ;
	ikos:modified "2021-12-17T12:00:00+00:00"^^xsd:dateTime ;
	dct:modified "2021-12-17T12:00:00+00:00"^^xsd:dateTime  ; 
	ikos:retired "2021-12-17T12:00:00+00:00"^^xsd:dateTime ;
	skos:exactMatch subj:15073024 ;
	skos:broader	medtop:20001108 .

medtop:20001120
	rdf:type skos:Concept ;
	skos:prefLabel	"regional games"@en-GB ;
	skos:definition	"A competition where individuals or teams from a region of a country may participate. Called *Games*"@en-GB ;
	skos:note	"Retired December 2021."@en-GB ;
	skos:inScheme <http://cv.iptc.org/newscodes/mediatopic/>  ;
	ikos:created "2009-10-22T02:00:00+00:00"^^xsd:dateTime ;
	dct:created "2009-10-22T02:00:00+00:00"^^xsd:dateTime ;
	ikos:modified "2021-12-17T12:00:00+00:00"^^xsd:dateTime ;
	dct:modified "2021-12-17T12:00:00+00:00"^^xsd:dateTime  ; 
	ikos:retired "2021-12-17T12:00:00+00:00"^^xsd:dateTime ;
	skos:broadMatch subj:15073000 ;
	skos:broader	medtop:20001108 .

medtop:20001121
	rdf:type skos:Concept ;
	skos:prefLabel	"world championship"@en-GB ;
	skos:definition	"A competition where individuals or teams from the five continents may participate. Called *World Championship*"@en-GB ;
	skos:note	"Retired December 2021."@en-GB ;
	skos:inScheme <http://cv.iptc.org/newscodes/mediatopic/>  ;
	ikos:created "2009-10-22T02:00:00+00:00"^^xsd:dateTime ;
	dct:created "2009-10-22T02:00:00+00:00"^^xsd:dateTime ;
	ikos:modified "2021-12-17T12:00:00+00:00"^^xsd:dateTime ;
	dct:modified "2021-12-17T12:00:00+00:00"^^xsd:dateTime  ; 
	ikos:retired "2021-12-17T12:00:00+00:00"^^xsd:dateTime ;
	skos:exactMatch subj:15073026 ;
	skos:exactMatch <https://www.wikidata.org/entity/Q1344963> ;
	skos:broader	medtop:20001108 .

medtop:20001122
	rdf:type skos:Concept ;
	skos:prefLabel	"world cup"@en-GB ;
	skos:definition	"A competition where individuals or teams from the five continents may participate. Called *World Cup*"@en-GB ;
	skos:note	"Retired December 2021."@en-GB ;
	skos:inScheme <http://cv.iptc.org/newscodes/mediatopic/>  ;
	ikos:created "2009-10-22T02:00:00+00:00"^^xsd:dateTime ;
	dct:created "2009-10-22T02:00:00+00:00"^^xsd:dateTime ;
	ikos:modified "2021-12-17T12:00:00+00:00"^^xsd:dateTime ;
	dct:modified "2021-12-17T12:00:00+00:00"^^xsd:dateTime  ; 
	ikos:retired "2021-12-17T12:00:00+00:00"^^xsd:dateTime ;
	skos:exactMatch subj:15073018 ;
	skos:exactMatch <https://www.wikidata.org/entity/Q1936368> ;
	skos:broader	medtop:20001108 .

medtop:20001123
	rdf:type skos:Concept ;
	skos:prefLabel	"world games"@en-GB ;
	skos:definition	"A competition where individuals or teams from the five continents may participate. Called *World Games*"@en-GB ;
	skos:note	"Retired December 2021."@en-GB ;
	skos:inScheme <http://cv.iptc.org/newscodes/mediatopic/>  ;
	ikos:created "2009-10-22T02:00:00+00:00"^^xsd:dateTime ;
	dct:created "2009-10-22T02:00:00+00:00"^^xsd:dateTime ;
	ikos:modified "2021-12-17T12:00:00+00:00"^^xsd:dateTime ;
	dct:modified "2021-12-17T12:00:00+00:00"^^xsd:dateTime  ; 
	ikos:retired "2021-12-17T12:00:00+00:00"^^xsd:dateTime ;
	skos:exactMatch subj:15073017 ;
	skos:exactMatch <https://www.wikidata.org/entity/Q673097> ;
	skos:broader	medtop:20001108 .

medtop:20001124
	rdf:type skos:Concept ;
	skos:prefLabel	"sport industry"@en-GB ;
	skos:definition	"Commercial issues related to sport"@en-GB ;
	skos:inScheme <http://cv.iptc.org/newscodes/mediatopic/>  ;
	ikos:created "2009-10-22T02:00:00+00:00"^^xsd:dateTime ;
	dct:created "2009-10-22T02:00:00+00:00"^^xsd:dateTime ;
	ikos:modified "2021-02-18T12:00:00+00:00"^^xsd:dateTime ;
	dct:modified "2021-02-18T12:00:00+00:00"^^xsd:dateTime  ;
	skos:broadMatch subj:15000000 ;
	skos:exactMatch <https://www.wikidata.org/entity/Q4438117> ;
	skos:broader	medtop:15000000 .

medtop:20001125
	rdf:type skos:Concept ;
	skos:prefLabel	"sport organisation"@en-GB ;
	skos:definition	"Organisations or associations that govern sports"@en-GB ;
	skos:inScheme <http://cv.iptc.org/newscodes/mediatopic/>  ;
	ikos:created "2009-10-22T02:00:00+00:00"^^xsd:dateTime ;
	dct:created "2009-10-22T02:00:00+00:00"^^xsd:dateTime ;
	ikos:modified "2023-10-02T12:00:00+00:00"^^xsd:dateTime ;
	dct:modified "2023-10-02T12:00:00+00:00"^^xsd:dateTime  ;
	skos:exactMatch <https://www.wikidata.org/entity/Q4438121> ;
	skos:exactMatch subj:15058000 ;
	skos:broader	medtop:15000000 .

medtop:20001126
	rdf:type skos:Concept ;
	skos:prefLabel	"sport venue"@en-GB ;
	skos:definition	"Gymnasiums, stadiums, arenas or facilities where sports events take place"@en-GB ;
	skos:inScheme <http://cv.iptc.org/newscodes/mediatopic/>  ;
	ikos:created "2009-10-22T02:00:00+00:00"^^xsd:dateTime ;
	dct:created "2009-10-22T02:00:00+00:00"^^xsd:dateTime ;
	ikos:modified "2021-03-31T12:00:00+00:00"^^xsd:dateTime ;
	dct:modified "2021-03-31T12:00:00+00:00"^^xsd:dateTime  ;
	skos:exactMatch <https://www.wikidata.org/entity/Q1076486> ;
	skos:broadMatch subj:15000000 ;
	skos:broader	medtop:15000000 .

medtop:20001128
	rdf:type skos:Concept ;
	skos:prefLabel	"weather forecast"@en-GB ;
	skos:definition	"The long- or short-term meteorological prediction and reporting of the upcoming weather for a given region"@en-GB ;
	skos:inScheme <http://cv.iptc.org/newscodes/mediatopic/>  ;
	ikos:created "2009-10-22T02:00:00+00:00"^^xsd:dateTime ;
	dct:created "2009-10-22T02:00:00+00:00"^^xsd:dateTime ;
	ikos:modified "2021-02-18T12:00:00+00:00"^^xsd:dateTime ;
	dct:modified "2021-02-18T12:00:00+00:00"^^xsd:dateTime  ;
	skos:exactMatch <https://www.wikidata.org/entity/Q182868> ;
	skos:exactMatch subj:17001000 ;
	skos:broader	medtop:17000000 .

medtop:20001129
	rdf:type skos:Concept ;
	skos:prefLabel	"weather phenomena"@en-GB ;
	skos:definition	"Short- or long-term meteorological phenomena worthy of study, reporting or public advisory such as climate change, storms, heat waves or tornadoes"@en-GB ;
	skos:inScheme <http://cv.iptc.org/newscodes/mediatopic/>  ;
	ikos:created "2009-10-22T02:00:00+00:00"^^xsd:dateTime ;
	dct:created "2009-10-22T02:00:00+00:00"^^xsd:dateTime ;
	ikos:modified "2021-05-05T12:00:00+00:00"^^xsd:dateTime ;
	dct:modified "2021-05-05T12:00:00+00:00"^^xsd:dateTime  ;
	skos:broadMatch subj:17003001 ;
	skos:exactMatch <https://www.wikidata.org/entity/Q1329451> ;
	skos:broader	medtop:17000000 .

medtop:20001130
	rdf:type skos:Concept ;
	skos:prefLabel	"weather statistic"@en-GB ;
	skos:definition	"Numerical facts about the weather such as temperature, barometric pressure, river levels, humidity or high and low tides"@en-GB ;
	skos:inScheme <http://cv.iptc.org/newscodes/mediatopic/>  ;
	ikos:created "2009-10-22T02:00:00+00:00"^^xsd:dateTime ;
	dct:created "2009-10-22T02:00:00+00:00"^^xsd:dateTime ;
	ikos:modified "2021-02-18T12:00:00+00:00"^^xsd:dateTime ;
	dct:modified "2021-02-18T12:00:00+00:00"^^xsd:dateTime  ;
	skos:exactMatch subj:17004000 ;
	skos:broader	medtop:17000000 .

medtop:20001131
	rdf:type skos:Concept ;
	skos:prefLabel	"weather warning"@en-GB ;
	skos:definition	"Alerts issued to the public about severe or notable weather in their area"@en-GB ;
	skos:inScheme <http://cv.iptc.org/newscodes/mediatopic/>  ;
	ikos:created "2009-10-22T02:00:00+00:00"^^xsd:dateTime ;
	dct:created "2009-10-22T02:00:00+00:00"^^xsd:dateTime ;
	ikos:modified "2021-02-18T12:00:00+00:00"^^xsd:dateTime ;
	dct:modified "2021-02-18T12:00:00+00:00"^^xsd:dateTime  ;
	skos:exactMatch subj:17005000 ;
	skos:exactMatch <https://www.wikidata.org/entity/Q7978253> ;
	skos:broader	medtop:17000000 .

medtop:20001132
	rdf:type skos:Concept ;
	skos:prefLabel	"cultural policies"@en-GB ;
	skos:definition	"Government policies affecting cultural affairs"@en-GB ;
	skos:inScheme <http://cv.iptc.org/newscodes/mediatopic/>  ;
	ikos:created "2012-10-04T12:00:00+00:00"^^xsd:dateTime ;
	dct:created "2012-10-04T12:00:00+00:00"^^xsd:dateTime ;
	ikos:modified "2021-07-12T12:00:00+00:00"^^xsd:dateTime ;
	dct:modified "2021-07-12T12:00:00+00:00"^^xsd:dateTime  ;
	skos:exactMatch <https://www.wikidata.org/entity/Q1711347> ;
	skos:broader	medtop:20000621 .

medtop:20001133
	rdf:type skos:Concept ;
	skos:prefLabel	"musical"@en-GB ;
	skos:definition	"A genre of music theatre in which singing and dancing play an essential part of the storytelling"@en-GB ;
	skos:inScheme <http://cv.iptc.org/newscodes/mediatopic/>  ;
	ikos:created "2012-10-04T12:00:00+00:00"^^xsd:dateTime ;
	dct:created "2012-10-04T12:00:00+00:00"^^xsd:dateTime ;
	ikos:modified "2021-09-30T12:00:00+00:00"^^xsd:dateTime ;
	dct:modified "2021-09-30T12:00:00+00:00"^^xsd:dateTime  ;
	skos:exactMatch <https://www.wikidata.org/entity/Q2743> ;
	skos:broader	medtop:20000029 .

medtop:20001134
	rdf:type skos:Concept ;
	skos:prefLabel	"operetta"@en-GB ;
	skos:definition	"A genre of music theatre that usually has a light or humorous theme where some of the libretto is usually spoken rather than sung."@en-GB ;
	skos:inScheme <http://cv.iptc.org/newscodes/mediatopic/>  ;
	ikos:created "2012-10-04T12:00:00+00:00"^^xsd:dateTime ;
	dct:created "2012-10-04T12:00:00+00:00"^^xsd:dateTime ;
	ikos:modified "2021-09-30T12:00:00+00:00"^^xsd:dateTime ;
	dct:modified "2021-09-30T12:00:00+00:00"^^xsd:dateTime  ;
	skos:exactMatch <https://www.wikidata.org/entity/Q170384> ;
	skos:broader	medtop:20000029 .

medtop:20001135
	rdf:type skos:Concept ;
	skos:prefLabel	"art exhibition"@en-GB ;
	skos:definition	"Temporary presentation of art in museums, art halls or galleries"@en-GB ;
	skos:inScheme <http://cv.iptc.org/newscodes/mediatopic/>  ;
	ikos:created "2012-10-04T12:00:00+00:00"^^xsd:dateTime ;
	dct:created "2012-10-04T12:00:00+00:00"^^xsd:dateTime ;
	ikos:modified "2023-03-31T12:00:00+00:00"^^xsd:dateTime ;
	dct:modified "2023-03-31T12:00:00+00:00"^^xsd:dateTime  ;
	skos:exactMatch <https://www.wikidata.org/entity/Q667276> ;
	skos:broader	medtop:20000038 .

medtop:20001136
	rdf:type skos:Concept ;
	skos:prefLabel	"trade show or expo"@en-GB ;
	skos:definition	"Market place to display and trade goods or services"@en-GB ;
	skos:inScheme <http://cv.iptc.org/newscodes/mediatopic/>  ;
	ikos:created "2012-10-04T12:00:00+00:00"^^xsd:dateTime ;
	dct:created "2012-10-04T12:00:00+00:00"^^xsd:dateTime ;
	ikos:modified "2023-03-31T12:00:00+00:00"^^xsd:dateTime ;
	dct:modified "2023-03-31T12:00:00+00:00"^^xsd:dateTime  ;
	skos:exactMatch <https://www.wikidata.org/entity/Q57305> ;
	skos:broader	medtop:20001371 .

medtop:20001137
	rdf:type skos:Concept ;
	skos:prefLabel	"stock recommendation"@en-GB ;
	skos:definition	"An analyst's recommendation for particular stocks. May include the analyst s price target for the stock."@en-GB ;
	skos:changeNote	"Retired. Use medtop:20000396 stocks and/or genre:Analysis instead."@en-GB ;
	skos:inScheme <http://cv.iptc.org/newscodes/mediatopic/>  ;
	ikos:created "2012-10-04T12:00:00+00:00"^^xsd:dateTime ;
	dct:created "2012-10-04T12:00:00+00:00"^^xsd:dateTime ;
	ikos:modified "2023-03-31T12:00:00+00:00"^^xsd:dateTime ;
	dct:modified "2023-03-31T12:00:00+00:00"^^xsd:dateTime  ; 
	ikos:retired "2023-03-31T12:00:00+00:00"^^xsd:dateTime ;
	skos:broader	medtop:20000396 ;
	skos:narrower	medtop:20001138 ;
	skos:narrower	medtop:20001139 ;
	skos:narrower	medtop:20001140 .

medtop:20001138
	rdf:type skos:Concept ;
	skos:prefLabel	"buy recommendation"@en-GB ;
	skos:definition	"An analyst's recommendation to buy particular stocks. May include the analyst s price target for the stock."@en-GB ;
	skos:changeNote	"Retired. Use medtop:20000396 stocks and/or genre:Analysis instead."@en-GB ;
	skos:inScheme <http://cv.iptc.org/newscodes/mediatopic/>  ;
	ikos:created "2012-10-04T12:00:00+00:00"^^xsd:dateTime ;
	dct:created "2012-10-04T12:00:00+00:00"^^xsd:dateTime ;
	ikos:modified "2023-03-31T12:00:00+00:00"^^xsd:dateTime ;
	dct:modified "2023-03-31T12:00:00+00:00"^^xsd:dateTime  ; 
	ikos:retired "2023-03-31T12:00:00+00:00"^^xsd:dateTime ;
	skos:broader	medtop:20001137 .

medtop:20001139
	rdf:type skos:Concept ;
	skos:prefLabel	"hold recommendation"@en-GB ;
	skos:definition	"An analyst's recommendation to hold particular stocks. May include the analyst s price target for the stock."@en-GB ;
	skos:changeNote	"Retired. Use medtop:20000396 stocks and/or genre:Analysis instead."@en-GB ;
	skos:inScheme <http://cv.iptc.org/newscodes/mediatopic/>  ;
	ikos:created "2012-10-04T12:00:00+00:00"^^xsd:dateTime ;
	dct:created "2012-10-04T12:00:00+00:00"^^xsd:dateTime ;
	ikos:modified "2023-03-31T12:00:00+00:00"^^xsd:dateTime ;
	dct:modified "2023-03-31T12:00:00+00:00"^^xsd:dateTime  ; 
	ikos:retired "2023-03-31T12:00:00+00:00"^^xsd:dateTime ;
	skos:broader	medtop:20001137 .

medtop:20001140
	rdf:type skos:Concept ;
	skos:prefLabel	"sell recommendation"@en-GB ;
	skos:definition	"An analyst's recommendation to sell particular stocks. May include the analyst s price target for the stock."@en-GB ;
	skos:changeNote	"Retired. Use medtop:20000396 stocks and/or genre:Analysis instead."@en-GB ;
	skos:inScheme <http://cv.iptc.org/newscodes/mediatopic/>  ;
	ikos:created "2012-10-04T12:00:00+00:00"^^xsd:dateTime ;
	dct:created "2012-10-04T12:00:00+00:00"^^xsd:dateTime ;
	ikos:modified "2023-03-31T12:00:00+00:00"^^xsd:dateTime ;
	dct:modified "2023-03-31T12:00:00+00:00"^^xsd:dateTime  ; 
	ikos:retired "2023-03-31T12:00:00+00:00"^^xsd:dateTime ;
	skos:broader	medtop:20001137 .

medtop:20001141
	rdf:type skos:Concept ;
	skos:prefLabel	"hot stock"@en-GB ;
	skos:definition	"Remarkable price movements of a particular stock."@en-GB ;
	skos:changeNote	"Retired. Use medtop:20000396 stocks and/or genre:Analysis instead."@en-GB ;
	skos:inScheme <http://cv.iptc.org/newscodes/mediatopic/>  ;
	ikos:created "2012-10-04T12:00:00+00:00"^^xsd:dateTime ;
	dct:created "2012-10-04T12:00:00+00:00"^^xsd:dateTime ;
	ikos:modified "2023-03-31T12:00:00+00:00"^^xsd:dateTime ;
	dct:modified "2023-03-31T12:00:00+00:00"^^xsd:dateTime  ; 
	ikos:retired "2023-03-31T12:00:00+00:00"^^xsd:dateTime ;
	skos:broader	medtop:20000396 .

medtop:20001142
	rdf:type skos:Concept ;
	skos:prefLabel	"recreational hiking and climbing"@en-GB ;
	skos:definition	"Sportive activities in the mountains including climbing and hiking"@en-GB ;
	skos:inScheme <http://cv.iptc.org/newscodes/mediatopic/>  ;
	ikos:created "2012-10-04T12:00:00+00:00"^^xsd:dateTime ;
	dct:created "2012-10-04T12:00:00+00:00"^^xsd:dateTime ;
	ikos:modified "2023-10-02T12:00:00+00:00"^^xsd:dateTime ;
	dct:modified "2023-10-02T12:00:00+00:00"^^xsd:dateTime  ;
	skos:exactMatch <https://www.wikidata.org/entity/Q3505012> ;
	skos:broader	medtop:20000560 .

medtop:20001143
	rdf:type skos:Concept ;
	skos:prefLabel	"party"@en-GB ;
	skos:definition	"A social gathering of invited guests, often involving eating, drinking, dancing or the playing of games"@en-GB ;
	skos:inScheme <http://cv.iptc.org/newscodes/mediatopic/>  ;
	ikos:created "2012-10-04T12:00:00+00:00"^^xsd:dateTime ;
	dct:created "2012-10-04T12:00:00+00:00"^^xsd:dateTime ;
	ikos:modified "2021-07-12T12:00:00+00:00"^^xsd:dateTime ;
	dct:modified "2021-07-12T12:00:00+00:00"^^xsd:dateTime  ;
	skos:exactMatch <https://www.wikidata.org/entity/Q200538> ;
	skos:broader	medtop:20000565 .

medtop:20001144
	rdf:type skos:Concept ;
	skos:prefLabel	"civilian service"@en-GB ;
	skos:definition	"Unpaid service for the community as civilian"@en-GB ;
	skos:inScheme <http://cv.iptc.org/newscodes/mediatopic/>  ;
	ikos:created "2012-10-04T12:00:00+00:00"^^xsd:dateTime ;
	dct:created "2012-10-04T12:00:00+00:00"^^xsd:dateTime ;
	ikos:modified "2021-07-12T12:00:00+00:00"^^xsd:dateTime ;
	dct:modified "2021-07-12T12:00:00+00:00"^^xsd:dateTime  ;
	skos:exactMatch <https://www.wikidata.org/entity/Q702635> ;
	skos:broader	medtop:20000594 .

medtop:20001145
	rdf:type skos:Concept ;
	skos:prefLabel	"military service"@en-GB ;
	skos:definition	"Service by an individual in an army or militia. Service may be on a volunteer basis or a result of an involuntary draft or government requirement."@en-GB ;
	skos:inScheme <http://cv.iptc.org/newscodes/mediatopic/>  ;
	ikos:created "2012-10-04T12:00:00+00:00"^^xsd:dateTime ;
	dct:created "2012-10-04T12:00:00+00:00"^^xsd:dateTime ;
	ikos:modified "2021-07-12T12:00:00+00:00"^^xsd:dateTime ;
	dct:modified "2021-07-12T12:00:00+00:00"^^xsd:dateTime  ;
	skos:exactMatch <https://www.wikidata.org/entity/Q209572> ;
	skos:broader	medtop:20000599 .

medtop:20001146
	rdf:type skos:Concept ;
	skos:prefLabel	"integration policy"@en-GB ;
	skos:definition	"Improving the co-existence of groups of the society"@en-GB ;
	skos:inScheme <http://cv.iptc.org/newscodes/mediatopic/>  ;
	ikos:created "2012-10-04T12:00:00+00:00"^^xsd:dateTime ;
	dct:created "2012-10-04T12:00:00+00:00"^^xsd:dateTime ;
	ikos:modified "2021-07-12T12:00:00+00:00"^^xsd:dateTime ;
	dct:modified "2021-07-12T12:00:00+00:00"^^xsd:dateTime  ;
	skos:exactMatch <https://www.wikidata.org/entity/Q370735> ;
	skos:broader	medtop:20000626 .

medtop:20001147
	rdf:type skos:Concept ;
	skos:prefLabel	"sports policies"@en-GB ;
	skos:definition	"Government policies affecting sports"@en-GB ;
	skos:inScheme <http://cv.iptc.org/newscodes/mediatopic/>  ;
	ikos:created "2012-10-04T12:00:00+00:00"^^xsd:dateTime ;
	dct:created "2012-10-04T12:00:00+00:00"^^xsd:dateTime ;
	ikos:modified "2021-07-12T12:00:00+00:00"^^xsd:dateTime ;
	dct:modified "2021-07-12T12:00:00+00:00"^^xsd:dateTime  ;
	skos:broader	medtop:20000621 .

medtop:20001148
	rdf:type skos:Concept ;
	skos:prefLabel	"sports transaction"@en-GB ;
	skos:definition	"The transfer of an athlete from one team to another, the hiring or drafting of an athlete onto a team or the change in professional status of a player on a team"@en-GB ;
	skos:inScheme <http://cv.iptc.org/newscodes/mediatopic/>  ;
	ikos:created "2012-10-04T12:00:00+00:00"^^xsd:dateTime ;
	dct:created "2012-10-04T12:00:00+00:00"^^xsd:dateTime ;
	ikos:modified "2021-07-12T12:00:00+00:00"^^xsd:dateTime ;
	dct:modified "2021-07-12T12:00:00+00:00"^^xsd:dateTime  ;
	skos:exactMatch <https://www.wikidata.org/wiki/Q18515440> ;
	skos:broader	medtop:15000000 .

medtop:20001149
	rdf:type skos:Concept ;
	skos:prefLabel	"cross-country skiing"@en-GB ;
	skos:definition	"Nordic ski race competed in relatively-flat, snowy countryside on narrow skis."@en-GB ;
	skos:note	"Was retired but reinstated in August 2019"@en-GB ;
	skos:inScheme <http://cv.iptc.org/newscodes/mediatopic/>  ;
	ikos:created "2014-01-17T12:00:00+00:00"^^xsd:dateTime ;
	dct:created "2014-01-17T12:00:00+00:00"^^xsd:dateTime ;
	ikos:modified "2021-02-18T12:00:00+00:00"^^xsd:dateTime ;
	dct:modified "2021-02-18T12:00:00+00:00"^^xsd:dateTime  ;
	skos:exactMatch subj:15043001 ;
	skos:exactMatch <https://www.wikidata.org/entity/Q179687> ;
	skos:broader	medtop:20001056 .

medtop:20001150
	rdf:type skos:Concept ;
	skos:prefLabel	"Nordic combined"@en-GB ;
	skos:definition	"Competition combining cross-country skiing and ski jumping"@en-GB ;
	skos:note	"Was retired but reinstated in August 2019"@en-GB ;
	skos:inScheme <http://cv.iptc.org/newscodes/mediatopic/>  ;
	ikos:created "2014-01-20T12:00:00+00:00"^^xsd:dateTime ;
	dct:created "2014-01-20T12:00:00+00:00"^^xsd:dateTime ;
	ikos:modified "2021-02-18T12:00:00+00:00"^^xsd:dateTime ;
	dct:modified "2021-02-18T12:00:00+00:00"^^xsd:dateTime  ;
	skos:exactMatch subj:15043013 ;
	skos:exactMatch <https://www.wikidata.org/entity/Q201965> ;
	skos:broader	medtop:20001056 .

medtop:20001151
	rdf:type skos:Concept ;
	skos:prefLabel	"short track speed skating"@en-GB ;
	skos:definition	"Races competed by four or more skaters at a time on a small oval ice track"@en-GB ;
	skos:inScheme <http://cv.iptc.org/newscodes/mediatopic/>  ;
	ikos:created "2014-01-20T12:00:00+00:00"^^xsd:dateTime ;
	dct:created "2014-01-20T12:00:00+00:00"^^xsd:dateTime ;
	ikos:modified "2021-02-18T12:00:00+00:00"^^xsd:dateTime ;
	dct:modified "2021-02-18T12:00:00+00:00"^^xsd:dateTime  ;
	skos:exactMatch subj:15056007 ;
	skos:exactMatch <https://www.wikidata.org/entity/Q193654> ;
	skos:broader	medtop:20000822 .

medtop:20001152
	rdf:type skos:Concept ;
	skos:prefLabel	"artistic gymnastics"@en-GB ;
	skos:definition	"Gymnasts perform artistic and acrobatic moves on different apparatus. There are 6 events for men and 4 for women"@en-GB ;
	skos:inScheme <http://cv.iptc.org/newscodes/mediatopic/>  ;
	ikos:created "2014-04-11T12:00:00+00:00"^^xsd:dateTime ;
	dct:created "2014-04-11T12:00:00+00:00"^^xsd:dateTime ;
	ikos:modified "2021-07-12T12:00:00+00:00"^^xsd:dateTime ;
	dct:modified "2021-07-12T12:00:00+00:00"^^xsd:dateTime  ;
	ikos:hasFacet aspfacet:artisticgymtype ;
	skos:exactMatch <https://www.wikidata.org/entity/Q326827> ;
	skos:broader	medtop:20000942 ;
	skos:narrower	medtop:20000944 ;
	skos:narrower	medtop:20000946 ;
	skos:narrower	medtop:20000948 ;
	skos:narrower	medtop:20000949 ;
	skos:narrower	medtop:20000950 ;
	skos:narrower	medtop:20000953 ;
	skos:narrower	medtop:20000956 ;
	skos:narrower	medtop:20000957 .

medtop:20001153
	rdf:type skos:Concept ;
	skos:prefLabel	"Telemark skiing"@en-GB ;
	skos:definition	"Races combining downhill and cross-country skiing events with unique Telemark techniques and equipment."@en-GB ;
	skos:inScheme <http://cv.iptc.org/newscodes/mediatopic/>  ;
	ikos:created "2014-11-07T12:00:00+00:00"^^xsd:dateTime ;
	dct:created "2014-11-07T12:00:00+00:00"^^xsd:dateTime ;
	ikos:modified "2021-07-12T12:00:00+00:00"^^xsd:dateTime ;
	dct:modified "2021-07-12T12:00:00+00:00"^^xsd:dateTime  ;
	skos:exactMatch <https://www.wikidata.org/entity/Q50620> ;
	skos:broader	medtop:20001056 .

medtop:20001154
	rdf:type skos:Concept ;
	skos:prefLabel	"chess"@en-GB ;
	skos:definition	"Competition between two players using a chequered board with 16 pieces to each side, each with specific ranges of movement depending on their identity"@en-GB ;
	skos:inScheme <http://cv.iptc.org/newscodes/mediatopic/>  ;
	ikos:created "2014-11-07T12:00:00+00:00"^^xsd:dateTime ;
	dct:created "2014-11-07T12:00:00+00:00"^^xsd:dateTime ;
	ikos:modified "2021-07-12T12:00:00+00:00"^^xsd:dateTime ;
	dct:modified "2021-07-12T12:00:00+00:00"^^xsd:dateTime  ;
	skos:exactMatch <https://www.wikidata.org/entity/Q718> ;
	skos:broader	medtop:20000822 .

medtop:20001155
	rdf:type skos:Concept ;
	skos:prefLabel	"roller sports"@en-GB ;
	skos:definition	"Various competitions using wheeled equipment such as roller skates, inline skates, and skateboards."@en-GB ;
	skos:inScheme <http://cv.iptc.org/newscodes/mediatopic/>  ;
	ikos:created "2014-11-07T12:00:00+00:00"^^xsd:dateTime ;
	dct:created "2014-11-07T12:00:00+00:00"^^xsd:dateTime ;
	ikos:modified "2021-07-12T12:00:00+00:00"^^xsd:dateTime ;
	dct:modified "2021-07-12T12:00:00+00:00"^^xsd:dateTime  ;
	skos:exactMatch <https://www.wikidata.org/entity/Q2164355> ;
	skos:broader	medtop:20000822 ;
	skos:narrower	medtop:20001025 ;
	skos:narrower	medtop:20001156 .

medtop:20001156
	rdf:type skos:Concept ;
	skos:prefLabel	"skateboarding"@en-GB ;
	skos:definition	"Competitions involving stunts and acrobatic feats performed on a skateboard using various ramps and other obstacles"@en-GB ;
	skos:inScheme <http://cv.iptc.org/newscodes/mediatopic/>  ;
	ikos:created "2014-11-07T12:00:00+00:00"^^xsd:dateTime ;
	dct:created "2014-11-07T12:00:00+00:00"^^xsd:dateTime ;
	ikos:modified "2021-07-12T12:00:00+00:00"^^xsd:dateTime ;
	dct:modified "2021-07-12T12:00:00+00:00"^^xsd:dateTime  ;
	skos:exactMatch <https://www.wikidata.org/entity/Q842284> ;
	skos:broader	medtop:20001155 .

medtop:20001157
	rdf:type skos:Concept ;
	skos:prefLabel	"martial arts"@en-GB ;
	skos:definition	"Martial arts are codified systems and traditions of combat practices, which are practiced for a variety of reasons: self-defence, competition, physical health and fitness, entertainment, as well as mental, physical, and spiritual development."@en-GB ;
	skos:inScheme <http://cv.iptc.org/newscodes/mediatopic/>  ;
	ikos:created "2015-08-27T12:00:00+00:00"^^xsd:dateTime ;
	dct:created "2015-08-27T12:00:00+00:00"^^xsd:dateTime ;
	ikos:modified "2021-07-12T12:00:00+00:00"^^xsd:dateTime ;
	dct:modified "2021-07-12T12:00:00+00:00"^^xsd:dateTime  ;
	skos:exactMatch <https://www.wikidata.org/entity/Q11417> ;
	skos:broader	medtop:20000822 ;
	skos:narrower	medtop:20000969 ;
	skos:narrower	medtop:20000977 ;
	skos:narrower	medtop:20000983 ;
	skos:narrower	medtop:20000984 ;
	skos:narrower	medtop:20000985 ;
	skos:narrower	medtop:20001009 ;
	skos:narrower	medtop:20001084 ;
	skos:narrower	medtop:20001102 ;
	skos:narrower	medtop:20001231 ;
	skos:narrower	medtop:20001308 ;
	skos:narrower	medtop:20001310 ;
	skos:narrower	medtop:20001311 .

medtop:20001158
	rdf:type skos:Concept ;
	skos:prefLabel	"entrepreneurship"@en-GB ;
	skos:definition	"The process of designing, launching and running a new business."@en-GB ;
	skos:inScheme <http://cv.iptc.org/newscodes/mediatopic/>  ;
	ikos:created "2016-04-04T12:00:00+00:00"^^xsd:dateTime ;
	dct:created "2016-04-04T12:00:00+00:00"^^xsd:dateTime ;
	ikos:modified "2021-07-12T12:00:00+00:00"^^xsd:dateTime ;
	dct:modified "2021-07-12T12:00:00+00:00"^^xsd:dateTime  ;
	skos:exactMatch <https://www.wikidata.org/entity/Q3908516> ;
	skos:broader	medtop:20000349 .

medtop:20001159
	rdf:type skos:Concept ;
	skos:prefLabel	"public contract"@en-GB ;
	skos:definition	"Written contracts between companies and public authorities for the execution of works, the supply of products or the provision of services."@en-GB ;
	skos:inScheme <http://cv.iptc.org/newscodes/mediatopic/>  ;
	ikos:created "2016-04-04T12:00:00+00:00"^^xsd:dateTime ;
	dct:created "2016-04-04T12:00:00+00:00"^^xsd:dateTime ;
	ikos:modified "2021-07-12T12:00:00+00:00"^^xsd:dateTime ;
	dct:modified "2021-07-12T12:00:00+00:00"^^xsd:dateTime  ;
	skos:exactMatch <https://www.wikidata.org/entity/Q529458> ;
	skos:broader	medtop:20000192 .

medtop:20001160
	rdf:type skos:Concept ;
	skos:prefLabel	"handicrafts"@en-GB ;
	skos:definition	"The creators and sellers of crafts and the making and selling of the supplies used to make those crafts"@en-GB ;
	skos:inScheme <http://cv.iptc.org/newscodes/mediatopic/>  ;
	ikos:created "2016-04-04T12:00:00+00:00"^^xsd:dateTime ;
	dct:created "2016-04-04T12:00:00+00:00"^^xsd:dateTime ;
	ikos:modified "2023-03-31T12:00:00+00:00"^^xsd:dateTime ;
	dct:modified "2023-03-31T12:00:00+00:00"^^xsd:dateTime  ;
	skos:exactMatch <https://www.wikidata.org/entity/Q877729> ;
	skos:broader	medtop:20000243 .

medtop:20001161
	rdf:type skos:Concept ;
	skos:prefLabel	"Internet of Things"@en-GB ;
	skos:definition	"A network of devices using microchips, electronic sensors and communication by the Internet"@en-GB ;
	skos:changeNote	"Retired. Use medtop:20000226 hardware, or generic medtop:20000225 computing and information technology as appropriate."@en-GB ;
	skos:inScheme <http://cv.iptc.org/newscodes/mediatopic/>  ;
	ikos:created "2016-04-04T12:00:00+00:00"^^xsd:dateTime ;
	dct:created "2016-04-04T12:00:00+00:00"^^xsd:dateTime ;
	ikos:modified "2023-03-31T12:00:00+00:00"^^xsd:dateTime ;
	dct:modified "2023-03-31T12:00:00+00:00"^^xsd:dateTime  ; 
	ikos:retired "2023-03-31T12:00:00+00:00"^^xsd:dateTime ;
	skos:exactMatch <https://www.wikidata.org/entity/Q251212> ;
	skos:broader	medtop:20000225 .

medtop:20001162
	rdf:type skos:Concept ;
	skos:prefLabel	"asset management"@en-GB ;
	skos:definition	"Managing investments on behalf of others"@en-GB ;
	skos:inScheme <http://cv.iptc.org/newscodes/mediatopic/>  ;
	ikos:created "2016-04-04T12:00:00+00:00"^^xsd:dateTime ;
	dct:created "2016-04-04T12:00:00+00:00"^^xsd:dateTime ;
	ikos:modified "2023-03-31T12:00:00+00:00"^^xsd:dateTime ;
	dct:modified "2023-03-31T12:00:00+00:00"^^xsd:dateTime  ;
	skos:exactMatch <https://www.wikidata.org/entity/Q873442> ;
	skos:broader	medtop:20001370 .

medtop:20001163
	rdf:type skos:Concept ;
	skos:prefLabel	"client relationship management"@en-GB ;
	skos:definition	"Creating and maintaining a relationship with the customers to increase sales."@en-GB ;
	skos:inScheme <http://cv.iptc.org/newscodes/mediatopic/>  ;
	ikos:created "2016-04-04T12:00:00+00:00"^^xsd:dateTime ;
	dct:created "2016-04-04T12:00:00+00:00"^^xsd:dateTime ;
	ikos:modified "2023-03-31T12:00:00+00:00"^^xsd:dateTime ;
	dct:modified "2023-03-31T12:00:00+00:00"^^xsd:dateTime  ;
	skos:exactMatch <https://www.wikidata.org/entity/Q485643> ;
	skos:broader	medtop:20000192 .

medtop:20001164
	rdf:type skos:Concept ;
	skos:prefLabel	"payment service"@en-GB ;
	skos:definition	"Services for executing payments including cash, cheque, credit card, debit card, direct debit, electronic funds transfer, internet banking, electronic and mobile payment."@en-GB ;
	skos:inScheme <http://cv.iptc.org/newscodes/mediatopic/>  ;
	ikos:created "2016-04-04T12:00:00+00:00"^^xsd:dateTime ;
	dct:created "2016-04-04T12:00:00+00:00"^^xsd:dateTime ;
	ikos:modified "2023-03-31T12:00:00+00:00"^^xsd:dateTime ;
	dct:modified "2023-03-31T12:00:00+00:00"^^xsd:dateTime  ;
	skos:exactMatch <https://www.wikidata.org/entity/Q986008> ;
	skos:broader	medtop:20001371 .

medtop:20001165
	rdf:type skos:Concept ;
	skos:prefLabel	"capital goods"@en-GB ;
	skos:definition	"Durable goods used in the production of other goods or services."@en-GB ;
	skos:inScheme <http://cv.iptc.org/newscodes/mediatopic/>  ;
	ikos:created "2016-04-04T12:00:00+00:00"^^xsd:dateTime ;
	dct:created "2016-04-04T12:00:00+00:00"^^xsd:dateTime ;
	ikos:modified "2023-03-31T12:00:00+00:00"^^xsd:dateTime ;
	dct:modified "2023-03-31T12:00:00+00:00"^^xsd:dateTime  ; 
	ikos:retired "2023-03-31T12:00:00+00:00"^^xsd:dateTime ;
	skos:exactMatch <https://www.wikidata.org/entity/Q56573293> ;
	skos:broader	medtop:20000294 .

medtop:20001166
	rdf:type skos:Concept ;
	skos:prefLabel	"railway manufacturing"@en-GB ;
	skos:definition	"Manufactures of rolling stock and suppliers for the maintenance and repair of railroads"@en-GB ;
	skos:inScheme <http://cv.iptc.org/newscodes/mediatopic/>  ;
	ikos:created "2016-04-04T12:00:00+00:00"^^xsd:dateTime ;
	dct:created "2016-04-04T12:00:00+00:00"^^xsd:dateTime ;
	ikos:modified "2023-03-31T12:00:00+00:00"^^xsd:dateTime ;
	dct:modified "2023-03-31T12:00:00+00:00"^^xsd:dateTime  ;
	skos:exactMatch <https://www.wikidata.org/entity/Q2995256> ;
	skos:broader	medtop:20000294 .

medtop:20001167
	rdf:type skos:Concept ;
	skos:prefLabel	"medical equipment"@en-GB ;
	skos:definition	"Manufacture of medical and surgical devices for diagnosis and treatment such as optical and imaging equipment"@en-GB ;
	skos:inScheme <http://cv.iptc.org/newscodes/mediatopic/>  ;
	ikos:created "2016-04-04T12:00:00+00:00"^^xsd:dateTime ;
	dct:created "2016-04-04T12:00:00+00:00"^^xsd:dateTime ;
	ikos:modified "2023-03-31T12:00:00+00:00"^^xsd:dateTime ;
	dct:modified "2023-03-31T12:00:00+00:00"^^xsd:dateTime  ;
	skos:exactMatch <https://www.wikidata.org/wiki/Q63383285> ;
	skos:broader	medtop:20001354 .

medtop:20001168
	rdf:type skos:Concept ;
	skos:prefLabel	"pet product and service"@en-GB ;
	skos:definition	"Hygiene products, care and nutrition for pets"@en-GB ;
	skos:inScheme <http://cv.iptc.org/newscodes/mediatopic/>  ;
	ikos:created "2016-04-04T12:00:00+00:00"^^xsd:dateTime ;
	dct:created "2016-04-04T12:00:00+00:00"^^xsd:dateTime ;
	ikos:modified "2023-03-31T12:00:00+00:00"^^xsd:dateTime ;
	dct:modified "2023-03-31T12:00:00+00:00"^^xsd:dateTime  ;
	skos:exactMatch <https://www.wikidata.org/entity/Q85792903> ;
	skos:broader	medtop:20000243 .

medtop:20001169
	rdf:type skos:Concept ;
	skos:prefLabel	"e-cigarette"@en-GB ;
	skos:definition	"An electronic cigarette is a battery-operated device with an atomizer and a cartridge containing either a nicotine or a non-nicotine liquid solution."@en-GB ;
	skos:changeNote	"Retired. Use medtop:20000330 tobacco and nicotine instead."@en-GB ;
	skos:inScheme <http://cv.iptc.org/newscodes/mediatopic/>  ;
	ikos:created "2016-04-04T12:00:00+00:00"^^xsd:dateTime ;
	dct:created "2016-04-04T12:00:00+00:00"^^xsd:dateTime ;
	ikos:modified "2023-03-31T12:00:00+00:00"^^xsd:dateTime ;
	dct:modified "2023-03-31T12:00:00+00:00"^^xsd:dateTime  ; 
	ikos:retired "2023-03-31T12:00:00+00:00"^^xsd:dateTime ;
	skos:exactMatch <https://www.wikidata.org/entity/Q189511> ;
	skos:broader	medtop:20000322 .

medtop:20001170
	rdf:type skos:Concept ;
	skos:prefLabel	"logistics"@en-GB ;
	skos:definition	"Supply chain, inventory management and transportation of products."@en-GB ;
	skos:inScheme <http://cv.iptc.org/newscodes/mediatopic/>  ;
	ikos:created "2016-04-04T12:00:00+00:00"^^xsd:dateTime ;
	dct:created "2016-04-04T12:00:00+00:00"^^xsd:dateTime ;
	ikos:modified "2023-03-31T12:00:00+00:00"^^xsd:dateTime ;
	dct:modified "2023-03-31T12:00:00+00:00"^^xsd:dateTime  ;
	skos:exactMatch <https://www.wikidata.org/entity/Q177777> ;
	skos:broader	medtop:20000337 .

medtop:20001171
	rdf:type skos:Concept ;
	skos:prefLabel	"sharing economy"@en-GB ;
	skos:definition	"Peer-to-peer-based sharing of access to goods and services."@en-GB ;
	skos:inScheme <http://cv.iptc.org/newscodes/mediatopic/>  ;
	ikos:created "2016-04-04T12:00:00+00:00"^^xsd:dateTime ;
	dct:created "2016-04-04T12:00:00+00:00"^^xsd:dateTime ;
	ikos:modified "2021-07-12T12:00:00+00:00"^^xsd:dateTime ;
	dct:modified "2021-07-12T12:00:00+00:00"^^xsd:dateTime  ;
	skos:exactMatch <https://www.wikidata.org/entity/Q2277143> ;
	skos:broader	medtop:20000344 .

medtop:20001172
	rdf:type skos:Concept ;
	skos:prefLabel	"small and medium enterprise"@en-GB ;
	skos:definition	"A small and medium enterprise (SME) is a company whose number of employees, balance, and turnover cannot exceed certain limits set by the country where it is located."@en-GB ;
	skos:inScheme <http://cv.iptc.org/newscodes/mediatopic/>  ;
	ikos:created "2016-04-04T12:00:00+00:00"^^xsd:dateTime ;
	dct:created "2016-04-04T12:00:00+00:00"^^xsd:dateTime ;
	ikos:modified "2021-07-12T12:00:00+00:00"^^xsd:dateTime ;
	dct:modified "2021-07-12T12:00:00+00:00"^^xsd:dateTime  ;
	skos:exactMatch <https://www.wikidata.org/entity/Q622439> ;
	skos:broader	medtop:20000349 .

medtop:20001173
	rdf:type skos:Concept ;
	skos:prefLabel	"regulatory authority"@en-GB ;
	skos:definition	"Authority responsible for the regulation or supervision of a business sector."@en-GB ;
	skos:inScheme <http://cv.iptc.org/newscodes/mediatopic/>  ;
	ikos:created "2016-04-04T12:00:00+00:00"^^xsd:dateTime ;
	dct:created "2016-04-04T12:00:00+00:00"^^xsd:dateTime ;
	ikos:modified "2021-07-12T12:00:00+00:00"^^xsd:dateTime ;
	dct:modified "2021-07-12T12:00:00+00:00"^^xsd:dateTime  ;
	skos:exactMatch <https://www.wikidata.org/entity/Q55875130> ;
	skos:broader	medtop:20000593 .

medtop:20001174
	rdf:type skos:Concept ;
	skos:prefLabel	"regional development policy"@en-GB ;
	skos:definition	"Public or private actions carried out to develop a region."@en-GB ;
	skos:inScheme <http://cv.iptc.org/newscodes/mediatopic/>  ;
	ikos:created "2016-04-04T12:00:00+00:00"^^xsd:dateTime ;
	dct:created "2016-04-04T12:00:00+00:00"^^xsd:dateTime ;
	ikos:modified "2021-07-12T12:00:00+00:00"^^xsd:dateTime ;
	dct:modified "2021-07-12T12:00:00+00:00"^^xsd:dateTime  ;
	skos:exactMatch <https://www.wikidata.org/entity/Q482379> ;
	skos:broader	medtop:20000626 .

medtop:20001175
	rdf:type skos:Concept ;
	skos:prefLabel	"artistic swimming"@en-GB ;
	skos:definition	"A sport in which swimmers, in solo, duet or team configurations, perform coordinated or identical movements in time to music. They are judged and are awarded points for body position, control, and the degree of difficulty of the moves."@en-GB ;
	skos:inScheme <http://cv.iptc.org/newscodes/mediatopic/>  ;
	ikos:created "2016-04-05T12:00:00+00:00"^^xsd:dateTime ;
	dct:created "2016-04-05T12:00:00+00:00"^^xsd:dateTime ;
	ikos:modified "2021-07-12T12:00:00+00:00"^^xsd:dateTime ;
	dct:modified "2021-07-12T12:00:00+00:00"^^xsd:dateTime  ;
	skos:exactMatch <https://www.wikidata.org/entity/Q180692> ;
	skos:broader	medtop:20000822 ;
	skos:narrower	medtop:20001081 ;
	skos:narrower	medtop:20001082 .

medtop:20001176
	rdf:type skos:Concept ;
	skos:prefLabel	"rugby"@en-GB ;
	skos:definition	"A form of football developed in Rugby (England) played with an oval ball that may be kicked, carried and passed from hand to hand. Points are scored when one team carries the ball over the other team's goal line or kicks the ball between two goal posts."@en-GB ;
	skos:inScheme <http://cv.iptc.org/newscodes/mediatopic/>  ;
	ikos:created "2016-04-05T12:00:00+00:00"^^xsd:dateTime ;
	dct:created "2016-04-05T12:00:00+00:00"^^xsd:dateTime ;
	ikos:modified "2021-07-12T12:00:00+00:00"^^xsd:dateTime ;
	dct:modified "2021-07-12T12:00:00+00:00"^^xsd:dateTime  ;
	skos:exactMatch <https://www.wikidata.org/entity/Q5378> ;
	skos:broader	medtop:20000822 ;
	skos:narrower	medtop:20001035 ;
	skos:narrower	medtop:20001036 ;
	skos:narrower	medtop:20001037 .

medtop:20001177
	rdf:type skos:Concept ;
	skos:prefLabel	"Olympic Games"@en-GB ;
	skos:definition	"Games organised by the International Olympic Committee and held each 4 years in summer or winter."@en-GB ;
	skos:inScheme <http://cv.iptc.org/newscodes/mediatopic/>  ;
	ikos:created "2016-08-24T12:00:00+00:00"^^xsd:dateTime ;
	dct:created "2016-08-24T12:00:00+00:00"^^xsd:dateTime ;
	ikos:modified "2021-12-17T12:00:00+00:00"^^xsd:dateTime ;
	dct:modified "2021-12-17T12:00:00+00:00"^^xsd:dateTime  ;
	skos:exactMatch <https://www.wikidata.org/entity/Q5389> ;
	skos:broader	medtop:20001108 .

medtop:20001178
	rdf:type skos:Concept ;
	skos:prefLabel	"Paralympic Games"@en-GB ;
	skos:definition	"Games for disabled athletes organised by the International Paralympic Committee and held each 4 years in winter or summer"@en-GB ;
	skos:inScheme <http://cv.iptc.org/newscodes/mediatopic/>  ;
	ikos:created "2016-08-24T12:00:00+00:00"^^xsd:dateTime ;
	dct:created "2016-08-24T12:00:00+00:00"^^xsd:dateTime ;
	ikos:modified "2021-12-17T12:00:00+00:00"^^xsd:dateTime ;
	dct:modified "2021-12-17T12:00:00+00:00"^^xsd:dateTime  ;
	skos:exactMatch <https://www.wikidata.org/entity/Q73633> ;
	skos:broader	medtop:20001108 .

medtop:20001179
	rdf:type skos:Concept ;
	skos:prefLabel	"series"@en-GB ;
	skos:definition	"A connected set of fictional or non-fictional program episodes that run under the same title."@en-GB ;
	skos:inScheme <http://cv.iptc.org/newscodes/mediatopic/>  ;
	ikos:created "2017-11-16T12:00:00+00:00"^^xsd:dateTime ;
	dct:created "2017-11-16T12:00:00+00:00"^^xsd:dateTime ;
	ikos:modified "2021-07-12T12:00:00+00:00"^^xsd:dateTime ;
	dct:modified "2021-07-12T12:00:00+00:00"^^xsd:dateTime  ;
	skos:exactMatch <https://www.wikidata.org/wiki/Q7725310> ;
	skos:broader	medtop:20000002 .

medtop:20001180
	rdf:type skos:Concept ;
	skos:prefLabel	"drama (theatre)"@en-GB ;
	skos:definition	"A genre of theatre where dramatic or comedic plays are performed on the stage"@en-GB ;
	skos:inScheme <http://cv.iptc.org/newscodes/mediatopic/>  ;
	ikos:created "2018-04-09T12:00:00+00:00"^^xsd:dateTime ;
	dct:created "2018-04-09T12:00:00+00:00"^^xsd:dateTime ;
	ikos:modified "2021-07-12T12:00:00+00:00"^^xsd:dateTime ;
	dct:modified "2021-07-12T12:00:00+00:00"^^xsd:dateTime  ;
	skos:exactMatch <https://www.wikidata.org/entity/Q39892385> ;
	skos:broader	medtop:20000029 .

medtop:20001181
	rdf:type skos:Concept ;
	skos:prefLabel	"festival"@en-GB ;
	skos:definition	"Events showcasing artistic endeavours, often regularly occurring, such as dance, music, theatre, poetry or comedy festivals"@en-GB ;
	skos:inScheme <http://cv.iptc.org/newscodes/mediatopic/>  ;
	ikos:created "2018-04-09T12:00:00+00:00"^^xsd:dateTime ;
	dct:created "2018-04-09T12:00:00+00:00"^^xsd:dateTime ;
	ikos:modified "2021-07-12T12:00:00+00:00"^^xsd:dateTime ;
	dct:modified "2021-07-12T12:00:00+00:00"^^xsd:dateTime  ;
	skos:exactMatch <https://www.wikidata.org/entity/Q4801521> ;
	skos:broader	medtop:20000002 ;
	skos:narrower	medtop:20000006 .

medtop:20001182
	rdf:type skos:Concept ;
	skos:prefLabel	"social media"@en-GB ;
	skos:definition	"Content created to be shared within online social networks"@en-GB ;
	skos:inScheme <http://cv.iptc.org/newscodes/mediatopic/>  ;
	ikos:created "2018-04-09T12:00:00+00:00"^^xsd:dateTime ;
	dct:created "2018-04-09T12:00:00+00:00"^^xsd:dateTime ;
	ikos:modified "2021-07-12T12:00:00+00:00"^^xsd:dateTime ;
	dct:modified "2021-07-12T12:00:00+00:00"^^xsd:dateTime  ;
	skos:exactMatch <https://www.wikidata.org/entity/Q202833> ;
	skos:broader	medtop:20000045 ;
	skos:narrower	medtop:20001192 .

medtop:20001183
	rdf:type skos:Concept ;
	skos:prefLabel	"eSports"@en-GB ;
	skos:definition	"Competitions involving video games played by professional gamers"@en-GB ;
	skos:inScheme <http://cv.iptc.org/newscodes/mediatopic/>  ;
	ikos:created "2018-04-19T12:00:00+00:00"^^xsd:dateTime ;
	dct:created "2018-04-19T12:00:00+00:00"^^xsd:dateTime ;
	ikos:modified "2021-07-12T12:00:00+00:00"^^xsd:dateTime ;
	dct:modified "2021-07-12T12:00:00+00:00"^^xsd:dateTime  ;
	skos:exactMatch <https://www.wikidata.org/entity/Q300920> ;
	skos:broader	medtop:20000822 .

medtop:20001184
	rdf:type skos:Concept ;
	skos:prefLabel	"hip hop"@en-GB ;
	skos:definition	"A genre of music developed in African American communities in the United States in the 1970s which consists of rapping usually with an electronic backing"@en-GB ;
	skos:inScheme <http://cv.iptc.org/newscodes/mediatopic/>  ;
	ikos:created "2019-04-06T12:00:00+00:00"^^xsd:dateTime ;
	dct:created "2019-04-06T12:00:00+00:00"^^xsd:dateTime ;
	ikos:modified "2021-07-12T12:00:00+00:00"^^xsd:dateTime ;
	dct:modified "2021-07-12T12:00:00+00:00"^^xsd:dateTime  ;
	skos:exactMatch <https://www.wikidata.org/entity/Q11401> ;
	skos:broader	medtop:20000021 .

medtop:20001185
	rdf:type skos:Concept ;
	skos:prefLabel	"r&b"@en-GB ;
	skos:definition	"A genre of music originated in African American communities in the 1940s and featuring soulful vocals"@en-GB ;
	skos:inScheme <http://cv.iptc.org/newscodes/mediatopic/>  ;
	ikos:created "2019-04-06T12:00:00+00:00"^^xsd:dateTime ;
	dct:created "2019-04-06T12:00:00+00:00"^^xsd:dateTime ;
	ikos:modified "2021-07-12T12:00:00+00:00"^^xsd:dateTime ;
	dct:modified "2021-07-12T12:00:00+00:00"^^xsd:dateTime  ;
	skos:exactMatch <https://www.wikidata.org/entity/Q45981> ;
	skos:broader	medtop:20000021 .

medtop:20001186
	rdf:type skos:Concept ;
	skos:prefLabel	"heavy metal"@en-GB ;
	skos:definition	"A genre of loud, aggressive rock music that was developed in the late 1960s and early 1970s"@en-GB ;
	skos:inScheme <http://cv.iptc.org/newscodes/mediatopic/>  ;
	ikos:created "2019-04-06T12:00:00+00:00"^^xsd:dateTime ;
	dct:created "2019-04-06T12:00:00+00:00"^^xsd:dateTime ;
	ikos:modified "2021-07-12T12:00:00+00:00"^^xsd:dateTime ;
	dct:modified "2021-07-12T12:00:00+00:00"^^xsd:dateTime  ;
	skos:exactMatch <https://www.wikidata.org/entity/Q38848> ;
	skos:broader	medtop:20000021 .

medtop:20001187
	rdf:type skos:Concept ;
	skos:prefLabel	"dance band music"@en-GB ;
	skos:definition	"A Swedish genre of music characterized by music inspired by swing, schlager, country, jazz and rock that is often danced to in pairs"@en-GB ;
	skos:inScheme <http://cv.iptc.org/newscodes/mediatopic/>  ;
	ikos:created "2019-04-06T12:00:00+00:00"^^xsd:dateTime ;
	dct:created "2019-04-06T12:00:00+00:00"^^xsd:dateTime ;
	ikos:modified "2021-07-12T12:00:00+00:00"^^xsd:dateTime ;
	dct:modified "2021-07-12T12:00:00+00:00"^^xsd:dateTime  ;
	skos:exactMatch <https://www.wikidata.org/entity/Q1164847> ;
	skos:broader	medtop:20000021 .

medtop:20001188
	rdf:type skos:Concept ;
	skos:prefLabel	"electronic dance music"@en-GB ;
	skos:definition	"A genre of music that employs electronic instruments and is primarily made for nightclubs, raves, and festivals"@en-GB ;
	skos:inScheme <http://cv.iptc.org/newscodes/mediatopic/>  ;
	ikos:created "2019-04-06T12:00:00+00:00"^^xsd:dateTime ;
	dct:created "2019-04-06T12:00:00+00:00"^^xsd:dateTime ;
	ikos:modified "2021-07-12T12:00:00+00:00"^^xsd:dateTime ;
	dct:modified "2021-07-12T12:00:00+00:00"^^xsd:dateTime  ;
	skos:exactMatch <https://www.wikidata.org/entity/Q851213> ;
	skos:broader	medtop:20000021 .

medtop:20001189
	rdf:type skos:Concept ;
	skos:prefLabel	"children's music"@en-GB ;
	skos:definition	"A genre of music featuring songs composed and performed for children"@en-GB ;
	skos:inScheme <http://cv.iptc.org/newscodes/mediatopic/>  ;
	ikos:created "2019-04-06T12:00:00+00:00"^^xsd:dateTime ;
	dct:created "2019-04-06T12:00:00+00:00"^^xsd:dateTime ;
	ikos:modified "2021-07-12T12:00:00+00:00"^^xsd:dateTime ;
	dct:modified "2021-07-12T12:00:00+00:00"^^xsd:dateTime  ;
	skos:exactMatch <https://www.wikidata.org/entity/Q493169> ;
	skos:broader	medtop:20000021 .

medtop:20001190
	rdf:type skos:Concept ;
	skos:prefLabel	"stand-up comedy"@en-GB ;
	skos:definition	"A comic style in which a comedian performs a series of jokes or stories in front of a live audience, usually speaking directly to them"@en-GB ;
	skos:inScheme <http://cv.iptc.org/newscodes/mediatopic/>  ;
	ikos:created "2019-04-06T12:00:00+00:00"^^xsd:dateTime ;
	dct:created "2019-04-06T12:00:00+00:00"^^xsd:dateTime ;
	ikos:modified "2021-07-12T12:00:00+00:00"^^xsd:dateTime ;
	dct:modified "2021-07-12T12:00:00+00:00"^^xsd:dateTime  ;
	skos:exactMatch <https://www.wikidata.org/entity/Q145806> ;
	skos:broader	medtop:20000029 .

medtop:20001191
	rdf:type skos:Concept ;
	skos:prefLabel	"cabaret"@en-GB ;
	skos:definition	"A form of theatrical entertainment featuring music, song, dance, recitation, or drama that is performed in a nightclub or restaurant while the audience eats or drinks at tables"@en-GB ;
	skos:inScheme <http://cv.iptc.org/newscodes/mediatopic/>  ;
	ikos:created "2019-04-06T12:00:00+00:00"^^xsd:dateTime ;
	dct:created "2019-04-06T12:00:00+00:00"^^xsd:dateTime ;
	ikos:modified "2021-09-30T12:00:00+00:00"^^xsd:dateTime ;
	dct:modified "2021-09-30T12:00:00+00:00"^^xsd:dateTime  ;
	skos:exactMatch <https://www.wikidata.org/entity/Q27976507> ;
	skos:broader	medtop:20000029 .

medtop:20001192
	rdf:type skos:Concept ;
	skos:prefLabel	"influencers"@en-GB ;
	skos:definition	"Persons who distribute content on internet forums and social media and are followed by many people thereby influencing them to buy and use products"@en-GB ;
	skos:inScheme <http://cv.iptc.org/newscodes/mediatopic/>  ;
	ikos:created "2019-04-06T12:00:00+00:00"^^xsd:dateTime ;
	dct:created "2019-04-06T12:00:00+00:00"^^xsd:dateTime ;
	ikos:modified "2021-07-12T12:00:00+00:00"^^xsd:dateTime ;
	dct:modified "2021-07-12T12:00:00+00:00"^^xsd:dateTime  ;
	skos:exactMatch <https://www.wikidata.org/entity/Q2906862> ;
	skos:broader	medtop:20001182 .

medtop:20001193
	rdf:type skos:Concept ;
	skos:prefLabel	"sexual misconduct"@en-GB ;
	skos:definition	"Unwanted behaviour of a sexual nature that is of lesser offense than felony sexual assault, particularly when behavior occurs in a normally non-sexual situation, or where there is some aspect of personal power or authority involved"@en-GB ;
	skos:inScheme <http://cv.iptc.org/newscodes/mediatopic/>  ;
	ikos:created "2019-04-06T12:00:00+00:00"^^xsd:dateTime ;
	dct:created "2019-04-06T12:00:00+00:00"^^xsd:dateTime ;
	ikos:modified "2021-07-12T12:00:00+00:00"^^xsd:dateTime ;
	dct:modified "2021-07-12T12:00:00+00:00"^^xsd:dateTime  ;
	skos:exactMatch <https://www.wikidata.org/entity/Q7458798> ;
	skos:broader	medtop:20000802 .

medtop:20001194
	rdf:type skos:Concept ;
	skos:prefLabel	"accounting crime"@en-GB ;
	skos:definition	"The intentional misrepresentation or alteration of accounting records regarding sales, revenues, expenses and other factors"@en-GB ;
	skos:inScheme <http://cv.iptc.org/newscodes/mediatopic/>  ;
	ikos:created "2019-04-06T12:00:00+00:00"^^xsd:dateTime ;
	dct:created "2019-04-06T12:00:00+00:00"^^xsd:dateTime ;
	ikos:modified "2021-07-12T12:00:00+00:00"^^xsd:dateTime ;
	dct:modified "2021-07-12T12:00:00+00:00"^^xsd:dateTime  ;
	skos:exactMatch <https://www.wikidata.org/entity/Q41799931> ;
	skos:broader	medtop:20000087 .

medtop:20001195
	rdf:type skos:Concept ;
	skos:prefLabel	"tax evasion"@en-GB ;
	skos:definition	"The illegal evasion of taxes by individuals, corporations, and trusts"@en-GB ;
	skos:inScheme <http://cv.iptc.org/newscodes/mediatopic/>  ;
	ikos:created "2019-04-06T12:00:00+00:00"^^xsd:dateTime ;
	dct:created "2019-04-06T12:00:00+00:00"^^xsd:dateTime ;
	ikos:modified "2021-07-12T12:00:00+00:00"^^xsd:dateTime ;
	dct:modified "2021-07-12T12:00:00+00:00"^^xsd:dateTime  ;
	skos:exactMatch <https://www.wikidata.org/entity/Q6502151> ;
	skos:broader	medtop:20000097 .

medtop:20001196
	rdf:type skos:Concept ;
	skos:prefLabel	"reckless driving"@en-GB ;
	skos:definition	"Serious traffic violations that are likely to, or have led to, the endangerment, injury or death of a person or persons, or the endangerment of or significant property damage"@en-GB ;
	skos:inScheme <http://cv.iptc.org/newscodes/mediatopic/>  ;
	ikos:created "2019-04-06T12:00:00+00:00"^^xsd:dateTime ;
	dct:created "2019-04-06T12:00:00+00:00"^^xsd:dateTime ;
	ikos:modified "2021-07-12T12:00:00+00:00"^^xsd:dateTime ;
	dct:modified "2021-07-12T12:00:00+00:00"^^xsd:dateTime  ;
	skos:exactMatch <https://www.wikidata.org/entity/Q657433> ;
	skos:broader	medtop:20000082 .

medtop:20001197
	rdf:type skos:Concept ;
	skos:prefLabel	"administrative law"@en-GB ;
	skos:definition	"Body of law that governs the actions of governmental administrative agencies"@en-GB ;
	skos:inScheme <http://cv.iptc.org/newscodes/mediatopic/>  ;
	ikos:created "2019-04-06T12:00:00+00:00"^^xsd:dateTime ;
	dct:created "2019-04-06T12:00:00+00:00"^^xsd:dateTime ;
	ikos:modified "2021-07-12T12:00:00+00:00"^^xsd:dateTime ;
	dct:modified "2021-07-12T12:00:00+00:00"^^xsd:dateTime  ;
	skos:exactMatch <https://www.wikidata.org/entity/Q171251> ;
	skos:broader	medtop:20000121 .

medtop:20001198
	rdf:type skos:Concept ;
	skos:prefLabel	"court-ordered psychiatric treatment"@en-GB ;
	skos:definition	"Psychiatric treatment imposed upon persons with mental health conditions in prisons and jails or as a condition of probation, supervision or parole"@en-GB ;
	skos:inScheme <http://cv.iptc.org/newscodes/mediatopic/>  ;
	ikos:created "2019-04-06T12:00:00+00:00"^^xsd:dateTime ;
	dct:created "2019-04-06T12:00:00+00:00"^^xsd:dateTime ;
	ikos:modified "2021-07-12T12:00:00+00:00"^^xsd:dateTime ;
	dct:modified "2021-07-12T12:00:00+00:00"^^xsd:dateTime  ;
	skos:exactMatch <https://www.wikidata.org/entity/Q12007954> ;
	skos:broader	medtop:20000134 .

medtop:20001199
	rdf:type skos:Concept ;
	skos:prefLabel	"suspended sentence"@en-GB ;
	skos:definition	"Legal arrangement where a judge delays the serving of a sentence by a person who has been found guilty of a crime in order to give them a probationary period"@en-GB ;
	skos:inScheme <http://cv.iptc.org/newscodes/mediatopic/>  ;
	ikos:created "2019-04-06T12:00:00+00:00"^^xsd:dateTime ;
	dct:created "2019-04-06T12:00:00+00:00"^^xsd:dateTime ;
	ikos:modified "2021-07-12T12:00:00+00:00"^^xsd:dateTime ;
	dct:modified "2021-07-12T12:00:00+00:00"^^xsd:dateTime  ;
	skos:exactMatch <https://www.wikidata.org/entity/Q4737759> ;
	skos:broader	medtop:20000134 .

medtop:20001200
	rdf:type skos:Concept ;
	skos:prefLabel	"dropped criminal investigation"@en-GB ;
	skos:definition	"When police and/or prosecutors end an investigation without a conclusion"@en-GB ;
	skos:changeNote	"Moved from 20001200 (prosecution) to 20000131 (criminal investigation)"@en-GB ;
	skos:inScheme <http://cv.iptc.org/newscodes/mediatopic/>  ;
	ikos:created "2019-04-06T12:00:00+00:00"^^xsd:dateTime ;
	dct:created "2019-04-06T12:00:00+00:00"^^xsd:dateTime ;
	ikos:modified "2021-07-12T12:00:00+00:00"^^xsd:dateTime ;
	dct:modified "2021-07-12T12:00:00+00:00"^^xsd:dateTime  ;
	skos:exactMatch <https://www.wikidata.org/entity/Q178146> ;
	skos:broader	medtop:20000131 .

medtop:20001201
	rdf:type skos:Concept ;
	skos:prefLabel	"wildlife traffic accident"@en-GB ;
	skos:definition	"Traffic accidents involving wild animals"@en-GB ;
	skos:inScheme <http://cv.iptc.org/newscodes/mediatopic/>  ;
	ikos:created "2019-04-06T12:00:00+00:00"^^xsd:dateTime ;
	dct:created "2019-04-06T12:00:00+00:00"^^xsd:dateTime ;
	ikos:modified "2021-07-12T12:00:00+00:00"^^xsd:dateTime ;
	dct:modified "2021-07-12T12:00:00+00:00"^^xsd:dateTime  ;
	skos:exactMatch <https://www.wikidata.org/entity/Q1324130> ;
	skos:broader	medtop:20000147 .

medtop:20001202
	rdf:type skos:Concept ;
	skos:prefLabel	"wildfire"@en-GB ;
	skos:definition	"An uncontrolled fire in an area of combustible vegetation"@en-GB ;
	skos:inScheme <http://cv.iptc.org/newscodes/mediatopic/>  ;
	ikos:created "2019-04-06T12:00:00+00:00"^^xsd:dateTime ;
	dct:created "2019-04-06T12:00:00+00:00"^^xsd:dateTime ;
	ikos:modified "2021-07-12T12:00:00+00:00"^^xsd:dateTime ;
	dct:modified "2021-07-12T12:00:00+00:00"^^xsd:dateTime  ;
	skos:exactMatch <https://www.wikidata.org/entity/Q169950> ;
	skos:broader	medtop:20000150 .

medtop:20001203
	rdf:type skos:Concept ;
	skos:prefLabel	"textile arts"@en-GB ;
	skos:definition	"Arts and crafts that use plant, animal, or synthetic fibres to construct practical or decorative object"@en-GB ;
	skos:inScheme <http://cv.iptc.org/newscodes/mediatopic/>  ;
	ikos:created "2019-04-06T12:00:00+00:00"^^xsd:dateTime ;
	dct:created "2019-04-06T12:00:00+00:00"^^xsd:dateTime ;
	ikos:modified "2021-07-12T12:00:00+00:00"^^xsd:dateTime ;
	dct:modified "2021-07-12T12:00:00+00:00"^^xsd:dateTime  ;
	skos:exactMatch <https://www.wikidata.org/entity/Q10988986> ;
	skos:broader	medtop:20000031 .

medtop:20001204
	rdf:type skos:Concept ;
	skos:prefLabel	"woodworking"@en-GB ;
	skos:definition	"The activity or skill of making items, such as furniture or cabinets, from wood"@en-GB ;
	skos:inScheme <http://cv.iptc.org/newscodes/mediatopic/>  ;
	ikos:created "2019-04-06T12:00:00+00:00"^^xsd:dateTime ;
	dct:created "2019-04-06T12:00:00+00:00"^^xsd:dateTime ;
	ikos:modified "2021-07-12T12:00:00+00:00"^^xsd:dateTime ;
	dct:modified "2021-07-12T12:00:00+00:00"^^xsd:dateTime  ;
	skos:exactMatch <https://www.wikidata.org/entity/Q816871> ;
	skos:broader	medtop:20000031 .

medtop:20001205
	rdf:type skos:Concept ;
	skos:prefLabel	"forging"@en-GB ;
	skos:definition	"The shaping of metal using localized compressive forces, such as heating and hammering"@en-GB ;
	skos:inScheme <http://cv.iptc.org/newscodes/mediatopic/>  ;
	ikos:created "2019-04-06T12:00:00+00:00"^^xsd:dateTime ;
	dct:created "2019-04-06T12:00:00+00:00"^^xsd:dateTime ;
	ikos:modified "2021-07-12T12:00:00+00:00"^^xsd:dateTime ;
	dct:modified "2021-07-12T12:00:00+00:00"^^xsd:dateTime  ;
	skos:exactMatch <https://www.wikidata.org/entity/Q193057> ;
	skos:broader	medtop:20000031 .

medtop:20001206
	rdf:type skos:Concept ;
	skos:prefLabel	"self-employment"@en-GB ;
	skos:definition	"A situation in which an individual works for themselves as a freelancer or business owner instead of working for an employer that pays a salary or a wage"@en-GB ;
	skos:inScheme <http://cv.iptc.org/newscodes/mediatopic/>  ;
	ikos:created "2019-04-06T12:00:00+00:00"^^xsd:dateTime ;
	dct:created "2019-04-06T12:00:00+00:00"^^xsd:dateTime ;
	ikos:modified "2021-07-12T12:00:00+00:00"^^xsd:dateTime ;
	dct:modified "2021-07-12T12:00:00+00:00"^^xsd:dateTime  ;
	skos:exactMatch <https://www.wikidata.org/entity/Q1005490> ;
	skos:broader	medtop:20000509 .

medtop:20001207
	rdf:type skos:Concept ;
	skos:prefLabel	"biofuel"@en-GB ;
	skos:definition	"Fuel that is derived from biomass, such as ethanol"@en-GB ;
	skos:inScheme <http://cv.iptc.org/newscodes/mediatopic/>  ;
	ikos:created "2019-04-06T12:00:00+00:00"^^xsd:dateTime ;
	dct:created "2019-04-06T12:00:00+00:00"^^xsd:dateTime ;
	ikos:modified "2023-03-31T12:00:00+00:00"^^xsd:dateTime ;
	dct:modified "2023-03-31T12:00:00+00:00"^^xsd:dateTime  ;
	skos:exactMatch <https://www.wikidata.org/entity/Q128991> ;
	skos:broader	medtop:20000256 .

medtop:20001208
	rdf:type skos:Concept ;
	skos:prefLabel	"geothermal power"@en-GB ;
	skos:definition	"Thermal energy that is generated and stored in the Earth"@en-GB ;
	skos:inScheme <http://cv.iptc.org/newscodes/mediatopic/>  ;
	ikos:created "2019-04-06T12:00:00+00:00"^^xsd:dateTime ;
	dct:created "2019-04-06T12:00:00+00:00"^^xsd:dateTime ;
	ikos:modified "2023-03-31T12:00:00+00:00"^^xsd:dateTime ;
	dct:modified "2023-03-31T12:00:00+00:00"^^xsd:dateTime  ;
	skos:exactMatch <https://www.wikidata.org/entity/Q3215493> ;
	skos:broader	medtop:20000257 .

medtop:20001209
	rdf:type skos:Concept ;
	skos:prefLabel	"solar power"@en-GB ;
	skos:definition	"Electricity generated and harvested from the sun's rays"@en-GB ;
	skos:inScheme <http://cv.iptc.org/newscodes/mediatopic/>  ;
	ikos:created "2019-04-06T12:00:00+00:00"^^xsd:dateTime ;
	dct:created "2019-04-06T12:00:00+00:00"^^xsd:dateTime ;
	ikos:modified "2023-03-31T12:00:00+00:00"^^xsd:dateTime ;
	dct:modified "2023-03-31T12:00:00+00:00"^^xsd:dateTime  ;
	skos:exactMatch <https://www.wikidata.org/entity/Q1483757> ;
	skos:broader	medtop:20000257 .

medtop:20001210
	rdf:type skos:Concept ;
	skos:prefLabel	"hydroelectric power"@en-GB ;
	skos:definition	"Electricity produced from hydropower when water flows through turbines"@en-GB ;
	skos:inScheme <http://cv.iptc.org/newscodes/mediatopic/>  ;
	ikos:created "2019-04-06T12:00:00+00:00"^^xsd:dateTime ;
	dct:created "2019-04-06T12:00:00+00:00"^^xsd:dateTime ;
	ikos:modified "2023-03-31T12:00:00+00:00"^^xsd:dateTime ;
	dct:modified "2023-03-31T12:00:00+00:00"^^xsd:dateTime  ;
	skos:exactMatch <https://www.wikidata.org/entity/Q80638> ;
	skos:broader	medtop:20000257 .

medtop:20001211
	rdf:type skos:Concept ;
	skos:prefLabel	"wind power"@en-GB ;
	skos:definition	"Electricity that is generated by kinetic energy of wind, usually produced by windmills or turbines"@en-GB ;
	skos:inScheme <http://cv.iptc.org/newscodes/mediatopic/>  ;
	ikos:created "2019-04-06T12:00:00+00:00"^^xsd:dateTime ;
	dct:created "2019-04-06T12:00:00+00:00"^^xsd:dateTime ;
	ikos:modified "2023-03-31T12:00:00+00:00"^^xsd:dateTime ;
	dct:modified "2023-03-31T12:00:00+00:00"^^xsd:dateTime  ;
	skos:exactMatch <https://www.wikidata.org/entity/Q43302> ;
	skos:broader	medtop:20000257 .

medtop:20001212
	rdf:type skos:Concept ;
	skos:prefLabel	"religious school"@en-GB ;
	skos:definition	"School that has a religious component in its operations or its curriculum"@en-GB ;
	skos:inScheme <http://cv.iptc.org/newscodes/mediatopic/>  ;
	ikos:created "2019-04-06T12:00:00+00:00"^^xsd:dateTime ;
	dct:created "2019-04-06T12:00:00+00:00"^^xsd:dateTime ;
	ikos:modified "2021-09-30T12:00:00+00:00"^^xsd:dateTime ;
	dct:modified "2021-09-30T12:00:00+00:00"^^xsd:dateTime  ;
	skos:exactMatch <https://www.wikidata.org/entity/Q1971849> ;
	skos:broader	medtop:20000400 .

medtop:20001213
	rdf:type skos:Concept ;
	skos:prefLabel	"state school"@en-GB ;
	skos:definition	"Schools maintained by public funds, usually government-imposed taxes"@en-GB ;
	skos:inScheme <http://cv.iptc.org/newscodes/mediatopic/>  ;
	ikos:created "2019-04-06T12:00:00+00:00"^^xsd:dateTime ;
	dct:created "2019-04-06T12:00:00+00:00"^^xsd:dateTime ;
	ikos:modified "2021-09-30T12:00:00+00:00"^^xsd:dateTime ;
	dct:modified "2021-09-30T12:00:00+00:00"^^xsd:dateTime  ;
	skos:exactMatch <https://www.wikidata.org/entity/Q1080794> ;
	skos:broader	medtop:20000400 .

medtop:20001214
	rdf:type skos:Concept ;
	skos:prefLabel	"private school"@en-GB ;
	skos:definition	"Schools maintained by private funds and organisations"@en-GB ;
	skos:inScheme <http://cv.iptc.org/newscodes/mediatopic/>  ;
	ikos:created "2019-04-06T12:00:00+00:00"^^xsd:dateTime ;
	dct:created "2019-04-06T12:00:00+00:00"^^xsd:dateTime ;
	ikos:modified "2021-09-30T12:00:00+00:00"^^xsd:dateTime ;
	dct:modified "2021-09-30T12:00:00+00:00"^^xsd:dateTime  ;
	skos:exactMatch <https://www.wikidata.org/entity/Q423208> ;
	skos:broader	medtop:20000400 .

medtop:20001215
	rdf:type skos:Concept ;
	skos:prefLabel	"independent school"@en-GB ;
	skos:definition	"Schools funded by money from taxes via government, but run by companies, organisations or cooperatives"@en-GB ;
	skos:inScheme <http://cv.iptc.org/newscodes/mediatopic/>  ;
	ikos:created "2019-04-06T12:00:00+00:00"^^xsd:dateTime ;
	dct:created "2019-04-06T12:00:00+00:00"^^xsd:dateTime ;
	ikos:modified "2021-09-30T12:00:00+00:00"^^xsd:dateTime ;
	dct:modified "2021-09-30T12:00:00+00:00"^^xsd:dateTime  ;
	skos:exactMatch <https://www.wikidata.org/entity/Q3238833> ;
	skos:broader	medtop:20000400 .

medtop:20001216
	rdf:type skos:Concept ;
	skos:prefLabel	"vocational education"@en-GB ;
	skos:definition	"Education that provides students with practical experience and training in a particular occupational field. It is sometimes referred to as career education or technical education"@en-GB ;
	skos:inScheme <http://cv.iptc.org/newscodes/mediatopic/>  ;
	ikos:created "2019-04-06T12:00:00+00:00"^^xsd:dateTime ;
	dct:created "2019-04-06T12:00:00+00:00"^^xsd:dateTime ;
	ikos:modified "2021-09-30T12:00:00+00:00"^^xsd:dateTime ;
	dct:modified "2021-09-30T12:00:00+00:00"^^xsd:dateTime  ;
	skos:exactMatch <https://www.wikidata.org/entity/Q6869278> ;
	skos:broader	medtop:05000000 .

medtop:20001217
	rdf:type skos:Concept ;
	skos:prefLabel	"educational grading"@en-GB ;
	skos:definition	"The evaluation of a student's achievement on a test, assignment or course and the policies and methods around assigning those grades"@en-GB ;
	skos:inScheme <http://cv.iptc.org/newscodes/mediatopic/>  ;
	ikos:created "2019-04-06T12:00:00+00:00"^^xsd:dateTime ;
	dct:created "2019-04-06T12:00:00+00:00"^^xsd:dateTime ;
	ikos:modified "2021-09-30T12:00:00+00:00"^^xsd:dateTime ;
	dct:modified "2021-09-30T12:00:00+00:00"^^xsd:dateTime  ;
	skos:exactMatch <https://www.wikidata.org/entity/Q18185> ;
	skos:broader	medtop:05000000 .

medtop:20001218
	rdf:type skos:Concept ;
	skos:prefLabel	"pandemic"@en-GB ;
	skos:definition	"An epidemic of infectious disease that has spread across a large region or even worldwide"@en-GB ;
	skos:changeNote	"Retired. Use medtop:20000449 epidemic and pandemic instead."@en-GB ;
	skos:inScheme <http://cv.iptc.org/newscodes/mediatopic/>  ;
	ikos:created "2019-04-06T12:00:00+00:00"^^xsd:dateTime ;
	dct:created "2019-04-06T12:00:00+00:00"^^xsd:dateTime ;
	ikos:modified "2022-06-14T12:00:00+00:00"^^xsd:dateTime ;
	dct:modified "2022-06-14T12:00:00+00:00"^^xsd:dateTime  ; 
	ikos:retired "2022-06-14T12:00:00+00:00"^^xsd:dateTime ;
	skos:exactMatch <https://www.wikidata.org/entity/Q12184> ;
	skos:broader	medtop:20000449 .

medtop:20001219
	rdf:type skos:Concept ;
	skos:prefLabel	"drug rehabilitation"@en-GB ;
	skos:definition	"Medical or psychotherapeutic treatment for dependency on substances such as alcohol, prescription and controlled drugs"@en-GB ;
	skos:inScheme <http://cv.iptc.org/newscodes/mediatopic/>  ;
	ikos:created "2019-04-06T12:00:00+00:00"^^xsd:dateTime ;
	dct:created "2019-04-06T12:00:00+00:00"^^xsd:dateTime ;
	ikos:modified "2022-06-14T12:00:00+00:00"^^xsd:dateTime ;
	dct:modified "2022-06-14T12:00:00+00:00"^^xsd:dateTime  ;
	skos:exactMatch <https://www.wikidata.org/entity/Q1260022> ;
	skos:broader	medtop:20000464 .

medtop:20001220
	rdf:type skos:Concept ;
	skos:prefLabel	"general practice"@en-GB ;
	skos:definition	"The treatment of a wide range of acute and long-term medical conditions and symptoms"@en-GB ;
	skos:changeNote	"Retired. Use general health terms instead."@en-GB ;
	skos:inScheme <http://cv.iptc.org/newscodes/mediatopic/>  ;
	ikos:created "2019-04-06T12:00:00+00:00"^^xsd:dateTime ;
	dct:created "2019-04-06T12:00:00+00:00"^^xsd:dateTime ;
	ikos:modified "2022-06-14T12:00:00+00:00"^^xsd:dateTime ;
	dct:modified "2022-06-14T12:00:00+00:00"^^xsd:dateTime  ; 
	ikos:retired "2022-06-14T12:00:00+00:00"^^xsd:dateTime ;
	skos:exactMatch <https://www.wikidata.org/entity/Q33127638> ;
	skos:broader	medtop:20000487 .

medtop:20001221
	rdf:type skos:Concept ;
	skos:prefLabel	"emergency care"@en-GB ;
	skos:definition	"Immediate care of patients with critical medical emergencies, either inside or outside of a hospital"@en-GB ;
	skos:inScheme <http://cv.iptc.org/newscodes/mediatopic/>  ;
	ikos:created "2019-04-06T12:00:00+00:00"^^xsd:dateTime ;
	dct:created "2019-04-06T12:00:00+00:00"^^xsd:dateTime ;
	ikos:modified "2022-06-14T12:00:00+00:00"^^xsd:dateTime ;
	dct:modified "2022-06-14T12:00:00+00:00"^^xsd:dateTime  ;
	skos:exactMatch <https://www.wikidata.org/entity/Q67323460> ;
	skos:broader	medtop:20000464 .

medtop:20001222
	rdf:type skos:Concept ;
	skos:prefLabel	"orthopaedics"@en-GB ;
	skos:definition	"A medical specialisation that focuses on conditions involving the musculoskeletal system"@en-GB ;
	skos:changeNote	"Retired. Use medtop:20000456 injury instead."@en-GB ;
	skos:inScheme <http://cv.iptc.org/newscodes/mediatopic/>  ;
	ikos:created "2019-04-06T12:00:00+00:00"^^xsd:dateTime ;
	dct:created "2019-04-06T12:00:00+00:00"^^xsd:dateTime ;
	ikos:modified "2022-06-14T12:00:00+00:00"^^xsd:dateTime ;
	dct:modified "2022-06-14T12:00:00+00:00"^^xsd:dateTime  ; 
	ikos:retired "2022-06-14T12:00:00+00:00"^^xsd:dateTime ;
	skos:exactMatch <https://www.wikidata.org/entity/Q216685> ;
	skos:broader	medtop:20000487 .

medtop:20001223
	rdf:type skos:Concept ;
	skos:prefLabel	"oncology"@en-GB ;
	skos:definition	"A medical specialisation that focuses on the prevention, diagnosis, and treatment of cancer"@en-GB ;
	skos:changeNote	"Retired. Use medtop:20000447 cancer instead."@en-GB ;
	skos:inScheme <http://cv.iptc.org/newscodes/mediatopic/>  ;
	ikos:created "2019-04-06T12:00:00+00:00"^^xsd:dateTime ;
	dct:created "2019-04-06T12:00:00+00:00"^^xsd:dateTime ;
	ikos:modified "2022-06-14T12:00:00+00:00"^^xsd:dateTime ;
	dct:modified "2022-06-14T12:00:00+00:00"^^xsd:dateTime  ; 
	ikos:retired "2022-06-14T12:00:00+00:00"^^xsd:dateTime ;
	skos:exactMatch <https://www.wikidata.org/entity/Q162555> ;
	skos:broader	medtop:20000487 .

medtop:20001224
	rdf:type skos:Concept ;
	skos:prefLabel	"radiology"@en-GB ;
	skos:definition	"A medical specialisation that focuses on the use of medical imaging (such as x-rays) and radiation to diagnose and sometimes also treat diseases within the body"@en-GB ;
	skos:changeNote	"Retired."@en-GB ;
	skos:inScheme <http://cv.iptc.org/newscodes/mediatopic/>  ;
	ikos:created "2019-04-06T12:00:00+00:00"^^xsd:dateTime ;
	dct:created "2019-04-06T12:00:00+00:00"^^xsd:dateTime ;
	ikos:modified "2022-06-14T12:00:00+00:00"^^xsd:dateTime ;
	dct:modified "2022-06-14T12:00:00+00:00"^^xsd:dateTime  ; 
	ikos:retired "2022-06-14T12:00:00+00:00"^^xsd:dateTime ;
	skos:exactMatch <https://www.wikidata.org/entity/Q77604> ;
	skos:broader	medtop:20000487 .

medtop:20001225
	rdf:type skos:Concept ;
	skos:prefLabel	"eye care"@en-GB ;
	skos:definition	"The medical profession and field of study devoted to diagnosing, preventing and treating eye conditions"@en-GB ;
	skos:inScheme <http://cv.iptc.org/newscodes/mediatopic/>  ;
	ikos:created "2019-04-06T12:00:00+00:00"^^xsd:dateTime ;
	dct:created "2019-04-06T12:00:00+00:00"^^xsd:dateTime ;
	ikos:modified "2022-06-14T12:00:00+00:00"^^xsd:dateTime ;
	dct:modified "2022-06-14T12:00:00+00:00"^^xsd:dateTime  ;
	skos:exactMatch <https://www.wikidata.org/entity/Q161437> ;
	skos:broader	medtop:20000487 .

medtop:20001226
	rdf:type skos:Concept ;
	skos:prefLabel	"surgical medicine"@en-GB ;
	skos:definition	"A medical specialisation that focuses on the treatment of injuries or disorders of the body by incision or manipulation, especially with instruments"@en-GB ;
	skos:changeNote	"Retired. Use medtop:20001228 surgery instead."@en-GB ;
	skos:inScheme <http://cv.iptc.org/newscodes/mediatopic/>  ;
	ikos:created "2019-04-06T12:00:00+00:00"^^xsd:dateTime ;
	dct:created "2019-04-06T12:00:00+00:00"^^xsd:dateTime ;
	ikos:modified "2022-06-14T12:00:00+00:00"^^xsd:dateTime ;
	dct:modified "2022-06-14T12:00:00+00:00"^^xsd:dateTime  ; 
	ikos:retired "2022-06-14T12:00:00+00:00"^^xsd:dateTime ;
	skos:exactMatch <https://www.wikidata.org/entity/Q40821> ;
	skos:broader	medtop:20000487 .

medtop:20001227
	rdf:type skos:Concept ;
	skos:prefLabel	"psychiatry"@en-GB ;
	skos:definition	"A medical specialisation that focuses on the diagnosis, prevention and treatment of mental disorders"@en-GB ;
	skos:changeNote	"Retired. Use medtop:20000458 mental health instead."@en-GB ;
	skos:inScheme <http://cv.iptc.org/newscodes/mediatopic/>  ;
	ikos:created "2019-04-06T12:00:00+00:00"^^xsd:dateTime ;
	dct:created "2019-04-06T12:00:00+00:00"^^xsd:dateTime ;
	ikos:modified "2022-06-14T12:00:00+00:00"^^xsd:dateTime ;
	dct:modified "2022-06-14T12:00:00+00:00"^^xsd:dateTime  ; 
	ikos:retired "2022-06-14T12:00:00+00:00"^^xsd:dateTime ;
	skos:exactMatch <https://www.wikidata.org/entity/Q7867> ;
	skos:broader	medtop:20000487 .

medtop:20001228
	rdf:type skos:Concept ;
	skos:prefLabel	"surgery"@en-GB ;
	skos:definition	"The use of incisions made by medical instruments to investigate or treat a medical condition or injury"@en-GB ;
	skos:inScheme <http://cv.iptc.org/newscodes/mediatopic/>  ;
	ikos:created "2019-04-06T12:00:00+00:00"^^xsd:dateTime ;
	dct:created "2019-04-06T12:00:00+00:00"^^xsd:dateTime ;
	ikos:modified "2021-07-12T12:00:00+00:00"^^xsd:dateTime ;
	dct:modified "2021-07-12T12:00:00+00:00"^^xsd:dateTime  ;
	skos:exactMatch <https://www.wikidata.org/entity/Q40821> ;
	skos:broader	medtop:20000464 .

medtop:20001229
	rdf:type skos:Concept ;
	skos:prefLabel	"healthcare clinic"@en-GB ;
	skos:definition	"Local medical facility or doctor's office associated with a general medicine practice, staffed by one or many doctors, focusing on outpatient treatment or giving recommendations to visit a specialist or hospital"@en-GB ;
	skos:inScheme <http://cv.iptc.org/newscodes/mediatopic/>  ;
	ikos:created "2019-04-06T12:00:00+00:00"^^xsd:dateTime ;
	dct:created "2019-04-06T12:00:00+00:00"^^xsd:dateTime ;
	ikos:modified "2021-07-12T12:00:00+00:00"^^xsd:dateTime ;
	dct:modified "2021-07-12T12:00:00+00:00"^^xsd:dateTime  ;
	skos:exactMatch <https://www.wikidata.org/entity/Q1774898> ;
	skos:broader	medtop:20000461 .

medtop:20001230
	rdf:type skos:Concept ;
	skos:prefLabel	"environmental, social and governance policy (ESG)"@en-GB ;
	skos:definition	"A company's business practices reflecting responsible social, ethical and environmental policies, sometimes known as corporate social responsibility"@en-GB ;
	skos:inScheme <http://cv.iptc.org/newscodes/mediatopic/>  ;
	ikos:created "2019-04-06T12:00:00+00:00"^^xsd:dateTime ;
	dct:created "2019-04-06T12:00:00+00:00"^^xsd:dateTime ;
	ikos:modified "2023-03-31T12:00:00+00:00"^^xsd:dateTime ;
	dct:modified "2023-03-31T12:00:00+00:00"^^xsd:dateTime  ;
	skos:exactMatch <https://www.wikidata.org/entity/Q218600> ;
	skos:broader	medtop:20000199 .

medtop:20001231
	rdf:type skos:Concept ;
	skos:prefLabel	"mixed martial arts"@en-GB ;
	skos:definition	"A full-contact combat sport using techniques from various combat sports and martial arts"@en-GB ;
	skos:inScheme <http://cv.iptc.org/newscodes/mediatopic/>  ;
	ikos:created "2019-04-06T12:00:00+00:00"^^xsd:dateTime ;
	dct:created "2019-04-06T12:00:00+00:00"^^xsd:dateTime ;
	ikos:modified "2021-07-12T12:00:00+00:00"^^xsd:dateTime ;
	dct:modified "2021-07-12T12:00:00+00:00"^^xsd:dateTime  ;
	skos:exactMatch <https://www.wikidata.org/entity/Q114466> ;
	skos:broader	medtop:20001157 .

medtop:20001232
	rdf:type skos:Concept ;
	skos:prefLabel	"elderly care"@en-GB ;
	skos:definition	"The long-term care of the elderly provided by residential institutions or by paid daily help in the home"@en-GB ;
	skos:inScheme <http://cv.iptc.org/newscodes/mediatopic/>  ;
	ikos:created "2019-06-26T12:00:00+00:00"^^xsd:dateTime ;
	dct:created "2019-06-26T12:00:00+00:00"^^xsd:dateTime ;
	ikos:modified "2021-07-12T12:00:00+00:00"^^xsd:dateTime ;
	dct:modified "2021-07-12T12:00:00+00:00"^^xsd:dateTime  ;
	skos:exactMatch <https://www.wikidata.org/entity/Q437458> ;
	skos:broader	medtop:20000817 .

medtop:20001233
	rdf:type skos:Concept ;
	skos:prefLabel	"name ceremony"@en-GB ;
	skos:definition	"Event at which an infant, youth, or adult is given a name"@en-GB ;
	skos:inScheme <http://cv.iptc.org/newscodes/mediatopic/>  ;
	ikos:created "2019-06-26T12:00:00+00:00"^^xsd:dateTime ;
	dct:created "2019-06-26T12:00:00+00:00"^^xsd:dateTime ;
	ikos:modified "2021-07-12T12:00:00+00:00"^^xsd:dateTime ;
	dct:modified "2021-07-12T12:00:00+00:00"^^xsd:dateTime  ;
	skos:exactMatch <https://www.wikidata.org/entity/Q3534263> ;
	skos:broader	medtop:20000501 .

medtop:20001234
	rdf:type skos:Concept ;
	skos:prefLabel	"graduation"@en-GB ;
	skos:definition	"A ceremony, also known as commencement, at which a person receives a diploma or academic degree"@en-GB ;
	skos:inScheme <http://cv.iptc.org/newscodes/mediatopic/>  ;
	ikos:created "2019-06-26T12:00:00+00:00"^^xsd:dateTime ;
	dct:created "2019-06-26T12:00:00+00:00"^^xsd:dateTime ;
	ikos:modified "2021-07-12T12:00:00+00:00"^^xsd:dateTime ;
	dct:modified "2021-07-12T12:00:00+00:00"^^xsd:dateTime  ;
	skos:exactMatch <https://www.wikidata.org/entity/Q1054021> ;
	skos:broader	medtop:20000501 .

medtop:20001235
	rdf:type skos:Concept ;
	skos:prefLabel	"funeral and memorial service"@en-GB ;
	skos:definition	"A ceremony to memorialise a deceased person"@en-GB ;
	skos:inScheme <http://cv.iptc.org/newscodes/mediatopic/>  ;
	ikos:created "2019-06-26T12:00:00+00:00"^^xsd:dateTime ;
	dct:created "2019-06-26T12:00:00+00:00"^^xsd:dateTime ;
	ikos:modified "2021-07-12T12:00:00+00:00"^^xsd:dateTime ;
	dct:modified "2021-07-12T12:00:00+00:00"^^xsd:dateTime  ;
	skos:exactMatch <https://www.wikidata.org/entity/Q201676> ;
	skos:broader	medtop:20000501 .

medtop:20001236
	rdf:type skos:Concept ;
	skos:prefLabel	"wedding"@en-GB ;
	skos:definition	"Marriage ceremony and the events and parties surrounding it, such as wedding receptions, engagement parties, bridal showers and hen or stag parties"@en-GB ;
	skos:inScheme <http://cv.iptc.org/newscodes/mediatopic/>  ;
	ikos:created "2019-06-26T12:00:00+00:00"^^xsd:dateTime ;
	dct:created "2019-06-26T12:00:00+00:00"^^xsd:dateTime ;
	ikos:modified "2021-07-12T12:00:00+00:00"^^xsd:dateTime ;
	dct:modified "2021-07-12T12:00:00+00:00"^^xsd:dateTime  ;
	skos:exactMatch <https://www.wikidata.org/entity/Q49836> ;
	skos:broader	medtop:20000501 .

medtop:20001237
	rdf:type skos:Concept ;
	skos:prefLabel	"anniversary"@en-GB ;
	skos:definition	"The celebration or commemoration of a significant amount of years since an event or a notable person's birth or death"@en-GB ;
	skos:inScheme <http://cv.iptc.org/newscodes/mediatopic/>  ;
	ikos:created "2019-06-26T12:00:00+00:00"^^xsd:dateTime ;
	dct:created "2019-06-26T12:00:00+00:00"^^xsd:dateTime ;
	ikos:modified "2021-07-12T12:00:00+00:00"^^xsd:dateTime ;
	dct:modified "2021-07-12T12:00:00+00:00"^^xsd:dateTime  ;
	skos:exactMatch <https://www.wikidata.org/entity/Q1062856> ;
	skos:broader	medtop:08000000 .

medtop:20001238
	rdf:type skos:Concept ;
	skos:prefLabel	"birthday"@en-GB ;
	skos:definition	"A celebration on the anniversary of a person's birth."@en-GB ;
	skos:inScheme <http://cv.iptc.org/newscodes/mediatopic/>  ;
	ikos:created "2019-06-26T12:00:00+00:00"^^xsd:dateTime ;
	dct:created "2019-06-26T12:00:00+00:00"^^xsd:dateTime ;
	ikos:modified "2021-07-12T12:00:00+00:00"^^xsd:dateTime ;
	dct:modified "2021-07-12T12:00:00+00:00"^^xsd:dateTime  ;
	skos:exactMatch <https://www.wikidata.org/entity/Q47223> ;
	skos:broader	medtop:08000000 .

medtop:20001239
	rdf:type skos:Concept ;
	skos:prefLabel	"exercise and fitness"@en-GB ;
	skos:definition	"Physical activity with the purpose to maintain and improve health and wellness, gain stamina or for enjoyment"@en-GB ;
	skos:inScheme <http://cv.iptc.org/newscodes/mediatopic/>  ;
	ikos:created "2019-06-26T12:00:00+00:00"^^xsd:dateTime ;
	dct:created "2019-06-26T12:00:00+00:00"^^xsd:dateTime ;
	ikos:modified "2021-12-17T12:00:00+00:00"^^xsd:dateTime ;
	dct:modified "2021-12-17T12:00:00+00:00"^^xsd:dateTime  ;
	skos:exactMatch <https://www.wikidata.org/entity/Q219067> ;
	skos:broader	medtop:20001339 .

medtop:20001240
	rdf:type skos:Concept ;
	skos:prefLabel	"bodybuilding"@en-GB ;
	skos:definition	"Competitions where participants perform specific poses to display their muscles that have been strengthened and enlarged through strenuous exercise. Competitors are judged based on criteria such as symmetry, muscularity and conditioning."@en-GB ;
	skos:inScheme <http://cv.iptc.org/newscodes/mediatopic/>  ;
	ikos:created "2019-06-26T12:00:00+00:00"^^xsd:dateTime ;
	dct:created "2019-06-26T12:00:00+00:00"^^xsd:dateTime ;
	ikos:modified "2021-07-12T12:00:00+00:00"^^xsd:dateTime ;
	dct:modified "2021-07-12T12:00:00+00:00"^^xsd:dateTime  ;
	skos:exactMatch <https://www.wikidata.org/entity/Q124100> ;
	skos:broader	medtop:20000822 .

medtop:20001241
	rdf:type skos:Concept ;
	skos:prefLabel	"horseback riding"@en-GB ;
	skos:definition	"The riding of horses for leisure or light exercise."@en-GB ;
	skos:inScheme <http://cv.iptc.org/newscodes/mediatopic/>  ;
	ikos:created "2019-06-26T12:00:00+00:00"^^xsd:dateTime ;
	dct:created "2019-06-26T12:00:00+00:00"^^xsd:dateTime ;
	ikos:modified "2021-07-12T12:00:00+00:00"^^xsd:dateTime ;
	dct:modified "2021-07-12T12:00:00+00:00"^^xsd:dateTime  ;
	skos:exactMatch <https://www.wikidata.org/entity/Q179226> ;
	skos:broader	medtop:20000560 .

medtop:20001242
	rdf:type skos:Concept ;
	skos:prefLabel	"steeplechase (athletics)"@en-GB ;
	skos:definition	"Obstacle race in athletics including barriers and water jumps"@en-GB ;
	skos:inScheme <http://cv.iptc.org/newscodes/mediatopic/>  ;
	ikos:created "2019-07-23T12:00:00+00:00"^^xsd:dateTime ;
	dct:created "2019-07-23T12:00:00+00:00"^^xsd:dateTime ;
	ikos:modified "2021-07-12T12:00:00+00:00"^^xsd:dateTime ;
	dct:modified "2021-07-12T12:00:00+00:00"^^xsd:dateTime  ;
	skos:exactMatch <https://www.wikidata.org/entity/Q223836> ;
	skos:broader	medtop:20000827 .

medtop:20001243
	rdf:type skos:Concept ;
	skos:prefLabel	"oil and gas"@en-GB ;
	skos:definition	"The exploration, extraction, refining, transporting and marketing of petroleum products and natural gas"@en-GB ;
	skos:inScheme <http://cv.iptc.org/newscodes/mediatopic/>  ;
	ikos:created "2019-07-25T12:00:00+00:00"^^xsd:dateTime ;
	dct:created "2019-07-25T12:00:00+00:00"^^xsd:dateTime ;
	ikos:modified "2023-03-31T12:00:00+00:00"^^xsd:dateTime ;
	dct:modified "2023-03-31T12:00:00+00:00"^^xsd:dateTime  ;
	skos:exactMatch subj:04005004 ;
	skos:exactMatch <https://www.wikidata.org/entity/Q862571> ;
	skos:broader	medtop:20000256 ;
	skos:narrower	medtop:20000259 ;
	skos:narrower	medtop:20000262 ;
	skos:narrower	medtop:20000263 ;
	skos:narrower	medtop:20000268 .

medtop:20001244
	rdf:type skos:Concept ;
	skos:prefLabel	"utilities"@en-GB ;
	skos:definition	"The providing of basic services to the public, such as supplying water, waste removal, heating and cooling"@en-GB ;
	skos:inScheme <http://cv.iptc.org/newscodes/mediatopic/>  ;
	ikos:created "2019-07-25T12:00:00+00:00"^^xsd:dateTime ;
	dct:created "2019-07-25T12:00:00+00:00"^^xsd:dateTime ;
	ikos:modified "2023-03-31T12:00:00+00:00"^^xsd:dateTime ;
	dct:modified "2023-03-31T12:00:00+00:00"^^xsd:dateTime  ;
	skos:exactMatch <https://www.wikidata.org/entity/Q58891990> ;
	skos:broader	medtop:20000209 ;
	skos:narrower	medtop:20000260 ;
	skos:narrower	medtop:20000269 ;
	skos:narrower	medtop:20000270 ;
	skos:narrower	medtop:20001291 .

medtop:20001245
	rdf:type skos:Concept ;
	skos:prefLabel	"infrastructure projects"@en-GB ;
	skos:definition	"The construction of the fundamental facilities and systems serving a country, city, or other area, including roads, bridges, dams, tunnels, telecommunications and electrical grids"@en-GB ;
	skos:inScheme <http://cv.iptc.org/newscodes/mediatopic/>  ;
	ikos:created "2019-07-25T12:00:00+00:00"^^xsd:dateTime ;
	dct:created "2019-07-25T12:00:00+00:00"^^xsd:dateTime ;
	ikos:modified "2021-07-12T12:00:00+00:00"^^xsd:dateTime ;
	dct:modified "2021-07-12T12:00:00+00:00"^^xsd:dateTime  ;
	skos:broader	medtop:20000235 .

medtop:20001246
	rdf:type skos:Concept ;
	skos:prefLabel	"commercial building"@en-GB ;
	skos:definition	"The construction of buildings for commerce and business, including office buildings, retail shops, restaurants, hotels and stadiums"@en-GB ;
	skos:changeNote	"Retired. Use medtop:20001367 commercial real estate instead."@en-GB ;
	skos:inScheme <http://cv.iptc.org/newscodes/mediatopic/>  ;
	ikos:created "2019-07-25T12:00:00+00:00"^^xsd:dateTime ;
	dct:created "2019-07-25T12:00:00+00:00"^^xsd:dateTime ;
	ikos:modified "2023-03-31T12:00:00+00:00"^^xsd:dateTime ;
	dct:modified "2023-03-31T12:00:00+00:00"^^xsd:dateTime  ; 
	ikos:retired "2023-03-31T12:00:00+00:00"^^xsd:dateTime ;
	skos:broader	medtop:20000235 .

medtop:20001247
	rdf:type skos:Concept ;
	skos:prefLabel	"collecting"@en-GB ;
	skos:definition	"The hobby of seeking, locating, acquiring, organising, cataloguing, displaying, storing or maintaining items that are of interest to an individual collector"@en-GB ;
	skos:inScheme <http://cv.iptc.org/newscodes/mediatopic/>  ;
	ikos:created "2019-07-30T12:00:00+00:00"^^xsd:dateTime ;
	dct:created "2019-07-30T12:00:00+00:00"^^xsd:dateTime ;
	ikos:modified "2021-07-12T12:00:00+00:00"^^xsd:dateTime ;
	dct:modified "2021-07-12T12:00:00+00:00"^^xsd:dateTime  ;
	skos:exactMatch <https://www.wikidata.org/entity/Q208165> ;
	skos:broader	medtop:20000550 .

medtop:20001248
	rdf:type skos:Concept ;
	skos:prefLabel	"cosmetics"@en-GB ;
	skos:definition	"Products applied to the body to enhance appearance, such as lipstick, eyeliner, foundation and nail polish, and the trends surrounding the application of these products"@en-GB ;
	skos:inScheme <http://cv.iptc.org/newscodes/mediatopic/>  ;
	ikos:created "2019-07-30T12:00:00+00:00"^^xsd:dateTime ;
	dct:created "2019-07-30T12:00:00+00:00"^^xsd:dateTime ;
	ikos:modified "2021-07-12T12:00:00+00:00"^^xsd:dateTime ;
	dct:modified "2021-07-12T12:00:00+00:00"^^xsd:dateTime  ;
	skos:exactMatch <https://www.wikidata.org/entity/Q131207> ;
	skos:broader	medtop:20000011 .

medtop:20001249
	rdf:type skos:Concept ;
	skos:prefLabel	"hairstyles"@en-GB ;
	skos:definition	"Trends surrounding the cutting and styling of hair"@en-GB ;
	skos:inScheme <http://cv.iptc.org/newscodes/mediatopic/>  ;
	ikos:created "2019-07-30T12:00:00+00:00"^^xsd:dateTime ;
	dct:created "2019-07-30T12:00:00+00:00"^^xsd:dateTime ;
	ikos:modified "2021-07-12T12:00:00+00:00"^^xsd:dateTime ;
	dct:modified "2021-07-12T12:00:00+00:00"^^xsd:dateTime  ;
	skos:exactMatch <https://www.wikidata.org/entity/Q327496> ;
	skos:broader	medtop:20000011 .

medtop:20001250
	rdf:type skos:Concept ;
	skos:prefLabel	"body modification"@en-GB ;
	skos:definition	"Actions taken to permanently or semi-permanently change body appearance, such as piercing and tattooing"@en-GB ;
	skos:inScheme <http://cv.iptc.org/newscodes/mediatopic/>  ;
	ikos:created "2019-07-30T12:00:00+00:00"^^xsd:dateTime ;
	dct:created "2019-07-30T12:00:00+00:00"^^xsd:dateTime ;
	ikos:modified "2021-07-12T12:00:00+00:00"^^xsd:dateTime ;
	dct:modified "2021-07-12T12:00:00+00:00"^^xsd:dateTime  ;
	skos:exactMatch <https://www.wikidata.org/entity/Q890057> ;
	skos:broader	medtop:20000572 ;
	skos:narrower	medtop:20001251 ;
	skos:narrower	medtop:20001252 .

medtop:20001251
	rdf:type skos:Concept ;
	skos:prefLabel	"tattooing"@en-GB ;
	skos:definition	"A form of body modification where a design is made by inserting ink, dyes and pigments into the dermis layer of the skin to permanently change the pigment"@en-GB ;
	skos:inScheme <http://cv.iptc.org/newscodes/mediatopic/>  ;
	ikos:created "2019-07-30T12:00:00+00:00"^^xsd:dateTime ;
	dct:created "2019-07-30T12:00:00+00:00"^^xsd:dateTime ;
	ikos:modified "2021-07-12T12:00:00+00:00"^^xsd:dateTime ;
	dct:modified "2021-07-12T12:00:00+00:00"^^xsd:dateTime  ;
	skos:exactMatch <https://www.wikidata.org/entity/Q43006> ;
	skos:broader	medtop:20001250 .

medtop:20001252
	rdf:type skos:Concept ;
	skos:prefLabel	"piercing"@en-GB ;
	skos:definition	"A form of body modification involving the puncturing or cutting of a part of the human body, creating an opening in which jewellery may be worn or where an implant could be inserted"@en-GB ;
	skos:inScheme <http://cv.iptc.org/newscodes/mediatopic/>  ;
	ikos:created "2019-07-30T12:00:00+00:00"^^xsd:dateTime ;
	dct:created "2019-07-30T12:00:00+00:00"^^xsd:dateTime ;
	ikos:modified "2021-07-12T12:00:00+00:00"^^xsd:dateTime ;
	dct:modified "2021-07-12T12:00:00+00:00"^^xsd:dateTime  ;
	skos:exactMatch <https://www.wikidata.org/entity/Q157943> ;
	skos:broader	medtop:20001250 .

medtop:20001253
	rdf:type skos:Concept ;
	skos:prefLabel	"cooking and baking"@en-GB ;
	skos:definition	"Interest in preparing meals or baked goods"@en-GB ;
	skos:inScheme <http://cv.iptc.org/newscodes/mediatopic/>  ;
	ikos:created "2019-07-30T12:00:00+00:00"^^xsd:dateTime ;
	dct:created "2019-07-30T12:00:00+00:00"^^xsd:dateTime ;
	ikos:modified "2021-07-12T12:00:00+00:00"^^xsd:dateTime ;
	dct:modified "2021-07-12T12:00:00+00:00"^^xsd:dateTime  ;
	skos:broader	medtop:20000568 .

medtop:20001254
	rdf:type skos:Concept ;
	skos:prefLabel	"beer, wine and spirits"@en-GB ;
	skos:definition	"Interest in the consumption, production and collection of alcoholic beverages"@en-GB ;
	skos:inScheme <http://cv.iptc.org/newscodes/mediatopic/>  ;
	ikos:created "2019-07-30T12:00:00+00:00"^^xsd:dateTime ;
	dct:created "2019-07-30T12:00:00+00:00"^^xsd:dateTime ;
	ikos:modified "2021-07-12T12:00:00+00:00"^^xsd:dateTime ;
	dct:modified "2021-07-12T12:00:00+00:00"^^xsd:dateTime  ;
	skos:broader	medtop:20000568 .

medtop:20001255
	rdf:type skos:Concept ;
	skos:prefLabel	"home renovation"@en-GB ;
	skos:definition	"Interest in renovating one's property"@en-GB ;
	skos:inScheme <http://cv.iptc.org/newscodes/mediatopic/>  ;
	ikos:created "2019-07-30T12:00:00+00:00"^^xsd:dateTime ;
	dct:created "2019-07-30T12:00:00+00:00"^^xsd:dateTime ;
	ikos:modified "2021-07-12T12:00:00+00:00"^^xsd:dateTime ;
	dct:modified "2021-07-12T12:00:00+00:00"^^xsd:dateTime  ;
	skos:exactMatch <https://www.wikidata.org/entity/Q2789106> ;
	skos:broader	medtop:20000570 .

medtop:20001256
	rdf:type skos:Concept ;
	skos:prefLabel	"interior decoration"@en-GB ;
	skos:definition	"Interest in decorating one's home"@en-GB ;
	skos:inScheme <http://cv.iptc.org/newscodes/mediatopic/>  ;
	ikos:created "2019-07-30T12:00:00+00:00"^^xsd:dateTime ;
	dct:created "2019-07-30T12:00:00+00:00"^^xsd:dateTime ;
	ikos:modified "2021-07-12T12:00:00+00:00"^^xsd:dateTime ;
	dct:modified "2021-07-12T12:00:00+00:00"^^xsd:dateTime  ;
	skos:exactMatch <https://www.wikidata.org/entity/Q179232> ;
	skos:broader	medtop:20000570 .

medtop:20001257
	rdf:type skos:Concept ;
	skos:prefLabel	"gardening"@en-GB ;
	skos:definition	"Interest in working in one's garden"@en-GB ;
	skos:inScheme <http://cv.iptc.org/newscodes/mediatopic/>  ;
	ikos:created "2019-07-30T12:00:00+00:00"^^xsd:dateTime ;
	dct:created "2019-07-30T12:00:00+00:00"^^xsd:dateTime ;
	ikos:modified "2021-07-12T12:00:00+00:00"^^xsd:dateTime ;
	dct:modified "2021-07-12T12:00:00+00:00"^^xsd:dateTime  ;
	skos:exactMatch <https://www.wikidata.org/entity/Q124946> ;
	skos:broader	medtop:20000570 .

medtop:20001258
	rdf:type skos:Concept ;
	skos:prefLabel	"consumer electronics"@en-GB ;
	skos:definition	"Electronic devices, such as computers, smart phones or televisions, designed and sold for personal use"@en-GB ;
	skos:inScheme <http://cv.iptc.org/newscodes/mediatopic/>  ;
	ikos:created "2019-08-02T12:00:00+00:00"^^xsd:dateTime ;
	dct:created "2019-08-02T12:00:00+00:00"^^xsd:dateTime ;
	ikos:modified "2021-07-12T12:00:00+00:00"^^xsd:dateTime ;
	dct:modified "2021-07-12T12:00:00+00:00"^^xsd:dateTime  ;
	skos:exactMatch <https://www.wikidata.org/entity/Q581105> ;
	skos:broader	medtop:20000243 .

medtop:20001259
	rdf:type skos:Concept ;
	skos:prefLabel	"political convention"@en-GB ;
	skos:definition	"Meeting of political party to nominate a candidate, choose a party leader or set policy"@en-GB ;
	skos:inScheme <http://cv.iptc.org/newscodes/mediatopic/>  ;
	ikos:created "2019-09-05T12:00:00+00:00"^^xsd:dateTime ;
	dct:created "2019-09-05T12:00:00+00:00"^^xsd:dateTime ;
	ikos:modified "2021-07-12T12:00:00+00:00"^^xsd:dateTime ;
	dct:modified "2021-07-12T12:00:00+00:00"^^xsd:dateTime  ;
	skos:exactMatch <https://www.wikidata.org/entity/Q16487126> ;
	skos:broader	medtop:20000593 .

medtop:20001260
	rdf:type skos:Concept ;
	skos:prefLabel	"political committees"@en-GB ;
	skos:definition	"A legislative sub-group that focuses on a specific area or action"@en-GB ;
	skos:inScheme <http://cv.iptc.org/newscodes/mediatopic/>  ;
	ikos:created "2019-09-05T12:00:00+00:00"^^xsd:dateTime ;
	dct:created "2019-09-05T12:00:00+00:00"^^xsd:dateTime ;
	ikos:modified "2021-07-12T12:00:00+00:00"^^xsd:dateTime ;
	dct:modified "2021-07-12T12:00:00+00:00"^^xsd:dateTime  ;
	skos:exactMatch <https://www.wikidata.org/entity/Q2986700> ;
	skos:broader	medtop:20000593 .

medtop:20001261
	rdf:type skos:Concept ;
	skos:prefLabel	"heads of government"@en-GB ;
	skos:definition	"The highest official in the executive branch of a sovereign state, a federated state, or a self-governing colony"@en-GB ;
	skos:inScheme <http://cv.iptc.org/newscodes/mediatopic/>  ;
	ikos:created "2019-09-05T12:00:00+00:00"^^xsd:dateTime ;
	dct:created "2019-09-05T12:00:00+00:00"^^xsd:dateTime ;
	ikos:modified "2021-07-12T12:00:00+00:00"^^xsd:dateTime ;
	dct:modified "2021-07-12T12:00:00+00:00"^^xsd:dateTime  ;
	skos:exactMatch <https://www.wikidata.org/entity/Q2285706> ;
	skos:broader	medtop:20000593 .

medtop:20001262
	rdf:type skos:Concept ;
	skos:prefLabel	"public inquiry"@en-GB ;
	skos:definition	"An official review of events or actions ordered by a government body, including royal commissions"@en-GB ;
	skos:inScheme <http://cv.iptc.org/newscodes/mediatopic/>  ;
	ikos:created "2019-09-05T12:00:00+00:00"^^xsd:dateTime ;
	dct:created "2019-09-05T12:00:00+00:00"^^xsd:dateTime ;
	ikos:modified "2021-07-12T12:00:00+00:00"^^xsd:dateTime ;
	dct:modified "2021-07-12T12:00:00+00:00"^^xsd:dateTime  ;
	skos:exactMatch <https://www.wikidata.org/entity/Q20669447> ;
	skos:broader	medtop:20000593 .

medtop:20001263
	rdf:type skos:Concept ;
	skos:prefLabel	"church elections"@en-GB ;
	skos:definition	"Elections to choose leaders to run church organisations at various levels"@en-GB ;
	skos:inScheme <http://cv.iptc.org/newscodes/mediatopic/>  ;
	ikos:created "2019-09-05T12:00:00+00:00"^^xsd:dateTime ;
	dct:created "2019-09-05T12:00:00+00:00"^^xsd:dateTime ;
	ikos:modified "2021-07-12T12:00:00+00:00"^^xsd:dateTime ;
	dct:modified "2021-07-12T12:00:00+00:00"^^xsd:dateTime  ;
	skos:exactMatch <https://www.wikidata.org/entity/Q6980735> ;
	skos:broader	medtop:20000574 .

medtop:20001264
	rdf:type skos:Concept ;
	skos:prefLabel	"infrastructure policy"@en-GB ;
	skos:definition	"Policies regarding the development and maintenance of the fundamental facilities of a country, city or other area that make business activity possible, such as communication, transportation and distribution networks"@en-GB ;
	skos:inScheme <http://cv.iptc.org/newscodes/mediatopic/>  ;
	ikos:created "2019-09-05T12:00:00+00:00"^^xsd:dateTime ;
	dct:created "2019-09-05T12:00:00+00:00"^^xsd:dateTime ;
	ikos:modified "2021-07-12T12:00:00+00:00"^^xsd:dateTime ;
	dct:modified "2021-07-12T12:00:00+00:00"^^xsd:dateTime  ;
	skos:broader	medtop:20000626 .

medtop:20001265
	rdf:type skos:Concept ;
	skos:prefLabel	"local government policy"@en-GB ;
	skos:definition	"Policies for the development and maintenance of a local government area"@en-GB ;
	skos:inScheme <http://cv.iptc.org/newscodes/mediatopic/>  ;
	ikos:created "2019-09-05T12:00:00+00:00"^^xsd:dateTime ;
	dct:created "2019-09-05T12:00:00+00:00"^^xsd:dateTime ;
	ikos:modified "2021-07-12T12:00:00+00:00"^^xsd:dateTime ;
	dct:modified "2021-07-12T12:00:00+00:00"^^xsd:dateTime  ;
	skos:exactMatch <https://www.wikidata.org/entity/Q1780384> ;
	skos:broader	medtop:20000621 .

medtop:20001266
	rdf:type skos:Concept ;
	skos:prefLabel	"political debates"@en-GB ;
	skos:definition	"Organised debates between political candidates, live in front of an audience or broadcast in some manner"@en-GB ;
	skos:inScheme <http://cv.iptc.org/newscodes/mediatopic/>  ;
	ikos:created "2019-09-05T12:00:00+00:00"^^xsd:dateTime ;
	dct:created "2019-09-05T12:00:00+00:00"^^xsd:dateTime ;
	ikos:modified "2021-07-12T12:00:00+00:00"^^xsd:dateTime ;
	dct:modified "2021-07-12T12:00:00+00:00"^^xsd:dateTime  ;
	skos:broader	medtop:20000574 .

medtop:20001267
	rdf:type skos:Concept ;
	skos:prefLabel	"Midsummer"@en-GB ;
	skos:definition	"Northern European celebrations that accompany the Summer solstice"@en-GB ;
	skos:inScheme <http://cv.iptc.org/newscodes/mediatopic/>  ;
	ikos:created "2019-09-05T12:00:00+00:00"^^xsd:dateTime ;
	dct:created "2019-09-05T12:00:00+00:00"^^xsd:dateTime ;
	ikos:modified "2021-07-12T12:00:00+00:00"^^xsd:dateTime ;
	dct:modified "2021-07-12T12:00:00+00:00"^^xsd:dateTime  ;
	skos:exactMatch <https://www.wikidata.org/entity/Q154502> ;
	skos:broader	medtop:20000552 .

medtop:20001268
	rdf:type skos:Concept ;
	skos:prefLabel	"National day"@en-GB ;
	skos:definition	"A designated day to celebrate a nation"@en-GB ;
	skos:inScheme <http://cv.iptc.org/newscodes/mediatopic/>  ;
	ikos:created "2019-09-05T12:00:00+00:00"^^xsd:dateTime ;
	dct:created "2019-09-05T12:00:00+00:00"^^xsd:dateTime ;
	ikos:modified "2021-07-12T12:00:00+00:00"^^xsd:dateTime ;
	dct:modified "2021-07-12T12:00:00+00:00"^^xsd:dateTime  ;
	skos:exactMatch <https://www.wikidata.org/entity/Q57598> ;
	skos:broader	medtop:20000552 .

medtop:20001269
	rdf:type skos:Concept ;
	skos:prefLabel	"New year"@en-GB ;
	skos:definition	"The celebration of the end of one calendar year and the start of next"@en-GB ;
	skos:inScheme <http://cv.iptc.org/newscodes/mediatopic/>  ;
	ikos:created "2019-09-05T12:00:00+00:00"^^xsd:dateTime ;
	dct:created "2019-09-05T12:00:00+00:00"^^xsd:dateTime ;
	ikos:modified "2021-07-12T12:00:00+00:00"^^xsd:dateTime ;
	dct:modified "2021-07-12T12:00:00+00:00"^^xsd:dateTime  ;
	skos:exactMatch <https://www.wikidata.org/entity/Q196627> ;
	skos:broader	medtop:20000552 .

medtop:20001270
	rdf:type skos:Concept ;
	skos:prefLabel	"Halloween"@en-GB ;
	skos:definition	"A celebration observed in a number of countries on 31 October with activities including trick-or-treating, wearing costumes, carving pumpkins,visiting haunted attractions, telling scary stories and watching horror films"@en-GB ;
	skos:inScheme <http://cv.iptc.org/newscodes/mediatopic/>  ;
	ikos:created "2019-09-05T12:00:00+00:00"^^xsd:dateTime ;
	dct:created "2019-09-05T12:00:00+00:00"^^xsd:dateTime ;
	ikos:modified "2021-07-12T12:00:00+00:00"^^xsd:dateTime ;
	dct:modified "2021-07-12T12:00:00+00:00"^^xsd:dateTime  ;
	skos:exactMatch <https://www.wikidata.org/entity/Q251868> ;
	skos:broader	medtop:20000551 .

medtop:20001271
	rdf:type skos:Concept ;
	skos:prefLabel	"All Saints Day"@en-GB ;
	skos:definition	"Christian festival celebrated in honour of all the saints, known and unknown. Holiday is also known as All Hallows' Day, Hallowmas, Feast of All Saints or Solemnity of All Saints."@en-GB ;
	skos:inScheme <http://cv.iptc.org/newscodes/mediatopic/>  ;
	ikos:created "2019-09-05T12:00:00+00:00"^^xsd:dateTime ;
	dct:created "2019-09-05T12:00:00+00:00"^^xsd:dateTime ;
	ikos:modified "2021-12-17T12:00:00+00:00"^^xsd:dateTime ;
	dct:modified "2021-12-17T12:00:00+00:00"^^xsd:dateTime  ;
	skos:exactMatch <https://www.wikidata.org/entity/Q587> ;
	skos:broader	medtop:20000690 .

medtop:20001272
	rdf:type skos:Concept ;
	skos:prefLabel	"Walpurgis night"@en-GB ;
	skos:definition	"The eve of the Christian feast day of Saint Walpurga, an 8th-century abbess in Francia, celebrated on the night of 30 April and the day of 1 May"@en-GB ;
	skos:inScheme <http://cv.iptc.org/newscodes/mediatopic/>  ;
	ikos:created "2019-09-05T12:00:00+00:00"^^xsd:dateTime ;
	dct:created "2019-09-05T12:00:00+00:00"^^xsd:dateTime ;
	ikos:modified "2021-07-12T12:00:00+00:00"^^xsd:dateTime ;
	dct:modified "2021-07-12T12:00:00+00:00"^^xsd:dateTime  ;
	skos:exactMatch <https://www.wikidata.org/entity/Q200982> ;
	skos:broader	medtop:20000690 .

medtop:20001273
	rdf:type skos:Concept ;
	skos:prefLabel	"baptism"@en-GB ;
	skos:definition	"A Christian religious rite, sometimes also called a Christening, involving the sprinkling of holy water onto a person's forehead or immersing them in water, symbolising purification and admission to the Church"@en-GB ;
	skos:inScheme <http://cv.iptc.org/newscodes/mediatopic/>  ;
	ikos:created "2019-09-05T12:00:00+00:00"^^xsd:dateTime ;
	dct:created "2019-09-05T12:00:00+00:00"^^xsd:dateTime ;
	ikos:modified "2021-12-17T12:00:00+00:00"^^xsd:dateTime ;
	dct:modified "2021-12-17T12:00:00+00:00"^^xsd:dateTime  ;
	skos:exactMatch <https://www.wikidata.org/entity/Q35856> ;
	skos:broader	medtop:20000696 .

medtop:20001274
	rdf:type skos:Concept ;
	skos:prefLabel	"contraception"@en-GB ;
	skos:definition	"A method or device used to prevent pregnancy"@en-GB ;
	skos:inScheme <http://cv.iptc.org/newscodes/mediatopic/>  ;
	ikos:created "2019-09-05T12:00:00+00:00"^^xsd:dateTime ;
	dct:created "2019-09-05T12:00:00+00:00"^^xsd:dateTime ;
	ikos:modified "2021-07-12T12:00:00+00:00"^^xsd:dateTime ;
	dct:modified "2021-07-12T12:00:00+00:00"^^xsd:dateTime  ;
	skos:exactMatch <https://www.wikidata.org/entity/Q122224> ;
	skos:broader	medtop:20000784 .

medtop:20001275
	rdf:type skos:Concept ;
	skos:prefLabel	"gig economy"@en-GB ;
	skos:definition	"a labour market consisting of individual suppliers on short-term contracts or freelance work as opposed to permanent jobs, such as drivers or delivery workers"@en-GB ;
	skos:inScheme <http://cv.iptc.org/newscodes/mediatopic/>  ;
	ikos:created "2019-10-07T12:00:00+00:00"^^xsd:dateTime ;
	dct:created "2019-10-07T12:00:00+00:00"^^xsd:dateTime ;
	ikos:modified "2021-07-12T12:00:00+00:00"^^xsd:dateTime ;
	dct:modified "2021-07-12T12:00:00+00:00"^^xsd:dateTime  ;
	skos:exactMatch <https://www.wikidata.org/entity/Q56408801> ;
	skos:broader	medtop:20000523 .

medtop:20001276
	rdf:type skos:Concept ;
	skos:prefLabel	"parental leave"@en-GB ;
	skos:definition	"Time off work to give birth or care for a child"@en-GB ;
	skos:inScheme <http://cv.iptc.org/newscodes/mediatopic/>  ;
	ikos:created "2019-10-07T12:00:00+00:00"^^xsd:dateTime ;
	dct:created "2019-10-07T12:00:00+00:00"^^xsd:dateTime ;
	ikos:modified "2021-07-12T12:00:00+00:00"^^xsd:dateTime ;
	dct:modified "2021-07-12T12:00:00+00:00"^^xsd:dateTime  ;
	skos:exactMatch <https://www.wikidata.org/entity/Q328566> ;
	skos:broader	medtop:20000509 .

medtop:20001277
	rdf:type skos:Concept ;
	skos:prefLabel	"volunteering"@en-GB ;
	skos:definition	"Unpaid work undertaken freely by individuals as a service to others"@en-GB ;
	skos:inScheme <http://cv.iptc.org/newscodes/mediatopic/>  ;
	ikos:created "2019-10-07T12:00:00+00:00"^^xsd:dateTime ;
	dct:created "2019-10-07T12:00:00+00:00"^^xsd:dateTime ;
	ikos:modified "2021-07-12T12:00:00+00:00"^^xsd:dateTime ;
	dct:modified "2021-07-12T12:00:00+00:00"^^xsd:dateTime  ;
	skos:exactMatch <https://www.wikidata.org/entity/Q188844> ;
	skos:broader	medtop:20000509 .

medtop:20001278
	rdf:type skos:Concept ;
	skos:prefLabel	"cooperative"@en-GB ;
	skos:definition	"An organisation which is owned and run jointly by its members, who share the profits or benefits of their work"@en-GB ;
	skos:inScheme <http://cv.iptc.org/newscodes/mediatopic/>  ;
	ikos:created "2019-10-07T12:00:00+00:00"^^xsd:dateTime ;
	dct:created "2019-10-07T12:00:00+00:00"^^xsd:dateTime ;
	ikos:modified "2021-07-12T12:00:00+00:00"^^xsd:dateTime ;
	dct:modified "2021-07-12T12:00:00+00:00"^^xsd:dateTime  ;
	skos:exactMatch <https://www.wikidata.org/entity/Q4539> ;
	skos:broader	medtop:20000349 .

medtop:20001279
	rdf:type skos:Concept ;
	skos:prefLabel	"cryptocurrency"@en-GB ;
	skos:definition	"An internet-based medium of exchange using cryptography to conduct financial transactions"@en-GB ;
	skos:inScheme <http://cv.iptc.org/newscodes/mediatopic/>  ;
	ikos:created "2019-10-07T12:00:00+00:00"^^xsd:dateTime ;
	dct:created "2019-10-07T12:00:00+00:00"^^xsd:dateTime ;
	ikos:modified "2021-07-12T12:00:00+00:00"^^xsd:dateTime ;
	dct:modified "2021-07-12T12:00:00+00:00"^^xsd:dateTime  ;
	skos:exactMatch <https://www.wikidata.org/entity/Q13479982> ;
	skos:broader	medtop:20000355 .

medtop:20001280
	rdf:type skos:Concept ;
	skos:prefLabel	"hurricane"@en-GB ;
	skos:definition	"A type of storm also called a tropical cyclone, which forms over tropical or subtropical waters"@en-GB ;
	skos:inScheme <http://cv.iptc.org/newscodes/mediatopic/>  ;
	ikos:created "2019-10-07T12:00:00+00:00"^^xsd:dateTime ;
	dct:created "2019-10-07T12:00:00+00:00"^^xsd:dateTime ;
	ikos:modified "2021-07-12T12:00:00+00:00"^^xsd:dateTime ;
	dct:modified "2021-07-12T12:00:00+00:00"^^xsd:dateTime  ;
	skos:exactMatch <https://www.wikidata.org/entity/Q58197759> ;
	skos:broader	medtop:20000157 .

medtop:20001281
	rdf:type skos:Concept ;
	skos:prefLabel	"racquetball"@en-GB ;
	skos:definition	"A racquet sport similar to squash in which the ball must bounce once before being struck and with a greater area of in-bound play"@en-GB ;
	skos:inScheme <http://cv.iptc.org/newscodes/mediatopic/>  ;
	ikos:created "2019-10-07T12:00:00+00:00"^^xsd:dateTime ;
	dct:created "2019-10-07T12:00:00+00:00"^^xsd:dateTime ;
	ikos:modified "2021-07-12T12:00:00+00:00"^^xsd:dateTime ;
	dct:modified "2021-07-12T12:00:00+00:00"^^xsd:dateTime  ;
	skos:exactMatch <https://www.wikidata.org/entity/Q754586> ;
	skos:broader	medtop:20000822 .

medtop:20001282
	rdf:type skos:Concept ;
	skos:prefLabel	"ringette"@en-GB ;
	skos:definition	"A team sport usually played on ice by skaters using a straight stick. Players pass and shoot a rubber ring in order to place it in the opponent's goal"@en-GB ;
	skos:inScheme <http://cv.iptc.org/newscodes/mediatopic/>  ;
	ikos:created "2019-10-07T12:00:00+00:00"^^xsd:dateTime ;
	dct:created "2019-10-07T12:00:00+00:00"^^xsd:dateTime ;
	ikos:modified "2021-07-12T12:00:00+00:00"^^xsd:dateTime ;
	dct:modified "2021-07-12T12:00:00+00:00"^^xsd:dateTime  ;
	skos:exactMatch <https://www.wikidata.org/entity/Q1972786> ;
	skos:broader	medtop:20000822 .

medtop:20001283
	rdf:type skos:Concept ;
	skos:prefLabel	"human smuggling and trafficking"@en-GB ;
	skos:definition	"The illegal transporting of people from one country or area to another. When the result is forced labour or sexual exploitation, the crime is considered trafficking."@en-GB ;
	skos:inScheme <http://cv.iptc.org/newscodes/mediatopic/>  ;
	ikos:created "2019-11-20T12:00:00+00:00"^^xsd:dateTime ;
	dct:created "2019-11-20T12:00:00+00:00"^^xsd:dateTime ;
	ikos:modified "2021-07-12T12:00:00+00:00"^^xsd:dateTime ;
	dct:modified "2021-07-12T12:00:00+00:00"^^xsd:dateTime  ;
	skos:exactMatch <https://www.wikidata.org/entity/Q181784> ;
	skos:broader	medtop:20000082 .

medtop:20001284
	rdf:type skos:Concept ;
	skos:prefLabel	"bullying"@en-GB ;
	skos:definition	"Taking actions meant to harm, coerce and intimidate another person perceived as vulnerable. These actions can be taken in person or online."@en-GB ;
	skos:inScheme <http://cv.iptc.org/newscodes/mediatopic/>  ;
	ikos:created "2019-11-20T12:00:00+00:00"^^xsd:dateTime ;
	dct:created "2019-11-20T12:00:00+00:00"^^xsd:dateTime ;
	ikos:modified "2021-07-12T12:00:00+00:00"^^xsd:dateTime ;
	dct:modified "2021-07-12T12:00:00+00:00"^^xsd:dateTime  ;
	skos:exactMatch <https://www.wikidata.org/entity/Q240126> ;
	skos:broader	medtop:20000802 .

medtop:20001285
	rdf:type skos:Concept ;
	skos:prefLabel	"vandalism"@en-GB ;
	skos:definition	"Deliberately damaging or destroying public or private property"@en-GB ;
	skos:inScheme <http://cv.iptc.org/newscodes/mediatopic/>  ;
	ikos:created "2019-11-20T12:00:00+00:00"^^xsd:dateTime ;
	dct:created "2019-11-20T12:00:00+00:00"^^xsd:dateTime ;
	ikos:modified "2021-07-12T12:00:00+00:00"^^xsd:dateTime ;
	dct:modified "2021-07-12T12:00:00+00:00"^^xsd:dateTime  ;
	skos:exactMatch <https://www.wikidata.org/entity/Q6160> ;
	skos:broader	medtop:20000082 .

medtop:20001286
	rdf:type skos:Concept ;
	skos:prefLabel	"arm wrestling"@en-GB ;
	skos:definition	"A form of wrestling in which two participants grapple arm-to-arm"@en-GB ;
	skos:inScheme <http://cv.iptc.org/newscodes/mediatopic/>  ;
	ikos:created "2019-11-25T12:00:00+00:00"^^xsd:dateTime ;
	dct:created "2019-11-25T12:00:00+00:00"^^xsd:dateTime ;
	ikos:modified "2021-07-12T12:00:00+00:00"^^xsd:dateTime ;
	dct:modified "2021-07-12T12:00:00+00:00"^^xsd:dateTime  ;
	skos:exactMatch <https://www.wikidata.org/entity/Q282772> ;
	skos:broader	medtop:20000822 .

medtop:20001287
	rdf:type skos:Concept ;
	skos:prefLabel	"supreme and high court"@en-GB ;
	skos:definition	"matters related to supreme or high courts, including nominations and rulings"@en-GB ;
	skos:inScheme <http://cv.iptc.org/newscodes/mediatopic/>  ;
	ikos:created "2019-11-25T12:00:00+00:00"^^xsd:dateTime ;
	dct:created "2019-11-25T12:00:00+00:00"^^xsd:dateTime ;
	ikos:modified "2021-07-12T12:00:00+00:00"^^xsd:dateTime ;
	dct:modified "2021-07-12T12:00:00+00:00"^^xsd:dateTime  ;
	skos:exactMatch <https://www.wikidata.org/entity/Q190752> ;
	skos:broader	medtop:20000107 .

medtop:20001288
	rdf:type skos:Concept ;
	skos:prefLabel	"indigenous people"@en-GB ;
	skos:definition	"People who are the original owners and caretakers of a given region, also known as native peoples, first peoples or aboriginal peoples, in contrast to groups that have settled, occupied or colonised the area more recently"@en-GB ;
	skos:inScheme <http://cv.iptc.org/newscodes/mediatopic/>  ;
	ikos:created "2019-11-25T12:00:00+00:00"^^xsd:dateTime ;
	dct:created "2019-11-25T12:00:00+00:00"^^xsd:dateTime ;
	ikos:modified "2021-07-12T12:00:00+00:00"^^xsd:dateTime ;
	dct:modified "2021-07-12T12:00:00+00:00"^^xsd:dateTime  ;
	skos:exactMatch <https://www.wikidata.org/entity/Q103817> ;
	skos:broader	medtop:20000788 .

medtop:20001289
	rdf:type skos:Concept ;
	skos:prefLabel	"sales channel"@en-GB ;
	skos:definition	"Indirect or direct ways of bringing products or services to market so that they can be purchased by consumers"@en-GB ;
	skos:inScheme <http://cv.iptc.org/newscodes/mediatopic/>  ;
	ikos:created "2019-11-25T12:00:00+00:00"^^xsd:dateTime ;
	dct:created "2019-11-25T12:00:00+00:00"^^xsd:dateTime ;
	ikos:modified "2023-03-31T12:00:00+00:00"^^xsd:dateTime ;
	dct:modified "2023-03-31T12:00:00+00:00"^^xsd:dateTime  ;
	skos:exactMatch <https://www.wikidata.org/entity/Q6576947> ;
	skos:broader	medtop:20000209 ;
	skos:narrower	medtop:20000252 ;
	skos:narrower	medtop:20000255 ;
	skos:narrower	medtop:20000273 .

medtop:20001290
	rdf:type skos:Concept ;
	skos:prefLabel	"public housing"@en-GB ;
	skos:definition	"Housing that is owned or managed by a government or nonprofit organisation and rented to tenants with the aim of making housing affordable. Eligibility for such housing arrangements varies country to country."@en-GB ;
	skos:inScheme <http://cv.iptc.org/newscodes/mediatopic/>  ;
	ikos:created "2020-08-05T12:00:00+00:00"^^xsd:dateTime ;
	dct:created "2020-08-05T12:00:00+00:00"^^xsd:dateTime ;
	ikos:modified "2021-07-12T12:00:00+00:00"^^xsd:dateTime ;
	dct:modified "2021-07-12T12:00:00+00:00"^^xsd:dateTime  ;
	skos:exactMatch <https://www.wikidata.org/entity/Q6532502> ;
	skos:broader	medtop:20000817 .

medtop:20001291
	rdf:type skos:Concept ;
	skos:prefLabel	"heating and cooling"@en-GB ;
	skos:definition	"The business of supplying heat or cooling to private residences and commercial buildings"@en-GB ;
	skos:inScheme <http://cv.iptc.org/newscodes/mediatopic/>  ;
	ikos:created "2020-08-05T12:00:00+00:00"^^xsd:dateTime ;
	dct:created "2020-08-05T12:00:00+00:00"^^xsd:dateTime ;
	ikos:modified "2023-03-31T12:00:00+00:00"^^xsd:dateTime ;
	dct:modified "2023-03-31T12:00:00+00:00"^^xsd:dateTime  ;
	skos:exactMatch <https://www.wikidata.org/entity/Q1798773> ;
	skos:broader	medtop:20001244 .

medtop:20001292
	rdf:type skos:Concept ;
	skos:prefLabel	"economic development incentive"@en-GB ;
	skos:definition	"funding, financial incentive programmes and subsidies to stimulate businesses and parts of the economy"@en-GB ;
	skos:inScheme <http://cv.iptc.org/newscodes/mediatopic/>  ;
	ikos:created "2020-08-05T12:00:00+00:00"^^xsd:dateTime ;
	dct:created "2020-08-05T12:00:00+00:00"^^xsd:dateTime ;
	ikos:modified "2021-07-12T12:00:00+00:00"^^xsd:dateTime ;
	dct:modified "2021-07-12T12:00:00+00:00"^^xsd:dateTime  ;
	skos:exactMatch <https://www.wikidata.org/entity/Q5333369> ;
	skos:broader	medtop:20000345 .

medtop:20001293
	rdf:type skos:Concept ;
	skos:prefLabel	"streaming service"@en-GB ;
	skos:definition	"Providers of entertainment (music, movies, series, etc.) that deliver the content via an internet connection to the subscriber's computer, TV or mobile device"@en-GB ;
	skos:inScheme <http://cv.iptc.org/newscodes/mediatopic/>  ;
	ikos:created "2020-08-05T12:00:00+00:00"^^xsd:dateTime ;
	dct:created "2020-08-05T12:00:00+00:00"^^xsd:dateTime ;
	ikos:modified "2023-03-31T12:00:00+00:00"^^xsd:dateTime ;
	dct:modified "2023-03-31T12:00:00+00:00"^^xsd:dateTime  ;
	skos:exactMatch <https://www.wikidata.org/entity/Q63241860> ;
	skos:broader	medtop:20000304 .

medtop:20001294
	rdf:type skos:Concept ;
	skos:prefLabel	"crowdfunding"@en-GB ;
	skos:definition	"The funding of a project or venture by raising small amounts of money from a large number of people, typically via the internet"@en-GB ;
	skos:inScheme <http://cv.iptc.org/newscodes/mediatopic/>  ;
	ikos:created "2020-08-05T12:00:00+00:00"^^xsd:dateTime ;
	dct:created "2020-08-05T12:00:00+00:00"^^xsd:dateTime ;
	ikos:modified "2023-03-31T12:00:00+00:00"^^xsd:dateTime ;
	dct:modified "2023-03-31T12:00:00+00:00"^^xsd:dateTime  ;
	skos:exactMatch <https://www.wikidata.org/entity/Q348303> ;
	skos:broader	medtop:20000183 .

medtop:20001295
	rdf:type skos:Concept ;
	skos:prefLabel	"outsourcing"@en-GB ;
	skos:definition	"Business practice in which services or job functions are farmed out to a third party"@en-GB ;
	skos:inScheme <http://cv.iptc.org/newscodes/mediatopic/>  ;
	ikos:created "2020-08-05T12:00:00+00:00"^^xsd:dateTime ;
	dct:created "2020-08-05T12:00:00+00:00"^^xsd:dateTime ;
	ikos:modified "2021-07-12T12:00:00+00:00"^^xsd:dateTime ;
	dct:modified "2021-07-12T12:00:00+00:00"^^xsd:dateTime  ;
	skos:exactMatch <https://www.wikidata.org/entity/Q61515> ;
	skos:broader	medtop:20000192 .

medtop:20001296
	rdf:type skos:Concept ;
	skos:prefLabel	"shopping mall"@en-GB ;
	skos:definition	"A large building or series of connected buildings that contain a variety of retail stores and food vendors"@en-GB ;
	skos:inScheme <http://cv.iptc.org/newscodes/mediatopic/>  ;
	ikos:created "2020-08-05T12:00:00+00:00"^^xsd:dateTime ;
	dct:created "2020-08-05T12:00:00+00:00"^^xsd:dateTime ;
	ikos:modified "2021-07-12T12:00:00+00:00"^^xsd:dateTime ;
	dct:modified "2021-07-12T12:00:00+00:00"^^xsd:dateTime  ;
	skos:exactMatch <https://www.wikidata.org/entity/Q97395548> ;
	skos:broader	medtop:20000252 .

medtop:20001297
	rdf:type skos:Concept ;
	skos:prefLabel	"shopping district and high street"@en-GB ;
	skos:definition	"Primary retail streets of towns or cities containing individual stores and restaurants"@en-GB ;
	skos:inScheme <http://cv.iptc.org/newscodes/mediatopic/>  ;
	ikos:created "2020-08-05T12:00:00+00:00"^^xsd:dateTime ;
	dct:created "2020-08-05T12:00:00+00:00"^^xsd:dateTime ;
	ikos:modified "2021-07-12T12:00:00+00:00"^^xsd:dateTime ;
	dct:modified "2021-07-12T12:00:00+00:00"^^xsd:dateTime  ;
	skos:exactMatch <https://www.wikidata.org/entity/Q21000333> ;
	skos:broader	medtop:20000252 .

medtop:20001298
	rdf:type skos:Concept ;
	skos:prefLabel	"artificial intelligence"@en-GB ;
	skos:definition	"An attempt to let computers simulate how the human brain works by applying statistical, heuristic or machine learning methods and algorithms to large datasets. Enables a long range of automatic functions like image recognition and categorisation."@en-GB ;
	skos:inScheme <http://cv.iptc.org/newscodes/mediatopic/>  ;
	ikos:created "2020-08-05T12:00:00+00:00"^^xsd:dateTime ;
	dct:created "2020-08-05T12:00:00+00:00"^^xsd:dateTime ;
	ikos:modified "2021-07-12T12:00:00+00:00"^^xsd:dateTime ;
	dct:modified "2021-07-12T12:00:00+00:00"^^xsd:dateTime  ;
	skos:exactMatch <https://www.wikidata.org/entity/Q11660> ;
	skos:broader	medtop:20000763 .

medtop:20001299
	rdf:type skos:Concept ;
	skos:prefLabel	"surveillance"@en-GB ;
	skos:definition	"Monitoring the activities of the individual through the use of cameras and data in order to prevent or uncover criminal activities"@en-GB ;
	skos:inScheme <http://cv.iptc.org/newscodes/mediatopic/>  ;
	ikos:created "2020-08-05T12:00:00+00:00"^^xsd:dateTime ;
	dct:created "2020-08-05T12:00:00+00:00"^^xsd:dateTime ;
	ikos:modified "2021-07-12T12:00:00+00:00"^^xsd:dateTime ;
	dct:modified "2021-07-12T12:00:00+00:00"^^xsd:dateTime  ;
	skos:exactMatch <https://www.wikidata.org/entity/Q334401> ;
	skos:broader	medtop:20000129 .

medtop:20001300
	rdf:type skos:Concept ;
	skos:prefLabel	"privacy"@en-GB ;
	skos:definition	"The right of an individual or group to keep information about themselves private"@en-GB ;
	skos:inScheme <http://cv.iptc.org/newscodes/mediatopic/>  ;
	ikos:created "2020-08-05T12:00:00+00:00"^^xsd:dateTime ;
	dct:created "2020-08-05T12:00:00+00:00"^^xsd:dateTime ;
	ikos:modified "2021-07-12T12:00:00+00:00"^^xsd:dateTime ;
	dct:modified "2021-07-12T12:00:00+00:00"^^xsd:dateTime  ;
	skos:exactMatch <https://www.wikidata.org/entity/Q188728> ;
	skos:broader	medtop:20000587 .

medtop:20001301
	rdf:type skos:Concept ;
	skos:prefLabel	"sport achievement"@en-GB ;
	skos:definition	"Records or honours earned by athletes for their performance"@en-GB ;
	skos:inScheme <http://cv.iptc.org/newscodes/mediatopic/>  ;
	ikos:created "2021-02-18T12:00:00+00:00"^^xsd:dateTime ;
	dct:created "2021-02-18T12:00:00+00:00"^^xsd:dateTime ;
	ikos:modified "2021-07-12T12:00:00+00:00"^^xsd:dateTime ;
	dct:modified "2021-07-12T12:00:00+00:00"^^xsd:dateTime  ;
	skos:broader	medtop:15000000 ;
	skos:narrower	medtop:20001302 ;
	skos:narrower	medtop:20001303 ;
	skos:narrower	medtop:20001304 .

medtop:20001302
	rdf:type skos:Concept ;
	skos:prefLabel	"sports record"@en-GB ;
	skos:definition	"The best performance to date by an athlete or team in a sport discipline"@en-GB ;
	skos:inScheme <http://cv.iptc.org/newscodes/mediatopic/>  ;
	ikos:created "2021-02-18T12:00:00+00:00"^^xsd:dateTime ;
	dct:created "2021-02-18T12:00:00+00:00"^^xsd:dateTime ;
	ikos:modified "2022-09-23T12:00:00+00:00"^^xsd:dateTime ;
	dct:modified "2022-09-23T12:00:00+00:00"^^xsd:dateTime  ;
	skos:broader	medtop:20001301 .

medtop:20001303
	rdf:type skos:Concept ;
	skos:prefLabel	"sports medal and trophy"@en-GB ;
	skos:definition	"Award given to an athlete or team for placing in a sports competition, such as a gold medal at the Olympics or the Stanley Cup in ice hockey"@en-GB ;
	skos:inScheme <http://cv.iptc.org/newscodes/mediatopic/>  ;
	ikos:created "2021-02-18T12:00:00+00:00"^^xsd:dateTime ;
	dct:created "2021-02-18T12:00:00+00:00"^^xsd:dateTime ;
	ikos:modified "2022-09-23T12:00:00+00:00"^^xsd:dateTime ;
	dct:modified "2022-09-23T12:00:00+00:00"^^xsd:dateTime  ;
	skos:broadMatch <https://www.wikidata.org/entity/Q15229207> ;
	skos:broader	medtop:20001301 .

medtop:20001304
	rdf:type skos:Concept ;
	skos:prefLabel	"sports honour"@en-GB ;
	skos:definition	"Honour given to a player for achievements over a career, season or single event, unrelated to event outcome, usually awarded by a panel of judges or a popular vote. Examples include player of the game, most valuable player award or hall of fame induction."@en-GB ;
	skos:inScheme <http://cv.iptc.org/newscodes/mediatopic/>  ;
	ikos:created "2021-02-18T12:00:00+00:00"^^xsd:dateTime ;
	dct:created "2021-02-18T12:00:00+00:00"^^xsd:dateTime ;
	ikos:modified "2022-09-23T12:00:00+00:00"^^xsd:dateTime ;
	dct:modified "2022-09-23T12:00:00+00:00"^^xsd:dateTime  ;
	skos:exactMatch <https://www.wikidata.org/entity/Q15229207> ;
	skos:broader	medtop:20001301 .

medtop:20001305
	rdf:type skos:Concept ;
	skos:prefLabel	"padel"@en-GB ;
	skos:definition	"Racquet sport typically played in doubles on an enclosed court"@en-GB ;
	skos:inScheme <http://cv.iptc.org/newscodes/mediatopic/>  ;
	ikos:created "2021-02-18T12:00:00+00:00"^^xsd:dateTime ;
	dct:created "2021-02-18T12:00:00+00:00"^^xsd:dateTime ;
	ikos:modified "2021-07-12T12:00:00+00:00"^^xsd:dateTime ;
	dct:modified "2021-07-12T12:00:00+00:00"^^xsd:dateTime  ;
	skos:exactMatch <https://www.wikidata.org/entity/Q1582389> ;
	skos:broader	medtop:20000822 .

medtop:20001306
	rdf:type skos:Concept ;
	skos:prefLabel	"kiting"@en-GB ;
	skos:definition	"Action sport where a person harnesses the power of the wind to propel themselves across water, land or snow on a board, snowboard or skis. Variations of the sport are called kiteboarding/kitesurfing, snowkiting or landkiting."@en-GB ;
	skos:inScheme <http://cv.iptc.org/newscodes/mediatopic/>  ;
	ikos:created "2021-02-18T12:00:00+00:00"^^xsd:dateTime ;
	dct:created "2021-02-18T12:00:00+00:00"^^xsd:dateTime ;
	ikos:modified "2021-07-12T12:00:00+00:00"^^xsd:dateTime ;
	dct:modified "2021-07-12T12:00:00+00:00"^^xsd:dateTime  ;
	skos:exactMatch <https://www.wikidata.org/entity/Q219554> ;
	skos:broader	medtop:20000822 .

medtop:20001307
	rdf:type skos:Concept ;
	skos:prefLabel	"stand up paddleboarding (SUP)"@en-GB ;
	skos:definition	"Water sport using a board and paddle to propel through the water while standing"@en-GB ;
	skos:inScheme <http://cv.iptc.org/newscodes/mediatopic/>  ;
	ikos:created "2021-02-18T12:00:00+00:00"^^xsd:dateTime ;
	dct:created "2021-02-18T12:00:00+00:00"^^xsd:dateTime ;
	ikos:modified "2021-07-12T12:00:00+00:00"^^xsd:dateTime ;
	dct:modified "2021-07-12T12:00:00+00:00"^^xsd:dateTime  ;
	skos:exactMatch <https://www.wikidata.org/entity/Q2035123> ;
	skos:broader	medtop:20000822 .

medtop:20001308
	rdf:type skos:Concept ;
	skos:prefLabel	"krav maga"@en-GB ;
	skos:definition	"Fighting and self-defence sport that combines elements from aikido, boxing, judo, karate and wrestling"@en-GB ;
	skos:inScheme <http://cv.iptc.org/newscodes/mediatopic/>  ;
	ikos:created "2021-02-18T12:00:00+00:00"^^xsd:dateTime ;
	dct:created "2021-02-18T12:00:00+00:00"^^xsd:dateTime ;
	ikos:modified "2021-07-12T12:00:00+00:00"^^xsd:dateTime ;
	dct:modified "2021-07-12T12:00:00+00:00"^^xsd:dateTime  ;
	skos:exactMatch <https://www.wikidata.org/entity/Q184733> ;
	skos:broader	medtop:20001157 .

medtop:20001309
	rdf:type skos:Concept ;
	skos:prefLabel	"cheerleading"@en-GB ;
	skos:definition	"Cheer squads competing against each other to perform a routine that includes stunts, jumps and tumbling set to music. Squads are judged on difficulty and execution."@en-GB ;
	skos:inScheme <http://cv.iptc.org/newscodes/mediatopic/>  ;
	ikos:created "2021-02-18T12:00:00+00:00"^^xsd:dateTime ;
	dct:created "2021-02-18T12:00:00+00:00"^^xsd:dateTime ;
	ikos:modified "2021-07-12T12:00:00+00:00"^^xsd:dateTime ;
	dct:modified "2021-07-12T12:00:00+00:00"^^xsd:dateTime  ;
	skos:exactMatch <https://www.wikidata.org/entity/Q61391> ;
	skos:broader	medtop:20000822 .

medtop:20001310
	rdf:type skos:Concept ;
	skos:prefLabel	"kickboxing"@en-GB ;
	skos:definition	"Stand-up combat sport based on kicking and punching an opponent"@en-GB ;
	skos:inScheme <http://cv.iptc.org/newscodes/mediatopic/>  ;
	ikos:created "2021-02-18T12:00:00+00:00"^^xsd:dateTime ;
	dct:created "2021-02-18T12:00:00+00:00"^^xsd:dateTime ;
	ikos:modified "2021-07-12T12:00:00+00:00"^^xsd:dateTime ;
	dct:modified "2021-07-12T12:00:00+00:00"^^xsd:dateTime  ;
	skos:exactMatch <https://www.wikidata.org/entity/Q178678> ;
	skos:broader	medtop:20001157 .

medtop:20001311
	rdf:type skos:Concept ;
	skos:prefLabel	"sambo (martial art)"@en-GB ;
	skos:definition	"Style of martial art originating in the Soviet Union that is recognised as a form of amateur wrestling"@en-GB ;
	skos:inScheme <http://cv.iptc.org/newscodes/mediatopic/>  ;
	ikos:created "2021-02-18T12:00:00+00:00"^^xsd:dateTime ;
	dct:created "2021-02-18T12:00:00+00:00"^^xsd:dateTime ;
	ikos:modified "2021-07-12T12:00:00+00:00"^^xsd:dateTime ;
	dct:modified "2021-07-12T12:00:00+00:00"^^xsd:dateTime  ;
	skos:exactMatch <https://www.wikidata.org/entity/Q106500> ;
	skos:broader	medtop:20001157 .

medtop:20001312
	rdf:type skos:Concept ;
	skos:prefLabel	"political leadership"@en-GB ;
	skos:definition	"The leaders within a political party"@en-GB ;
	skos:inScheme <http://cv.iptc.org/newscodes/mediatopic/>  ;
	ikos:created "2021-02-18T12:00:00+00:00"^^xsd:dateTime ;
	dct:created "2021-02-18T12:00:00+00:00"^^xsd:dateTime ;
	ikos:modified "2021-07-12T12:00:00+00:00"^^xsd:dateTime ;
	dct:modified "2021-07-12T12:00:00+00:00"^^xsd:dateTime  ;
	skos:exactMatch <https://www.wikidata.org/entity/Q1553195> ;
	skos:broader	medtop:20000651 .

medtop:20001313
	rdf:type skos:Concept ;
	skos:prefLabel	"shootings"@en-GB ;
	skos:definition	"An act of violence committed by individuals with the use of armed weapons"@en-GB ;
	skos:inScheme <http://cv.iptc.org/newscodes/mediatopic/>  ;
	ikos:created "2021-02-18T12:00:00+00:00"^^xsd:dateTime ;
	dct:created "2021-02-18T12:00:00+00:00"^^xsd:dateTime ;
	ikos:modified "2021-07-12T12:00:00+00:00"^^xsd:dateTime ;
	dct:modified "2021-07-12T12:00:00+00:00"^^xsd:dateTime  ;
	skos:exactMatch <https://www.wikidata.org/entity/Q2252077> ;
	skos:broader	medtop:20000082 .

medtop:20001314
	rdf:type skos:Concept ;
	skos:prefLabel	"animal abuse"@en-GB ;
	skos:definition	"The infliction of cruelty or neglect onto animals by humans"@en-GB ;
	skos:inScheme <http://cv.iptc.org/newscodes/mediatopic/>  ;
	ikos:created "2021-02-18T12:00:00+00:00"^^xsd:dateTime ;
	dct:created "2021-02-18T12:00:00+00:00"^^xsd:dateTime ;
	ikos:modified "2021-07-12T12:00:00+00:00"^^xsd:dateTime ;
	dct:modified "2021-07-12T12:00:00+00:00"^^xsd:dateTime  ;
	skos:exactMatch <https://www.wikidata.org/entity/Q40053> ;
	skos:broader	medtop:20000082 .

medtop:20001315
	rdf:type skos:Concept ;
	skos:prefLabel	"zoo"@en-GB ;
	skos:definition	"A park where visitors can see both wild and tame animals that are kept in cages or enclosed areas"@en-GB ;
	skos:inScheme <http://cv.iptc.org/newscodes/mediatopic/>  ;
	ikos:created "2021-02-18T12:00:00+00:00"^^xsd:dateTime ;
	dct:created "2021-02-18T12:00:00+00:00"^^xsd:dateTime ;
	ikos:modified "2021-07-12T12:00:00+00:00"^^xsd:dateTime ;
	dct:modified "2021-07-12T12:00:00+00:00"^^xsd:dateTime  ;
	skos:exactMatch <https://www.wikidata.org/entity/Q43501> ;
	skos:broader	medtop:20000553 .

medtop:20001316
	rdf:type skos:Concept ;
	skos:prefLabel	"border disputes"@en-GB ;
	skos:definition	"Diplomatic issues between two countries surrounding the border, sometimes involving military conflict"@en-GB ;
	skos:inScheme <http://cv.iptc.org/newscodes/mediatopic/>  ;
	ikos:created "2021-02-18T12:00:00+00:00"^^xsd:dateTime ;
	dct:created "2021-02-18T12:00:00+00:00"^^xsd:dateTime ;
	ikos:modified "2021-07-12T12:00:00+00:00"^^xsd:dateTime ;
	dct:modified "2021-07-12T12:00:00+00:00"^^xsd:dateTime  ;
	skos:exactMatch <https://www.wikidata.org/entity/Q1078001> ;
	skos:broader	medtop:20000638 .

medtop:20001317
	rdf:type skos:Concept ;
	skos:prefLabel	"child care"@en-GB ;
	skos:definition	"Services and facilities that look after children while their parents are working or away, including daycare centres and programmes"@en-GB ;
	skos:inScheme <http://cv.iptc.org/newscodes/mediatopic/>  ;
	ikos:created "2021-02-18T12:00:00+00:00"^^xsd:dateTime ;
	dct:created "2021-02-18T12:00:00+00:00"^^xsd:dateTime ;
	ikos:modified "2021-07-12T12:00:00+00:00"^^xsd:dateTime ;
	dct:modified "2021-07-12T12:00:00+00:00"^^xsd:dateTime  ;
	skos:exactMatch <https://www.wikidata.org/entity/Q1455871> ;
	skos:broader	medtop:20000817 .

medtop:20001318
	rdf:type skos:Concept ;
	skos:prefLabel	"pests"@en-GB ;
	skos:definition	"Animals or insects that invade a human space causing destruction or unsanitary conditions"@en-GB ;
	skos:inScheme <http://cv.iptc.org/newscodes/mediatopic/>  ;
	ikos:created "2021-02-18T12:00:00+00:00"^^xsd:dateTime ;
	dct:created "2021-02-18T12:00:00+00:00"^^xsd:dateTime ;
	ikos:modified "2022-06-14T12:00:00+00:00"^^xsd:dateTime ;
	dct:modified "2022-06-14T12:00:00+00:00"^^xsd:dateTime  ;
	skos:exactMatch <https://www.wikidata.org/entity/Q219174> ;
	skos:broader	medtop:20000500 .

medtop:20001319
	rdf:type skos:Concept ;
	skos:prefLabel	"disinformation and misinformation"@en-GB ;
	skos:definition	"The spread of false information regardless of intent"@en-GB ;
	skos:inScheme <http://cv.iptc.org/newscodes/mediatopic/>  ;
	ikos:created "2021-02-18T12:00:00+00:00"^^xsd:dateTime ;
	dct:created "2021-02-18T12:00:00+00:00"^^xsd:dateTime ;
	ikos:modified "2021-07-12T12:00:00+00:00"^^xsd:dateTime ;
	dct:modified "2021-07-12T12:00:00+00:00"^^xsd:dateTime  ;
	skos:exactMatch <https://www.wikidata.org/entity/Q13579947> ;
	skos:broader	medtop:20000045 .

medtop:20001320
	rdf:type skos:Concept ;
	skos:prefLabel	"torture"@en-GB ;
	skos:definition	"Intentionally inflicting severe physical or psychological pain in order to punish the victim or get the victim to take an action or give information"@en-GB ;
	skos:inScheme <http://cv.iptc.org/newscodes/mediatopic/>  ;
	ikos:created "2021-05-05T12:00:00+00:00"^^xsd:dateTime ;
	dct:created "2021-05-05T12:00:00+00:00"^^xsd:dateTime ;
	ikos:modified "2021-12-21T12:00:00+00:00"^^xsd:dateTime ;
	dct:modified "2021-12-21T12:00:00+00:00"^^xsd:dateTime  ;
	skos:exactMatch <https://www.wikidata.org/entity/Q132781> ;
	skos:broader	medtop:20000082 .

medtop:20001321
	rdf:type skos:Concept ;
	skos:prefLabel	"drowning"@en-GB ;
	skos:definition	"When a person's airpipe and lungs become filled with water causing death or injury, most often caused by falling into or bathing in rivers, lakes or the ocean"@en-GB ;
	skos:inScheme <http://cv.iptc.org/newscodes/mediatopic/>  ;
	ikos:created "2021-05-05T12:00:00+00:00"^^xsd:dateTime ;
	dct:created "2021-05-05T12:00:00+00:00"^^xsd:dateTime ;
	ikos:modified "2021-12-21T12:00:00+00:00"^^xsd:dateTime ;
	dct:modified "2021-12-21T12:00:00+00:00"^^xsd:dateTime  ;
	skos:exactMatch <https://www.wikidata.org/entity/Q506616> ;
	skos:broader	medtop:20000139 .

medtop:20001322
	rdf:type skos:Concept ;
	skos:prefLabel	"poisoning"@en-GB ;
	skos:definition	"When a substance in sufficient quantity adversely affects the body and its functions"@en-GB ;
	skos:inScheme <http://cv.iptc.org/newscodes/mediatopic/>  ;
	ikos:created "2021-05-05T12:00:00+00:00"^^xsd:dateTime ;
	dct:created "2021-05-05T12:00:00+00:00"^^xsd:dateTime ;
	ikos:modified "2021-12-21T12:00:00+00:00"^^xsd:dateTime ;
	dct:modified "2021-12-21T12:00:00+00:00"^^xsd:dateTime  ;
	skos:exactMatch <https://www.wikidata.org/entity/Q114953> ;
	skos:broader	medtop:20000446 .

medtop:20001323
	rdf:type skos:Concept ;
	skos:prefLabel	"sports coaching"@en-GB ;
	skos:definition	"The staff responsible for the training and on-field management of a sports team"@en-GB ;
	skos:inScheme <http://cv.iptc.org/newscodes/mediatopic/>  ;
	ikos:created "2021-05-05T12:00:00+00:00"^^xsd:dateTime ;
	dct:created "2021-05-05T12:00:00+00:00"^^xsd:dateTime ;
	ikos:modified "2021-12-21T12:00:00+00:00"^^xsd:dateTime ;
	dct:modified "2021-12-21T12:00:00+00:00"^^xsd:dateTime  ;
	skos:exactMatch <https://www.wikidata.org/entity/Q106195625> ;
	skos:broader	medtop:15000000 .

medtop:20001324
	rdf:type skos:Concept ;
	skos:prefLabel	"sports management and ownership"@en-GB ;
	skos:definition	"The executive leadership and owners of a sports team"@en-GB ;
	skos:inScheme <http://cv.iptc.org/newscodes/mediatopic/>  ;
	ikos:created "2021-05-05T12:00:00+00:00"^^xsd:dateTime ;
	dct:created "2021-05-05T12:00:00+00:00"^^xsd:dateTime ;
	ikos:modified "2021-12-21T12:00:00+00:00"^^xsd:dateTime ;
	dct:modified "2021-12-21T12:00:00+00:00"^^xsd:dateTime  ;
	skos:exactMatch <https://www.wikidata.org/entity/Q26481809> ;
	skos:broader	medtop:15000000 .

medtop:20001325
	rdf:type skos:Concept ;
	skos:prefLabel	"sports officiating"@en-GB ;
	skos:definition	"Referees, umpires and other staff who enforce the rules of a sport from on the field of play"@en-GB ;
	skos:inScheme <http://cv.iptc.org/newscodes/mediatopic/>  ;
	ikos:created "2021-05-05T12:00:00+00:00"^^xsd:dateTime ;
	dct:created "2021-05-05T12:00:00+00:00"^^xsd:dateTime ;
	ikos:modified "2021-12-21T12:00:00+00:00"^^xsd:dateTime ;
	dct:modified "2021-12-21T12:00:00+00:00"^^xsd:dateTime  ;
	skos:exactMatch <https://www.wikidata.org/entity/Q94271838> ;
	skos:broader	medtop:15000000 .

medtop:20001326
	rdf:type skos:Concept ;
	skos:prefLabel	"women's rights"@en-GB ;
	skos:definition	"Feminism, restrictions on the rights of women and the fight for equality with men"@en-GB ;
	skos:inScheme <http://cv.iptc.org/newscodes/mediatopic/>  ;
	ikos:created "2021-05-05T12:00:00+00:00"^^xsd:dateTime ;
	dct:created "2021-05-05T12:00:00+00:00"^^xsd:dateTime ;
	ikos:modified "2021-12-21T12:00:00+00:00"^^xsd:dateTime ;
	dct:modified "2021-12-21T12:00:00+00:00"^^xsd:dateTime  ;
	skos:exactMatch <https://www.wikidata.org/entity/Q223569> ;
	skos:broader	medtop:20000587 .

medtop:20001327
	rdf:type skos:Concept ;
	skos:prefLabel	"women"@en-GB ;
	skos:definition	"People who identify as female, focusing on the group as a demographic, and accomplishments, such as the first woman to achieve a milestone or serve in a role"@en-GB ;
	skos:inScheme <http://cv.iptc.org/newscodes/mediatopic/>  ;
	ikos:created "2021-05-05T12:00:00+00:00"^^xsd:dateTime ;
	dct:created "2021-05-05T12:00:00+00:00"^^xsd:dateTime ;
	ikos:modified "2021-12-21T12:00:00+00:00"^^xsd:dateTime ;
	dct:modified "2021-12-21T12:00:00+00:00"^^xsd:dateTime  ;
	skos:exactMatch <https://www.wikidata.org/entity/Q467> ;
	skos:broader	medtop:20000788 .

medtop:20001328
	rdf:type skos:Concept ;
	skos:prefLabel	"men"@en-GB ;
	skos:definition	"People who identify as male, focusing on the group as a demographic, and masculinity"@en-GB ;
	skos:inScheme <http://cv.iptc.org/newscodes/mediatopic/>  ;
	ikos:created "2021-05-05T12:00:00+00:00"^^xsd:dateTime ;
	dct:created "2021-05-05T12:00:00+00:00"^^xsd:dateTime ;
	ikos:modified "2021-12-21T12:00:00+00:00"^^xsd:dateTime ;
	dct:modified "2021-12-21T12:00:00+00:00"^^xsd:dateTime  ;
	skos:exactMatch <https://www.wikidata.org/entity/Q8441> ;
	skos:broader	medtop:20000788 .

medtop:20001329
	rdf:type skos:Concept ;
	skos:prefLabel	"3x3 basketball"@en-GB ;
	skos:definition	"A variation of basketball played three a side on one basketball hoop"@en-GB ;
	skos:inScheme <http://cv.iptc.org/newscodes/mediatopic/>  ;
	ikos:created "2021-07-12T12:00:00+00:00"^^xsd:dateTime ;
	dct:created "2021-07-12T12:00:00+00:00"^^xsd:dateTime ;
	ikos:modified "2021-12-21T12:00:00+00:00"^^xsd:dateTime ;
	dct:modified "2021-12-21T12:00:00+00:00"^^xsd:dateTime  ;
	skos:exactMatch <https://www.wikidata.org/entity/Q210550> ;
	skos:broader	medtop:20000822 .

medtop:20001330
	rdf:type skos:Concept ;
	skos:prefLabel	"canoe slalom"@en-GB ;
	skos:definition	"Competitors navigate a canoe or a kayak on a white-water course, passing through a combination of upstream and downstream gates on river rapids in the fastest time possible"@en-GB ;
	skos:inScheme <http://cv.iptc.org/newscodes/mediatopic/>  ;
	ikos:created "2021-07-12T12:00:00+00:00"^^xsd:dateTime ;
	dct:created "2021-07-12T12:00:00+00:00"^^xsd:dateTime ;
	ikos:modified "2021-12-21T12:00:00+00:00"^^xsd:dateTime ;
	dct:modified "2021-12-21T12:00:00+00:00"^^xsd:dateTime  ;
	skos:exactMatch <https://www.wikidata.org/entity/Q31874> ;
	skos:broader	medtop:20000822 .

medtop:20001331
	rdf:type skos:Concept ;
	skos:prefLabel	"canoe sprint"@en-GB ;
	skos:definition	"Taking place on a flatwater course, multiple canoes take off at once and race each other to the finish"@en-GB ;
	skos:inScheme <http://cv.iptc.org/newscodes/mediatopic/>  ;
	ikos:created "2021-07-12T12:00:00+00:00"^^xsd:dateTime ;
	dct:created "2021-07-12T12:00:00+00:00"^^xsd:dateTime ;
	ikos:modified "2021-12-21T12:00:00+00:00"^^xsd:dateTime ;
	dct:modified "2021-12-21T12:00:00+00:00"^^xsd:dateTime  ;
	skos:exactMatch <https://www.wikidata.org/entity/Q1141850> ;
	skos:broader	medtop:20000822 .

medtop:20001332
	rdf:type skos:Concept ;
	skos:prefLabel	"bmx freesytle"@en-GB ;
	skos:definition	"Riders are given a fixed time to perform acrobatics tricks and skills, with tricks scored on multiple aspects including difficulty, originality, execution, height and creativity"@en-GB ;
	skos:inScheme <http://cv.iptc.org/newscodes/mediatopic/>  ;
	ikos:created "2021-07-12T12:00:00+00:00"^^xsd:dateTime ;
	dct:created "2021-07-12T12:00:00+00:00"^^xsd:dateTime ;
	ikos:modified "2021-12-21T12:00:00+00:00"^^xsd:dateTime ;
	dct:modified "2021-12-21T12:00:00+00:00"^^xsd:dateTime  ;
	skos:exactMatch <https://www.wikidata.org/entity/Q2192643> ;
	skos:broader	medtop:20000822 .

medtop:20001333
	rdf:type skos:Concept ;
	skos:prefLabel	"road cycling"@en-GB ;
	skos:definition	"Cycling events held on roads, including road races and time trials"@en-GB ;
	skos:inScheme <http://cv.iptc.org/newscodes/mediatopic/>  ;
	ikos:created "2021-07-12T12:00:00+00:00"^^xsd:dateTime ;
	dct:created "2021-07-12T12:00:00+00:00"^^xsd:dateTime ;
	ikos:modified "2021-12-21T12:00:00+00:00"^^xsd:dateTime ;
	dct:modified "2021-12-21T12:00:00+00:00"^^xsd:dateTime  ;
	skos:exactMatch <https://www.wikidata.org/entity/Q3609> ;
	skos:broader	medtop:20000822 .

medtop:20001334
	rdf:type skos:Concept ;
	skos:prefLabel	"track cycling"@en-GB ;
	skos:definition	"Cycling competitions held on tracks, including sprint, team sprint, keirin, team pursuit, omnium and madison events"@en-GB ;
	skos:inScheme <http://cv.iptc.org/newscodes/mediatopic/>  ;
	ikos:created "2021-07-12T12:00:00+00:00"^^xsd:dateTime ;
	dct:created "2021-07-12T12:00:00+00:00"^^xsd:dateTime ;
	ikos:modified "2021-12-21T12:00:00+00:00"^^xsd:dateTime ;
	dct:modified "2021-12-21T12:00:00+00:00"^^xsd:dateTime  ;
	skos:exactMatch <https://www.wikidata.org/entity/Q221635> ;
	skos:broader	medtop:20000822 .

medtop:20001335
	rdf:type skos:Concept ;
	skos:prefLabel	"football 5-a-side"@en-GB ;
	skos:definition	"A variation of association football in which each team fields five players and play is on a smaller pitch. An official Summer Paralympics sport."@en-GB ;
	skos:inScheme <http://cv.iptc.org/newscodes/mediatopic/>  ;
	ikos:created "2021-07-12T12:00:00+00:00"^^xsd:dateTime ;
	dct:created "2021-07-12T12:00:00+00:00"^^xsd:dateTime ;
	ikos:modified "2021-12-21T12:00:00+00:00"^^xsd:dateTime ;
	dct:modified "2021-12-21T12:00:00+00:00"^^xsd:dateTime  ;
	skos:exactMatch <https://www.wikidata.org/entity/Q5465786> ;
	skos:broader	medtop:20000822 .

medtop:20001336
	rdf:type skos:Concept ;
	skos:prefLabel	"goalball"@en-GB ;
	skos:definition	"A team sport for athletes with a vision impairment, using a ball containing bells"@en-GB ;
	skos:inScheme <http://cv.iptc.org/newscodes/mediatopic/>  ;
	ikos:created "2021-07-12T12:00:00+00:00"^^xsd:dateTime ;
	dct:created "2021-07-12T12:00:00+00:00"^^xsd:dateTime ;
	ikos:modified "2021-12-21T12:00:00+00:00"^^xsd:dateTime ;
	dct:modified "2021-12-21T12:00:00+00:00"^^xsd:dateTime  ;
	skos:exactMatch <https://www.wikidata.org/entity/Q647559> ;
	skos:broader	medtop:20000822 .

medtop:20001337
	rdf:type skos:Concept ;
	skos:prefLabel	"online and remote learning"@en-GB ;
	skos:definition	"Learning where a student and teacher are not physically present in the same location. Instruction can occur synchronously or asynchronously and utilizes technology such as video conferencing, online assessments and video conferencing."@en-GB ;
	skos:inScheme <http://cv.iptc.org/newscodes/mediatopic/>  ;
	ikos:created "2021-09-30T12:00:00+00:00"^^xsd:dateTime ;
	dct:created "2021-09-30T12:00:00+00:00"^^xsd:dateTime ;
	ikos:modified "2021-12-21T12:00:00+00:00"^^xsd:dateTime ;
	dct:modified "2021-12-21T12:00:00+00:00"^^xsd:dateTime  ;
	skos:exactMatch <https://www.wikidata.org/entity/Q182250> ;
	skos:broader	medtop:05000000 .

medtop:20001338
	rdf:type skos:Concept ;
	skos:prefLabel	"education policy"@en-GB ;
	skos:definition	"Government programmes and policies related to education and proposals to change or protests against those positions"@en-GB ;
	skos:changeNote	"Moved from medtop:05000000 to medtop:20000621"@en-GB ;
	skos:inScheme <http://cv.iptc.org/newscodes/mediatopic/>  ;
	ikos:created "2021-12-17T12:00:00+00:00"^^xsd:dateTime ;
	dct:created "2021-12-17T12:00:00+00:00"^^xsd:dateTime ;
	ikos:modified "2022-09-23T12:00:00+00:00"^^xsd:dateTime ;
	dct:modified "2022-09-23T12:00:00+00:00"^^xsd:dateTime  ;
	skos:exactMatch <https://www.wikidata.org/entity/Q452348> ;
	skos:broader	medtop:20000621 .

medtop:20001339
	rdf:type skos:Concept ;
	skos:prefLabel	"wellness"@en-GB ;
	skos:definition	"The active pursuit of good mental and physical health"@en-GB ;
	skos:inScheme <http://cv.iptc.org/newscodes/mediatopic/>  ;
	ikos:created "2021-12-17T12:00:00+00:00"^^xsd:dateTime ;
	dct:created "2021-12-17T12:00:00+00:00"^^xsd:dateTime ;
	ikos:modified "2021-12-21T12:00:00+00:00"^^xsd:dateTime ;
	dct:modified "2021-12-21T12:00:00+00:00"^^xsd:dateTime  ;
	skos:exactMatch <https://www.wikidata.org/entity/Q1077209> ;
	skos:broader	medtop:10000000 ;
	skos:narrower	medtop:20001239 ;
	skos:narrower	medtop:20001340 .

medtop:20001340
	rdf:type skos:Concept ;
	skos:prefLabel	"mental wellbeing"@en-GB ;
	skos:definition	"The personal pursuit of mental health through activities such as meditation, stress reduction, technology detoxes and journalling"@en-GB ;
	skos:inScheme <http://cv.iptc.org/newscodes/mediatopic/>  ;
	ikos:created "2021-12-17T12:00:00+00:00"^^xsd:dateTime ;
	dct:created "2021-12-17T12:00:00+00:00"^^xsd:dateTime ;
	ikos:modified "2021-12-21T12:00:00+00:00"^^xsd:dateTime ;
	dct:modified "2021-12-21T12:00:00+00:00"^^xsd:dateTime  ;
	skos:exactMatch <https://www.wikidata.org/entity/Q317309> ;
	skos:broader	medtop:20001339 .

medtop:20001341
	rdf:type skos:Concept ;
	skos:prefLabel	"regular competition"@en-GB ;
	skos:definition	"A competitive sporting season where teams or individuals contend for a place in the standings or rankings"@en-GB ;
	skos:inScheme <http://cv.iptc.org/newscodes/mediatopic/>  ;
	ikos:created "2021-12-17T12:00:00+00:00"^^xsd:dateTime ;
	dct:created "2021-12-17T12:00:00+00:00"^^xsd:dateTime ;
	ikos:modified "2021-12-21T12:00:00+00:00"^^xsd:dateTime ;
	dct:modified "2021-12-21T12:00:00+00:00"^^xsd:dateTime  ;
	skos:exactMatch <https://www.wikidata.org/entity/Q27020041> ;
	skos:broader	medtop:20001108 .

medtop:20001342
	rdf:type skos:Concept ;
	skos:prefLabel	"playoff championship"@en-GB ;
	skos:definition	"A competitive tournament, often played after the regular season of a sports league by the top competitors to determine the league champion or a similar accolade. Can also apply to an all-in elimination tournament meant to produce a final champion."@en-GB ;
	skos:inScheme <http://cv.iptc.org/newscodes/mediatopic/>  ;
	ikos:created "2021-12-17T12:00:00+00:00"^^xsd:dateTime ;
	dct:created "2021-12-17T12:00:00+00:00"^^xsd:dateTime ;
	ikos:modified "2021-12-21T12:00:00+00:00"^^xsd:dateTime ;
	dct:modified "2021-12-21T12:00:00+00:00"^^xsd:dateTime  ;
	skos:exactMatch <https://www.wikidata.org/entity/Q1079023> ;
	skos:broader	medtop:20001108 .

medtop:20001343
	rdf:type skos:Concept ;
	skos:prefLabel	"final game"@en-GB ;
	skos:definition	"Single game that determines the winner of a championship, such as the Super Bowl or Champions League Final"@en-GB ;
	skos:inScheme <http://cv.iptc.org/newscodes/mediatopic/>  ;
	ikos:created "2021-12-17T12:00:00+00:00"^^xsd:dateTime ;
	dct:created "2021-12-17T12:00:00+00:00"^^xsd:dateTime ;
	ikos:modified "2021-12-21T12:00:00+00:00"^^xsd:dateTime ;
	dct:modified "2021-12-21T12:00:00+00:00"^^xsd:dateTime  ;
	skos:exactMatch <https://www.wikidata.org/entity/Q1366722> ;
	skos:broader	medtop:20001108 .

medtop:20001344
	rdf:type skos:Concept ;
	skos:prefLabel	"Catholicism"@en-GB ;
	skos:definition	"Largest Christian religion in the world encompassing the Roman Catholic Church which is led by the pope, and Old Catholicism, a breakaway movement founded in 1870 that denies the dogma of infallibility of the pope"@en-GB ;
	skos:inScheme <http://cv.iptc.org/newscodes/mediatopic/>  ;
	ikos:created "2021-12-17T12:00:00+00:00"^^xsd:dateTime ;
	dct:created "2021-12-17T12:00:00+00:00"^^xsd:dateTime ;
	ikos:modified "2021-12-21T12:00:00+00:00"^^xsd:dateTime ;
	dct:modified "2021-12-21T12:00:00+00:00"^^xsd:dateTime  ;
	skos:exactMatch <https://www.wikidata.org/entity/Q1841> ;
	skos:broader	medtop:20000659 .

medtop:20001345
	rdf:type skos:Concept ;
	skos:prefLabel	"bar and bat mitzvah"@en-GB ;
	skos:definition	"Young person becoming an adult in the Jewish faith"@en-GB ;
	skos:inScheme <http://cv.iptc.org/newscodes/mediatopic/>  ;
	ikos:created "2021-12-17T12:00:00+00:00"^^xsd:dateTime ;
	dct:created "2021-12-17T12:00:00+00:00"^^xsd:dateTime ;
	ikos:modified "2021-12-21T12:00:00+00:00"^^xsd:dateTime ;
	dct:modified "2021-12-21T12:00:00+00:00"^^xsd:dateTime  ;
	skos:exactMatch <https://www.wikidata.org/entity/Q75673> ;
	skos:broader	medtop:20000696 .

medtop:20001346
	rdf:type skos:Concept ;
	skos:prefLabel	"canonisation"@en-GB ;
	skos:definition	"The declaration of a deceased person as an officially recognised saint"@en-GB ;
	skos:inScheme <http://cv.iptc.org/newscodes/mediatopic/>  ;
	ikos:created "2021-12-17T12:00:00+00:00"^^xsd:dateTime ;
	dct:created "2021-12-17T12:00:00+00:00"^^xsd:dateTime ;
	ikos:modified "2021-12-21T12:00:00+00:00"^^xsd:dateTime ;
	dct:modified "2021-12-21T12:00:00+00:00"^^xsd:dateTime  ;
	skos:exactMatch <https://www.wikidata.org/entity/Q51621> ;
	skos:broader	medtop:20000696 .

medtop:20001347
	rdf:type skos:Concept ;
	skos:prefLabel	"Shia Islam"@en-GB ;
	skos:definition	"The second largest branch of Islam believing that the Prophet Muhammad designated Ali ibn Abi Talib as his successor"@en-GB ;
	skos:inScheme <http://cv.iptc.org/newscodes/mediatopic/>  ;
	ikos:created "2021-12-17T12:00:00+00:00"^^xsd:dateTime ;
	dct:created "2021-12-17T12:00:00+00:00"^^xsd:dateTime ;
	ikos:modified "2021-12-21T12:00:00+00:00"^^xsd:dateTime ;
	dct:modified "2021-12-21T12:00:00+00:00"^^xsd:dateTime  ;
	skos:exactMatch <https://www.wikidata.org/entity/Q9585> ;
	skos:broader	medtop:20000677 .

medtop:20001348
	rdf:type skos:Concept ;
	skos:prefLabel	"Sunni Islam"@en-GB ;
	skos:definition	"The largest branch of Islam believing that the Prophet Muhammad did not designate a successor"@en-GB ;
	skos:inScheme <http://cv.iptc.org/newscodes/mediatopic/>  ;
	ikos:created "2021-12-17T12:00:00+00:00"^^xsd:dateTime ;
	dct:created "2021-12-17T12:00:00+00:00"^^xsd:dateTime ;
	ikos:modified "2021-12-21T12:00:00+00:00"^^xsd:dateTime ;
	dct:modified "2021-12-21T12:00:00+00:00"^^xsd:dateTime  ;
	skos:exactMatch <https://www.wikidata.org/entity/Q483654> ;
	skos:broader	medtop:20000677 .

medtop:20001349
	rdf:type skos:Concept ;
	skos:prefLabel	"atheism and agnosticism"@en-GB ;
	skos:definition	"The belief that god does not exist or that it is impossible to know whether a god exists"@en-GB ;
	skos:inScheme <http://cv.iptc.org/newscodes/mediatopic/>  ;
	ikos:created "2021-12-17T12:00:00+00:00"^^xsd:dateTime ;
	dct:created "2021-12-17T12:00:00+00:00"^^xsd:dateTime ;
	ikos:modified "2021-12-21T12:00:00+00:00"^^xsd:dateTime ;
	dct:modified "2021-12-21T12:00:00+00:00"^^xsd:dateTime  ;
	skos:exactMatch <https://www.wikidata.org/entity/Q7066> ;
	skos:broader	medtop:20000657 .

medtop:20001350
	rdf:type skos:Concept ;
	skos:prefLabel	"Eid al-Adha"@en-GB ;
	skos:definition	"Muslim festival marking the culmination of the annual hajj pilgrimage and commemorating the willingness of the Prophet Ibrahim to sacrifice his son"@en-GB ;
	skos:inScheme <http://cv.iptc.org/newscodes/mediatopic/>  ;
	ikos:created "2021-12-17T12:00:00+00:00"^^xsd:dateTime ;
	dct:created "2021-12-17T12:00:00+00:00"^^xsd:dateTime ;
	ikos:modified "2021-12-21T12:00:00+00:00"^^xsd:dateTime ;
	dct:modified "2021-12-21T12:00:00+00:00"^^xsd:dateTime  ;
	skos:exactMatch <https://www.wikidata.org/entity/Q514400> ;
	skos:broader	medtop:20000690 .

medtop:20001351
	rdf:type skos:Concept ;
	skos:prefLabel	"Hasidism"@en-GB ;
	skos:definition	"Jewish religious group that believes that the Torah is the literal word of God and that carrying out this word is what gives meaning and purpose to life"@en-GB ;
	skos:inScheme <http://cv.iptc.org/newscodes/mediatopic/>  ;
	ikos:created "2021-12-17T12:00:00+00:00"^^xsd:dateTime ;
	dct:created "2021-12-17T12:00:00+00:00"^^xsd:dateTime ;
	ikos:modified "2021-12-21T12:00:00+00:00"^^xsd:dateTime ;
	dct:modified "2021-12-21T12:00:00+00:00"^^xsd:dateTime  ;
	skos:exactMatch <https://www.wikidata.org/entity/Q171201> ;
	skos:broader	medtop:20000679 .

medtop:20001352
	rdf:type skos:Concept ;
	skos:prefLabel	"Hanukkah"@en-GB ;
	skos:definition	"Jewish festival, sometimes spelled Chanukah, observed by lighting the candles of a menorah"@en-GB ;
	skos:inScheme <http://cv.iptc.org/newscodes/mediatopic/>  ;
	ikos:created "2021-12-17T12:00:00+00:00"^^xsd:dateTime ;
	dct:created "2021-12-17T12:00:00+00:00"^^xsd:dateTime ;
	ikos:modified "2021-12-21T12:00:00+00:00"^^xsd:dateTime ;
	dct:modified "2021-12-21T12:00:00+00:00"^^xsd:dateTime  ;
	skos:exactMatch <https://www.wikidata.org/entity/Q130881> ;
	skos:broader	medtop:20000690 .

medtop:20001353
	rdf:type skos:Concept ;
	skos:prefLabel	"tsunami"@en-GB ;
	skos:definition	"High and powerful ocean waves caused by an underwater land disturbance, such as an earthquake or volcanic eruption, known to cause significant damage and loss when they hit land"@en-GB ;
	skos:inScheme <http://cv.iptc.org/newscodes/mediatopic/>  ;
	ikos:created "2022-02-03T12:00:00+00:00"^^xsd:dateTime ;
	dct:created "2022-02-03T12:00:00+00:00"^^xsd:dateTime ;
	ikos:modified "2022-02-03T12:00:00+00:00"^^xsd:dateTime ;
	dct:modified "2022-02-03T12:00:00+00:00"^^xsd:dateTime  ;
	skos:exactMatch <https://www.wikidata.org/entity/Q8070> ;
	skos:broader	medtop:20000151 .

medtop:20001354
	rdf:type skos:Concept ;
	skos:prefLabel	"healthcare industry"@en-GB ;
	skos:definition	"Goods and services to treat patients through curative, preventive, rehabilitative and palliative care"@en-GB ;
	skos:inScheme <http://cv.iptc.org/newscodes/mediatopic/>  ;
	ikos:created "2022-06-14T12:00:00+00:00"^^xsd:dateTime ;
	dct:created "2022-06-14T12:00:00+00:00"^^xsd:dateTime ;
	ikos:modified "2022-06-14T12:00:00+00:00"^^xsd:dateTime ;
	dct:modified "2022-06-14T12:00:00+00:00"^^xsd:dateTime  ;
	skos:exactMatch <https://www.wikidata.org/entity/Q15067276> ;
	skos:broader	medtop:20000209 ;
	skos:narrower	medtop:20000218 ;
	skos:narrower	medtop:20000223 ;
	skos:narrower	medtop:20000278 ;
	skos:narrower	medtop:20001167 .

medtop:20001355
	rdf:type skos:Concept ;
	skos:prefLabel	"developmental disorder"@en-GB ;
	skos:definition	"Conditions due to an impairment in learning, language or behavior areas, such as autism, aspergers and dyslexia"@en-GB ;
	skos:inScheme <http://cv.iptc.org/newscodes/mediatopic/>  ;
	ikos:created "2022-06-14T12:00:00+00:00"^^xsd:dateTime ;
	dct:created "2022-06-14T12:00:00+00:00"^^xsd:dateTime ;
	ikos:modified "2022-06-14T12:00:00+00:00"^^xsd:dateTime ;
	dct:modified "2022-06-14T12:00:00+00:00"^^xsd:dateTime  ;
	skos:exactMatch <https://www.wikidata.org/entity/Q15067276> ;
	skos:broader	medtop:20000446 .

medtop:20001356
	rdf:type skos:Concept ;
	skos:prefLabel	"depression"@en-GB ;
	skos:definition	"A mental health disorder characterised by persistently depressed mood and loss of interest in activities, causing significant impairment in daily life"@en-GB ;
	skos:inScheme <http://cv.iptc.org/newscodes/mediatopic/>  ;
	ikos:created "2022-06-14T12:00:00+00:00"^^xsd:dateTime ;
	dct:created "2022-06-14T12:00:00+00:00"^^xsd:dateTime ;
	ikos:modified "2022-06-14T12:00:00+00:00"^^xsd:dateTime ;
	dct:modified "2022-06-14T12:00:00+00:00"^^xsd:dateTime  ;
	skos:exactMatch <https://www.wikidata.org/entity/Q4340209> ;
	skos:broader	medtop:20000458 .

medtop:20001357
	rdf:type skos:Concept ;
	skos:prefLabel	"anxiety and stress"@en-GB ;
	skos:definition	"A mental health disorder characterised by feelings of worry, anxiousness or fear that are strong enough to interfere with one's daily activities"@en-GB ;
	skos:inScheme <http://cv.iptc.org/newscodes/mediatopic/>  ;
	ikos:created "2022-06-14T12:00:00+00:00"^^xsd:dateTime ;
	dct:created "2022-06-14T12:00:00+00:00"^^xsd:dateTime ;
	ikos:modified "2022-06-14T12:00:00+00:00"^^xsd:dateTime ;
	dct:modified "2022-06-14T12:00:00+00:00"^^xsd:dateTime  ;
	skos:exactMatch <https://www.wikidata.org/entity/Q544006> ;
	skos:broader	medtop:20000458 .

medtop:20001358
	rdf:type skos:Concept ;
	skos:prefLabel	"public health"@en-GB ;
	skos:definition	"Organised public or private measures designed to prevent disease, promote health and prolong life among the population as a whole"@en-GB ;
	skos:inScheme <http://cv.iptc.org/newscodes/mediatopic/>  ;
	ikos:created "2022-06-14T12:00:00+00:00"^^xsd:dateTime ;
	dct:created "2022-06-14T12:00:00+00:00"^^xsd:dateTime ;
	ikos:modified "2022-06-14T12:00:00+00:00"^^xsd:dateTime ;
	dct:modified "2022-06-14T12:00:00+00:00"^^xsd:dateTime  ;
	skos:exactMatch <https://www.wikidata.org/entity/Q189603> ;
	skos:broader	medtop:07000000 .

medtop:20001359
	rdf:type skos:Concept ;
	skos:prefLabel	"pregnancy and childbirth"@en-GB ;
	skos:definition	"Social and medical issues around pregnancy and giving birth including, doulas and midwives, obstetrics and medical concerns"@en-GB ;
	skos:inScheme <http://cv.iptc.org/newscodes/mediatopic/>  ;
	ikos:created "2022-06-14T12:00:00+00:00"^^xsd:dateTime ;
	dct:created "2022-06-14T12:00:00+00:00"^^xsd:dateTime ;
	ikos:modified "2022-06-14T12:00:00+00:00"^^xsd:dateTime ;
	dct:modified "2022-06-14T12:00:00+00:00"^^xsd:dateTime  ;
	skos:exactMatch <https://www.wikidata.org/entity/Q11995> ;
	skos:broader	medtop:20000780 .

medtop:20001360
	rdf:type skos:Concept ;
	skos:prefLabel	"fraternal and community group"@en-GB ;
	skos:definition	"Social organisations whose members freely associate for a mutually beneficial purpose such as for social, professional or honorary principles. Groups include Rotary clubs, Lions clubs or Freemasons."@en-GB ;
	skos:inScheme <http://cv.iptc.org/newscodes/mediatopic/>  ;
	ikos:created "2022-09-23T12:00:00+00:00"^^xsd:dateTime ;
	dct:created "2022-09-23T12:00:00+00:00"^^xsd:dateTime ;
	ikos:modified "2022-09-23T12:00:00+00:00"^^xsd:dateTime ;
	dct:modified "2022-09-23T12:00:00+00:00"^^xsd:dateTime  ;
	skos:exactMatch <https://www.wikidata.org/entity/Q996839> ;
	skos:broader	medtop:20000768 .

medtop:20001361
	rdf:type skos:Concept ;
	skos:prefLabel	"cyber warfare"@en-GB ;
	skos:definition	"Cyber attacks, or suspected attacks, involving a government entity as either the sponsor or the target, or preventive measures against these types of actions"@en-GB ;
	skos:inScheme <http://cv.iptc.org/newscodes/mediatopic/>  ;
	ikos:created "2022-09-23T12:00:00+00:00"^^xsd:dateTime ;
	dct:created "2022-09-23T12:00:00+00:00"^^xsd:dateTime ;
	ikos:modified "2022-09-23T12:00:00+00:00"^^xsd:dateTime ;
	dct:modified "2022-09-23T12:00:00+00:00"^^xsd:dateTime  ;
	skos:exactMatch <https://www.wikidata.org/entity/Q849340> ;
	skos:broader	medtop:16000000 .

medtop:20001362
	rdf:type skos:Concept ;
	skos:prefLabel	"public transport"@en-GB ;
	skos:definition	"Forms of transportation, such as buses and trains, that charge set fares, run on fixed routes and are available to the general public"@en-GB ;
	skos:inScheme <http://cv.iptc.org/newscodes/mediatopic/>  ;
	ikos:created "2022-09-23T12:00:00+00:00"^^xsd:dateTime ;
	dct:created "2022-09-23T12:00:00+00:00"^^xsd:dateTime ;
	ikos:modified "2022-09-23T12:00:00+00:00"^^xsd:dateTime ;
	dct:modified "2022-09-23T12:00:00+00:00"^^xsd:dateTime  ;
	skos:exactMatch <https://www.wikidata.org/entity/Q178512> ;
	skos:broader	medtop:20000337 .

medtop:20001363
	rdf:type skos:Concept ;
	skos:prefLabel	"taxi and ride-hailing"@en-GB ;
	skos:definition	"On-demand ride service, provided by taxi companies or tech companies such as Uber and Lyft, the drivers who transport passengers and the rules and regulations imposed upon these companies within a region"@en-GB ;
	skos:inScheme <http://cv.iptc.org/newscodes/mediatopic/>  ;
	ikos:created "2022-09-23T12:00:00+00:00"^^xsd:dateTime ;
	dct:created "2022-09-23T12:00:00+00:00"^^xsd:dateTime ;
	ikos:modified "2022-09-23T12:00:00+00:00"^^xsd:dateTime ;
	dct:modified "2022-09-23T12:00:00+00:00"^^xsd:dateTime  ;
	skos:exactMatch <https://www.wikidata.org/entity/Q82650> ;
	skos:broader	medtop:20000337 .

medtop:20001364
	rdf:type skos:Concept ;
	skos:prefLabel	"shared transport"@en-GB ;
	skos:definition	"A network of vehicles, such as cars, bikes and scooters, that can be rented by travellers on an as-needed basis for short-term use"@en-GB ;
	skos:inScheme <http://cv.iptc.org/newscodes/mediatopic/>  ;
	ikos:created "2022-09-23T12:00:00+00:00"^^xsd:dateTime ;
	dct:created "2022-09-23T12:00:00+00:00"^^xsd:dateTime ;
	ikos:modified "2022-09-23T12:00:00+00:00"^^xsd:dateTime ;
	dct:modified "2022-09-23T12:00:00+00:00"^^xsd:dateTime  ;
	skos:exactMatch <https://www.wikidata.org/entity/Q7489559> ;
	skos:broader	medtop:20000337 .

medtop:20001365
	rdf:type skos:Concept ;
	skos:prefLabel	"business reporting and performance"@en-GB ;
	skos:definition	"Measuring and reporting on the performance of a business"@en-GB ;
	skos:inScheme <http://cv.iptc.org/newscodes/mediatopic/>  ;
	ikos:created "2023-03-31T12:00:00+00:00"^^xsd:dateTime ;
	dct:created "2023-03-31T12:00:00+00:00"^^xsd:dateTime ;
	ikos:modified "2023-03-31T12:00:00+00:00"^^xsd:dateTime ;
	dct:modified "2023-03-31T12:00:00+00:00"^^xsd:dateTime  ;
	skos:exactMatch <https://www.wikidata.org/entity/Q5001933> ;
	skos:broader	medtop:20000170 ;
	skos:narrower	medtop:20000172 ;
	skos:narrower	medtop:20000176 ;
	skos:narrower	medtop:20000178 ;
	skos:narrower	medtop:20000179 ;
	skos:narrower	medtop:20000180 .

medtop:20001366
	rdf:type skos:Concept ;
	skos:prefLabel	"business restructuring"@en-GB ;
	skos:definition	"Changes to the structure of a business or organisation"@en-GB ;
	skos:inScheme <http://cv.iptc.org/newscodes/mediatopic/>  ;
	ikos:created "2023-03-31T12:00:00+00:00"^^xsd:dateTime ;
	dct:created "2023-03-31T12:00:00+00:00"^^xsd:dateTime ;
	ikos:modified "2023-03-31T12:00:00+00:00"^^xsd:dateTime ;
	dct:modified "2023-03-31T12:00:00+00:00"^^xsd:dateTime  ;
	skos:exactMatch <https://www.wikidata.org/entity/Q1376796> ;
	skos:broader	medtop:20000170 ;
	skos:narrower	medtop:20000197 ;
	skos:narrower	medtop:20000200 ;
	skos:narrower	medtop:20000201 ;
	skos:narrower	medtop:20000203 ;
	skos:narrower	medtop:20000204 .

medtop:20001367
	rdf:type skos:Concept ;
	skos:prefLabel	"commercial real estate"@en-GB ;
	skos:definition	"The building and sale of property used for business purposes rather than as a living space"@en-GB ;
	skos:inScheme <http://cv.iptc.org/newscodes/mediatopic/>  ;
	ikos:created "2023-03-31T12:00:00+00:00"^^xsd:dateTime ;
	dct:created "2023-03-31T12:00:00+00:00"^^xsd:dateTime ;
	ikos:modified "2023-03-31T12:00:00+00:00"^^xsd:dateTime ;
	dct:modified "2023-03-31T12:00:00+00:00"^^xsd:dateTime  ;
	skos:exactMatch <https://www.wikidata.org/entity/Q1520439> ;
	skos:broader	medtop:20000235 .

medtop:20001368
	rdf:type skos:Concept ;
	skos:prefLabel	"residential real estate"@en-GB ;
	skos:definition	"The building and sale of property to be used as living space"@en-GB ;
	skos:inScheme <http://cv.iptc.org/newscodes/mediatopic/>  ;
	ikos:created "2023-03-31T12:00:00+00:00"^^xsd:dateTime ;
	dct:created "2023-03-31T12:00:00+00:00"^^xsd:dateTime ;
	ikos:modified "2023-03-31T12:00:00+00:00"^^xsd:dateTime ;
	dct:modified "2023-03-31T12:00:00+00:00"^^xsd:dateTime  ;
	skos:exactMatch <https://www.wikidata.org/entity/Q1403389> ;
	skos:broader	medtop:20000235 .

medtop:20001369
	rdf:type skos:Concept ;
	skos:prefLabel	"podcast"@en-GB ;
	skos:definition	"Podcast networks and the people who create and distribute audio content, typically in a series format, to audiences"@en-GB ;
	skos:inScheme <http://cv.iptc.org/newscodes/mediatopic/>  ;
	ikos:created "2023-03-31T12:00:00+00:00"^^xsd:dateTime ;
	dct:created "2023-03-31T12:00:00+00:00"^^xsd:dateTime ;
	ikos:modified "2023-03-31T12:00:00+00:00"^^xsd:dateTime ;
	dct:modified "2023-03-31T12:00:00+00:00"^^xsd:dateTime  ;
	skos:exactMatch <https://www.wikidata.org/entity/Q20899> ;
	skos:broader	medtop:20000304 .

medtop:20001370
	rdf:type skos:Concept ;
	skos:prefLabel	"financial service"@en-GB ;
	skos:definition	"Professional services involving the investment, lending or management of money and other assets"@en-GB ;
	skos:inScheme <http://cv.iptc.org/newscodes/mediatopic/>  ;
	ikos:created "2023-03-31T12:00:00+00:00"^^xsd:dateTime ;
	dct:created "2023-03-31T12:00:00+00:00"^^xsd:dateTime ;
	ikos:modified "2023-03-31T12:00:00+00:00"^^xsd:dateTime ;
	dct:modified "2023-03-31T12:00:00+00:00"^^xsd:dateTime  ;
	skos:exactMatch <https://www.wikidata.org/entity/Q837171> ;
	skos:broader	medtop:20000209 ;
	skos:narrower	medtop:20000272 ;
	skos:narrower	medtop:20000274 ;
	skos:narrower	medtop:20000279 ;
	skos:narrower	medtop:20000280 ;
	skos:narrower	medtop:20000287 ;
	skos:narrower	medtop:20000292 ;
	skos:narrower	medtop:20001162 .

medtop:20001371
	rdf:type skos:Concept ;
	skos:prefLabel	"business service"@en-GB ;
	skos:definition	"Services provided to business operations and for individuals, such as consulting, legal representation and job placement"@en-GB ;
	skos:inScheme <http://cv.iptc.org/newscodes/mediatopic/>  ;
	ikos:created "2023-03-31T12:00:00+00:00"^^xsd:dateTime ;
	dct:created "2023-03-31T12:00:00+00:00"^^xsd:dateTime ;
	ikos:modified "2023-03-31T12:00:00+00:00"^^xsd:dateTime ;
	dct:modified "2023-03-31T12:00:00+00:00"^^xsd:dateTime  ;
	skos:exactMatch <https://www.wikidata.org/entity/Q25351891> ;
	skos:broader	medtop:20000209 ;
	skos:narrower	medtop:20000275 ;
	skos:narrower	medtop:20000276 ;
	skos:narrower	medtop:20000281 ;
	skos:narrower	medtop:20000282 ;
	skos:narrower	medtop:20000288 ;
	skos:narrower	medtop:20000290 ;
	skos:narrower	medtop:20000291 ;
	skos:narrower	medtop:20000293 ;
	skos:narrower	medtop:20001136 ;
	skos:narrower	medtop:20001164 .

medtop:20001372
	rdf:type skos:Concept ;
	skos:prefLabel	"news industry"@en-GB ;
	skos:definition	"The production and distribution of content about newsworthy events through print, broadcast, video or electronic media"@en-GB ;
	skos:inScheme <http://cv.iptc.org/newscodes/mediatopic/>  ;
	ikos:created "2023-03-31T12:00:00+00:00"^^xsd:dateTime ;
	dct:created "2023-03-31T12:00:00+00:00"^^xsd:dateTime ;
	ikos:modified "2023-03-31T12:00:00+00:00"^^xsd:dateTime ;
	dct:modified "2023-03-31T12:00:00+00:00"^^xsd:dateTime  ;
	skos:exactMatch <https://www.wikidata.org/entity/Q1193236> ;
	skos:broader	medtop:20000304 .

medtop:20001373
	rdf:type skos:Concept ;
	skos:prefLabel	"diversity, equity and inclusion"@en-GB ;
	skos:definition	"Efforts that seeks to promote the fair treatment and full participation of groups of people who have historically been underrepresented or subject to discrimination on the basis of identity or disability"@en-GB ;
	skos:inScheme <http://cv.iptc.org/newscodes/mediatopic/>  ;
	ikos:created "2023-03-31T12:00:00+00:00"^^xsd:dateTime ;
	dct:created "2023-03-31T12:00:00+00:00"^^xsd:dateTime ;
	ikos:modified "2023-03-31T12:00:00+00:00"^^xsd:dateTime ;
	dct:modified "2023-03-31T12:00:00+00:00"^^xsd:dateTime  ;
	skos:exactMatch <https://www.wikidata.org/entity/Q109801645> ;
	skos:broader	medtop:14000000 .

medtop:20001374
	rdf:type skos:Concept ;
	skos:prefLabel	"sustainability"@en-GB ;
	skos:definition	"Actions by businesses, governments and individuals to counter major environmental problems, including climate change, loss of biodiversity, loss of ecosystem services, land degradation and air and water pollution"@en-GB ;
	skos:inScheme <http://cv.iptc.org/newscodes/mediatopic/>  ;
	ikos:created "2023-10-02T12:00:00+00:00"^^xsd:dateTime ;
	dct:created "2023-10-02T12:00:00+00:00"^^xsd:dateTime ;
	ikos:modified "2023-10-02T12:00:00+00:00"^^xsd:dateTime ;
	dct:modified "2023-10-02T12:00:00+00:00"^^xsd:dateTime  ;
	skos:exactMatch <https://www.wikidata.org/entity/Q219416> ;
	skos:broader	medtop:06000000 .

medtop:20001375
	rdf:type skos:Concept ;
	skos:prefLabel	"profit sharing"@en-GB ;
	skos:definition	"A system by which employees are paid a share of the net profits of their employer. These earnings are distinct from and additional to regular wages."@en-GB ;
	skos:inScheme <http://cv.iptc.org/newscodes/mediatopic/>  ;
	ikos:created "2023-10-02T12:00:00+00:00"^^xsd:dateTime ;
	dct:created "2023-10-02T12:00:00+00:00"^^xsd:dateTime ;
	ikos:modified "2023-10-02T12:00:00+00:00"^^xsd:dateTime ;
	dct:modified "2023-10-02T12:00:00+00:00"^^xsd:dateTime  ;
	skos:exactMatch <https://www.wikidata.org/entity/Q1419726> ;
	skos:broader	medtop:20000518 .
